@prefix daml: <http://www.daml.org/2001/03/daml+oil#> .
@prefix umbel: <http://umbel.org/umbel/sc/#> .
@prefix xml: <http://www.w3.org/XML/1998/namespace> .
@prefix rdf: <http://www.w3.org/1999/02/22-rdf-syntax-ns#> .
@prefix GO: <http://www.geneontology.org/dtd/go.dtd#> .
@prefix xsd: <http://www.w3.org/2001/XMLSchema#> .
@prefix owl: <http://www.w3.org/2002/07/owl#> .
@prefix ex: <http://www.nist.gov/itl/ssd/Experiments#> .
@prefix bc: <http://www.nist.gov/itl/ssd/Biochem#> .
@prefix dbpedia: <http://dbpedia.org/resource/#> .
@prefix : <http://www.nist.gov/itl/ssd/Materials#> .
@prefix or: <http://www.nist.gov/itl/ssd/OntologyRequirements#> .
@prefix doc: <http://www.nist.gov/itl/ssd/Document#> .
@prefix rdfs: <http://www.w3.org/2000/01/rdf-schema#> .
@base <http://www.nist.gov/itl/ssd/Materials.owl> .

<http://www.nist.gov/itl/ssd/Materials.owl> rdf:type owl:Ontology ;
                                            
                                            owl:imports <http://www.nist.gov/itl/ssd/Biochem.owl> ,
                                                        <http://www.nist.gov/itl/ssd/Document.n3> .


#################################################################
#
#    Annotation properties
#
#################################################################


or:UnitTypeFor rdf:type owl:AnnotationProperty .



or:unitTypeFor rdf:type owl:AnnotationProperty .





#################################################################
#
#    Datatypes
#
#################################################################




#################################################################
#
#    Object Properties
#
#################################################################


###  http://www.nist.gov/itl/ssd/Biochem#componentElement

bc:componentElement rdf:type owl:IrreflexiveProperty ;
                    
                    rdfs:range bc:ChemicalElement .



###  http://www.nist.gov/itl/ssd/Biochem#constituentType

bc:constituentType rdfs:domain or:MaterialType ;
                   
                   rdfs:range or:MaterialType .



###  http://www.nist.gov/itl/ssd/Biochem#hasMolecularStructure

bc:hasMolecularStructure rdfs:range :Microstructure .



###  http://www.nist.gov/itl/ssd/Materials.owl#classOfMaterial

:classOfMaterial rdf:type owl:ObjectProperty ;
                 
                 rdfs:comment "OBJECT classOfMaterial MATERIAL_TYPE means that OBJECT is made out of the general type of material MATERIAL_TYPE.  Use subclassOfMaterial, if referring to a more specific type."@en ;
                 
                 rdfs:domain :MaterialObject ;
                 
                 rdfs:range or:MaterialType .



###  http://www.nist.gov/itl/ssd/Materials.owl#coatingOf

:coatingOf rdf:type owl:AsymmetricProperty ,
                    owl:IrreflexiveProperty ,
                    owl:ObjectProperty ;
           
           rdfs:comment "The property 'coating Of' relates a coating material to the object which it coats."@en ;
           
           rdfs:domain :MaterialObject ;
           
           rdfs:range :MaterialObject ;
           
           owl:propertyDisjointWith :embeddedIn ,
                                    :substrate ,
                                    :weldedTo .



###  http://www.nist.gov/itl/ssd/Materials.owl#compositionSpecification

:compositionSpecification rdf:type owl:ObjectProperty ;
                          
                          rdfs:comment "The property composition Secification relates an object to a specification of the type of material (e.g., an alloy) of which it is composed."@en ;
                          
                          rdfs:range <http://www.nist.gov/itl/ssd/Document.n3#Specification> ;
                          
                          rdfs:domain :MaterialObject .



###  http://www.nist.gov/itl/ssd/Materials.owl#concentrationLevel

:concentrationLevel rdf:type owl:FunctionalProperty ,
                             owl:ObjectProperty ;
                    
                    rdfs:comment "The property 'concentration Level' specifies what the concentration of the specified Material Type is for a given Material Portion.."@en ;
                    
                    rdfs:range bc:Concentration ;
                    
                    rdfs:domain :MaterialPortion .



###  http://www.nist.gov/itl/ssd/Materials.owl#concentrationOfMaterialType

:concentrationOfMaterialType rdf:type owl:FunctionalProperty ,
                                      owl:ObjectProperty ;
                             
                             rdfs:comment "The property 'concentration Of Material Type' links a Substance Concentration to the type of material (Material Type) for which it is a concentration."@en ;
                             
                             rdfs:domain bc:Concentration ;
                             
                             rdfs:range or:MaterialType .



###  http://www.nist.gov/itl/ssd/Materials.owl#diffusivity

:diffusivity rdf:type owl:ObjectProperty ;
             
             rdfs:comment "Diffusivity is the ratio between the molar flux due to molecular diffusion and the gradient in the concentration of the species (or the driving force for diffusion).  Diffusivity is generally prescribed for a given pair of species in a given phase at a given temperature. For a multi-component system, it is prescribed for each pair of species in the system.  Diffusivity is measured in Area per unit time -- in SI, m^2/s."@en ;
             
             rdfs:range :AreaPerTime .



###  http://www.nist.gov/itl/ssd/Materials.owl#drivingForceForDiffusion

:drivingForceForDiffusion rdf:type owl:ObjectProperty ;
                          
                          rdfs:seeAlso "Definitions of terms for diffusion in the solid state (IUPAC Recommendations 1999), Pure Appl. Chem. 71, 1307-1325." ;
                          
                          rdfs:comment "The property ``driving Force'' relates an instance of Diffusion to any type influence which causes the jump frequency for a jump in one direction between two given sites to differ from that for a jump in the opposite direction between exactly analogous sites. Driving forces include gradients of stress, electrical potential, object temperature or chemical potential."@en ;
                          
                          <http://www.nist.gov/itl/ssd/OntologyRequirements.owl#termString> "diffusion driving force"@en ,
                                                                                            "driving force"@en ;
                          
                          rdfs:domain :Diffusion ;
                          
                          rdfs:range or:MeasurableProperty .



###  http://www.nist.gov/itl/ssd/Materials.owl#embeddedIn

:embeddedIn rdf:type owl:AsymmetricProperty ,
                     owl:IrreflexiveProperty ,
                     owl:ObjectProperty ;
            
            rdfs:domain :MaterialObject ;
            
            rdfs:range :MaterialObject ;
            
            owl:propertyDisjointWith :substrate ,
                                     :weldedTo .



###  http://www.nist.gov/itl/ssd/Materials.owl#enthalpyOfFusion

:enthalpyOfFusion rdf:type owl:FunctionalProperty ,
                           owl:ObjectProperty ;
                  
                  rdfs:comment "The enthalpy of fusion is the change in enthalpy required to melt one mole of a substance at its melting point."@en ;
                  
                  rdfs:domain bc:ChemicalSubstance ;
                  
                  rdfs:range or:Energy .



###  http://www.nist.gov/itl/ssd/Materials.owl#enthalpyOfSystem

:enthalpyOfSystem rdf:type owl:FunctionalProperty ,
                           owl:ObjectProperty ;
                  
                  rdfs:comment """Enthalpy is a measure of the total energy of a Thermodynamic System. It includes the internal energy, which is the energy required to create a system, and the amount of energy required to make room for it by displacing its environment and establishing its volume and pressure.

Enthalpy is not directly measured, Changes in enthalpy are.""" .



###  http://www.nist.gov/itl/ssd/Materials.owl#gibbsEnergy

:gibbsEnergy rdf:type owl:FunctionalProperty ,
                      owl:ObjectProperty ;
             
             rdfs:comment "The property `gibbs Energy'  specifies the Gibbs free energy of a Thermodynamic System, which specifies the “useful” work obtainable from a closed thermodynamic system at a constant temperature and pressure."@en ;
             
             rdfs:domain :ThermodynamicSystem ;
             
             rdfs:range or:Energy .



###  http://www.nist.gov/itl/ssd/Materials.owl#hasChemicalComposition

:hasChemicalComposition rdf:type owl:FunctionalProperty ,
                                 owl:ObjectProperty ;
                        
                        rdfs:comment "The property 'has Chemical Composition' relates some Material Substance to its Chemical Composition'."@en ;
                        
                        rdfs:range bc:ChemicalComposition ;
                        
                        rdfs:domain bc:MaterialSubstance .



###  http://www.nist.gov/itl/ssd/Materials.owl#hasHeatCapacity

:hasHeatCapacity rdf:type owl:ObjectProperty ;
                 
                 rdfs:domain :MaterialObject .



###  http://www.nist.gov/itl/ssd/Materials.owl#hasLatticeConstant

:hasLatticeConstant rdf:type owl:ObjectProperty ;
                    
                    rdfs:comment "The lattice Constant of a Crystal Lattice is the constant distance between unit cells.  A cubic lattice has a single lattice constant, while other forms of crystal have three.  The constant may be temperature dependant."@en ;
                    
                    rdfs:domain :CrystalLattice ;
                    
                    rdfs:range or:Distance .



###  http://www.nist.gov/itl/ssd/Materials.owl#hasMaterialForm

:hasMaterialForm rdf:type owl:ObjectProperty ;
                 
                 rdfs:comment "The predicate 'has Material Form' relates a Material Object to its Material Form."@en ;
                 
                 rdfs:range :MaterialForm ;
                 
                 rdfs:domain :MaterialObject .



###  http://www.nist.gov/itl/ssd/Materials.owl#hasMicrostructure

:hasMicrostructure rdf:type owl:ObjectProperty .



###  http://www.nist.gov/itl/ssd/Materials.owl#hasSpecificHeat

:hasSpecificHeat rdf:type owl:FunctionalProperty ,
                          owl:ObjectProperty ;
                 
                 rdfs:domain bc:ChemicalSubstance ;
                 
                 rdfs:range :SpecificHeatCapacity .



###  http://www.nist.gov/itl/ssd/Materials.owl#hasSubstanceConcentration

:hasSubstanceConcentration rdf:type owl:ObjectProperty ;
                           
                           rdfs:comment "The property 'has Substance Concentration' specifies for each Chemical Composition the specific concentration of one of its substances (called Substance Concentration).  Unless there is only a single substance type, a given Chemical Composition has multiple Substance Concentrations."@en ;
                           
                           rdfs:domain bc:ChemicalComposition ;
                           
                           rdfs:range bc:Concentration .



###  http://www.nist.gov/itl/ssd/Materials.owl#heatOfFusion

:heatOfFusion rdf:type owl:FunctionalProperty ,
                       owl:ObjectProperty ;
              
              rdfs:comment "The heat of fusion is the change in enthalpy per unit mass required to melt oa substance at its melting point."@en ;
              
              rdfs:domain bc:ChemicalSubstance ;
              
              rdfs:range :EnergyPerMass .



###  http://www.nist.gov/itl/ssd/Materials.owl#helmholtzEnergy

:helmholtzEnergy rdf:type owl:ObjectProperty ;
                 
                 rdfs:comment "The property `helmholtz Energy'  specifies the Helmholtz free energy of a Thermodynamic System, which specifies the “useful” work obtainable from a closed thermodynamic system at a constant temperature and volume.."@en .



###  http://www.nist.gov/itl/ssd/Materials.owl#isotopeOfElementType

:isotopeOfElementType rdf:type owl:FunctionalProperty ,
                               owl:ObjectProperty ;
                      
                      rdfs:comment "The property 'isotope Of Element Type' specifies the Element of which an Isotope is an isotope of."@en ;
                      
                      rdfs:range bc:ChemicalElement ;
                      
                      rdfs:domain bc:Isotope .



###  http://www.nist.gov/itl/ssd/Materials.owl#molarHeatCapacity

:molarHeatCapacity rdf:type owl:ObjectProperty ;
                   
                   rdfs:comment "The molar heat capacity is the heat capacity per mole of a pure substance."@en ;
                   
                   rdfs:domain bc:ChemicalSubstance ,
                               :PureSubstance .



###  http://www.nist.gov/itl/ssd/Materials.owl#peritecticTemperature

:peritecticTemperature rdf:type owl:ObjectProperty ;
                       
                       rdfs:comment "In a peritectic reaction a liquid and solid phase of fixed proportions react at a fixed temperature to yield a single solid phase.  The peritectic temperature is the temperature at which this happens."@en ;
                       
                       rdfs:domain :PhysicalMixture ;
                       
                       rdfs:range or:Temperature .



###  http://www.nist.gov/itl/ssd/Materials.owl#phaseOfMaterial

:phaseOfMaterial rdf:type owl:ObjectProperty ;
                 
                 rdfs:comment "The property 'phase Of Material' relates a Material Object to its Material Phase (e.g., crystalline, gel, liquid, ...)."@en ;
                 
                 rdfs:domain :MaterialObject ;
                 
                 rdfs:range :MaterialPhaseComposition .



###  http://www.nist.gov/itl/ssd/Materials.owl#physicalDecompositions

:physicalDecompositions rdf:type owl:ObjectProperty ;
                        
                        rdfs:comment "(physicalDecompositions WHOLE PART) means that PART is a spatial part or component of WHOLE, in a very broad sense of 'part' whereby PART might or might not be spatially continuous or discrete. Thus PART might be discontinuous, or diffused throughout WHOLE."@en ;
                        
                        rdfs:range :MaterialObject ;
                        
                        rdfs:domain :MaterialObject .



###  http://www.nist.gov/itl/ssd/Materials.owl#relativePermittivity

:relativePermittivity rdf:type owl:ObjectProperty ;
                      
                      rdfs:domain bc:MaterialSubstance ;
                      
                      rdfs:range :ElectricPolarizability .



###  http://www.nist.gov/itl/ssd/Materials.owl#solidus

:solidus rdf:type owl:ObjectProperty ;
         
         rdfs:domain or:MaterialType .



###  http://www.nist.gov/itl/ssd/Materials.owl#solute

:solute rdf:type owl:ObjectProperty ;
        
        rdfs:comment "The property 'solute' relates a Chemical Solution to a material that is a solute in the solution."@en ;
        
        rdfs:domain :ChemicalSolution ;
        
        rdfs:range :PureSubstance .



###  http://www.nist.gov/itl/ssd/Materials.owl#solvent

:solvent rdf:type owl:FunctionalProperty ,
                  owl:ObjectProperty ;
         
         rdfs:comment "The property 'solvent' relates a Chemical Solution to the material that is the solvent in the solution."@en ;
         
         rdfs:range bc:MaterialSubstance ;
         
         rdfs:domain :ChemicalSolution .



###  http://www.nist.gov/itl/ssd/Materials.owl#sourcesMaterialType

:sourcesMaterialType rdf:type owl:ObjectProperty ;
                     
                     rdfs:comment "The property 'sources Material Type' relates a Material Source Organization to a Material Type that it regularly can provide to others."@en ;
                     
                     rdfs:range or:MaterialType .



###  http://www.nist.gov/itl/ssd/Materials.owl#structuralIsomers

:structuralIsomers rdf:type owl:IrreflexiveProperty ,
                            owl:ObjectProperty ,
                            owl:SymmetricProperty ;
                   
                   rdfs:comment "Two chemical compounds are stereoisomers if they have the same simple chemical formula, but have different arrangements of the bonds between theiir atoms."@en ;
                   
                   rdfs:range bc:ChemicalObjectTypeByChemicalSpecies ;
                   
                   rdfs:domain bc:ChemicalObjectTypeByChemicalSpecies .



###  http://www.nist.gov/itl/ssd/Materials.owl#subclassOfMaterial

:subclassOfMaterial rdf:type owl:ObjectProperty ;
                    
                    rdfs:comment "OBJECT subclassOfMaterial MATERIAL_TYPE means that OBJECT is made of of the specific type of material MATERIAL_TYPE.  Use classOfMaterial, if referring to a more general type."@en ;
                    
                    rdfs:domain :MaterialObject ;
                    
                    rdfs:range or:MaterialType .



###  http://www.nist.gov/itl/ssd/Materials.owl#substrate

:substrate rdf:type owl:AsymmetricProperty ,
                    owl:IrreflexiveProperty ,
                    owl:ObjectProperty ;
           
           rdfs:range :MaterialObject ;
           
           rdfs:domain :MaterialObject ;
           
           owl:propertyDisjointWith :weldedTo .



###  http://www.nist.gov/itl/ssd/Materials.owl#weldedTo

:weldedTo rdf:type owl:IrreflexiveProperty ,
                   owl:ObjectProperty ,
                   owl:SymmetricProperty ;
          
          rdfs:range :MaterialObject ;
          
          rdfs:domain :MaterialObject .



###  http://www.nist.gov/itl/ssd/OntologyRequirements#objectActedOn

or:objectActedOn rdf:type owl:ObjectProperty .



###  http://www.nist.gov/itl/ssd/OntologyRequirements#outputCreated

or:outputCreated rdf:type owl:ObjectProperty .



###  http://www.nist.gov/itl/ssd/OntologyRequirements#subEvents

or:subEvents rdf:type owl:ObjectProperty .



###  http://www.nist.gov/itl/ssd/OntologyRequirements#unitTypeFor

or:unitTypeFor rdfs:subPropertyOf owl:topObjectProperty .





#################################################################
#
#    Data properties
#
#################################################################


###  http://www.nist.gov/itl/ssd/Materials.owl#strunzClassification

:strunzClassification rdf:type owl:DatatypeProperty ;
                      
                      rdfs:comment "The Strunz (or Nickel-Strunz) classification is a scheme for categorizing minerals based upon their chemical composition.  The predicate strunzClassification relates a mineratl to its Strunz classification code."@en ;
                      
                      rdfs:domain :MineralType ;
                      
                      rdfs:range rdf:PlainLiteral .



###  http://www.nist.gov/itl/ssd/Materials.owl#uncertaintyConfidenceLevel

:uncertaintyConfidenceLevel rdf:type owl:DatatypeProperty ;
                            
                            rdfs:domain or:MeasurableQuantity ;
                            
                            rdfs:range xsd:float .



###  http://www.nist.gov/itl/ssd/OntologyRequirements#nickName

or:nickName rdf:type owl:DatatypeProperty .





#################################################################
#
#    Classes
#
#################################################################


###  http://www.nist.gov/itl/ssd/Biochem#Actinium

bc:Actinium rdfs:subClassOf :ElementalMetal .



###  http://www.nist.gov/itl/ssd/Biochem#Aluminum

bc:Aluminum rdfs:subClassOf :ElementalMetal .



###  http://www.nist.gov/itl/ssd/Biochem#Americium

bc:Americium rdfs:subClassOf :ElementalMetal .



###  http://www.nist.gov/itl/ssd/Biochem#Atom

bc:Atom owl:disjointWith bc:Polymer .



###  http://www.nist.gov/itl/ssd/Biochem#Berkelium

bc:Berkelium rdfs:subClassOf :ElementalMetal .



###  http://www.nist.gov/itl/ssd/Biochem#Beryllium

bc:Beryllium rdfs:subClassOf :ElementalMetal .



###  http://www.nist.gov/itl/ssd/Biochem#BiologicalProcess

bc:BiologicalProcess owl:disjointWith :MicrostructureEvolution ,
                                      or:MechanicalProcess .



###  http://www.nist.gov/itl/ssd/Biochem#BiologicalProperty

bc:BiologicalProperty owl:disjointWith bc:ChemicalProperty .



###  http://www.nist.gov/itl/ssd/Biochem#Bismuth

bc:Bismuth rdfs:subClassOf :ElementalMetal .



###  http://www.nist.gov/itl/ssd/Biochem#Bohrium

bc:Bohrium rdfs:subClassOf :ElementalMetal .



###  http://www.nist.gov/itl/ssd/Biochem#Cadmium

bc:Cadmium rdfs:subClassOf :ElementalMetal .



###  http://www.nist.gov/itl/ssd/Biochem#Calcium

bc:Calcium rdfs:subClassOf :ElementalMetal .



###  http://www.nist.gov/itl/ssd/Biochem#Californium

bc:Californium rdfs:subClassOf :ElementalMetal .



###  http://www.nist.gov/itl/ssd/Biochem#Cerium

bc:Cerium rdfs:subClassOf :ElementalMetal .



###  http://www.nist.gov/itl/ssd/Biochem#Cesium

bc:Cesium rdfs:subClassOf :ElementalMetal .



###  http://www.nist.gov/itl/ssd/Biochem#ChemicalObject

bc:ChemicalObject owl:disjointWith :Vacuum .



###  http://www.nist.gov/itl/ssd/Biochem#ChemicalObjectType

bc:ChemicalObjectType rdf:type owl:Class ;
                      
                      owl:disjointWith :MineralType ;
                      
                      rdfs:comment """A Chemical Object Type is a class of chemicals defined by their chemical structure.  Instances include fully specified chemical compounds, such as H2O and generic types such as Ketone and DNA.

The more specific class, Chemical Object Type By Chemical Species, denotes the fully-specified compounds (other than stereoisomers)."""@en .



###  http://www.nist.gov/itl/ssd/Biochem#ChemicalObjectTypeByChemicalSpecies

bc:ChemicalObjectTypeByChemicalSpecies rdf:type owl:Class .



###  http://www.nist.gov/itl/ssd/Biochem#ChemicalProperty

bc:ChemicalProperty rdfs:subClassOf or:MeasurableProperty ;
                    
                    owl:disjointWith :MeasurableMechanicalProperty ;
                    
                    <http://www.w3.org/2004/02/skos/core#note> "Similar to \"Chemical\" in Ashino's 2010 Minerals Ontology."@en .



###  http://www.nist.gov/itl/ssd/Biochem#ChemicalSubstance

bc:ChemicalSubstance owl:disjointWith :CompositeMaterial ,
                                      :Vacuum .



###  http://www.nist.gov/itl/ssd/Biochem#Chromium

bc:Chromium rdfs:subClassOf :ElementalMetal .



###  http://www.nist.gov/itl/ssd/Biochem#Cobalt

bc:Cobalt rdfs:subClassOf :ElementalMetal .



###  http://www.nist.gov/itl/ssd/Biochem#Copernicium

bc:Copernicium rdf:type owl:Class ;
               
               rdfs:subClassOf :ElementalMetal .



###  http://www.nist.gov/itl/ssd/Biochem#Copper

bc:Copper rdfs:subClassOf :ElementalMetal .



###  http://www.nist.gov/itl/ssd/Biochem#Curium

bc:Curium rdfs:subClassOf :ElementalMetal .



###  http://www.nist.gov/itl/ssd/Biochem#Dubnium

bc:Dubnium rdfs:subClassOf :ElementalMetal .



###  http://www.nist.gov/itl/ssd/Biochem#Dysprosium

bc:Dysprosium rdfs:subClassOf :ElementalMetal .



###  http://www.nist.gov/itl/ssd/Biochem#Einsteinium

bc:Einsteinium rdfs:subClassOf :ElementalMetal .



###  http://www.nist.gov/itl/ssd/Biochem#ElementalSubstance

bc:ElementalSubstance owl:disjointWith :Boride ,
                                       :Carbide ,
                                       :Halide .



###  http://www.nist.gov/itl/ssd/Biochem#Erbium

bc:Erbium rdfs:subClassOf :ElementalMetal .



###  http://www.nist.gov/itl/ssd/Biochem#Europium

bc:Europium rdfs:subClassOf :ElementalMetal .



###  http://www.nist.gov/itl/ssd/Biochem#Fermium

bc:Fermium rdfs:subClassOf :ElementalMetal .



###  http://www.nist.gov/itl/ssd/Biochem#Francium

bc:Francium rdfs:subClassOf :ElementalMetal .



###  http://www.nist.gov/itl/ssd/Biochem#Gadolinium

bc:Gadolinium rdfs:subClassOf :ElementalMetal .



###  http://www.nist.gov/itl/ssd/Biochem#Gallium

bc:Gallium rdfs:subClassOf :ElementalMetal .



###  http://www.nist.gov/itl/ssd/Biochem#Gold

bc:Gold rdfs:subClassOf :ElementalMetal .



###  http://www.nist.gov/itl/ssd/Biochem#Hafnium

bc:Hafnium rdfs:subClassOf :ElementalMetal .



###  http://www.nist.gov/itl/ssd/Biochem#Hassium

bc:Hassium rdfs:subClassOf :ElementalMetal .



###  http://www.nist.gov/itl/ssd/Biochem#Holmium

bc:Holmium rdfs:subClassOf :ElementalMetal .



###  http://www.nist.gov/itl/ssd/Biochem#Indium

bc:Indium rdfs:subClassOf :ElementalMetal .



###  http://www.nist.gov/itl/ssd/Biochem#Iridium

bc:Iridium rdfs:subClassOf :ElementalMetal .



###  http://www.nist.gov/itl/ssd/Biochem#Iron

bc:Iron rdfs:subClassOf :ElementalMetal .



###  http://www.nist.gov/itl/ssd/Biochem#Lanthanum

bc:Lanthanum rdfs:subClassOf :ElementalMetal .



###  http://www.nist.gov/itl/ssd/Biochem#Lawrencium

bc:Lawrencium rdfs:subClassOf :ElementalMetal .



###  http://www.nist.gov/itl/ssd/Biochem#Lead

bc:Lead rdfs:subClassOf :ElementalMetal .



###  http://www.nist.gov/itl/ssd/Biochem#Lithium

bc:Lithium rdfs:subClassOf :ElementalMetal .



###  http://www.nist.gov/itl/ssd/Biochem#Lutetium

bc:Lutetium rdfs:subClassOf :ElementalMetal .



###  http://www.nist.gov/itl/ssd/Biochem#Magnesium

bc:Magnesium rdfs:subClassOf :ElementalMetal .



###  http://www.nist.gov/itl/ssd/Biochem#Manganese

bc:Manganese rdfs:subClassOf :ElementalMetal .



###  http://www.nist.gov/itl/ssd/Biochem#Mendelevium

bc:Mendelevium rdfs:subClassOf :ElementalMetal .



###  http://www.nist.gov/itl/ssd/Biochem#Mercury

bc:Mercury rdfs:subClassOf :ElementalMetal .



###  http://www.nist.gov/itl/ssd/Biochem#Metal

bc:Metal owl:disjointWith :LiquidSlag ,
                          :Semiconductor ,
                          :Vacuum ;
         
         or:referenceURL "http://www.matweb.com/index.aspx"^^xsd:anyURI ;
         
         <http://www.nist.gov/itl/ssd/OntologyRequirements.owl#termString> "metal"@en .



###  http://www.nist.gov/itl/ssd/Biochem#Molybdenum

bc:Molybdenum rdfs:subClassOf :ElementalMetal .



###  http://www.nist.gov/itl/ssd/Biochem#Neodymium

bc:Neodymium rdfs:subClassOf :ElementalMetal .



###  http://www.nist.gov/itl/ssd/Biochem#Neptunium

bc:Neptunium rdfs:subClassOf :ElementalMetal .



###  http://www.nist.gov/itl/ssd/Biochem#Nickel

bc:Nickel rdfs:subClassOf :ElementalMetal .



###  http://www.nist.gov/itl/ssd/Biochem#Niobium

bc:Niobium rdfs:subClassOf :ElementalMetal .



###  http://www.nist.gov/itl/ssd/Biochem#Nobelium

bc:Nobelium rdfs:subClassOf :ElementalMetal .



###  http://www.nist.gov/itl/ssd/Biochem#Osmium

bc:Osmium rdfs:subClassOf :ElementalMetal .



###  http://www.nist.gov/itl/ssd/Biochem#Oxide

bc:Oxide rdf:type owl:Class ;
         
         rdfs:subClassOf :PureSubstance ;
         
         owl:disjointWith :Boride ,
                          :Carbide ,
                          :Clathrate .



###  http://www.nist.gov/itl/ssd/Biochem#Palladium

bc:Palladium rdfs:subClassOf :ElementalMetal .



###  http://www.nist.gov/itl/ssd/Biochem#Platinum

bc:Platinum rdfs:subClassOf :ElementalMetal .



###  http://www.nist.gov/itl/ssd/Biochem#Plutonium

bc:Plutonium rdfs:subClassOf :ElementalMetal .



###  http://www.nist.gov/itl/ssd/Biochem#Polymer

bc:Polymer owl:disjointWith :Fullerine .



###  http://www.nist.gov/itl/ssd/Biochem#Potassium

bc:Potassium rdfs:subClassOf :ElementalMetal .



###  http://www.nist.gov/itl/ssd/Biochem#Praseodymium

bc:Praseodymium rdfs:subClassOf :ElementalMetal .



###  http://www.nist.gov/itl/ssd/Biochem#Promethium

bc:Promethium rdfs:subClassOf :ElementalMetal .



###  http://www.nist.gov/itl/ssd/Biochem#Protactinium

bc:Protactinium rdfs:subClassOf :ElementalMetal .



###  http://www.nist.gov/itl/ssd/Biochem#ProteinTypeByStructure

bc:ProteinTypeByStructure rdfs:subClassOf :PolymericMicrostructure .



###  http://www.nist.gov/itl/ssd/Biochem#Radium

bc:Radium rdfs:subClassOf :ElementalMetal .



###  http://www.nist.gov/itl/ssd/Biochem#Rhenium

bc:Rhenium rdfs:subClassOf :ElementalMetal .



###  http://www.nist.gov/itl/ssd/Biochem#Rhodium

bc:Rhodium rdfs:subClassOf :ElementalMetal .



###  http://www.nist.gov/itl/ssd/Biochem#Rubidium

bc:Rubidium rdfs:subClassOf :ElementalMetal .



###  http://www.nist.gov/itl/ssd/Biochem#Ruthenium

bc:Ruthenium rdfs:subClassOf :ElementalMetal .



###  http://www.nist.gov/itl/ssd/Biochem#Rutherfordium

bc:Rutherfordium rdfs:subClassOf :ElementalMetal .



###  http://www.nist.gov/itl/ssd/Biochem#Samarium

bc:Samarium rdfs:subClassOf :ElementalMetal .



###  http://www.nist.gov/itl/ssd/Biochem#Scandium

bc:Scandium rdfs:subClassOf :ElementalMetal .



###  http://www.nist.gov/itl/ssd/Biochem#Seaborgium

bc:Seaborgium rdfs:subClassOf :ElementalMetal .



###  http://www.nist.gov/itl/ssd/Biochem#Silver

bc:Silver rdfs:subClassOf :ElementalMetal .



###  http://www.nist.gov/itl/ssd/Biochem#Sodium

bc:Sodium rdfs:subClassOf :ElementalMetal .



###  http://www.nist.gov/itl/ssd/Biochem#Strontium

bc:Strontium rdfs:subClassOf :ElementalMetal .



###  http://www.nist.gov/itl/ssd/Biochem#Tantalum

bc:Tantalum rdfs:subClassOf :ElementalMetal .



###  http://www.nist.gov/itl/ssd/Biochem#Technetium

bc:Technetium rdfs:subClassOf :ElementalMetal .



###  http://www.nist.gov/itl/ssd/Biochem#Terbium

bc:Terbium rdfs:subClassOf :ElementalMetal .



###  http://www.nist.gov/itl/ssd/Biochem#Thallium

bc:Thallium rdfs:subClassOf :ElementalMetal .



###  http://www.nist.gov/itl/ssd/Biochem#Thorium

bc:Thorium rdfs:subClassOf :ElementalMetal .



###  http://www.nist.gov/itl/ssd/Biochem#Thulium

bc:Thulium rdfs:subClassOf :ElementalMetal .



###  http://www.nist.gov/itl/ssd/Biochem#Tin

bc:Tin rdfs:subClassOf :ElementalMetal .



###  http://www.nist.gov/itl/ssd/Biochem#Titanium

bc:Titanium rdfs:subClassOf :ElementalMetal .



###  http://www.nist.gov/itl/ssd/Biochem#Tungsten

bc:Tungsten rdfs:subClassOf :ElementalMetal .



###  http://www.nist.gov/itl/ssd/Biochem#UnitOfConcentration

bc:UnitOfConcentration owl:disjointWith :UnitOfCharge ,
                                        :UnitOfElectricCurrent ,
                                        :UnitOfElectricalConductivity ,
                                        :UnitOfInverseAreaPerTime ,
                                        :UnitOfSpecificHeatCapacity .



###  http://www.nist.gov/itl/ssd/Biochem#Uranium

bc:Uranium rdfs:subClassOf :ElementalMetal .



###  http://www.nist.gov/itl/ssd/Biochem#Vanadium

bc:Vanadium rdfs:subClassOf :ElementalMetal .



###  http://www.nist.gov/itl/ssd/Biochem#Water

bc:Water owl:disjointWith :AluminumOxide ,
                          :MagnesiumOxide ,
                          :SiliconOxide ,
                          :TitaniumOxide ,
                          :ZirconiumOxide .



###  http://www.nist.gov/itl/ssd/Biochem#Ytterbium

bc:Ytterbium rdfs:subClassOf :ElementalMetal .



###  http://www.nist.gov/itl/ssd/Biochem#Yttrium

bc:Yttrium rdfs:subClassOf :ElementalMetal .



###  http://www.nist.gov/itl/ssd/Biochem#Zinc

bc:Zinc rdfs:subClassOf :ElementalMetal .



###  http://www.nist.gov/itl/ssd/Biochem#Zirconium

bc:Zirconium rdfs:subClassOf :ElementalMetal .



###  http://www.nist.gov/itl/ssd/Document#MakingAPrediction

doc:MakingAPrediction owl:disjointWith or:Designing ,
                                       or:Manufacturing .



###  http://www.nist.gov/itl/ssd/Experiments#Experiment

ex:Experiment rdf:type owl:Class ;
              
              rdfs:subClassOf or:IntentionalCreation ,
                              [ rdf:type owl:Restriction ;
                                owl:onProperty or:subEvents ;
                                owl:someValuesFrom or:DataCollection
                              ] ;
              
              owl:disjointWith or:Designing ,
                               or:Development ,
                               or:Manufacturing .



###  http://www.nist.gov/itl/ssd/Materials.owl#ASTMSteel

:ASTMSteel rdf:type owl:Class ;
           
           rdfs:subClassOf :Steel ;
           
           or:referenceURL "http://www.matweb.com/index.aspx"^^xsd:anyURI ;
           
           rdfs:comment "ASTM Steel is steel that has been graded by ASTM and meets certain performance requirements.  Different ASTM steels may be alloy steel, carbon steel, stainless steel, forged, heat treated, etc."@en ;
           
           <http://www.nist.gov/itl/ssd/OntologyRequirements.owl#termString> "ASTM steel"@en .



###  http://www.nist.gov/itl/ssd/Materials.owl#AcousticProperty

:AcousticProperty rdf:type owl:Class ;
                  
                  rdfs:subClassOf or:MeasurableMaterialProperty ;
                  
                  owl:disjointWith :ElectricalProperty ,
                                   :MagneticProperty ,
                                   :MechanicalProperty ,
                                   :OpticalProperty ,
                                   :RadiologicalProperty ,
                                   :ThermalProperty ,
                                   :ThermochemicalProperty .



###  http://www.nist.gov/itl/ssd/Materials.owl#Aerogel

:Aerogel rdf:type owl:Class ;
         
         rdfs:subClassOf :Ceramic ,
                         :EngineeredMaterial ;
         
         or:referenceURL "http://www.matweb.com/index.aspx"^^xsd:anyURI ;
         
         rdfs:comment "Aerogel is a synthetic porous ultralight solid with extremely low density and thermal conductivity derived from a gel through supercritical drying, in which the liquid component of the gel has been replaced with a gas."@en ;
         
         <http://www.nist.gov/itl/ssd/OntologyRequirements.owl#termString> "aerogel"@en .



###  http://www.nist.gov/itl/ssd/Materials.owl#Aerosol

:Aerosol rdf:type owl:Class ;
         
         rdfs:subClassOf :Colloid ,
                         :ComplexFluid ,
                         :GaseousSubstance ;
         
         owl:disjointWith :Alloy ,
                          :ColloidalSol ,
                          :Emulsion ,
                          :Foam ,
                          :GasMixture ,
                          :GelSubstance ;
         
         rdfs:comment "An aerosol is a colloid suspension of fine solid particles or liquid droplets in a pure gas or Gas Mixture."@en .



###  http://www.nist.gov/itl/ssd/Materials.owl#AlkylCelluloseEthers

:AlkylCelluloseEthers rdf:type owl:Class ;
                      
                      rdfs:subClassOf :CelluloseEther ;
                      
                      owl:disjointWith :CarboxymethylCellulose ,
                                       :HydroxyalkylCelluloseEther .



###  http://www.nist.gov/itl/ssd/Materials.owl#AlkylatedNaphthalene

:AlkylatedNaphthalene rdf:type owl:Class ;
                      
                      rdfs:subClassOf :FluidLubricant ;
                      
                      owl:disjointWith :AluminumGellant ,
                                       :LithiumGellant ,
                                       :MultiplyAlkylatedCyclopentane ,
                                       :OrganicSoapGellant ,
                                       :PTFEGellant ,
                                       :Perfluoropolyether ,
                                       :Polyalphaolefin ,
                                       :Polyglycol ,
                                       :PolyphenyletherBaseLubricant ,
                                       :Quenchant ,
                                       :SiliconeBaseLubricant ,
                                       :SiliconeGellant ,
                                       :SyntheticEtherBase ,
                                       :UreaGellant ,
                                       :WhiteMineralOil ,
                                       :ZincOxideLubricant ;
                      
                      or:referenceURL "http://www.matweb.com/index.aspx"^^xsd:anyURI ;
                      
                      <http://www.nist.gov/itl/ssd/OntologyRequirements.owl#termString> "AN"@en ,
                                                                                        "alkylated naphthalene"@en .



###  http://www.nist.gov/itl/ssd/Materials.owl#Alloy

:Alloy rdf:type owl:Class ;
       
       rdfs:subClassOf bc:Metal ,
                       :PhysicalMixture ,
                       :SolidSubstance ;
       
       owl:disjointWith :ChemicalSuspension ,
                        :CompositeMaterial ,
                        :Foam ,
                        :GelSubstance ,
                        :LiquidFoam ,
                        :PasteSubstance .



###  http://www.nist.gov/itl/ssd/Materials.owl#AlloyCastIron

:AlloyCastIron rdf:type owl:Class ;
               
               rdfs:subClassOf :CastIron ;
               
               owl:disjointWith :DuctileIron ,
                                :GrayCastIron ,
                                :MalleableIron ,
                                :WhiteCastIron ;
               
               or:referenceURL "http://www.matweb.com/index.aspx"^^xsd:anyURI ;
               
               <http://www.nist.gov/itl/ssd/OntologyRequirements.owl#termString> "alloy cast iron"@en .



###  http://www.nist.gov/itl/ssd/Materials.owl#AlloySteel

:AlloySteel rdf:type owl:Class ;
            
            rdfs:subClassOf :Steel ;
            
            owl:disjointWith :CarbonSteel ,
                             :ChromMolySteel ;
            
            or:referenceURL "http://www.matweb.com/index.aspx"^^xsd:anyURI ;
            
            rdfs:comment "Steel with no carbide forming elements."@en ;
            
            <http://www.nist.gov/itl/ssd/OntologyRequirements.owl#termString> "alloy steel"@en .



###  http://www.nist.gov/itl/ssd/Materials.owl#AlloyType

:AlloyType rdf:type owl:Class ;
           
           rdfs:subClassOf or:MaterialType .



###  http://www.nist.gov/itl/ssd/Materials.owl#AlloyTypeByFormingProcess

:AlloyTypeByFormingProcess rdf:type owl:Class ;
                           
                           rdfs:subClassOf :AlloyType .



###  http://www.nist.gov/itl/ssd/Materials.owl#AlloyTypeByMainConstituent

:AlloyTypeByMainConstituent rdf:type owl:Class ;
                            
                            rdfs:subClassOf :AlloyType .



###  http://www.nist.gov/itl/ssd/Materials.owl#AluminumAlloy

:AluminumAlloy rdf:type owl:Class ;
               
               rdfs:subClassOf :NonFerrousAlloy ,
                               [ rdf:type owl:Restriction ;
                                 owl:onProperty :physicalDecompositions ;
                                 owl:someValuesFrom bc:Aluminum
                               ] ;
               
               or:referenceURL "http://www.matweb.com/index.aspx"^^xsd:anyURI ;
               
               rdfs:comment "An alloy that contains Aluminum but not Iron."@en .



###  http://www.nist.gov/itl/ssd/Materials.owl#AluminumGellant

:AluminumGellant rdf:type owl:Class ;
                 
                 rdfs:subClassOf :FluidLubricant ;
                 
                 owl:disjointWith :LithiumGellant ,
                                  :MultiplyAlkylatedCyclopentane ,
                                  :OrganicSoapGellant ,
                                  :PTFEGellant ,
                                  :Perfluoropolyether ,
                                  :Polyalphaolefin ,
                                  :Polyglycol ,
                                  :PolyphenyletherBaseLubricant ,
                                  :Quenchant ,
                                  :SiliconeBaseLubricant ,
                                  :SiliconeGellant ,
                                  :SyntheticEtherBase ,
                                  :UreaGellant ,
                                  :WhiteMineralOil ,
                                  :ZincOxideLubricant ;
                 
                 or:referenceURL "http://www.matweb.com/index.aspx"^^xsd:anyURI ;
                 
                 <http://www.nist.gov/itl/ssd/OntologyRequirements.owl#termString> "aluminum gellant"@en .



###  http://www.nist.gov/itl/ssd/Materials.owl#AluminumOxide

:AluminumOxide rdf:type owl:Class ;
               
               rdfs:subClassOf bc:Oxide ;
               
               owl:disjointWith :MagnesiumOxide ,
                                :SiliconOxide ,
                                :TitaniumOxide ,
                                :ZirconiumOxide ;
               
               or:referenceURL "http://www.matweb.com/index.aspx"^^xsd:anyURI ;
               
               <http://www.nist.gov/itl/ssd/OntologyRequirements.owl#termString> "aluminum oxide"@en .



###  http://www.nist.gov/itl/ssd/Materials.owl#AmbipolarDIffusion

:AmbipolarDIffusion rdf:type owl:Class ;
                    
                    rdfs:subClassOf :SolidDiffusion ;
                    
                    rdfs:comment "Ambipolar diffusion is diffusion in systems with two or more diffusion species with opposite electrical charge."@en ;
                    
                    rdfs:seeAlso "Definitions of terms for diffusion in the solid state (IUPAC Recommendations 1999), Pure Appl. Chem. 71, 1307-1325."@en .



###  http://www.nist.gov/itl/ssd/Materials.owl#AmorphousMetal

:AmorphousMetal rdf:type owl:Class ;
                
                rdfs:subClassOf :EngineeredAlloy ,
                                :ManufacturedGlass ;
                
                owl:disjointWith :OpticalGlass ;
                
                rdfs:comment "An amorphous metal (also known metallic glass or glassy metal) is an alloy with a disordered atomic-scale structure."@en .



###  http://www.nist.gov/itl/ssd/Materials.owl#AmorphousMicrostructure

:AmorphousMicrostructure rdf:type owl:Class ;
                         
                         rdfs:subClassOf :Microstructure ;
                         
                         owl:disjointWith :CeramicMicrostructure ,
                                          :CompositeMicrostructure ,
                                          :CrystalStructure .



###  http://www.nist.gov/itl/ssd/Materials.owl#AmorphousSubstance

:AmorphousSubstance rdf:type owl:Class ;
                    
                    rdfs:subClassOf :SolidSubstance ;
                    
                    owl:disjointWith :CompositeMaterial ,
                                     :CrystallineSubstance ,
                                     :GaseousSubstance ;
                    
                    rdfs:comment "Material in a solid amorphous (non-crystalline) phase."@en .



###  http://www.nist.gov/itl/ssd/Materials.owl#AqueousSolution

:AqueousSolution rdf:type owl:Class ;
                 
                 owl:equivalentClass [ rdf:type owl:Class ;
                                       owl:intersectionOf ( :LiquidSolution
                                                            [ rdf:type owl:Restriction ;
                                                              owl:onProperty :solvent ;
                                                              owl:allValuesFrom bc:Water
                                                            ]
                                                          )
                                     ] ;
                 
                 rdfs:subClassOf :LiquidSolution ;
                 
                 owl:disjointWith :IonicLiquidSolution ,
                                  :NonIonicOrAqueousLiquidSolution ;
                 
                 rdfs:comment "A solution in which liquid water is the solvent."@en .



###  http://www.nist.gov/itl/ssd/Materials.owl#AreaPerTime

:AreaPerTime rdf:type owl:Class ;
             
             owl:equivalentClass [ rdf:type owl:Class ;
                                   owl:intersectionOf ( or:MeasurableQuantity
                                                        [ rdf:type owl:Restriction ;
                                                          owl:onProperty or:unitsFor ;
                                                          owl:someValuesFrom :UnitOfAreaPerTime
                                                        ]
                                                      )
                                 ] ;
             
             rdfs:subClassOf or:MeasurableQuantity ,
                             [ rdf:type owl:Restriction ;
                               owl:onProperty or:unitsFor ;
                               owl:allValuesFrom :UnitOfAreaPerTime
                             ] ;
             
             owl:disjointWith :EnergyPerMass ,
                              or:Area ,
                              or:ComputerStorageCapacity ,
                              or:Distance ,
                              or:Duration ,
                              or:Energy ,
                              or:Force ,
                              or:Mass ,
                              or:Pressure ,
                              or:Temperature ,
                              or:Volume .



###  http://www.nist.gov/itl/ssd/Materials.owl#ArsenateMineral

:ArsenateMineral rdf:type owl:Class ;
                 
                 rdfs:subClassOf :Mineral ;
                 
                 rdfs:comment "The class of minerals with the arsenate (AsO4) ion."@en .



###  http://www.nist.gov/itl/ssd/Materials.owl#AscendingDiffusion

:AscendingDiffusion rdf:type owl:Class ;
                    
                    rdfs:subClassOf :SolidDiffusion ;
                    
                    owl:disjointWith :SelfDiffusion ;
                    
                    rdfs:comment "Ascending Diffusion is a type of diffusion that can take place in alloys of metals under the influence of stress gradients.  When the constituents are of different sizes, the larger elements tend to move in the directions of the dilated regions.  Thus ascending diffusion disturbs the uniform distribution of the constiuentes and sets up a concentration gradient which opposes the stress gradient."@en ;
                    
                    rdfs:seeAlso "Definitions of terms for diffusion in the solid state (IUPAC Recommendations 1999), Pure Appl. Chem. 71, 1307-1325."@en .



###  http://www.nist.gov/itl/ssd/Materials.owl#Auricupride

:Auricupride rdf:type owl:Class ;
             
             rdfs:subClassOf :BinaryAlloy ,
                             :CopperAlloy ,
                             :NativeMetal ,
                             [ rdf:type owl:Restriction ;
                               owl:onProperty :physicalDecompositions ;
                               owl:someValuesFrom bc:Gold
                             ] ;
             
             owl:disjointWith :EngineeredAlloy ;
             
             rdfs:comment "Auricupride is a natural alloy that combines copper and gold. Its chemical formula is Cu3Au. The alloy crystallizes in the Cubic crystal system and occurs as malleable grains or platey masses. It is an opaque yellow with a reddish tint. It has a hardness of 3.5 and a specific gravity of 11.5."@en .



###  http://www.nist.gov/itl/ssd/Materials.owl#AusteniticSteel

:AusteniticSteel rdf:type owl:Class ;
                 
                 rdfs:subClassOf :Steel ;
                 
                 owl:disjointWith :FerriticStainlessSteel ;
                 
                 or:referenceURL "http://www.matweb.com/index.aspx"^^xsd:anyURI ;
                 
                 rdfs:comment "Austenitic Steel is steel that has enough nickel and chromium or manganese to retain austenite at atmospheric temperatures"@en ;
                 
                 <http://www.nist.gov/itl/ssd/OntologyRequirements.owl#termString> "austenitic steel "@en .



###  http://www.nist.gov/itl/ssd/Materials.owl#Bakelite

:Bakelite rdf:type owl:Class ;
          
          rdfs:subClassOf :EngineeredMaterial ,
                          :Thermoset ;
          
          owl:disjointWith :Polyester ;
          
          rdfs:comment "Bakelite (polyoxybenzylmethylenglycolanhydride) is a thermosetting resin-like substance produced by the condensation reaction of carbolic acid and formaldehyde."@en .



###  http://www.nist.gov/itl/ssd/Materials.owl#BinaryAlloy

:BinaryAlloy rdf:type owl:Class ;
             
             rdfs:subClassOf :Alloy ;
             
             owl:disjointWith :Superalloy ;
             
             rdfs:comment "A Binary Alloy is an Alloy composed of exactly two different metals."@en .



###  http://www.nist.gov/itl/ssd/Materials.owl#BinarySolutionPhase

:BinarySolutionPhase rdf:type owl:Class ;
                     
                     rdfs:subClassOf :MaterialPhaseComposition .



###  http://www.nist.gov/itl/ssd/Materials.owl#BodyCenteredCubicCrystalStructure

:BodyCenteredCubicCrystalStructure rdf:type owl:Class ;
                                   
                                   rdfs:subClassOf :CubicCrystalStructure ;
                                   
                                   owl:disjointWith :FaceCenteredCubicCrystalStructure .



###  http://www.nist.gov/itl/ssd/Materials.owl#Boiling

:Boiling rdf:type owl:Class ;
         
         rdfs:subClassOf :Evaporating ;
         
         rdfs:comment "Boiling is the Phase Change event at a liquid's 'boiling point' at which the partial pressure of the gas reaches the environmental pressure.  During boiling, increasing amounts of the liquid evaporate as heat is added to the system although the temperature of the system remains basically constant."@en .



###  http://www.nist.gov/itl/ssd/Materials.owl#Borate

:Borate rdf:type owl:Class ;
        
        rdfs:subClassOf :Mineral .



###  http://www.nist.gov/itl/ssd/Materials.owl#Boride

:Boride rdf:type owl:Class ;
        
        rdfs:subClassOf :PureSubstance ;
        
        owl:disjointWith :Carbide ,
                         :Halide ;
        
        rdfs:comment "A  boride is a chemical compound between boron and a less electronegative element."@en ;
        
        <http://www.nist.gov/itl/ssd/OntologyRequirements.owl#termString> "boride"@en .



###  http://www.nist.gov/itl/ssd/Materials.owl#BorideBasedCeramic

:BorideBasedCeramic rdf:type owl:Class ;
                    
                    rdfs:subClassOf :Ceramic ;
                    
                    owl:disjointWith :ChalcogenBasedCeramic ,
                                     :OxideBasedCeramic ,
                                     :PnictideCeramic ;
                    
                    or:referenceURL "http://www.matweb.com/index.aspx"^^xsd:anyURI .



###  http://www.nist.gov/itl/ssd/Materials.owl#Brass

:Brass rdf:type owl:Class ;
       
       rdfs:subClassOf :CopperAlloy ,
                       :EngineeredAlloy ,
                       [ rdf:type owl:Restriction ;
                         owl:onProperty :physicalDecompositions ;
                         owl:someValuesFrom bc:Zinc
                       ] ;
       
       rdfs:comment "Brass is an alloy of copper and zinc; the proportions of zinc and copper can be varied to create a range of brasses with varying properties.  Other metals (lead, tin, aluminum, nickel, traces of iron) may be added in specific proportions for specific brass alloys."@en .



###  http://www.nist.gov/itl/ssd/Materials.owl#Bronze

:Bronze rdf:type owl:Class ;
        
        rdfs:subClassOf :CopperAlloy ,
                        :EngineeredAlloy ;
        
        rdfs:comment "Bronze is a metal alloy consisting primarily of copper, usually with tin as the main additive. There are many different bronze alloys but modern bronze is typically 88% copper and 12% tin.  Bronzes with the secondary additive other than tin or zinc include Aluminum Bronze and Silicon Bronze.  Phosphor Bronze is a Brass (main additive is zinc) with a significant amount of Phosphor (up to 1%) as an additional additive."@en .



###  http://www.nist.gov/itl/ssd/Materials.owl#Buckling

:Buckling rdf:type owl:Class ;
          
          rdfs:subClassOf :Deformation ;
          
          owl:disjointWith :Compaction ;
          
          rdfs:comment "Buckling is a Deformation Process of an object bending under compressive stress."@en .



###  http://www.nist.gov/itl/ssd/Materials.owl#Buckyball

:Buckyball rdf:type owl:Class ;
           
           rdfs:subClassOf :Fullerine ;
           
           owl:disjointWith :CarbonNanotube ;
           
           rdfs:comment "A Buckyball is a Fullerene in the shape of a ball with at least 60 carbon atoms.  Buckyballs have been discovered in soot with 60, 70, 76, 80, and 84 carbon atoms."@en .



###  http://www.nist.gov/itl/ssd/Materials.owl#Carbide

:Carbide rdf:type owl:Class ;
         
         rdfs:subClassOf :PureSubstance ;
         
         owl:disjointWith :Halide ;
         
         rdfs:comment "A carbide is a chemical compound composed of carbon and a less electronegative element."@en ;
         
         <http://www.nist.gov/itl/ssd/OntologyRequirements.owl#termString> "carbide"@en .



###  http://www.nist.gov/itl/ssd/Materials.owl#CarbideBasedCeramic

:CarbideBasedCeramic rdf:type owl:Class ;
                     
                     rdfs:subClassOf :Ceramic ;
                     
                     or:referenceURL "http://www.matweb.com/index.aspx"^^xsd:anyURI .



###  http://www.nist.gov/itl/ssd/Materials.owl#CarbideBasedCermet

:CarbideBasedCermet rdf:type owl:Class ;
                    
                    rdfs:subClassOf :CarbideBasedCeramic ,
                                    :Cermet .



###  http://www.nist.gov/itl/ssd/Materials.owl#CarbonBlack

:CarbonBlack rdf:type owl:Class ;
             
             rdfs:subClassOf bc:Carbon ,
                             :PolycrystallineMaterial ;
             
             owl:disjointWith :CarbonFiber ,
                              :Diamond ,
                              :Fullerine ,
                              :Graphite ;
             
             or:referenceURL "http://www.matweb.com/index.aspx"^^xsd:anyURI ;
             
             rdfs:comment "Carbon black (also known as acetylene black, channel black, furnace black, lamp black or thermal black) is a material produced by the incomplete combustion of heavy petroleum products such as FCC tar, coal tar, ethylene cracking tar, and a small amount from vegetable oil. Carbon black is a form of amorphous carbon that has a high surface-area-to-volume ratio, although its surface-area-to-volume ratio is low compared to that of activated carbon. It is dissimilar to soot in its much higher surface-area-to-volume ratio and significantly lower (negligible and non-bioavailable) PAH (polycyclic aromatic hydrocarbon) content."@en ;
             
             <http://www.nist.gov/itl/ssd/OntologyRequirements.owl#termString> "acetylene black"@en ,
                                                                               "carbon fiber"@en ,
                                                                               "channel black"@en ,
                                                                               "furnace black"@en ,
                                                                               "lamp black"@en ,
                                                                               "thermal black"@en .



###  http://www.nist.gov/itl/ssd/Materials.owl#CarbonFiber

:CarbonFiber rdf:type owl:Class ;
             
             rdfs:subClassOf bc:Carbon ,
                             :PolycrystallineMaterial ;
             
             owl:disjointWith :Diamond ,
                              :Graphite ;
             
             or:referenceURL "http://www.matweb.com/index.aspx"^^xsd:anyURI ;
             
             <http://www.nist.gov/itl/ssd/OntologyRequirements.owl#termString> "CF"@en ;
             
             rdfs:comment "Carbon fiber, alternatively graphite fiber, carbon graphite or CF, is a material consisting of fibers about 5–10 μm in diameter and composed mostly of carbon atoms. The carbon atoms are bonded together in crystals that are more or less aligned parallel to the long axis of the fiber."@en ;
             
             <http://www.nist.gov/itl/ssd/OntologyRequirements.owl#termString> "carbon fiber"@en ,
                                                                               "carbon graphite"@en ,
                                                                               "graphite fiber"@en .



###  http://www.nist.gov/itl/ssd/Materials.owl#CarbonNanotube

:CarbonNanotube rdf:type owl:Class ;
                
                rdfs:subClassOf :Fullerine ;
                
                rdfs:comment "Carbon Nanotubes are tubular Fullerenes"@en .



###  http://www.nist.gov/itl/ssd/Materials.owl#CarbonSteel

:CarbonSteel rdf:type owl:Class ;
             
             rdfs:subClassOf :Steel ;
             
             owl:disjointWith :ChromMolySteel ,
                              :HighSpeedSteel ,
                              :StainlessSteel ;
             
             or:referenceURL "http://www.matweb.com/index.aspx"^^xsd:anyURI ;
             
             rdfs:comment """Carbon steel is steel where the main interstitial alloying constituent is carbon. 

 The American Iron and Steel Institute (AISI) defines carbon steel as the following: ``Steel is considered to be carbon steel when no minimum content is specified or required for chromium, cobalt, molybdenum, nickel, niobium, titanium, tungsten, vanadium or zirconium, or any other element to be added to obtain a desired alloying effect; when the specified minimum for copper does not exceed 1.04 percent; or when the maximum content specified for any of the following elements does not exceed the percentages noted: manganese 1.65, silicon 0.60, copper 0.60.''"""@en ;
             
             <http://www.nist.gov/itl/ssd/OntologyRequirements.owl#termString> "carbon steel"@en .



###  http://www.nist.gov/itl/ssd/Materials.owl#Carbonate

:Carbonate rdf:type owl:Class ;
           
           rdfs:subClassOf :Mineral .



###  http://www.nist.gov/itl/ssd/Materials.owl#CarboxymethylCellulose

:CarboxymethylCellulose rdf:type owl:Class ;
                        
                        rdfs:subClassOf :CelluloseEther ;
                        
                        owl:disjointWith :HydroxyalkylCelluloseEther ;
                        
                        rdfs:comment "Carboxymethyl cellulose (CMC) (or cellulose gum) is a cellulose derivative with carboxymethyl groups (-CH2-COOH) bound to some of the hydroxyl groups of the glucopyranose monomers that make up the cellulose backbone."@en .



###  http://www.nist.gov/itl/ssd/Materials.owl#CastAlloy

:CastAlloy rdf:type owl:Class ;
           
           rdfs:subClassOf :EngineeredAlloy ;
           
           owl:disjointWith :CompactedPowderAlloy ,
                            :WroughtAlloy ;
           
           rdfs:comment "A Cast Alloy is one which is formed by pouring molten metal into a mold and letting it harden."@en .



###  http://www.nist.gov/itl/ssd/Materials.owl#CastIron

:CastIron rdf:type owl:Class ;
          
          rdfs:subClassOf :CastAlloy ,
                          :FerrousAlloy ;
          
          or:referenceURL "http://www.matweb.com/index.aspx"^^xsd:anyURI ;
          
          <http://www.nist.gov/itl/ssd/OntologyRequirements.owl#termString> "cast iron"@en .



###  http://www.nist.gov/itl/ssd/Materials.owl#CellularPrecipitationFromSolution

:CellularPrecipitationFromSolution rdf:type owl:Class ;
                                   
                                   rdfs:subClassOf :PrecipitationFromSolution .



###  http://www.nist.gov/itl/ssd/Materials.owl#Cellulose

:Cellulose rdf:type owl:Class ;
           
           rdfs:subClassOf :PolymerSubstance ;
           
           owl:disjointWith :Elastomer ,
                            :EngineeredMaterial ,
                            :Polyester ;
           
           rdfs:comment "Cellulose is an organic compound with the formula (C6H10O5)n, a polysaccharide consisting of a linear chain of several hundred to over ten thousand β(1→4) linked D-glucose units."@en .



###  http://www.nist.gov/itl/ssd/Materials.owl#CelluloseAcetate

:CelluloseAcetate rdf:type owl:Class ;
                  
                  rdfs:subClassOf :CelluloseEster ;
                  
                  owl:disjointWith :CelluloseDiacetate ,
                                   :CelluloseSulfate ,
                                   :CelluloseTriacetate ,
                                   :Nitrocellulose ;
                  
                  rdfs:comment "Cellulose acetate is the acetate ester of cellulose."@en .



###  http://www.nist.gov/itl/ssd/Materials.owl#CelluloseDiacetate

:CelluloseDiacetate rdf:type owl:Class ;
                    
                    rdfs:subClassOf :CelluloseEster ;
                    
                    owl:disjointWith :CelluloseSulfate ,
                                     :CelluloseTriacetate ,
                                     :Nitrocellulose ;
                    
                    rdfs:comment "Cellulose diacetate (or simply `diacetate') is a synthetic polymer made by treating cellulose with acetic acid. It consists of two acetate radicals on each monomer of the cellulose molecule."@en .



###  http://www.nist.gov/itl/ssd/Materials.owl#CelluloseEster

:CelluloseEster rdf:type owl:Class ;
                
                rdfs:subClassOf :CellulosticPlastic ;
                
                owl:disjointWith :CelluloseEther ;
                
                rdfs:comment "A Cellulose Ester is a Cellulostic Plastic with the hydroxyl groups of Cellulose replaced by a radical not connected via an oxygen (i.e., an ether)."@en .



###  http://www.nist.gov/itl/ssd/Materials.owl#CelluloseEther

:CelluloseEther rdf:type owl:Class ;
                
                rdfs:subClassOf :CellulosticPlastic ;
                
                rdfs:comment "A Cellulose Ester is a Cellulostic Plastic with the hydroxyl groups of Cellulose replaced by a radical connected via an oxygen (i.e., an ether)."@en .



###  http://www.nist.gov/itl/ssd/Materials.owl#CelluloseSulfate

:CelluloseSulfate rdf:type owl:Class ;
                  
                  rdfs:subClassOf :CelluloseEster ;
                  
                  owl:disjointWith :CelluloseTriacetate ,
                                   :Nitrocellulose .



###  http://www.nist.gov/itl/ssd/Materials.owl#CelluloseTriacetate

:CelluloseTriacetate rdf:type owl:Class ;
                     
                     rdfs:subClassOf :CelluloseEster ;
                     
                     owl:disjointWith :Nitrocellulose ;
                     
                     rdfs:comment "Cellulose triacetate (or triacetate, CTA, or TAC) is manufactured from cellulose and a source of acetate esters, typically acetic anhydride.  It is similar chemically to cellulose acetate, with the distinguishing characteristics being that in triacetate (Federal Trade Commission definition) at least ``92 percent of the hydroxyl groups are acetylated.'' "@en .



###  http://www.nist.gov/itl/ssd/Materials.owl#CellulosticPlastic

:CellulosticPlastic rdf:type owl:Class ;
                    
                    rdfs:subClassOf :Thermoplastic ;
                    
                    owl:disjointWith :Polyester ,
                                     :Polyolefin ,
                                     :VinylPolymer ;
                    
                    or:referenceURL "http://www.matweb.com/index.aspx"^^xsd:anyURI ;
                    
                    rdfs:comment "A celluloistic plastic is a plastic derived from cellulose."@en .



###  http://www.nist.gov/itl/ssd/Materials.owl#Ceramic

:Ceramic rdf:type owl:Class ;
         
         rdfs:subClassOf :SolidSubstance ;
         
         owl:disjointWith :PolymerSubstance ,
                          :SolidFoam ,
                          :SolidSol .



###  http://www.nist.gov/itl/ssd/Materials.owl#CeramicHydride

:CeramicHydride rdf:type owl:Class ;
                
                rdfs:subClassOf :Ceramic ;
                
                or:referenceURL "http://www.matweb.com/index.aspx"^^xsd:anyURI ;
                
                <http://www.nist.gov/itl/ssd/OntologyRequirements.owl#termString> "ceramic hydride"@en ,
                                                                                  "hydride"@en .



###  http://www.nist.gov/itl/ssd/Materials.owl#CeramicMatrixComposite

:CeramicMatrixComposite rdf:type owl:Class ;
                        
                        rdfs:subClassOf :Ceramic ,
                                        :CompositeMaterial ,
                                        :EngineeredMaterial ;
                        
                        owl:disjointWith :CeramicResin ,
                                         :Cermet ,
                                         :GlassCeramic ;
                        
                        or:referenceURL "http://www.matweb.com/index.aspx"^^xsd:anyURI ;
                        
                        <http://www.nist.gov/itl/ssd/OntologyRequirements.owl#termString> "CMC"@en ;
                        
                        rdfs:comment "Ceramic matrix composites (CMCs) are a subgroup of composite materials as well as a subgroup of technical ceramics. They consist of ceramic fibers embedded in a ceramic matrix, thus forming a ceramic fiber reinforced ceramic (CFRC) material. The matrix and fibers can consist of any ceramic material, whereby carbon and carbon fibers can also be considered a ceramic material."@en ;
                        
                        <http://www.nist.gov/itl/ssd/OntologyRequirements.owl#termString> "ceramic matrix composite"@en .



###  http://www.nist.gov/itl/ssd/Materials.owl#CeramicMicrostructure

:CeramicMicrostructure rdf:type owl:Class ;
                       
                       rdfs:subClassOf :Microstructure ;
                       
                       owl:disjointWith :CompositeMicrostructure ,
                                        :CrystalStructure ,
                                        :MetallicMicrostructure ,
                                        :PolymericMicrostructure ;
                       
                       rdfs:comment "Ceramic Microstructure is the material Microstructure of ceramic substancs with components ranging around 0.1 to 100 microns. The microstructure includes grains, secondary phases, grain boundaries, pores, micro-cracks and hardness microindentions."@en .



###  http://www.nist.gov/itl/ssd/Materials.owl#CeramicResin

:CeramicResin rdf:type owl:Class ;
              
              rdfs:subClassOf :Ceramic ,
                              :EngineeredMaterial ;
              
              or:referenceURL "http://www.matweb.com/index.aspx"^^xsd:anyURI ;
              
              <http://www.nist.gov/itl/ssd/OntologyRequirements.owl#termString> "ceramic resin"@en ,
                                                                                "high temperature ceramic resin"@en .



###  http://www.nist.gov/itl/ssd/Materials.owl#Cermet

:Cermet rdf:type owl:Class ;
        
        rdfs:subClassOf :Ceramic ,
                        :CompositeMaterial ,
                        :EngineeredMaterial ;
        
        rdfs:comment "Cermet is a composite material composed of ceramic and metallic materials."@en ;
        
        <http://www.nist.gov/itl/ssd/OntologyRequirements.owl#termString> "cermet"@en .



###  http://www.nist.gov/itl/ssd/Materials.owl#ChalcogenBasedCeramic

:ChalcogenBasedCeramic rdf:type owl:Class ;
                       
                       rdfs:subClassOf :Ceramic ;
                       
                       owl:disjointWith :NitrideBasedCeramic ,
                                        :OxideBasedCeramic ;
                       
                       or:referenceURL "http://www.matweb.com/index.aspx"^^xsd:anyURI ;
                       
                       <http://www.nist.gov/itl/ssd/OntologyRequirements.owl#termString> "chalcogenide"@en ,
                                                                                         "chalcogenide ceramic"@en .



###  http://www.nist.gov/itl/ssd/Materials.owl#ChemicalDiffusion

:ChemicalDiffusion rdf:type owl:Class ;
                   
                   rdfs:subClassOf :Diffusion ;
                   
                   owl:disjointWith :SelfDiffusion ,
                                    :Thermomigration ;
                   
                   rdfs:comment "Chemical Diffusion is diffusion under the influence of a gradient in chemical composition.  In concentrated solid solutions, e.g. A(1-x)Bx, or in diffusion couples, the motion of one constituent causes a counterflow of the other constituent(s) or vacancies.  Also called ``interdiffusion''."@en ;
                   
                   rdfs:seeAlso "Definitions of terms for diffusion in the solid state (IUPAC Recommendations 1999), Pure Appl. Chem. 71, 1307-1325."@en .



###  http://www.nist.gov/itl/ssd/Materials.owl#ChemicalSolution

:ChemicalSolution rdf:type owl:Class ;
                  
                  rdfs:subClassOf :PhysicalMixture ;
                  
                  owl:disjointWith :Colloid ,
                                   :ComplexFluid ,
                                   :CompositeMaterial ,
                                   :GelSubstance ,
                                   :PasteSubstance ;
                  
                  rdfs:comment "A Chemical Solution is a homogeneous mixture composed of only one phase. In such a mixture, one or more solutes (chemical substances) are dissolved in a larger quantity of another substance, known as a solvent.The solution more or less takes on the characteristics of the solvent, including its phase."@en .



###  http://www.nist.gov/itl/ssd/Materials.owl#ChemicalSuspension

:ChemicalSuspension rdf:type owl:Class ;
                    
                    rdfs:subClassOf :ComplexFluid ;
                    
                    owl:disjointWith :Colloid ,
                                     :GelSubstance ;
                    
                    rdfs:comment "A Chemical Suspension is a heterogeneous fluid containing solid particles that are sufficiently large that the particles will settle out (sedimentation) if the fluid is undisturbed for a sufficent length of time.. "@en .



###  http://www.nist.gov/itl/ssd/Materials.owl#ChromMolySteel

:ChromMolySteel rdf:type owl:Class ;
                
                rdfs:subClassOf :Steel ;
                
                owl:disjointWith :StainlessSteel ;
                
                or:referenceURL "http://www.matweb.com/index.aspx"^^xsd:anyURI ;
                
                <http://www.nist.gov/itl/ssd/OntologyRequirements.owl#termString> "CRMO"@en ,
                                                                                  "Crome-moly steels are steels that have chromium and molybdenum as alloying elements"@en ,
                                                                                  "chrome-moly steel"@en ,
                                                                                  "cromoly steel"@en .



###  http://www.nist.gov/itl/ssd/Materials.owl#Clathrate

:Clathrate rdf:type owl:Class ;
           
           rdfs:subClassOf bc:ChemicalSubstance ;
           
           owl:disjointWith :Vacuum ;
           
           rdfs:comment "A clathrate is a chemical substance consisting of a lattice of one type of molecule trapping and containing a second type of molecule."@en .



###  http://www.nist.gov/itl/ssd/Materials.owl#Clay

:Clay rdf:type owl:Class ;
      
      rdfs:subClassOf :PasteSubstance ;
      
      or:referenceURL "http://www.matweb.com/index.aspx"^^xsd:anyURI ;
      
      rdfs:comment "Clay is an earthy material that is plastic when moist but hard when fired, that is composed mainly of fine particles of hydrous aluminum silicates and other minerals, and that is used for brick, tile, and pottery.  Particles of clay are less than 5 microns in size according to the sedimentologists' definition; geologists and soil scientists use a limit of 2 microns, while colloid chemists define clays to have particles of under 1 micron in size."@en ;
      
      <http://www.nist.gov/itl/ssd/OntologyRequirements.owl#termString> "clay"@en .



###  http://www.nist.gov/itl/ssd/Materials.owl#ClosedCellFoam

:ClosedCellFoam rdf:type owl:Class ;
                
                rdfs:subClassOf :SolidFoam ;
                
                owl:disjointWith :OpenCellFoam ;
                
                rdfs:comment "A Closed-Cell Foam is a Solid Foam with a high proportion of intact bubbles."@en .



###  http://www.nist.gov/itl/ssd/Materials.owl#CobaltAlloy

:CobaltAlloy rdf:type owl:Class ;
             
             rdfs:subClassOf :NonFerrousAlloy ,
                             [ rdf:type owl:Restriction ;
                               owl:onProperty :physicalDecompositions ;
                               owl:someValuesFrom bc:Cobalt
                             ] ;
             
             or:referenceURL "http://www.matweb.com/index.aspx"^^xsd:anyURI ;
             
             rdfs:comment "An alloy that contains Cobalt but not Iron."@en .



###  http://www.nist.gov/itl/ssd/Materials.owl#ColinearInterstitialcyMechanism

:ColinearInterstitialcyMechanism rdf:type owl:Class ;
                                 
                                 rdfs:subClassOf :InterstitialcyMechanism ;
                                 
                                 owl:disjointWith :DirectInterstitialMechanism ,
                                                  :NonCollinearInterstitialcyMechanism ;
                                 
                                 rdfs:seeAlso "Definitions of terms for diffusion in the solid state (IUPAC Recommendations 1999), Pure Appl. Chem. 71, 1307-1325." ;
                                 
                                 rdfs:comment "The Collinear Iinterstitialcy Mechanism is an interstitialcy mechanism in which an interstitial atom and the lattice atom which it displaces move along the same straight line."@en .



###  http://www.nist.gov/itl/ssd/Materials.owl#Colloid

:Colloid rdf:type owl:Class ;
         
         rdfs:subClassOf :PhysicalMixture ;
         
         owl:disjointWith :CompositeMaterial ;
         
         rdfs:comment """A colloid is a solid, liquid, or gasseous substance comprised of one or more substances microscopically dispersed evenly throughout another substance (the dispersion medium).  

A colloidal system consists of two separate phases: a dispersed phase (or internal phase) and a continuous phase.  Either of the phases may be solid, liquid, or gas, however, both phases can not be gas."""@en .



###  http://www.nist.gov/itl/ssd/Materials.owl#ColloidalSol

:ColloidalSol rdf:type owl:Class ;
              
              rdfs:subClassOf :Colloid ,
                              :LiquidSubstance ;
              
              owl:disjointWith :Emulsion ,
                               :Foam ,
                               :LiquidSlag ,
                               :LiquidSolution ;
              
              rdfs:comment "A Colloidal Sol is a colloidal suspension of very small solid particles in a continuous liquid medium."@en .



###  http://www.nist.gov/itl/ssd/Materials.owl#CompactedPowderAlloy

:CompactedPowderAlloy rdf:type owl:Class ;
                      
                      rdfs:subClassOf :EngineeredAlloy ;
                      
                      owl:disjointWith :WroughtAlloy ;
                      
                      rdfs:comment "A Compacted Powder Alloy is produced by the  powder metallurgy process, generally consisting of four basic steps: (1) powder manufacture, (2) powder blending,(3) compacting, (4) either sintering or metal injection molding. "@en .



###  http://www.nist.gov/itl/ssd/Materials.owl#Compaction

:Compaction rdf:type owl:Class ;
            
            rdfs:subClassOf :Deformation ;
            
            owl:disjointWith :MaterialCreep ;
            
            rdfs:comment "Compaction is a process of pressing material such that it deforms and occupies less space.  Compaction can be intentional or not."@en .



###  http://www.nist.gov/itl/ssd/Materials.owl#ComplexFluid

:ComplexFluid rdf:type owl:Class ;
              
              rdfs:subClassOf :FluidSubstance ,
                              :PhysicalMixture ;
              
              owl:disjointWith :SolidSol ;
              
              rdfs:comment "Complex fluids are mixtures that have a coexistence between two phases: solid–liquid (suspensions or solutions of macromolecules such as polymers), solid–gas (granular), liquid–gas (foams) and liquid–liquid (emulsions)."@en .



###  http://www.nist.gov/itl/ssd/Materials.owl#CompositeMaterial

:CompositeMaterial rdf:type owl:Class ;
                   
                   rdfs:subClassOf :PhysicalMixture ,
                                   :SolidSubstance ;
                   
                   owl:disjointWith :CrystallineSubstance ,
                                    :GlassyMaterial .



###  http://www.nist.gov/itl/ssd/Materials.owl#CompositeMicrostructure

:CompositeMicrostructure rdf:type owl:Class ;
                         
                         rdfs:subClassOf :Microstructure ;
                         
                         owl:disjointWith :CrystalStructure ,
                                          :MetallicMicrostructure ,
                                          :PolymericMicrostructure ;
                         
                         rdfs:comment "A Composite Microstructure is a material Microstructure of a materials made from two or more constituent materials with significantly different physical or chemical properties which remain separate and distinct at microscopic scale within the finished structure."@en .



###  http://www.nist.gov/itl/ssd/Materials.owl#Compressibility

:Compressibility rdf:type owl:Class ;
                 
                 rdfs:subClassOf :DeformationProperty ;
                 
                 owl:disjointWith :ElasticModulus ,
                                  :FractureStrength ,
                                  :Hardness ,
                                  :Stiffness .



###  http://www.nist.gov/itl/ssd/Materials.owl#ConcentrationProfile

:ConcentrationProfile rdf:type owl:Class ;
                      
                      rdfs:subClassOf or:CurveSegment ;
                      
                      rdfs:comment "A Concentration Profile is a Curve of the variation in the concentration of a diffusing species as a function of distance in a material."@en ;
                      
                      rdfs:seeAlso "Definitions of terms for diffusion in the solid state (IUPAC Recommendations 1999), Pure Appl. Chem. 71, 1307-1325."@en .



###  http://www.nist.gov/itl/ssd/Materials.owl#Concrete

:Concrete rdf:type owl:Class ;
          
          rdfs:subClassOf :CompositeMaterial ,
                          :EngineeredMaterial ;
          
          or:referenceURL "http://www.matweb.com/index.aspx"^^xsd:anyURI ;
          
          <http://www.nist.gov/itl/ssd/OntologyRequirements.owl#termString> "concrete"@en .



###  http://www.nist.gov/itl/ssd/Materials.owl#Condensing

:Condensing rdf:type owl:Class ;
            
            rdfs:subClassOf :PhaseChange ;
            
            owl:disjointWith :CrystallinePhaseChange ,
                             :OrderDisorderPhaseTransformation ,
                             :PrecipitationFromSolution ,
                             :SolidToSolidPhaseTransformation ,
                             :Solidification ,
                             :Vaporization ;
            
            rdfs:comment "Condensing is the Phase Change from a gasseous state to a liquid state."@en .



###  http://www.nist.gov/itl/ssd/Materials.owl#CoolingProcess

:CoolingProcess rdf:type owl:Class ;
                
                rdfs:subClassOf :TemperatureChangeProcess ;
                
                rdfs:comment "A Cooling Process is a Temperature Change Process during which an object looses heat.  This could be due to endothermic reactions, the object radiating heat or warming up its environment, or some combination of these.. "@en .



###  http://www.nist.gov/itl/ssd/Materials.owl#CopperAlloy

:CopperAlloy rdf:type owl:Class ;
             
             rdfs:subClassOf :NonFerrousAlloy ,
                             [ rdf:type owl:Restriction ;
                               owl:onProperty :physicalDecompositions ;
                               owl:someValuesFrom bc:Copper
                             ] ;
             
             or:referenceURL "http://www.matweb.com/index.aspx"^^xsd:anyURI ;
             
             rdfs:comment "An alloy that contains Copper but little or no Iron."@en .



###  http://www.nist.gov/itl/ssd/Materials.owl#Cracking

:Cracking rdf:type owl:Class ;
          
          rdfs:subClassOf or:MechanicalProcess ,
                          or:MovementEvent ;
          
          owl:disjointWith :MaterialFatigue ,
                           :MicroscopicDiffusionMovement ,
                           :PhaseChange ,
                           :TemperatureChangeProcess ,
                           :ThermalExpansion ;
          
          rdfs:comment "Cracking is a Mechanical Process in which some solid object is cracked -- at either a macroscopic or microscopic level.  The cracked material need not be broken into separate pieces."@en .



###  http://www.nist.gov/itl/ssd/Materials.owl#CrowdionMechanism

:CrowdionMechanism rdf:type owl:Class ;
                   
                   rdfs:subClassOf :NonCollinearInterstitialcyMechanism ;
                   
                   owl:disjointWith :DumbellIntersticialcyMechanism ;
                   
                   rdfs:comment "Definitions of terms for diffusion in the solid state (IUPAC Recommendations 1999), Pure Appl. Chem. 71, 1307-1325." ,
                                "The Crowdion Mechanismi is a hypothesized mechanism in which diffusion takes place by a co-operative movement of a group of atoms one of which is typically centred on an interstitial position with the others relaxed from their normal lattice sites to accommodate the additional ‘crowdion’."@en ;
                   
                   <http://www.w3.org/2004/02/skos/core#note> "There was a big scientific controversy over the question if crowdions actually exist as a metastable interstitial configuration in the seventies. This controversy has never been finally resolved; however, most researchers in the field believe that it does not exist."@en ;
                   
                   rdfs:seeAlso "http://www.tf.uni-kiel.de/matwis/amat/def_en/kap_1/advanced/t1_3_1.html"@en .



###  http://www.nist.gov/itl/ssd/Materials.owl#CrystalGrain

:CrystalGrain rdf:type owl:Class ;
              
              rdfs:subClassOf :CrystallineSubstance ;
              
              rdfs:comment "Crystal grains or crystallites are small, often microscopic crystals that, held together through highly defective boundaries, constitute a polycrystalline solid."@en .



###  http://www.nist.gov/itl/ssd/Materials.owl#CrystalLattice

:CrystalLattice rdf:type owl:Class ;
                
                rdfs:subClassOf or:PhysicalObject ;
                
                owl:disjointWith :Vacuum .



###  http://www.nist.gov/itl/ssd/Materials.owl#CrystalStructure

:CrystalStructure rdf:type owl:Class ;
                  
                  rdfs:subClassOf :Microstructure ,
                                  or:MaterialType ;
                  
                  owl:disjointWith :MineralType ,
                                   :MultiphaseMaterialType ,
                                   :PolymericMicrostructure ;
                  
                  rdfs:comment "A crystal structure is composed of a pattern, a set of atoms arranged in a particular way, and a lattice exhibiting long-range order and symmetry."@en .



###  http://www.nist.gov/itl/ssd/Materials.owl#CrystallinePhaseChange

:CrystallinePhaseChange rdf:type owl:Class ;
                        
                        rdfs:subClassOf :MicrostructureEvolution ,
                                        :SolidToSolidPhaseTransformation ;
                        
                        owl:disjointWith :OrderDisorderPhaseTransformation ,
                                         :Solidification ,
                                         :Vaporization ;
                        
                        rdfs:comment "A Crystalline Phase Change is a Phase Change in which the phase changes between crystalline phases."@en .



###  http://www.nist.gov/itl/ssd/Materials.owl#CrystallineSubstance

:CrystallineSubstance rdf:type owl:Class ;
                      
                      rdfs:subClassOf bc:MaterialSubstance ;
                      
                      owl:disjointWith :GaseousSubstance ,
                                       :PasteSubstance ,
                                       :PolymerSubstance ,
                                       :Vacuum ;
                      
                      rdfs:comment "Material in a crystalline phase"@en .



###  http://www.nist.gov/itl/ssd/Materials.owl#CubicCrystalStructure

:CubicCrystalStructure rdf:type owl:Class ;
                       
                       rdfs:subClassOf :CrystalLattice ;
                       
                       owl:disjointWith :MonoclinicCrystalStructure ,
                                        :OrthorhombicCrystalStructure ,
                                        :TetragonalCrystalStructure ,
                                        :TriclinicCrystalStructure ,
                                        :TrigonalCrystalStructure .



###  http://www.nist.gov/itl/ssd/Materials.owl#Deformation

:Deformation rdf:type owl:Class ;
             
             rdfs:subClassOf or:MechanicalProcess ;
             
             rdfs:comment "Deformation is a Mechanical Process in which a solid or semi-solid object changes shape in response to outside forces."@en .



###  http://www.nist.gov/itl/ssd/Materials.owl#DeformationProperty

:DeformationProperty rdf:type owl:Class ;
                     
                     rdfs:subClassOf :MeasurableMechanicalProperty ;
                     
                     owl:disjointWith :Entropy ,
                                      :Strength ,
                                      :TransportProperty .



###  http://www.nist.gov/itl/ssd/Materials.owl#DeviatonicDominantPhaseTransformation

:DeviatonicDominantPhaseTransformation rdf:type owl:Class ;
                                       
                                       rdfs:subClassOf :LatticeDistortivePhaseTransformation ;
                                       
                                       owl:disjointWith :DilationDominantPhaseTransformation ;
                                       
                                       rdfs:comment "A deviatonic Dominant Phase Transformation is dominated in a sheer distortion in the lattice, with cutting plates perpendicular to the sheer undistorted."@en .



###  http://www.nist.gov/itl/ssd/Materials.owl#Diamond

:Diamond rdf:type owl:Class ;
         
         rdfs:subClassOf bc:Carbon ,
                         :SolidCrystallineSubstance ;
         
         owl:disjointWith :Graphite ;
         
         or:referenceURL "http://www.matweb.com/index.aspx"^^xsd:anyURI ;
         
         <http://www.nist.gov/itl/ssd/OntologyRequirements.owl#termString> "diamond"@en .



###  http://www.nist.gov/itl/ssd/Materials.owl#DielectricProperty

:DielectricProperty rdf:type owl:Class ;
                    
                    rdfs:subClassOf :ElectricalProperty ;
                    
                    owl:disjointWith :ElectricPolarizability ;
                    
                    rdfs:comment "Dielectric Properties are properties of a Dielectric -- an insulating material that undergoes polarization in an electric field."@en .



###  http://www.nist.gov/itl/ssd/Materials.owl#Diffusion

:Diffusion rdf:type owl:Class ;
           
           rdfs:subClassOf or:MechanicalProcess ,
                           or:MovementEvent ;
           
           owl:disjointWith :MaterialFatigue ,
                            :PhaseChange ,
                            :TemperatureChangeProcess ,
                            :ThermalExpansion ;
           
           rdfs:comment "Diffusion is the process of the spread of particles through random motion from regions of higher concentration to regions of lower concentration. The time dependence of the statistical distribution in space is given by the diffusion equation."@en .



###  http://www.nist.gov/itl/ssd/Materials.owl#DiffusionBonding

:DiffusionBonding rdf:type owl:Class ;
                  
                  rdfs:subClassOf <http://www.nist.gov/itl/ssd/Biochem.owl#ChemicalProcess> ;
                  
                  rdfs:seeAlso "Definitions of terms for diffusion in the solid state (IUPAC Recommendations 1999), Pure Appl. Chem. 71, 1307-1325."@en ;
                  
                  rdfs:comment "Diffusion Bonding is a solid state bonding process that joins two materials by a diffusion reaction."@en .



###  http://www.nist.gov/itl/ssd/Materials.owl#DiffusionInducedGrainBoundaryMigration

:DiffusionInducedGrainBoundaryMigration rdf:type owl:Class ;
                                        
                                        rdfs:subClassOf :MicroscopicDiffusionMovement ,
                                                        :MicrostructureEvolution ;
                                        
                                        owl:disjointWith :ExchangeMechanismForDiffusion ,
                                                         :FiveFrequencyDiffusionModel ,
                                                         :InterstitialcyMechanism ,
                                                         :RelaxationMethodForDiffusion ;
                                        
                                        rdfs:seeAlso "Definitions of terms for diffusion in the solid state (IUPAC Recommendations 1999), Pure Appl. Chem. 71, 1307-1325." ;
                                        
                                        rdfs:comment "If a polycrystalline material undergoes an interdiffusion process, the grain boundaries move in a direction perpendicular to the diffusion flux.  As a result the concentrations in the regions swept by the boundaries change.  This is called ``Diffusion-Induced Grain boundary Migration'' (DIGM)."@en ;
                                        
                                        <http://www.nist.gov/itl/ssd/OntologyRequirements.owl#termString> "diffusion induced grain boundary migration"@en .



###  http://www.nist.gov/itl/ssd/Materials.owl#DiffusionMovementMechanism

:DiffusionMovementMechanism rdf:type owl:Class ;
                            
                            rdfs:subClassOf or:EventType ;
                            
                            rdfs:comment "A Diffusion Movement Mechanism is a type of microscopic movement which is responsible for diffusion."@en .



###  http://www.nist.gov/itl/ssd/Materials.owl#DiffusionProperty

:DiffusionProperty rdf:type owl:Class ;
                   
                   rdfs:subClassOf or:MeasurableMaterialProperty ;
                   
                   rdfs:comment "A Diffusion Property is a physical property of some physical material or object, related from diffusion, whether chemical, electrical, magnetic, or thermal diffusion. "@en .



###  http://www.nist.gov/itl/ssd/Materials.owl#DiffusionalPhaseTransformation

:DiffusionalPhaseTransformation rdf:type owl:Class ;
                                
                                rdfs:subClassOf :PhaseChange ;
                                
                                rdfs:comment "A diffusional transformation is a phase change that occurs via the long-range diffusion of atoms"@en .



###  http://www.nist.gov/itl/ssd/Materials.owl#DiffusionlessPhaseTransformation

:DiffusionlessPhaseTransformation rdf:type owl:Class ;
                                  
                                  rdfs:subClassOf :CrystallinePhaseChange ;
                                  
                                  daml:seeAlso "http://en.wikipedia.org/w/index.php?title=File:Diffusionless_classification.svg" ;
                                  
                                  rdfs:comment "A diffusionless transformation is a phase change that occurs without the long-range diffusion of atoms but rather by some form of cooperative, homogeneous movement of many atoms that results in a change in crystal structure. These movements are small, usually less than the interatomic distances, and the atoms maintain their relative relationships."@en .



###  http://www.nist.gov/itl/ssd/Materials.owl#DilationDominantPhaseTransformation

:DilationDominantPhaseTransformation rdf:type owl:Class ;
                                     
                                     rdfs:subClassOf :LatticeDistortivePhaseTransformation ;
                                     
                                     rdfs:comment "A Dilation Dominant Phase Transformation is dominated by the expansion or contraction of the atomic lattice."@en .



###  http://www.nist.gov/itl/ssd/Materials.owl#DirectInterstitialMechanism

:DirectInterstitialMechanism rdf:type owl:Class ;
                             
                             rdfs:subClassOf :InterstitialcyMechanism ;
                             
                             owl:disjointWith :NonCollinearInterstitialcyMechanism ;
                             
                             rdfs:seeAlso "Definitions of terms for diffusion in the solid state (IUPAC Recommendations 1999), Pure Appl. Chem. 71, 1307-1325."@en ;
                             
                             rdfs:comment "In the Direct Interstitial Mechanism diffusion takes place by the direct migration of an interstitial species from one interstitial position to another."@en .



###  http://www.nist.gov/itl/ssd/Materials.owl#DisorderedBCCPhase

:DisorderedBCCPhase rdf:type owl:Class ;
                    
                    rdfs:subClassOf :BodyCenteredCubicCrystalStructure ;
                    
                    owl:disjointWith :OrderedBCCPhase .



###  http://www.nist.gov/itl/ssd/Materials.owl#DisorderedFCCPhase

:DisorderedFCCPhase rdf:type owl:Class ;
                    
                    rdfs:subClassOf :FaceCenteredCubicCrystalStructure ;
                    
                    owl:disjointWith :OrderedFCCPhase .



###  http://www.nist.gov/itl/ssd/Materials.owl#DisorderedHCPPhase

:DisorderedHCPPhase rdf:type owl:Class ;
                    
                    rdfs:subClassOf :HexagonalClosePackedCrystalStructure ;
                    
                    owl:disjointWith :OrderedHCPPhase .



###  http://www.nist.gov/itl/ssd/Materials.owl#DisorderedSolidSolution

:DisorderedSolidSolution rdf:type owl:Class ;
                         
                         rdfs:subClassOf :MaterialPhaseComposition .



###  http://www.nist.gov/itl/ssd/Materials.owl#DissociativeDiffusion

:DissociativeDiffusion rdf:type owl:Class ;
                       
                       rdfs:subClassOf :Heterodiffusion ;
                       
                       owl:disjointWith :InterchangeDiffusion ;
                       
                       rdfs:seeAlso "Definitions of terms for diffusion in the solid state (IUPAC Recommendations 1999), Pure Appl. Chem. 71, 1307-1325."@en ;
                       
                       rdfs:comment "Dissociative diffusion is the process by which foreign atoms predominantly present at normal lattice sites migrate via interstitial sites."@en .



###  http://www.nist.gov/itl/ssd/Materials.owl#DistortedHexagonalCrystalStructure

:DistortedHexagonalCrystalStructure rdf:type owl:Class ;
                                    
                                    rdfs:subClassOf :HexagonalCrystalStructure ;
                                    
                                    owl:disjointWith :DoubleHexagonalClosePackedCrystalStructure ,
                                                     :HexagonalClosePackedCrystalStructure .



###  http://www.nist.gov/itl/ssd/Materials.owl#DivacancyMechanism

:DivacancyMechanism rdf:type owl:Class ;
                    
                    rdfs:subClassOf :VacancyDiffusionMechanism ;
                    
                    owl:disjointWith :FiveFrequencyDiffusionModel ,
                                     :RelaxationMethodForDiffusion ;
                    
                    rdfs:seeAlso "Definitions of terms for diffusion in the solid state (IUPAC Recommendations 1999), Pure Appl. Chem. 71, 1307-1325."@en ;
                    
                    rdfs:comment "The Divacancy Mechanism is the diffusion process by which a crystal lattice vacancy pair is used by any constituent species of the material to effect diffusion."@en .



###  http://www.nist.gov/itl/ssd/Materials.owl#DoubleHexagonalClosePackedCrystalStructure

:DoubleHexagonalClosePackedCrystalStructure rdf:type owl:Class ;
                                            
                                            rdfs:subClassOf :HexagonalCrystalStructure ;
                                            
                                            owl:disjointWith :HexagonalClosePackedCrystalStructure .



###  http://www.nist.gov/itl/ssd/Materials.owl#DuctileIron

:DuctileIron rdf:type owl:Class ;
             
             rdfs:subClassOf :CastIron ;
             
             owl:disjointWith :GrayCastIron ,
                              :MalleableIron ,
                              :WhiteCastIron ;
             
             or:referenceURL "http://www.matweb.com/index.aspx"^^xsd:anyURI ;
             
             rdfs:comment "Ductile iron, also known as ductile cast iron, nodular cast iron, spheroidal graphite iron, spherulitic graphite cast iron, and SG iron, is a type of cast iron that is much more flexible and elastic than other cast irons, due to its nodular graphite inclusions."@en ;
             
             <http://www.nist.gov/itl/ssd/OntologyRequirements.owl#termString> "SG iron"@en ,
                                                                               "ductile cast iron"@en ,
                                                                               "ductile iron"@en ,
                                                                               "nodular cast iron"@en ,
                                                                               "spheroidal graphite iron"@en ,
                                                                               "spherulitic graphite cast iron"@en .



###  http://www.nist.gov/itl/ssd/Materials.owl#DumbellIntersticialcyMechanism

:DumbellIntersticialcyMechanism rdf:type owl:Class ;
                                
                                rdfs:subClassOf :NonCollinearInterstitialcyMechanism ;
                                
                                rdfs:seeAlso "Definitions of terms for diffusion in the solid state (IUPAC Recommendations 1999), Pure Appl. Chem. 71, 1307-1325."@en ;
                                
                                rdfs:comment "In some diffusion systems the equilibrium configuration during an interstitialcy jump consists of a dumbbell-like defect with each of the moving ions being displaced by an equal amount from the normal lattice position.  Diffusion taking place via such species is said to proceed by a Dumbbell Interstitialcy Mechanism."@en .



###  http://www.nist.gov/itl/ssd/Materials.owl#DuplexStainlessSteel

:DuplexStainlessSteel rdf:type owl:Class ;
                      
                      rdfs:subClassOf :StainlessSteel ;
                      
                      owl:disjointWith :FerriticStainlessSteel ;
                      
                      or:referenceURL "http://www.matweb.com/index.aspx"^^xsd:anyURI ;
                      
                      rdfs:comment "Duplex Stainless Steels have a mixed microstructure of austenite and ferrite, the aim usually being to produce a 50/50 mix, although in commercial alloys the ratio may be 40/60. Duplex stainless steels have roughly twice the strength compared to austenitic stainless steels and also improved resistance to localized corrosion, particularly pitting, crevice corrosion and stress corrosion cracking. They are characterized by high chromium (19–32%) and molybdenum (up to 5%) and lower nickel contents than austenitic stainless steels."@en ;
                      
                      <http://www.nist.gov/itl/ssd/OntologyRequirements.owl#termString> "duplex"@en ,
                                                                                        "duplex stainless steel"@en .



###  http://www.nist.gov/itl/ssd/Materials.owl#ElasticModulus

:ElasticModulus rdf:type owl:Class ;
                
                rdfs:subClassOf :DeformationProperty ;
                
                owl:disjointWith :FractureStrength ,
                                 :Hardness ,
                                 :TransportProperty ;
                
                rdfs:comment "An elastic modulus is defined as the slope of its stress–strain curve of a substance within the range where the deformation is elastic.  Three varieties of this are Young's modulus, the sheer modulus, and the bulk modulus."@en .



###  http://www.nist.gov/itl/ssd/Materials.owl#Elastomer

:Elastomer rdf:type owl:Class ;
           
           rdfs:subClassOf :PolymerSubstance ;
           
           owl:disjointWith :Polyester ;
           
           rdfs:comment """An elastomer is a polymer with viscoelasticity, generally having low Young's modulus and high yield strain compared with other materials. Each of the monomers which link to form the polymer is usually made of carbon, hydrogen, oxygen and/or silicon. Elastomers are amorphous polymers existing above their glass transition temperature, so that considerable segmental motion is possible. At ambient temperatures, rubbers are thus relatively soft and deformable.  Rubber is an example elastomer.

Elastomers are usually thermosets but may also be thermoplastic."""@en .



###  http://www.nist.gov/itl/ssd/Materials.owl#ElectricPolarizability

:ElectricPolarizability rdf:type owl:Class ;
                        
                        rdfs:subClassOf :ElectricalProperty ;
                        
                        rdfs:comment "Electric Polarizability is the tendency of a substance's charge distribution to be distorted from its normal shape by an external electric field.  It is specified by the material's relative permittivity (dielectric constant)."@en .



###  http://www.nist.gov/itl/ssd/Materials.owl#ElectricalProperty

:ElectricalProperty rdf:type owl:Class ;
                    
                    rdfs:subClassOf or:MeasurableMaterialProperty ;
                    
                    owl:disjointWith :MechanicalProperty ,
                                     :OpticalProperty ,
                                     :RadiologicalProperty ,
                                     :ThermalProperty .



###  http://www.nist.gov/itl/ssd/Materials.owl#Electromigration

:Electromigration rdf:type owl:Class ;
                  
                  rdfs:subClassOf or:MovementEvent ;
                  
                  rdfs:comment "Electromigration is the transport of particles under the influence of an electric field"@en .



###  http://www.nist.gov/itl/ssd/Materials.owl#ElectronicMagneticAlloy

:ElectronicMagneticAlloy rdf:type owl:Class ;
                         
                         rdfs:subClassOf :Alloy ;
                         
                         or:referenceURL "http://www.matweb.com/index.aspx"^^xsd:anyURI ;
                         
                         rdfs:comment "This means `Electronic/Magnetic Alloy' as the term is used in MatWeb.  The term exculdes most ferrous metals."@en ;
                         
                         <http://www.nist.gov/itl/ssd/OntologyRequirements.owl#termString> "electronic/magnetic alloy"@en .



###  http://www.nist.gov/itl/ssd/Materials.owl#ElementalMetal

:ElementalMetal rdf:type owl:Class ;
                
                rdfs:subClassOf bc:ElementalSubstance ,
                                bc:Metal ;
                
                owl:disjointWith :PhysicalMixture ;
                
                rdfs:comment "ElementalMetal is Metal composed of a single element.  It is disjoint from Alloy."@en .



###  http://www.nist.gov/itl/ssd/Materials.owl#Emulsion

:Emulsion rdf:type owl:Class ;
          
          rdfs:subClassOf :Colloid ,
                          :ComplexFluid ;
          
          owl:disjointWith :Foam ,
                           :GelSubstance ;
          
          rdfs:comment "An Emulsion is a Colloid of two or more liquids that are normally immiscible."@en .



###  http://www.nist.gov/itl/ssd/Materials.owl#EnergyPerMass

:EnergyPerMass rdf:type owl:Class ;
               
               owl:equivalentClass [ rdf:type owl:Class ;
                                     owl:intersectionOf ( or:MeasurableQuantity
                                                          [ rdf:type owl:Restriction ;
                                                            owl:onProperty or:unitsFor ;
                                                            owl:someValuesFrom :UnitOfEnergyPerMass
                                                          ]
                                                        )
                                   ] ;
               
               rdfs:subClassOf or:MeasurableQuantity ,
                               [ rdf:type owl:Restriction ;
                                 owl:onProperty or:unitsFor ;
                                 owl:someValuesFrom :UnitOfEnergyPerMass
                               ] ;
               
               owl:disjointWith or:Area ,
                                or:ComputerStorageCapacity ,
                                or:Distance ,
                                or:Duration ,
                                or:Energy ,
                                or:Force ,
                                or:Mass ,
                                or:Pressure ,
                                or:Temperature ,
                                or:Volume ;
               
               rdfs:comment "Energy Per Mass is an amount of Energy divided by an amount of Mass.  It is used to specify the amount of energy that enters or leaves a system dependent upon the mass of the system that results in, or is caused by, some type of change."@en .



###  http://www.nist.gov/itl/ssd/Materials.owl#EngineeredAlloy

:EngineeredAlloy rdf:type owl:Class ;
                 
                 owl:equivalentClass [ rdf:type owl:Class ;
                                       owl:intersectionOf ( :Alloy
                                                            :EngineeredMaterial
                                                          )
                                     ] ;
                 
                 rdfs:subClassOf :Alloy ,
                                 :EngineeredMaterial ;
                 
                 rdfs:comment "An Engineered Alloy is one that has been deliberately manufactured, not one that occurs naturally."@en .



###  http://www.nist.gov/itl/ssd/Materials.owl#EngineeredMaterial

:EngineeredMaterial rdf:type owl:Class ;
                    
                    owl:equivalentClass [ rdf:type owl:Class ;
                                          owl:intersectionOf ( bc:MaterialSubstance
                                                               or:Artifact
                                                             )
                                        ] ;
                    
                    rdfs:subClassOf bc:MaterialSubstance ,
                                    or:Artifact .



###  http://www.nist.gov/itl/ssd/Materials.owl#Entropy

:Entropy rdf:type owl:Class ;
         
         rdfs:subClassOf :MeasurableMechanicalProperty ;
         
         owl:disjointWith :Strength ,
                          :TransportProperty .



###  http://www.nist.gov/itl/ssd/Materials.owl#Ethulose

:Ethulose rdf:type owl:Class ;
          
          rdfs:subClassOf :HydroxyalkylCelluloseEther ;
          
          owl:disjointWith :HydroxyethylCellulose ,
                           :HydroxyethylMethylCellulose ,
                           :HydroxypropylCellulose ,
                           :Hypromellose ;
          
          rdfs:comment "Ethulose (or ethylhydroxyethylcellulose)  is a cellulose derivative with CH2CH3 and -CH2-CH2OH groups bound to some of the hydroxyl groups of the glucopyranose monomers that make up the cellulose backbone."@en .



###  http://www.nist.gov/itl/ssd/Materials.owl#EthylCellulose

:EthylCellulose rdf:type owl:Class ;
                
                rdfs:subClassOf :AlkylCelluloseEthers ;
                
                owl:disjointWith :EthylMethylCellulose ,
                                 :Methylcellulose ;
                
                rdfs:comment "Ethyl cellulose is a derivative of cellulose in which some of the hydroxyl groups on the repeating glucose units are converted into ethyl ether groups. The number of ethyl groups can vary."@en .



###  http://www.nist.gov/itl/ssd/Materials.owl#EthylMethylCellulose

:EthylMethylCellulose rdf:type owl:Class ;
                      
                      rdfs:subClassOf :AlkylCelluloseEthers ;
                      
                      owl:disjointWith :Methylcellulose ;
                      
                      rdfs:comment "Ethyl cellulose is a derivative of cellulose in which some of the hydroxyl groups on the repeating glucose units are converted into ethyl ether groups and some into methyl ether groups. "@en .



###  http://www.nist.gov/itl/ssd/Materials.owl#EutecticAlloy

:EutecticAlloy rdf:type owl:Class ;
               
               rdfs:subClassOf :EngineeredAlloy ;
               
               rdfs:comment "A Eutectic Alloy is an alloy that has a specific ratio of component metals that solidifies at a lower temperature than any other composition made up of the same ingredients."@en .



###  http://www.nist.gov/itl/ssd/Materials.owl#EutecticTransformation

:EutecticTransformation rdf:type owl:Class ;
                        
                        rdfs:subClassOf :Solidification ;
                        
                        owl:disjointWith :PeritecticReaction ,
                                         :SublimatingToSolid ;
                        
                        rdfs:comment "A Eutectic Transformation is a phase change in which a two component single phase liquid is cooled and transforms into two solid phases."@en .



###  http://www.nist.gov/itl/ssd/Materials.owl#EutectoidAlloy

:EutectoidAlloy rdf:type owl:Class ;
                
                rdfs:subClassOf :EngineeredAlloy ;
                
                rdfs:comment "A Eutectoid Alloy is one in which a solid phase has transformed into two different phases on cooling past the eutectoid point. "@en .



###  http://www.nist.gov/itl/ssd/Materials.owl#EutectoidPhaseTransformation

:EutectoidPhaseTransformation rdf:type owl:Class ;
                              
                              rdfs:subClassOf :CrystallinePhaseChange .



###  http://www.nist.gov/itl/ssd/Materials.owl#EutectoidSteel

:EutectoidSteel rdf:type owl:Class ;
                
                rdfs:subClassOf :EutectoidAlloy .



###  http://www.nist.gov/itl/ssd/Materials.owl#Evaporating

:Evaporating rdf:type owl:Class ;
             
             rdfs:subClassOf :Vaporization ;
             
             owl:disjointWith :OrderDisorderPhaseTransformation ,
                              :Sublimating ;
             
             rdfs:comment "Evaporating is the Phase Change from a liquid state to a gasseous state."@en .



###  http://www.nist.gov/itl/ssd/Materials.owl#ExchangeMechanismForDiffusion

:ExchangeMechanismForDiffusion rdf:type owl:Class ;
                               
                               rdfs:subClassOf :MicroscopicDiffusionMovement ;
                               
                               owl:disjointWith :InterstitialcyMechanism ,
                                                :VacancyDiffusionMechanism ;
                               
                               rdfs:seeAlso "Definitions of terms for diffusion in the solid state (IUPAC Recommendations 1999), Pure Appl. Chem. 71, 1307-1325."@en ;
                               
                               rdfs:comment "The Exchange mechanism for Diffusion is the atomic mechanism whereby diffusion takes place by the direct interchange of two neighbouring atoms."@en ;
                               
                               <http://www.nist.gov/itl/ssd/OntologyRequirements.owl#termString> "exchange mechanism"@en .



###  http://www.nist.gov/itl/ssd/Materials.owl#FaceCenteredCubicCrystalStructure

:FaceCenteredCubicCrystalStructure rdf:type owl:Class ;
                                   
                                   rdfs:subClassOf :CubicCrystalStructure .



###  http://www.nist.gov/itl/ssd/Materials.owl#FastIonicConductor

:FastIonicConductor rdf:type owl:Class ;
                    
                    rdfs:subClassOf :SolidSubstance ;
                    
                    owl:disjointWith :Semiconductor ;
                    
                    rdfs:comment "A Fast Ionic Conductor (or ``fast ion conductor'') is a solid material that exhibits a high ionic conductivity of the order of those found in molten salts ( Ωi > 0.001 Siemen/cm). An alternate term is ``superionic conductor''."@en ;
                    
                    rdfs:seeAlso "Definitions of terms for diffusion in the solid state (IUPAC Recommendations 1999), Pure Appl. Chem. 71, 1307-1325."@en .



###  http://www.nist.gov/itl/ssd/Materials.owl#Feldspar

:Feldspar rdf:type owl:Class ;
          
          rdfs:subClassOf :Silicate ;
          
          rdfs:comment "Feldspars (KAlSi3O8 – NaAlSi3O8 – CaAl2Si2O8) are a group of rock-forming tectosilicate minerals."@en ;
          
          <http://www.nist.gov/itl/ssd/OntologyRequirements.owl#termString> "feldspar"@en .



###  http://www.nist.gov/itl/ssd/Materials.owl#FeldsparClay

:FeldsparClay rdf:type owl:Class ;
              
              rdfs:subClassOf :Clay ,
                              [ rdf:type owl:Restriction ;
                                owl:onProperty bc:primaryConstituentType ;
                                owl:someValuesFrom :Feldspar
                              ] ;
              
              or:referenceURL "http://www.matweb.com/index.aspx"^^xsd:anyURI ;
              
              <http://www.nist.gov/itl/ssd/OntologyRequirements.owl#termString> "feldspar clay"@en .



###  http://www.nist.gov/itl/ssd/Materials.owl#FerriticStainlessSteel

:FerriticStainlessSteel rdf:type owl:Class ;
                        
                        rdfs:subClassOf :StainlessSteel ;
                        
                        or:referenceURL "http://www.matweb.com/index.aspx"^^xsd:anyURI ;
                        
                        rdfs:comment "Ferritic stainless steels contain between 10.5% and 27% chromium and very little nickel, if any, but some types can contain lead. Most compositions include molybdenum; some, aluminium or titanium. Common ferritic grades include 18Cr-2Mo, 26Cr-1Mo, 29Cr-4Mo, and 29Cr-4Mo-2Ni."@en ,
                                     "ferritic stainless steel"@en .



###  http://www.nist.gov/itl/ssd/Materials.owl#FerrousAlloy

:FerrousAlloy rdf:type owl:Class ;
              
              owl:equivalentClass [ rdf:type owl:Class ;
                                    owl:intersectionOf ( :Alloy
                                                         [ rdf:type owl:Restriction ;
                                                           owl:onProperty :physicalDecompositions ;
                                                           owl:someValuesFrom bc:Iron
                                                         ]
                                                       )
                                  ] ;
              
              rdfs:subClassOf :Alloy ;
              
              owl:disjointWith :NonFerrousAlloy ;
              
              or:referenceURL "http://www.matweb.com/index.aspx"^^xsd:anyURI ;
              
              rdfs:comment "A Ferrous Alloy is one that contains iron."@en ;
              
              <http://www.nist.gov/itl/ssd/OntologyRequirements.owl#termString> "ferrous alloy"@en ,
                                                                                "ferrous metal"@en .



###  http://www.nist.gov/itl/ssd/Materials.owl#FiveFrequencyDiffusionModel

:FiveFrequencyDiffusionModel rdf:type owl:Class ;
                             
                             rdfs:subClassOf :VacancyDiffusionMechanism ;
                             
                             owl:disjointWith :RelaxationMethodForDiffusion ;
                             
                             rdfs:seeAlso "Definitions of terms for diffusion in the solid state (IUPAC Recommendations 1999), Pure Appl. Chem. 71, 1307-1325."@en ;
                             
                             rdfs:comment "The Five-Frequency Diffusion Model is a type of movement of impurity diffusion via monovacancies in face-centred-cubic (fcc) metals or on an fcc sublattice in ionic crystals. It is assumed that the only host atom jumps that differ from jumps in the pure lattice are those made by nearest neighbours of the impurity."@en .



###  http://www.nist.gov/itl/ssd/Materials.owl#FluidLubricant

:FluidLubricant rdf:type owl:Class ;
                
                rdfs:subClassOf :EngineeredMaterial ,
                                :LiquidSubstance ;
                
                or:referenceURL "http://www.matweb.com/index.aspx"^^xsd:anyURI .



###  http://www.nist.gov/itl/ssd/Materials.owl#FluidSubstance

:FluidSubstance rdf:type owl:Class ;
                
                rdfs:subClassOf bc:MaterialSubstance ;
                
                owl:disjointWith :SolidFoam ,
                                 :Vacuum ;
                
                rdfs:comment "A Fluid is a Material Substance that continually flows under an applied shear stress. Fluids are a subset of the phases of matter and include liquids, gases, plasmas and, to some extent, granular substances and plastic solids."@en .



###  http://www.nist.gov/itl/ssd/Materials.owl#Foam

:Foam rdf:type owl:Class ;
      
      rdfs:subClassOf :Colloid ;
      
      owl:disjointWith :GaseousSubstance ,
                       :GelSubstance ,
                       :SolidSol ;
      
      rdfs:comment "A Foam is a Material Substance that is formed by trapping pockets of gas in a liquid (Liquid Foam) or solid (Solid Foam)."@en .



###  http://www.nist.gov/itl/ssd/Materials.owl#FractureStrength

:FractureStrength rdf:type owl:Class ;
                  
                  rdfs:subClassOf :DeformationProperty ;
                  
                  owl:disjointWith :Hardness ,
                                   :Stiffness ;
                  
                  rdfs:comment "Fracture Strength,or breaking strength, is the stress at which a specimen fails via fracture"@en .



###  http://www.nist.gov/itl/ssd/Materials.owl#Fracturing

:Fracturing rdf:type owl:Class ;
            
            rdfs:subClassOf :Cracking ;
            
            rdfs:comment "Fracturing is a Mechanical Process in which some solid object is cracked and separated into two, or more, pieces (at least locally) under the action of stress."@en .



###  http://www.nist.gov/itl/ssd/Materials.owl#Freezing

:Freezing rdf:type owl:Class ;
          
          rdfs:subClassOf :Solidification ;
          
          owl:disjointWith :SublimatingToSolid ;
          
          rdfs:comment "Freezing is the Phase Change from a liquid state to a solid state."@en .



###  http://www.nist.gov/itl/ssd/Materials.owl#Fullerine

:Fullerine rdf:type owl:Class ;
           
           rdfs:subClassOf bc:Molecule ;
           
           rdfs:comment "A Fullerene is a molecule composed entirely of carbon, in the form of a hollow sphere, ellipsoid or tube. Spherical fullerenes are called buckyballs. Cylindrical ones are called carbon nanotubes."@en ;
           
           <http://www.nist.gov/itl/ssd/OntologyRequirements.owl#termString> "fullerine"@en .



###  http://www.nist.gov/itl/ssd/Materials.owl#FunctionalGradientMaterial

:FunctionalGradientMaterial rdf:type owl:Class ;
                            
                            rdfs:subClassOf :SolidSubstance .



###  http://www.nist.gov/itl/ssd/Materials.owl#GasInLiquidSolution

:GasInLiquidSolution rdf:type owl:Class ;
                     
                     rdfs:subClassOf :LiquidSolution ,
                                     [ rdf:type owl:Restriction ;
                                       owl:onProperty :solute ;
                                       owl:someValuesFrom :GaseousSubstance
                                     ] ;
                     
                     rdfs:comment "A Gas In Liquid Solution is a Chemical Solution in which the soute is gasseous and the solvent is liquid."@en .



###  http://www.nist.gov/itl/ssd/Materials.owl#GasMixture

:GasMixture rdf:type owl:Class ;
            
            rdfs:subClassOf :GaseousSubstance ,
                            :PhysicalMixture ;
            
            rdfs:comment "A Gas Mixture is a  Physical Mixture of gasses.  Some definitions of the word 'solution' subsume gas mixtures."@en .



###  http://www.nist.gov/itl/ssd/Materials.owl#GaseousSubstance

:GaseousSubstance rdf:type owl:Class ;
                  
                  rdfs:subClassOf :FluidSubstance ;
                  
                  owl:disjointWith :GelSubstance ,
                                   :LiquidFoam ,
                                   :LiquidSubstance ,
                                   :PasteSubstance ,
                                   :SolidSubstance ;
                  
                  rdfs:comment "Material in a gasseous phase."@en .



###  http://www.nist.gov/itl/ssd/Materials.owl#GasseousDiffusion

:GasseousDiffusion rdf:type owl:Class ;
                   
                   rdfs:subClassOf :Diffusion .



###  http://www.nist.gov/itl/ssd/Materials.owl#GelSubstance

:GelSubstance rdf:type owl:Class ;
              
              rdfs:subClassOf :AmorphousSubstance ,
                              :Colloid ,
                              :ComplexFluid ;
              
              owl:disjointWith :GlassyMaterial ,
                               :PasteSubstance ,
                               :PowderySubstance ;
              
              rdfs:comment "Material in a gel phase."@en .



###  http://www.nist.gov/itl/ssd/Materials.owl#GlassCeramic

:GlassCeramic rdf:type owl:Class ;
              
              rdfs:subClassOf :Ceramic ,
                              :EngineeredMaterial ,
                              :PolycrystallineMaterial ;
              
              or:referenceURL "http://www.matweb.com/index.aspx"^^xsd:anyURI ;
              
              rdfs:comment "Glass-ceramics are polycrystalline material produced through controlled crystallization of base glass. Glass-ceramic materials share many properties with both glasses and ceramics. Glass-ceramics have an amorphous phase and one or more crystalline phases and are produced by a so called 'controlled crystallization'."@en ;
              
              <http://www.nist.gov/itl/ssd/OntologyRequirements.owl#termString> "glass ceramic"@en ,
                                                                                "glass-ceramic"@en .



###  http://www.nist.gov/itl/ssd/Materials.owl#GlassyMaterial

:GlassyMaterial rdf:type owl:Class ;
                
                rdfs:subClassOf :AmorphousSubstance ;
                
                or:referenceURL "http://www.matweb.com/index.aspx"^^xsd:anyURI ;
                
                rdfs:comment "A glassy material is a manufactured or natural glass, e.g. obsidian."@en ;
                
                <http://www.nist.gov/itl/ssd/OntologyRequirements.owl#termString> "glass"@en .



###  http://www.nist.gov/itl/ssd/Materials.owl#GorskiEffect

:GorskiEffect rdf:type owl:Class ;
              
              rdfs:subClassOf :SolidDiffusion ;
              
              rdfs:seeAlso "Definitions of terms for diffusion in the solid state (IUPAC Recommendations 1999), Pure Appl. Chem. 71, 1307-1325."@en ;
              
              rdfs:comment "The Gorski Effect is the migration of atoms in an elastically deformed material. The effect is particularly observed for solute atoms with a strong size effect and high diffusivity in a matrix, for instance hydrogen atoms in a metal."@en .



###  http://www.nist.gov/itl/ssd/Materials.owl#GrainBoundaryDiffusion

:GrainBoundaryDiffusion rdf:type owl:Class ;
                        
                        rdfs:subClassOf :ShortCircuitDiffusion ;
                        
                        rdfs:seeAlso "Definitions of terms for diffusion in the solid state (IUPAC Recommendations 1999), Pure Appl. Chem. 71, 1307-1325."@en ;
                        
                        rdfs:comment "Grain Boundary Diffusion is diffusion which takes place along a grain boundary."@en .



###  http://www.nist.gov/itl/ssd/Materials.owl#Graphite

:Graphite rdf:type owl:Class ;
          
          rdfs:subClassOf bc:Carbon ,
                          :SolidCrystallineSubstance ;
          
          or:referenceURL "http://www.matweb.com/index.aspx"^^xsd:anyURI ;
          
          <http://www.nist.gov/itl/ssd/OntologyRequirements.owl#termString> "graphite"@en .



###  http://www.nist.gov/itl/ssd/Materials.owl#GrayCastIron

:GrayCastIron rdf:type owl:Class ;
              
              rdfs:subClassOf :CastIron ;
              
              owl:disjointWith :MalleableIron ,
                               :WhiteCastIron ;
              
              or:referenceURL "http://www.matweb.com/index.aspx"^^xsd:anyURI ;
              
              rdfs:comment "Gray (cast) iron, or grey (cast) iron, is a type of cast iron that has a graphitic microstructure. It is named after the gray color of the fracture it forms, which is due to the presence of graphite"@en ;
              
              <http://www.nist.gov/itl/ssd/OntologyRequirements.owl#termString> "gray cast iron"@en ,
                                                                                "gray iron"@en ,
                                                                                "grey cast iron"@en ,
                                                                                "grey iron"@en .



###  http://www.nist.gov/itl/ssd/Materials.owl#Halide

:Halide rdf:type owl:Class ;
        
        rdfs:subClassOf :PureSubstance ;
        
        or:referenceURL "http://www.matweb.com/index.aspx"^^xsd:anyURI ;
        
        rdfs:comment "A Halide is a binary compound, of which one part is a halogen atom and the other part is an element or radical that is less electronegative (or more electropositive) than the halogen, to make a fluoride, chloride, bromide, iodide, or astatide compound. Many salts are halides."@en ;
        
        <http://www.nist.gov/itl/ssd/OntologyRequirements.owl#termString> "halide"@en .



###  http://www.nist.gov/itl/ssd/Materials.owl#HalideMineral

:HalideMineral rdf:type owl:Class ;
               
               rdfs:subClassOf :Mineral .



###  http://www.nist.gov/itl/ssd/Materials.owl#Hardness

:Hardness rdf:type owl:Class ;
          
          rdfs:subClassOf :DeformationProperty ;
          
          owl:disjointWith :Stiffness .



###  http://www.nist.gov/itl/ssd/Materials.owl#Hardwood

:Hardwood rdf:type owl:Class ;
          
          rdfs:subClassOf :Wood ;
          
          or:referenceURL "http://www.matweb.com/index.aspx"^^xsd:anyURI ;
          
          <http://www.nist.gov/itl/ssd/OntologyRequirements.owl#termString> "hardwood"@en .



###  http://www.nist.gov/itl/ssd/Materials.owl#Hastelloy

:Hastelloy rdf:type owl:Class ;
           
           rdfs:subClassOf :NickelAlloy ,
                           :Superalloy ;
           
           owl:disjointWith :Waspaloy ;
           
           rdfs:comment "Hastelloys are Nickel-based Superalloys produced by Haynes International, Inc.  \"Hastelloy\" is a trademarked name for more than 10 different alloys, which are further distinguished with alphanumeric designations."@en .



###  http://www.nist.gov/itl/ssd/Materials.owl#HeatingProcess

:HeatingProcess rdf:type owl:Class ;
                
                rdfs:subClassOf :TemperatureChangeProcess ;
                
                rdfs:comment "A Heating Process is a Temperature Change Process during which the temperature of an object increases.  This could be due to internal  generation of heat, external heat warming the object, or both. "@en .



###  http://www.nist.gov/itl/ssd/Materials.owl#Heterodiffusion

:Heterodiffusion rdf:type owl:Class ;
                 
                 rdfs:subClassOf :SolidDiffusion ;
                 
                 owl:disjointWith :SelfDiffusion ;
                 
                 rdfs:seeAlso "Definitions of terms for diffusion in the solid state (IUPAC Recommendations 1999), Pure Appl. Chem. 71, 1307-1325." ,
                              "Heterodiffusion is the diffusion of foreign atoms in a material.  Also called ``imurity diffusion'' or ``solute diffusion''."@en .



###  http://www.nist.gov/itl/ssd/Materials.owl#HexagonalClosePackedCrystalStructure

:HexagonalClosePackedCrystalStructure rdf:type owl:Class ;
                                      
                                      rdfs:subClassOf :HexagonalCrystalStructure .



###  http://www.nist.gov/itl/ssd/Materials.owl#HexagonalCrystalStructure

:HexagonalCrystalStructure rdf:type owl:Class ;
                           
                           rdfs:subClassOf :TrigonalCrystalStructure ;
                           
                           owl:disjointWith :RhombohedralCrystalStructure ;
                           
                           rdfs:comment "the hexagonal crystal system is one of the 7 crystal systems, the hexagonal lattice system is one of the 7 lattice systems, and the hexagonal crystal family is one of the 6 crystal families. They are closely related and often confused with each other, but they are not the same. The hexagonal lattice system consists of just one Bravais lattice type: the hexagonal one. The hexagonal crystal system consists of the 7 point groups such that all their space groups have the hexagonal lattice as underlying lattice. The hexagonal crystal family consists of the 12 point groups such that at least one of their space groups has the hexagonal lattice as underlying lattice, and is the union of the hexagonal crystal system and the trigonal crystal system."@en .



###  http://www.nist.gov/itl/ssd/Materials.owl#HighSpeedSteel

:HighSpeedSteel rdf:type owl:Class ;
                
                rdfs:subClassOf :ToolSteel ;
                
                rdfs:comment "High speed steel (HSS or HS) is a subset of tool steels, commonly used in cutting tools. It is superior to the older high carbon steel tools in that it can withstand higher temperatures without losing its temper. This property allows HSS to cut faster than high carbon steel, hence the name high speed steel. At room temperature, in their generally recommended heat treatment, HSS grades generally display high hardness (above HRC60) and a high abrasion resistance (generally linked to vanadium content often used in HSS) compared to common carbon and tool steels."@en .



###  http://www.nist.gov/itl/ssd/Materials.owl#HighStrengthSteel

:HighStrengthSteel rdf:type owl:Class ;
                   
                   rdfs:subClassOf :AlloySteel ;
                   
                   rdfs:comment "High-strength low-alloy steel (HSLA) is a type of alloy steel that provides better mechanical properties or greater resistance to corrosion than carbon steel.  HSLA steels vary from other steels in that they are not made to meet a specific chemical composition but rather to specific mechanical properties. They have a carbon content between 0.05–0.25% to retain formability and weldability. Other alloying elements include up to 2.0% manganese and small quantities of copper, nickel, niobium, nitrogen, vanadium, chromium, molybdenum, titanium, calcium, rare earth elements, or zirconium. Copper, titanium, vanadium, and niobium are added for strengthening purposes."@en .



###  http://www.nist.gov/itl/ssd/Materials.owl#HydroxyalkylCelluloseEther

:HydroxyalkylCelluloseEther rdf:type owl:Class ;
                            
                            rdfs:subClassOf :CelluloseEther .



###  http://www.nist.gov/itl/ssd/Materials.owl#HydroxyethylCellulose

:HydroxyethylCellulose rdf:type owl:Class ;
                       
                       rdfs:subClassOf :HydroxyalkylCelluloseEther ;
                       
                       owl:disjointWith :HydroxypropylCellulose ,
                                        :Hypromellose ;
                       
                       rdfs:comment "Hydroxymethyl cellulose is a cellulose derivative with carboxymethyl groups (-CH2-CH2-OH) bound to some of the hydroxyl groups of the glucopyranose monomers that make up the cellulose backbone."@en .



###  http://www.nist.gov/itl/ssd/Materials.owl#HydroxyethylMethylCellulose

:HydroxyethylMethylCellulose rdf:type owl:Class ;
                             
                             rdfs:subClassOf :HydroxyalkylCelluloseEther ;
                             
                             owl:disjointWith :Hypromellose ;
                             
                             rdfs:comment "Hydroxy ethyl methyl cellulose (HPC) is an ether of cellulose in which some of the hydroxyl groups in the repeating glucose units have been replaced with -CH3 or -CH2CH2OH.  The percentage of hydroxyl groups substituted can vary."@en .



###  http://www.nist.gov/itl/ssd/Materials.owl#HydroxypropylCellulose

:HydroxypropylCellulose rdf:type owl:Class ;
                        
                        rdfs:subClassOf :HydroxyalkylCelluloseEther ;
                        
                        owl:disjointWith :Hypromellose ;
                        
                        rdfs:comment "Hydroxypropyl cellulose (HPC) is an ether of cellulose in which some of the hydroxyl groups in the repeating glucose units have been hydroxypropylated forming -OCH2CH(OH)CH3 groups using propylene oxide.  The percentage of hydroxyl groups substituted can vary."@en .



###  http://www.nist.gov/itl/ssd/Materials.owl#Hypromellose

:Hypromellose rdf:type owl:Class ;
              
              rdfs:subClassOf :HydroxyalkylCelluloseEther ;
              
              rdfs:comment "Hypromellose (INN), short for hydroxypropyl methylcellulose (HPMC), is a cellulose derivative with CH3 and -CH2-CH(OH)CH3 groups bound to some of the hydroxyl groups of the glucopyranose monomers that make up the cellulose backbone."@en .



###  http://www.nist.gov/itl/ssd/Materials.owl#IndentationHardness

:IndentationHardness rdf:type owl:Class ;
                     
                     rdfs:subClassOf :Hardness ;
                     
                     rdfs:comment "Indentation Hardness measures the resistance of a sample to permanent plastic deformation due to a constant compression load.  Scales used (depending upon the hardness of the material) are Vickers, Shore, Rockwell, and Brinell."@en .



###  http://www.nist.gov/itl/ssd/Materials.owl#InterchangeDiffusion

:InterchangeDiffusion rdf:type owl:Class ;
                      
                      rdfs:subClassOf :Heterodiffusion ;
                      
                      rdfs:seeAlso "Definitions of terms for diffusion in the solid state (IUPAC Recommendations 1999), Pure Appl. Chem. 71, 1307-1325."@en ;
                      
                      rdfs:comment "Interchange Diffusion is diffusion in which foreign atoms predominately present at interstitital lattice sites migrate via normal sites."@en .



###  http://www.nist.gov/itl/ssd/Materials.owl#InterstitialDiffusion

:InterstitialDiffusion rdf:type owl:Class ;
                       
                       rdfs:subClassOf :LatticeDiffusion ;
                       
                       owl:disjointWith :VacancyWindEffect ;
                       
                       rdfs:seeAlso "Definitions of terms for diffusion in the solid state (IUPAC Recommendations 1999), Pure Appl. Chem. 71, 1307-1325."@en ;
                       
                       rdfs:comment "Interstitial Diffusion is diffusion that takes place via interstitial sites."@en ;
                       
                       <http://www.nist.gov/itl/ssd/OntologyRequirements.owl#termString> "interstitial diffusion"@en .



###  http://www.nist.gov/itl/ssd/Materials.owl#InterstitialcyMechanism

:InterstitialcyMechanism rdf:type owl:Class ;
                         
                         rdfs:subClassOf :MicroscopicDiffusionMovement ;
                         
                         owl:disjointWith :VacancyDiffusionMechanism ;
                         
                         rdfs:comment "A Interstitialcy Mechanism is a mechanism where migration of atoms in diffusion  occurs by an interstitial atom moving onto a normal lattice site whilst simultaneously the original lattice atom moves into an interstitial position."@en ;
                         
                         rdfs:seeAlso "Definitions of terms for diffusion in the solid state (IUPAC Recommendations 1999), Pure Appl. Chem. 71, 1307-1325." ;
                         
                         <http://www.nist.gov/itl/ssd/OntologyRequirements.owl#termString> "interstitialcy mechanism"@en .



###  http://www.nist.gov/itl/ssd/Materials.owl#IonicLiquid

:IonicLiquid rdf:type owl:Class ;
             
             rdfs:subClassOf :LiquidSubstance ;
             
             rdfs:comment "An ionic liquid is a salt in the liquid state."@en .



###  http://www.nist.gov/itl/ssd/Materials.owl#IonicLiquidSolution

:IonicLiquidSolution rdf:type owl:Class ;
                     
                     owl:equivalentClass [ rdf:type owl:Class ;
                                           owl:intersectionOf ( :IonicLiquid
                                                                :LiquidSolution
                                                              )
                                         ] ;
                     
                     rdfs:subClassOf :LiquidSolution ;
                     
                     owl:disjointWith :NonIonicOrAqueousLiquidSolution .



###  http://www.nist.gov/itl/ssd/Materials.owl#KaolinClay

:KaolinClay rdf:type owl:Class ;
            
            rdfs:subClassOf :Clay ;
            
            or:referenceURL "http://www.matweb.com/index.aspx"^^xsd:anyURI ;
            
            <http://www.nist.gov/itl/ssd/OntologyRequirements.owl#termString> "kaolin clay"@en .



###  http://www.nist.gov/itl/ssd/Materials.owl#KirkendallEffect

:KirkendallEffect rdf:type owl:Class ;
                  
                  rdfs:subClassOf :Heterodiffusion ;
                  
                  rdfs:seeAlso "Definitions of terms for diffusion in the solid state (IUPAC Recommendations 1999), Pure Appl. Chem. 71, 1307-1325."@en ;
                  
                  rdfs:comment "The Kirkendall Effect occurs during interdiffusion between specimens in a diffusion couple when the intrinsic diffusion coefficients of the components are different. The greater flux of atoms in one direction over the other direction causes the original interface, called the Kirkendall plane, to be displaced by a distance called the Kirkendall shift. This shift can be observed by the movement of inert markers."@en .



###  http://www.nist.gov/itl/ssd/Materials.owl#KirkendallPlane

:KirkendallPlane rdf:type owl:Class ;
                 
                 rdfs:subClassOf <http://www.nist.gov/itl/ssd/OntologyRequirements.owl#PlanarRegion> ;
                 
                 owl:disjointWith :MatanoPlane ;
                 
                 rdfs:seeAlso "Definitions of terms for diffusion in the solid state (IUPAC Recommendations 1999), Pure Appl. Chem. 71, 1307-1325." ;
                 
                 <http://www.nist.gov/itl/ssd/OntologyRequirements.owl#termString> "Kirkendall plane"@en ;
                 
                 rdfs:comment "The Kirkendall effect occurs during interdiffusion between specimens in a diffusion couple when the intrinsic diffusion coefficients of the components are different. The greater flux of atoms in one direction over the other direction causes the original interface, called the Kirkendall plane, to be displaced by a distance called the Kirkendall shift. This shift can be observed by the movement of inert markers."@en .



###  http://www.nist.gov/itl/ssd/Materials.owl#LaboratoryFrameOfReference

:LaboratoryFrameOfReference rdf:type owl:Class ;
                            
                            rdfs:subClassOf <http://www.nist.gov/itl/ssd/OntologyRequirements.owl#SpatialFrameOfReference> ;
                            
                            <http://www.nist.gov/itl/ssd/OntologyRequirements.owl#termString> "laboratory frame of reference"@en .



###  http://www.nist.gov/itl/ssd/Materials.owl#LaboratoryFrameOfReferenceForDiffusion

:LaboratoryFrameOfReferenceForDiffusion rdf:type owl:Class ;
                                        
                                        rdfs:subClassOf :LaboratoryFrameOfReference ;
                                        
                                        rdfs:seeAlso "Definitions of terms for diffusion in the solid state (IUPAC Recommendations 1999), Pure Appl. Chem. 71, 1307-1325." ;
                                        
                                        rdfs:comment "In binary diffusion the fluxes JA and JB of species A and B generally will be different. A frame of reference defined by the condition J=JB=0 is called the laboratory frame. A convenient laboratory frame is the end of the specimen since at the ends JA=JB=0, so that the condition JA=JB=0 is always fulfilled. The Matano plane is an example of a laboratory frame."@en ;
                                        
                                        <http://www.nist.gov/itl/ssd/OntologyRequirements.owl#termString> "laboratory frame"@en .



###  http://www.nist.gov/itl/ssd/Materials.owl#LatticeDiffusion

:LatticeDiffusion rdf:type owl:Class ;
                  
                  rdfs:subClassOf :SolidDiffusion ;
                  
                  owl:disjointWith :ShortCircuitDiffusion ,
                                   :SurfaceDiffusion ;
                  
                  rdfs:seeAlso "Definitions of terms for diffusion in the solid state (IUPAC Recommendations 1999), Pure Appl. Chem. 71, 1307-1325."@en ;
                  
                  rdfs:comment "Lattice diffusion is a diffusion process which takes place through the bulk lattice of the crystal and excludes such mechanisms as Short Circuit Diffusion along dislocations, Grain Boundary Diffusion, and Surface Diffusion.  Also called ``bulk diffusion'' or ``volume diffusion''."@en ;
                  
                  <http://www.nist.gov/itl/ssd/OntologyRequirements.owl#termString> "lattice diffusion"@en .



###  http://www.nist.gov/itl/ssd/Materials.owl#LatticeDistortivePhaseTransformation

:LatticeDistortivePhaseTransformation rdf:type owl:Class ;
                                      
                                      rdfs:subClassOf :DiffusionlessPhaseTransformation ;
                                      
                                      owl:disjointWith :ShufflePhaseTransformation ;
                                      
                                      rdfs:comment "Homogeneous lattice-distortive phase transformations are transformations from one Bravais lattice into a different one."@en .



###  http://www.nist.gov/itl/ssd/Materials.owl#LatticeFixedFrame

:LatticeFixedFrame rdf:type owl:Class ;
                   
                   rdfs:subClassOf <http://www.nist.gov/itl/ssd/OntologyRequirements.owl#SpatialFrameOfReference> ;
                   
                   rdfs:seeAlso "Definitions of terms for diffusion in the solid state (IUPAC Recommendations 1999), Pure Appl. Chem. 71, 1307-1325."@en ;
                   
                   <http://www.nist.gov/itl/ssd/OntologyRequirements.owl#termString> "Kirkendall frame"@en ;
                   
                   rdfs:comment """The Lattice Fixed Frame is used when the diffusion flux gives rise to a net flux of material. The lattice fixed frame, also called inert-marker or Kirkendall frame, moves with the local flux of the material. The
Kirkendall plane is an example of a lattice fixed frame. The frame is in the general case not connected to an average velocity of the constituents, but to the velocity of the markers."""@en ;
                   
                   <http://www.nist.gov/itl/ssd/OntologyRequirements.owl#termString> "inert marker frame"@en ,
                                                                                     "lattice fixed frame"@en .



###  http://www.nist.gov/itl/ssd/Materials.owl#LavesPhase

:LavesPhase rdf:type owl:Class ;
            
            rdfs:subClassOf :ThermodynamicPhase ;
            
            rdfs:comment "Laves phases are intermetallic phases that have composition AB2.  In general, the A atoms are ordered as in diamond, hexagonal diamond, or a related structure, and the B atoms form tetrahedra around the A atoms for the AB2 structure.  There are three different classification classes: cubic, hexagonal MgZn2, and hexagonal MgNi2. "@en .



###  http://www.nist.gov/itl/ssd/Materials.owl#LeadAlloy

:LeadAlloy rdf:type owl:Class ;
           
           rdfs:subClassOf :NonFerrousAlloy ,
                           [ rdf:type owl:Restriction ;
                             owl:onProperty :physicalDecompositions ;
                             owl:someValuesFrom bc:Lead
                           ] ;
           
           or:referenceURL "http://www.matweb.com/index.aspx"^^xsd:anyURI ;
           
           rdfs:comment "An alloy that contains Lead but not Iron."@en .



###  http://www.nist.gov/itl/ssd/Materials.owl#LiquidAerosol

:LiquidAerosol rdf:type owl:Class ;
               
               rdfs:subClassOf :Aerosol ;
               
               owl:disjointWith :SolidAerosol ;
               
               rdfs:comment "A Liquid Aerosol is a colloid suspension of liquid droplets in a gas."@en .



###  http://www.nist.gov/itl/ssd/Materials.owl#LiquidCrystallineSubstance

:LiquidCrystallineSubstance rdf:type owl:Class ;
                            
                            rdfs:subClassOf :CrystallineSubstance ;
                            
                            owl:disjointWith :SolidCrystallineSubstance .



###  http://www.nist.gov/itl/ssd/Materials.owl#LiquidDiffusion

:LiquidDiffusion rdf:type owl:Class ;
                 
                 rdfs:subClassOf :Diffusion .



###  http://www.nist.gov/itl/ssd/Materials.owl#LiquidFoam

:LiquidFoam rdf:type owl:Class ;
            
            rdfs:subClassOf :ComplexFluid ,
                            :Foam ;
            
            rdfs:comment "A Liqulid Foam is a substance that is formed by trapping pockets of gas within liquid membranes."@en .



###  http://www.nist.gov/itl/ssd/Materials.owl#LiquidInLiquidSolution

:LiquidInLiquidSolution rdf:type owl:Class ;
                        
                        rdfs:subClassOf :LiquidSolution ,
                                        [ rdf:type owl:Restriction ;
                                          owl:onProperty :solute ;
                                          owl:someValuesFrom :LiquidSubstance
                                        ] ;
                        
                        rdfs:comment "A Liquid In Liquid Solution is a Chemical Solution in which the soute and solvent are both liquid."@en .



###  http://www.nist.gov/itl/ssd/Materials.owl#LiquidSlag

:LiquidSlag rdf:type owl:Class ;
            
            rdfs:subClassOf :EngineeredMaterial ,
                            :LiquidSubstance ,
                            :PhysicalMixture ;
            
            rdfs:comment "Liquid Slag is formed during steel production, floating on top of the liquid steel."@en .



###  http://www.nist.gov/itl/ssd/Materials.owl#LiquidSolution

:LiquidSolution rdf:type owl:Class ;
                
                rdfs:subClassOf :ChemicalSolution ,
                                :LiquidSubstance ,
                                [ rdf:type owl:Restriction ;
                                  owl:onProperty :solvent ;
                                  owl:onClass :LiquidSubstance ;
                                  owl:qualifiedCardinality "1"^^xsd:nonNegativeInteger
                                ] ;
                
                rdfs:comment "A Liquid Solution is a Chemical Solution in which both the solvent and the solution itself are liquids.  The solute may be solid, liquid, or gas."@en .



###  http://www.nist.gov/itl/ssd/Materials.owl#LiquidSubstance

:LiquidSubstance rdf:type owl:Class ;
                 
                 rdfs:subClassOf :FluidSubstance ;
                 
                 owl:disjointWith :SolidSubstance ;
                 
                 rdfs:comment "Material in a liquid phase."@en .



###  http://www.nist.gov/itl/ssd/Materials.owl#Liquidus

:Liquidus rdf:type owl:Class ;
          
          rdfs:subClassOf or:CurveSegment ;
          
          rdfs:comment "A Liquidus is a Curve on a temperature-concentration Phase Diagram above which a given substance is completely liquid.  Between the Liquidus and the Solidus, the substance is a mixture of solid and liquid phases."@en .



###  http://www.nist.gov/itl/ssd/Materials.owl#LithiumGellant

:LithiumGellant rdf:type owl:Class ;
                
                rdfs:subClassOf :FluidLubricant ;
                
                owl:disjointWith :MultiplyAlkylatedCyclopentane ,
                                 :OrganicSoapGellant ,
                                 :PTFEGellant ,
                                 :Perfluoropolyether ,
                                 :Polyalphaolefin ,
                                 :Polyglycol ,
                                 :PolyphenyletherBaseLubricant ,
                                 :Quenchant ,
                                 :SiliconeBaseLubricant ,
                                 :SiliconeGellant ,
                                 :SyntheticEtherBase ,
                                 :UreaGellant ,
                                 :WhiteMineralOil ,
                                 :ZincOxideLubricant ;
                
                or:referenceURL "http://www.matweb.com/index.aspx"^^xsd:anyURI ;
                
                <http://www.nist.gov/itl/ssd/OntologyRequirements.owl#termString> "lithium gellant"@en .



###  http://www.nist.gov/itl/ssd/Materials.owl#MachinableCeramic

:MachinableCeramic rdf:type owl:Class ;
                   
                   rdfs:subClassOf :Ceramic ,
                                   :EngineeredMaterial ;
                   
                   or:referenceURL "http://www.matweb.com/index.aspx"^^xsd:anyURI ;
                   
                   rdfs:comment "Machinable Ceramic is a ceramic substance that can be machined on conventional shop equipment with standard cutting tools."@en ;
                   
                   <http://www.nist.gov/itl/ssd/OntologyRequirements.owl#termString> "machinable ceramic"@en .



###  http://www.nist.gov/itl/ssd/Materials.owl#MagnesiumAlloy

:MagnesiumAlloy rdf:type owl:Class ;
                
                rdfs:subClassOf :NonFerrousAlloy ,
                                [ rdf:type owl:Restriction ;
                                  owl:onProperty :physicalDecompositions ;
                                  owl:someValuesFrom bc:Magnesium
                                ] ;
                
                or:referenceURL "http://www.matweb.com/index.aspx"^^xsd:anyURI ;
                
                rdfs:comment "An alloy that contains Magnesium but not Iron."@en .



###  http://www.nist.gov/itl/ssd/Materials.owl#MagnesiumOxide

:MagnesiumOxide rdf:type owl:Class ;
                
                rdfs:subClassOf bc:Oxide ;
                
                owl:disjointWith :SiliconOxide ,
                                 :TitaniumOxide ,
                                 :ZirconiumOxide ;
                
                or:referenceURL "http://www.matweb.com/index.aspx"^^xsd:anyURI ;
                
                <http://www.nist.gov/itl/ssd/OntologyRequirements.owl#termString> "magnesium oxide"@en .



###  http://www.nist.gov/itl/ssd/Materials.owl#MagneticProperty

:MagneticProperty rdf:type owl:Class ;
                  
                  rdfs:subClassOf or:MeasurableMaterialProperty ;
                  
                  owl:disjointWith :MechanicalProperty ,
                                   :OpticalProperty ,
                                   :RadiologicalProperty ,
                                   :ThermalProperty .



###  http://www.nist.gov/itl/ssd/Materials.owl#MalleableIron

:MalleableIron rdf:type owl:Class ;
               
               rdfs:subClassOf :CastIron ;
               
               owl:disjointWith :WhiteCastIron ;
               
               or:referenceURL "http://www.matweb.com/index.aspx"^^xsd:anyURI ;
               
               rdfs:comment "Malleable iron is cast as white iron, the structure being a metastable carbide in a pearlitic matrix. Through an annealing heat treatment, the brittle structure as first cast, is transformed into the malleable form. Carbon agglomerates into small roughly spherical aggregates of graphite leaving a matrix of ferrite or pearlite according to the exact heat treat used. Three basic types of malleable iron are recognized within the casting industry: Blackheart malleable iron, Whiteheart malleable iron and Pearlitic malleable iron."@en ;
               
               <http://www.nist.gov/itl/ssd/OntologyRequirements.owl#termString> "malleable iron"@en .



###  http://www.nist.gov/itl/ssd/Materials.owl#ManufacturedGlass

:ManufacturedGlass rdf:type owl:Class ;
                   
                   owl:equivalentClass [ rdf:type owl:Class ;
                                         owl:intersectionOf ( :EngineeredMaterial
                                                              :GlassyMaterial
                                                            )
                                       ] ;
                   
                   rdfs:subClassOf :GlassyMaterial .



###  http://www.nist.gov/itl/ssd/Materials.owl#MartensiticPhaseTransformation

:MartensiticPhaseTransformation rdf:type owl:Class ;
                                
                                rdfs:subClassOf :DeviatonicDominantPhaseTransformation ;
                                
                                owl:disjointWith :QuasimartensiticPhaseTranformation ;
                                
                                daml:seeAlso "http://en.wikipedia.org/w/index.php?title=File:Diffusionless_classification.svg" ;
                                
                                rdfs:comment "Shear dominated transformations can be classified according to the magnitude of the strain energies involved compared to the innate vibrations of the atoms in the lattice and hence whether the strain energies have a notable influence on the kinetics of the transformation and the morphology of the resulting phase. If the strain energy is a significant factor then the transformations are dubbed martensitic and if it is not the transformation is referred to as quasi-martensitic."@en .



###  http://www.nist.gov/itl/ssd/Materials.owl#MassSpectrometer

:MassSpectrometer rdf:type owl:Class ;
                  
                  rdfs:subClassOf :Spectrometer ;
                  
                  rdfs:comment "A Mass Spectrometer is a device used for determining masses of particles, for determining the elemental composition of a sample or molecule, and for elucidating the chemical structures of molecules. Mass spectrometry works by ionizing chemical compounds to generate charged molecules or molecule fragments and measuring their mass-to-charge ratios."@en .



###  http://www.nist.gov/itl/ssd/Materials.owl#MatanoPlane

:MatanoPlane rdf:type owl:Class ;
             
             rdfs:subClassOf <http://www.nist.gov/itl/ssd/OntologyRequirements.owl#PlanarRegion> ;
             
             rdfs:seeAlso "Definitions of terms for diffusion in the solid state (IUPAC Recommendations 1999), Pure Appl. Chem. 71, 1307-1325." ;
             
             <http://www.nist.gov/itl/ssd/OntologyRequirements.owl#termString> "Matano plane"@en ;
             
             rdfs:comment "The Matano plane is the interface through which equal amounts of substance have moved in the positive and negative directions during interdiffusion."@en .



###  http://www.nist.gov/itl/ssd/Materials.owl#MaterialCreep

:MaterialCreep rdf:type owl:Class ;
               
               rdfs:subClassOf :Deformation ;
               
               rdfs:comment "Material Creep is a permanent deformation over time under the influence of stresses."@en .



###  http://www.nist.gov/itl/ssd/Materials.owl#MaterialFatigue

:MaterialFatigue rdf:type owl:Class ;
                 
                 rdfs:subClassOf or:MechanicalProcess ;
                 
                 owl:disjointWith :MicroscopicDiffusionMovement ,
                                  :PhaseChange ,
                                  :TemperatureChangeProcess ,
                                  :ThermalExpansion ;
                 
                 rdfs:comment "Material Fatigue is progressive and localized structural damage that occurs when a material is subjected to cyclic loading."@en .



###  http://www.nist.gov/itl/ssd/Materials.owl#MaterialForm

:MaterialForm rdf:type owl:Class ;
              
              rdfs:subClassOf or:ObjectType ;
              
              rdfs:comment "A Material Form designates a type of material by its form, e.g., Composite Substance, Alloy, Suspension, Pure Substance, Crystaline."@en .



###  http://www.nist.gov/itl/ssd/Materials.owl#MaterialObject

:MaterialObject rdf:type owl:Class ;
                
                owl:equivalentClass [ rdf:type owl:Class ;
                                      owl:intersectionOf ( or:PhysicalObject
                                                           [ rdf:type owl:Class ;
                                                             owl:complementOf :Vacuum
                                                           ]
                                                         )
                                    ] ;
                
                rdfs:subClassOf or:PhysicalObject ;
                
                owl:disjointWith :Vacuum .



###  http://www.nist.gov/itl/ssd/Materials.owl#MaterialPhaseComposition

:MaterialPhaseComposition rdf:type owl:Class ;
                          
                          rdfs:subClassOf or:ObjectType ;
                          
                          rdfs:comment "The class of Material Phases."@en .



###  http://www.nist.gov/itl/ssd/Materials.owl#MaterialPortion

:MaterialPortion rdf:type owl:Class ;
                 
                 rdfs:subClassOf bc:MaterialSubstance ;
                 
                 owl:disjointWith :Vacuum ;
                 
                 rdfs:comment """A 'Material Portion' is part of a heterogeneous portion of a Material Substance that has a certain property.  It is normally diffused throughout an object, but it may be in multiple pieces.  It could be all the grains of one type in a piece of granite, all the zinc in a piece of brass, all the Carbon Dioxide in a room, etc.  

A Material Portion comprises some percentage of the object of which it is a portion by volume and likely a different percentage of the same object by mass (weight).  The Material Portion has different properties than the object as a whole and different properties from other Material Portions of the same Physical Object."""@en .



###  http://www.nist.gov/itl/ssd/Materials.owl#MeanMassFrameOfReference

:MeanMassFrameOfReference rdf:type owl:Class ;
                          
                          rdfs:subClassOf <http://www.nist.gov/itl/ssd/OntologyRequirements.owl#SpatialFrameOfReference> ;
                          
                          rdfs:seeAlso "Definitions of terms for diffusion in the solid state (IUPAC Recommendations 1999), Pure Appl. Chem. 71, 1307-1325." ;
                          
                          rdfs:comment "The mean-mass frame RM moves in such a way that the net flux of mass traversing a plane normal to the diffusion direction is zero everywhere and at all times  The mean-mass reference frame is also known as the barycentric frame of reference."@en ;
                          
                          <http://www.nist.gov/itl/ssd/OntologyRequirements.owl#termString> "barycentric frame of reference"@en ,
                                                                                            "mean-mass frame"@en ,
                                                                                            "mean-mass frame of reference"@en .



###  http://www.nist.gov/itl/ssd/Materials.owl#MeanMolarFrameOfReference

:MeanMolarFrameOfReference rdf:type owl:Class ;
                           
                           rdfs:subClassOf <http://www.nist.gov/itl/ssd/OntologyRequirements.owl#SpatialFrameOfReference> ;
                           
                           rdfs:seeAlso "Definitions of terms for diffusion in the solid state (IUPAC Recommendations 1999), Pure Appl. Chem. 71, 1307-1325." ;
                           
                           rdfs:comment """The mean-molar frame of reference RN moves with respect to the laboratory frame so that the net flux expressed in number of moles of material traversing a plane normal to the diffusion direction is zero
everywhere and at all times  The frame is also called number-fixed frame."""@en ;
                           
                           <http://www.nist.gov/itl/ssd/OntologyRequirements.owl#termString> "mean-molar frame"@en ,
                                                                                             "mean-molar frame of reference"@en ,
                                                                                             "number-fixed frame"@en ,
                                                                                             "number-fixed frame of reference"@en .



###  http://www.nist.gov/itl/ssd/Materials.owl#MeanVolumeFrameOfReference

:MeanVolumeFrameOfReference rdf:type owl:Class ;
                            
                            rdfs:subClassOf <http://www.nist.gov/itl/ssd/OntologyRequirements.owl#SpatialFrameOfReference> ;
                            
                            rdfs:seeAlso "Definitions of terms for diffusion in the solid state (IUPAC Recommendations 1999), Pure Appl. Chem. 71, 1307-1325." ;
                            
                            <http://www.nist.gov/itl/ssd/OntologyRequirements.owl#termString> "Fick’s reference frame"@en ;
                            
                            rdfs:comment "The mean-volume frame RV moves with respect to the laboratory frame R0 so that the net flux expressed in volume of material traversing a plane normal to the diffusion direction is zero everywhere and at all times.  The mean-volume frame is also known as Fick’s reference frame."@en ;
                            
                            <http://www.nist.gov/itl/ssd/OntologyRequirements.owl#termString> "mean-volume frame"@en ,
                                                                                              "mean-volume frame of reference"@en ,
                                                                                              "volume-fixed frame"@en ,
                                                                                              "volume-fixed frame of reference"@en .



###  http://www.nist.gov/itl/ssd/Materials.owl#MeasurableMechanicalProperty

:MeasurableMechanicalProperty rdf:type owl:Class ;
                              
                              owl:equivalentClass [ rdf:type owl:Class ;
                                                    owl:intersectionOf ( :MechanicalProperty
                                                                         or:MeasurableMaterialProperty
                                                                       )
                                                  ] ;
                              
                              rdfs:subClassOf :MechanicalProperty ,
                                              or:MeasurableMaterialProperty ;
                              
                              rdfs:comment "A Measurable Mechanical Property is any Mechanical Property of some physical material or object that has a numeric value with a unit of measure.  This includes properties as mass, melting point, and temperature.  A Mechanical Property is distinguished from a Chemical Property, Electrical Property, or Magnetic Property. "@en .



###  http://www.nist.gov/itl/ssd/Materials.owl#MechanicalProperty

:MechanicalProperty rdf:type owl:Class ;
                    
                    rdfs:subClassOf or:MaterialProperty ;
                    
                    owl:disjointWith :RadiologicalProperty ,
                                     :ThermalProperty ;
                    
                    rdfs:comment "A Mechanical Property is a physical property of some physical material or object, such as mass,concentration, or microstructure.  A Mechanical Property is distinguished from a Chemical Property, Electrical Property, Magnetic Property, or Thermal Property. "@en ;
                    
                    <http://www.w3.org/2004/02/skos/core#note> "Similar to \"Mechanical\" in Ashino's 2010 Minerals Ontology."@en .



###  http://www.nist.gov/itl/ssd/Materials.owl#Melting

:Melting rdf:type owl:Class ;
         
         rdfs:subClassOf :OrderDisorderPhaseTransformation ;
         
         owl:disjointWith :PeritecticDecomposition ,
                          :Sublimating ;
         
         rdfs:comment "Melting is the Phase Change from a solid state to a liquid state."@en .



###  http://www.nist.gov/itl/ssd/Materials.owl#MetalMatrixComposite

:MetalMatrixComposite rdf:type owl:Class ;
                      
                      rdfs:subClassOf :CompositeMaterial ,
                                      :EngineeredMaterial .



###  http://www.nist.gov/itl/ssd/Materials.owl#MetallicMicrostructure

:MetallicMicrostructure rdf:type owl:Class ;
                        
                        rdfs:subClassOf :Microstructure ;
                        
                        owl:disjointWith :PolymericMicrostructure ;
                        
                        rdfs:comment "A Metallic Microstructure is a material Microstructure typical of metals."@en .



###  http://www.nist.gov/itl/ssd/Materials.owl#Methylcellulose

:Methylcellulose rdf:type owl:Class ;
                 
                 rdfs:subClassOf :AlkylCelluloseEthers ;
                 
                 rdfs:comment "Methyl cellulose is produced by heating cellulose with caustic solution and treating it with methyl chloride. In the substitution reaction, the hydroxyl residuesare replaced by methoxide (-OCH3 groups).  Different kinds of methyl cellulose can be prepared depending on the number of hydroxyl groups substituted."@en .



###  http://www.nist.gov/itl/ssd/Materials.owl#Microfracturing

:Microfracturing rdf:type owl:Class ;
                 
                 rdfs:subClassOf :Cracking ,
                                 :MicroscopicMovement ;
                 
                 owl:disjointWith :MicroscopicDiffusionMovement ;
                 
                 rdfs:comment "Microfracturing is Fracturing at a microscopic scale."@en .



###  http://www.nist.gov/itl/ssd/Materials.owl#MicroscopicDiffusionMovement

:MicroscopicDiffusionMovement rdf:type owl:Class ;
                              
                              rdfs:subClassOf :MicroscopicMovement ;
                              
                              owl:disjointWith :PhaseChange ,
                                               :TemperatureChangeProcess ,
                                               :ThermalExpansion ;
                              
                              rdfs:comment "A Microscopic Diffusion Movement is the movement of an atom or crystal vacancy from one site to another as part of a larger process of diffusion."@en .



###  http://www.nist.gov/itl/ssd/Materials.owl#MicroscopicMovement

:MicroscopicMovement rdf:type owl:Class ;
                     
                     rdfs:subClassOf or:MovementEvent ;
                     
                     rdfs:comment "Microscopic Movement is movement on a microscopic scale."@en .



###  http://www.nist.gov/itl/ssd/Materials.owl#Microstructure

:Microstructure rdf:type owl:Class ;
                
                rdfs:subClassOf :MechanicalProperty ;
                
                rdfs:comment "Microstructure is defined as the structure of a material, which can be examined by microscopic examination of a prepared surface or thin foil of the material. The microstructure of a material can be broadly classified as metallic, polymeric, ceramic, or composite."@en .



###  http://www.nist.gov/itl/ssd/Materials.owl#MicrostructureEvolution

:MicrostructureEvolution rdf:type owl:Class ;
                         
                         rdfs:subClassOf <http://www.nist.gov/itl/ssd/OntologyRequirements.owl#PhysicalEvent> ;
                         
                         owl:disjointWith :TemperatureChangeProcess ,
                                          or:PurposefulAction ;
                         
                         rdfs:comment "Microstructural Evolution is the process of change in the Microstructure of materials by any mechanism.  Microsctructrure Evolution may alter a material's the macroscopic properties. This process can be a result of mechanical and thermal loading, chemical transformation, radiation, or by other conditions."@en .



###  http://www.nist.gov/itl/ssd/Materials.owl#MicrostructurePrediction

:MicrostructurePrediction rdf:type owl:Class ;
                          
                          rdfs:subClassOf doc:Prediction ;
                          
                          rdfs:comment "Microstructure Prediction is the prediction of the Microstructure of a material based on its component materials and method of production."@en .



###  http://www.nist.gov/itl/ssd/Materials.owl#Mineral

:Mineral rdf:type owl:Class ;
         
         rdfs:subClassOf :SolidSubstance ;
         
         owl:disjointWith or:Artifact ;
         
         rdfs:comment "A mineral is a naturally occurring non-biological substance that is solid and stable at room temperature, representable by a chemical formula, and has an ordered atomic structure.  Some rocks may be composed of a single mineral, while others are aggregates of minerals or non-minerals, and do not have a specific chemical composition."@en .



###  http://www.nist.gov/itl/ssd/Materials.owl#MineralType

:MineralType rdf:type owl:Class ;
             
             rdfs:subClassOf or:MaterialType ;
             
             rdfs:comment "A Mineral Type is a type of natural occuring mineral."@en .



###  http://www.nist.gov/itl/ssd/Materials.owl#MolecularSimulationModel

:MolecularSimulationModel rdf:type owl:Class ;
                          
                          rdfs:subClassOf or:SimulationModel ;
                          
                          rdfs:comment "Molecular Simulation Model is a model of the behaviour of a molecular system as a function of time."@en .



###  http://www.nist.gov/itl/ssd/Materials.owl#MolybdenumAlloy

:MolybdenumAlloy rdf:type owl:Class ;
                 
                 rdfs:subClassOf :NonFerrousAlloy ,
                                 [ rdf:type owl:Restriction ;
                                   owl:onProperty :physicalDecompositions ;
                                   owl:someValuesFrom bc:Molybdenum
                                 ] ;
                 
                 or:referenceURL "http://www.matweb.com/index.aspx"^^xsd:anyURI ;
                 
                 rdfs:comment "An alloy that contains Molybdenum but not Iron."@en .



###  http://www.nist.gov/itl/ssd/Materials.owl#MonoclinicCrystalStructure

:MonoclinicCrystalStructure rdf:type owl:Class ;
                            
                            rdfs:subClassOf :CrystalLattice ;
                            
                            owl:disjointWith :OrthorhombicCrystalStructure ,
                                             :TetragonalCrystalStructure ,
                                             :TriclinicCrystalStructure ,
                                             :TrigonalCrystalStructure .



###  http://www.nist.gov/itl/ssd/Materials.owl#MultiphaseDiffusion

:MultiphaseDiffusion rdf:type owl:Class ;
                     
                     rdfs:subClassOf :SolidDiffusion ;
                     
                     rdfs:seeAlso "Definitions of terms for diffusion in the solid state (IUPAC Recommendations 1999), Pure Appl. Chem. 71, 1307-1325."@en ;
                     
                     rdfs:comment "Multiphase Diffusion is a diffusion process leading to the formation of a new interface, such as occurs during formation of allotropic structures, new phases, solid solutions, and/or chemical reactions.  Also called ``reaction diffusion''."@en ;
                     
                     <http://www.nist.gov/itl/ssd/OntologyRequirements.owl#termString> "multiphase diffusion"@en ,
                                                                                       "reaction diffusion"@en .



###  http://www.nist.gov/itl/ssd/Materials.owl#MultiphaseMaterialType

:MultiphaseMaterialType rdf:type owl:Class ;
                        
                        rdfs:subClassOf or:MaterialType ;
                        
                        rdfs:comment "A multiphase material consists of more than one material phases, with concentration (which could be specified by volume) for each phase.  The phases could be different states of matter or different Crystal Structures."@en .



###  http://www.nist.gov/itl/ssd/Materials.owl#MultiplyAlkylatedCyclopentane

:MultiplyAlkylatedCyclopentane rdf:type owl:Class ;
                               
                               rdfs:subClassOf :FluidLubricant ;
                               
                               owl:disjointWith :OrganicSoapGellant ,
                                                :PTFEGellant ,
                                                :Perfluoropolyether ,
                                                :Polyalphaolefin ,
                                                :PolyphenyletherBaseLubricant ,
                                                :Quenchant ,
                                                :SiliconeBaseLubricant ,
                                                :SiliconeGellant ,
                                                :SyntheticEtherBase ,
                                                :UreaGellant ,
                                                :WhiteMineralOil ,
                                                :ZincOxideLubricant ;
                               
                               or:referenceURL "http://www.matweb.com/index.aspx"^^xsd:anyURI ;
                               
                               <http://www.nist.gov/itl/ssd/OntologyRequirements.owl#termString> "MAC"@en ,
                                                                                                 "multiply-alkylated cyclopentane"@en .



###  http://www.nist.gov/itl/ssd/Materials.owl#NanoMaterial

:NanoMaterial rdf:type owl:Class ;
              
              rdfs:subClassOf bc:MaterialSubstance ;
              
              rdfs:comment """A nanomaterial (according to the European Commission) is ``a natural, incidental or manufactured material containing particles, in an unbound state or as an aggregate or as an agglomerate and where, for 50% or more of the particles in the number size distribution, one or more external dimensions is in the size range 1 nm – 100 nm. In specific cases and where warranted by concerns for the environment, health, safety or competitiveness the number size distribution threshold of 50% may be replaced by a threshold between 1 and 50%.''
"""@en .



###  http://www.nist.gov/itl/ssd/Materials.owl#NativeMetal

:NativeMetal rdf:type owl:Class ;
             
             rdfs:subClassOf :Mineral ;
             
             rdfs:comment "A Native Metal is a mineral that is a metal that occurs in nature in uncombined form with a distinct mineral structure. This includes elemental metals and inatural ntermetallic alloys."@en .



###  http://www.nist.gov/itl/ssd/Materials.owl#NickelAlloy

:NickelAlloy rdf:type owl:Class ;
             
             rdfs:subClassOf :NonFerrousAlloy ,
                             [ rdf:type owl:Restriction ;
                               owl:onProperty :physicalDecompositions ;
                               owl:someValuesFrom bc:Nickel
                             ] ;
             
             or:referenceURL "http://www.matweb.com/index.aspx"^^xsd:anyURI ;
             
             rdfs:comment "An alloy that contains Nickel but not Iron."@en .



###  http://www.nist.gov/itl/ssd/Materials.owl#NitrateMineral

:NitrateMineral rdf:type owl:Class ;
                
                rdfs:subClassOf :Mineral .



###  http://www.nist.gov/itl/ssd/Materials.owl#NitrideBasedCeramic

:NitrideBasedCeramic rdf:type owl:Class ;
                     
                     rdfs:subClassOf :PnictideCeramic ;
                     
                     owl:disjointWith :PhosphideBasedCeramic ;
                     
                     or:referenceURL "http://www.matweb.com/index.aspx"^^xsd:anyURI ;
                     
                     <http://www.nist.gov/itl/ssd/OntologyRequirements.owl#termString> "nitride"@en ,
                                                                                       "nitride ceramic"@en ,
                                                                                       "nitride-based ceramic"@en .



###  http://www.nist.gov/itl/ssd/Materials.owl#Nitrocellulose

:Nitrocellulose rdf:type owl:Class ;
                
                rdfs:subClassOf :CelluloseEster ;
                
                rdfs:comment "Nitrocellulose is a highly flammable resin compound formed by nitrating cellulose."@en .



###  http://www.nist.gov/itl/ssd/Materials.owl#NonCollinearInterstitialcyMechanism

:NonCollinearInterstitialcyMechanism rdf:type owl:Class ;
                                     
                                     rdfs:subClassOf :InterstitialcyMechanism ;
                                     
                                     rdfs:seeAlso "Definitions of terms for diffusion in the solid state (IUPAC Recommendations 1999), Pure Appl. Chem. 71, 1307-1325."@en ;
                                     
                                     rdfs:comment "The Non-Collinear Interstitialcy Mechanism is an interstitialcy mechanism in which the interstitial atom and the lattice atom which it displaces do not move along the same straight line."@en .



###  http://www.nist.gov/itl/ssd/Materials.owl#NonFerrousAlloy

:NonFerrousAlloy rdf:type owl:Class ;
                 
                 owl:equivalentClass [ rdf:type owl:Class ;
                                       owl:intersectionOf ( :Alloy
                                                            [ rdf:type owl:Class ;
                                                              owl:complementOf [ rdf:type owl:Restriction ;
                                                                                 owl:onProperty :physicalDecompositions ;
                                                                                 owl:someValuesFrom bc:Iron
                                                                               ]
                                                            ]
                                                          )
                                     ] ;
                 
                 rdfs:subClassOf :Alloy ;
                 
                 rdfs:comment "A non-ferrous alloy is one that does not contain iron."@en .



###  http://www.nist.gov/itl/ssd/Materials.owl#NonFerrousAlloyTypeByMainConstituent

:NonFerrousAlloyTypeByMainConstituent rdf:type owl:Class ;
                                      
                                      rdfs:subClassOf :AlloyTypeByMainConstituent .



###  http://www.nist.gov/itl/ssd/Materials.owl#NonIonicOrAqueousLiquidSolution

:NonIonicOrAqueousLiquidSolution rdf:type owl:Class ;
                                 
                                 owl:equivalentClass [ rdf:type owl:Class ;
                                                       owl:intersectionOf ( :LiquidSolution
                                                                            [ rdf:type owl:Class ;
                                                                              owl:complementOf :AqueousSolution
                                                                            ]
                                                                            [ rdf:type owl:Class ;
                                                                              owl:complementOf :IonicLiquid
                                                                            ]
                                                                          )
                                                     ] ;
                                 
                                 rdfs:subClassOf :LiquidSolution .



###  http://www.nist.gov/itl/ssd/Materials.owl#Obsidian

:Obsidian rdf:type owl:Class ;
          
          rdfs:subClassOf :GlassyMaterial ;
          
          owl:disjointWith or:Artifact ;
          
          rdfs:comment "Obsidian is a naturally occuring glass."@en .



###  http://www.nist.gov/itl/ssd/Materials.owl#OpenCellFoam

:OpenCellFoam rdf:type owl:Class ;
              
              rdfs:subClassOf :SolidFoam ;
              
              rdfs:comment "An Open-Cell Foam is a solid foam with few a low proportion of intact bubbles."@en .



###  http://www.nist.gov/itl/ssd/Materials.owl#OpticalGlass

:OpticalGlass rdf:type owl:Class ;
              
              rdfs:subClassOf :ManufacturedGlass ;
              
              or:referenceURL "http://www.matweb.com/index.aspx"^^xsd:anyURI ;
              
              rdfs:comment "Optical Glass is a glass that is formulated very precisely so that its optical properties are known, and is manufactured to ensure that it is free of impurities and variability."@en ;
              
              <http://www.nist.gov/itl/ssd/OntologyRequirements.owl#termString> "optical glass"@en .



###  http://www.nist.gov/itl/ssd/Materials.owl#OpticalProperty

:OpticalProperty rdf:type owl:Class ;
                 
                 rdfs:subClassOf or:MeasurableMaterialProperty ;
                 
                 owl:disjointWith :RadiologicalProperty ,
                                  :ThermalProperty .



###  http://www.nist.gov/itl/ssd/Materials.owl#OrderDisorderPhaseTransformation

:OrderDisorderPhaseTransformation rdf:type owl:Class ;
                                  
                                  rdfs:subClassOf :PhaseChange ;
                                  
                                  owl:disjointWith :PrecipitationFromSolution ,
                                                   :SolidToSolidPhaseTransformation ,
                                                   :Solidification ;
                                  
                                  rdfs:comment "An Order-Disorder Phase Transformation is one in which the phase changes from an ordered phase to a disordered one."@en .



###  http://www.nist.gov/itl/ssd/Materials.owl#OrderedBCCPhase

:OrderedBCCPhase rdf:type owl:Class ;
                 
                 rdfs:subClassOf :BodyCenteredCubicCrystalStructure .



###  http://www.nist.gov/itl/ssd/Materials.owl#OrderedFCCPhase

:OrderedFCCPhase rdf:type owl:Class ;
                 
                 rdfs:subClassOf :FaceCenteredCubicCrystalStructure .



###  http://www.nist.gov/itl/ssd/Materials.owl#OrderedHCPPhase

:OrderedHCPPhase rdf:type owl:Class ;
                 
                 rdfs:subClassOf :HexagonalClosePackedCrystalStructure .



###  http://www.nist.gov/itl/ssd/Materials.owl#OrderedSolidSolution

:OrderedSolidSolution rdf:type owl:Class ;
                      
                      rdfs:subClassOf :MaterialPhaseComposition .



###  http://www.nist.gov/itl/ssd/Materials.owl#OrganicMineral

:OrganicMineral rdf:type owl:Class ;
                
                rdfs:subClassOf :Mineral .



###  http://www.nist.gov/itl/ssd/Materials.owl#OrganicSoapGellant

:OrganicSoapGellant rdf:type owl:Class ;
                    
                    rdfs:subClassOf :FluidLubricant ;
                    
                    owl:disjointWith :PTFEGellant ,
                                     :Perfluoropolyether ,
                                     :Polyalphaolefin ,
                                     :Polyglycol ,
                                     :PolyphenyletherBaseLubricant ,
                                     :Quenchant ,
                                     :SiliconeBaseLubricant ,
                                     :SiliconeGellant ,
                                     :SyntheticEtherBase ,
                                     :UreaGellant ,
                                     :WhiteMineralOil ,
                                     :ZincOxideLubricant ;
                    
                    or:referenceURL "http://www.matweb.com/index.aspx"^^xsd:anyURI ;
                    
                    <http://www.nist.gov/itl/ssd/OntologyRequirements.owl#termString> "organic soap gellant"@en .



###  http://www.nist.gov/itl/ssd/Materials.owl#OrthorhombicCrystalStructure

:OrthorhombicCrystalStructure rdf:type owl:Class ;
                              
                              rdfs:subClassOf :CrystalLattice ;
                              
                              owl:disjointWith :TetragonalCrystalStructure ,
                                               :TriclinicCrystalStructure ,
                                               :TrigonalCrystalStructure .



###  http://www.nist.gov/itl/ssd/Materials.owl#OxideBasedCeramic

:OxideBasedCeramic rdf:type owl:Class ;
                   
                   rdfs:subClassOf :Ceramic ;
                   
                   owl:disjointWith :PnictideCeramic ;
                   
                   or:referenceURL "http://www.matweb.com/index.aspx"^^xsd:anyURI ;
                   
                   <http://www.nist.gov/itl/ssd/OntologyRequirements.owl#termString> "ceramic  oxide"@en ,
                                                                                     "oxide"@en .



###  http://www.nist.gov/itl/ssd/Materials.owl#OxideMineral

:OxideMineral rdf:type owl:Class ;
              
              rdfs:subClassOf :Mineral .



###  http://www.nist.gov/itl/ssd/Materials.owl#PTFEGellant

:PTFEGellant rdf:type owl:Class ;
             
             rdfs:subClassOf :FluidLubricant ;
             
             owl:disjointWith :Perfluoropolyether ,
                              :Polyalphaolefin ,
                              :Polyglycol ,
                              :PolyphenyletherBaseLubricant ,
                              :Quenchant ,
                              :SiliconeBaseLubricant ,
                              :SiliconeGellant ,
                              :SyntheticEtherBase ,
                              :UreaGellant ,
                              :WhiteMineralOil ,
                              :ZincOxideLubricant ;
             
             or:referenceURL "http://www.matweb.com/index.aspx"^^xsd:anyURI ;
             
             <http://www.nist.gov/itl/ssd/OntologyRequirements.owl#termString> "PTFE gellant"@en ,
                                                                               "polytetrafluoroethylene gellant"@en .



###  http://www.nist.gov/itl/ssd/Materials.owl#PasteSubstance

:PasteSubstance rdf:type owl:Class ;
                
                rdfs:subClassOf :ChemicalSuspension ;
                
                owl:disjointWith :PowderySubstance ;
                
                rdfs:comment "A Paste is a substance that behaves as a solid until a sufficiently large load or stress is applied, at which point it flows like a fluid.  Pastes typically consist of a suspension of granular material in a background fluid.  Pastes are distinct from gels, whose particles interconnect."@en .



###  http://www.nist.gov/itl/ssd/Materials.owl#Perfluoropolyether

:Perfluoropolyether rdf:type owl:Class ;
                    
                    rdfs:subClassOf :FluidLubricant ;
                    
                    owl:disjointWith :Polyalphaolefin ,
                                     :Polyglycol ,
                                     :PolyphenyletherBaseLubricant ,
                                     :Quenchant ,
                                     :SiliconeBaseLubricant ,
                                     :SiliconeGellant ,
                                     :SyntheticEtherBase ,
                                     :UreaGellant ,
                                     :WhiteMineralOil ,
                                     :ZincOxideLubricant ;
                    
                    or:referenceURL "http://www.matweb.com/index.aspx"^^xsd:anyURI ;
                    
                    <http://www.nist.gov/itl/ssd/OntologyRequirements.owl#termString> "PFPE"@en ,
                                                                                      "perfluoropolyether"@en .



###  http://www.nist.gov/itl/ssd/Materials.owl#PeritecticAlloy

:PeritecticAlloy rdf:type owl:Class ;
                 
                 rdfs:subClassOf :EngineeredAlloy ;
                 
                 rdfs:comment "A Peritectic Alloy is an alloy that has a specific ratio of component metals that solidifies (through a Pertectic Reaction) from a mixture of liquid and solid of a different crystalline structure."@en .



###  http://www.nist.gov/itl/ssd/Materials.owl#PeritecticDecomposition

:PeritecticDecomposition rdf:type owl:Class ;
                         
                         rdfs:subClassOf :OrderDisorderPhaseTransformation ;
                         
                         owl:disjointWith :Vaporization ;
                         
                         rdfs:comment "In Peritectic Decomposition a solid compound decomposes into another solid compound and a liquid."@en .



###  http://www.nist.gov/itl/ssd/Materials.owl#PeritecticReaction

:PeritecticReaction rdf:type owl:Class ;
                    
                    rdfs:subClassOf :Solidification ;
                    
                    owl:disjointWith :SublimatingToSolid ;
                    
                    rdfs:comment "A Peritectic Reaction is a Phase Change of a mixture of liquid and solid of a one crystalline structure solidifying into a solid with a different crystalline structure and a fixed ratio of constituant metals.  The resulting solid is a PeritecticAlloy."@en .



###  http://www.nist.gov/itl/ssd/Materials.owl#PermanentMagnet

:PermanentMagnet rdf:type owl:Class ;
                 
                 rdfs:subClassOf :Ceramic ;
                 
                 owl:disjointWith :Piezoceramic .



###  http://www.nist.gov/itl/ssd/Materials.owl#PhaseChange

:PhaseChange rdf:type owl:Class ;
             
             rdfs:subClassOf or:MechanicalProcess ;
             
             owl:disjointWith :ThermalExpansion ;
             
             rdfs:comment "A Phase Change or phase transformation is a change in the Material Phase of an object."@en .



###  http://www.nist.gov/itl/ssd/Materials.owl#PhosphateMineral

:PhosphateMineral rdf:type owl:Class ;
                  
                  rdfs:subClassOf :Mineral .



###  http://www.nist.gov/itl/ssd/Materials.owl#PhosphideBasedCeramic

:PhosphideBasedCeramic rdf:type owl:Class ;
                       
                       rdfs:subClassOf :PnictideCeramic ;
                       
                       or:referenceURL "http://www.matweb.com/index.aspx"^^xsd:anyURI ;
                       
                       <http://www.nist.gov/itl/ssd/OntologyRequirements.owl#termString> "phosphide"@en ,
                                                                                         "phosphide ceramic"@en ,
                                                                                         "phosphide-based ceramic"@en .



###  http://www.nist.gov/itl/ssd/Materials.owl#PhysicalMixture

:PhysicalMixture rdf:type owl:Class ;
                 
                 rdfs:subClassOf bc:MaterialSubstance ;
                 
                 owl:disjointWith :PureSubstance ,
                                  :Vacuum ;
                 
                 rdfs:comment "A Physical Mixture is a material made up by two or more different substances which are mixed but are not combined chemically.  In the physical combination, the identities of the constituant substances are retained.  Types of mixture include alloys, solutions, suspensions, and colloids."@en .



###  http://www.nist.gov/itl/ssd/Materials.owl#Piezoceramic

:Piezoceramic rdf:type owl:Class ;
              
              rdfs:subClassOf :Ceramic ,
                              :EngineeredMaterial ;
              
              or:referenceURL "http://www.matweb.com/index.aspx"^^xsd:anyURI ;
              
              rdfs:comment "piezoceramic"@en ,
                           "piezoceramic material"@en ,
                           "piezoelectric ceramic"@en .



###  http://www.nist.gov/itl/ssd/Materials.owl#PipeDiffusion

:PipeDiffusion rdf:type owl:Class ;
               
               rdfs:subClassOf :ShortCircuitDiffusion ;
               
               rdfs:seeAlso "Definitions of terms for diffusion in the solid state (IUPAC Recommendations 1999), Pure Appl. Chem. 71, 1307-1325."@en ;
               
               rdfs:comment "Pipe Diffusion is diffusion which takes place along a dislocation line."@en .



###  http://www.nist.gov/itl/ssd/Materials.owl#Plywood

:Plywood rdf:type owl:Class ;
         
         rdfs:subClassOf :SandwichComposite ,
                         :Wood ;
         
         rdfs:comment "Plywood is a manufactured wood panel Sadwich Composite of thin sheets of Wood."@en .



###  http://www.nist.gov/itl/ssd/Materials.owl#PnictideCeramic

:PnictideCeramic rdf:type owl:Class ;
                 
                 rdfs:subClassOf :Ceramic ;
                 
                 or:referenceURL "http://www.matweb.com/index.aspx"^^xsd:anyURI ;
                 
                 rdfs:comment "The pnictogens are the chemical elements in group 15 ( VB or VA) of the periodic table. This group is also known as the nitrogen family. It consists of the elements nitrogen (N), phosphorus (P), arsenic (As), antimony (Sb), bismuth (Bi).  Pnictides are binary compounds formed from this chemical group."@en ;
                 
                 <http://www.nist.gov/itl/ssd/OntologyRequirements.owl#termString> "pnictide"@en ,
                                                                                   "pnictide ceramic"@en .



###  http://www.nist.gov/itl/ssd/Materials.owl#Polyacrylate

:Polyacrylate rdf:type owl:Class ;
              
              rdfs:subClassOf :Thermoplastic ;
              
              rdfs:comment "Polyacrylates (`acrylate polymers' or `acrylics') are polymers  polymers are based on the structure of acrylic acid, which consists of a vinyl group and a carboxylic acid terminus."@en .



###  http://www.nist.gov/itl/ssd/Materials.owl#Polyacrylonitrile

:Polyacrylonitrile rdf:type owl:Class ;
                   
                   rdfs:subClassOf :VinylPolymer ;
                   
                   owl:disjointWith :Polybutadiene ,
                                    :Polyethylene ,
                                    :Polypropylene ,
                                    :Polystyrene ,
                                    :PolyvinylAcetate ,
                                    :PolyvinylAlcohol ,
                                    :PolyvinylChloride ;
                   
                   rdfs:comment "Polyacrylonitrile is made by polymerization of the monomer acrylonitrile."@en .



###  http://www.nist.gov/itl/ssd/Materials.owl#Polyalphaolefin

:Polyalphaolefin rdf:type owl:Class ;
                 
                 rdfs:subClassOf :FluidLubricant ;
                 
                 owl:disjointWith :Polyglycol ,
                                  :PolyphenyletherBaseLubricant ,
                                  :Quenchant ,
                                  :SiliconeBaseLubricant ,
                                  :SiliconeGellant ,
                                  :SyntheticEtherBase ,
                                  :UreaGellant ,
                                  :WhiteMineralOil ,
                                  :ZincOxideLubricant ;
                 
                 or:referenceURL "http://www.matweb.com/index.aspx"^^xsd:anyURI ;
                 
                 <http://www.nist.gov/itl/ssd/OntologyRequirements.owl#termString> "PAO"@en ,
                                                                                   "polyalphaolefin"@en .



###  http://www.nist.gov/itl/ssd/Materials.owl#Polybutadiene

:Polybutadiene rdf:type owl:Class ;
               
               rdfs:subClassOf :VinylPolymer ;
               
               owl:disjointWith :Polyethylene ,
                                :Polypropylene ,
                                :Polystyrene ,
                                :PolyvinylAcetate ,
                                :PolyvinylAlcohol ,
                                :PolyvinylChloride ;
               
               rdfs:comment "Polybutadiene is a synthetic rubber that is a polymer formed from the polymerization process of the monomer 1,3-butadiene."@en .



###  http://www.nist.gov/itl/ssd/Materials.owl#Polybutylene

:Polybutylene rdf:type owl:Class ;
              
              rdfs:subClassOf :Polyolefin ;
              
              owl:disjointWith :Polymethylpentene ,
                               :VinylPolymer ;
              
              rdfs:comment "Polybutylene (polybutene-1, poly(1-butene), PB-1) is a polyolefin or saturated polymer with the chemical formula (C4H8)n"@en .



###  http://www.nist.gov/itl/ssd/Materials.owl#PolycrystallineMaterial

:PolycrystallineMaterial rdf:type owl:Class ;
                         
                         rdfs:subClassOf :SolidCrystallineSubstance ;
                         
                         owl:disjointWith :SingleCrystallineMaterial ;
                         
                         rdfs:comment "Polycrystalline material is solid material made up of multiple crystals."@en .



###  http://www.nist.gov/itl/ssd/Materials.owl#Polyester

:Polyester rdf:type owl:Class ;
           
           rdfs:subClassOf :PolymerSubstance ;
           
           owl:disjointWith :Polyolefin ,
                            :VinylPolymer ;
           
           rdfs:comment """Polyester is a category of polymers which contain the ester functional group in their main chain. Although there are many polyesters, the term \"polyester\" as a specific material most commonly refers to polyethylene terephthalate (PET). Polyesters include naturally occurring chemicals, such as in the cutin of plant cuticles, as well as synthetics through step-growth polymerization such as polycarbonate and polybutyrate. Natural polyesters and a few synthetic ones are biodegradable, but most synthetic polyesters are not.

Depending on the chemical structure, polyester can be a thermoplastic or thermoset; however, the most common polyesters are thermoplastics."""@en ;
           
           <http://www.nist.gov/itl/ssd/OntologyRequirements.owl#termString> "polyester"@en .



###  http://www.nist.gov/itl/ssd/Materials.owl#Polyester-TP

:Polyester-TP rdf:type owl:Class ;
              
              rdfs:subClassOf :Polyester ,
                              :Thermoplastic ;
              
              or:referenceURL "http://www.matweb.com/index.aspx"^^xsd:anyURI ;
              
              <http://www.nist.gov/itl/ssd/OntologyRequirements.owl#termString> "polyester, TP"@en ,
                                                                                "thermoplastic polyester"@en .



###  http://www.nist.gov/itl/ssd/Materials.owl#Polyester-TS

:Polyester-TS rdf:type owl:Class ;
              
              rdfs:subClassOf :Polyester ,
                              :Thermoset ;
              
              or:referenceURL "http://www.matweb.com/index.aspx"^^xsd:anyURI ;
              
              <http://www.nist.gov/itl/ssd/OntologyRequirements.owl#termString> "polyester, TS"@en ,
                                                                                "thermosetting polyester"@en .



###  http://www.nist.gov/itl/ssd/Materials.owl#Polyethylene

:Polyethylene rdf:type owl:Class ;
              
              rdfs:subClassOf :Polyolefin ,
                              :VinylPolymer ;
              
              owl:disjointWith :Polypropylene ,
                               :Polystyrene ,
                               :PolyvinylAcetate ,
                               :PolyvinylAlcohol ,
                               :PolyvinylChloride ;
              
              or:referenceURL ""^^xsd:anyURI ;
              
              rdfs:comment "Polyethylene (abbreviated PE) or polythene (IUPAC name polyethene or poly(methylene)) is  made by polymerization of ethene. Many kinds of polyethylene are known, but they almost always have the chemical formula (C2H4)nH2."@en .



###  http://www.nist.gov/itl/ssd/Materials.owl#Polyglycol

:Polyglycol rdf:type owl:Class ;
            
            rdfs:subClassOf :FluidLubricant ;
            
            owl:disjointWith :PolyphenyletherBaseLubricant ,
                             :Quenchant ,
                             :SiliconeBaseLubricant ,
                             :SiliconeGellant ,
                             :SyntheticEtherBase ,
                             :UreaGellant ,
                             :WhiteMineralOil ,
                             :ZincOxideLubricant ;
            
            or:referenceURL "http://www.matweb.com/index.aspx"^^xsd:anyURI ;
            
            <http://www.nist.gov/itl/ssd/OntologyRequirements.owl#termString> "polyglycol"@en .



###  http://www.nist.gov/itl/ssd/Materials.owl#PolymerMetalInteraction

:PolymerMetalInteraction rdf:type owl:Class ;
                         
                         rdfs:subClassOf <http://www.nist.gov/itl/ssd/Biochem.owl#ChemicalProcess> ,
                                         [ rdf:type owl:Restriction ;
                                           owl:onProperty or:objectActedOn ;
                                           owl:someValuesFrom bc:Metal
                                         ] ,
                                         [ rdf:type owl:Restriction ;
                                           owl:onProperty or:objectActedOn ;
                                           owl:someValuesFrom :PolymerSubstance
                                         ] ;
                         
                         rdfs:comment "A Polymer-Metal Interaction is a Chemical Process in which a Polymer and metallic particles interact."@en .



###  http://www.nist.gov/itl/ssd/Materials.owl#PolymerSubstance

:PolymerSubstance rdf:type owl:Class ;
                  
                  rdfs:subClassOf bc:MaterialSubstance .



###  http://www.nist.gov/itl/ssd/Materials.owl#PolymericMicrostructure

:PolymericMicrostructure rdf:type owl:Class ;
                         
                         rdfs:subClassOf :Microstructure ;
                         
                         rdfs:comment "Polymeric Microstructure is a non-crystalline material Microstructure of a substance composed of polymers."@en .



###  http://www.nist.gov/itl/ssd/Materials.owl#Polymethylpentene

:Polymethylpentene rdf:type owl:Class ;
                   
                   rdfs:subClassOf :Polyolefin ;
                   
                   owl:disjointWith :VinylPolymer ;
                   
                   or:referenceURL "http://www.matweb.com/index.aspx"^^xsd:anyURI ;
                   
                   rdfs:comment "Polymethylpentene (PMP) is a thermoplastic polymer of methylpentene monomer units."@en .



###  http://www.nist.gov/itl/ssd/Materials.owl#Polyolefin

:Polyolefin rdf:type owl:Class ;
            
            rdfs:subClassOf :Thermoplastic ;
            
            or:referenceURL "http://www.matweb.com/index.aspx"^^xsd:anyURI ;
            
            rdfs:comment "A polyolefin (or polyalkene) is a polymer produced from a simple olefin (or ``alkene'' with the general formula CnH2n) as a monomer."@en .



###  http://www.nist.gov/itl/ssd/Materials.owl#PolyphenyletherBaseLubricant

:PolyphenyletherBaseLubricant rdf:type owl:Class ;
                              
                              rdfs:subClassOf :FluidLubricant ;
                              
                              owl:disjointWith :Quenchant ,
                                               :SiliconeBaseLubricant ,
                                               :SiliconeGellant ,
                                               :SyntheticEtherBase ,
                                               :UreaGellant ,
                                               :WhiteMineralOil ,
                                               :ZincOxideLubricant ;
                              
                              or:referenceURL "http://www.matweb.com/index.aspx"^^xsd:anyURI ;
                              
                              <http://www.nist.gov/itl/ssd/OntologyRequirements.owl#termString> "PPE base"@en ,
                                                                                                "PPE base lubricant"@en ,
                                                                                                "polyphenylether base"@en ,
                                                                                                "polyphenylether base lubricant"@en .



###  http://www.nist.gov/itl/ssd/Materials.owl#Polypropylene

:Polypropylene rdf:type owl:Class ;
               
               rdfs:subClassOf :Polyolefin ,
                               :VinylPolymer ;
               
               owl:disjointWith :Polystyrene ,
                                :PolyvinylAcetate ,
                                :PolyvinylAlcohol ,
                                :PolyvinylChloride ;
               
               or:referenceURL "http://www.matweb.com/index.aspx"^^xsd:anyURI ;
               
               <http://www.nist.gov/itl/ssd/OntologyRequirements.owl#termString> "PP"@en ;
               
               rdfs:comment "Polypropylene (PP), also known as polypropene, is a thermoplastic polymer from the monomer propylene."@en ;
               
               <http://www.nist.gov/itl/ssd/OntologyRequirements.owl#termString> "polypropylene"@en .



###  http://www.nist.gov/itl/ssd/Materials.owl#Polystyrene

:Polystyrene rdf:type owl:Class ;
             
             rdfs:subClassOf :VinylPolymer ;
             
             owl:disjointWith :PolyvinylAcetate ,
                              :PolyvinylAlcohol ,
                              :PolyvinylChloride ;
             
             or:referenceURL "http://www.matweb.com/index.aspx"^^xsd:anyURI ;
             
             <http://www.nist.gov/itl/ssd/OntologyRequirements.owl#termString> "PS"@en ;
             
             rdfs:comment "Polystyrene is made from styrene or 'vinyl benzene'."@en ;
             
             <http://www.nist.gov/itl/ssd/OntologyRequirements.owl#termString> "polystyrene"@en .



###  http://www.nist.gov/itl/ssd/Materials.owl#PolyvinylAcetate

:PolyvinylAcetate rdf:type owl:Class ;
                  
                  rdfs:subClassOf :VinylPolymer ;
                  
                  owl:disjointWith :PolyvinylAlcohol ,
                                   :PolyvinylChloride ;
                  
                  rdfs:comment "Polyvinyl acetate (PVAc) is made by polymerization of vinyl acetate."@en .



###  http://www.nist.gov/itl/ssd/Materials.owl#PolyvinylAlcohol

:PolyvinylAlcohol rdf:type owl:Class ;
                  
                  rdfs:subClassOf :VinylPolymer ;
                  
                  owl:disjointWith :PolyvinylChloride ;
                  
                  rdfs:comment "Polyvinyl alcohol (PVA) is produced by hydrolysis of polyvinyl acetate."@en .



###  http://www.nist.gov/itl/ssd/Materials.owl#PolyvinylChloride

:PolyvinylChloride rdf:type owl:Class ;
                   
                   rdfs:subClassOf :VinylPolymer ;
                   
                   or:referenceURL "http://www.matweb.com/index.aspx"^^xsd:anyURI ;
                   
                   <http://www.nist.gov/itl/ssd/OntologyRequirements.owl#termString> "PVC"@en ;
                   
                   rdfs:comment "Polyvinyl chloride (PVC) is made by polymerization of the monomer vinyl chloride (chloroethene) CH2=CHCl"@en ;
                   
                   <http://www.nist.gov/itl/ssd/OntologyRequirements.owl#termString> "polyvynl chloride"@en ,
                                                                                     "vinyl"@en .



###  http://www.nist.gov/itl/ssd/Materials.owl#PowderySubstance

:PowderySubstance rdf:type owl:Class ;
                  
                  rdfs:subClassOf :SolidSubstance ;
                  
                  rdfs:comment "material in a solid powdery phase"@en .



###  http://www.nist.gov/itl/ssd/Materials.owl#Power

:Power rdf:type owl:Class ;
       
       owl:equivalentClass [ rdf:type owl:Class ;
                             owl:intersectionOf ( or:MeasurableQuantity
                                                  [ rdf:type owl:Restriction ;
                                                    owl:onProperty or:unitsFor ;
                                                    owl:someValuesFrom :UnitOfPower
                                                  ]
                                                )
                           ] ;
       
       rdfs:subClassOf or:MeasurableQuantity ,
                       [ rdf:type owl:Restriction ;
                         owl:onProperty or:unitsFor ;
                         owl:allValuesFrom :UnitOfPower
                       ] .



###  http://www.nist.gov/itl/ssd/Materials.owl#PrecipitationFromSolution

:PrecipitationFromSolution rdf:type owl:Class ;
                           
                           rdfs:subClassOf :DiffusionalPhaseTransformation ;
                           
                           owl:disjointWith :SolidToSolidPhaseTransformation ,
                                            :Solidification ,
                                            :Vaporization .



###  http://www.nist.gov/itl/ssd/Materials.owl#PureSubstance

:PureSubstance rdf:type owl:Class ;
               
               rdfs:subClassOf bc:ChemicalSubstance ;
               
               rdfs:comment "A Pure Substance is a substance made up of a single form of molecule, or in the case of a metal, a single type of atom.  This does not not mean that there may not be impurities."@en .



###  http://www.nist.gov/itl/ssd/Materials.owl#Quartz

:Quartz rdf:type owl:Class ;
        
        rdfs:subClassOf :Silicate ;
        
        rdfs:comment "Quartz is a common mineral of SiO4 with a hexagonal crystalline structure.  Impurities may color this otherwise colorless mineral."@en .



###  http://www.nist.gov/itl/ssd/Materials.owl#QuasimartensiticPhaseTranformation

:QuasimartensiticPhaseTranformation rdf:type owl:Class ;
                                    
                                    rdfs:subClassOf :DeviatonicDominantPhaseTransformation ;
                                    
                                    rdfs:comment "Shear dominated transformations can be classified according to the magnitude of the strain energies involved compared to the innate vibrations of the atoms in the lattice and hence whether the strain energies have a notable influence on the kinetics of the transformation and the morphology of the resulting phase. If the strain energy is a significant factor then the transformations are dubbed martensitic and if it is not the transformation is referred to as quasi-martensitic."@en .



###  http://www.nist.gov/itl/ssd/Materials.owl#Quenchant

:Quenchant rdf:type owl:Class ;
           
           rdfs:subClassOf :FluidLubricant ;
           
           owl:disjointWith :SiliconeBaseLubricant ,
                            :SiliconeGellant ,
                            :SyntheticEtherBase ,
                            :UreaGellant ,
                            :WhiteMineralOil ,
                            :ZincOxideLubricant ;
           
           or:referenceURL "http://www.matweb.com/index.aspx"^^xsd:anyURI ;
           
           <http://www.nist.gov/itl/ssd/OntologyRequirements.owl#termString> "quenchant"@en .



###  http://www.nist.gov/itl/ssd/Materials.owl#RadioactiveMaterial

:RadioactiveMaterial rdf:type owl:Class ;
                     
                     rdfs:subClassOf bc:MaterialSubstance ;
                     
                     owl:disjointWith :Vacuum ;
                     
                     rdfs:comment "The class of all material that is radioactive."@en .



###  http://www.nist.gov/itl/ssd/Materials.owl#Radioisotope

:Radioisotope rdf:type owl:Class ;
              
              rdfs:subClassOf bc:Isotope ;
              
              owl:disjointWith :StableIsotope ;
              
              rdfs:comment "A Radioisotope is an Isotope that is a subclass of Radioactive Material."@en .



###  http://www.nist.gov/itl/ssd/Materials.owl#RadiologicalProperty

:RadiologicalProperty rdf:type owl:Class ;
                      
                      rdfs:subClassOf or:MeasurableMaterialProperty ;
                      
                      owl:disjointWith :ThermalProperty .



###  http://www.nist.gov/itl/ssd/Materials.owl#ReinforcedPlastic

:ReinforcedPlastic rdf:type owl:Class ;
                   
                   rdfs:subClassOf :CompositeMaterial ,
                                   :EngineeredMaterial ,
                                   :PolymerSubstance ;
                   
                   rdfs:comment "A Fibre-reinforced plastic (FRP) (also fibre-reinforced polymer) is a composite material made of a polymer matrix reinforced with fibres. The fibres may be glass, carbon, aramid, paper, wood, or asbestos. The polymer may be an epoxy, vinylester, polyester thermosetting plastic, or phenol formaldehyde resin."@en .



###  http://www.nist.gov/itl/ssd/Materials.owl#RelaxationMethodForDiffusion

:RelaxationMethodForDiffusion rdf:type owl:Class ;
                              
                              rdfs:subClassOf :VacancyDiffusionMechanism ;
                              
                              rdfs:seeAlso "Definitions of terms for diffusion in the solid state (IUPAC Recommendations 1999), Pure Appl. Chem. 71, 1307-1325."@en ;
                              
                              rdfs:comment "In the Relaxation Mechanism for diffusion, the atoms close to a vacancy relax to such an extent that the regular lattice structure out to several atom distances disappears and diffusion occurs by an irregular jostling motion similar to that for atoms in a liquid."@en .



###  http://www.nist.gov/itl/ssd/Materials.owl#ReneAlloy

:ReneAlloy rdf:type owl:Class ;
           
           rdfs:subClassOf :NickelAlloy ,
                           :Superalloy ;
           
           rdfs:comment " Rene Alloys are Superalloys developed by General Electric."@en .



###  http://www.nist.gov/itl/ssd/Materials.owl#RheologicalProperty

:RheologicalProperty rdf:type owl:Class ;
                     
                     rdfs:subClassOf :MeasurableMechanicalProperty ;
                     
                     rdfs:comment "Rheological Properties are the quantitative and qualitative relationships between deformations and stresses of a material.  Such properties include shear stress, viscosity, linear viscoelastic properties, and elongational properties."@en .



###  http://www.nist.gov/itl/ssd/Materials.owl#RhombohedralCrystalStructure

:RhombohedralCrystalStructure rdf:type owl:Class ;
                              
                              rdfs:subClassOf :TrigonalCrystalStructure ;
                              
                              rdfs:comment """A lattice system is described by three basis vectors. In the rhombohedral system, the crystal is described by vectors of equal length, no two of which are orthogonal. The rhombohedral system can be thought of as the cubic system stretched along a body diagonal. a = b = c; α = β = γ ≠ 90°. In some classification schemes, the rhombohedral lattice system is combined with the hexagonal lattice system and grouped into a larger hexagonal family.

There is only one rhombohedral Bravais lattice."""@en .



###  http://www.nist.gov/itl/ssd/Materials.owl#RingMechanismForDiffusion

:RingMechanismForDiffusion rdf:type owl:Class ;
                           
                           rdfs:subClassOf :MicroscopicDiffusionMovement ;
                           
                           rdfs:comment "The Ring Mechanism for Diffusion is a variation of the exchange mechanism in which a group of atoms moves around in a circular fashion, each atom in the group taking the place of its neighbour in the direction of motion."@en ;
                           
                           <http://www.nist.gov/itl/ssd/OntologyRequirements.owl#termString> "ring mechanism"@en ,
                                                                                             "ring mechanism for diffusion"@en .



###  http://www.nist.gov/itl/ssd/Materials.owl#SandwichComposite

:SandwichComposite rdf:type owl:Class ;
                   
                   rdfs:subClassOf :CompositeMaterial ,
                                   :EngineeredMaterial .



###  http://www.nist.gov/itl/ssd/Materials.owl#ScratchHardness

:ScratchHardness rdf:type owl:Class ;
                 
                 rdfs:subClassOf :Hardness ;
                 
                 rdfs:comment "Scratch hardness is the measure of how resistant a sample is to fracture or permanent plastic deformation due to friction from a sharp object."@en .



###  http://www.nist.gov/itl/ssd/Materials.owl#SelfDiffusion

:SelfDiffusion rdf:type owl:Class ;
               
               rdfs:subClassOf :SolidDiffusion ;
               
               rdfs:seeAlso "Definitions of terms for diffusion in the solid state (IUPAC Recommendations 1999), Pure Appl. Chem. 71, 1307-1325."@en ;
               
               rdfs:comment "Self-diffusion is diffusion which takes place in the absence of a chemical potential gradient, describing the uncorrelated movement of a particle."@en ;
               
               <http://www.nist.gov/itl/ssd/OntologyRequirements.owl#termString> "self-diffusion"@en .



###  http://www.nist.gov/itl/ssd/Materials.owl#Semiconductor

:Semiconductor rdf:type owl:Class ;
               
               rdfs:subClassOf bc:MaterialSubstance ;
               
               rdfs:comment "A semiconductor has electrical conductivity intermediate between that of a conductor and an insulator.  Semiconductors differ from metals in their characteristic property of decreasing electrical resistivity with increasing temperature.  Common semiconducting materials are crystalline solids, but amorphous and liquid semiconductors are also known"@en .



###  http://www.nist.gov/itl/ssd/Materials.owl#ShortCircuitDiffusion

:ShortCircuitDiffusion rdf:type owl:Class ;
                       
                       rdfs:subClassOf :SolidDiffusion ;
                       
                       rdfs:seeAlso "Definitions of terms for diffusion in the solid state (IUPAC Recommendations 1999), Pure Appl. Chem. 71, 1307-1325."@en ;
                       
                       rdfs:comment "Short Circuit Diffusion is a diffusion process occurring via grain boundaries, surfaces, or dislocations.  Short circuit diffusion mechanisms often cause diffusion in polycrystalline materials to proceed more quickly than in single crystals."@en .



###  http://www.nist.gov/itl/ssd/Materials.owl#ShufflePhaseTransformation

:ShufflePhaseTransformation rdf:type owl:Class ;
                            
                            rdfs:subClassOf :DiffusionlessPhaseTransformation ;
                            
                            rdfs:comment "Shuffle transformations involve the small movement of atoms within the unit cell. As a result pure shuffles do not normally result in a shape change of the unit cell - only its symmetry and structure."@en .



###  http://www.nist.gov/itl/ssd/Materials.owl#Silicate

:Silicate rdf:type owl:Class ;
          
          rdfs:subClassOf :Mineral .



###  http://www.nist.gov/itl/ssd/Materials.owl#SiliconOxide

:SiliconOxide rdf:type owl:Class ;
              
              rdfs:subClassOf bc:Oxide ;
              
              owl:disjointWith :TitaniumOxide ,
                               :ZirconiumOxide ;
              
              or:referenceURL "http://www.matweb.com/index.aspx"^^xsd:anyURI ;
              
              <http://www.nist.gov/itl/ssd/OntologyRequirements.owl#termString> "silicon oxide"@en .



###  http://www.nist.gov/itl/ssd/Materials.owl#SiliconeBaseLubricant

:SiliconeBaseLubricant rdf:type owl:Class ;
                       
                       rdfs:subClassOf :FluidLubricant ;
                       
                       owl:disjointWith :SiliconeGellant ,
                                        :SyntheticEtherBase ,
                                        :UreaGellant ,
                                        :WhiteMineralOil ,
                                        :ZincOxideLubricant ;
                       
                       or:referenceURL "http://www.matweb.com/index.aspx"^^xsd:anyURI ;
                       
                       <http://www.nist.gov/itl/ssd/OntologyRequirements.owl#termString> "silicone base"@en ,
                                                                                         "silicone base lubricant"@en .



###  http://www.nist.gov/itl/ssd/Materials.owl#SiliconeGellant

:SiliconeGellant rdf:type owl:Class ;
                 
                 rdfs:subClassOf :FluidLubricant ;
                 
                 owl:disjointWith :SyntheticEtherBase ,
                                  :UreaGellant ,
                                  :WhiteMineralOil ,
                                  :ZincOxideLubricant ;
                 
                 or:referenceURL "http://www.matweb.com/index.aspx"^^xsd:anyURI ;
                 
                 <http://www.nist.gov/itl/ssd/OntologyRequirements.owl#termString> "silicone gellant"@en .



###  http://www.nist.gov/itl/ssd/Materials.owl#SingleCrystallineMaterial

:SingleCrystallineMaterial rdf:type owl:Class ;
                           
                           rdfs:subClassOf :SolidCrystallineSubstance ;
                           
                           rdfs:comment "Single Crystalline Material, is material formed from a single crystal."@en .



###  http://www.nist.gov/itl/ssd/Materials.owl#SinglePhaseMaterialPortion

:SinglePhaseMaterialPortion rdf:type owl:Class ;
                            
                            rdfs:subClassOf :MaterialPortion ;
                            
                            rdfs:comment "A Single Phase Material Portion is a portion of an object all of which has the same Material Phase Composition.  For example, it might be the portion of an alloy consisting of all grains of a single metal that have a specific crystalline structure."@en .



###  http://www.nist.gov/itl/ssd/Materials.owl#SingleWalledCarbonNanotube

:SingleWalledCarbonNanotube rdf:type owl:Class ;
                            
                            rdfs:subClassOf :CarbonNanotube ;
                            
                            rdfs:comment "Single Walled Carbon Nanotubes (SWCNTs) are the simplest kind of Carbon Nanotubes -- without any concentric structures. "@en .



###  http://www.nist.gov/itl/ssd/Materials.owl#Softwood

:Softwood rdf:type owl:Class ;
          
          rdfs:subClassOf :Wood ;
          
          or:referenceURL "http://www.matweb.com/index.aspx"^^xsd:anyURI ;
          
          <http://www.nist.gov/itl/ssd/OntologyRequirements.owl#termString> "softwood"@en .



###  http://www.nist.gov/itl/ssd/Materials.owl#SolidAerosol

:SolidAerosol rdf:type owl:Class ;
              
              rdfs:subClassOf :Aerosol ;
              
              rdfs:comment "A Solid Aerosol is a colloid suspension of fine solid particles in a gas."@en .



###  http://www.nist.gov/itl/ssd/Materials.owl#SolidCrystallineSubstance

:SolidCrystallineSubstance rdf:type owl:Class ;
                           
                           rdfs:subClassOf :CrystallineSubstance ,
                                           :SolidSubstance .



###  http://www.nist.gov/itl/ssd/Materials.owl#SolidDiffusion

:SolidDiffusion rdf:type owl:Class ;
                
                rdfs:subClassOf :Diffusion .



###  http://www.nist.gov/itl/ssd/Materials.owl#SolidFoam

:SolidFoam rdf:type owl:Class ;
           
           rdfs:subClassOf :Foam ,
                           :SolidSubstance ;
           
           rdfs:comment "A Solid Foam is a substance that is formed by trapping pockets of gas in a solid."@en .



###  http://www.nist.gov/itl/ssd/Materials.owl#SolidInLiquidSolution

:SolidInLiquidSolution rdf:type owl:Class ;
                       
                       rdfs:subClassOf :LiquidSolution ,
                                       [ rdf:type owl:Restriction ;
                                         owl:onProperty :solute ;
                                         owl:someValuesFrom :SolidSubstance
                                       ] ;
                       
                       rdfs:comment "A Solid In Liquid Solution is a Chemical Solution in which the soute is solid and the solvent is liquid."@en .



###  http://www.nist.gov/itl/ssd/Materials.owl#SolidSol

:SolidSol rdf:type owl:Class ;
          
          rdfs:subClassOf :Colloid ,
                          :SolidSubstance ;
          
          rdfs:comment "A Solid Sol is a type of colloid, with one solid phase dispersed inside another solid phase.  The phases remain distinct, so the result is not a solution."@en .



###  http://www.nist.gov/itl/ssd/Materials.owl#SolidSubstance

:SolidSubstance rdf:type owl:Class ;
                
                rdfs:subClassOf bc:MaterialSubstance ;
                
                owl:disjointWith :Vacuum ;
                
                rdfs:comment "Material in a solid phase."@en .



###  http://www.nist.gov/itl/ssd/Materials.owl#SolidToSolidPhaseTransformation

:SolidToSolidPhaseTransformation rdf:type owl:Class ;
                                 
                                 rdfs:subClassOf :PhaseChange ;
                                 
                                 owl:disjointWith :Solidification ,
                                                  :Vaporization ;
                                 
                                 rdfs:comment "A Solid to Solid Phase Transformation is a phase transition from one solid phase to another."@en .



###  http://www.nist.gov/itl/ssd/Materials.owl#Solidification

:Solidification rdf:type owl:Class ;
                
                rdfs:subClassOf :PhaseChange ;
                
                owl:disjointWith :Vaporization ;
                
                rdfs:comment "Solidification is a phase change of a material from a liquid, gasseous, or mixed state to a solid state."@en .



###  http://www.nist.gov/itl/ssd/Materials.owl#Solidus

:Solidus rdf:type owl:Class ;
         
         rdfs:subClassOf or:CurveSegment ;
         
         rdfs:comment "A Solidus is a Curve on a temperature-concentration Phase Diagram below which a given substance is completely solid."@en .



###  http://www.nist.gov/itl/ssd/Materials.owl#SpecificHeatCapacity

:SpecificHeatCapacity rdf:type owl:Class ;
                      
                      rdfs:subClassOf :ThermalProperty ;
                      
                      rdfs:comment "The Specific Heat Capacity (or specific heat) is the heat capacity per unit mass of a material, measured in Joules/(kg K)  (in SI units). "@en ;
                      
                      <http://www.nist.gov/itl/ssd/OntologyRequirements.owl#termString> "specific heat"@en ,
                                                                                        "specific heat capacity"@en .



###  http://www.nist.gov/itl/ssd/Materials.owl#Spectrometer

:Spectrometer rdf:type owl:Class ;
              
              rdfs:subClassOf or:LaboratoryEquipment ,
                              or:MeasuringDevice .



###  http://www.nist.gov/itl/ssd/Materials.owl#Spectrophotometer

:Spectrophotometer rdf:type owl:Class ;
                   
                   rdfs:subClassOf :Spectrometer ,
                                   or:Photometer ;
                   
                   rdfs:comment "A  Spectrophotometer is a photometer that measures light intensity as a function of its wavelength."@en .



###  http://www.nist.gov/itl/ssd/Materials.owl#SpringSteel

:SpringSteel rdf:type owl:Class ;
             
             rdfs:subClassOf :CarbonSteel ;
             
             rdfs:comment "Spring steel is a low alloy, medium carbon steel or high carbon steel with a very high yield strength. This allows objects made of spring steel to return to their original shape despite significant bending or twist."@en .



###  http://www.nist.gov/itl/ssd/Materials.owl#StableIsotope

:StableIsotope rdf:type owl:Class ;
               
               rdfs:subClassOf bc:Isotope ;
               
               rdfs:comment "A Stable Isotope is one that is not radioactive"@en .



###  http://www.nist.gov/itl/ssd/Materials.owl#StainlessSteel

:StainlessSteel rdf:type owl:Class ;
                
                rdfs:subClassOf :Steel ;
                
                owl:disjointWith :ToolSteel ;
                
                <http://www.nist.gov/itl/ssd/OntologyRequirements.owl#termString> "CRES"@en ,
                                                                                  "Stainless steel is  a steel alloy with a minimum of 10.5% to 11% chromium content by mass."@en ,
                                                                                  "corrosion-resistant steel"@en ,
                                                                                  "inox"@en ,
                                                                                  "inox steel"@en ,
                                                                                  "stainless steel"@en .



###  http://www.nist.gov/itl/ssd/Materials.owl#StateOfMatter

:StateOfMatter rdf:type owl:Class ;
               
               rdfs:subClassOf :MaterialPhaseComposition ;
               
               rdfs:comment "A basic State Of Matter is Solid, Liquid, Gas, or Plasma.  "@en .



###  http://www.nist.gov/itl/ssd/Materials.owl#Steel

:Steel rdf:type owl:Class ;
       
       rdfs:subClassOf :EngineeredAlloy ,
                       :FerrousAlloy .



###  http://www.nist.gov/itl/ssd/Materials.owl#Stiffness

:Stiffness rdf:type owl:Class ;
           
           rdfs:subClassOf :DeformationProperty .



###  http://www.nist.gov/itl/ssd/Materials.owl#Strength

:Strength rdf:type owl:Class ;
          
          rdfs:subClassOf :MeasurableMechanicalProperty ;
          
          owl:disjointWith :TransportProperty .



###  http://www.nist.gov/itl/ssd/Materials.owl#Sublimating

:Sublimating rdf:type owl:Class ;
             
             rdfs:subClassOf :OrderDisorderPhaseTransformation ,
                             :Vaporization ;
             
             rdfs:comment "Sublimating is the Phase Change from a solid state directly to a gasseous state without passing through an intermediate liquid state"@en .



###  http://www.nist.gov/itl/ssd/Materials.owl#SublimatingToSolid

:SublimatingToSolid rdf:type owl:Class ;
                    
                    rdfs:subClassOf :Solidification ;
                    
                    rdfs:comment "SublimatingToSolid is the phase change from a gasseous state to a solid state without going through an intermediate liquid state."@en .



###  http://www.nist.gov/itl/ssd/Materials.owl#Sulfate

:Sulfate rdf:type owl:Class ;
         
         rdfs:subClassOf :Mineral .



###  http://www.nist.gov/itl/ssd/Materials.owl#SulfideCeramic

:SulfideCeramic rdf:type owl:Class ;
                
                rdfs:subClassOf :ChalcogenBasedCeramic ;
                
                or:referenceURL "http://www.matweb.com/index.aspx"^^xsd:anyURI ;
                
                <http://www.nist.gov/itl/ssd/OntologyRequirements.owl#termString> "sulfide"@en ,
                                                                                  "sulfide ceramic"@en .



###  http://www.nist.gov/itl/ssd/Materials.owl#SulfideMineral

:SulfideMineral rdf:type owl:Class ;
                
                rdfs:subClassOf :Mineral .



###  http://www.nist.gov/itl/ssd/Materials.owl#SulfosaltMineral

:SulfosaltMineral rdf:type owl:Class ;
                  
                  rdfs:subClassOf :Mineral .



###  http://www.nist.gov/itl/ssd/Materials.owl#Superalloy

:Superalloy rdf:type owl:Class ;
            
            rdfs:subClassOf :EngineeredAlloy ;
            
            rdfs:comment "A Superalloy, or high-performance alloy, is an alloy that exhibits excellent mechanical strength and creep resistance at high temperatures, good surface stability, and corrosion and oxidation resistance. Superalloys typically have a matrix with an austenitic face-centered cubic crystal structure. A superalloy's base alloying element is usually nickel, cobalt, or nickel-iron."@en .



###  http://www.nist.gov/itl/ssd/Materials.owl#SurfaceDiffusion

:SurfaceDiffusion rdf:type owl:Class ;
                  
                  rdfs:subClassOf :ShortCircuitDiffusion ;
                  
                  rdfs:seeAlso "Definitions of terms for diffusion in the solid state (IUPAC Recommendations 1999), Pure Appl. Chem. 71, 1307-1325."@en ;
                  
                  rdfs:comment "Surface diffusion is diffusion that takes place on a surface."@en .



###  http://www.nist.gov/itl/ssd/Materials.owl#SyntheticEtherBase

:SyntheticEtherBase rdf:type owl:Class ;
                    
                    rdfs:subClassOf :FluidLubricant ;
                    
                    owl:disjointWith :UreaGellant ,
                                     :WhiteMineralOil ,
                                     :ZincOxideLubricant ;
                    
                    or:referenceURL "http://www.matweb.com/index.aspx"^^xsd:anyURI ;
                    
                    <http://www.nist.gov/itl/ssd/OntologyRequirements.owl#termString> "synthetic ether base"@en ,
                                                                                      "synthetic ether base lubricant"@en .



###  http://www.nist.gov/itl/ssd/Materials.owl#TemperatureChangeProcess

:TemperatureChangeProcess rdf:type owl:Class ;
                          
                          rdfs:subClassOf or:MechanicalProcess ;
                          
                          owl:disjointWith :ThermalExpansion ;
                          
                          rdfs:comment "A Temperature Change Process is a process during which the temperature of an object increases or decreases.  "@en .



###  http://www.nist.gov/itl/ssd/Materials.owl#TetragonalCrystalStructure

:TetragonalCrystalStructure rdf:type owl:Class ;
                            
                            rdfs:subClassOf :CrystalLattice ;
                            
                            owl:disjointWith :TriclinicCrystalStructure ,
                                             :TrigonalCrystalStructure ;
                            
                            rdfs:comment """Tetragonal crystal lattices result from stretching a cubic lattice along one of its lattice vectors, so that the cube becomes a rectangular prism with a square base (a by a) and height (c, which is different from a).

There are two tetragonal Bravais lattices: the simple (or primitive) tetragonal (from stretching the simple-cubic lattice) and the body-centered tetragonal (from stretching either the face-centered or the body-centered cubic lattice)."""@en .



###  http://www.nist.gov/itl/ssd/Materials.owl#ThermalExpansion

:ThermalExpansion rdf:type owl:Class ;
                  
                  rdfs:subClassOf or:MechanicalProcess ;
                  
                  rdfs:comment "Thermal Expansion is a Mechanical Process in which an object changes size (expands or contracts) in response to a change in temperature."@en .



###  http://www.nist.gov/itl/ssd/Materials.owl#ThermalProperty

:ThermalProperty rdf:type owl:Class ;
                 
                 rdfs:subClassOf or:MeasurableMaterialProperty ;
                 
                 <http://www.w3.org/2004/02/skos/core#note> "Similar to \"Thermal\" in Ashino's 2010 Minerals Ontology."@en .



###  http://www.nist.gov/itl/ssd/Materials.owl#ThermochemicalProperty

:ThermochemicalProperty rdf:type owl:Class ;
                        
                        rdfs:subClassOf or:MeasurableMaterialProperty .



###  http://www.nist.gov/itl/ssd/Materials.owl#ThermodynamicPhase

:ThermodynamicPhase rdf:type owl:Class ;
                    
                    rdfs:subClassOf or:ObjectType ;
                    
                    rdfs:comment "A Thermodynamic Phase is defined as a type region of space throughout which all physical properties of a material (composition, enthalpy content, StateOfMatter, and other properties are essentially uniform.  A material may be of a single phase, or at a microscopic level, be composed of regions of two (or more) phases.  A thermodynamic Phase Diagram depicts the boundaries among Thermodynamic Phases and binary (or multi-) phase fields.  "@en .



###  http://www.nist.gov/itl/ssd/Materials.owl#ThermodynamicSystem

:ThermodynamicSystem rdf:type owl:Class ;
                     
                     rdfs:subClassOf or:PhysicalObject ;
                     
                     rdfs:comment "A thermodynamic system is a precisely defined macroscopic region of the universe, often called a physical system.  The set of thermodynamic parameters necessary to uniquely define a system is called the thermodynamic state of a system. The state of a system is expressed as a functional relationship, the equation of state, between its parameters. A system is in thermodynamic equilibrium when the state of the system does not change with time."@en .



###  http://www.nist.gov/itl/ssd/Materials.owl#Thermomigration

:Thermomigration rdf:type owl:Class ;
                 
                 rdfs:subClassOf :Diffusion ;
                 
                 rdfs:seeAlso "Definitions of terms for diffusion in the solid state (IUPAC Recommendations 1999), Pure Appl. Chem. 71, 1307-1325."@en ;
                 
                 rdfs:comment "Thermomigration is diffusion resulting from a temperature gradient.  This is also called thermal diffusion, the Ludwig-Soret effect, or the Soret effect."@en .



###  http://www.nist.gov/itl/ssd/Materials.owl#Thermoplastic

:Thermoplastic rdf:type owl:Class ;
               
               rdfs:subClassOf :EngineeredMaterial ,
                               :PolymerSubstance ;
               
               owl:disjointWith :Thermoset ;
               
               or:referenceURL "http://www.matweb.com/index.aspx"^^xsd:anyURI ;
               
               rdfs:comment "A Thermoplastic, or thermosoftening plastic, is a polymer that becomes pliable or moldable above a specific temperature, and returns to a solid state upon cooling. This property allows thermoplastics to be remolded."@en .



###  http://www.nist.gov/itl/ssd/Materials.owl#Thermoset

:Thermoset rdf:type owl:Class ;
           
           rdfs:subClassOf :PolymerSubstance ;
           
           rdfs:comment "A thermosetting plastic (or Thermoset) is polymer material that irreversibly cures. The cure may be done through heat (generally above 200 °C (392 °F)), through a chemical reaction (two-part epoxy, for example), or irradiation such as electron beam processing."@en ;
           
           <http://www.nist.gov/itl/ssd/OntologyRequirements.owl#termString> "thermoset"@en ,
                                                                             "thermosetting plastic"@en .



###  http://www.nist.gov/itl/ssd/Materials.owl#ThinFilm

:ThinFilm rdf:type owl:Class ;
          
          rdfs:subClassOf bc:MaterialSubstance ;
          
          rdfs:comment "A thin film is a layer of material ranging from fractions of a nanometer (monolayer) to several microns in thickness."@en .



###  http://www.nist.gov/itl/ssd/Materials.owl#TinAlloy

:TinAlloy rdf:type owl:Class ;
          
          rdfs:subClassOf :NonFerrousAlloy ,
                          [ rdf:type owl:Restriction ;
                            owl:onProperty :physicalDecompositions ;
                            owl:someValuesFrom bc:Tin
                          ] ;
          
          or:referenceURL "http://www.matweb.com/index.aspx"^^xsd:anyURI ;
          
          rdfs:comment "An alloy that contains Tin but not Iron."@en .



###  http://www.nist.gov/itl/ssd/Materials.owl#TitaniumOxide

:TitaniumOxide rdf:type owl:Class ;
               
               rdfs:subClassOf bc:Oxide ;
               
               owl:disjointWith :ZirconiumOxide ;
               
               or:referenceURL "http://www.matweb.com/index.aspx"^^xsd:anyURI ;
               
               <http://www.nist.gov/itl/ssd/OntologyRequirements.owl#termString> "titanium oxide"@en .



###  http://www.nist.gov/itl/ssd/Materials.owl#ToolSteel

:ToolSteel rdf:type owl:Class ;
           
           rdfs:subClassOf :Steel ;
           
           or:referenceURL "http://www.matweb.com/index.aspx"^^xsd:anyURI ;
           
           rdfs:comment """Tool steel refers to a variety of carbon and alloy steels that are particularly well-suited to be made into tools. Their suitability comes from their distinctive hardness, resistance to abrasion, their ability to hold a cutting edge, and/or their resistance to deformation at elevated temperatures (red-hardness). Tool steel is generally heat-treated.

Tool steel has a carbon content between 0.7% and 1.5%. The manganese content is often kept low to minimize the possibility of cracking during water quenching."""@en ;
           
           <http://www.nist.gov/itl/ssd/OntologyRequirements.owl#termString> "tool steel"@en .



###  http://www.nist.gov/itl/ssd/Materials.owl#TracerDiffusion

:TracerDiffusion rdf:type owl:Class ;
                 
                 rdfs:subClassOf :Diffusion ;
                 
                 rdfs:seeAlso "Definitions of terms for diffusion in the solid state (IUPAC Recommendations 1999), Pure Appl. Chem. 71, 1307-1325."@en ;
                 
                 rdfs:comment "Tracer diffusion refers to the migration of a tagged atom through a material of which it is a component."@en .



###  http://www.nist.gov/itl/ssd/Materials.owl#TransparencyLevel

:TransparencyLevel rdf:type owl:Class ;
                   
                   rdfs:subClassOf or:Quantity .



###  http://www.nist.gov/itl/ssd/Materials.owl#TransportProperty

:TransportProperty rdf:type owl:Class ;
                   
                   rdfs:subClassOf :MeasurableMechanicalProperty .



###  http://www.nist.gov/itl/ssd/Materials.owl#TriclinicCrystalStructure

:TriclinicCrystalStructure rdf:type owl:Class ;
                           
                           rdfs:subClassOf :CrystalLattice ;
                           
                           rdfs:comment "The triclinic lattice is the least symmetric of the 14 three-dimensional Bravais lattices. It has (itself) the minimum symmetry all lattices have: points of inversion at each lattice point and at 7 more points for each lattice point: at the midpoints of the edges and the faces, and at the center points. It is the only lattice type that itself has no mirror planes."@en .



###  http://www.nist.gov/itl/ssd/Materials.owl#TrigonalCrystalStructure

:TrigonalCrystalStructure rdf:type owl:Class ;
                          
                          rdfs:subClassOf :CrystalLattice ;
                          
                          rdfs:comment "The trigonal crystal system is the only crystal system whose point groups have more than one lattice system associated with their space groups: the hexagonal and rhombohedral lattices both appear."@en .



###  http://www.nist.gov/itl/ssd/Materials.owl#UnitOfAreaPerTime

:UnitOfAreaPerTime rdf:type owl:Class ;
                   
                   rdfs:subClassOf or:UnitOfMeasure ;
                   
                   owl:disjointWith :UnitOfCharge ,
                                    :UnitOfElectricCurrent ,
                                    :UnitOfElectricalConductivity ,
                                    :UnitOfElectricalResistance ,
                                    :UnitOfElectricalResistivity ,
                                    :UnitOfEnergyPerMass ,
                                    :UnitOfInverseAreaPerTime ,
                                    :UnitOfSpecificHeatCapacity ,
                                    :UnitOfThermalConductivity ,
                                    or:CurrencyUnit ,
                                    or:UnitOfArea ,
                                    or:UnitOfComputerStorageCapacity ,
                                    or:UnitOfDensity ,
                                    or:UnitOfDistance ,
                                    or:UnitOfDuration ,
                                    or:UnitOfEnergy ,
                                    or:UnitOfForce ,
                                    or:UnitOfMass .



###  http://www.nist.gov/itl/ssd/Materials.owl#UnitOfCapacitance

:UnitOfCapacitance rdf:type owl:Class ;
                   
                   rdfs:subClassOf or:UnitOfMeasure .



###  http://www.nist.gov/itl/ssd/Materials.owl#UnitOfCharge

:UnitOfCharge rdf:type owl:Class ;
              
              rdfs:subClassOf or:UnitOfMeasure ;
              
              owl:disjointWith :UnitOfElectricCurrent ,
                               :UnitOfElectricalConductance ,
                               :UnitOfElectricalConductivity ,
                               :UnitOfElectricalResistance ,
                               :UnitOfElectricalResistivity ,
                               :UnitOfEnergyPerMass ,
                               :UnitOfEnergyPerTemperatureDifference ,
                               :UnitOfForcePerVolume ,
                               :UnitOfInverseAreaPerTime ,
                               :UnitOfInverseTemperatureDifference ,
                               :UnitOfInverseTime ,
                               :UnitOfPower ,
                               :UnitOfSpecificHeatCapacity ,
                               :UnitOfTemperatureDifference ,
                               :UnitOfThermalConductivity ,
                               :UnitOfToughness ,
                               or:UnitOfAcceleration ,
                               or:UnitOfArea ,
                               or:UnitOfComputerStorageCapacity ,
                               or:UnitOfDensity ,
                               or:UnitOfDistance ,
                               or:UnitOfDuration ,
                               or:UnitOfEnergy ,
                               or:UnitOfForce ,
                               or:UnitOfMass ,
                               or:UnitOfPressure ,
                               or:UnitOfSpreadRate ,
                               or:UnitOfTemperature ,
                               or:UnitOfVelocity ,
                               or:UnitOfVoltage ,
                               or:UnitOfVolume ,
                               <http://www.nist.gov/itl/ssd/OntologyRequirements.owl#DimensionlessUnit> ,
                               <http://www.nist.gov/itl/ssd/OntologyRequirements.owl#UnitOfVelocitySquared> .



###  http://www.nist.gov/itl/ssd/Materials.owl#UnitOfElectricCurrent

:UnitOfElectricCurrent rdf:type owl:Class ;
                       
                       rdfs:subClassOf or:UnitOfMeasure ;
                       
                       owl:disjointWith :UnitOfElectricalConductance ,
                                        :UnitOfElectricalConductivity ,
                                        :UnitOfElectricalResistance ,
                                        :UnitOfElectricalResistivity ,
                                        :UnitOfEnergyPerMass ,
                                        :UnitOfEnergyPerTemperatureDifference ,
                                        :UnitOfForcePerVolume ,
                                        :UnitOfInverseTemperatureDifference ,
                                        :UnitOfInverseTime ,
                                        :UnitOfPower ,
                                        :UnitOfSpecificHeatCapacity ,
                                        :UnitOfTemperatureDifference ,
                                        :UnitOfThermalConductivity ,
                                        :UnitOfToughness ,
                                        or:UnitOfAcceleration ,
                                        or:UnitOfArea ,
                                        or:UnitOfComputerStorageCapacity ,
                                        or:UnitOfDensity ,
                                        or:UnitOfDistance ,
                                        or:UnitOfDuration ,
                                        or:UnitOfEnergy ,
                                        or:UnitOfForce ,
                                        or:UnitOfMass ,
                                        or:UnitOfPressure ,
                                        or:UnitOfSpreadRate ,
                                        or:UnitOfTemperature ,
                                        or:UnitOfVelocity ,
                                        or:UnitOfVoltage ,
                                        or:UnitOfVolume ,
                                        <http://www.nist.gov/itl/ssd/OntologyRequirements.owl#DimensionlessUnit> ,
                                        <http://www.nist.gov/itl/ssd/OntologyRequirements.owl#UnitOfVelocitySquared> .



###  http://www.nist.gov/itl/ssd/Materials.owl#UnitOfElectricalConductance

:UnitOfElectricalConductance rdf:type owl:Class ;
                             
                             rdfs:subClassOf or:UnitOfMeasure ;
                             
                             owl:disjointWith :UnitOfInverseAreaPerTime ,
                                              :UnitOfSpecificHeatCapacity ,
                                              :UnitOfTemperatureDifference .



###  http://www.nist.gov/itl/ssd/Materials.owl#UnitOfElectricalConductivity

:UnitOfElectricalConductivity rdf:type owl:Class ;
                              
                              rdfs:subClassOf or:UnitOfMeasure ;
                              
                              owl:disjointWith :UnitOfElectricalResistance ,
                                               :UnitOfElectricalResistivity ,
                                               :UnitOfEnergyPerMass ,
                                               :UnitOfInverseAreaPerTime ,
                                               :UnitOfSpecificHeatCapacity ,
                                               :UnitOfTemperatureDifference ,
                                               :UnitOfThermalConductivity ,
                                               or:CurrencyUnit ,
                                               or:UnitOfAcceleration ,
                                               or:UnitOfArea ,
                                               or:UnitOfComputerStorageCapacity ,
                                               or:UnitOfDensity ,
                                               or:UnitOfDistance ,
                                               or:UnitOfDuration ,
                                               or:UnitOfEnergy ,
                                               or:UnitOfForce ,
                                               or:UnitOfMass ,
                                               or:UnitOfPressure ,
                                               or:UnitOfSpreadRate ,
                                               or:UnitOfTemperature ,
                                               or:UnitOfVoltage ,
                                               or:UnitOfVolume ,
                                               <http://www.nist.gov/itl/ssd/OntologyRequirements.owl#DimensionlessUnit> .



###  http://www.nist.gov/itl/ssd/Materials.owl#UnitOfElectricalResistance

:UnitOfElectricalResistance rdf:type owl:Class ;
                            
                            rdfs:subClassOf or:UnitOfMeasure ;
                            
                            owl:disjointWith :UnitOfElectricalResistivity ,
                                             :UnitOfEnergyPerMass ,
                                             :UnitOfInverseAreaPerTime ,
                                             :UnitOfSpecificHeatCapacity ,
                                             :UnitOfTemperatureDifference ,
                                             :UnitOfThermalConductivity ,
                                             or:CurrencyUnit ,
                                             or:UnitOfArea ,
                                             or:UnitOfComputerStorageCapacity ,
                                             or:UnitOfDensity ,
                                             or:UnitOfDistance ,
                                             or:UnitOfDuration ,
                                             or:UnitOfEnergy ,
                                             or:UnitOfMass ,
                                             or:UnitOfPressure ,
                                             or:UnitOfSpreadRate ,
                                             or:UnitOfTemperature ,
                                             or:UnitOfVoltage ,
                                             or:UnitOfVolume .



###  http://www.nist.gov/itl/ssd/Materials.owl#UnitOfElectricalResistivity

:UnitOfElectricalResistivity rdf:type owl:Class ;
                             
                             rdfs:subClassOf or:UnitOfMeasure ;
                             
                             owl:disjointWith :UnitOfEnergyPerMass ,
                                              :UnitOfInverseAreaPerTime ,
                                              :UnitOfSpecificHeatCapacity ,
                                              :UnitOfTemperatureDifference ,
                                              :UnitOfThermalConductivity ,
                                              or:CurrencyUnit ,
                                              or:UnitOfArea ,
                                              or:UnitOfComputerStorageCapacity ,
                                              or:UnitOfDensity ,
                                              or:UnitOfDistance ,
                                              or:UnitOfDuration ,
                                              or:UnitOfEnergy ,
                                              or:UnitOfForce ,
                                              or:UnitOfMass ,
                                              or:UnitOfPressure ,
                                              or:UnitOfSpreadRate ,
                                              or:UnitOfTemperature ,
                                              or:UnitOfVoltage ,
                                              or:UnitOfVolume .



###  http://www.nist.gov/itl/ssd/Materials.owl#UnitOfEnergyPerMass

:UnitOfEnergyPerMass rdf:type owl:Class ;
                     
                     rdfs:subClassOf or:UnitOfMeasure ;
                     
                     owl:disjointWith :UnitOfInverseAreaPerTime ,
                                      :UnitOfSpecificHeatCapacity ,
                                      :UnitOfTemperatureDifference ,
                                      :UnitOfThermalConductivity ,
                                      or:UnitOfArea ,
                                      or:UnitOfComputerStorageCapacity ,
                                      or:UnitOfDensity ,
                                      or:UnitOfDistance ,
                                      or:UnitOfDuration ,
                                      or:UnitOfEnergy ,
                                      or:UnitOfForce ,
                                      or:UnitOfMass ,
                                      or:UnitOfSpreadRate ,
                                      or:UnitOfTemperature ,
                                      or:UnitOfVoltage ,
                                      or:UnitOfVolume ;
                     
                     rdfs:comment "A Unit Of Energy Per Mass is a Unit Of Energy divided by a Unit Of Mass.  E.g., Joules per Gram."@en .



###  http://www.nist.gov/itl/ssd/Materials.owl#UnitOfEnergyPerTemperatureDifference

:UnitOfEnergyPerTemperatureDifference rdf:type owl:Class ;
                                      
                                      rdfs:subClassOf or:UnitOfMeasure ;
                                      
                                      owl:disjointWith :UnitOfTemperatureDifference .



###  http://www.nist.gov/itl/ssd/Materials.owl#UnitOfForcePerVolume

:UnitOfForcePerVolume rdf:type owl:Class ;
                      
                      rdfs:subClassOf or:UnitOfMeasure ;
                      
                      owl:disjointWith :UnitOfSpecificHeatCapacity ,
                                       :UnitOfTemperatureDifference .



###  http://www.nist.gov/itl/ssd/Materials.owl#UnitOfInductance

:UnitOfInductance rdf:type owl:Class ;
                  
                  rdfs:subClassOf or:UnitOfMeasure .



###  http://www.nist.gov/itl/ssd/Materials.owl#UnitOfInverseAreaPerTime

:UnitOfInverseAreaPerTime rdf:type owl:Class ;
                          
                          rdfs:subClassOf or:UnitOfMeasure ;
                          
                          owl:disjointWith :UnitOfSpecificHeatCapacity ,
                                           :UnitOfTemperatureDifference ,
                                           :UnitOfThermalConductivity ,
                                           or:CurrencyUnit ,
                                           or:UnitOfAcceleration ,
                                           or:UnitOfArea ,
                                           or:UnitOfComputerStorageCapacity ,
                                           or:UnitOfDensity ,
                                           or:UnitOfDistance ,
                                           or:UnitOfDuration ,
                                           or:UnitOfEnergy ,
                                           or:UnitOfForce ,
                                           or:UnitOfMass ,
                                           or:UnitOfPressure ,
                                           or:UnitOfSpreadRate ,
                                           or:UnitOfTemperature ,
                                           or:UnitOfVelocity ,
                                           or:UnitOfVoltage ,
                                           or:UnitOfVolume ,
                                           <http://www.nist.gov/itl/ssd/OntologyRequirements.owl#DimensionlessUnit> ;
                          
                          rdfs:comment "A Unit of Inverse Area per Time has the dimension of 1/ Area / Duration."@en .



###  http://www.nist.gov/itl/ssd/Materials.owl#UnitOfInverseTemperatureDifference

:UnitOfInverseTemperatureDifference rdf:type owl:Class ;
                                    
                                    rdfs:subClassOf or:UnitOfMeasure ;
                                    
                                    owl:disjointWith :UnitOfTemperatureDifference .



###  http://www.nist.gov/itl/ssd/Materials.owl#UnitOfInverseTime

:UnitOfInverseTime rdf:type owl:Class ;
                   
                   rdfs:subClassOf or:UnitOfMeasure ;
                   
                   owl:disjointWith :UnitOfSpecificHeatCapacity ,
                                    :UnitOfTemperatureDifference .



###  http://www.nist.gov/itl/ssd/Materials.owl#UnitOfPower

:UnitOfPower rdf:type owl:Class ;
             
             rdfs:subClassOf or:UnitOfMeasure .



###  http://www.nist.gov/itl/ssd/Materials.owl#UnitOfPrecision

:UnitOfPrecision rdf:type owl:Class ;
                 
                 rdfs:subClassOf or:UnitOfMeasure ;
                 
                 owl:disjointWith :UnitOfSpecificHeatCapacity .



###  http://www.nist.gov/itl/ssd/Materials.owl#UnitOfSpecificHeatCapacity

:UnitOfSpecificHeatCapacity rdf:type owl:Class ;
                            
                            rdfs:subClassOf or:UnitOfMeasure ;
                            
                            owl:disjointWith :UnitOfTemperatureDifference ,
                                             :UnitOfThermalConductivity ,
                                             :UnitOfToughness ,
                                             or:CurrencyUnit ,
                                             or:UnitOfAcceleration ,
                                             or:UnitOfArea ,
                                             or:UnitOfComputerStorageCapacity ,
                                             or:UnitOfDensity ,
                                             or:UnitOfDuration ,
                                             or:UnitOfEnergy ,
                                             or:UnitOfForce ,
                                             or:UnitOfMass ,
                                             or:UnitOfPressure ,
                                             or:UnitOfSpreadRate ,
                                             or:UnitOfTemperature ,
                                             or:UnitOfVelocity ,
                                             or:UnitOfVoltage ,
                                             or:UnitOfVolume ,
                                             <http://www.nist.gov/itl/ssd/OntologyRequirements.owl#DimensionlessUnit> ,
                                             <http://www.nist.gov/itl/ssd/OntologyRequirements.owl#UnitOfVelocitySquared> .



###  http://www.nist.gov/itl/ssd/Materials.owl#UnitOfTemperatureDifference

:UnitOfTemperatureDifference rdf:type owl:Class ;
                             
                             rdfs:subClassOf or:UnitOfMeasure ;
                             
                             owl:disjointWith :UnitOfThermalConductivity ,
                                              :UnitOfToughness ,
                                              or:UnitOfEnergy ,
                                              or:UnitOfForce ,
                                              or:UnitOfMass ,
                                              or:UnitOfPressure ,
                                              or:UnitOfSpreadRate ,
                                              or:UnitOfVelocity ,
                                              or:UnitOfVoltage ,
                                              or:UnitOfVolume ,
                                              <http://www.nist.gov/itl/ssd/OntologyRequirements.owl#UnitOfVelocitySquared> ;
                             
                             rdfs:comment "A Unit of Temperature Difference is a Unit of Measure that indicates the differnce in temperature between two things.  A Celsius Degree and a Kelvin Degree have the same magnitude, and thus there is no difference between them as units of Temperature Difference."@en .



###  http://www.nist.gov/itl/ssd/Materials.owl#UnitOfThermalConductivity

:UnitOfThermalConductivity rdf:type owl:Class ;
                           
                           rdfs:subClassOf or:UnitOfMeasure ;
                           
                           owl:disjointWith or:CurrencyUnit ,
                                            or:UnitOfArea ,
                                            or:UnitOfComputerStorageCapacity ,
                                            or:UnitOfDensity ,
                                            or:UnitOfDistance ,
                                            or:UnitOfDuration ,
                                            or:UnitOfEnergy ,
                                            or:UnitOfForce ,
                                            or:UnitOfMass ,
                                            or:UnitOfPressure ,
                                            or:UnitOfSpreadRate ,
                                            or:UnitOfTemperature ,
                                            or:UnitOfVoltage ,
                                            or:UnitOfVolume ;
                           
                           rdfs:comment "Units Of Thermal Conductivity have the dimension Mass * Distance / (Temperature * Duration^3) .  The SI unit is Watts/(m K)."@en .



###  http://www.nist.gov/itl/ssd/Materials.owl#UnitOfToughness

:UnitOfToughness rdf:type owl:Class ;
                 
                 rdfs:subClassOf or:UnitOfMeasure ;
                 
                 owl:disjointWith or:UnitOfSpreadRate .



###  http://www.nist.gov/itl/ssd/Materials.owl#UphillDiffusion

:UphillDiffusion rdf:type owl:Class ;
                 
                 rdfs:subClassOf :SolidDiffusion ;
                 
                 rdfs:seeAlso "Definitions of terms for diffusion in the solid state (IUPAC Recommendations 1999), Pure Appl. Chem. 71, 1307-1325."@en ;
                 
                 rdfs:comment "Uphill Diffusion is a diffusion process in which a diffusing species migrates against its concentration gradient. It occurs in ternary and higher order systems either because of therymodynamic effects or because of differences in mobilities of the species."@en ;
                 
                 <http://www.nist.gov/itl/ssd/OntologyRequirements.owl#termString> "uphill diffusion"@en .



###  http://www.nist.gov/itl/ssd/Materials.owl#UreaGellant

:UreaGellant rdf:type owl:Class ;
             
             rdfs:subClassOf :FluidLubricant ;
             
             owl:disjointWith :WhiteMineralOil ,
                              :ZincOxideLubricant ;
             
             or:referenceURL "http://www.matweb.com/index.aspx"^^xsd:anyURI ;
             
             <http://www.nist.gov/itl/ssd/OntologyRequirements.owl#termString> "urea gellant"@en .



###  http://www.nist.gov/itl/ssd/Materials.owl#VacancyDiffusionMechanism

:VacancyDiffusionMechanism rdf:type owl:Class ;
                           
                           rdfs:subClassOf :MicroscopicDiffusionMovement ;
                           
                           rdfs:seeAlso "Definitions of terms for diffusion in the solid state (IUPAC Recommendations 1999), Pure Appl. Chem. 71, 1307-1325."@en ;
                           
                           rdfs:comment "The Vacancy Diffusion Mechanism is a mechanism where diffusion is made possible by the exchange of positions between the diffusing species and a vacancy."@en .



###  http://www.nist.gov/itl/ssd/Materials.owl#VacancyWindEffect

:VacancyWindEffect rdf:type owl:Class ;
                   
                   rdfs:subClassOf :SolidDiffusion ;
                   
                   rdfs:seeAlso "Definitions of terms for diffusion in the solid state (IUPAC Recommendations 1999), Pure Appl. Chem. 71, 1307-1325." ;
                   
                   rdfs:comment "The Vacancy WindEffect occurs if diffusion gives rise to a flux of vacancies in one direction.  In this case, the availability of vacancies for a given substitutional atom is biased. The atoms will be able to jump more frequently to the ‘windward’ side since the vacancy concentration at that side is higher than at the ‘leeward’ side. Therefore there is a preferential diffusion against the vacancy wind."@en ;
                   
                   <http://www.nist.gov/itl/ssd/OntologyRequirements.owl#termString> "vacancy wind effect"@en .



###  http://www.nist.gov/itl/ssd/Materials.owl#Vacuum

:Vacuum rdf:type owl:Class ;
        
        rdfs:subClassOf bc:MaterialSubstance ;
        
        owl:disjointWith or:Artifact ;
        
        rdfs:comment "Vacuum is the absense of Material Substance, but can be considered to be the substance that something in a vacuum is surrounded by."@en .



###  http://www.nist.gov/itl/ssd/Materials.owl#VanadateMineral

:VanadateMineral rdf:type owl:Class ;
                 
                 rdfs:subClassOf :Mineral .



###  http://www.nist.gov/itl/ssd/Materials.owl#Vaporization

:Vaporization rdf:type owl:Class ;
              
              rdfs:subClassOf :PhaseChange ;
              
              rdfs:comment "Vaporization is the Phase Change from a solid or liquid state to a gasseous state."@en .



###  http://www.nist.gov/itl/ssd/Materials.owl#VinylPolymer

:VinylPolymer rdf:type owl:Class ;
              
              rdfs:subClassOf :Thermoplastic ;
              
              rdfs:comment "Vinyl polymers are a group of polymers derived from vinyl monomers. Their backbone is an extended alkane chain, made by polymerizing an alkene group (C=C) into a chain (..-C-C-C-C-..).  Vinyl polymers are produced catalytically."@en .



###  http://www.nist.gov/itl/ssd/Materials.owl#Viscosity

:Viscosity rdf:type owl:Class ;
           
           rdfs:subClassOf :TransportProperty ;
           
           rdfs:comment "Diffusivity is the ratio between the molar flux due to molecular diffusion and the gradient in the concentration of the species (or the driving force for diffusion).  Diffusivity is generally prescribed for a given pair of species in a given phase at a given temperature. For a multi-component system, it is prescribed for each pair of species in the system.  Diffusivity is measured in Area per unit time -- in SI, m^2/s."@en .



###  http://www.nist.gov/itl/ssd/Materials.owl#Waspaloy

:Waspaloy rdf:type owl:Class ;
          
          rdfs:subClassOf :NickelAlloy ,
                          :Superalloy ;
          
          rdfs:comment "Waspaloy is a registered trademark of United Technologies Corp that refers to an age hardening austenitic nickel-based superalloy used for high-temperature applications."@en .



###  http://www.nist.gov/itl/ssd/Materials.owl#WhiteCastIron

:WhiteCastIron rdf:type owl:Class ;
               
               rdfs:subClassOf :CastIron ;
               
               or:referenceURL "http://www.matweb.com/index.aspx"^^xsd:anyURI ;
               
               rdfs:comment "White cast iron, is a type of cast iron that is named after the white color of the fracture it forms, which is due to the presence of cementite."@en ;
               
               <http://www.nist.gov/itl/ssd/OntologyRequirements.owl#termString> "white cast iron"@en .



###  http://www.nist.gov/itl/ssd/Materials.owl#WhiteMineralOil

:WhiteMineralOil rdf:type owl:Class ;
                 
                 rdfs:subClassOf :FluidLubricant ;
                 
                 owl:disjointWith :ZincOxideLubricant ;
                 
                 or:referenceURL "http://www.matweb.com/index.aspx"^^xsd:anyURI ;
                 
                 <http://www.nist.gov/itl/ssd/OntologyRequirements.owl#termString> "white mineral oil"@en .



###  http://www.nist.gov/itl/ssd/Materials.owl#Wood

:Wood rdf:type owl:Class ;
      
      rdfs:subClassOf :CompositeMaterial ,
                      :SolidSubstance ;
      
      rdfs:comment "Wood is a hard, fibrous tissue found in many trees. It is an organic material, a natural composite of cellulose fibers (which are strong in tension) embedded in a matrix of lignin which resists compression."@en .



###  http://www.nist.gov/itl/ssd/Materials.owl#WroughtAlloy

:WroughtAlloy rdf:type owl:Class ;
              
              rdfs:subClassOf :EngineeredAlloy ;
              
              rdfs:comment "A Wrought Alloy is one in which soft heated metal is mechanically worked (often by hammering) into shape, possibly after casting."@en .



###  http://www.nist.gov/itl/ssd/Materials.owl#ZeroFluxPlane

:ZeroFluxPlane rdf:type owl:Class ;
               
               rdfs:subClassOf <http://www.nist.gov/itl/ssd/OntologyRequirements.owl#PlanarRegion> ;
               
               rdfs:seeAlso "Definitions of terms for diffusion in the solid state (IUPAC Recommendations 1999), Pure Appl. Chem. 71, 1307-1325."@en ;
               
               rdfs:comment "In multicomponent diffusion-couple experiments the fluxes of individual components may go to zero at specific locations along the axis of the couple. These locations are called Zero Flux Planes."@en ;
               
               <http://www.nist.gov/itl/ssd/OntologyRequirements.owl#termString> "zero flux plane"@en .



###  http://www.nist.gov/itl/ssd/Materials.owl#ZincAlloy

:ZincAlloy rdf:type owl:Class ;
           
           rdfs:subClassOf :NonFerrousAlloy ,
                           [ rdf:type owl:Restriction ;
                             owl:onProperty :physicalDecompositions ;
                             owl:someValuesFrom bc:Zinc
                           ] ;
           
           or:referenceURL "http://www.matweb.com/index.aspx"^^xsd:anyURI ;
           
           rdfs:comment "An alloy that contains Zinc but not Iron."@en .



###  http://www.nist.gov/itl/ssd/Materials.owl#ZincOxide

:ZincOxide rdf:type owl:Class ;
           
           rdfs:subClassOf bc:Oxide ;
           
           <http://www.nist.gov/itl/ssd/OntologyRequirements.owl#termString> "zinc oxide"@en .



###  http://www.nist.gov/itl/ssd/Materials.owl#ZincOxideLubricant

:ZincOxideLubricant rdf:type owl:Class ;
                    
                    rdfs:subClassOf :FluidLubricant ;
                    
                    or:referenceURL "http://www.matweb.com/index.aspx"^^xsd:anyURI ;
                    
                    rdfs:comment "Zinc Oxide Lubricant is an artificial lubricant with Zinc Oxide as a gellant."@en ;
                    
                    <http://www.nist.gov/itl/ssd/OntologyRequirements.owl#termString> "zinc oxide lubricant"@en .



###  http://www.nist.gov/itl/ssd/Materials.owl#ZirconiumOxide

:ZirconiumOxide rdf:type owl:Class ;
                
                rdfs:subClassOf bc:Oxide ;
                
                or:referenceURL "http://www.matweb.com/index.aspx"^^xsd:anyURI ;
                
                <http://www.nist.gov/itl/ssd/OntologyRequirements.owl#termString> "zirconium oxide"@en .



###  http://www.nist.gov/itl/ssd/OntologyRequirements#Algorithm

or:Algorithm rdf:type owl:Class .



###  http://www.nist.gov/itl/ssd/OntologyRequirements#ApplicationProgram

or:ApplicationProgram rdf:type owl:Class .



###  http://www.nist.gov/itl/ssd/OntologyRequirements#Area

or:Area rdfs:subClassOf [ rdf:type owl:Restriction ;
                          owl:onProperty or:unitsFor ;
                          owl:allValuesFrom or:UnitOfArea
                        ] .



###  http://www.nist.gov/itl/ssd/OntologyRequirements#AreaChart

or:AreaChart rdf:type owl:Class .



###  http://www.nist.gov/itl/ssd/OntologyRequirements#Artifact




###  http://www.nist.gov/itl/ssd/OntologyRequirements#Certifying

or:Certifying rdf:type owl:Class .



###  http://www.nist.gov/itl/ssd/OntologyRequirements#ComputerImageFile

or:ComputerImageFile rdf:type owl:Class .



###  http://www.nist.gov/itl/ssd/OntologyRequirements#ComputerStorageCapacity

or:ComputerStorageCapacity owl:disjointWith or:Energy ,
                                            or:Force ,
                                            or:Pressure .



###  http://www.nist.gov/itl/ssd/OntologyRequirements#CreationEvent

or:CreationEvent rdf:type owl:Class .



###  http://www.nist.gov/itl/ssd/OntologyRequirements#CurrencyUnit




###  http://www.nist.gov/itl/ssd/OntologyRequirements#CurveSegment

or:CurveSegment rdf:type owl:Class .



###  http://www.nist.gov/itl/ssd/OntologyRequirements#DataCollection

or:DataCollection rdf:type owl:Class .



###  http://www.nist.gov/itl/ssd/OntologyRequirements#DataTable

or:DataTable rdf:type owl:Class .



###  http://www.nist.gov/itl/ssd/OntologyRequirements#DatabaseSearch

or:DatabaseSearch rdf:type owl:Class .



###  http://www.nist.gov/itl/ssd/OntologyRequirements#DeployingAProduct

or:DeployingAProduct rdf:type owl:Class .



###  http://www.nist.gov/itl/ssd/OntologyRequirements#Design

or:Design rdf:type owl:Class .



###  http://www.nist.gov/itl/ssd/OntologyRequirements#Designing

or:Designing rdf:type owl:Class ;
             
             owl:disjointWith or:Development .



###  http://www.nist.gov/itl/ssd/OntologyRequirements#Development




###  http://www.nist.gov/itl/ssd/OntologyRequirements#Distance

or:Distance owl:disjointWith or:Energy ,
                             or:Force ,
                             or:Pressure .



###  http://www.nist.gov/itl/ssd/OntologyRequirements#Duration

or:Duration owl:disjointWith or:Energy ,
                             or:Force ,
                             or:Pressure .



###  http://www.nist.gov/itl/ssd/OntologyRequirements#Energy

or:Energy rdf:type owl:Class ;
          
          owl:disjointWith or:Force ,
                           or:Mass ,
                           or:Pressure ,
                           or:Temperature ,
                           or:Volume .



###  http://www.nist.gov/itl/ssd/OntologyRequirements#Evaluation

or:Evaluation rdf:type owl:Class .



###  http://www.nist.gov/itl/ssd/OntologyRequirements#EventType

or:EventType rdf:type owl:Class .



###  http://www.nist.gov/itl/ssd/OntologyRequirements#ExperimentPlanning

or:ExperimentPlanning rdf:type owl:Class ;
                      
                      rdfs:subClassOf [ rdf:type owl:Restriction ;
                                        owl:onProperty or:outputCreated ;
                                        owl:someValuesFrom ex:Experiment
                                      ] .



###  http://www.nist.gov/itl/ssd/OntologyRequirements#ExpressedQuantity

or:ExpressedQuantity rdf:type owl:Class ;
                     
                     rdfs:subClassOf [ rdf:type owl:Restriction ;
                                       owl:onProperty or:unitsFor ;
                                       owl:onClass or:UnitOfMeasure ;
                                       owl:qualifiedCardinality "1"^^xsd:nonNegativeInteger
                                     ] .



###  http://www.nist.gov/itl/ssd/OntologyRequirements#Force

or:Force rdf:type owl:Class ;
         
         owl:disjointWith or:Mass ,
                          or:Pressure ,
                          or:Temperature ,
                          or:Volume .



###  http://www.nist.gov/itl/ssd/OntologyRequirements#GovernmentalOrganization

or:GovernmentalOrganization rdf:type owl:Class .



###  http://www.nist.gov/itl/ssd/OntologyRequirements#GraphicalImage

or:GraphicalImage rdf:type owl:Class ;
                  
                  rdfs:subClassOf or:Information .



###  http://www.nist.gov/itl/ssd/OntologyRequirements#Manufacturing

or:Manufacturing rdf:type owl:Class .



###  http://www.nist.gov/itl/ssd/OntologyRequirements#Mass

or:Mass owl:disjointWith or:Pressure .



###  http://www.nist.gov/itl/ssd/OntologyRequirements#MechanicalProcess

or:MechanicalProcess rdf:type owl:Class .



###  http://www.nist.gov/itl/ssd/OntologyRequirements#NonTangibleThing

or:NonTangibleThing rdfs:subClassOf owl:Thing .



###  http://www.nist.gov/itl/ssd/OntologyRequirements#PredictionMethod

or:PredictionMethod rdf:type owl:Class .



###  http://www.nist.gov/itl/ssd/OntologyRequirements#Pressure

or:Pressure owl:disjointWith or:Temperature ,
                             or:Volume .



###  http://www.nist.gov/itl/ssd/OntologyRequirements#PurposefulAction




###  http://www.nist.gov/itl/ssd/OntologyRequirements#Quantity

or:Quantity rdf:type owl:Class ;
            
            <http://www.w3.org/2004/02/skos/core#note> "Similar to \"Property\" in Ashino's 2010 Minerals Ontology."@en .



###  http://www.nist.gov/itl/ssd/OntologyRequirements#Recommending

or:Recommending rdf:type owl:Class .



###  http://www.nist.gov/itl/ssd/OntologyRequirements#ResearchOrganization

or:ResearchOrganization rdf:type owl:Class .



###  http://www.nist.gov/itl/ssd/OntologyRequirements#SimulationModel

or:SimulationModel rdf:type owl:Class .



###  http://www.nist.gov/itl/ssd/OntologyRequirements#Software

or:Software rdf:type owl:Class .



###  http://www.nist.gov/itl/ssd/OntologyRequirements#StateOfBeing

or:StateOfBeing rdf:type owl:Class .



###  http://www.nist.gov/itl/ssd/OntologyRequirements#Technique

or:Technique rdf:type owl:Class .



###  http://www.nist.gov/itl/ssd/OntologyRequirements#Temperature




###  http://www.nist.gov/itl/ssd/OntologyRequirements#UnitOfAcceleration




###  http://www.nist.gov/itl/ssd/OntologyRequirements#UnitOfArea

or:UnitOfArea owl:disjointWith or:UnitOfDensity ,
                               or:UnitOfSpreadRate .



###  http://www.nist.gov/itl/ssd/OntologyRequirements#UnitOfComputerStorageCapacity

or:UnitOfComputerStorageCapacity owl:disjointWith or:UnitOfDensity ,
                                                  or:UnitOfVoltage ,
                                                  or:UnitOfVolume .



###  http://www.nist.gov/itl/ssd/OntologyRequirements#UnitOfDensity

or:UnitOfDensity owl:disjointWith or:UnitOfDistance ,
                                  or:UnitOfDuration .



###  http://www.nist.gov/itl/ssd/OntologyRequirements#UnitOfDistance




###  http://www.nist.gov/itl/ssd/OntologyRequirements#UnitOfDuration




###  http://www.nist.gov/itl/ssd/OntologyRequirements#UnitOfEnergy




###  http://www.nist.gov/itl/ssd/OntologyRequirements#UnitOfForce

or:UnitOfForce rdfs:comment "A Unit Of Force is a Unit Of Measure for measuring force.  It is the product of Unit Of Mass times a Unit Of Acceleration. The SI unit is the Newton."@en .



###  http://www.nist.gov/itl/ssd/OntologyRequirements#UnitOfMass




###  http://www.nist.gov/itl/ssd/OntologyRequirements#UnitOfPressure




###  http://www.nist.gov/itl/ssd/OntologyRequirements#UnitOfSpreadRate

or:UnitOfSpreadRate owl:disjointWith or:UnitOfTemperature ,
                                     or:UnitOfVelocity ,
                                     or:UnitOfVoltage ,
                                     or:UnitOfVolume ,
                                     <http://www.nist.gov/itl/ssd/OntologyRequirements.owl#UnitOfVelocitySquared> .



###  http://www.nist.gov/itl/ssd/OntologyRequirements#UnitOfTemperature

or:UnitOfTemperature owl:disjointWith or:UnitOfVolume ;
                     
                     rdfs:comment "A Unit of Temperature is a Unit of Measure used for specifying the temperature of something.  Two different Units of Temperatures may have the same magnitude, but different offsets, so are not the same.  A Degree Celsius is different from a Degree Kelvin, for example since 100 C = 373.15 K."@en .



###  http://www.nist.gov/itl/ssd/OntologyRequirements#UnitOfVelocity




###  http://www.nist.gov/itl/ssd/OntologyRequirements#UnitOfVoltage




###  http://www.nist.gov/itl/ssd/OntologyRequirements#UnitOfVolume




###  http://www.nist.gov/itl/ssd/OntologyRequirements#Volume




###  http://www.nist.gov/itl/ssd/OntologyRequirements.owl#DimensionlessUnit




###  http://www.nist.gov/itl/ssd/OntologyRequirements.owl#UnitOfVelocitySquared






#################################################################
#
#    Individuals
#
#################################################################


###  http://www.nist.gov/itl/ssd/Biochem#Actinium

bc:Actinium rdf:type owl:NamedIndividual .



###  http://www.nist.gov/itl/ssd/Biochem#Aluminum

bc:Aluminum rdf:type owl:NamedIndividual .



###  http://www.nist.gov/itl/ssd/Biochem#Americium

bc:Americium rdf:type owl:NamedIndividual .



###  http://www.nist.gov/itl/ssd/Biochem#Antimony

bc:Antimony rdf:type owl:NamedIndividual .



###  http://www.nist.gov/itl/ssd/Biochem#Argon

bc:Argon rdf:type owl:NamedIndividual .



###  http://www.nist.gov/itl/ssd/Biochem#Arsenic

bc:Arsenic rdf:type owl:NamedIndividual .



###  http://www.nist.gov/itl/ssd/Biochem#Astatine

bc:Astatine rdf:type owl:NamedIndividual .



###  http://www.nist.gov/itl/ssd/Biochem#Barium

bc:Barium rdf:type owl:NamedIndividual .



###  http://www.nist.gov/itl/ssd/Biochem#Berkelium

bc:Berkelium rdf:type owl:NamedIndividual .



###  http://www.nist.gov/itl/ssd/Biochem#Beryllium

bc:Beryllium rdf:type owl:NamedIndividual .



###  http://www.nist.gov/itl/ssd/Biochem#Bismuth

bc:Bismuth rdf:type owl:NamedIndividual .



###  http://www.nist.gov/itl/ssd/Biochem#Bohrium

bc:Bohrium rdf:type owl:NamedIndividual .



###  http://www.nist.gov/itl/ssd/Biochem#Boron

bc:Boron rdf:type owl:NamedIndividual .



###  http://www.nist.gov/itl/ssd/Biochem#Bromine

bc:Bromine rdf:type owl:NamedIndividual .



###  http://www.nist.gov/itl/ssd/Biochem#Cadmium

bc:Cadmium rdf:type owl:NamedIndividual .



###  http://www.nist.gov/itl/ssd/Biochem#Calcium

bc:Calcium rdf:type owl:NamedIndividual .



###  http://www.nist.gov/itl/ssd/Biochem#Californium

bc:Californium rdf:type owl:NamedIndividual .



###  http://www.nist.gov/itl/ssd/Biochem#Carbon

bc:Carbon rdf:type owl:NamedIndividual .



###  http://www.nist.gov/itl/ssd/Biochem#CcsPerLiter

bc:CcsPerLiter rdf:type <http://www.nist.gov/itl/ssd/OntologyRequirements.owl#DimensionlessUnit> ,
                        <http://www.nist.gov/itl/ssd/OntologyRequirements.owl#MetricUnit> .



###  http://www.nist.gov/itl/ssd/Biochem#Cerium

bc:Cerium rdf:type owl:NamedIndividual .



###  http://www.nist.gov/itl/ssd/Biochem#Cesium

bc:Cesium rdf:type owl:NamedIndividual .



###  http://www.nist.gov/itl/ssd/Biochem#Chlorine

bc:Chlorine rdf:type owl:NamedIndividual .



###  http://www.nist.gov/itl/ssd/Biochem#Chromium

bc:Chromium rdf:type owl:NamedIndividual .



###  http://www.nist.gov/itl/ssd/Biochem#Cobalt

bc:Cobalt rdf:type owl:NamedIndividual .



###  http://www.nist.gov/itl/ssd/Biochem#ConcentrationByMass

bc:ConcentrationByMass or:unitTypeFor bc:UnitOfConcentrationByMass .



###  http://www.nist.gov/itl/ssd/Biochem#ConcentrationByVolume

bc:ConcentrationByVolume or:unitTypeFor bc:UnitOfConcentrationByVolume .



###  http://www.nist.gov/itl/ssd/Biochem#Copernicium

bc:Copernicium rdf:type owl:NamedIndividual .



###  http://www.nist.gov/itl/ssd/Biochem#Copper

bc:Copper rdf:type owl:NamedIndividual .



###  http://www.nist.gov/itl/ssd/Biochem#Curium

bc:Curium rdf:type owl:NamedIndividual .



###  http://www.nist.gov/itl/ssd/Biochem#Dubnium

bc:Dubnium rdf:type owl:NamedIndividual .



###  http://www.nist.gov/itl/ssd/Biochem#Dysprosium

bc:Dysprosium rdf:type owl:NamedIndividual .



###  http://www.nist.gov/itl/ssd/Biochem#Einsteinium

bc:Einsteinium rdf:type owl:NamedIndividual .



###  http://www.nist.gov/itl/ssd/Biochem#Erbium

bc:Erbium rdf:type owl:NamedIndividual .



###  http://www.nist.gov/itl/ssd/Biochem#Europium

bc:Europium rdf:type owl:NamedIndividual .



###  http://www.nist.gov/itl/ssd/Biochem#Fermium

bc:Fermium rdf:type owl:NamedIndividual .



###  http://www.nist.gov/itl/ssd/Biochem#Fluorine

bc:Fluorine rdf:type owl:NamedIndividual .



###  http://www.nist.gov/itl/ssd/Biochem#Francium

bc:Francium rdf:type owl:NamedIndividual .



###  http://www.nist.gov/itl/ssd/Biochem#Germanium

bc:Germanium rdf:type owl:NamedIndividual .



###  http://www.nist.gov/itl/ssd/Biochem#Gold

bc:Gold rdf:type owl:NamedIndividual .



###  http://www.nist.gov/itl/ssd/Biochem#GramsPerLiter

bc:GramsPerLiter rdf:type <http://www.nist.gov/itl/ssd/OntologyRequirements.owl#MetricUnit> .



###  http://www.nist.gov/itl/ssd/Biochem#Hafnium

bc:Hafnium rdf:type owl:NamedIndividual .



###  http://www.nist.gov/itl/ssd/Biochem#Hassium

bc:Hassium rdf:type owl:NamedIndividual .



###  http://www.nist.gov/itl/ssd/Biochem#Helium

bc:Helium rdf:type owl:NamedIndividual .



###  http://www.nist.gov/itl/ssd/Biochem#Holmium

bc:Holmium rdf:type owl:NamedIndividual .



###  http://www.nist.gov/itl/ssd/Biochem#Hydrogen

bc:Hydrogen rdf:type owl:NamedIndividual .



###  http://www.nist.gov/itl/ssd/Biochem#Indium

bc:Indium rdf:type owl:NamedIndividual .



###  http://www.nist.gov/itl/ssd/Biochem#Iodine

bc:Iodine rdf:type owl:NamedIndividual .



###  http://www.nist.gov/itl/ssd/Biochem#Iridium

bc:Iridium rdf:type owl:NamedIndividual .



###  http://www.nist.gov/itl/ssd/Biochem#Iron

bc:Iron rdf:type owl:NamedIndividual .



###  http://www.nist.gov/itl/ssd/Biochem#Krypton

bc:Krypton rdf:type owl:NamedIndividual .



###  http://www.nist.gov/itl/ssd/Biochem#Lanthanum

bc:Lanthanum rdf:type owl:NamedIndividual .



###  http://www.nist.gov/itl/ssd/Biochem#Lawrencium

bc:Lawrencium rdf:type owl:NamedIndividual .



###  http://www.nist.gov/itl/ssd/Biochem#Lead

bc:Lead rdf:type owl:NamedIndividual .



###  http://www.nist.gov/itl/ssd/Biochem#Lithium

bc:Lithium rdf:type owl:NamedIndividual .



###  http://www.nist.gov/itl/ssd/Biochem#Lutetium

bc:Lutetium rdf:type owl:NamedIndividual .



###  http://www.nist.gov/itl/ssd/Biochem#Magnesium

bc:Magnesium rdf:type owl:NamedIndividual .



###  http://www.nist.gov/itl/ssd/Biochem#Manganese

bc:Manganese rdf:type owl:NamedIndividual .



###  http://www.nist.gov/itl/ssd/Biochem#Meitnerium

bc:Meitnerium rdf:type owl:NamedIndividual .



###  http://www.nist.gov/itl/ssd/Biochem#Mendelevium

bc:Mendelevium rdf:type owl:NamedIndividual .



###  http://www.nist.gov/itl/ssd/Biochem#Mercury

bc:Mercury rdf:type owl:NamedIndividual .



###  http://www.nist.gov/itl/ssd/Biochem#Molybdenum

bc:Molybdenum rdf:type owl:NamedIndividual .



###  http://www.nist.gov/itl/ssd/Biochem#Neodymium

bc:Neodymium rdf:type owl:NamedIndividual .



###  http://www.nist.gov/itl/ssd/Biochem#Neon

bc:Neon rdf:type owl:NamedIndividual .



###  http://www.nist.gov/itl/ssd/Biochem#Neptunium

bc:Neptunium rdf:type owl:NamedIndividual .



###  http://www.nist.gov/itl/ssd/Biochem#Nickel

bc:Nickel rdf:type owl:NamedIndividual .



###  http://www.nist.gov/itl/ssd/Biochem#Niobium

bc:Niobium rdf:type owl:NamedIndividual .



###  http://www.nist.gov/itl/ssd/Biochem#Nitrogen

bc:Nitrogen rdf:type owl:NamedIndividual .



###  http://www.nist.gov/itl/ssd/Biochem#Nobelium

bc:Nobelium rdf:type owl:NamedIndividual .



###  http://www.nist.gov/itl/ssd/Biochem#Osmium

bc:Osmium rdf:type owl:NamedIndividual .



###  http://www.nist.gov/itl/ssd/Biochem#Oxide

bc:Oxide rdf:type owl:NamedIndividual .



###  http://www.nist.gov/itl/ssd/Biochem#Oxygen

bc:Oxygen rdf:type owl:NamedIndividual .



###  http://www.nist.gov/itl/ssd/Biochem#Palladium

bc:Palladium rdf:type owl:NamedIndividual .



###  http://www.nist.gov/itl/ssd/Biochem#PercentByVolume

bc:PercentByVolume rdf:type <http://www.nist.gov/itl/ssd/OntologyRequirements.owl#DimensionlessUnit> .



###  http://www.nist.gov/itl/ssd/Biochem#Phosphorus

bc:Phosphorus rdf:type owl:NamedIndividual .



###  http://www.nist.gov/itl/ssd/Biochem#Platinum

bc:Platinum rdf:type owl:NamedIndividual .



###  http://www.nist.gov/itl/ssd/Biochem#Plutonium

bc:Plutonium rdf:type owl:NamedIndividual .



###  http://www.nist.gov/itl/ssd/Biochem#Polonium

bc:Polonium rdf:type owl:NamedIndividual .



###  http://www.nist.gov/itl/ssd/Biochem#Potassium

bc:Potassium rdf:type owl:NamedIndividual .



###  http://www.nist.gov/itl/ssd/Biochem#Praseodymium

bc:Praseodymium rdf:type owl:NamedIndividual .



###  http://www.nist.gov/itl/ssd/Biochem#Promethium

bc:Promethium rdf:type owl:NamedIndividual .



###  http://www.nist.gov/itl/ssd/Biochem#Protactinium

bc:Protactinium rdf:type owl:NamedIndividual .



###  http://www.nist.gov/itl/ssd/Biochem#Radium

bc:Radium rdf:type owl:NamedIndividual .



###  http://www.nist.gov/itl/ssd/Biochem#Radon

bc:Radon rdf:type owl:NamedIndividual .



###  http://www.nist.gov/itl/ssd/Biochem#Rhenium

bc:Rhenium rdf:type owl:NamedIndividual .



###  http://www.nist.gov/itl/ssd/Biochem#Rhodium

bc:Rhodium rdf:type owl:NamedIndividual .



###  http://www.nist.gov/itl/ssd/Biochem#Samarium

bc:Samarium rdf:type owl:NamedIndividual .



###  http://www.nist.gov/itl/ssd/Biochem#Scandium

bc:Scandium rdf:type owl:NamedIndividual .



###  http://www.nist.gov/itl/ssd/Biochem#Seaborgium

bc:Seaborgium rdf:type owl:NamedIndividual .



###  http://www.nist.gov/itl/ssd/Biochem#Selenium

bc:Selenium rdf:type owl:NamedIndividual .



###  http://www.nist.gov/itl/ssd/Biochem#Silicon

bc:Silicon rdf:type owl:NamedIndividual .



###  http://www.nist.gov/itl/ssd/Biochem#Silver

bc:Silver rdf:type owl:NamedIndividual .



###  http://www.nist.gov/itl/ssd/Biochem#Sodium

bc:Sodium rdf:type owl:NamedIndividual .



###  http://www.nist.gov/itl/ssd/Biochem#Strontium

bc:Strontium rdf:type owl:NamedIndividual .



###  http://www.nist.gov/itl/ssd/Biochem#Sulfur

bc:Sulfur rdf:type owl:NamedIndividual .



###  http://www.nist.gov/itl/ssd/Biochem#Tantalum

bc:Tantalum rdf:type owl:NamedIndividual .



###  http://www.nist.gov/itl/ssd/Biochem#Technetium

bc:Technetium rdf:type owl:NamedIndividual .



###  http://www.nist.gov/itl/ssd/Biochem#Tellurium

bc:Tellurium rdf:type owl:NamedIndividual .



###  http://www.nist.gov/itl/ssd/Biochem#Terbium

bc:Terbium rdf:type owl:NamedIndividual .



###  http://www.nist.gov/itl/ssd/Biochem#Thallium

bc:Thallium rdf:type owl:NamedIndividual .



###  http://www.nist.gov/itl/ssd/Biochem#Thorium

bc:Thorium rdf:type owl:NamedIndividual .



###  http://www.nist.gov/itl/ssd/Biochem#Thulium

bc:Thulium rdf:type owl:NamedIndividual .



###  http://www.nist.gov/itl/ssd/Biochem#Tin

bc:Tin rdf:type owl:NamedIndividual .



###  http://www.nist.gov/itl/ssd/Biochem#Titanium

bc:Titanium rdf:type owl:NamedIndividual .



###  http://www.nist.gov/itl/ssd/Biochem#Uranium

bc:Uranium rdf:type owl:NamedIndividual .



###  http://www.nist.gov/itl/ssd/Biochem#Vanadium

bc:Vanadium rdf:type owl:NamedIndividual .



###  http://www.nist.gov/itl/ssd/Biochem#Water

bc:Water rdf:type owl:NamedIndividual .



###  http://www.nist.gov/itl/ssd/Biochem#Xenon

bc:Xenon rdf:type owl:NamedIndividual .



###  http://www.nist.gov/itl/ssd/Biochem#Ytterbium

bc:Ytterbium rdf:type owl:NamedIndividual .



###  http://www.nist.gov/itl/ssd/Biochem#Yttrium

bc:Yttrium rdf:type owl:NamedIndividual .



###  http://www.nist.gov/itl/ssd/Biochem#Zinc

bc:Zinc rdf:type owl:NamedIndividual .



###  http://www.nist.gov/itl/ssd/Biochem#Zirconium

bc:Zirconium rdf:type owl:NamedIndividual .



###  http://www.nist.gov/itl/ssd/Materials.owl#ActivationVolumeForDiffusion

:ActivationVolumeForDiffusion rdf:type :DiffusionProperty ,
                                       owl:NamedIndividual ;
                              
                              rdfs:seeAlso "Definitions of terms for diffusion in the solid state (IUPAC Recommendations 1999), Pure Appl. Chem. 71, 1307-1325."@en ;
                              
                              rdfs:comment "The Activiation Volume for Diffusion is a parameter for a diffusiive system "@en ;
                              
                              or:unitTypeFor or:UnitOfVolume .



###  http://www.nist.gov/itl/ssd/Materials.owl#Activity_Chemical

:Activity_Chemical rdf:type bc:MeasurableChemicalProperty ,
                            owl:NamedIndividual ;
                   
                   rdfs:comment "In chemical thermodynamics, activity (symbol a) is a measure of the 'effective concentration' of a species in a mixture, meaning that the species's chemical potential depends on the activity of a real solution in the same way that it would depend on concentration for an ideal solution."@en ;
                   
                   or:unitTypeFor <http://www.nist.gov/itl/ssd/OntologyRequirements.owl#DimensionlessUnit> .



###  http://www.nist.gov/itl/ssd/Materials.owl#Alloy

:Alloy rdf:type :MaterialForm ,
                owl:NamedIndividual .



###  http://www.nist.gov/itl/ssd/Materials.owl#AluminumAlloy

:AluminumAlloy rdf:type :NonFerrousAlloyTypeByMainConstituent ,
                        owl:NamedIndividual ;
               
               or:referenceURL "http://www.matweb.com/index.aspx"^^xsd:anyURI ;
               
               rdfs:comment "An alloy that contains Aluminum but not Iron."@en ;
               
               bc:primaryConstituentType bc:Aluminum .



###  http://www.nist.gov/itl/ssd/Materials.owl#AluminumOxide

:AluminumOxide rdf:type bc:ChemicalSubstanceTypeByChemicalSpecies ,
                        owl:NamedIndividual ;
               
               or:referenceURL "http://www.matweb.com/index.aspx"^^xsd:anyURI ;
               
               <http://www.nist.gov/itl/ssd/OntologyRequirements.owl#termString> "aluminum oxide"@en .



###  http://www.nist.gov/itl/ssd/Materials.owl#AmorphousSubstance

:AmorphousSubstance rdf:type :MaterialForm ,
                             :MaterialPhaseComposition ,
                             owl:NamedIndividual ;
                    
                    rdfs:comment "Material in a solid amorphous (non-crystalline) phase."@en .



###  http://www.nist.gov/itl/ssd/Materials.owl#Ampere

:Ampere rdf:type :UnitOfElectricCurrent ,
                 <http://www.nist.gov/itl/ssd/OntologyRequirements.owl#SI_Unit> ,
                 owl:NamedIndividual .



###  http://www.nist.gov/itl/ssd/Materials.owl#AreaOfSurface

:AreaOfSurface rdf:type :MeasurableMechanicalProperty ,
                        owl:NamedIndividual ;
               
               or:unitTypeFor or:UnitOfArea .



###  http://www.nist.gov/itl/ssd/Materials.owl#AreaPerTime

:AreaPerTime rdf:type or:MeasurableQuantityType ,
                      owl:NamedIndividual .



###  http://www.nist.gov/itl/ssd/Materials.owl#Auricupride

:Auricupride rdf:type :AlloyType ,
                      :MineralType ,
                      owl:NamedIndividual ;
             
             :strunzClassification "01.AA.10a"^^xsd:string ;
             
             rdfs:comment "Auricupride is a natural alloy that combines copper and gold. Its chemical formula is Cu3Au. The alloy crystallizes in the Cubic crystal system and occurs as malleable grains or platey masses. It is an opaque yellow with a reddish tint. It has a hardness of 3.5 and a specific gravity of 11.5."@en ;
             
             bc:componentElement bc:Copper ;
             
             bc:primaryConstituentType bc:Copper ;
             
             bc:componentElement bc:Gold .



###  http://www.nist.gov/itl/ssd/Materials.owl#BTUperFtHourFahrenheit

:BTUperFtHourFahrenheit rdf:type :UnitOfThermalConductivity ,
                                 <http://www.nist.gov/itl/ssd/OntologyRequirements.owl#NonMetricUnit> ,
                                 owl:NamedIndividual .



###  http://www.nist.gov/itl/ssd/Materials.owl#BodyCenteredCubicCrystalStructure

:BodyCenteredCubicCrystalStructure rdf:type :CrystalStructure ,
                                            owl:NamedIndividual ;
                                   
                                   or:nickName "bcc" .



###  http://www.nist.gov/itl/ssd/Materials.owl#Brass

:Brass rdf:type :AlloyType ,
                owl:NamedIndividual ;
       
       rdfs:comment "Brass is an alloy of copper and zinc; the proportions of zinc and copper can be varied to create a range of brasses with varying properties.  Other metals (lead, tin, aluminum, nickel, traces of iron) may be added in specific proportions for specific brass alloys."@en ;
       
       bc:primaryConstituentType bc:Copper ;
       
       bc:componentElement bc:Copper ,
                           bc:Zinc .



###  http://www.nist.gov/itl/ssd/Materials.owl#BreakdownPotential

:BreakdownPotential rdf:type :DielectricProperty ,
                             owl:NamedIndividual .



###  http://www.nist.gov/itl/ssd/Materials.owl#BrinellHardness

:BrinellHardness rdf:type :IndentationHardness ,
                          owl:NamedIndividual .



###  http://www.nist.gov/itl/ssd/Materials.owl#Bronze

:Bronze rdf:type :AlloyType ,
                 owl:NamedIndividual ;
        
        rdfs:comment "Bronze is a metal alloy consisting primarily of copper, usually with tin as the main additive. There are many different bronze alloys but modern bronze is typically 88% copper and 12% tin.  Bronzes with the secondary additive other than tin or zinc include Aluminum Bronze and Silicon Bronze.  Phosphor Bronze is a Brass (main additive is zinc) with a significant amount of Phosphor (up to 1%) as an additional additive."@en ;
        
        bc:primaryConstituentType bc:Copper ;
        
        bc:componentElement bc:Copper ,
                            bc:Tin .



###  http://www.nist.gov/itl/ssd/Materials.owl#BulkDensity

:BulkDensity rdf:type :MeasurableMechanicalProperty ,
                      owl:NamedIndividual ;
             
             rdfs:comment "Bulk density is a property of powders, granules and other particulate matter. It is defined as the mass of the particles of the material divided by the total volume they occupy. The total volume includes particle volume, inter-particle void volume and internal pore volume."@en ;
             
             or:unitTypeFor or:UnitOfDensity .



###  http://www.nist.gov/itl/ssd/Materials.owl#BulkModulus

:BulkModulus rdf:type :ElasticModulus ,
                      :Stiffness ,
                      owl:NamedIndividual ;
             
             rdfs:comment "The Bulk Modulus is the inverse of the Isothermal Compressibility."@en ,
                          "bulk modulus" ;
             
             or:unitTypeFor or:UnitOfPressure .



###  http://www.nist.gov/itl/ssd/Materials.owl#BulkModulusPressureDerivitive

:BulkModulusPressureDerivitive rdf:type :DeformationProperty ,
                                        owl:NamedIndividual .



###  http://www.nist.gov/itl/ssd/Materials.owl#CALAPHAD

:CALAPHAD rdf:type or:PredictionMethod ,
                   owl:NamedIndividual ;
          
          rdfs:comment "CALPHAD is a method for the CALculation of PHAse Diagrams of multi-phase mixtures such as alloys."@en .



###  http://www.nist.gov/itl/ssd/Materials.owl#CastAlloy

:CastAlloy rdf:type :AlloyTypeByFormingProcess ,
                    owl:NamedIndividual ;
           
           rdfs:comment "A Cast Alloy is one which is formed by pouring molten metal into a mold and letting it harden."@en .



###  http://www.nist.gov/itl/ssd/Materials.owl#Casting_MaterialProcessing

:Casting_MaterialProcessing rdf:type owl:NamedIndividual .



###  http://www.nist.gov/itl/ssd/Materials.owl#CelsiusDegree

:CelsiusDegree rdf:type :UnitOfTemperatureDifference ,
                        owl:NamedIndividual ;
               
               rdfs:comment "A Celsius Degree is the Unit Of Temperature Difference equal to the differerence between zero and one Degrees Celsius or zero and one Degrees Kelvin.   A Celsius Degree has the same magnitude as a Kelvin degree.  A Fahrenheit Degree is 5/9 of a Celsius Degree."@en ;
               
               <http://www.nist.gov/itl/ssd/OntologyRequirements.owl#termString> "Celsius degree"@en ,
                                                                                 "Kelvin degree"@en .



###  http://www.nist.gov/itl/ssd/Materials.owl#ChannelDieCompression

:ChannelDieCompression rdf:type owl:NamedIndividual .



###  http://www.nist.gov/itl/ssd/Materials.owl#ChemicalDiffusionCoefficient

:ChemicalDiffusionCoefficient rdf:type bc:MeasurableChemicalProperty ,
                                       :DiffusionProperty ,
                                       owl:NamedIndividual ;
                              
                              rdfs:seeAlso "Definitions of terms for diffusion in the solid state (IUPAC Recommendations 1999), Pure Appl. Chem. 71, 1307-1325."@en ;
                              
                              or:unitTypeFor :AreaPerTime .



###  http://www.nist.gov/itl/ssd/Materials.owl#ChemicalPotential

:ChemicalPotential rdf:type bc:MeasurableChemicalProperty ,
                            owl:NamedIndividual ;
                   
                   rdfs:comment "The chemical potential of a species in a mixture can be defined as the ratio of the free energy of the mixture to the amount of that species in the mixture (usually calculated in moles).  Electrons in solids have a similar chemical potential, being the change in free energy when electrons are added or removed from the system. In the case of electrons, the chemical potential is usually expressed in energy per particle rather than energy per mole"@en ;
                   
                   <http://www.nist.gov/itl/ssd/OntologyRequirements.owl#termString> "chemical potential"@en ,
                                                                                     "partial molar free energy"@en .



###  http://www.nist.gov/itl/ssd/Materials.owl#Coating

:Coating rdf:type owl:NamedIndividual .



###  http://www.nist.gov/itl/ssd/Materials.owl#CobaltAlloy

:CobaltAlloy rdf:type :NonFerrousAlloyTypeByMainConstituent ,
                      owl:NamedIndividual ;
             
             or:referenceURL "http://www.matweb.com/index.aspx"^^xsd:anyURI ;
             
             rdfs:comment "An alloy that contains Cobalt but not Iron."@en ;
             
             bc:primaryConstituentType bc:Cobalt .



###  http://www.nist.gov/itl/ssd/Materials.owl#ColinearInterstitialcyMechanism

:ColinearInterstitialcyMechanism rdf:type :DiffusionMovementMechanism ,
                                          owl:NamedIndividual ;
                                 
                                 rdfs:seeAlso "Definitions of terms for diffusion in the solid state (IUPAC Recommendations 1999), Pure Appl. Chem. 71, 1307-1325." ;
                                 
                                 rdfs:comment "The Collinear Iinterstitialcy Mechanism is an interstitialcy mechanism in which an interstitial atom and the lattice atom which it displaces move along the same straight line."@en .



###  http://www.nist.gov/itl/ssd/Materials.owl#CompactedPowderAlloy

:CompactedPowderAlloy rdf:type :AlloyTypeByFormingProcess ,
                               owl:NamedIndividual ;
                      
                      rdfs:comment "A Compacted Powder Alloy is produced by the  powder metallurgy process, generally consisting of four basic steps: (1) powder manufacture, (2) powder blending,(3) compacting, (4) either sintering or metal injection molding. "@en .



###  http://www.nist.gov/itl/ssd/Materials.owl#CompositeSubstance

:CompositeSubstance rdf:type :MaterialForm ,
                             owl:NamedIndividual .



###  http://www.nist.gov/itl/ssd/Materials.owl#CompressiveStrength

:CompressiveStrength rdf:type :DeformationProperty ,
                              owl:NamedIndividual ;
                     
                     rdfs:comment "Compressive strength is the capacity of a material or structure to withstand axially directed pushing forces before being crushed."@en ;
                     
                     <http://www.nist.gov/itl/ssd/OntologyRequirements.owl#termString> "compressive strength"@en ;
                     
                     or:unitTypeFor or:UnitOfPressure .



###  http://www.nist.gov/itl/ssd/Materials.owl#ConductivityDiffusionCoefficient

:ConductivityDiffusionCoefficient rdf:type :DiffusionProperty ,
                                           :ElectricalProperty ,
                                           owl:NamedIndividual ;
                                  
                                  rdfs:seeAlso "Definitions of terms for diffusion in the solid state (IUPAC Recommendations 1999), Pure Appl. Chem. 71, 1307-1325."@en ;
                                  
                                  rdfs:comment "The Conductivity Diffusion Coefficient of a mobile charged particle species (ion or electron) is derived from the measured partial electrical conductivity of that species by the Nernst-Einstein equation."@en ;
                                  
                                  or:unitTypeFor :AreaPerTime .



###  http://www.nist.gov/itl/ssd/Materials.owl#CopperAlloy

:CopperAlloy rdf:type :NonFerrousAlloyTypeByMainConstituent ,
                      owl:NamedIndividual ;
             
             or:referenceURL "http://www.matweb.com/index.aspx"^^xsd:anyURI ;
             
             rdfs:comment "An alloy that contains Copper but little or no Iron."@en ;
             
             bc:primaryConstituentType bc:Copper .



###  http://www.nist.gov/itl/ssd/Materials.owl#Coulomb

:Coulomb rdf:type :UnitOfCharge ,
                  <http://www.nist.gov/itl/ssd/OntologyRequirements.owl#SI_Unit> ,
                  owl:NamedIndividual .



###  http://www.nist.gov/itl/ssd/Materials.owl#Creep

:Creep rdf:type :DeformationProperty ,
                owl:NamedIndividual ;
       
       rdfs:comment "Creep is the tendency of a solid material to move slowly or deform (via Material Creep) permanently under the influence of stresses. "@en ;
       
       <http://www.nist.gov/itl/ssd/OntologyRequirements.owl#termString> "creep"@en .



###  http://www.nist.gov/itl/ssd/Materials.owl#CriticalDensity

:CriticalDensity rdf:type :MeasurableMechanicalProperty ,
                          owl:NamedIndividual ;
                 
                 or:unitTypeFor or:UnitOfDensity .



###  http://www.nist.gov/itl/ssd/Materials.owl#CriticalPressure

:CriticalPressure rdf:type :ThermalProperty ,
                           owl:NamedIndividual ;
                  
                  rdfs:comment "A critical point for a substance is defined as the  temperature (Critical Temperature) and  pressure (Critical Pressure) at which phase boundaries cease to exist."@en ;
                  
                  <http://www.nist.gov/itl/ssd/OntologyRequirements.owl#termString> "critical temperature"@en ;
                  
                  or:unitTypeFor or:UnitOfPressure .



###  http://www.nist.gov/itl/ssd/Materials.owl#CriticalTemperature

:CriticalTemperature rdf:type :ThermalProperty ,
                              owl:NamedIndividual ;
                     
                     rdfs:comment "A critical point for a substance is defined as the  temperature (Critical Temperature) and  pressure (Critical Pressure) at which phase boundaries cease to exist."@en ;
                     
                     <http://www.nist.gov/itl/ssd/OntologyRequirements.owl#termString> "critical temperature"@en ;
                     
                     or:unitTypeFor or:UnitOfTemperature .



###  http://www.nist.gov/itl/ssd/Materials.owl#CrowdionMechanism

:CrowdionMechanism rdf:type :DiffusionMovementMechanism ,
                            owl:NamedIndividual ;
                   
                   rdfs:comment "Definitions of terms for diffusion in the solid state (IUPAC Recommendations 1999), Pure Appl. Chem. 71, 1307-1325." ,
                                "The Crowdion Mechanismi is a hypothesized mechanism in which diffusion takes place by a co-operative movement of a group of atoms one of which is typically centred on an interstitial position with the others relaxed from their normal lattice sites to accommodate the additional ‘crowdion’."@en ;
                   
                   <http://www.w3.org/2004/02/skos/core#note> "There was a big scientific controversy over the question if crowdions actually exist as a metastable interstitial configuration in the seventies. This controversy has never been finally resolved; however, most researchers in the field believe that it does not exist."@en ;
                   
                   rdfs:seeAlso "http://www.tf.uni-kiel.de/matwis/amat/def_en/kap_1/advanced/t1_3_1.html"@en .



###  http://www.nist.gov/itl/ssd/Materials.owl#CrystallineSubstance

:CrystallineSubstance rdf:type :MaterialPhaseComposition ,
                               owl:NamedIndividual ;
                      
                      rdfs:comment "Material in a crystalline phase"@en .



###  http://www.nist.gov/itl/ssd/Materials.owl#DarkenEquation

:DarkenEquation rdf:type or:Equation ,
                         owl:NamedIndividual ;
                
                rdfs:seeAlso "Definitions of terms for diffusion in the solid state (IUPAC Recommendations 1999), Pure Appl. Chem. 71, 1307-1325."@en ;
                
                rdfs:comment "The Darken equation represents Fick's laws adapted to binary systems."@en .



###  http://www.nist.gov/itl/ssd/Materials.owl#DefectDiffusionCoefficient

:DefectDiffusionCoefficient rdf:type :DiffusionProperty ,
                                     owl:NamedIndividual ;
                            
                            rdfs:seeAlso "Definitions of terms for diffusion in the solid state (IUPAC Recommendations 1999), Pure Appl. Chem. 71, 1307-1325."@en ;
                            
                            rdfs:comment "In the case of diffusion via a vacancy mechanism, the diffusion coefficient associated with the movement of vacancies in the opposite direction to the movement of diffusing species is called the Vacancy Diffusion Coefficient.  The Defect Diffusion Coefficient covers not only the diffusion of vacancies, but also of other defects such as interstitials."@en ;
                            
                            <http://www.nist.gov/itl/ssd/OntologyRequirements.owl#termString> "defect diffusion coefficient"@en ;
                            
                            or:unitTypeFor :AreaPerTime .



###  http://www.nist.gov/itl/ssd/Materials.owl#DielectricConstant

:DielectricConstant rdf:type :DielectricProperty ,
                             owl:NamedIndividual .



###  http://www.nist.gov/itl/ssd/Materials.owl#DielectricStrength

:DielectricStrength rdf:type :DielectricProperty ,
                             owl:NamedIndividual ;
                    
                    rdfs:comment "Dielectric Strength is the maximum electric field strength that a material can withstand without breaking down.  This has slightly different meanings for insulators, dielectrics, and combinations of dielectrics and conductors."@en .



###  http://www.nist.gov/itl/ssd/Materials.owl#DiffusionCorrelationFactor

:DiffusionCorrelationFactor rdf:type :DiffusionProperty ,
                                     owl:NamedIndividual ;
                            
                            rdfs:seeAlso "Definitions of terms for diffusion in the solid state (IUPAC Recommendations 1999), Pure Appl. Chem. 71, 1307-1325."@en ;
                            
                            rdfs:comment "When the motion of a diffusing species is dependent on the presence of a defect on a neighbouring site, e.g. a tracer diffusing by a vacancy mechanism, the jumps of the diffusing species will not be random, but are correlated. The Diffusion Correlation Factor, f, is a measure of the deviation of the motion of the diffusing atoms from the random walk."@en ;
                            
                            or:unitTypeFor <http://www.nist.gov/itl/ssd/OntologyRequirements.owl#DimensionlessUnit> .



###  http://www.nist.gov/itl/ssd/Materials.owl#DiffusionFlux

:DiffusionFlux rdf:type :DiffusionProperty ,
                        owl:NamedIndividual ;
               
               rdfs:seeAlso "Definitions of terms for diffusion in the solid state (IUPAC Recommendations 1999), Pure Appl. Chem. 71, 1307-1325."@en ;
               
               rdfs:comment "The diffusion flux Ji gives the number of species i crossing a unit area, fixed relative to the local centre of mass, per unit of time."@en ;
               
               or:unitTypeFor :UnitOfInverseAreaPerTime .



###  http://www.nist.gov/itl/ssd/Materials.owl#DiffusionInducedGrainBoundaryMigration

:DiffusionInducedGrainBoundaryMigration rdf:type :DiffusionMovementMechanism ,
                                                 owl:NamedIndividual ;
                                        
                                        rdfs:seeAlso "Definitions of terms for diffusion in the solid state (IUPAC Recommendations 1999), Pure Appl. Chem. 71, 1307-1325." ;
                                        
                                        rdfs:comment "If a polycrystalline material undergoes an interdiffusion process, the grain boundaries move in a direction perpendicular to the diffusion flux.  As a result the concentrations in the regions swept by the boundaries change.  This is called ``Diffusion-Induced Grain boundary Migration'' (DIGM)."@en ;
                                        
                                        <http://www.nist.gov/itl/ssd/OntologyRequirements.owl#termString> "diffusion induced grain boundary migration"@en .



###  http://www.nist.gov/itl/ssd/Materials.owl#DiffusionJumpFrequency

:DiffusionJumpFrequency rdf:type :DiffusionProperty ,
                                 owl:NamedIndividual ;
                        
                        rdfs:seeAlso "Definitions of terms for diffusion in the solid state (IUPAC Recommendations 1999), Pure Appl. Chem. 71, 1307-1325." ;
                        
                        rdfs:comment "In Diffusion, the jump frequency of a particle i towards a given nearest-neighbour site is denoted by Gamma(i). The total Diffusion Jump Frequency, Gamma, denotes the average number of jumps of particles per unit time."@en ;
                        
                        <http://www.nist.gov/itl/ssd/OntologyRequirements.owl#termString> "diffusion jump frequency"@en ,
                                                                                          "jump frequency"@en ;
                        
                        or:unitTypeFor :UnitOfInverseTime .



###  http://www.nist.gov/itl/ssd/Materials.owl#DiffusionPath

:DiffusionPath rdf:type <http://www.nist.gov/itl/ssd/Document.n3#GenericScientificModel> ,
                        owl:NamedIndividual ;
               
               rdfs:seeAlso "Definitions of terms for diffusion in the solid state (IUPAC Recommendations 1999), Pure Appl. Chem. 71, 1307-1325."@en ;
               
               rdfs:comment "The sequence of structural and compositional modifications developed during isothermal diffusion in multiphase, multicomponent diffusion systems is called a Diffusion Path. This path is generally plotted superposed upon an isothermal phase diagram."@en .



###  http://www.nist.gov/itl/ssd/Materials.owl#DiffusionPotential

:DiffusionPotential rdf:type :DiffusionProperty ,
                             owl:NamedIndividual ;
                    
                    rdfs:seeAlso "Definitions of terms for diffusion in the solid state (IUPAC Recommendations 1999), Pure Appl. Chem. 71, 1307-1325."@en ;
                    
                    rdfs:comment "During diffusion of charged particles in ionic or electronic conducting solids an electrical charge is built up due to the differences in mobilities of the diffusing particles. The corresponding electrostatic potential, phi, is known as the Diffusion Potential."@en ;
                    
                    or:unitTypeFor or:UnitOfVoltage .



###  http://www.nist.gov/itl/ssd/Materials.owl#Diffusivity

:Diffusivity rdf:type :TransportProperty ,
                      owl:NamedIndividual ;
             
             rdfs:comment "Diffusivity is the ratio between the molar flux due to molecular diffusion and the gradient in the concentration of the species (or the driving force for diffusion).  Diffusivity is generally prescribed for a given pair of species in a given phase at a given temperature. For a multi-component system, it is prescribed for each pair of species in the system.  Diffusivity is measured in Area per unit time -- in SI, m^2/s."@en ;
             
             or:unitTypeFor :AreaPerTime .



###  http://www.nist.gov/itl/ssd/Materials.owl#DiffusivityTensor

:DiffusivityTensor rdf:type :DiffusionProperty ,
                            owl:NamedIndividual ;
                   
                   rdfs:seeAlso "Definitions of terms for diffusion in the solid state (IUPAC Recommendations 1999), Pure Appl. Chem. 71, 1307-1325."@en ;
                   
                   rdfs:comment "In an anisotropic crystal lattice the diffusion coefficient is generally direction dependent and has to be represented by a three-dimensional tensor with components Dij. Under these circumstances the diffusion coefficient is also called the ``Diffusivity Tensor or ``diffusion tensor''."@en .



###  http://www.nist.gov/itl/ssd/Materials.owl#DirectInterstitialMechanism

:DirectInterstitialMechanism rdf:type :DiffusionMovementMechanism ,
                                      owl:NamedIndividual ;
                             
                             rdfs:seeAlso "Definitions of terms for diffusion in the solid state (IUPAC Recommendations 1999), Pure Appl. Chem. 71, 1307-1325."@en ;
                             
                             rdfs:comment "In the Direct Interstitial Mechanism diffusion takes place by the direct migration of an interstitial species from one interstitial position to another."@en .



###  http://www.nist.gov/itl/ssd/Materials.owl#DistortedHexagonalCrystalStructure

:DistortedHexagonalCrystalStructure rdf:type :CrystalStructure ,
                                             owl:NamedIndividual .



###  http://www.nist.gov/itl/ssd/Materials.owl#DivacancyMechanism

:DivacancyMechanism rdf:type :DiffusionMovementMechanism ,
                             owl:NamedIndividual ;
                    
                    rdfs:seeAlso "Definitions of terms for diffusion in the solid state (IUPAC Recommendations 1999), Pure Appl. Chem. 71, 1307-1325."@en ;
                    
                    rdfs:comment "The Divacancy Mechanism is the diffusion process by which a crystal lattice vacancy pair is used by any constituent species of the material to effect diffusion."@en .



###  http://www.nist.gov/itl/ssd/Materials.owl#DollarUS

:DollarUS rdf:type or:PrimaryCurrencyUnit ,
                   owl:NamedIndividual .



###  http://www.nist.gov/itl/ssd/Materials.owl#DoubleHexagonalClosePackedCrystalStructure

:DoubleHexagonalClosePackedCrystalStructure rdf:type :CrystalStructure ,
                                                     owl:NamedIndividual .



###  http://www.nist.gov/itl/ssd/Materials.owl#DriftVelocity

:DriftVelocity rdf:type :DiffusionProperty ,
                        owl:NamedIndividual ;
               
               rdfs:seeAlso "Definitions of terms for diffusion in the solid state (IUPAC Recommendations 1999), Pure Appl. Chem. 71, 1307-1325." ;
               
               rdfs:comment "The application of a driving force gives atoms a greater than random probability of jumping in the direction of the gradient. Atoms are said to have an average Drift Velocity vF in that direction and contribute a term cvF to the diffusion flux."@en ;
               
               or:unitTypeFor or:UnitOfVelocity .



###  http://www.nist.gov/itl/ssd/Materials.owl#DumbellIntersticialcyMechanism

:DumbellIntersticialcyMechanism rdf:type :DiffusionMovementMechanism ,
                                         owl:NamedIndividual ;
                                
                                rdfs:seeAlso "Definitions of terms for diffusion in the solid state (IUPAC Recommendations 1999), Pure Appl. Chem. 71, 1307-1325."@en ;
                                
                                rdfs:comment "In some diffusion systems the equilibrium configuration during an interstitialcy jump consists of a dumbbell-like defect with each of the moving ions being displaced by an equal amount from the normal lattice position.  Diffusion taking place via such species is said to proceed by a Dumbbell Interstitialcy Mechanism."@en .



###  http://www.nist.gov/itl/ssd/Materials.owl#Dyne

:Dyne rdf:type or:UnitOfForce ,
               <http://www.nist.gov/itl/ssd/OntologyRequirements.owl#CGS_Unit> ,
               owl:NamedIndividual .



###  http://www.nist.gov/itl/ssd/Materials.owl#EffectiveDiffusionCoefficient

:EffectiveDiffusionCoefficient rdf:type :DiffusionProperty ,
                                        owl:NamedIndividual ;
                               
                               rdfs:seeAlso "Definitions of terms for diffusion in the solid state (IUPAC Recommendations 1999), Pure Appl. Chem. 71, 1307-1325."@en ;
                               
                               rdfs:comment "In alloys or compounds transport of material can occur under the influence of a driving force, at constant composition in the whole sample. Examples are found in viscous creep and sintering processes. In this case the fluxes of the diffusing species must be coupled. In an ionic crystal a similar condition holds due to the necessity of preserving electroneutrality.  The Effective Diffusion Coefficient is a weighted average of the diffusion coefficients of the various diffusing species to provide an overall measure of the diffusion rate."@en ;
                               
                               or:unitTypeFor :UnitOfAreaPerTime .



###  http://www.nist.gov/itl/ssd/Materials.owl#EinsteinSmoluchowskiEquation

:EinsteinSmoluchowskiEquation rdf:type or:Equation ,
                                       owl:NamedIndividual ;
                              
                              rdfs:seeAlso "Definitions of terms for diffusion in the solid state (IUPAC Recommendations 1999), Pure Appl. Chem. 71, 1307-1325."@en ;
                              
                              rdfs:comment "The Einstein-Smoluchowski Equation relates diffusivity to the mobility of particles in a substance and the temperature.  Specializations of this equation specify the mobility in terms of electrical or other parameters."@en .



###  http://www.nist.gov/itl/ssd/Materials.owl#ElasticModulus

:ElasticModulus rdf:type owl:NamedIndividual ;
                
                rdfs:comment "An elastic modulus is defined as the slope of its stress–strain curve of a substance within the range where the deformation is elastic.  Three varieties of this are Young's modulus, the sheer modulus, and the bulk modulus."@en ;
                
                or:unitTypeFor or:UnitOfPressure .



###  http://www.nist.gov/itl/ssd/Materials.owl#ElectrialResistivity

:ElectrialResistivity rdf:type or:MeasurableQuantityType ,
                               owl:NamedIndividual .



###  http://www.nist.gov/itl/ssd/Materials.owl#ElectricPolarizability

:ElectricPolarizability rdf:type :DielectricProperty ,
                                 or:MeasurableQuantityType ,
                                 owl:NamedIndividual ;
                        
                        rdfs:comment "Electric Polarizability is the tendency of a substance's charge distribution to be distorted from its normal shape by an external electric field.  It is specified by the material's relative permittivity (dielectric constant)."@en .



###  http://www.nist.gov/itl/ssd/Materials.owl#ElectricalConductivity

:ElectricalConductivity rdf:type :ElectricalProperty ,
                                 or:MeasurableQuantityType ,
                                 owl:NamedIndividual ;
                        
                        rdfs:comment """Electrical Conductivity is a measure of how easily electric current flows through a material. High conductivity indicates a material readily allows the movement of electric charge.  The  SI unit of electrical conductivity is siemens per metre (S/m).

The inverse of Electrical Conductivity is Electrical Resistivity."""@en ;
                        
                        <http://www.nist.gov/itl/ssd/OntologyRequirements.owl#termString> "electrical conductivity"@en ,
                                                                                          "specific conductance"@en ;
                        
                        or:unitTypeFor :UnitOfElectricalConductivity .



###  http://www.nist.gov/itl/ssd/Materials.owl#ElectricalDiffusionMobility

:ElectricalDiffusionMobility rdf:type :DiffusionProperty ,
                                      owl:NamedIndividual ;
                             
                             rdfs:seeAlso "Definitions of terms for diffusion in the solid state (IUPAC Recommendations 1999), Pure Appl. Chem. 71, 1307-1325." ;
                             
                             rdfs:comment "Mass transport of charged species due to electrical force is described as Electrical Mobility (or 'electrochemical mobility') and is calculated as the average drift velocity per unit of electrical field strength.  Note that this is different from the Species Diffusion Mobility that is a ration of the drift velocity to the force, not a field strength.  The electrical mobility is thus the species mobility devided by the absolute electrical charge on the species."@en ;
                             
                             <http://www.nist.gov/itl/ssd/OntologyRequirements.owl#termString> "electrical diffusion mobility"@en ,
                                                                                               "electrical mobility"@en ,
                                                                                               "electrochemical mobility"@en .



###  http://www.nist.gov/itl/ssd/Materials.owl#ElectricalPotential

:ElectricalPotential rdf:type :ElectricalProperty ,
                              owl:NamedIndividual ;
                     
                     rdfs:comment "Electrical Potential (``voltage\" or \"electric tension\"), is the difference in electric potential between two points — or the difference in electric potential energy of a unit test charge transported between two points. It is is equal to the work which would have to be done, per unit charge, against a static electric field to move the charge between two points.  It is measured in units of electric potential: volts (equal to joules per coulomb)."@en ;
                     
                     <http://www.nist.gov/itl/ssd/OntologyRequirements.owl#termString> "electrical potential"@en ,
                                                                                       "voltage"@en ;
                     
                     or:unitTypeFor or:Volt .



###  http://www.nist.gov/itl/ssd/Materials.owl#ElectricalResistivity

:ElectricalResistivity rdf:type :ElectricalProperty ,
                                owl:NamedIndividual ;
                       
                       rdfs:comment """Electrical Resistivity is a measure of how strongly a material opposes the flow of electric current. Low resistivity indicates a material readily allows the movement of electric charge. The SI unit of electrical resistivity is the ohm⋅metre (Ω⋅m).

Electrical Resistivity is the inverse of Electrical Conductivity."""@en ;
                       
                       <http://www.nist.gov/itl/ssd/OntologyRequirements.owl#termString> "electrical resistivity"@en ,
                                                                                         "resistivity"@en ,
                                                                                         "specific electrical resistance"@en ,
                                                                                         "volume resistivity"@en ;
                       
                       or:unitTypeFor :UnitOfElectricalResistivity .



###  http://www.nist.gov/itl/ssd/Materials.owl#Elongation

:Elongation rdf:type :DeformationProperty ,
                     owl:NamedIndividual ;
            
            rdfs:comment "Elongation is the ratio of the reference length of an object to its changed length, whether caused by external loads, gravitation, or thermal expansion/contraction."@en ;
            
            <http://www.nist.gov/itl/ssd/OntologyRequirements.owl#termString> "elongation"@en ;
            
            or:unitTypeFor <http://www.nist.gov/itl/ssd/OntologyRequirements.owl#DimensionlessUnit> .



###  http://www.nist.gov/itl/ssd/Materials.owl#EnergyPerMass

:EnergyPerMass rdf:type or:MeasurableQuantityType ,
                        owl:NamedIndividual ;
               
               rdfs:comment "Energy Per Mass is an amount of Energy divided by an amount of Mass.  It is used to specify the amount of energy that enters or leaves a system dependent upon the mass of the system that results in, or is caused by, some type of change."@en .



###  http://www.nist.gov/itl/ssd/Materials.owl#EnthalpyOfFormation

:EnthalpyOfFormation rdf:type :ThermochemicalProperty ,
                              owl:NamedIndividual ;
                     
                     rdfs:comment "The standard enthalpy of formation or standard heat of formation of a compound is the change of enthalpy that accompanies the formation of 1 mole of the compound from its elements, with all substances in their standard states."@en ;
                     
                     <http://www.nist.gov/itl/ssd/OntologyRequirements.owl#termString> "enthalpy of formation"@en ,
                                                                                       "heat of formation"@en ,
                                                                                       "standard enthalpy of formation"@en ,
                                                                                       "standard heat of formation"@en ;
                     
                     or:unitTypeFor or:UnitOfEnergy .



###  http://www.nist.gov/itl/ssd/Materials.owl#EnthalpyOfMixing

:EnthalpyOfMixing rdf:type :ThermalProperty ,
                           owl:NamedIndividual ;
                  
                  rdfs:comment "The enthalpy of mixing (or ``heat of mixing'') is the heat that is taken up or released upon mixing of two (non-reactive) chemical substances."@en ;
                  
                  <http://www.nist.gov/itl/ssd/OntologyRequirements.owl#termString> "enthalpy of mixing"@en ,
                                                                                    "heat of mixing"@en ;
                  
                  or:unitTypeFor or:UnitOfEnergy .



###  http://www.nist.gov/itl/ssd/Materials.owl#EnthalpyOfTransformation

:EnthalpyOfTransformation rdf:type :ThermalProperty ,
                                   owl:NamedIndividual ;
                          
                          <http://www.nist.gov/itl/ssd/OntologyRequirements.owl#termString> "Enthalpy of transformation is the heat released or absorbed by a body or a thermodynamic system during a phase transition such as the melting (Latent Heat of Fusion) or boiling (Latent Heat of Vaporization).  "@en ,
                                                                                            "enthalpy of transformation"@en ,
                                                                                            "latent heat"@en .



###  http://www.nist.gov/itl/ssd/Materials.owl#Euro

:Euro rdf:type or:PrimaryCurrencyUnit ,
               owl:NamedIndividual .



###  http://www.nist.gov/itl/ssd/Materials.owl#EuroCent

:EuroCent rdf:type or:SecondaryCurrencyUnit ,
                   owl:NamedIndividual .



###  http://www.nist.gov/itl/ssd/Materials.owl#ExchangeMechansimForDiffusion

:ExchangeMechansimForDiffusion rdf:type :DiffusionMovementMechanism ,
                                        owl:NamedIndividual .



###  http://www.nist.gov/itl/ssd/Materials.owl#Extruding

:Extruding rdf:type owl:NamedIndividual .



###  http://www.nist.gov/itl/ssd/Materials.owl#FaceCenteredCubicCrystalStructure

:FaceCenteredCubicCrystalStructure rdf:type :CrystalStructure ,
                                            owl:NamedIndividual ;
                                   
                                   or:nickName "fcc" .



###  http://www.nist.gov/itl/ssd/Materials.owl#FahrenheitDegree

:FahrenheitDegree rdf:type :UnitOfTemperatureDifference ,
                           owl:NamedIndividual ;
                  
                  rdfs:comment "A Fahrenheit Degree is the Unit Of Temperature Difference equal to the differerence between zero and one Degrees Fahrenheit.  A Fahrenheit Degree is 5/9 of a CelsiusDegree."@en ;
                  
                  <http://www.nist.gov/itl/ssd/OntologyRequirements.owl#termString> "Fahrenheight degree"@en .



###  http://www.nist.gov/itl/ssd/Materials.owl#Farad

:Farad rdf:type :UnitOfCapacitance ,
                <http://www.nist.gov/itl/ssd/OntologyRequirements.owl#SI_Unit> ,
                owl:NamedIndividual .



###  http://www.nist.gov/itl/ssd/Materials.owl#FatigueEnduranceLimit

:FatigueEnduranceLimit rdf:type :DeformationProperty ,
                                owl:NamedIndividual ;
                       
                       rdfs:comment "Fatigue endurance limit (fatigue limit, endurance limit,  fatigue strength) is the amplitude (or range) of cyclic stress that can be applied to the material without causing fatigue failure."@en ;
                       
                       <http://www.nist.gov/itl/ssd/OntologyRequirements.owl#termString> "endurance limit"@en ,
                                                                                         "fatigue endurance limit"@en ,
                                                                                         "fatigue limit"@en ,
                                                                                         "fatigue strength"@en ;
                       
                       or:unitTypeFor or:UnitOfPressure .



###  http://www.nist.gov/itl/ssd/Materials.owl#FerrousAlloy

:FerrousAlloy rdf:type :AlloyTypeByMainConstituent ,
                       owl:NamedIndividual ;
              
              or:referenceURL "http://www.matweb.com/index.aspx"^^xsd:anyURI ;
              
              rdfs:comment "A Ferrous Alloy is one that contains iron."@en ;
              
              <http://www.nist.gov/itl/ssd/OntologyRequirements.owl#termString> "ferrous alloy"@en ,
                                                                                "ferrous metal"@en ;
              
              bc:primaryConstituentType bc:Iron .



###  http://www.nist.gov/itl/ssd/Materials.owl#FicksFirstLawOfDiffusion

:FicksFirstLawOfDiffusion rdf:type <http://www.nist.gov/itl/ssd/Document.n3#GenericScientificModel> ,
                                   owl:NamedIndividual ;
                          
                          rdfs:seeAlso "Definitions of terms for diffusion in the solid state (IUPAC Recommendations 1999), Pure Appl. Chem. 71, 1307-1325."@en ;
                          
                          rdfs:comment "Fick’s First Law Of Diffusion states the relationship between the flux and the concentration gradient of a diffusing species."@en .



###  http://www.nist.gov/itl/ssd/Materials.owl#FicksSecondLawOfDiffusion

:FicksSecondLawOfDiffusion rdf:type <http://www.nist.gov/itl/ssd/Document.n3#GenericScientificModel> ,
                                    owl:NamedIndividual ;
                           
                           rdfs:seeAlso "Definitions of terms for diffusion in the solid state (IUPAC Recommendations 1999), Pure Appl. Chem. 71, 1307-1325."@en ;
                           
                           rdfs:comment "Fick’s Second Law Of Diffusion states the relationship between the concentration gradient of a species and the rate of change of its concentration (dc/dt) caused by its diffusion."@en .



###  http://www.nist.gov/itl/ssd/Materials.owl#FiveFrequencyDiffusionModel

:FiveFrequencyDiffusionModel rdf:type :DiffusionMovementMechanism ,
                                      owl:NamedIndividual ;
                             
                             rdfs:seeAlso "Definitions of terms for diffusion in the solid state (IUPAC Recommendations 1999), Pure Appl. Chem. 71, 1307-1325."@en ;
                             
                             rdfs:comment "The Five-Frequency Diffusion Model is a type of movement of impurity diffusion via monovacancies in face-centred-cubic (fcc) metals or on an fcc sublattice in ionic crystals. It is assumed that the only host atom jumps that differ from jumps in the pure lattice are those made by nearest neighbours of the impurity."@en .



###  http://www.nist.gov/itl/ssd/Materials.owl#Forging_MaterialProcessing

:Forging_MaterialProcessing rdf:type owl:NamedIndividual .



###  http://www.nist.gov/itl/ssd/Materials.owl#FractureToughness

:FractureToughness rdf:type :DeformationProperty ,
                            owl:NamedIndividual ;
                   
                   rdfs:comment "Fracture Toughness is a measure of a substance's ability to resist Fracturing."@en ;
                   
                   <http://www.nist.gov/itl/ssd/OntologyRequirements.owl#termString> "fracture toughness"@en ,
                                                                                     "toughness"@en ;
                   
                   or:unitTypeFor :UnitOfToughness .



###  http://www.nist.gov/itl/ssd/Materials.owl#Franklin

:Franklin rdf:type :UnitOfCharge ,
                   <http://www.nist.gov/itl/ssd/OntologyRequirements.owl#MetricUnit> ,
                   owl:NamedIndividual ;
          
          <http://www.nist.gov/itl/ssd/OntologyRequirements.owl#termString> "franklin"@en .



###  http://www.nist.gov/itl/ssd/Materials.owl#FreeElectronDensity

:FreeElectronDensity rdf:type :ElectricalProperty ,
                              or:MeasurableQuantityType ,
                              owl:NamedIndividual .



###  http://www.nist.gov/itl/ssd/Materials.owl#Gadolinium

:Gadolinium rdf:type owl:NamedIndividual .



###  http://www.nist.gov/itl/ssd/Materials.owl#Gallium

:Gallium rdf:type owl:NamedIndividual .



###  http://www.nist.gov/itl/ssd/Materials.owl#GaseousSubstance

:GaseousSubstance rdf:type :MaterialForm ,
                           :StateOfMatter ,
                           owl:NamedIndividual ;
                  
                  rdfs:comment "Material in a gasseous phase."@en .



###  http://www.nist.gov/itl/ssd/Materials.owl#GelSubstance

:GelSubstance rdf:type :MaterialPhaseComposition ,
                       owl:NamedIndividual ;
              
              rdfs:comment "Material in a gel phase."@en .



###  http://www.nist.gov/itl/ssd/Materials.owl#GlassTemperature

:GlassTemperature rdf:type :ThermalProperty ,
                           owl:NamedIndividual ;
                  
                  rdfs:comment "The Glass Temperature (``glass-liquid transition temperature'' or ``glass transition temperature'') is the reversible transition in amorphous materials (or in amorphous regions within semicrystalline materials) from a hard and relatively brittle state into a molten or rubber-like state."@en ;
                  
                  <http://www.nist.gov/itl/ssd/OntologyRequirements.owl#termString> "glass temperature"@en ,
                                                                                    "glass transition temperature"@en ,
                                                                                    "glass-liquid transition temperature"@en ;
                  
                  or:unitTypeFor or:UnitOfTemperature .



###  http://www.nist.gov/itl/ssd/Materials.owl#HeatCapacity

:HeatCapacity rdf:type :ThermalProperty ,
                       owl:NamedIndividual ;
              
              rdfs:comment "Heat capacity (thermal capacity) is the measurable physical quantity that characterizes the amount of heat required to change a substance's temperature by a given amount.  It is commonly expressed in expressed in units of joule(s) (J) per degree kelvin (K)." ;
              
              <http://www.nist.gov/itl/ssd/OntologyRequirements.owl#termString> "enthalpy difference"@en ,
                                                                                "heat capacity"@en ,
                                                                                "thermal capacity"@en ;
              
              or:unitTypeFor or:UnitOfEnergy .



###  http://www.nist.gov/itl/ssd/Materials.owl#HeatTreating

:HeatTreating rdf:type owl:NamedIndividual .



###  http://www.nist.gov/itl/ssd/Materials.owl#Henry

:Henry rdf:type :UnitOfInductance ,
                <http://www.nist.gov/itl/ssd/OntologyRequirements.owl#SI_Unit> ,
                owl:NamedIndividual .



###  http://www.nist.gov/itl/ssd/Materials.owl#HexagonalClosePackedCrystalStructure

:HexagonalClosePackedCrystalStructure rdf:type :CrystalStructure ,
                                               owl:NamedIndividual .



###  http://www.nist.gov/itl/ssd/Materials.owl#Hydroforming

:Hydroforming rdf:type owl:NamedIndividual .



###  http://www.nist.gov/itl/ssd/Materials.owl#IntrinsicDiffusionCoefficient

:IntrinsicDiffusionCoefficient rdf:type :DiffusionProperty ,
                                        owl:NamedIndividual ;
                               
                               rdfs:seeAlso "Definitions of terms for diffusion in the solid state (IUPAC Recommendations 1999), Pure Appl. Chem. 71, 1307-1325."@en ;
                               
                               rdfs:comment "In multicomponent diffusion, each individual component has its own Intrinsic Diffusion Coefficient."@en ;
                               
                               or:unitTypeFor :UnitOfAreaPerTime .



###  http://www.nist.gov/itl/ssd/Materials.owl#IntrinsicDiffusivity

:IntrinsicDiffusivity rdf:type :MeasurableMechanicalProperty ,
                               owl:NamedIndividual .



###  http://www.nist.gov/itl/ssd/Materials.owl#InverseDegreeCelsius

:InverseDegreeCelsius rdf:type :UnitOfInverseTemperatureDifference ,
                               <http://www.nist.gov/itl/ssd/OntologyRequirements.owl#MetricUnit> ,
                               owl:NamedIndividual ;
                      
                      <http://www.nist.gov/itl/ssd/OntologyRequirements.owl#termString> "1 / 1K" ,
                                                                                        "1 / 1C" ;
                      
                      rdfs:comment "An Inverse Degree Celsius is equal to 1/ (1 C)  ; equivalently 1/ (1 K) ."@en ;
                      
                      <http://www.nist.gov/itl/ssd/OntologyRequirements.owl#termString> "inverse Celsius degree"@en ,
                                                                                        "inverse kelvin degree"@en .



###  http://www.nist.gov/itl/ssd/Materials.owl#InverseMeterSquaredPerSecond

:InverseMeterSquaredPerSecond rdf:type :UnitOfInverseAreaPerTime ,
                                       <http://www.nist.gov/itl/ssd/OntologyRequirements.owl#MetricUnit> ,
                                       owl:NamedIndividual ;
                              
                              rdfs:comment "The unit, Inverse Meter Squared per Second equals 1 meter^-2 / second."@en .



###  http://www.nist.gov/itl/ssd/Materials.owl#InverseSecond

:InverseSecond rdf:type :UnitOfInverseTime ,
                        owl:NamedIndividual ;
               
               rdfs:comment "One Inverse Second = 1/second ."@en .



###  http://www.nist.gov/itl/ssd/Materials.owl#IonBeamSputtering

:IonBeamSputtering rdf:type owl:NamedIndividual .



###  http://www.nist.gov/itl/ssd/Materials.owl#IsothermalCompressibility

:IsothermalCompressibility rdf:type :Compressibility ,
                                    owl:NamedIndividual .



###  http://www.nist.gov/itl/ssd/Materials.owl#JoulePerKg

:JoulePerKg rdf:type :UnitOfEnergyPerMass ,
                     <http://www.nist.gov/itl/ssd/OntologyRequirements.owl#MetricUnit> ,
                     owl:NamedIndividual ;
            
            rdfs:comment "Joules per kilogram"@en .



###  http://www.nist.gov/itl/ssd/Materials.owl#JoulePerKgK

:JoulePerKgK rdf:type :UnitOfSpecificHeatCapacity ,
                      <http://www.nist.gov/itl/ssd/OntologyRequirements.owl#SI_Unit> ,
                      owl:NamedIndividual ;
             
             <http://www.nist.gov/itl/ssd/OntologyRequirements.owl#termString> "J/(kg*K)" ,
                                                                               "joule per kg - degree kelvin"@en .



###  http://www.nist.gov/itl/ssd/Materials.owl#KgPerM3

:KgPerM3 rdf:type or:UnitOfDensity ,
                  <http://www.nist.gov/itl/ssd/OntologyRequirements.owl#MetricUnit> ,
                  owl:NamedIndividual ;
         
         rdfs:comment "Kilograms per cubic meter"@en .



###  http://www.nist.gov/itl/ssd/Materials.owl#KirkendallVelocity

:KirkendallVelocity rdf:type :DiffusionProperty ,
                             owl:NamedIndividual ;
                    
                    rdfs:seeAlso "Definitions of terms for diffusion in the solid state (IUPAC Recommendations 1999), Pure Appl. Chem. 71, 1307-1325." ;
                    
                    <http://www.nist.gov/itl/ssd/OntologyRequirements.owl#termString> "Kirkendall velocity" ;
                    
                    rdfs:comment "The Kirkendall velocity is the velocity of the diffusion zone in a multicomponent system, relative to the fixed ends of the specimen. It results from the net nonzero flux of vacancies in the diffusion region."@en .



###  http://www.nist.gov/itl/ssd/Materials.owl#KsiSquareRootOfInch

:KsiSquareRootOfInch rdf:type :UnitOfToughness ,
                              <http://www.nist.gov/itl/ssd/OntologyRequirements.owl#NonMetricUnit> ,
                              owl:NamedIndividual ;
                     
                     <http://www.nist.gov/itl/ssd/OntologyRequirements.owl#termString> "ksi*(inch)^1/2" ;
                     
                     owl:sameAs :PascalSquareRootOfMeter .



###  http://www.nist.gov/itl/ssd/Materials.owl#LAMMPS

:LAMMPS rdf:type or:ApplicationProgram ,
                 owl:NamedIndividual ;
        
        rdfs:comment "LAMMPS (Large-scale Atomic/Molecular Massively Parallel Simulator) is an open-source molecular dynamics program from Sandia National Laboratories"@en .



###  http://www.nist.gov/itl/ssd/Materials.owl#Lapping

:Lapping rdf:type owl:NamedIndividual .



###  http://www.nist.gov/itl/ssd/Materials.owl#LatentHeatOfFusion

:LatentHeatOfFusion rdf:type :ThermalProperty ,
                             owl:NamedIndividual ;
                    
                    rdfs:comment "The latent heat of fusion (or ``enthalpy of fusion'') is the change in enthalpy resulting from heating one mole of a substance to change its state from a solid to a liquid."@en ;
                    
                    <http://www.nist.gov/itl/ssd/OntologyRequirements.owl#termString> "enthalpy of fusion"@en ,
                                                                                      "latent heat of fusion"@en ;
                    
                    or:unitTypeFor or:UnitOfEnergy .



###  http://www.nist.gov/itl/ssd/Materials.owl#LatentHeatOfVaporization

:LatentHeatOfVaporization rdf:type :ThermalProperty ,
                                   owl:NamedIndividual ;
                          
                          rdfs:comment "The latent heat of vaporization (or ``enthalpy of vaporization'' or ``heat of evaporation'') is the energy required to transform a given quantity of a substance from a liquid into a gas at a given pressure (often atmospheric pressure)."@en ;
                          
                          <http://www.nist.gov/itl/ssd/OntologyRequirements.owl#termString> "enthalpy of vaporization"@en ,
                                                                                            "heat of evaporation"@en ,
                                                                                            "heat of vaporization"@en ,
                                                                                            "latent heat of vaporization"@en ;
                          
                          or:unitTypeFor or:UnitOfEnergy .



###  http://www.nist.gov/itl/ssd/Materials.owl#LatheSectioning

:LatheSectioning rdf:type owl:NamedIndividual .



###  http://www.nist.gov/itl/ssd/Materials.owl#LeadAlloy

:LeadAlloy rdf:type :NonFerrousAlloyTypeByMainConstituent ,
                    owl:NamedIndividual ;
           
           or:referenceURL "http://www.matweb.com/index.aspx"^^xsd:anyURI ;
           
           rdfs:comment "An alloy that contains Lead but not Iron."@en ;
           
           bc:primaryConstituentType bc:Lead .



###  http://www.nist.gov/itl/ssd/Materials.owl#LinearCompressibility

:LinearCompressibility rdf:type :Compressibility ,
                                owl:NamedIndividual .



###  http://www.nist.gov/itl/ssd/Materials.owl#LiquidSubstance

:LiquidSubstance rdf:type :MaterialForm ,
                          :StateOfMatter ,
                          owl:NamedIndividual ;
                 
                 rdfs:comment "Material in a liquid phase."@en .



###  http://www.nist.gov/itl/ssd/Materials.owl#LiquidusTemperature

:LiquidusTemperature rdf:type :ThermalProperty ,
                              owl:NamedIndividual ;
                     
                     rdfs:comment "The liquidus temperature, TL or Tliq, is mostly used for glasses, alloys and rocks. It specifies the maximum temperature at which crystals can co-exist with liquid in thermodynamic equilibrium.  For a mixture the solidus temperature depends upon the relative concentration of the substances in the liquid   Above the liquidus temperature the material is homogeneous and liquid at equilibrium. Below the liquidus temperature  crystals form in the liquid.."@en .



###  http://www.nist.gov/itl/ssd/Materials.owl#LossCoefficient

:LossCoefficient rdf:type :DeformationProperty ,
                          owl:NamedIndividual ;
                 
                 rdfs:comment "The Loss Coefficient measures the degree to which a material dissipates vibrational energy.  It is the natural log of the ratio of successive amplitudes of vibration in the material."@en ;
                 
                 <http://www.nist.gov/itl/ssd/OntologyRequirements.owl#termString> "damping capacity"@en ,
                                                                                   "loss coefficient"@en ;
                 
                 or:unitTypeFor <http://www.nist.gov/itl/ssd/OntologyRequirements.owl#DimensionlessUnit> .



###  http://www.nist.gov/itl/ssd/Materials.owl#MagnesiumAlloy

:MagnesiumAlloy rdf:type :NonFerrousAlloyTypeByMainConstituent ,
                         owl:NamedIndividual ;
                
                or:referenceURL "http://www.matweb.com/index.aspx"^^xsd:anyURI ;
                
                rdfs:comment "An alloy that contains Magnesium but not Iron."@en ;
                
                bc:primaryConstituentType bc:Magnesium .



###  http://www.nist.gov/itl/ssd/Materials.owl#MagnesiumOxide

:MagnesiumOxide rdf:type bc:ChemicalSubstanceTypeByChemicalSpecies ,
                         owl:NamedIndividual ;
                
                or:referenceURL "http://www.matweb.com/index.aspx"^^xsd:anyURI ;
                
                <http://www.nist.gov/itl/ssd/OntologyRequirements.owl#termString> "magnesium oxide"@en .



###  http://www.nist.gov/itl/ssd/Materials.owl#MagneticMoment

:MagneticMoment rdf:type :MagneticProperty ,
                         owl:NamedIndividual .



###  http://www.nist.gov/itl/ssd/Materials.owl#MagneticPermeability

:MagneticPermeability rdf:type :MagneticProperty ,
                               owl:NamedIndividual ;
                      
                      rdfs:comment """Magnetic Permeability is the measure of the ability of a material to support the formation of a magnetic field within itself. In other words, it is the degree of magnetization that a material obtains in response to an applied magnetic field.  The reciprocal of magnetic permeability is magnetic reluctivity.

In SI units, permeability is measured in henrys per meter (H·m−1), or newtons per ampere squared (N·A−2)."""@en .



###  http://www.nist.gov/itl/ssd/Materials.owl#MagneticSuscepibility

:MagneticSuscepibility rdf:type :MagneticProperty ,
                                owl:NamedIndividual ;
                       
                       rdfs:comment "Magnetic Susceptibility is a dimensionless proportionality constant that indicates the degree of magnetization of a material in response to an applied magnetic field."@en .



###  http://www.nist.gov/itl/ssd/Materials.owl#MassOfObject

:MassOfObject rdf:type :MeasurableMechanicalProperty ,
                       owl:NamedIndividual ;
              
              or:unitTypeFor or:UnitOfMass .



###  http://www.nist.gov/itl/ssd/Materials.owl#MaterialSuspension

:MaterialSuspension rdf:type :MaterialForm ,
                             owl:NamedIndividual .



###  http://www.nist.gov/itl/ssd/Materials.owl#MaterialToughness

:MaterialToughness rdf:type :DeformationProperty ,
                            owl:NamedIndividual ;
                   
                   rdfs:comment "Material  Toughness is the ability of a material to absorb energy and plastically deform without fracturing.  It can be defined as the amount of energy per volume that a material can absorb before rupturing or as the resistance to fracture of a material when stressed."@en ;
                   
                   <http://www.nist.gov/itl/ssd/OntologyRequirements.owl#termString> "material toughness"@en ,
                                                                                     "toughness"@en .



###  http://www.nist.gov/itl/ssd/Materials.owl#MaximumServiceTemperature

:MaximumServiceTemperature rdf:type :ThermalProperty ,
                                    owl:NamedIndividual ;
                           
                           or:unitTypeFor or:UnitOfTemperature .



###  http://www.nist.gov/itl/ssd/Materials.owl#MechanicalStress

:MechanicalStress rdf:type :DeformationProperty ,
                           owl:NamedIndividual ;
                  
                  rdfs:comment "Stress is a measure of the internal forces acting within a deformable body. Quantitatively, it is a measure of the average force per unit area of a surface within the body on which internal forces which arise as a reaction to external forces applied to the body act."@en ;
                  
                  <http://www.nist.gov/itl/ssd/OntologyRequirements.owl#termString> "mechanical stress"@en ,
                                                                                    "stress"@en ;
                  
                  or:unitTypeFor or:UnitOfPressure .



###  http://www.nist.gov/itl/ssd/Materials.owl#MeltingPoint

:MeltingPoint rdf:type :ThermalProperty ,
                       owl:NamedIndividual ;
              
              or:unitTypeFor or:UnitOfTemperature .



###  http://www.nist.gov/itl/ssd/Materials.owl#MicrosectioningThroughAnodizing

:MicrosectioningThroughAnodizing rdf:type owl:NamedIndividual .



###  http://www.nist.gov/itl/ssd/Materials.owl#MicrosectioningThroughChemicalDissolution

:MicrosectioningThroughChemicalDissolution rdf:type owl:NamedIndividual .



###  http://www.nist.gov/itl/ssd/Materials.owl#MicrosectioningThroughSputtering

:MicrosectioningThroughSputtering rdf:type owl:NamedIndividual .



###  http://www.nist.gov/itl/ssd/Materials.owl#MicrotomeSectioning

:MicrotomeSectioning rdf:type owl:NamedIndividual .



###  http://www.nist.gov/itl/ssd/Materials.owl#MohsHardness

:MohsHardness rdf:type :ScratchHardness ,
                       owl:NamedIndividual ;
              
              rdfs:comment "The Mohs scale of mineral hardness characterizes the scratch resistance of various minerals through the ability of a harder material to scratch a softer material.  On the scale Talc is 1; Gypsum is 2; Calcite is 3; Fluorite is 4; Apatite is 5; Orthoclase Feldspar is 6; Quartz is 7; Topaz is 8; Corundum is 9; and Diamond is 10."@en .



###  http://www.nist.gov/itl/ssd/Materials.owl#Molality

:Molality rdf:type bc:Concentration ,
                   owl:NamedIndividual ;
          
          rdfs:comment "In chemistry, Molality of a solvent/solute combination is defined as the amount of solute, (in moles), divided by the mass of the solvent (in kg), (not the mass of the solution)."@en .



###  http://www.nist.gov/itl/ssd/Materials.owl#MolarHeatCapacity

:MolarHeatCapacity rdf:type :ThermalProperty ,
                            owl:NamedIndividual ;
                   
                   rdfs:comment "The Molar Heat Capacity is the heat capacity per unit mass of a material, measured in Joules/(mole K)  (in SI units). "@en .



###  http://www.nist.gov/itl/ssd/Materials.owl#Molarity

:Molarity rdf:type bc:Concentration ,
                   owl:NamedIndividual ;
          
          rdfs:comment "In chemistry, the Molarity (or molar concentration), is defined as the amount of a mixture constituent (in moles) divided by the volume of the mixture."@en .



###  http://www.nist.gov/itl/ssd/Materials.owl#MolybdenumAlloy

:MolybdenumAlloy rdf:type :NonFerrousAlloyTypeByMainConstituent ,
                          owl:NamedIndividual ;
                 
                 or:referenceURL "http://www.matweb.com/index.aspx"^^xsd:anyURI ;
                 
                 rdfs:comment "An alloy that contains Molybdenum but not Iron."@en ;
                 
                 bc:primaryConstituentType bc:Molybdenum .



###  http://www.nist.gov/itl/ssd/Materials.owl#MonoclinicCrystalStructure

:MonoclinicCrystalStructure rdf:type :CrystalStructure ,
                                     owl:NamedIndividual .



###  http://www.nist.gov/itl/ssd/Materials.owl#NernstPlanckEquation

:NernstPlanckEquation rdf:type or:Equation ,
                               owl:NamedIndividual ;
                      
                      rdfs:seeAlso "Definitions of terms for diffusion in the solid state (IUPAC Recommendations 1999), Pure Appl. Chem. 71, 1307-1325."@en ;
                      
                      rdfs:comment "For interdiffusion of two ionic crystals, the Nernst-Planck Equation expresses the relationsip between the intrinsic diffusion coefficients and the tracer diffusion coefficients depending on the mole fractio ns of the two constiuents.  This relation holds under that assumption that only the two specified components are moble, and that they diffuse on a common sublatice."@en .



###  http://www.nist.gov/itl/ssd/Materials.owl#NeumannsPrinciple

:NeumannsPrinciple rdf:type <http://www.nist.gov/itl/ssd/Document.n3#GenericScientificModel> ,
                            owl:NamedIndividual ;
                   
                   rdfs:seeAlso "Definitions of terms for diffusion in the solid state (IUPAC Recommendations 1999), Pure Appl. Chem. 71, 1307-1325."@en ;
                   
                   rdfs:comment "Neumann’s principle (also known as Curie principle or Curie–Neumann’s principle) states that if a coordinate transformation follows the symmetry operations of the crystalline lattice in question, then that transformation leaves the diffusivity tensor invariant."@en .



###  http://www.nist.gov/itl/ssd/Materials.owl#Newton

:Newton rdf:type or:UnitOfForce ,
                 <http://www.nist.gov/itl/ssd/OntologyRequirements.owl#SI_Unit> ,
                 owl:NamedIndividual .



###  http://www.nist.gov/itl/ssd/Materials.owl#NickelAlloy

:NickelAlloy rdf:type :NonFerrousAlloyTypeByMainConstituent ,
                      owl:NamedIndividual ;
             
             or:referenceURL "http://www.matweb.com/index.aspx"^^xsd:anyURI ;
             
             rdfs:comment "An alloy that contains Nickel but not Iron."@en ;
             
             bc:primaryConstituentType bc:Nickel .



###  http://www.nist.gov/itl/ssd/Materials.owl#NonFerrousAlloy

:NonFerrousAlloy rdf:type :AlloyTypeByMainConstituent ,
                          owl:NamedIndividual ;
                 
                 rdfs:comment "A non-ferrous alloy is one that does not contain iron."@en .
[ rdf:type owl:NegativePropertyAssertion ;
  owl:targetIndividual bc:Iron ;
  owl:assertionProperty bc:primaryConstituentType ;
  owl:sourceIndividual :NonFerrousAlloy
] .



###  http://www.nist.gov/itl/ssd/Materials.owl#Ohm

:Ohm rdf:type :UnitOfElectricalResistance ,
              <http://www.nist.gov/itl/ssd/OntologyRequirements.owl#SI_Unit> ,
              owl:NamedIndividual .



###  http://www.nist.gov/itl/ssd/Materials.owl#OhmMeter

:OhmMeter rdf:type :UnitOfElectricalResistivity ,
                   <http://www.nist.gov/itl/ssd/OntologyRequirements.owl#SI_Unit> ,
                   owl:NamedIndividual .



###  http://www.nist.gov/itl/ssd/Materials.owl#OnsagersGeneralizedDiffusionEquation

:OnsagersGeneralizedDiffusionEquation rdf:type or:Equation ,
                                               owl:NamedIndividual ;
                                      
                                      rdfs:seeAlso "Definitions of terms for diffusion in the solid state (IUPAC Recommendations 1999), Pure Appl. Chem. 71, 1307-1325."@en .



###  http://www.nist.gov/itl/ssd/Materials.owl#Opaque

:Opaque rdf:type :TransparencyLevel ,
                 owl:NamedIndividual .



###  http://www.nist.gov/itl/ssd/Materials.owl#OrthorhombicCrystalStructure

:OrthorhombicCrystalStructure rdf:type :CrystalStructure ,
                                       owl:NamedIndividual .



###  http://www.nist.gov/itl/ssd/Materials.owl#PascalSquareRootOfMeter

:PascalSquareRootOfMeter rdf:type :UnitOfToughness ,
                                  <http://www.nist.gov/itl/ssd/OntologyRequirements.owl#SI_Unit> ,
                                  owl:NamedIndividual ;
                         
                         <http://www.nist.gov/itl/ssd/OntologyRequirements.owl#termString> "Ps*(m)^1/2" ;
                         
                         rdfs:comment "This is equal to 1 Pa*(M)^1/2 ."@en .



###  http://www.nist.gov/itl/ssd/Materials.owl#PasteSubstance

:PasteSubstance rdf:type :MaterialPhaseComposition ,
                         owl:NamedIndividual ;
                
                rdfs:comment "A Paste is a substance that behaves as a solid until a sufficiently large load or stress is applied, at which point it flows like a fluid.  Pastes typically consist of a suspension of granular material in a background fluid.  Pastes are distinct from gels, whose particles interconnect."@en .



###  http://www.nist.gov/itl/ssd/Materials.owl#PoissonRatio

:PoissonRatio rdf:type :DeformationProperty ,
                       owl:NamedIndividual ;
              
              <http://www.nist.gov/itl/ssd/OntologyRequirements.owl#termString> "Poisson ratio"@en ;
              
              or:unitTypeFor "The Poisson Ratio of a material is the ratio, when an object composed of that material is stretched, of the transverse contraction or strain (perpendicular to the applied load), to the extension or axial strain in the direction of the applied load."@en ,
                             <http://www.nist.gov/itl/ssd/OntologyRequirements.owl#DimensionlessUnit> .



###  http://www.nist.gov/itl/ssd/Materials.owl#Polishing

:Polishing rdf:type owl:NamedIndividual .



###  http://www.nist.gov/itl/ssd/Materials.owl#PoundForce

:PoundForce rdf:type or:UnitOfForce ,
                     <http://www.nist.gov/itl/ssd/OntologyRequirements.owl#NonMetricUnit> ,
                     owl:NamedIndividual ;
            
            <http://www.nist.gov/itl/ssd/OntologyRequirements.owl#termString> "pound"@en .



###  http://www.nist.gov/itl/ssd/Materials.owl#PoundSterling

:PoundSterling rdf:type or:PrimaryCurrencyUnit ,
                        owl:NamedIndividual .



###  http://www.nist.gov/itl/ssd/Materials.owl#PowderySubstance

:PowderySubstance rdf:type :MaterialPhaseComposition ,
                           owl:NamedIndividual ;
                  
                  rdfs:comment "material in a solid powdery phase"@en .



###  http://www.nist.gov/itl/ssd/Materials.owl#PureSubstance

:PureSubstance rdf:type :MaterialForm ,
                        owl:NamedIndividual ;
               
               rdfs:comment "A Pure Substance is a substance made up of a single form of molecule, or in the case of a metal, a single type of atom.  This does not not mean that there may not be impurities."@en .



###  http://www.nist.gov/itl/ssd/Materials.owl#Quartz

:Quartz rdf:type :MineralType ,
                 owl:NamedIndividual ;
        
        rdfs:comment "Quartz is a common mineral of SiO4 with a hexagonal crystalline structure.  Impurities may color this otherwise colorless mineral."@en .



###  http://www.nist.gov/itl/ssd/Materials.owl#ReboundHardness

:ReboundHardness rdf:type :Hardness ,
                          owl:NamedIndividual .



###  http://www.nist.gov/itl/ssd/Materials.owl#RefractiveIndex

:RefractiveIndex rdf:type :OpticalProperty ,
                          owl:NamedIndividual ;
                 
                 or:unitTypeFor <http://www.nist.gov/itl/ssd/OntologyRequirements.owl#DimensionlessUnit> .



###  http://www.nist.gov/itl/ssd/Materials.owl#RelaxationMethodForDiffusion

:RelaxationMethodForDiffusion rdf:type :DiffusionMovementMechanism ,
                                       owl:NamedIndividual ;
                              
                              rdfs:seeAlso "Definitions of terms for diffusion in the solid state (IUPAC Recommendations 1999), Pure Appl. Chem. 71, 1307-1325."@en ;
                              
                              rdfs:comment "In the Relaxation Mechanism for diffusion, the atoms close to a vacancy relax to such an extent that the regular lattice structure out to several atom distances disappears and diffusion occurs by an irregular jostling motion similar to that for atoms in a liquid."@en .



###  http://www.nist.gov/itl/ssd/Materials.owl#RhombohedralCrystalStructure

:RhombohedralCrystalStructure rdf:type :CrystalStructure ,
                                       owl:NamedIndividual ;
                              
                              rdfs:comment """A lattice system is described by three basis vectors. In the rhombohedral system, the crystal is described by vectors of equal length, no two of which are orthogonal. The rhombohedral system can be thought of as the cubic system stretched along a body diagonal. a = b = c; α = β = γ ≠ 90°. In some classification schemes, the rhombohedral lattice system is combined with the hexagonal lattice system and grouped into a larger hexagonal family.

There is only one rhombohedral Bravais lattice."""@en .



###  http://www.nist.gov/itl/ssd/Materials.owl#Rinsing

:Rinsing rdf:type owl:NamedIndividual .



###  http://www.nist.gov/itl/ssd/Materials.owl#RockwellAHardness

:RockwellAHardness rdf:type :IndentationHardness ,
                            owl:NamedIndividual ;
                   
                   or:acronym "HRA" ;
                   
                   rdfs:comment "A Rockwell Hardness scale using a load of 60 kgf and a 120° diamond cone indenter."@en .



###  http://www.nist.gov/itl/ssd/Materials.owl#RockwellBHardness

:RockwellBHardness rdf:type :IndentationHardness ,
                            owl:NamedIndividual ;
                   
                   or:acronym "HRB" ;
                   
                   rdfs:comment "A Rockwell Hardness scale using a load of 100 kgf and a 1⁄8-inch-diameter (1.588 mm) steel sphere indenter."@en .



###  http://www.nist.gov/itl/ssd/Materials.owl#RockwellCHardness

:RockwellCHardness rdf:type :IndentationHardness ,
                            owl:NamedIndividual ;
                   
                   rdfs:comment "A Rockwell Hardness scale using a load of 150 kgf and a 120° diamond cone indenter."@en ;
                   
                   or:acronym "HRC" .



###  http://www.nist.gov/itl/ssd/Materials.owl#RockwellDHardness

:RockwellDHardness rdf:type :IndentationHardness ,
                            owl:NamedIndividual ;
                   
                   rdfs:comment "A Rockwell Hardness scale using a load of 100 kgf and a 120° diamond cone indenter."@en ;
                   
                   or:acronym "HRD" .



###  http://www.nist.gov/itl/ssd/Materials.owl#RockwellEHardness

:RockwellEHardness rdf:type :IndentationHardness ,
                            owl:NamedIndividual ;
                   
                   rdfs:comment "A Rockwell Hardness scale using a load of 100 kgf and a 1⁄8-inch-diameter (3.175 mm) steel sphere indenter."@en ;
                   
                   or:acronym "HRE" .



###  http://www.nist.gov/itl/ssd/Materials.owl#RockwellFHardness

:RockwellFHardness rdf:type :IndentationHardness ,
                            owl:NamedIndividual ;
                   
                   or:acronym "HRF" ;
                   
                   rdfs:comment "A Rockwell Hardness scale using a load of 60 kgf and a 1⁄16-inch-diameter (1.588 mm) steel sphere indenter."@en .



###  http://www.nist.gov/itl/ssd/Materials.owl#RockwellGHardness

:RockwellGHardness rdf:type :IndentationHardness ,
                            owl:NamedIndividual ;
                   
                   rdfs:comment "A Rockwell Hardness scale using a load of 150 kgf and a 1⁄16-inch-diameter (1.588 mm) steel sphere indenter."@en ;
                   
                   or:acronym "HRG" .



###  http://www.nist.gov/itl/ssd/Materials.owl#Rolling_MaterialProcessing

:Rolling_MaterialProcessing rdf:type owl:NamedIndividual .



###  http://www.nist.gov/itl/ssd/Materials.owl#Rubidium

:Rubidium rdf:type owl:NamedIndividual .



###  http://www.nist.gov/itl/ssd/Materials.owl#Ruthenium

:Ruthenium rdf:type owl:NamedIndividual .



###  http://www.nist.gov/itl/ssd/Materials.owl#Rutherfordium

:Rutherfordium rdf:type owl:NamedIndividual .



###  http://www.nist.gov/itl/ssd/Materials.owl#SandiaNationalLaboratories

:SandiaNationalLaboratories rdf:type or:ResearchOrganization ,
                                     owl:NamedIndividual .



###  http://www.nist.gov/itl/ssd/Materials.owl#SectioningByGrinding

:SectioningByGrinding rdf:type owl:NamedIndividual .



###  http://www.nist.gov/itl/ssd/Materials.owl#SelfDiffusionCoefficient

:SelfDiffusionCoefficient rdf:type :DiffusionProperty ,
                                   owl:NamedIndividual ;
                          
                          rdfs:seeAlso "Definitions of terms for diffusion in the solid state (IUPAC Recommendations 1999), Pure Appl. Chem. 71, 1307-1325." ,
                                       "IUPAC Gold Book, http://goldbook.iupac.org/S05582.html" ;
                          
                          rdfs:comment "The Self-Diffusion Coefficient is the diffusion coefficient Di^* of species i when the chemical potential gradient equals zero."@en ;
                          
                          <http://www.nist.gov/itl/ssd/OntologyRequirements.owl#termString> "self-diffusion coefficient"@en ;
                          
                          or:unitTypeFor :UnitOfAreaPerTime .



###  http://www.nist.gov/itl/ssd/Materials.owl#ShearModulus

:ShearModulus rdf:type :ElasticModulus ,
                       :Stiffness ,
                       owl:NamedIndividual ;
              
              rdfs:comment "The Shear Modulus (modulus of rigidity) describes a material's response to shearing strains. It is defined as the ratio of shear stress to the shear strain"@en ;
              
              <http://www.nist.gov/itl/ssd/OntologyRequirements.owl#termString> "modulus of rigidity"@en ;
              
              rdfs:comment "shear modulus"@en ;
              
              or:unitTypeFor or:UnitOfPressure .



###  http://www.nist.gov/itl/ssd/Materials.owl#SheetForming

:SheetForming rdf:type owl:NamedIndividual .



###  http://www.nist.gov/itl/ssd/Materials.owl#ShoreHardness

:ShoreHardness rdf:type :IndentationHardness ,
                        owl:NamedIndividual .



###  http://www.nist.gov/itl/ssd/Materials.owl#Siemens

:Siemens rdf:type :UnitOfElectricalConductance ,
                  <http://www.nist.gov/itl/ssd/OntologyRequirements.owl#SI_Unit> ,
                  owl:NamedIndividual ;
         
         rdfs:comment "The siemens (SI unit symbol: S) is the unit of electric conductance and electric admittance in the International System of Units (SI). Conductance and admittance are the reciprocals of resistance and impedance respectively, hence one siemens is equal to the reciprocal of one ohm, and is also referred to as the mho."@en ;
         
         <http://www.nist.gov/itl/ssd/OntologyRequirements.owl#termString> "mho"@en ,
                                                                           "siemens"@en .



###  http://www.nist.gov/itl/ssd/Materials.owl#SiemensPerMeter

:SiemensPerMeter rdf:type :UnitOfElectricalConductivity ,
                          <http://www.nist.gov/itl/ssd/OntologyRequirements.owl#SI_Unit> ,
                          owl:NamedIndividual .



###  http://www.nist.gov/itl/ssd/Materials.owl#SignificantDigits

:SignificantDigits rdf:type :UnitOfPrecision ,
                            <http://www.nist.gov/itl/ssd/OntologyRequirements.owl#NonMetricUnit> ,
                            owl:NamedIndividual .



###  http://www.nist.gov/itl/ssd/Materials.owl#SiliconOxide

:SiliconOxide rdf:type bc:ChemicalSubstanceTypeByChemicalSpecies ,
                       owl:NamedIndividual ;
              
              or:referenceURL "http://www.matweb.com/index.aspx"^^xsd:anyURI ;
              
              <http://www.nist.gov/itl/ssd/OntologyRequirements.owl#termString> "silicon oxide"@en .



###  http://www.nist.gov/itl/ssd/Materials.owl#Sintering

:Sintering rdf:type owl:NamedIndividual .



###  http://www.nist.gov/itl/ssd/Materials.owl#SolidCrystallineSubstance

:SolidCrystallineSubstance rdf:type :MaterialForm ,
                                    owl:NamedIndividual .



###  http://www.nist.gov/itl/ssd/Materials.owl#SolidSubstance

:SolidSubstance rdf:type :MaterialForm ,
                         :StateOfMatter ,
                         owl:NamedIndividual ;
                
                rdfs:comment "Material in a solid phase."@en .



###  http://www.nist.gov/itl/ssd/Materials.owl#SolidusTemperature

:SolidusTemperature rdf:type :ThermalProperty ,
                             owl:NamedIndividual ;
                    
                    rdfs:comment "The solidus temperature is the temperature (below which a given substance is completely solid and above which it it a mxture of a liquid of one composition and solid crystals of a different compostion."@en ;
                    
                    or:unitTypeFor or:UnitOfTemperature .



###  http://www.nist.gov/itl/ssd/Materials.owl#SoundVelocity

:SoundVelocity rdf:type :AcousticProperty ,
                        owl:NamedIndividual ;
               
               rdfs:comment "Sound Velocity for a substance depends on temperature and to a greater or lesser extent on frequency.  For a gas or vapor it depends on temperature and pressure. For a solid, there are two speeds of sound at the same temperature and frequency, that of a longitudinal (compression) wave, and that of a transverse wave.  In thin rods, the interaction of these two types of waves results in a third sound velocity intermediate between the transverse and longitudinal velocities."@en ;
               
               or:unitTypeFor or:UnitOfVelocity .



###  http://www.nist.gov/itl/ssd/Materials.owl#SpeciesDiffusionMobility

:SpeciesDiffusionMobility rdf:type :DiffusionProperty ,
                                   owl:NamedIndividual ;
                          
                          rdfs:seeAlso "Definitions of terms for diffusion in the solid state (IUPAC Recommendations 1999), Pure Appl. Chem. 71, 1307-1325." ;
                          
                          rdfs:comment "Mass transport in diffusion is described by the mobility of the diffusing species (`Species Diffusion Mobility' -- called `atomic mobility' if atoms are diffusing).  This mobility is equal to the drift velocity of the species divided by the force on the particles."@en ;
                          
                          <http://www.nist.gov/itl/ssd/OntologyRequirements.owl#termString> "atomic mobility"@en ,
                                                                                            "diffusion mobility"@en ,
                                                                                            "diffusion mobility of a species"@en ,
                                                                                            "mobility"@en ,
                                                                                            "species diffusion mobility"@en .



###  http://www.nist.gov/itl/ssd/Materials.owl#SpecificHeatCapacity

:SpecificHeatCapacity rdf:type :ThermalProperty ,
                               owl:NamedIndividual ;
                      
                      rdfs:comment "The Specific Heat Capacity (or specific heat) is the heat capacity per unit mass of a material, measured in Joules/(kg K)  (in SI units). "@en ;
                      
                      <http://www.nist.gov/itl/ssd/OntologyRequirements.owl#termString> "specific heat"@en ,
                                                                                        "specific heat capacity"@en ;
                      
                      or:unitTypeFor :UnitOfSpecificHeatCapacity .



###  http://www.nist.gov/itl/ssd/Materials.owl#SpecificStrength

:SpecificStrength rdf:type :DeformationProperty ,
                           owl:NamedIndividual ;
                  
                  rdfs:comment "The specific strength is a material's ultimate tensile strength (force per unit area at failure) divided by its density. It is also known as the strength-to-weight ratio or strength/weight ratio. The SI unit for specific strength is N·m/kg which is equivalent to (m/s)^2."@en ;
                  
                  or:unitTypeFor <http://www.nist.gov/itl/ssd/OntologyRequirements.owl#UnitOfVelocitySquared> .



###  http://www.nist.gov/itl/ssd/Materials.owl#SquareCmPerSecond

:SquareCmPerSecond rdf:type :UnitOfAreaPerTime ,
                            <http://www.nist.gov/itl/ssd/OntologyRequirements.owl#CGS_Unit> ,
                            owl:NamedIndividual .



###  http://www.nist.gov/itl/ssd/Materials.owl#SquareMeterPerSecond

:SquareMeterPerSecond rdf:type :UnitOfAreaPerTime ,
                               <http://www.nist.gov/itl/ssd/OntologyRequirements.owl#SI_Unit> ,
                               owl:NamedIndividual .



###  http://www.nist.gov/itl/ssd/Materials.owl#StressGradient

:StressGradient rdf:type :DeformationProperty ,
                         owl:NamedIndividual ;
                
                rdfs:seeAlso "Definitions of terms for diffusion in the solid state (IUPAC Recommendations 1999), Pure Appl. Chem. 71, 1307-1325." ;
                
                <http://www.nist.gov/itl/ssd/OntologyRequirements.owl#termString> "gradient of stress"@en ,
                                                                                  "stress gradient"@en .



###  http://www.nist.gov/itl/ssd/Materials.owl#TemperatureOfObject

:TemperatureOfObject rdf:type :ThermalProperty ,
                              owl:NamedIndividual ;
                     
                     rdfs:comment "The property ``Temperature Of Object'' specifies the temperature of some physical object.  The temperature can be expressed in Celcius or kelvins."@en ;
                     
                     or:unitTypeFor or:UnitOfTemperature .



###  http://www.nist.gov/itl/ssd/Materials.owl#TensileModulus

:TensileModulus rdf:type :ElasticModulus ,
                         :Stiffness ,
                         owl:NamedIndividual ;
                
                rdfs:comment "The Tensile Modulus (or Young's modulus) is a measure of the stiffness of an elastic material and is a quantity used to characterize materials. It is defined as the ratio of the uniaxial stress over the uniaxial strain in the range of stress in which Hooke's Law holds.["@en ;
                
                <http://www.nist.gov/itl/ssd/OntologyRequirements.owl#termString> "Young's modulus" ;
                
                rdfs:comment "tensile modulus"@en ;
                
                or:unitTypeFor or:UnitOfPressure .



###  http://www.nist.gov/itl/ssd/Materials.owl#TetragonalCrystalStructure

:TetragonalCrystalStructure rdf:type :CrystalStructure ,
                                     owl:NamedIndividual ;
                            
                            rdfs:comment """Tetragonal crystal lattices result from stretching a cubic lattice along one of its lattice vectors, so that the cube becomes a rectangular prism with a square base (a by a) and height (c, which is different from a).

There are two tetragonal Bravais lattices: the simple (or primitive) tetragonal (from stretching the simple-cubic lattice) and the body-centered tetragonal (from stretching either the face-centered or the body-centered cubic lattice)."""@en .



###  http://www.nist.gov/itl/ssd/Materials.owl#ThermalConductivity

:ThermalConductivity rdf:type :ThermalProperty ,
                              owl:NamedIndividual ;
                     
                     rdfs:comment "Thermal conductivity, (symbol: lambda or kappa), is the property of a material's ability to conduct heat, normally measured in W/(m·K)."@en ;
                     
                     <http://www.nist.gov/itl/ssd/OntologyRequirements.owl#termString> "thermal conductivity"@en ;
                     
                     or:unitTypeFor :UnitOfThermalConductivity .



###  http://www.nist.gov/itl/ssd/Materials.owl#ThermalExpansionCoefficient

:ThermalExpansionCoefficient rdf:type :ThermalProperty ,
                                      owl:NamedIndividual ;
                             
                             rdfs:comment "The Thermal Expansion Coefficient of a material is the relative amount it expands per unit increase in temperature.  In SI units it is measured in inverse Celsius degrees."@en ;
                             
                             or:unitTypeFor :UnitOfInverseTemperatureDifference .



###  http://www.nist.gov/itl/ssd/Materials.owl#ThermalShockResistance

:ThermalShockResistance rdf:type :ThermalProperty ,
                                 owl:NamedIndividual ;
                        
                        rdfs:comment "Thermal Shock Resistance is a measure of the resistance of an object to the initiation of thermal fracturing, measured as the maximum temperature difference to allow a steady heat flow."@en ;
                        
                        <http://www.nist.gov/itl/ssd/OntologyRequirements.owl#termString> "thermal shock resistance"@en ;
                        
                        or:unitTypeFor :UnitOfTemperatureDifference .



###  http://www.nist.gov/itl/ssd/Materials.owl#TinAlloy

:TinAlloy rdf:type :NonFerrousAlloyTypeByMainConstituent ,
                   owl:NamedIndividual ;
          
          or:referenceURL "http://www.matweb.com/index.aspx"^^xsd:anyURI ;
          
          rdfs:comment "An alloy that contains Tin but not Iron."@en ;
          
          bc:primaryConstituentType bc:Tin .



###  http://www.nist.gov/itl/ssd/Materials.owl#TitaniumOxide

:TitaniumOxide rdf:type bc:ChemicalSubstanceTypeByChemicalSpecies ,
                        owl:NamedIndividual ;
               
               or:referenceURL "http://www.matweb.com/index.aspx"^^xsd:anyURI ;
               
               <http://www.nist.gov/itl/ssd/OntologyRequirements.owl#termString> "titanium oxide"@en .



###  http://www.nist.gov/itl/ssd/Materials.owl#TracerDiffusionCoefficient

:TracerDiffusionCoefficient rdf:type :DiffusionProperty ,
                                     owl:NamedIndividual ;
                            
                            or:idString "Di*" ;
                            
                            rdfs:seeAlso "Definitions of terms for diffusion in the solid state (IUPAC Recommendations 1999), Pure Appl. Chem. 71, 1307-1325." ;
                            
                            rdfs:comment "The Tracer diffusion coefficient is the diffusion coefficient Di* as defined by Fick’s First law for an isotopically labeled atom. The term is usually restricted to the particular simple situation in which a tracer isotope in very dilute concentration is diffused into an otherwise homogeneous material with no driving forces other than the concentration gradient of the tracer itself."@en ;
                            
                            <http://www.nist.gov/itl/ssd/OntologyRequirements.owl#termString> "tracer diffusion coefficient"@en ;
                            
                            or:unitTypeFor :UnitOfAreaPerTime .



###  http://www.nist.gov/itl/ssd/Materials.owl#Translucent

:Translucent rdf:type :TransparencyLevel ,
                      owl:NamedIndividual .



###  http://www.nist.gov/itl/ssd/Materials.owl#Transparency

:Transparency rdf:type :OpticalProperty ,
                       owl:NamedIndividual .



###  http://www.nist.gov/itl/ssd/Materials.owl#Transparent

:Transparent rdf:type :TransparencyLevel ,
                      owl:NamedIndividual .



###  http://www.nist.gov/itl/ssd/Materials.owl#TriclinicCrystalStructure

:TriclinicCrystalStructure rdf:type :CrystalStructure ,
                                    owl:NamedIndividual ;
                           
                           rdfs:comment "The triclinic lattice is the least symmetric of the 14 three-dimensional Bravais lattices. It has (itself) the minimum symmetry all lattices have: points of inversion at each lattice point and at 7 more points for each lattice point: at the midpoints of the edges and the faces, and at the center points. It is the only lattice type that itself has no mirror planes."@en .



###  http://www.nist.gov/itl/ssd/Materials.owl#TrigonalCrystalStructure

:TrigonalCrystalStructure rdf:type :CrystalStructure ,
                                   owl:NamedIndividual ;
                          
                          rdfs:comment "The trigonal crystal system is the only crystal system whose point groups have more than one lattice system associated with their space groups: the hexagonal and rhombohedral lattices both appear."@en .



###  http://www.nist.gov/itl/ssd/Materials.owl#UKPenny

:UKPenny rdf:type or:SecondaryCurrencyUnit ,
                  owl:NamedIndividual .



###  http://www.nist.gov/itl/ssd/Materials.owl#USCent

:USCent rdf:type or:SecondaryCurrencyUnit ,
                 owl:NamedIndividual .



###  http://www.nist.gov/itl/ssd/Materials.owl#UltimateTensileStrength

:UltimateTensileStrength rdf:type :DeformationProperty ,
                                  owl:NamedIndividual ;
                         
                         or:unitTypeFor "Ultimate tensile strength (UTS), often shortened to tensile strength (TS) or ultimate strength, is the maximum stress that a material can withstand while being stretched or pulled before necking, which is when the specimen's cross-section starts to significantly contract. Tensile strength is the opposite of compressive strength and the values can be quite different."@en ;
                         
                         <http://www.nist.gov/itl/ssd/OntologyRequirements.owl#termString> "tensile strength"@en ;
                         
                         rdfs:comment "ultimate strength"@en ;
                         
                         <http://www.nist.gov/itl/ssd/OntologyRequirements.owl#termString> "ultimate tensile strength"@en ;
                         
                         or:unitTypeFor or:UnitOfPressure .



###  http://www.nist.gov/itl/ssd/Materials.owl#UnitOfAreaPerTime

:UnitOfAreaPerTime rdf:type or:InterconvertibleUnitType ,
                            owl:NamedIndividual .



###  http://www.nist.gov/itl/ssd/Materials.owl#UnitOfElectricalConductivity

:UnitOfElectricalConductivity rdf:type or:InterconvertibleUnitType ,
                                       owl:NamedIndividual .



###  http://www.nist.gov/itl/ssd/Materials.owl#UnitOfElectricalResistivity

:UnitOfElectricalResistivity rdf:type or:InterconvertibleUnitType ,
                                      owl:NamedIndividual .



###  http://www.nist.gov/itl/ssd/Materials.owl#UnitOfEnergyPerMass

:UnitOfEnergyPerMass rdf:type or:InterconvertibleUnitType ,
                              owl:NamedIndividual ;
                     
                     rdfs:comment "A Unit Of Energy Per Mass is a Unit Of Energy divided by a Unit Of Mass.  E.g., Joules per Gram."@en .



###  http://www.nist.gov/itl/ssd/Materials.owl#UnitOfEnergyPerTemperatureDifference

:UnitOfEnergyPerTemperatureDifference rdf:type or:InterconvertibleUnitType ,
                                               owl:NamedIndividual .



###  http://www.nist.gov/itl/ssd/Materials.owl#UnitOfHeatCapacityPerMass

:UnitOfHeatCapacityPerMass rdf:type or:InterconvertibleUnitType ,
                                    owl:NamedIndividual .



###  http://www.nist.gov/itl/ssd/Materials.owl#UnitOfInverseAreaPerTime

:UnitOfInverseAreaPerTime rdf:type or:InterconvertibleUnitType ,
                                   owl:NamedIndividual ;
                          
                          rdfs:comment "A Unit of Inverse Area per Time has the dimension of 1/ Area / Duration."@en .



###  http://www.nist.gov/itl/ssd/Materials.owl#UnitOfInverseTemperatureDifference

:UnitOfInverseTemperatureDifference rdf:type or:InterconvertibleUnitType ,
                                             owl:NamedIndividual .



###  http://www.nist.gov/itl/ssd/Materials.owl#UnitOfInverseTime

:UnitOfInverseTime rdf:type or:InterconvertibleUnitType ,
                            owl:NamedIndividual .



###  http://www.nist.gov/itl/ssd/Materials.owl#UnitOfPower

:UnitOfPower rdf:type or:InterconvertibleUnitType ,
                      owl:NamedIndividual .



###  http://www.nist.gov/itl/ssd/Materials.owl#UnitOfSpecificHeatCapacity

:UnitOfSpecificHeatCapacity rdf:type or:InterconvertibleUnitType ,
                                     owl:NamedIndividual .



###  http://www.nist.gov/itl/ssd/Materials.owl#UnitOfTemperatureDifference

:UnitOfTemperatureDifference rdf:type or:InterconvertibleUnitType ,
                                      owl:NamedIndividual ;
                             
                             rdfs:comment "A Unit of Temperature Difference is a Unit of Measure that indicates the differnce in temperature between two things.  A Celsius Degree and a Kelvin Degree have the same magnitude, and thus there is no difference between them as units of Temperature Difference."@en .



###  http://www.nist.gov/itl/ssd/Materials.owl#UnitOfThermalConductivity

:UnitOfThermalConductivity rdf:type or:InterconvertibleUnitType ,
                                    owl:NamedIndividual ;
                           
                           rdfs:comment "Units Of Thermal Conductivity have the dimension Mass * Distance / (Temperature * Duration^3) .  The SI unit is Watts/(m K)."@en .



###  http://www.nist.gov/itl/ssd/Materials.owl#UnitOfToughness

:UnitOfToughness rdf:type or:InterconvertibleUnitType ,
                          owl:NamedIndividual .



###  http://www.nist.gov/itl/ssd/Materials.owl#VacancyDiffusionCoefficient

:VacancyDiffusionCoefficient rdf:type :DiffusionProperty ,
                                      owl:NamedIndividual ;
                             
                             rdfs:seeAlso "Definitions of terms for diffusion in the solid state (IUPAC Recommendations 1999), Pure Appl. Chem. 71, 1307-1325." ;
                             
                             rdfs:comment "In the case of diffusion via a vacancy mechanism, the diffusion coefficient associated with the movement of vacancies in the opposite direction to the movement of diffusing species is called the Vacancy Diffusion Coefficient."@en ;
                             
                             <http://www.nist.gov/itl/ssd/OntologyRequirements.owl#termString> "vacancy diffusion coefficient"@en .



###  http://www.nist.gov/itl/ssd/Materials.owl#VacancyDiffusionMechanism

:VacancyDiffusionMechanism rdf:type :DiffusionMovementMechanism ,
                                    owl:NamedIndividual ;
                           
                           rdfs:seeAlso "Definitions of terms for diffusion in the solid state (IUPAC Recommendations 1999), Pure Appl. Chem. 71, 1307-1325."@en ;
                           
                           rdfs:comment "The Vacancy Diffusion Mechanism is a mechanism where diffusion is made possible by the exchange of positions between the diffusing species and a vacancy."@en .



###  http://www.nist.gov/itl/ssd/Materials.owl#VickersHardness

:VickersHardness rdf:type :IndentationHardness ,
                          owl:NamedIndividual .



###  http://www.nist.gov/itl/ssd/Materials.owl#VolumeCompressibility

:VolumeCompressibility rdf:type :Compressibility ,
                                owl:NamedIndividual .



###  http://www.nist.gov/itl/ssd/Materials.owl#VolumeOfObject

:VolumeOfObject rdf:type :MeasurableMechanicalProperty ,
                         owl:NamedIndividual ;
                
                or:unitTypeFor or:UnitOfVolume .



###  http://www.nist.gov/itl/ssd/Materials.owl#Washing

:Washing rdf:type owl:NamedIndividual .



###  http://www.nist.gov/itl/ssd/Materials.owl#Watt

:Watt rdf:type :UnitOfPower ,
               <http://www.nist.gov/itl/ssd/OntologyRequirements.owl#SI_Unit> ,
               owl:NamedIndividual .



###  http://www.nist.gov/itl/ssd/Materials.owl#WattsPerMeterKelvin

:WattsPerMeterKelvin rdf:type :UnitOfThermalConductivity ,
                              <http://www.nist.gov/itl/ssd/OntologyRequirements.owl#SI_Unit> ,
                              owl:NamedIndividual .



###  http://www.nist.gov/itl/ssd/Materials.owl#WearRateCoefficient

:WearRateCoefficient rdf:type :MeasurableMechanicalProperty ,
                              owl:NamedIndividual .



###  http://www.nist.gov/itl/ssd/Materials.owl#Welding

:Welding rdf:type owl:NamedIndividual .



###  http://www.nist.gov/itl/ssd/Materials.owl#WroughtAlloy

:WroughtAlloy rdf:type :AlloyTypeByFormingProcess ,
                       owl:NamedIndividual ;
              
              rdfs:comment "A Wrought Alloy is one in which soft heated metal is mechanically worked (often by hammering) into shape, possibly after casting."@en .



###  http://www.nist.gov/itl/ssd/Materials.owl#YieldStrength

:YieldStrength rdf:type :DeformationProperty ,
                        owl:NamedIndividual ;
               
               rdfs:comment "The yield strength or yield point of a material is defined as the stress at which a material begins to deform plastically. Below the yield point the material will deform elastically and will return to its original shape when the applied stress is removed. Once the yield point is passed, some fraction of the deformation will be permanent and non-reversible."@en ;
               
               or:unitTypeFor or:UnitOfPressure .



###  http://www.nist.gov/itl/ssd/Materials.owl#ZincAlloy

:ZincAlloy rdf:type :NonFerrousAlloyTypeByMainConstituent ,
                    owl:NamedIndividual ;
           
           or:referenceURL "http://www.matweb.com/index.aspx"^^xsd:anyURI ;
           
           rdfs:comment "An alloy that contains Zinc but not Iron."@en ;
           
           bc:primaryConstituentType bc:Zinc .



###  http://www.nist.gov/itl/ssd/Materials.owl#ZincOxide

:ZincOxide rdf:type bc:ChemicalSubstanceTypeByChemicalSpecies ,
                    owl:NamedIndividual ;
           
           <http://www.nist.gov/itl/ssd/OntologyRequirements.owl#termString> "zinc oxide"@en .



###  http://www.nist.gov/itl/ssd/Materials.owl#ZirconiumOxide

:ZirconiumOxide rdf:type bc:ChemicalSubstanceTypeByChemicalSpecies ,
                         owl:NamedIndividual ;
                
                or:referenceURL "http://www.matweb.com/index.aspx"^^xsd:anyURI ;
                
                <http://www.nist.gov/itl/ssd/OntologyRequirements.owl#termString> "zirconium oxide"@en .



###  http://www.nist.gov/itl/ssd/OntologyRequirements#ComputerStorageCapacity

or:ComputerStorageCapacity or:unitTypeFor or:UnitOfComputerStorageCapacity .



###  http://www.nist.gov/itl/ssd/OntologyRequirements#DegreeCelsius

or:DegreeCelsius rdfs:comment "A Degree Celsius is a Unit of Temperature that specifies an an absolute temperature.-- how many Celsius Degrees the temperature is above (or if negative, below) the freezing point of water.  Adding 273.15 to a temperature specified in Degrees Celsius gives the value of the temperature in Degrees Kelvin.  To refer to temperature differences, use the Unit Of Temperature Difference, Celsius Degree."@en .



###  http://www.nist.gov/itl/ssd/OntologyRequirements#DegreeKelvin

or:DegreeKelvin rdfs:comment "A Degree Kelvin is a Unit of Temperature that specifies an an absolute temperature.-- how many Celsius Degrees the temperature is above Absolute Zero.  Subtracting 273.15 from a temperature specified in Degrees Kelvin gives the value of the temperature in Degrees Celsius.  To refer to temperature differences, use the Unit Of Temperature Difference, Celsius Degree."@en .



###  http://www.nist.gov/itl/ssd/OntologyRequirements#UnitOfTemperature

or:UnitOfTemperature rdfs:comment "A Unit of Temperature is a Unit of Measure used for specifying the temperature of something.  Two different Units of Temperatures may have the same magnitude, but different offsets, so are not the same.  A Degree Celsius is different from a Degree Kelvin, for example since 100 C = 373.15 K."@en .



###  http://www.nist.gov/itl/ssd/OntologyRequirements#Volt

or:Volt <http://www.nist.gov/itl/ssd/OntologyRequirements.owl#termString> "joules per coulomb"@en ,
                                                                          "volt"@en .





#################################################################
#
#    Annotations
#
#################################################################


or:Nanoliter <http://www.nist.gov/itl/ssd/OntologyRequirements.owl#termString> "nanoliter"@en ,
                                                                               "nanolitre"@en ,
                                                                               "nl"@en .



or:Liter <http://www.nist.gov/itl/ssd/OntologyRequirements.owl#termString> "l"@en ,
                                                                           "liter"@en ,
                                                                           "litre"@en .



or:CubicMeter <http://www.nist.gov/itl/ssd/OntologyRequirements.owl#termString> "cubic meter"@en ,
                                                                                "cubic metre"@en .



or:Pascal-UnitOfPressure <http://www.nist.gov/itl/ssd/OntologyRequirements.owl#termString> "pascal"@en .



or:Microliter <http://www.nist.gov/itl/ssd/OntologyRequirements.owl#termString> "microliter"@en ,
                                                                                "microlitre"@en .



or:Milliliter <http://www.nist.gov/itl/ssd/OntologyRequirements.owl#termString> "cc"@en ,
                                                                                "cubic centimeter"@en ,
                                                                                "cubic centimetre"@en ,
                                                                                "milliliter"@en ,
                                                                                "millilitre"@en ,
                                                                                "ml"@en .



or:Meter <http://www.nist.gov/itl/ssd/OntologyRequirements.owl#termString> "meter"@en ,
                                                                           "metre"@en .



or:Centimeter <http://www.nist.gov/itl/ssd/OntologyRequirements.owl#termString> "centimeter"@en ,
                                                                                "centimetre"@en .



<http://www.nist.gov/itl/ssd/OntologyRequirements.owl#Nanometer> <http://www.nist.gov/itl/ssd/OntologyRequirements.owl#termString> "nanometer"@en ,
                                                                                                                                   "nanometre"@en .



or:ElectronVolt <http://www.nist.gov/itl/ssd/OntologyRequirements.owl#termString> "electron volt"@en ,
                                                                                  "ev"@en .



or:MmHg <http://www.nist.gov/itl/ssd/OntologyRequirements.owl#termString> "millimeter of mercury"@en ,
                                                                          "mm Hg"@en .



or:Millimeter <http://www.nist.gov/itl/ssd/OntologyRequirements.owl#termString> "millimeter"@en ,
                                                                                "millimetre"@en .



or:DegreeFahrenheit rdfs:comment "A Degree Fahrenheit is a Unit of Temperature that specifies an an absolute temperature.-- how many Fahrenheit Degrees the temperature is above (or if negative, below) 32 Fahrenheit Degrees below the freezing point of water.  To refer to temperature differences, use the Unit Of Temperature Difference, Fahrenheit Degree."@en .



bc:VaporPressure <http://www.nist.gov/itl/ssd/OntologyRequirements.owl#termString> "vapor pressure"@en .



or:Bar-UnitOfPressure <http://www.nist.gov/itl/ssd/OntologyRequirements.owl#termString> "10^5 Pascals"@en ,
                                                                                        "Pa*10^5"@en ,
                                                                                        "bar"@en .



or:catalogNumber <http://www.w3.org/2004/02/skos/core#note> "Something can have different catalog numbers in different catalogs.  To be functional, a ternary relation that specifies the catalog is needed.  Specializations of this relation (XCatalogNumber) can be functional."@en .



or:BritishThermalUnit <http://www.nist.gov/itl/ssd/OntologyRequirements.owl#termString> "BTU"@en ,
                                                                                        "British thermal unit"@en .



<http://www.nist.gov/itl/ssd/OntologyRequirements.owl#AvogadrosNumber> <http://www.nist.gov/itl/ssd/OntologyRequirements.owl#termString> "Avodadro's number"@en .



or:Femtoliter <http://www.nist.gov/itl/ssd/OntologyRequirements.owl#termString> "femtoliter"@en ,
                                                                                "femtolitre"@en .



or:PSI <http://www.nist.gov/itl/ssd/OntologyRequirements.owl#termString> "PSI"@en .





#################################################################
#
#    General axioms
#
#################################################################


[ rdf:type owl:AllDifferent ;
  owl:distinctMembers ( :CelsiusDegree
                        :FahrenheitDegree
                        or:DegreeCelsius
                        or:DegreeKelvin
                      )
] .
[ rdf:type owl:AllDifferent ;
  owl:distinctMembers ( :Opaque
                        :Transparent
                      )
] .
[ rdf:type owl:AllDifferent ;
  owl:distinctMembers ( :Opaque
                        :Translucent
                      )
] .
[ rdf:type owl:AllDifferent ;
  owl:distinctMembers ( :Translucent
                        :Transparent
                      )
] .




###  Generated by the OWL API (version 3.2.3.1824) http://owlapi.sourceforge.net

