<?xml version="1.0"?>


<!DOCTYPE rdf:RDF [
    <!ENTITY owl "http://www.w3.org/2002/07/owl#" >
    <!ENTITY xsd "http://www.w3.org/2001/XMLSchema#" >
    <!ENTITY skos "http://www.w3.org/2004/02/skos/core#" >
    <!ENTITY bc "http://www.nist.gov/itl/ssd/Biochem#" >
    <!ENTITY oil "http://www.daml.org/2001/03/daml+oil#" >
    <!ENTITY rdfs "http://www.w3.org/2000/01/rdf-schema#" >
    <!ENTITY doc "http://www.nist.gov/itl/ssd/Document#" >
    <!ENTITY mat "http://www.nist.gov/itl/ssd/Materials#" >
    <!ENTITY exp "http://www.nist.gov/itl/ssd/Experiments#" >
    <!ENTITY rdf "http://www.w3.org/1999/02/22-rdf-syntax-ns#" >
    <!ENTITY or "http://www.nist.gov/itl/ssd/OntologyRequirements#" >
]>


<rdf:RDF xmlns="http://www.nist.gov/itl/ssd/Materials#"
     xml:base="http://www.nist.gov/itl/ssd/Materials"
     xmlns:exp="http://www.nist.gov/itl/ssd/Experiments#"
     xmlns:rdfs="http://www.w3.org/2000/01/rdf-schema#"
     xmlns:or="http://www.nist.gov/itl/ssd/OntologyRequirements#"
     xmlns:mat="http://www.nist.gov/itl/ssd/Materials#"
     xmlns:owl="http://www.w3.org/2002/07/owl#"
     xmlns:xsd="http://www.w3.org/2001/XMLSchema#"
     xmlns:doc="http://www.nist.gov/itl/ssd/Document#"
     xmlns:rdf="http://www.w3.org/1999/02/22-rdf-syntax-ns#"
     xmlns:skos="http://www.w3.org/2004/02/skos/core#"
     xmlns:bc="http://www.nist.gov/itl/ssd/Biochem#"
     xmlns:oil="http://www.daml.org/2001/03/daml+oil#">
    <owl:Ontology rdf:about="http://www.nist.gov/itl/ssd/Materials">
        <owl:imports rdf:resource="http://www.nist.gov/itl/ssd/Biochem"/>
        <owl:imports rdf:resource="http://www.nist.gov/itl/ssd/Document"/>
    </owl:Ontology>
    


    <!-- 
    ///////////////////////////////////////////////////////////////////////////////////////
    //
    // Annotation properties
    //
    ///////////////////////////////////////////////////////////////////////////////////////
     -->

    <owl:AnnotationProperty rdf:about="&or;unitTypeFor"/>
    


    <!-- 
    ///////////////////////////////////////////////////////////////////////////////////////
    //
    // Datatypes
    //
    ///////////////////////////////////////////////////////////////////////////////////////
     -->

    


    <!-- 
    ///////////////////////////////////////////////////////////////////////////////////////
    //
    // Object Properties
    //
    ///////////////////////////////////////////////////////////////////////////////////////
     -->

    


    <!-- http://www.nist.gov/itl/ssd/Biochem#componentElement -->

    <rdf:Description rdf:about="&bc;componentElement">
        <rdf:type rdf:resource="&owl;IrreflexiveProperty"/>
        <rdfs:range rdf:resource="&bc;ChemicalElement"/>
    </rdf:Description>
    


    <!-- http://www.nist.gov/itl/ssd/Biochem#constituentType -->

    <rdf:Description rdf:about="&bc;constituentType">
        <rdfs:domain rdf:resource="&or;MaterialType"/>
        <rdfs:range rdf:resource="&or;MaterialType"/>
    </rdf:Description>
    


    <!-- http://www.nist.gov/itl/ssd/Biochem#hasMolecularStructure -->

    <owl:ObjectProperty rdf:about="&bc;hasMolecularStructure">
        <rdfs:range rdf:resource="&mat;Microstructure"/>
    </owl:ObjectProperty>
    


    <!-- http://www.nist.gov/itl/ssd/Materials#classOfMaterial -->

    <owl:ObjectProperty rdf:about="&mat;classOfMaterial">
        <rdfs:comment xml:lang="en">OBJECT classOfMaterial MATERIAL_TYPE means that OBJECT is made out of the general type of material MATERIAL_TYPE.  Use subclassOfMaterial, if referring to a more specific type.</rdfs:comment>
        <rdfs:domain rdf:resource="&mat;MaterialObject"/>
        <rdfs:range rdf:resource="&or;MaterialType"/>
    </owl:ObjectProperty>
    


    <!-- http://www.nist.gov/itl/ssd/Materials#coatingOf -->

    <owl:ObjectProperty rdf:about="&mat;coatingOf">
        <rdf:type rdf:resource="&owl;AsymmetricProperty"/>
        <rdf:type rdf:resource="&owl;IrreflexiveProperty"/>
        <rdfs:comment xml:lang="en">The property &#39;coating Of&#39; relates a coating material to the object which it coats.</rdfs:comment>
        <rdfs:domain rdf:resource="&mat;MaterialObject"/>
        <rdfs:range rdf:resource="&mat;MaterialObject"/>
        <owl:propertyDisjointWith rdf:resource="&mat;embeddedIn"/>
        <owl:propertyDisjointWith rdf:resource="&mat;substrate"/>
        <owl:propertyDisjointWith rdf:resource="&mat;weldedTo"/>
    </owl:ObjectProperty>
    


    <!-- http://www.nist.gov/itl/ssd/Materials#compositionSpecification -->

    <owl:ObjectProperty rdf:about="&mat;compositionSpecification">
        <rdfs:comment xml:lang="en">The property composition Secification relates an object to a specification of the type of material (e.g., an alloy) of which it is composed.</rdfs:comment>
        <rdfs:range rdf:resource="&doc;Specification"/>
        <rdfs:domain rdf:resource="&mat;MaterialObject"/>
    </owl:ObjectProperty>
    


    <!-- http://www.nist.gov/itl/ssd/Materials#concentrationLevel -->

    <owl:ObjectProperty rdf:about="&mat;concentrationLevel">
        <rdf:type rdf:resource="&owl;FunctionalProperty"/>
        <rdfs:comment xml:lang="en">The property &#39;concentration Level&#39; specifies what the concentration of the specified Material Type is for a given Material Portion..</rdfs:comment>
        <rdfs:range rdf:resource="&bc;Concentration"/>
        <rdfs:domain rdf:resource="&mat;MaterialPortion"/>
    </owl:ObjectProperty>
    


    <!-- http://www.nist.gov/itl/ssd/Materials#concentrationOfMaterialType -->

    <owl:ObjectProperty rdf:about="&mat;concentrationOfMaterialType">
        <rdf:type rdf:resource="&owl;FunctionalProperty"/>
        <rdfs:comment xml:lang="en">The property &#39;concentration Of Material Type&#39; links a substance Concentration to the type of material (Material Type) for which it is a concentration.</rdfs:comment>
        <rdfs:domain rdf:resource="&bc;Concentration"/>
        <rdfs:range rdf:resource="&or;MaterialType"/>
    </owl:ObjectProperty>
    


    <!-- http://www.nist.gov/itl/ssd/Materials#diffusivity -->

    <owl:ObjectProperty rdf:about="&mat;diffusivity">
        <rdfs:comment xml:lang="en">Diffusivity is the ratio between the molar flux due to molecular diffusion and the gradient in the concentration of the species (or the driving force for diffusion).  Diffusivity is generally prescribed for a given pair of species in a given phase at a given temperature. For a multi-component system, it is prescribed for each pair of species in the system.  Diffusivity is measured in Area per unit time -- in SI, m^2/s.</rdfs:comment>
        <rdfs:range rdf:resource="&mat;AreaPerTime"/>
    </owl:ObjectProperty>
    


    <!-- http://www.nist.gov/itl/ssd/Materials#drivingForceForDiffusion -->

    <owl:ObjectProperty rdf:about="&mat;drivingForceForDiffusion">
        <rdfs:seeAlso>Definitions of terms for diffusion in the solid state (IUPAC Recommendations 1999), Pure Appl. Chem. 71, 1307-1325.</rdfs:seeAlso>
        <rdfs:comment xml:lang="en">The property ``driving Force&#39;&#39; relates an instance of Diffusion to any type influence which causes the jump frequency for a jump in one direction between two given sites to differ from that for a jump in the opposite direction between exactly analogous sites. Driving forces include gradients of stress, electrical potential, object temperature or chemical potential.</rdfs:comment>
        <or:termString xml:lang="en">diffusion driving force</or:termString>
        <or:termString xml:lang="en">driving force</or:termString>
        <rdfs:domain rdf:resource="&mat;Diffusion"/>
        <rdfs:range rdf:resource="&or;MeasurableProperty"/>
    </owl:ObjectProperty>
    


    <!-- http://www.nist.gov/itl/ssd/Materials#embeddedIn -->

    <owl:ObjectProperty rdf:about="&mat;embeddedIn">
        <rdf:type rdf:resource="&owl;AsymmetricProperty"/>
        <rdf:type rdf:resource="&owl;IrreflexiveProperty"/>
        <rdfs:domain rdf:resource="&mat;MaterialObject"/>
        <rdfs:range rdf:resource="&mat;MaterialObject"/>
        <owl:propertyDisjointWith rdf:resource="&mat;substrate"/>
        <owl:propertyDisjointWith rdf:resource="&mat;weldedTo"/>
    </owl:ObjectProperty>
    


    <!-- http://www.nist.gov/itl/ssd/Materials#enthalpyOfFusion -->

    <owl:ObjectProperty rdf:about="&mat;enthalpyOfFusion">
        <rdf:type rdf:resource="&owl;FunctionalProperty"/>
        <rdfs:comment xml:lang="en">The enthalpy of fusion is the change in enthalpy required to melt one mole of a substance at its melting point.</rdfs:comment>
        <rdfs:domain rdf:resource="&bc;ChemicalSubstance"/>
        <rdfs:range rdf:resource="&or;Energy"/>
    </owl:ObjectProperty>
    


    <!-- http://www.nist.gov/itl/ssd/Materials#enthalpyOfSystem -->

    <owl:ObjectProperty rdf:about="&mat;enthalpyOfSystem">
        <rdf:type rdf:resource="&owl;FunctionalProperty"/>
        <rdfs:comment>Enthalpy is a measure of the total energy of a Thermodynamic System. It includes the internal energy, which is the energy required to create a system, and the amount of energy required to make room for it by displacing its environment and establishing its volume and pressure.

Enthalpy is not directly measured, Changes in enthalpy are.</rdfs:comment>
    </owl:ObjectProperty>
    


    <!-- http://www.nist.gov/itl/ssd/Materials#gibbsEnergy -->

    <owl:ObjectProperty rdf:about="&mat;gibbsEnergy">
        <rdf:type rdf:resource="&owl;FunctionalProperty"/>
        <rdfs:comment xml:lang="en">The property `gibbs Energy&#39;  specifies the Gibbs free energy of a Thermodynamic System, which specifies the “useful” work obtainable from a closed thermodynamic system at a constant temperature and pressure.</rdfs:comment>
        <rdfs:domain rdf:resource="&mat;ThermodynamicSystem"/>
        <rdfs:range rdf:resource="&or;Energy"/>
    </owl:ObjectProperty>
    


    <!-- http://www.nist.gov/itl/ssd/Materials#hasChemicalComposition -->

    <owl:ObjectProperty rdf:about="&mat;hasChemicalComposition">
        <rdf:type rdf:resource="&owl;FunctionalProperty"/>
        <rdfs:comment xml:lang="en">The property &#39;has Chemical Composition&#39; relates some Material Substance to its Chemical Composition&#39;.</rdfs:comment>
        <rdfs:range rdf:resource="&bc;ChemicalComposition"/>
        <rdfs:domain rdf:resource="&bc;MaterialSubstance"/>
    </owl:ObjectProperty>
    


    <!-- http://www.nist.gov/itl/ssd/Materials#hasHeatCapacity -->

    <owl:ObjectProperty rdf:about="&mat;hasHeatCapacity">
        <rdfs:domain rdf:resource="&mat;MaterialObject"/>
    </owl:ObjectProperty>
    


    <!-- http://www.nist.gov/itl/ssd/Materials#hasLatticeConstant -->

    <owl:ObjectProperty rdf:about="&mat;hasLatticeConstant">
        <rdfs:comment xml:lang="en">The lattice Constant of a Crystal Lattice is the constant distance between unit cells.  A cubic lattice has a single lattice constant, while other forms of crystal have three.  The constant may be temperature dependant.</rdfs:comment>
        <rdfs:domain rdf:resource="&mat;CrystalLattice"/>
        <rdfs:range rdf:resource="&or;Distance"/>
    </owl:ObjectProperty>
    


    <!-- http://www.nist.gov/itl/ssd/Materials#hasMaterialForm -->

    <owl:ObjectProperty rdf:about="&mat;hasMaterialForm">
        <rdfs:comment xml:lang="en">The predicate &#39;has Material Form&#39; relates a Material Object to its Material Form.</rdfs:comment>
        <rdfs:range rdf:resource="&mat;MaterialForm"/>
        <rdfs:domain rdf:resource="&mat;MaterialObject"/>
    </owl:ObjectProperty>
    


    <!-- http://www.nist.gov/itl/ssd/Materials#hasMolecularStructure -->

    <owl:ObjectProperty rdf:about="&mat;hasMolecularStructure">
        <rdfs:range></rdfs:range>
        <rdfs:domain rdf:resource="&bc;ChemicalSubstance"/>
        <rdfs:range rdf:resource="&mat;Microstructure"/>
    </owl:ObjectProperty>
    


    <!-- http://www.nist.gov/itl/ssd/Materials#hasSubstanceConcentration -->

    <owl:ObjectProperty rdf:about="&mat;hasSubstanceConcentration">
        <rdfs:comment xml:lang="en">The property &#39;has Substance Concentration&#39; specifies for each Chemical Composition the specific concentration of one of its substances (called a Material Portion).  Unless there is only a single substance type, a given Chemical Composition has multiple substance concentrations.</rdfs:comment>
        <rdfs:domain rdf:resource="&bc;ChemicalComposition"/>
        <rdfs:range rdf:resource="&bc;Concentration"/>
    </owl:ObjectProperty>
    


    <!-- http://www.nist.gov/itl/ssd/Materials#heatOfFusion -->

    <owl:ObjectProperty rdf:about="&mat;heatOfFusion">
        <rdf:type rdf:resource="&owl;FunctionalProperty"/>
        <rdfs:comment xml:lang="en">The heat of fusion is the change in enthalpy per unit mass required to melt oa substance at its melting point.</rdfs:comment>
        <rdfs:domain rdf:resource="&bc;ChemicalSubstance"/>
        <rdfs:range rdf:resource="&mat;EnergyPerMass"/>
    </owl:ObjectProperty>
    


    <!-- http://www.nist.gov/itl/ssd/Materials#helmholtzEnergy -->

    <owl:ObjectProperty rdf:about="&mat;helmholtzEnergy">
        <rdfs:comment xml:lang="en">The property `helmholtz Energy&#39;  specifies the Helmholtz free energy of a Thermodynamic System, which specifies the “useful” work obtainable from a closed thermodynamic system at a constant temperature and volume..</rdfs:comment>
    </owl:ObjectProperty>
    


    <!-- http://www.nist.gov/itl/ssd/Materials#isotopeOfElementType -->

    <owl:ObjectProperty rdf:about="&mat;isotopeOfElementType">
        <rdf:type rdf:resource="&owl;FunctionalProperty"/>
        <rdfs:comment xml:lang="en">The property &#39;isotope Of Element Type&#39; specifies the Element of which an Isotope is an isotope of.</rdfs:comment>
        <rdfs:range rdf:resource="&bc;ChemicalElement"/>
        <rdfs:domain rdf:resource="&bc;Isotope"/>
    </owl:ObjectProperty>
    


    <!-- http://www.nist.gov/itl/ssd/Materials#molarHeatCapacity -->

    <owl:ObjectProperty rdf:about="&mat;molarHeatCapacity">
        <rdfs:comment xml:lang="en">The molar heat capacity is the heat capacity per mole of a pure substance.</rdfs:comment>
        <rdfs:domain rdf:resource="&bc;ChemicalSubstance"/>
        <rdfs:domain rdf:resource="&mat;PureSubstance"/>
    </owl:ObjectProperty>
    


    <!-- http://www.nist.gov/itl/ssd/Materials#peritecticTemperature -->

    <owl:ObjectProperty rdf:about="&mat;peritecticTemperature">
        <rdfs:comment xml:lang="en">In a peritectic reaction a liquid and solid phase of fixed proportions react at a fixed temperature to yield a single solid phase.  The peritectic temperature is the temperature at which this happens.</rdfs:comment>
        <rdfs:domain rdf:resource="&mat;PhysicalMixture"/>
        <rdfs:range rdf:resource="&or;Temperature"/>
    </owl:ObjectProperty>
    


    <!-- http://www.nist.gov/itl/ssd/Materials#phaseOfMaterial -->

    <owl:ObjectProperty rdf:about="&mat;phaseOfMaterial">
        <rdfs:comment xml:lang="en">The property &#39;phase Of Material&#39; relates a Material Object to its Material Phase (e.g., crystalline, gel, liquid, ...).</rdfs:comment>
        <rdfs:domain rdf:resource="&mat;MaterialObject"/>
        <rdfs:range rdf:resource="&mat;MaterialPhaseComposition"/>
    </owl:ObjectProperty>
    


    <!-- http://www.nist.gov/itl/ssd/Materials#physicalDecompositions -->

    <owl:ObjectProperty rdf:about="&mat;physicalDecompositions">
        <rdfs:comment xml:lang="en">(physicalDecompositions WHOLE PART) means that PART is a spatial part or component of WHOLE, in a very broad sense of &#39;part&#39; whereby PART might or might not be spatially continuous or discrete. Thus PART might be discontinuous, or diffused throughout WHOLE.</rdfs:comment>
        <rdfs:domain rdf:resource="&mat;MaterialObject"/>
        <rdfs:range rdf:resource="&mat;MaterialObject"/>
    </owl:ObjectProperty>
    


    <!-- http://www.nist.gov/itl/ssd/Materials#relativePermittivity -->

    <owl:ObjectProperty rdf:about="&mat;relativePermittivity">
        <rdfs:domain rdf:resource="&bc;MaterialSubstance"/>
        <rdfs:range rdf:resource="&mat;ElectricPolarizability"/>
    </owl:ObjectProperty>
    


    <!-- http://www.nist.gov/itl/ssd/Materials#solidus -->

    <owl:ObjectProperty rdf:about="&mat;solidus">
        <rdfs:domain rdf:resource="&or;MaterialType"/>
    </owl:ObjectProperty>
    


    <!-- http://www.nist.gov/itl/ssd/Materials#solute -->

    <owl:ObjectProperty rdf:about="&mat;solute">
        <rdfs:comment xml:lang="en">The property &#39;solute&#39; relates a Chemical Solution to a material that is a solute in the solution.</rdfs:comment>
        <rdfs:domain rdf:resource="&mat;ChemicalSolution"/>
        <rdfs:range rdf:resource="&mat;PureSubstance"/>
    </owl:ObjectProperty>
    


    <!-- http://www.nist.gov/itl/ssd/Materials#solvent -->

    <owl:ObjectProperty rdf:about="&mat;solvent">
        <rdf:type rdf:resource="&owl;FunctionalProperty"/>
        <rdfs:comment xml:lang="en">The property &#39;solvent&#39; relates a Chemical Solution to the material that is the solvent in the solution.</rdfs:comment>
        <rdfs:range rdf:resource="&bc;MaterialSubstance"/>
        <rdfs:domain rdf:resource="&mat;ChemicalSolution"/>
    </owl:ObjectProperty>
    


    <!-- http://www.nist.gov/itl/ssd/Materials#sourcesMaterialType -->

    <owl:ObjectProperty rdf:about="&mat;sourcesMaterialType">
        <rdfs:comment xml:lang="en">The property &#39;sources Material Type&#39; relates a Material Source Organization to a Material Type that it regularly can provide to others.</rdfs:comment>
        <rdfs:range rdf:resource="&or;MaterialType"/>
    </owl:ObjectProperty>
    


    <!-- http://www.nist.gov/itl/ssd/Materials#structuralIsomers -->

    <owl:ObjectProperty rdf:about="&mat;structuralIsomers">
        <rdf:type rdf:resource="&owl;IrreflexiveProperty"/>
        <rdf:type rdf:resource="&owl;SymmetricProperty"/>
        <rdfs:comment xml:lang="en">Two chemical compounds are stereoisomers if they have the same simple chemical formula, but have different arrangements of the bonds between theiir atoms.</rdfs:comment>
        <rdfs:domain rdf:resource="&bc;ChemicalObjectTypeByChemicalSpecies"/>
        <rdfs:range rdf:resource="&bc;ChemicalObjectTypeByChemicalSpecies"/>
    </owl:ObjectProperty>
    


    <!-- http://www.nist.gov/itl/ssd/Materials#subclassOfMaterial -->

    <owl:ObjectProperty rdf:about="&mat;subclassOfMaterial">
        <rdfs:comment xml:lang="en">OBJECT subclassOfMaterial MATERIAL_TYPE means that OBJECT is made of of the specific type of material MATERIAL_TYPE.  Use classOfMaterial, if referring to a more general type.</rdfs:comment>
        <rdfs:domain rdf:resource="&mat;MaterialObject"/>
        <rdfs:range rdf:resource="&or;MaterialType"/>
    </owl:ObjectProperty>
    


    <!-- http://www.nist.gov/itl/ssd/Materials#substrate -->

    <owl:ObjectProperty rdf:about="&mat;substrate">
        <rdf:type rdf:resource="&owl;AsymmetricProperty"/>
        <rdf:type rdf:resource="&owl;IrreflexiveProperty"/>
        <rdfs:domain rdf:resource="&mat;MaterialObject"/>
        <rdfs:range rdf:resource="&mat;MaterialObject"/>
        <owl:propertyDisjointWith rdf:resource="&mat;weldedTo"/>
    </owl:ObjectProperty>
    


    <!-- http://www.nist.gov/itl/ssd/Materials#weldedTo -->

    <owl:ObjectProperty rdf:about="&mat;weldedTo">
        <rdf:type rdf:resource="&owl;IrreflexiveProperty"/>
        <rdf:type rdf:resource="&owl;SymmetricProperty"/>
        <rdfs:domain rdf:resource="&mat;MaterialObject"/>
        <rdfs:range rdf:resource="&mat;MaterialObject"/>
    </owl:ObjectProperty>
    


    <!-- http://www.nist.gov/itl/ssd/OntologyRequirements#objectActedOn -->

    <owl:ObjectProperty rdf:about="&or;objectActedOn"/>
    


    <!-- http://www.nist.gov/itl/ssd/OntologyRequirements#outputCreated -->

    <owl:ObjectProperty rdf:about="&or;outputCreated"/>
    


    <!-- http://www.nist.gov/itl/ssd/OntologyRequirements#subEvents -->

    <owl:ObjectProperty rdf:about="&or;subEvents"/>
    


    <!-- http://www.nist.gov/itl/ssd/OntologyRequirements#unitTypeFor -->

    <rdf:Description rdf:about="&or;unitTypeFor">
        <rdfs:subPropertyOf rdf:resource="&owl;topObjectProperty"/>
    </rdf:Description>
    


    <!-- 
    ///////////////////////////////////////////////////////////////////////////////////////
    //
    // Data properties
    //
    ///////////////////////////////////////////////////////////////////////////////////////
     -->

    


    <!-- http://www.nist.gov/itl/ssd/Materials#ZAverageMolarMass -->

    <owl:DatatypeProperty rdf:about="&mat;ZAverageMolarMass">
        <rdf:type rdf:resource="&owl;FunctionalProperty"/>
        <or:referenceURL rdf:datatype="&xsd;anyURI">http://www.iupac.org/namespaces/ThermoML#nZAvgMolMass</or:referenceURL>
        <or:termString xml:lang="en">The Z- average molecular mass of a polymer. </or:termString>
        <rdfs:range rdf:resource="&owl;real"/>
        <rdfs:domain>
            <owl:Class>
                <owl:unionOf rdf:parseType="Collection">
                    <rdf:Description rdf:about="&bc;Polymer"/>
                    <rdf:Description rdf:about="&mat;PolymerSubstance"/>
                </owl:unionOf>
            </owl:Class>
        </rdfs:domain>
    </owl:DatatypeProperty>
    


    <!-- http://www.nist.gov/itl/ssd/Materials#cAIndexName -->

    <owl:DatatypeProperty rdf:about="&mat;cAIndexName">
        <or:referenceURL rdf:datatype="&xsd;anyURI">http://www.iupac.org/namespaces/ThermoML#sCASName</or:referenceURL>
        <or:termString xml:lang="en">CA Index name</or:termString>
        <rdfs:domain rdf:resource="&bc;ChemicalSubstanceTypeByChemicalSpecies"/>
        <rdfs:subPropertyOf rdf:resource="&or;nameString"/>
    </owl:DatatypeProperty>
    


    <!-- http://www.nist.gov/itl/ssd/Materials#cASRegistryNumber -->

    <owl:DatatypeProperty rdf:about="&mat;cASRegistryNumber">
        <rdf:type rdf:resource="&owl;FunctionalProperty"/>
        <or:referenceURL rdf:datatype="&xsd;anyURI">http://www.iupac.org/namespaces/ThermoML#nCASRNum</or:referenceURL>
        <or:termString xml:lang="en">CAS Registry number</or:termString>
        <rdfs:domain rdf:resource="&bc;ChemicalSubstanceTypeByChemicalSpecies"/>
        <rdfs:subPropertyOf rdf:resource="&or;idString"/>
        <rdfs:range rdf:resource="&xsd;string"/>
    </owl:DatatypeProperty>
    


    <!-- http://www.nist.gov/itl/ssd/Materials#commonName -->

    <owl:DatatypeProperty rdf:about="&mat;commonName">
        <or:referenceURL rdf:datatype="&xsd;anyURI">http://www.iupac.org/namespaces/ThermoML#sCommonName</or:referenceURL>
        <or:termString xml:lang="en">common name</or:termString>
        <rdfs:subPropertyOf rdf:resource="&or;nameString"/>
    </owl:DatatypeProperty>
    


    <!-- http://www.nist.gov/itl/ssd/Materials#degreeOfPolymerizationDispersity -->

    <owl:DatatypeProperty rdf:about="&mat;degreeOfPolymerizationDispersity">
        <or:referenceURL rdf:datatype="&xsd;anyURI">http://www.iupac.org/namespaces/ThermoML#nDegOfPolymerizationDispersity</or:referenceURL>
        <rdfs:range rdf:resource="&owl;real"/>
        <rdfs:domain>
            <owl:Class>
                <owl:unionOf rdf:parseType="Collection">
                    <rdf:Description rdf:about="&bc;Polymer"/>
                    <rdf:Description rdf:about="&mat;PolymerSubstance"/>
                </owl:unionOf>
            </owl:Class>
        </rdfs:domain>
    </owl:DatatypeProperty>
    


    <!-- http://www.nist.gov/itl/ssd/Materials#ecNumber -->

    <owl:DatatypeProperty rdf:about="&mat;ecNumber">
        <rdf:type rdf:resource="&owl;FunctionalProperty"/>
        <or:referenceURL rdf:datatype="&xsd;anyURI">http://www.iupac.org/namespaces/ThermoML#sECNumber</or:referenceURL>
        <or:termString xml:lang="en">EC number</or:termString>
        <rdfs:domain rdf:resource="&bc;ChemicalSubstanceTypeByChemicalSpecies"/>
        <rdfs:subPropertyOf rdf:resource="&or;idString"/>
        <rdfs:range rdf:resource="&xsd;string"/>
    </owl:DatatypeProperty>
    


    <!-- http://www.nist.gov/itl/ssd/Materials#iUPACName -->

    <owl:DatatypeProperty rdf:about="&mat;iUPACName">
        <or:referenceURL rdf:datatype="&xsd;anyURI">http://www.iupac.org/namespaces/ThermoML#sIUPACName</or:referenceURL>
        <or:termString xml:lang="en">IUPAC name</or:termString>
        <or:termString xml:lang="en">International Union of Physics and Applied Chemistry name</or:termString>
        <rdfs:comment xml:lang="en">International Union of Physics and Applied Chemistry name</rdfs:comment>
        <rdfs:domain rdf:resource="&bc;ChemicalSubstanceTypeByChemicalSpecies"/>
        <rdfs:subPropertyOf rdf:resource="&or;nameString"/>
    </owl:DatatypeProperty>
    


    <!-- http://www.nist.gov/itl/ssd/Materials#inChI -->

    <owl:DatatypeProperty rdf:about="&mat;inChI">
        <rdf:type rdf:resource="&owl;FunctionalProperty"/>
        <or:referenceURL rdf:datatype="&xsd;anyURI">http://www.iupac.org/namespaces/ThermoML#sStandardInChI</or:referenceURL>
        <rdfs:comment xml:lang="en">The IUPAC International Chemical Identifier (InChI)  formerly `IUPAC-NIST Chemical Identifier&#39; (INChI), formerly IUPAC Chemical Identifier (IChI), designed to provide a standard and human-readable way to encode molecular structure.</rdfs:comment>
        <rdfs:domain rdf:resource="&bc;ChemicalSubstanceTypeByChemicalSpecies"/>
        <rdfs:subPropertyOf rdf:resource="&bc;hasStructuralChemicalFormula"/>
        <rdfs:subPropertyOf rdf:resource="&or;idString"/>
        <rdfs:range rdf:resource="&xsd;string"/>
    </owl:DatatypeProperty>
    


    <!-- http://www.nist.gov/itl/ssd/Materials#inChiKey -->

    <owl:DatatypeProperty rdf:about="&mat;inChiKey">
        <rdf:type rdf:resource="&owl;FunctionalProperty"/>
        <or:referenceURL rdf:datatype="&xsd;anyURI">http://www.iupac.org/namespaces/ThermoML#sStandardInChIKey</or:referenceURL>
        <rdfs:comment xml:lang="en">The InChIKey, a hashed versio of the IUPAC International Chemical Identifier (InChI).</rdfs:comment>
        <rdfs:domain rdf:resource="&bc;ChemicalSubstanceTypeByChemicalSpecies"/>
        <rdfs:subPropertyOf rdf:resource="&or;idString"/>
        <rdfs:range rdf:resource="&xsd;string"/>
    </owl:DatatypeProperty>
    


    <!-- http://www.nist.gov/itl/ssd/Materials#ionicCharge -->

    <owl:DatatypeProperty rdf:about="&mat;ionicCharge">
        <rdf:type rdf:resource="&owl;FunctionalProperty"/>
        <or:referenceURL rdf:datatype="&xsd;anyURI">http://www.iupac.org/namespaces/ThermoML#nCharge</or:referenceURL>
        <rdfs:domain rdf:resource="&bc;Ion"/>
        <rdfs:range rdf:resource="&xsd;integer"/>
    </owl:DatatypeProperty>
    


    <!-- http://www.nist.gov/itl/ssd/Materials#molarMassDispersity -->

    <owl:DatatypeProperty rdf:about="&mat;molarMassDispersity">
        <or:referenceURL rdf:datatype="&xsd;anyURI">http://www.iupac.org/namespaces/ThermoML#nMolarMassDispersity</or:referenceURL>
        <rdfs:range rdf:resource="&owl;real"/>
        <rdfs:domain>
            <owl:Class>
                <owl:unionOf rdf:parseType="Collection">
                    <rdf:Description rdf:about="&bc;Polymer"/>
                    <rdf:Description rdf:about="&mat;PolymerSubstance"/>
                </owl:unionOf>
            </owl:Class>
        </rdfs:domain>
    </owl:DatatypeProperty>
    


    <!-- http://www.nist.gov/itl/ssd/Materials#numberAverageMolarMass -->

    <owl:DatatypeProperty rdf:about="&mat;numberAverageMolarMass">
        <rdf:type rdf:resource="&owl;FunctionalProperty"/>
        <or:referenceURL rdf:datatype="&xsd;anyURI">http://www.iupac.org/namespaces/ThermoML#nNumberAvgMolMass</or:referenceURL>
        <rdfs:comment xml:lang="en">The number average molecular mass of a polymer.  The value can be interpreted as atomic mass units per molecule or as (kilo)grams per (kilo)mole of the polymer.</rdfs:comment>
        <rdfs:range rdf:resource="&owl;real"/>
        <rdfs:domain>
            <owl:Class>
                <owl:unionOf rdf:parseType="Collection">
                    <rdf:Description rdf:about="&bc;Polymer"/>
                    <rdf:Description rdf:about="&mat;PolymerSubstance"/>
                </owl:unionOf>
            </owl:Class>
        </rdfs:domain>
    </owl:DatatypeProperty>
    


    <!-- http://www.nist.gov/itl/ssd/Materials#pdbID -->

    <owl:DatatypeProperty rdf:about="&mat;pdbID">
        <rdf:type rdf:resource="&owl;FunctionalProperty"/>
        <or:referenceURL rdf:datatype="&xsd;anyURI">http://www.iupac.org/namespaces/ThermoML#sPDBIdentifier</or:referenceURL>
        <or:termString xml:lang="en">PDB ID</or:termString>
        <or:termString xml:lang="en">Protein Databank ID</or:termString>
        <rdfs:comment xml:lang="en">The property `pdbID&#39; specifies the Protein Data Bank ID for a compound</rdfs:comment>
        <rdfs:domain rdf:resource="&bc;ChemicalSubstanceTypeByChemicalSpecies"/>
        <rdfs:subPropertyOf rdf:resource="&or;idString"/>
        <rdfs:range rdf:resource="&xsd;string"/>
    </owl:DatatypeProperty>
    


    <!-- http://www.nist.gov/itl/ssd/Materials#peakAverageMolecularMass -->

    <owl:DatatypeProperty rdf:about="&mat;peakAverageMolecularMass">
        <rdf:type rdf:resource="&owl;FunctionalProperty"/>
        <or:referenceURL rdf:datatype="&xsd;anyURI">http://www.iupac.org/namespaces/ThermoML#nPeakAvgMolMass</or:referenceURL>
        <rdfs:comment xml:lang="en">The peak average molecular mass of a polymer.  An average is expressed because a volume of the polymer may have varying length or quantity of different monomers (e.g. nucleic acids).  The value can be interpreted as atomic mass units per molecule or as (kilo)grams per (kilo)mole of the polymer.</rdfs:comment>
        <rdfs:range rdf:resource="&owl;real"/>
        <rdfs:subPropertyOf rdf:resource="&owl;topDataProperty"/>
        <rdfs:domain>
            <owl:Class>
                <owl:unionOf rdf:parseType="Collection">
                    <rdf:Description rdf:about="&bc;Polymer"/>
                    <rdf:Description rdf:about="&mat;PolymerSubstance"/>
                </owl:unionOf>
            </owl:Class>
        </rdfs:domain>
    </owl:DatatypeProperty>
    


    <!-- http://www.nist.gov/itl/ssd/Materials#pubChemId -->

    <owl:DatatypeProperty rdf:about="&mat;pubChemId">
        <rdf:type rdf:resource="&owl;FunctionalProperty"/>
        <or:referenceURL rdf:datatype="&xsd;anyURI">http://www.iupac.org/namespaces/ThermoML#nPubChemID</or:referenceURL>
        <rdfs:domain rdf:resource="&bc;ChemicalSubstanceTypeByChemicalSpecies"/>
        <rdfs:subPropertyOf rdf:resource="&or;idString"/>
        <rdfs:range rdf:resource="&xsd;string"/>
    </owl:DatatypeProperty>
    


    <!-- http://www.nist.gov/itl/ssd/Materials#sMILESNotation -->

    <owl:DatatypeProperty rdf:about="&mat;sMILESNotation">
        <or:referenceURL rdf:datatype="&xsd;anyURI">http://www.iupac.org/namespaces/ThermoML#sSmiles</or:referenceURL>
        <or:termString xml:lang="en">SMILES notation</or:termString>
        <or:termString xml:lang="en">Simplified molecular-input line-entry system notation</or:termString>
        <rdfs:subPropertyOf rdf:resource="&bc;hasStructuralChemicalFormula"/>
        <rdfs:subPropertyOf rdf:resource="&or;idString"/>
    </owl:DatatypeProperty>
    


    <!-- http://www.nist.gov/itl/ssd/Materials#strunzClassification -->

    <owl:DatatypeProperty rdf:about="&mat;strunzClassification">
        <rdfs:comment xml:lang="en">The Strunz (or Nickel-Strunz) classification is a scheme for categorizing minerals based upon their chemical composition.  The predicate strunzClassification relates a mineratl to its Strunz classification code.</rdfs:comment>
        <rdfs:domain rdf:resource="&mat;MineralType"/>
        <rdfs:range rdf:resource="&rdf;PlainLiteral"/>
    </owl:DatatypeProperty>
    


    <!-- http://www.nist.gov/itl/ssd/Materials#uncertaintyConfidenceLevel -->

    <owl:DatatypeProperty rdf:about="&mat;uncertaintyConfidenceLevel">
        <rdfs:domain rdf:resource="&or;MeasurableQuantity"/>
        <rdfs:range rdf:resource="&xsd;float"/>
    </owl:DatatypeProperty>
    


    <!-- http://www.nist.gov/itl/ssd/Materials#viscosityAverageMolarMass -->

    <owl:DatatypeProperty rdf:about="&mat;viscosityAverageMolarMass">
        <rdf:type rdf:resource="&owl;FunctionalProperty"/>
        <or:referenceURL rdf:datatype="&xsd;anyURI">http://www.iupac.org/namespaces/ThermoML#nViscosityAvgMolMass</or:referenceURL>
        <rdfs:comment xml:lang="en">The Z- average molecular mass of a polymer.</rdfs:comment>
        <rdfs:range rdf:resource="&owl;real"/>
        <rdfs:domain>
            <owl:Class>
                <owl:unionOf rdf:parseType="Collection">
                    <rdf:Description rdf:about="&bc;Polymer"/>
                    <rdf:Description rdf:about="&mat;PolymerSubstance"/>
                </owl:unionOf>
            </owl:Class>
        </rdfs:domain>
    </owl:DatatypeProperty>
    


    <!-- http://www.nist.gov/itl/ssd/Materials#weightAverageMolarMass -->

    <owl:DatatypeProperty rdf:about="&mat;weightAverageMolarMass">
        <rdf:type rdf:resource="&owl;FunctionalProperty"/>
        <or:referenceURL rdf:datatype="&xsd;anyURI">http://www.iupac.org/namespaces/ThermoML#nMassAvgMolMass</or:referenceURL>
        <rdfs:comment xml:lang="en">The weight average molecular mass of a polymer.  The value can be interpreted as atomic mass units per molecule or as (kilo)grams per (kilo)mole of the polymer.</rdfs:comment>
        <or:termString xml:lang="en">mass average molar mass</or:termString>
        <or:termString xml:lang="en">weight average molar mass</or:termString>
        <rdfs:range rdf:resource="&owl;real"/>
        <rdfs:domain>
            <owl:Class>
                <owl:unionOf rdf:parseType="Collection">
                    <rdf:Description rdf:about="&bc;Polymer"/>
                    <rdf:Description rdf:about="&mat;PolymerSubstance"/>
                </owl:unionOf>
            </owl:Class>
        </rdfs:domain>
    </owl:DatatypeProperty>
    


    <!-- http://www.nist.gov/itl/ssd/OntologyRequirements#nickName -->

    <owl:DatatypeProperty rdf:about="&or;nickName"/>
    


    <!-- 
    ///////////////////////////////////////////////////////////////////////////////////////
    //
    // Classes
    //
    ///////////////////////////////////////////////////////////////////////////////////////
     -->

    


    <!-- http://www.nist.gov/itl/ssd/Biochem#Actinium -->

    <rdf:Description rdf:about="&bc;Actinium">
        <rdfs:subClassOf rdf:resource="&mat;ElementalMetal"/>
    </rdf:Description>
    


    <!-- http://www.nist.gov/itl/ssd/Biochem#Aluminum -->

    <rdf:Description rdf:about="&bc;Aluminum">
        <rdfs:subClassOf rdf:resource="&mat;ElementalMetal"/>
    </rdf:Description>
    


    <!-- http://www.nist.gov/itl/ssd/Biochem#Americium -->

    <rdf:Description rdf:about="&bc;Americium">
        <rdfs:subClassOf rdf:resource="&mat;ElementalMetal"/>
    </rdf:Description>
    


    <!-- http://www.nist.gov/itl/ssd/Biochem#Atom -->

    <rdf:Description rdf:about="&bc;Atom">
        <owl:disjointWith rdf:resource="&bc;Polymer"/>
    </rdf:Description>
    


    <!-- http://www.nist.gov/itl/ssd/Biochem#Berkelium -->

    <rdf:Description rdf:about="&bc;Berkelium">
        <rdfs:subClassOf rdf:resource="&mat;ElementalMetal"/>
    </rdf:Description>
    


    <!-- http://www.nist.gov/itl/ssd/Biochem#Beryllium -->

    <rdf:Description rdf:about="&bc;Beryllium">
        <rdfs:subClassOf rdf:resource="&mat;ElementalMetal"/>
    </rdf:Description>
    


    <!-- http://www.nist.gov/itl/ssd/Biochem#BiologicalProcess -->

    <rdf:Description rdf:about="&bc;BiologicalProcess">
        <owl:disjointWith rdf:resource="&mat;MicrostructureEvolution"/>
        <owl:disjointWith rdf:resource="&or;MechanicalProcess"/>
    </rdf:Description>
    


    <!-- http://www.nist.gov/itl/ssd/Biochem#BiologicalProperty -->

    <rdf:Description rdf:about="&bc;BiologicalProperty">
        <owl:disjointWith rdf:resource="&bc;ChemicalProperty"/>
    </rdf:Description>
    


    <!-- http://www.nist.gov/itl/ssd/Biochem#Bismuth -->

    <rdf:Description rdf:about="&bc;Bismuth">
        <rdfs:subClassOf rdf:resource="&mat;ElementalMetal"/>
    </rdf:Description>
    


    <!-- http://www.nist.gov/itl/ssd/Biochem#Bohrium -->

    <rdf:Description rdf:about="&bc;Bohrium">
        <rdfs:subClassOf rdf:resource="&mat;ElementalMetal"/>
    </rdf:Description>
    


    <!-- http://www.nist.gov/itl/ssd/Biochem#Cadmium -->

    <rdf:Description rdf:about="&bc;Cadmium">
        <rdfs:subClassOf rdf:resource="&mat;ElementalMetal"/>
    </rdf:Description>
    


    <!-- http://www.nist.gov/itl/ssd/Biochem#Calcium -->

    <rdf:Description rdf:about="&bc;Calcium">
        <rdfs:subClassOf rdf:resource="&mat;ElementalMetal"/>
    </rdf:Description>
    


    <!-- http://www.nist.gov/itl/ssd/Biochem#Californium -->

    <rdf:Description rdf:about="&bc;Californium">
        <rdfs:subClassOf rdf:resource="&mat;ElementalMetal"/>
    </rdf:Description>
    


    <!-- http://www.nist.gov/itl/ssd/Biochem#Cerium -->

    <rdf:Description rdf:about="&bc;Cerium">
        <rdfs:subClassOf rdf:resource="&mat;ElementalMetal"/>
    </rdf:Description>
    


    <!-- http://www.nist.gov/itl/ssd/Biochem#Cesium -->

    <rdf:Description rdf:about="&bc;Cesium">
        <rdfs:subClassOf rdf:resource="&mat;ElementalMetal"/>
    </rdf:Description>
    


    <!-- http://www.nist.gov/itl/ssd/Biochem#ChemicalObject -->

    <rdf:Description rdf:about="&bc;ChemicalObject">
        <owl:disjointWith rdf:resource="&mat;Vacuum"/>
    </rdf:Description>
    


    <!-- http://www.nist.gov/itl/ssd/Biochem#ChemicalObjectType -->

    <owl:Class rdf:about="&bc;ChemicalObjectType">
        <owl:disjointWith rdf:resource="&mat;MineralType"/>
        <rdfs:comment xml:lang="en">A Chemical Object Type is a class of chemicals defined by their chemical structure.  Instances include fully specified chemical compounds, such as H2O and generic types such as Ketone and DNA.

The more specific class, Chemical Object Type By Chemical Species, denotes the fully-specified compounds (other than stereoisomers).</rdfs:comment>
    </owl:Class>
    


    <!-- http://www.nist.gov/itl/ssd/Biochem#ChemicalObjectTypeByChemicalSpecies -->

    <owl:Class rdf:about="&bc;ChemicalObjectTypeByChemicalSpecies"/>
    


    <!-- http://www.nist.gov/itl/ssd/Biochem#ChemicalProperty -->

    <rdf:Description rdf:about="&bc;ChemicalProperty">
        <owl:disjointWith rdf:resource="&mat;MeasurableMechanicalProperty"/>
        <skos:note xml:lang="en">Similar to &quot;Chemical&quot; in Ashino&#39;s 2010 Minerals Ontology.</skos:note>
    </rdf:Description>
    


    <!-- http://www.nist.gov/itl/ssd/Biochem#ChemicalSubstance -->

    <rdf:Description rdf:about="&bc;ChemicalSubstance">
        <owl:disjointWith rdf:resource="&mat;CompositeMaterial"/>
        <owl:disjointWith rdf:resource="&mat;Vacuum"/>
    </rdf:Description>
    


    <!-- http://www.nist.gov/itl/ssd/Biochem#ChemicalSubstanceTypeByChemicalSpecies -->

    <rdf:Description rdf:about="&bc;ChemicalSubstanceTypeByChemicalSpecies">
        <or:referenceURL rdf:datatype="&xsd;anyURI">http://sw.opencyc.org/2012/05/10/concept/en/ChemicalCompoundTypeByChemicalSpecies</or:referenceURL>
        <or:referenceURL rdf:datatype="&xsd;anyURI">http://www.iupac.org/namespaces/ThermoML#Compound</or:referenceURL>
    </rdf:Description>
    


    <!-- http://www.nist.gov/itl/ssd/Biochem#Chromium -->

    <rdf:Description rdf:about="&bc;Chromium">
        <rdfs:subClassOf rdf:resource="&mat;ElementalMetal"/>
    </rdf:Description>
    


    <!-- http://www.nist.gov/itl/ssd/Biochem#Cobalt -->

    <rdf:Description rdf:about="&bc;Cobalt">
        <rdfs:subClassOf rdf:resource="&mat;ElementalMetal"/>
    </rdf:Description>
    


    <!-- http://www.nist.gov/itl/ssd/Biochem#Copernicium -->

    <owl:Class rdf:about="&bc;Copernicium">
        <rdfs:subClassOf rdf:resource="&mat;ElementalMetal"/>
    </owl:Class>
    


    <!-- http://www.nist.gov/itl/ssd/Biochem#Copper -->

    <rdf:Description rdf:about="&bc;Copper">
        <rdfs:subClassOf rdf:resource="&mat;ElementalMetal"/>
    </rdf:Description>
    


    <!-- http://www.nist.gov/itl/ssd/Biochem#Curium -->

    <rdf:Description rdf:about="&bc;Curium">
        <rdfs:subClassOf rdf:resource="&mat;ElementalMetal"/>
    </rdf:Description>
    


    <!-- http://www.nist.gov/itl/ssd/Biochem#Dubnium -->

    <rdf:Description rdf:about="&bc;Dubnium">
        <rdfs:subClassOf rdf:resource="&mat;ElementalMetal"/>
    </rdf:Description>
    


    <!-- http://www.nist.gov/itl/ssd/Biochem#Dysprosium -->

    <rdf:Description rdf:about="&bc;Dysprosium">
        <rdfs:subClassOf rdf:resource="&mat;ElementalMetal"/>
    </rdf:Description>
    


    <!-- http://www.nist.gov/itl/ssd/Biochem#Einsteinium -->

    <rdf:Description rdf:about="&bc;Einsteinium">
        <rdfs:subClassOf rdf:resource="&mat;ElementalMetal"/>
    </rdf:Description>
    


    <!-- http://www.nist.gov/itl/ssd/Biochem#ElementalSubstance -->

    <rdf:Description rdf:about="&bc;ElementalSubstance">
        <owl:disjointWith rdf:resource="&mat;Boride"/>
        <owl:disjointWith rdf:resource="&mat;Carbide"/>
        <owl:disjointWith rdf:resource="&mat;Halide"/>
    </rdf:Description>
    


    <!-- http://www.nist.gov/itl/ssd/Biochem#Erbium -->

    <rdf:Description rdf:about="&bc;Erbium">
        <rdfs:subClassOf rdf:resource="&mat;ElementalMetal"/>
    </rdf:Description>
    


    <!-- http://www.nist.gov/itl/ssd/Biochem#Europium -->

    <rdf:Description rdf:about="&bc;Europium">
        <rdfs:subClassOf rdf:resource="&mat;ElementalMetal"/>
    </rdf:Description>
    


    <!-- http://www.nist.gov/itl/ssd/Biochem#Fermium -->

    <rdf:Description rdf:about="&bc;Fermium">
        <rdfs:subClassOf rdf:resource="&mat;ElementalMetal"/>
    </rdf:Description>
    


    <!-- http://www.nist.gov/itl/ssd/Biochem#Francium -->

    <rdf:Description rdf:about="&bc;Francium">
        <rdfs:subClassOf rdf:resource="&mat;ElementalMetal"/>
    </rdf:Description>
    


    <!-- http://www.nist.gov/itl/ssd/Biochem#Gadolinium -->

    <rdf:Description rdf:about="&bc;Gadolinium">
        <rdfs:subClassOf rdf:resource="&mat;ElementalMetal"/>
    </rdf:Description>
    


    <!-- http://www.nist.gov/itl/ssd/Biochem#Gallium -->

    <rdf:Description rdf:about="&bc;Gallium">
        <rdfs:subClassOf rdf:resource="&mat;ElementalMetal"/>
    </rdf:Description>
    


    <!-- http://www.nist.gov/itl/ssd/Biochem#Gold -->

    <rdf:Description rdf:about="&bc;Gold">
        <rdfs:subClassOf rdf:resource="&mat;ElementalMetal"/>
    </rdf:Description>
    


    <!-- http://www.nist.gov/itl/ssd/Biochem#Hafnium -->

    <rdf:Description rdf:about="&bc;Hafnium">
        <rdfs:subClassOf rdf:resource="&mat;ElementalMetal"/>
    </rdf:Description>
    


    <!-- http://www.nist.gov/itl/ssd/Biochem#Hassium -->

    <rdf:Description rdf:about="&bc;Hassium">
        <rdfs:subClassOf rdf:resource="&mat;ElementalMetal"/>
    </rdf:Description>
    


    <!-- http://www.nist.gov/itl/ssd/Biochem#Holmium -->

    <rdf:Description rdf:about="&bc;Holmium">
        <rdfs:subClassOf rdf:resource="&mat;ElementalMetal"/>
    </rdf:Description>
    


    <!-- http://www.nist.gov/itl/ssd/Biochem#Indium -->

    <rdf:Description rdf:about="&bc;Indium">
        <rdfs:subClassOf rdf:resource="&mat;ElementalMetal"/>
    </rdf:Description>
    


    <!-- http://www.nist.gov/itl/ssd/Biochem#Ion -->

    <rdf:Description rdf:about="&bc;Ion">
        <or:referenceURL rdf:datatype="&xsd;anyURI">http://www.iupac.org/namespaces/ThermoML#ion</or:referenceURL>
    </rdf:Description>
    


    <!-- http://www.nist.gov/itl/ssd/Biochem#Iridium -->

    <rdf:Description rdf:about="&bc;Iridium">
        <rdfs:subClassOf rdf:resource="&mat;ElementalMetal"/>
    </rdf:Description>
    


    <!-- http://www.nist.gov/itl/ssd/Biochem#Iron -->

    <rdf:Description rdf:about="&bc;Iron">
        <rdfs:subClassOf rdf:resource="&mat;ElementalMetal"/>
    </rdf:Description>
    


    <!-- http://www.nist.gov/itl/ssd/Biochem#Lanthanum -->

    <rdf:Description rdf:about="&bc;Lanthanum">
        <rdfs:subClassOf rdf:resource="&mat;ElementalMetal"/>
    </rdf:Description>
    


    <!-- http://www.nist.gov/itl/ssd/Biochem#Lawrencium -->

    <rdf:Description rdf:about="&bc;Lawrencium">
        <rdfs:subClassOf rdf:resource="&mat;ElementalMetal"/>
    </rdf:Description>
    


    <!-- http://www.nist.gov/itl/ssd/Biochem#Lead -->

    <rdf:Description rdf:about="&bc;Lead">
        <rdfs:subClassOf rdf:resource="&mat;ElementalMetal"/>
    </rdf:Description>
    


    <!-- http://www.nist.gov/itl/ssd/Biochem#Lithium -->

    <rdf:Description rdf:about="&bc;Lithium">
        <rdfs:subClassOf rdf:resource="&mat;ElementalMetal"/>
    </rdf:Description>
    


    <!-- http://www.nist.gov/itl/ssd/Biochem#Lutetium -->

    <rdf:Description rdf:about="&bc;Lutetium">
        <rdfs:subClassOf rdf:resource="&mat;ElementalMetal"/>
    </rdf:Description>
    


    <!-- http://www.nist.gov/itl/ssd/Biochem#Magnesium -->

    <rdf:Description rdf:about="&bc;Magnesium">
        <rdfs:subClassOf rdf:resource="&mat;ElementalMetal"/>
    </rdf:Description>
    


    <!-- http://www.nist.gov/itl/ssd/Biochem#Manganese -->

    <rdf:Description rdf:about="&bc;Manganese">
        <rdfs:subClassOf rdf:resource="&mat;ElementalMetal"/>
    </rdf:Description>
    


    <!-- http://www.nist.gov/itl/ssd/Biochem#Mendelevium -->

    <rdf:Description rdf:about="&bc;Mendelevium">
        <rdfs:subClassOf rdf:resource="&mat;ElementalMetal"/>
    </rdf:Description>
    


    <!-- http://www.nist.gov/itl/ssd/Biochem#Mercury -->

    <rdf:Description rdf:about="&bc;Mercury">
        <rdfs:subClassOf rdf:resource="&mat;ElementalMetal"/>
    </rdf:Description>
    


    <!-- http://www.nist.gov/itl/ssd/Biochem#Metal -->

    <rdf:Description rdf:about="&bc;Metal">
        <owl:disjointWith rdf:resource="&mat;LiquidSlag"/>
        <owl:disjointWith rdf:resource="&mat;Semiconductor"/>
        <owl:disjointWith rdf:resource="&mat;Vacuum"/>
        <or:referenceURL rdf:datatype="&xsd;anyURI">http://www.matweb.com/index.aspx</or:referenceURL>
        <or:termString xml:lang="en">metal</or:termString>
    </rdf:Description>
    


    <!-- http://www.nist.gov/itl/ssd/Biochem#Molybdenum -->

    <rdf:Description rdf:about="&bc;Molybdenum">
        <rdfs:subClassOf rdf:resource="&mat;ElementalMetal"/>
    </rdf:Description>
    


    <!-- http://www.nist.gov/itl/ssd/Biochem#Neodymium -->

    <rdf:Description rdf:about="&bc;Neodymium">
        <rdfs:subClassOf rdf:resource="&mat;ElementalMetal"/>
    </rdf:Description>
    


    <!-- http://www.nist.gov/itl/ssd/Biochem#Neptunium -->

    <rdf:Description rdf:about="&bc;Neptunium">
        <rdfs:subClassOf rdf:resource="&mat;ElementalMetal"/>
    </rdf:Description>
    


    <!-- http://www.nist.gov/itl/ssd/Biochem#Nickel -->

    <rdf:Description rdf:about="&bc;Nickel">
        <rdfs:subClassOf rdf:resource="&mat;ElementalMetal"/>
    </rdf:Description>
    


    <!-- http://www.nist.gov/itl/ssd/Biochem#Niobium -->

    <rdf:Description rdf:about="&bc;Niobium">
        <rdfs:subClassOf rdf:resource="&mat;ElementalMetal"/>
    </rdf:Description>
    


    <!-- http://www.nist.gov/itl/ssd/Biochem#Nobelium -->

    <rdf:Description rdf:about="&bc;Nobelium">
        <rdfs:subClassOf rdf:resource="&mat;ElementalMetal"/>
    </rdf:Description>
    


    <!-- http://www.nist.gov/itl/ssd/Biochem#Osmium -->

    <rdf:Description rdf:about="&bc;Osmium">
        <rdfs:subClassOf rdf:resource="&mat;ElementalMetal"/>
    </rdf:Description>
    


    <!-- http://www.nist.gov/itl/ssd/Biochem#Oxide -->

    <owl:Class rdf:about="&bc;Oxide">
        <rdfs:subClassOf rdf:resource="&mat;PureSubstance"/>
        <owl:disjointWith rdf:resource="&mat;Boride"/>
        <owl:disjointWith rdf:resource="&mat;Carbide"/>
        <owl:disjointWith rdf:resource="&mat;Clathrate"/>
    </owl:Class>
    


    <!-- http://www.nist.gov/itl/ssd/Biochem#Palladium -->

    <rdf:Description rdf:about="&bc;Palladium">
        <rdfs:subClassOf rdf:resource="&mat;ElementalMetal"/>
    </rdf:Description>
    


    <!-- http://www.nist.gov/itl/ssd/Biochem#Platinum -->

    <rdf:Description rdf:about="&bc;Platinum">
        <rdfs:subClassOf rdf:resource="&mat;ElementalMetal"/>
    </rdf:Description>
    


    <!-- http://www.nist.gov/itl/ssd/Biochem#Plutonium -->

    <rdf:Description rdf:about="&bc;Plutonium">
        <rdfs:subClassOf rdf:resource="&mat;ElementalMetal"/>
    </rdf:Description>
    


    <!-- http://www.nist.gov/itl/ssd/Biochem#Polymer -->

    <rdf:Description rdf:about="&bc;Polymer">
        <owl:disjointWith rdf:resource="&mat;Fullerine"/>
        <or:referenceURL rdf:datatype="&xsd;anyURI">http://www.iupac.org/namespaces/ThermoML#polymer</or:referenceURL>
    </rdf:Description>
    


    <!-- http://www.nist.gov/itl/ssd/Biochem#Potassium -->

    <rdf:Description rdf:about="&bc;Potassium">
        <rdfs:subClassOf rdf:resource="&mat;ElementalMetal"/>
    </rdf:Description>
    


    <!-- http://www.nist.gov/itl/ssd/Biochem#Praseodymium -->

    <rdf:Description rdf:about="&bc;Praseodymium">
        <rdfs:subClassOf rdf:resource="&mat;ElementalMetal"/>
    </rdf:Description>
    


    <!-- http://www.nist.gov/itl/ssd/Biochem#Promethium -->

    <rdf:Description rdf:about="&bc;Promethium">
        <rdfs:subClassOf rdf:resource="&mat;ElementalMetal"/>
    </rdf:Description>
    


    <!-- http://www.nist.gov/itl/ssd/Biochem#Protactinium -->

    <rdf:Description rdf:about="&bc;Protactinium">
        <rdfs:subClassOf rdf:resource="&mat;ElementalMetal"/>
    </rdf:Description>
    


    <!-- http://www.nist.gov/itl/ssd/Biochem#ProteinTypeByStructure -->

    <owl:Class rdf:about="&bc;ProteinTypeByStructure">
        <rdfs:subClassOf rdf:resource="&mat;PolymericMicrostructure"/>
    </owl:Class>
    


    <!-- http://www.nist.gov/itl/ssd/Biochem#Radium -->

    <rdf:Description rdf:about="&bc;Radium">
        <rdfs:subClassOf rdf:resource="&mat;ElementalMetal"/>
    </rdf:Description>
    


    <!-- http://www.nist.gov/itl/ssd/Biochem#Rhenium -->

    <rdf:Description rdf:about="&bc;Rhenium">
        <rdfs:subClassOf rdf:resource="&mat;ElementalMetal"/>
    </rdf:Description>
    


    <!-- http://www.nist.gov/itl/ssd/Biochem#Rhodium -->

    <rdf:Description rdf:about="&bc;Rhodium">
        <rdfs:subClassOf rdf:resource="&mat;ElementalMetal"/>
    </rdf:Description>
    


    <!-- http://www.nist.gov/itl/ssd/Biochem#Rubidium -->

    <rdf:Description rdf:about="&bc;Rubidium">
        <rdfs:subClassOf rdf:resource="&mat;ElementalMetal"/>
    </rdf:Description>
    


    <!-- http://www.nist.gov/itl/ssd/Biochem#Ruthenium -->

    <rdf:Description rdf:about="&bc;Ruthenium">
        <rdfs:subClassOf rdf:resource="&mat;ElementalMetal"/>
    </rdf:Description>
    


    <!-- http://www.nist.gov/itl/ssd/Biochem#Rutherfordium -->

    <rdf:Description rdf:about="&bc;Rutherfordium">
        <rdfs:subClassOf rdf:resource="&mat;ElementalMetal"/>
    </rdf:Description>
    


    <!-- http://www.nist.gov/itl/ssd/Biochem#Samarium -->

    <rdf:Description rdf:about="&bc;Samarium">
        <rdfs:subClassOf rdf:resource="&mat;ElementalMetal"/>
    </rdf:Description>
    


    <!-- http://www.nist.gov/itl/ssd/Biochem#Scandium -->

    <rdf:Description rdf:about="&bc;Scandium">
        <rdfs:subClassOf rdf:resource="&mat;ElementalMetal"/>
    </rdf:Description>
    


    <!-- http://www.nist.gov/itl/ssd/Biochem#Seaborgium -->

    <rdf:Description rdf:about="&bc;Seaborgium">
        <rdfs:subClassOf rdf:resource="&mat;ElementalMetal"/>
    </rdf:Description>
    


    <!-- http://www.nist.gov/itl/ssd/Biochem#Silver -->

    <rdf:Description rdf:about="&bc;Silver">
        <rdfs:subClassOf rdf:resource="&mat;ElementalMetal"/>
    </rdf:Description>
    


    <!-- http://www.nist.gov/itl/ssd/Biochem#Sodium -->

    <rdf:Description rdf:about="&bc;Sodium">
        <rdfs:subClassOf rdf:resource="&mat;ElementalMetal"/>
    </rdf:Description>
    


    <!-- http://www.nist.gov/itl/ssd/Biochem#Strontium -->

    <rdf:Description rdf:about="&bc;Strontium">
        <rdfs:subClassOf rdf:resource="&mat;ElementalMetal"/>
    </rdf:Description>
    


    <!-- http://www.nist.gov/itl/ssd/Biochem#Tantalum -->

    <rdf:Description rdf:about="&bc;Tantalum">
        <rdfs:subClassOf rdf:resource="&mat;ElementalMetal"/>
    </rdf:Description>
    


    <!-- http://www.nist.gov/itl/ssd/Biochem#Technetium -->

    <rdf:Description rdf:about="&bc;Technetium">
        <rdfs:subClassOf rdf:resource="&mat;ElementalMetal"/>
    </rdf:Description>
    


    <!-- http://www.nist.gov/itl/ssd/Biochem#Terbium -->

    <rdf:Description rdf:about="&bc;Terbium">
        <rdfs:subClassOf rdf:resource="&mat;ElementalMetal"/>
    </rdf:Description>
    


    <!-- http://www.nist.gov/itl/ssd/Biochem#Thallium -->

    <rdf:Description rdf:about="&bc;Thallium">
        <rdfs:subClassOf rdf:resource="&mat;ElementalMetal"/>
    </rdf:Description>
    


    <!-- http://www.nist.gov/itl/ssd/Biochem#Thorium -->

    <rdf:Description rdf:about="&bc;Thorium">
        <rdfs:subClassOf rdf:resource="&mat;ElementalMetal"/>
    </rdf:Description>
    


    <!-- http://www.nist.gov/itl/ssd/Biochem#Thulium -->

    <rdf:Description rdf:about="&bc;Thulium">
        <rdfs:subClassOf rdf:resource="&mat;ElementalMetal"/>
    </rdf:Description>
    


    <!-- http://www.nist.gov/itl/ssd/Biochem#Tin -->

    <rdf:Description rdf:about="&bc;Tin">
        <rdfs:subClassOf rdf:resource="&mat;ElementalMetal"/>
    </rdf:Description>
    


    <!-- http://www.nist.gov/itl/ssd/Biochem#Titanium -->

    <rdf:Description rdf:about="&bc;Titanium">
        <rdfs:subClassOf rdf:resource="&mat;ElementalMetal"/>
    </rdf:Description>
    


    <!-- http://www.nist.gov/itl/ssd/Biochem#Tungsten -->

    <rdf:Description rdf:about="&bc;Tungsten">
        <rdfs:subClassOf rdf:resource="&mat;ElementalMetal"/>
    </rdf:Description>
    


    <!-- http://www.nist.gov/itl/ssd/Biochem#UnitOfConcentration -->

    <rdf:Description rdf:about="&bc;UnitOfConcentration">
        <owl:disjointWith rdf:resource="&mat;UnitOfCharge"/>
        <owl:disjointWith rdf:resource="&mat;UnitOfElectricCurrent"/>
        <owl:disjointWith rdf:resource="&mat;UnitOfElectricalConductivity"/>
        <owl:disjointWith rdf:resource="&mat;UnitOfInverseAreaPerTime"/>
        <owl:disjointWith rdf:resource="&mat;UnitOfSpecificHeatCapacity"/>
    </rdf:Description>
    


    <!-- http://www.nist.gov/itl/ssd/Biochem#UnitOfConcentrationByMass -->

    <rdf:Description rdf:about="&bc;UnitOfConcentrationByMass">
        <owl:disjointWith rdf:resource="&bc;UnitOfConcentrationByVolume"/>
    </rdf:Description>
    


    <!-- http://www.nist.gov/itl/ssd/Biochem#UnitOfConcentrationByVolume -->

    <rdf:Description rdf:about="&bc;UnitOfConcentrationByVolume"/>
    


    <!-- http://www.nist.gov/itl/ssd/Biochem#Uranium -->

    <rdf:Description rdf:about="&bc;Uranium">
        <rdfs:subClassOf rdf:resource="&mat;ElementalMetal"/>
    </rdf:Description>
    


    <!-- http://www.nist.gov/itl/ssd/Biochem#Vanadium -->

    <rdf:Description rdf:about="&bc;Vanadium">
        <rdfs:subClassOf rdf:resource="&mat;ElementalMetal"/>
    </rdf:Description>
    


    <!-- http://www.nist.gov/itl/ssd/Biochem#Water -->

    <rdf:Description rdf:about="&bc;Water">
        <owl:disjointWith rdf:resource="&mat;AluminumOxide"/>
        <owl:disjointWith rdf:resource="&mat;MagnesiumOxide"/>
        <owl:disjointWith rdf:resource="&mat;SiliconOxide"/>
        <owl:disjointWith rdf:resource="&mat;TitaniumOxide"/>
        <owl:disjointWith rdf:resource="&mat;ZirconiumOxide"/>
    </rdf:Description>
    


    <!-- http://www.nist.gov/itl/ssd/Biochem#Ytterbium -->

    <rdf:Description rdf:about="&bc;Ytterbium">
        <rdfs:subClassOf rdf:resource="&mat;ElementalMetal"/>
    </rdf:Description>
    


    <!-- http://www.nist.gov/itl/ssd/Biochem#Yttrium -->

    <rdf:Description rdf:about="&bc;Yttrium">
        <rdfs:subClassOf rdf:resource="&mat;ElementalMetal"/>
    </rdf:Description>
    


    <!-- http://www.nist.gov/itl/ssd/Biochem#Zinc -->

    <rdf:Description rdf:about="&bc;Zinc">
        <rdfs:subClassOf rdf:resource="&mat;ElementalMetal"/>
    </rdf:Description>
    


    <!-- http://www.nist.gov/itl/ssd/Biochem#Zirconium -->

    <rdf:Description rdf:about="&bc;Zirconium">
        <rdfs:subClassOf rdf:resource="&mat;ElementalMetal"/>
    </rdf:Description>
    


    <!-- http://www.nist.gov/itl/ssd/Document#MakingAPrediction -->

    <rdf:Description rdf:about="&doc;MakingAPrediction">
        <owl:disjointWith rdf:resource="&or;Designing"/>
        <owl:disjointWith rdf:resource="&or;Manufacturing"/>
    </rdf:Description>
    


    <!-- http://www.nist.gov/itl/ssd/Experiments#Experiment -->

    <owl:Class rdf:about="&exp;Experiment">
        <rdfs:subClassOf rdf:resource="&or;IntentionalCreation"/>
        <rdfs:subClassOf>
            <owl:Restriction>
                <owl:onProperty rdf:resource="&or;subEvents"/>
                <owl:someValuesFrom rdf:resource="&or;DataCollection"/>
            </owl:Restriction>
        </rdfs:subClassOf>
        <owl:disjointWith rdf:resource="&or;Designing"/>
        <owl:disjointWith rdf:resource="&or;Development"/>
        <owl:disjointWith rdf:resource="&or;Manufacturing"/>
    </owl:Class>
    


    <!-- http://www.nist.gov/itl/ssd/Materials#AISI4000SeriesSteel -->

    <owl:Class rdf:about="&mat;AISI4000SeriesSteel">
        <rdfs:subClassOf rdf:resource="&mat;AlloySteel"/>
        <owl:disjointWith rdf:resource="&mat;AISI5000SeriesSteel"/>
        <owl:disjointWith rdf:resource="&mat;AISI6000SeriesSteel"/>
        <owl:disjointWith rdf:resource="&mat;AISI8000SeriesSteel"/>
        <owl:disjointWith rdf:resource="&mat;AISI9000SeriesSteel"/>
        <or:referenceURL rdf:datatype="&xsd;anyURI">http://www.matweb.com/index.aspx</or:referenceURL>
        <or:termString xml:lang="en">AISI 4000 series Steel</or:termString>
    </owl:Class>
    


    <!-- http://www.nist.gov/itl/ssd/Materials#AISI5000SeriesSteel -->

    <owl:Class rdf:about="&mat;AISI5000SeriesSteel">
        <rdfs:subClassOf rdf:resource="&mat;AlloySteel"/>
        <owl:disjointWith rdf:resource="&mat;AISI6000SeriesSteel"/>
        <owl:disjointWith rdf:resource="&mat;AISI8000SeriesSteel"/>
        <owl:disjointWith rdf:resource="&mat;AISI9000SeriesSteel"/>
        <or:referenceURL rdf:datatype="&xsd;anyURI">http://www.matweb.com/index.aspx</or:referenceURL>
        <or:termString xml:lang="en">AISI 5000 series Steel</or:termString>
    </owl:Class>
    


    <!-- http://www.nist.gov/itl/ssd/Materials#AISI6000SeriesSteel -->

    <owl:Class rdf:about="&mat;AISI6000SeriesSteel">
        <rdfs:subClassOf rdf:resource="&mat;AlloySteel"/>
        <owl:disjointWith rdf:resource="&mat;AISI8000SeriesSteel"/>
        <owl:disjointWith rdf:resource="&mat;AISI9000SeriesSteel"/>
        <or:referenceURL rdf:datatype="&xsd;anyURI">http://www.matweb.com/index.aspx</or:referenceURL>
        <or:termString xml:lang="en">AISI 6000 series Steel</or:termString>
    </owl:Class>
    


    <!-- http://www.nist.gov/itl/ssd/Materials#AISI8000SeriesSteel -->

    <owl:Class rdf:about="&mat;AISI8000SeriesSteel">
        <rdfs:subClassOf rdf:resource="&mat;AlloySteel"/>
        <owl:disjointWith rdf:resource="&mat;AISI9000SeriesSteel"/>
        <or:referenceURL rdf:datatype="&xsd;anyURI">http://www.matweb.com/index.aspx</or:referenceURL>
    </owl:Class>
    


    <!-- http://www.nist.gov/itl/ssd/Materials#AISI9000SeriesSteel -->

    <owl:Class rdf:about="&mat;AISI9000SeriesSteel">
        <rdfs:subClassOf rdf:resource="&mat;AlloySteel"/>
        <or:referenceURL rdf:datatype="&xsd;anyURI">http://www.matweb.com/index.aspx</or:referenceURL>
        <or:termString xml:lang="en">AISI 9000 series steel</or:termString>
    </owl:Class>
    


    <!-- http://www.nist.gov/itl/ssd/Materials#ASTMSteel -->

    <owl:Class rdf:about="&mat;ASTMSteel">
        <rdfs:subClassOf rdf:resource="&mat;Steel"/>
        <or:referenceURL rdf:datatype="&xsd;anyURI">http://www.matweb.com/index.aspx</or:referenceURL>
        <rdfs:comment xml:lang="en">ASTM Steel is steel that has been graded by ASTM and meets certain performance requirements.  Different ASTM steels may be alloy steel, carbon steel, stainless steel, forged, heat treated, etc.</rdfs:comment>
        <or:termString xml:lang="en">ASTM steel</or:termString>
    </owl:Class>
    


    <!-- http://www.nist.gov/itl/ssd/Materials#AcousticProperty -->

    <owl:Class rdf:about="&mat;AcousticProperty">
        <rdfs:subClassOf rdf:resource="&or;MeasurableMaterialProperty"/>
        <owl:disjointWith rdf:resource="&mat;ElectricalProperty"/>
        <owl:disjointWith rdf:resource="&mat;MagneticProperty"/>
        <owl:disjointWith rdf:resource="&mat;MechanicalProperty"/>
        <owl:disjointWith rdf:resource="&mat;OpticalProperty"/>
        <owl:disjointWith rdf:resource="&mat;RadiologicalProperty"/>
        <owl:disjointWith rdf:resource="&mat;ThermalProperty"/>
        <owl:disjointWith rdf:resource="&mat;ThermochemicalProperty"/>
    </owl:Class>
    


    <!-- http://www.nist.gov/itl/ssd/Materials#Aerogel -->

    <owl:Class rdf:about="&mat;Aerogel">
        <rdfs:subClassOf rdf:resource="&mat;Ceramic"/>
        <rdfs:subClassOf rdf:resource="&mat;EngineeredMaterial"/>
        <or:referenceURL rdf:datatype="&xsd;anyURI">http://www.matweb.com/index.aspx</or:referenceURL>
        <rdfs:comment xml:lang="en">Aerogel is a synthetic porous ultralight solid with extremely low density and thermal conductivity derived from a gel through supercritical drying, in which the liquid component of the gel has been replaced with a gas.</rdfs:comment>
        <or:termString xml:lang="en">aerogel</or:termString>
    </owl:Class>
    


    <!-- http://www.nist.gov/itl/ssd/Materials#Aerosol -->

    <owl:Class rdf:about="&mat;Aerosol">
        <rdfs:subClassOf rdf:resource="&mat;Colloid"/>
        <rdfs:subClassOf rdf:resource="&mat;ComplexFluid"/>
        <rdfs:subClassOf rdf:resource="&mat;GaseousSubstance"/>
        <owl:disjointWith rdf:resource="&mat;Alloy"/>
        <owl:disjointWith rdf:resource="&mat;ColloidalSol"/>
        <owl:disjointWith rdf:resource="&mat;Emulsion"/>
        <owl:disjointWith rdf:resource="&mat;Foam"/>
        <owl:disjointWith rdf:resource="&mat;GasMixture"/>
        <owl:disjointWith rdf:resource="&mat;GelSubstance"/>
        <rdfs:comment xml:lang="en">An aerosol is a colloid suspension of fine solid particles or liquid droplets in a pure gas or Gas Mixture.</rdfs:comment>
    </owl:Class>
    


    <!-- http://www.nist.gov/itl/ssd/Materials#AlkylCelluloseEthers -->

    <owl:Class rdf:about="&mat;AlkylCelluloseEthers">
        <rdfs:subClassOf rdf:resource="&mat;CelluloseEther"/>
        <owl:disjointWith rdf:resource="&mat;CarboxymethylCellulose"/>
        <owl:disjointWith rdf:resource="&mat;HydroxyalkylCelluloseEther"/>
    </owl:Class>
    


    <!-- http://www.nist.gov/itl/ssd/Materials#AlkylatedNaphthalene -->

    <owl:Class rdf:about="&mat;AlkylatedNaphthalene">
        <rdfs:subClassOf rdf:resource="&mat;FluidLubricant"/>
        <owl:disjointWith rdf:resource="&mat;AluminumGellant"/>
        <owl:disjointWith rdf:resource="&mat;LithiumGellant"/>
        <owl:disjointWith rdf:resource="&mat;MultiplyAlkylatedCyclopentane"/>
        <owl:disjointWith rdf:resource="&mat;OrganicSoapGellant"/>
        <owl:disjointWith rdf:resource="&mat;PTFEGellant"/>
        <owl:disjointWith rdf:resource="&mat;Perfluoropolyether"/>
        <owl:disjointWith rdf:resource="&mat;Polyalphaolefin"/>
        <owl:disjointWith rdf:resource="&mat;Polyglycol"/>
        <owl:disjointWith rdf:resource="&mat;PolyphenyletherBaseLubricant"/>
        <owl:disjointWith rdf:resource="&mat;Quenchant"/>
        <owl:disjointWith rdf:resource="&mat;SiliconeBaseLubricant"/>
        <owl:disjointWith rdf:resource="&mat;SiliconeGellant"/>
        <owl:disjointWith rdf:resource="&mat;SyntheticEtherBase"/>
        <owl:disjointWith rdf:resource="&mat;UreaGellant"/>
        <owl:disjointWith rdf:resource="&mat;WhiteMineralOil"/>
        <owl:disjointWith rdf:resource="&mat;ZincOxideLubricant"/>
        <or:referenceURL rdf:datatype="&xsd;anyURI">http://www.matweb.com/index.aspx</or:referenceURL>
        <or:termString xml:lang="en">AN</or:termString>
        <or:termString xml:lang="en">alkylated naphthalene</or:termString>
    </owl:Class>
    


    <!-- http://www.nist.gov/itl/ssd/Materials#Alloy -->

    <owl:Class rdf:about="&mat;Alloy">
        <rdfs:subClassOf rdf:resource="&bc;Metal"/>
        <rdfs:subClassOf rdf:resource="&mat;PhysicalMixture"/>
        <rdfs:subClassOf rdf:resource="&mat;SolidSubstance"/>
        <owl:disjointWith rdf:resource="&mat;ChemicalSuspension"/>
        <owl:disjointWith rdf:resource="&mat;CompositeMaterial"/>
        <owl:disjointWith rdf:resource="&mat;Foam"/>
        <owl:disjointWith rdf:resource="&mat;GelSubstance"/>
        <owl:disjointWith rdf:resource="&mat;LiquidFoam"/>
        <owl:disjointWith rdf:resource="&mat;PasteSubstance"/>
    </owl:Class>
    


    <!-- http://www.nist.gov/itl/ssd/Materials#AlloyCastIron -->

    <owl:Class rdf:about="&mat;AlloyCastIron">
        <rdfs:subClassOf rdf:resource="&mat;CastIron"/>
        <owl:disjointWith rdf:resource="&mat;DuctileIron"/>
        <owl:disjointWith rdf:resource="&mat;GrayCastIron"/>
        <owl:disjointWith rdf:resource="&mat;MalleableIron"/>
        <owl:disjointWith rdf:resource="&mat;WhiteCastIron"/>
        <or:referenceURL rdf:datatype="&xsd;anyURI">http://www.matweb.com/index.aspx</or:referenceURL>
        <or:termString xml:lang="en">alloy cast iron</or:termString>
    </owl:Class>
    


    <!-- http://www.nist.gov/itl/ssd/Materials#AlloySteel -->

    <owl:Class rdf:about="&mat;AlloySteel">
        <rdfs:subClassOf rdf:resource="&mat;Steel"/>
        <owl:disjointWith rdf:resource="&mat;CarbonSteel"/>
        <owl:disjointWith rdf:resource="&mat;ChromMolySteel"/>
        <or:referenceURL rdf:datatype="&xsd;anyURI">http://www.matweb.com/index.aspx</or:referenceURL>
        <rdfs:comment xml:lang="en">Steel with no carbide forming elements.</rdfs:comment>
        <or:termString xml:lang="en">alloy steel</or:termString>
    </owl:Class>
    


    <!-- http://www.nist.gov/itl/ssd/Materials#AlloyType -->

    <owl:Class rdf:about="&mat;AlloyType">
        <rdfs:subClassOf rdf:resource="&or;MaterialType"/>
    </owl:Class>
    


    <!-- http://www.nist.gov/itl/ssd/Materials#AlloyTypeByFormingProcess -->

    <owl:Class rdf:about="&mat;AlloyTypeByFormingProcess">
        <rdfs:subClassOf rdf:resource="&mat;AlloyType"/>
    </owl:Class>
    


    <!-- http://www.nist.gov/itl/ssd/Materials#AlloyTypeByMainConstituent -->

    <owl:Class rdf:about="&mat;AlloyTypeByMainConstituent">
        <rdfs:subClassOf rdf:resource="&mat;AlloyType"/>
    </owl:Class>
    


    <!-- http://www.nist.gov/itl/ssd/Materials#AluminumAlloy -->

    <owl:Class rdf:about="&mat;AluminumAlloy">
        <rdfs:subClassOf rdf:resource="&mat;NonFerrousAlloy"/>
        <rdfs:subClassOf>
            <owl:Restriction>
                <owl:onProperty rdf:resource="&mat;physicalDecompositions"/>
                <owl:someValuesFrom rdf:resource="&bc;Aluminum"/>
            </owl:Restriction>
        </rdfs:subClassOf>
        <or:referenceURL rdf:datatype="&xsd;anyURI">http://www.matweb.com/index.aspx</or:referenceURL>
        <rdfs:comment xml:lang="en">An alloy that contains Aluminum but not Iron.</rdfs:comment>
    </owl:Class>
    


    <!-- http://www.nist.gov/itl/ssd/Materials#AluminumGellant -->

    <owl:Class rdf:about="&mat;AluminumGellant">
        <rdfs:subClassOf rdf:resource="&mat;FluidLubricant"/>
        <owl:disjointWith rdf:resource="&mat;LithiumGellant"/>
        <owl:disjointWith rdf:resource="&mat;MultiplyAlkylatedCyclopentane"/>
        <owl:disjointWith rdf:resource="&mat;OrganicSoapGellant"/>
        <owl:disjointWith rdf:resource="&mat;PTFEGellant"/>
        <owl:disjointWith rdf:resource="&mat;Perfluoropolyether"/>
        <owl:disjointWith rdf:resource="&mat;Polyalphaolefin"/>
        <owl:disjointWith rdf:resource="&mat;Polyglycol"/>
        <owl:disjointWith rdf:resource="&mat;PolyphenyletherBaseLubricant"/>
        <owl:disjointWith rdf:resource="&mat;Quenchant"/>
        <owl:disjointWith rdf:resource="&mat;SiliconeBaseLubricant"/>
        <owl:disjointWith rdf:resource="&mat;SiliconeGellant"/>
        <owl:disjointWith rdf:resource="&mat;SyntheticEtherBase"/>
        <owl:disjointWith rdf:resource="&mat;UreaGellant"/>
        <owl:disjointWith rdf:resource="&mat;WhiteMineralOil"/>
        <owl:disjointWith rdf:resource="&mat;ZincOxideLubricant"/>
        <or:referenceURL rdf:datatype="&xsd;anyURI">http://www.matweb.com/index.aspx</or:referenceURL>
        <or:termString xml:lang="en">aluminum gellant</or:termString>
    </owl:Class>
    


    <!-- http://www.nist.gov/itl/ssd/Materials#AluminumOxide -->

    <owl:Class rdf:about="&mat;AluminumOxide">
        <rdfs:subClassOf rdf:resource="&bc;Oxide"/>
        <owl:disjointWith rdf:resource="&mat;MagnesiumOxide"/>
        <owl:disjointWith rdf:resource="&mat;SiliconOxide"/>
        <owl:disjointWith rdf:resource="&mat;TitaniumOxide"/>
        <owl:disjointWith rdf:resource="&mat;ZirconiumOxide"/>
        <or:referenceURL rdf:datatype="&xsd;anyURI">http://www.matweb.com/index.aspx</or:referenceURL>
        <or:termString xml:lang="en">aluminum oxide</or:termString>
    </owl:Class>
    


    <!-- http://www.nist.gov/itl/ssd/Materials#AmbipolarDIffusion -->

    <owl:Class rdf:about="&mat;AmbipolarDIffusion">
        <rdfs:subClassOf rdf:resource="&mat;SolidDiffusion"/>
        <rdfs:comment xml:lang="en">Ambipolar diffusion is diffusion in systems with two or more diffusion species with opposite electrical charge.</rdfs:comment>
        <rdfs:seeAlso xml:lang="en">Definitions of terms for diffusion in the solid state (IUPAC Recommendations 1999), Pure Appl. Chem. 71, 1307-1325.</rdfs:seeAlso>
    </owl:Class>
    


    <!-- http://www.nist.gov/itl/ssd/Materials#AmorphousMetal -->

    <owl:Class rdf:about="&mat;AmorphousMetal">
        <rdfs:subClassOf rdf:resource="&mat;EngineeredAlloy"/>
        <rdfs:subClassOf rdf:resource="&mat;ManufacturedGlass"/>
        <owl:disjointWith rdf:resource="&mat;OpticalGlass"/>
        <rdfs:comment xml:lang="en">An amorphous metal (also known metallic glass or glassy metal) is an alloy with a disordered atomic-scale structure.</rdfs:comment>
    </owl:Class>
    


    <!-- http://www.nist.gov/itl/ssd/Materials#AmorphousMicrostructure -->

    <owl:Class rdf:about="&mat;AmorphousMicrostructure">
        <rdfs:subClassOf rdf:resource="&mat;Microstructure"/>
        <owl:disjointWith rdf:resource="&mat;CeramicMicrostructure"/>
        <owl:disjointWith rdf:resource="&mat;CompositeMicrostructure"/>
        <owl:disjointWith rdf:resource="&mat;CrystalStructure"/>
    </owl:Class>
    


    <!-- http://www.nist.gov/itl/ssd/Materials#AmorphousSubstance -->

    <owl:Class rdf:about="&mat;AmorphousSubstance">
        <rdfs:subClassOf rdf:resource="&mat;SolidSubstance"/>
        <owl:disjointWith rdf:resource="&mat;CompositeMaterial"/>
        <owl:disjointWith rdf:resource="&mat;CrystallineSubstance"/>
        <owl:disjointWith rdf:resource="&mat;GaseousSubstance"/>
        <rdfs:comment xml:lang="en">Material in a solid amorphous (non-crystalline) phase.</rdfs:comment>
    </owl:Class>
    


    <!-- http://www.nist.gov/itl/ssd/Materials#AqueousSolution -->

    <owl:Class rdf:about="&mat;AqueousSolution">
        <owl:equivalentClass>
            <owl:Class>
                <owl:intersectionOf rdf:parseType="Collection">
                    <rdf:Description rdf:about="&mat;LiquidSolution"/>
                    <owl:Restriction>
                        <owl:onProperty rdf:resource="&mat;solvent"/>
                        <owl:allValuesFrom rdf:resource="&bc;Water"/>
                    </owl:Restriction>
                </owl:intersectionOf>
            </owl:Class>
        </owl:equivalentClass>
        <rdfs:subClassOf rdf:resource="&mat;LiquidSolution"/>
        <owl:disjointWith rdf:resource="&mat;IonicLiquidSolution"/>
        <owl:disjointWith rdf:resource="&mat;NonIonicOrAqueousLiquidSolution"/>
        <rdfs:comment xml:lang="en">A solution in which liquid water is the solvent.</rdfs:comment>
    </owl:Class>
    


    <!-- http://www.nist.gov/itl/ssd/Materials#AreaPerTime -->

    <owl:Class rdf:about="&mat;AreaPerTime">
        <owl:equivalentClass>
            <owl:Class>
                <owl:intersectionOf rdf:parseType="Collection">
                    <rdf:Description rdf:about="&or;MeasurableQuantity"/>
                    <owl:Restriction>
                        <owl:onProperty rdf:resource="&or;unitsFor"/>
                        <owl:someValuesFrom rdf:resource="&mat;UnitOfAreaPerTime"/>
                    </owl:Restriction>
                </owl:intersectionOf>
            </owl:Class>
        </owl:equivalentClass>
        <rdfs:subClassOf rdf:resource="&or;MeasurableQuantity"/>
        <rdfs:subClassOf>
            <owl:Restriction>
                <owl:onProperty rdf:resource="&or;unitsFor"/>
                <owl:allValuesFrom rdf:resource="&mat;UnitOfAreaPerTime"/>
            </owl:Restriction>
        </rdfs:subClassOf>
        <owl:disjointWith rdf:resource="&mat;EnergyPerMass"/>
        <owl:disjointWith rdf:resource="&or;Area"/>
        <owl:disjointWith rdf:resource="&or;ComputerStorageCapacity"/>
        <owl:disjointWith rdf:resource="&or;Distance"/>
        <owl:disjointWith rdf:resource="&or;Duration"/>
        <owl:disjointWith rdf:resource="&or;Energy"/>
        <owl:disjointWith rdf:resource="&or;Force"/>
        <owl:disjointWith rdf:resource="&or;Mass"/>
        <owl:disjointWith rdf:resource="&or;Pressure"/>
        <owl:disjointWith rdf:resource="&or;Temperature"/>
        <owl:disjointWith rdf:resource="&or;Volume"/>
    </owl:Class>
    


    <!-- http://www.nist.gov/itl/ssd/Materials#ArsenateMineral -->

    <owl:Class rdf:about="&mat;ArsenateMineral">
        <rdfs:subClassOf rdf:resource="&mat;Mineral"/>
        <rdfs:comment xml:lang="en">The class of minerals with the arsenate (AsO4) ion.</rdfs:comment>
    </owl:Class>
    


    <!-- http://www.nist.gov/itl/ssd/Materials#AscendingDiffusion -->

    <owl:Class rdf:about="&mat;AscendingDiffusion">
        <rdfs:subClassOf rdf:resource="&mat;SolidDiffusion"/>
        <owl:disjointWith rdf:resource="&mat;SelfDiffusion"/>
        <rdfs:comment xml:lang="en">Ascending Diffusion is a type of diffusion that can take place in alloys of metals under the influence of stress gradients.  When the constituents are of different sizes, the larger elements tend to move in the directions of the dilated regions.  Thus ascending diffusion disturbs the uniform distribution of the constiuentes and sets up a concentration gradient which opposes the stress gradient.</rdfs:comment>
        <rdfs:seeAlso xml:lang="en">Definitions of terms for diffusion in the solid state (IUPAC Recommendations 1999), Pure Appl. Chem. 71, 1307-1325.</rdfs:seeAlso>
    </owl:Class>
    


    <!-- http://www.nist.gov/itl/ssd/Materials#Auricupride -->

    <owl:Class rdf:about="&mat;Auricupride">
        <rdfs:subClassOf rdf:resource="&mat;BinaryAlloy"/>
        <rdfs:subClassOf rdf:resource="&mat;CopperAlloy"/>
        <rdfs:subClassOf rdf:resource="&mat;NativeMetal"/>
        <rdfs:subClassOf>
            <owl:Restriction>
                <owl:onProperty rdf:resource="&mat;physicalDecompositions"/>
                <owl:someValuesFrom rdf:resource="&bc;Gold"/>
            </owl:Restriction>
        </rdfs:subClassOf>
        <owl:disjointWith rdf:resource="&mat;EngineeredAlloy"/>
        <rdfs:comment xml:lang="en">Auricupride is a natural alloy that combines copper and gold. Its chemical formula is Cu3Au. The alloy crystallizes in the Cubic crystal system and occurs as malleable grains or platey masses. It is an opaque yellow with a reddish tint. It has a hardness of 3.5 and a specific gravity of 11.5.</rdfs:comment>
    </owl:Class>
    


    <!-- http://www.nist.gov/itl/ssd/Materials#AusteniticSteel -->

    <owl:Class rdf:about="&mat;AusteniticSteel">
        <rdfs:subClassOf rdf:resource="&mat;Steel"/>
        <owl:disjointWith rdf:resource="&mat;FerriticStainlessSteel"/>
        <or:referenceURL rdf:datatype="&xsd;anyURI">http://www.matweb.com/index.aspx</or:referenceURL>
        <rdfs:comment xml:lang="en">Austenitic Steel is steel that has enough nickel and chromium or manganese to retain austenite at atmospheric temperatures</rdfs:comment>
        <or:termString xml:lang="en">austenitic steel </or:termString>
    </owl:Class>
    


    <!-- http://www.nist.gov/itl/ssd/Materials#Bakelite -->

    <owl:Class rdf:about="&mat;Bakelite">
        <rdfs:subClassOf rdf:resource="&mat;EngineeredMaterial"/>
        <rdfs:subClassOf rdf:resource="&mat;Thermoset"/>
        <owl:disjointWith rdf:resource="&mat;Polyester"/>
        <rdfs:comment xml:lang="en">Bakelite (polyoxybenzylmethylenglycolanhydride) is a thermosetting resin-like substance produced by the condensation reaction of carbolic acid and formaldehyde.</rdfs:comment>
    </owl:Class>
    


    <!-- http://www.nist.gov/itl/ssd/Materials#BerylliumAlloy -->

    <owl:Class rdf:about="&mat;BerylliumAlloy">
        <rdfs:subClassOf rdf:resource="&mat;NonFerrousAlloy"/>
        <rdfs:subClassOf>
            <owl:Restriction>
                <owl:onProperty rdf:resource="&mat;physicalDecompositions"/>
                <owl:someValuesFrom rdf:resource="&bc;Beryllium"/>
            </owl:Restriction>
        </rdfs:subClassOf>
        <or:referenceURL rdf:datatype="&xsd;anyURI">http://www.matweb.com/index.aspx</or:referenceURL>
    </owl:Class>
    


    <!-- http://www.nist.gov/itl/ssd/Materials#BinaryAlloy -->

    <owl:Class rdf:about="&mat;BinaryAlloy">
        <rdfs:subClassOf rdf:resource="&mat;Alloy"/>
        <owl:disjointWith rdf:resource="&mat;Superalloy"/>
        <rdfs:comment xml:lang="en">A Binary Alloy is an Alloy composed of exactly two different metals.</rdfs:comment>
    </owl:Class>
    


    <!-- http://www.nist.gov/itl/ssd/Materials#BinarySolutionPhase -->

    <owl:Class rdf:about="&mat;BinarySolutionPhase">
        <rdfs:subClassOf rdf:resource="&mat;MaterialPhaseComposition"/>
    </owl:Class>
    


    <!-- http://www.nist.gov/itl/ssd/Materials#BismuthAlloy -->

    <owl:Class rdf:about="&mat;BismuthAlloy">
        <rdfs:subClassOf rdf:resource="&mat;NonFerrousAlloy"/>
        <rdfs:subClassOf>
            <owl:Restriction>
                <owl:onProperty rdf:resource="&mat;physicalDecompositions"/>
                <owl:someValuesFrom rdf:resource="&bc;Bismuth"/>
            </owl:Restriction>
        </rdfs:subClassOf>
        <or:referenceURL rdf:datatype="&xsd;anyURI">http://www.matweb.com/index.aspx</or:referenceURL>
    </owl:Class>
    


    <!-- http://www.nist.gov/itl/ssd/Materials#BodyCenteredCubicCrystalStructure -->

    <owl:Class rdf:about="&mat;BodyCenteredCubicCrystalStructure">
        <rdfs:subClassOf rdf:resource="&mat;CubicCrystalStructure"/>
        <owl:disjointWith rdf:resource="&mat;FaceCenteredCubicCrystalStructure"/>
    </owl:Class>
    


    <!-- http://www.nist.gov/itl/ssd/Materials#Boiling -->

    <owl:Class rdf:about="&mat;Boiling">
        <rdfs:subClassOf rdf:resource="&mat;Evaporating"/>
        <rdfs:comment xml:lang="en">Boiling is the Phase Change event at a liquid&#39;s &#39;boiling point&#39; at which the partial pressure of the gas reaches the environmental pressure.  During boiling, increasing amounts of the liquid evaporate as heat is added to the system although the temperature of the system remains basically constant.</rdfs:comment>
    </owl:Class>
    


    <!-- http://www.nist.gov/itl/ssd/Materials#Borate -->

    <owl:Class rdf:about="&mat;Borate">
        <rdfs:subClassOf rdf:resource="&mat;Mineral"/>
    </owl:Class>
    


    <!-- http://www.nist.gov/itl/ssd/Materials#Boride -->

    <owl:Class rdf:about="&mat;Boride">
        <rdfs:subClassOf rdf:resource="&mat;PureSubstance"/>
        <owl:disjointWith rdf:resource="&mat;Carbide"/>
        <owl:disjointWith rdf:resource="&mat;Halide"/>
        <rdfs:comment xml:lang="en">A  boride is a chemical compound between boron and a less electronegative element.</rdfs:comment>
        <or:termString xml:lang="en">boride</or:termString>
    </owl:Class>
    


    <!-- http://www.nist.gov/itl/ssd/Materials#BorideBasedCeramic -->

    <owl:Class rdf:about="&mat;BorideBasedCeramic">
        <rdfs:subClassOf rdf:resource="&mat;Ceramic"/>
        <owl:disjointWith rdf:resource="&mat;ChalcogenBasedCeramic"/>
        <owl:disjointWith rdf:resource="&mat;OxideBasedCeramic"/>
        <owl:disjointWith rdf:resource="&mat;PnictideCeramic"/>
        <or:referenceURL rdf:datatype="&xsd;anyURI">http://www.matweb.com/index.aspx</or:referenceURL>
    </owl:Class>
    


    <!-- http://www.nist.gov/itl/ssd/Materials#Brass -->

    <owl:Class rdf:about="&mat;Brass">
        <rdfs:subClassOf rdf:resource="&mat;CopperAlloy"/>
        <rdfs:subClassOf rdf:resource="&mat;EngineeredAlloy"/>
        <rdfs:subClassOf>
            <owl:Restriction>
                <owl:onProperty rdf:resource="&mat;physicalDecompositions"/>
                <owl:someValuesFrom rdf:resource="&bc;Zinc"/>
            </owl:Restriction>
        </rdfs:subClassOf>
        <rdfs:comment xml:lang="en">Brass is an alloy of copper and zinc; the proportions of zinc and copper can be varied to create a range of brasses with varying properties.  Other metals (lead, tin, aluminum, nickel, traces of iron) may be added in specific proportions for specific brass alloys.</rdfs:comment>
    </owl:Class>
    


    <!-- http://www.nist.gov/itl/ssd/Materials#Bronze -->

    <owl:Class rdf:about="&mat;Bronze">
        <rdfs:subClassOf rdf:resource="&mat;CopperAlloy"/>
        <rdfs:subClassOf rdf:resource="&mat;EngineeredAlloy"/>
        <rdfs:comment xml:lang="en">Bronze is a metal alloy consisting primarily of copper, usually with tin as the main additive. There are many different bronze alloys but modern bronze is typically 88% copper and 12% tin.  Bronzes with the secondary additive other than tin or zinc include Aluminum Bronze and Silicon Bronze.  Phosphor Bronze is a Brass (main additive is zinc) with a significant amount of Phosphor (up to 1%) as an additional additive.</rdfs:comment>
    </owl:Class>
    


    <!-- http://www.nist.gov/itl/ssd/Materials#Buckling -->

    <owl:Class rdf:about="&mat;Buckling">
        <rdfs:subClassOf rdf:resource="&mat;Deformation"/>
        <owl:disjointWith rdf:resource="&mat;Compaction"/>
        <rdfs:comment xml:lang="en">Buckling is a Deformation Process of an object bending under compressive stress.</rdfs:comment>
    </owl:Class>
    


    <!-- http://www.nist.gov/itl/ssd/Materials#Buckyball -->

    <owl:Class rdf:about="&mat;Buckyball">
        <rdfs:subClassOf rdf:resource="&mat;Fullerine"/>
        <owl:disjointWith rdf:resource="&mat;CarbonNanotube"/>
        <rdfs:comment xml:lang="en">A Buckyball is a Fullerene in the shape of a ball with at least 60 carbon atoms.  Buckyballs have been discovered in soot with 60, 70, 76, 80, and 84 carbon atoms.</rdfs:comment>
    </owl:Class>
    


    <!-- http://www.nist.gov/itl/ssd/Materials#Carbide -->

    <owl:Class rdf:about="&mat;Carbide">
        <rdfs:subClassOf rdf:resource="&mat;PureSubstance"/>
        <owl:disjointWith rdf:resource="&mat;Halide"/>
        <rdfs:comment xml:lang="en">A carbide is a chemical compound composed of carbon and a less electronegative element.</rdfs:comment>
        <or:termString xml:lang="en">carbide</or:termString>
    </owl:Class>
    


    <!-- http://www.nist.gov/itl/ssd/Materials#CarbideBasedCeramic -->

    <owl:Class rdf:about="&mat;CarbideBasedCeramic">
        <rdfs:subClassOf rdf:resource="&mat;Ceramic"/>
        <or:referenceURL rdf:datatype="&xsd;anyURI">http://www.matweb.com/index.aspx</or:referenceURL>
    </owl:Class>
    


    <!-- http://www.nist.gov/itl/ssd/Materials#CarbideBasedCermet -->

    <owl:Class rdf:about="&mat;CarbideBasedCermet">
        <rdfs:subClassOf rdf:resource="&mat;CarbideBasedCeramic"/>
        <rdfs:subClassOf rdf:resource="&mat;Cermet"/>
    </owl:Class>
    


    <!-- http://www.nist.gov/itl/ssd/Materials#CarbonBlack -->

    <owl:Class rdf:about="&mat;CarbonBlack">
        <rdfs:subClassOf rdf:resource="&bc;Carbon"/>
        <rdfs:subClassOf rdf:resource="&mat;PolycrystallineMaterial"/>
        <owl:disjointWith rdf:resource="&mat;CarbonFiber"/>
        <owl:disjointWith rdf:resource="&mat;Diamond"/>
        <owl:disjointWith rdf:resource="&mat;Fullerine"/>
        <owl:disjointWith rdf:resource="&mat;Graphite"/>
        <or:referenceURL rdf:datatype="&xsd;anyURI">http://www.matweb.com/index.aspx</or:referenceURL>
        <rdfs:comment xml:lang="en">Carbon black (also known as acetylene black, channel black, furnace black, lamp black or thermal black) is a material produced by the incomplete combustion of heavy petroleum products such as FCC tar, coal tar, ethylene cracking tar, and a small amount from vegetable oil. Carbon black is a form of amorphous carbon that has a high surface-area-to-volume ratio, although its surface-area-to-volume ratio is low compared to that of activated carbon. It is dissimilar to soot in its much higher surface-area-to-volume ratio and significantly lower (negligible and non-bioavailable) PAH (polycyclic aromatic hydrocarbon) content.</rdfs:comment>
        <or:termString xml:lang="en">acetylene black</or:termString>
        <or:termString xml:lang="en">carbon fiber</or:termString>
        <or:termString xml:lang="en">channel black</or:termString>
        <or:termString xml:lang="en">furnace black</or:termString>
        <or:termString xml:lang="en">lamp black</or:termString>
        <or:termString xml:lang="en">thermal black</or:termString>
    </owl:Class>
    


    <!-- http://www.nist.gov/itl/ssd/Materials#CarbonFiber -->

    <owl:Class rdf:about="&mat;CarbonFiber">
        <rdfs:subClassOf rdf:resource="&bc;Carbon"/>
        <rdfs:subClassOf rdf:resource="&mat;PolycrystallineMaterial"/>
        <owl:disjointWith rdf:resource="&mat;Diamond"/>
        <owl:disjointWith rdf:resource="&mat;Graphite"/>
        <or:referenceURL rdf:datatype="&xsd;anyURI">http://www.matweb.com/index.aspx</or:referenceURL>
        <or:termString xml:lang="en">CF</or:termString>
        <rdfs:comment xml:lang="en">Carbon fiber, alternatively graphite fiber, carbon graphite or CF, is a material consisting of fibers about 5–10 μm in diameter and composed mostly of carbon atoms. The carbon atoms are bonded together in crystals that are more or less aligned parallel to the long axis of the fiber.</rdfs:comment>
        <or:termString xml:lang="en">carbon fiber</or:termString>
        <or:termString xml:lang="en">carbon graphite</or:termString>
        <or:termString xml:lang="en">graphite fiber</or:termString>
    </owl:Class>
    


    <!-- http://www.nist.gov/itl/ssd/Materials#CarbonNanotube -->

    <owl:Class rdf:about="&mat;CarbonNanotube">
        <rdfs:subClassOf rdf:resource="&mat;Fullerine"/>
        <rdfs:comment xml:lang="en">Carbon Nanotubes are tubular Fullerenes</rdfs:comment>
    </owl:Class>
    


    <!-- http://www.nist.gov/itl/ssd/Materials#CarbonSteel -->

    <owl:Class rdf:about="&mat;CarbonSteel">
        <rdfs:subClassOf rdf:resource="&mat;Steel"/>
        <owl:disjointWith rdf:resource="&mat;ChromMolySteel"/>
        <owl:disjointWith rdf:resource="&mat;HighSpeedSteel"/>
        <owl:disjointWith rdf:resource="&mat;StainlessSteel"/>
        <or:referenceURL rdf:datatype="&xsd;anyURI">http://www.matweb.com/index.aspx</or:referenceURL>
        <rdfs:comment xml:lang="en">Carbon steel is steel where the main interstitial alloying constituent is carbon. 

 The American Iron and Steel Institute (AISI) defines carbon steel as the following: ``Steel is considered to be carbon steel when no minimum content is specified or required for chromium, cobalt, molybdenum, nickel, niobium, titanium, tungsten, vanadium or zirconium, or any other element to be added to obtain a desired alloying effect; when the specified minimum for copper does not exceed 1.04 percent; or when the maximum content specified for any of the following elements does not exceed the percentages noted: manganese 1.65, silicon 0.60, copper 0.60.&#39;&#39;</rdfs:comment>
        <or:termString xml:lang="en">carbon steel</or:termString>
    </owl:Class>
    


    <!-- http://www.nist.gov/itl/ssd/Materials#Carbonate -->

    <owl:Class rdf:about="&mat;Carbonate">
        <rdfs:subClassOf rdf:resource="&mat;Mineral"/>
    </owl:Class>
    


    <!-- http://www.nist.gov/itl/ssd/Materials#CarboxymethylCellulose -->

    <owl:Class rdf:about="&mat;CarboxymethylCellulose">
        <rdfs:subClassOf rdf:resource="&mat;CelluloseEther"/>
        <owl:disjointWith rdf:resource="&mat;HydroxyalkylCelluloseEther"/>
        <rdfs:comment xml:lang="en">Carboxymethyl cellulose (CMC) (or cellulose gum) is a cellulose derivative with carboxymethyl groups (-CH2-COOH) bound to some of the hydroxyl groups of the glucopyranose monomers that make up the cellulose backbone.</rdfs:comment>
    </owl:Class>
    


    <!-- http://www.nist.gov/itl/ssd/Materials#CastAlloy -->

    <owl:Class rdf:about="&mat;CastAlloy">
        <rdfs:subClassOf rdf:resource="&mat;EngineeredAlloy"/>
        <owl:disjointWith rdf:resource="&mat;CompactedPowderAlloy"/>
        <owl:disjointWith rdf:resource="&mat;WroughtAlloy"/>
        <rdfs:comment xml:lang="en">A Cast Alloy is one which is formed by pouring molten metal into a mold and letting it harden.</rdfs:comment>
    </owl:Class>
    


    <!-- http://www.nist.gov/itl/ssd/Materials#CastIron -->

    <owl:Class rdf:about="&mat;CastIron">
        <rdfs:subClassOf rdf:resource="&mat;CastAlloy"/>
        <rdfs:subClassOf rdf:resource="&mat;FerrousAlloy"/>
        <or:referenceURL rdf:datatype="&xsd;anyURI">http://www.matweb.com/index.aspx</or:referenceURL>
        <or:termString xml:lang="en">cast iron</or:termString>
    </owl:Class>
    


    <!-- http://www.nist.gov/itl/ssd/Materials#CastStainlessSteel -->

    <owl:Class rdf:about="&mat;CastStainlessSteel">
        <rdfs:subClassOf rdf:resource="&mat;StainlessSteel"/>
        <or:referenceURL rdf:datatype="&xsd;anyURI">http://www.matweb.com/index.aspx</or:referenceURL>
        <or:termString xml:lang="en">cast stainless steel</or:termString>
    </owl:Class>
    


    <!-- http://www.nist.gov/itl/ssd/Materials#CellularPrecipitationFromSolution -->

    <owl:Class rdf:about="&mat;CellularPrecipitationFromSolution">
        <rdfs:subClassOf rdf:resource="&mat;PrecipitationFromSolution"/>
    </owl:Class>
    


    <!-- http://www.nist.gov/itl/ssd/Materials#Cellulose -->

    <owl:Class rdf:about="&mat;Cellulose">
        <rdfs:subClassOf rdf:resource="&mat;PolymerSubstance"/>
        <owl:disjointWith rdf:resource="&mat;Elastomer"/>
        <owl:disjointWith rdf:resource="&mat;EngineeredMaterial"/>
        <owl:disjointWith rdf:resource="&mat;Polyester"/>
        <rdfs:comment xml:lang="en">Cellulose is an organic compound with the formula (C6H10O5)n, a polysaccharide consisting of a linear chain of several hundred to over ten thousand β(1→4) linked D-glucose units.</rdfs:comment>
    </owl:Class>
    


    <!-- http://www.nist.gov/itl/ssd/Materials#CelluloseAcetate -->

    <owl:Class rdf:about="&mat;CelluloseAcetate">
        <rdfs:subClassOf rdf:resource="&mat;CelluloseEster"/>
        <owl:disjointWith rdf:resource="&mat;CelluloseDiacetate"/>
        <owl:disjointWith rdf:resource="&mat;CelluloseSulfate"/>
        <owl:disjointWith rdf:resource="&mat;CelluloseTriacetate"/>
        <owl:disjointWith rdf:resource="&mat;Nitrocellulose"/>
        <rdfs:comment xml:lang="en">Cellulose acetate is the acetate ester of cellulose.</rdfs:comment>
    </owl:Class>
    


    <!-- http://www.nist.gov/itl/ssd/Materials#CelluloseDiacetate -->

    <owl:Class rdf:about="&mat;CelluloseDiacetate">
        <rdfs:subClassOf rdf:resource="&mat;CelluloseEster"/>
        <owl:disjointWith rdf:resource="&mat;CelluloseSulfate"/>
        <owl:disjointWith rdf:resource="&mat;CelluloseTriacetate"/>
        <owl:disjointWith rdf:resource="&mat;Nitrocellulose"/>
        <rdfs:comment xml:lang="en">Cellulose diacetate (or simply `diacetate&#39;) is a synthetic polymer made by treating cellulose with acetic acid. It consists of two acetate radicals on each monomer of the cellulose molecule.</rdfs:comment>
    </owl:Class>
    


    <!-- http://www.nist.gov/itl/ssd/Materials#CelluloseEster -->

    <owl:Class rdf:about="&mat;CelluloseEster">
        <rdfs:subClassOf rdf:resource="&mat;CellulosticPlastic"/>
        <owl:disjointWith rdf:resource="&mat;CelluloseEther"/>
        <rdfs:comment xml:lang="en">A Cellulose Ester is a Cellulostic Plastic with the hydroxyl groups of Cellulose replaced by a radical not connected via an oxygen (i.e., an ether).</rdfs:comment>
    </owl:Class>
    


    <!-- http://www.nist.gov/itl/ssd/Materials#CelluloseEther -->

    <owl:Class rdf:about="&mat;CelluloseEther">
        <rdfs:subClassOf rdf:resource="&mat;CellulosticPlastic"/>
        <rdfs:comment xml:lang="en">A Cellulose Ester is a Cellulostic Plastic with the hydroxyl groups of Cellulose replaced by a radical connected via an oxygen (i.e., an ether).</rdfs:comment>
    </owl:Class>
    


    <!-- http://www.nist.gov/itl/ssd/Materials#CelluloseSulfate -->

    <owl:Class rdf:about="&mat;CelluloseSulfate">
        <rdfs:subClassOf rdf:resource="&mat;CelluloseEster"/>
        <owl:disjointWith rdf:resource="&mat;CelluloseTriacetate"/>
        <owl:disjointWith rdf:resource="&mat;Nitrocellulose"/>
    </owl:Class>
    


    <!-- http://www.nist.gov/itl/ssd/Materials#CelluloseTriacetate -->

    <owl:Class rdf:about="&mat;CelluloseTriacetate">
        <rdfs:subClassOf rdf:resource="&mat;CelluloseEster"/>
        <owl:disjointWith rdf:resource="&mat;Nitrocellulose"/>
        <rdfs:comment xml:lang="en">Cellulose triacetate (or triacetate, CTA, or TAC) is manufactured from cellulose and a source of acetate esters, typically acetic anhydride.  It is similar chemically to cellulose acetate, with the distinguishing characteristics being that in triacetate (Federal Trade Commission definition) at least ``92 percent of the hydroxyl groups are acetylated.&#39;&#39; </rdfs:comment>
    </owl:Class>
    


    <!-- http://www.nist.gov/itl/ssd/Materials#CellulosticPlastic -->

    <owl:Class rdf:about="&mat;CellulosticPlastic">
        <rdfs:subClassOf rdf:resource="&mat;Thermoplastic"/>
        <owl:disjointWith rdf:resource="&mat;Polyester"/>
        <owl:disjointWith rdf:resource="&mat;Polyolefin"/>
        <owl:disjointWith rdf:resource="&mat;VinylPolymer"/>
        <or:referenceURL rdf:datatype="&xsd;anyURI">http://www.matweb.com/index.aspx</or:referenceURL>
        <rdfs:comment xml:lang="en">A celluloistic plastic is a plastic derived from cellulose.</rdfs:comment>
    </owl:Class>
    


    <!-- http://www.nist.gov/itl/ssd/Materials#Ceramic -->

    <owl:Class rdf:about="&mat;Ceramic">
        <rdfs:subClassOf rdf:resource="&mat;SolidSubstance"/>
        <owl:disjointWith rdf:resource="&mat;PolymerSubstance"/>
        <owl:disjointWith rdf:resource="&mat;SolidFoam"/>
        <owl:disjointWith rdf:resource="&mat;SolidSol"/>
    </owl:Class>
    


    <!-- http://www.nist.gov/itl/ssd/Materials#CeramicHydride -->

    <owl:Class rdf:about="&mat;CeramicHydride">
        <rdfs:subClassOf rdf:resource="&mat;Ceramic"/>
        <or:referenceURL rdf:datatype="&xsd;anyURI">http://www.matweb.com/index.aspx</or:referenceURL>
        <or:termString xml:lang="en">ceramic hydride</or:termString>
        <or:termString xml:lang="en">hydride</or:termString>
    </owl:Class>
    


    <!-- http://www.nist.gov/itl/ssd/Materials#CeramicMatrixComposite -->

    <owl:Class rdf:about="&mat;CeramicMatrixComposite">
        <rdfs:subClassOf rdf:resource="&mat;Ceramic"/>
        <rdfs:subClassOf rdf:resource="&mat;CompositeMaterial"/>
        <rdfs:subClassOf rdf:resource="&mat;EngineeredMaterial"/>
        <owl:disjointWith rdf:resource="&mat;CeramicResin"/>
        <owl:disjointWith rdf:resource="&mat;Cermet"/>
        <owl:disjointWith rdf:resource="&mat;GlassCeramic"/>
        <or:referenceURL rdf:datatype="&xsd;anyURI">http://www.matweb.com/index.aspx</or:referenceURL>
        <or:termString xml:lang="en">CMC</or:termString>
        <rdfs:comment xml:lang="en">Ceramic matrix composites (CMCs) are a subgroup of composite materials as well as a subgroup of technical ceramics. They consist of ceramic fibers embedded in a ceramic matrix, thus forming a ceramic fiber reinforced ceramic (CFRC) material. The matrix and fibers can consist of any ceramic material, whereby carbon and carbon fibers can also be considered a ceramic material.</rdfs:comment>
        <or:termString xml:lang="en">ceramic matrix composite</or:termString>
    </owl:Class>
    


    <!-- http://www.nist.gov/itl/ssd/Materials#CeramicMicrostructure -->

    <owl:Class rdf:about="&mat;CeramicMicrostructure">
        <rdfs:subClassOf rdf:resource="&mat;Microstructure"/>
        <owl:disjointWith rdf:resource="&mat;CompositeMicrostructure"/>
        <owl:disjointWith rdf:resource="&mat;CrystalStructure"/>
        <owl:disjointWith rdf:resource="&mat;MetallicMicrostructure"/>
        <owl:disjointWith rdf:resource="&mat;PolymericMicrostructure"/>
        <rdfs:comment xml:lang="en">Ceramic Microstructure is the material Microstructure of ceramic substancs with components ranging around 0.1 to 100 microns. The microstructure includes grains, secondary phases, grain boundaries, pores, micro-cracks and hardness microindentions.</rdfs:comment>
    </owl:Class>
    


    <!-- http://www.nist.gov/itl/ssd/Materials#CeramicResin -->

    <owl:Class rdf:about="&mat;CeramicResin">
        <rdfs:subClassOf rdf:resource="&mat;Ceramic"/>
        <rdfs:subClassOf rdf:resource="&mat;EngineeredMaterial"/>
        <or:referenceURL rdf:datatype="&xsd;anyURI">http://www.matweb.com/index.aspx</or:referenceURL>
        <or:termString xml:lang="en">ceramic resin</or:termString>
        <or:termString xml:lang="en">high temperature ceramic resin</or:termString>
    </owl:Class>
    


    <!-- http://www.nist.gov/itl/ssd/Materials#Cermet -->

    <owl:Class rdf:about="&mat;Cermet">
        <rdfs:subClassOf rdf:resource="&mat;Ceramic"/>
        <rdfs:subClassOf rdf:resource="&mat;CompositeMaterial"/>
        <rdfs:subClassOf rdf:resource="&mat;EngineeredMaterial"/>
        <rdfs:comment xml:lang="en">Cermet is a composite material composed of ceramic and metallic materials.</rdfs:comment>
        <or:termString xml:lang="en">cermet</or:termString>
    </owl:Class>
    


    <!-- http://www.nist.gov/itl/ssd/Materials#ChalcogenBasedCeramic -->

    <owl:Class rdf:about="&mat;ChalcogenBasedCeramic">
        <rdfs:subClassOf rdf:resource="&mat;Ceramic"/>
        <owl:disjointWith rdf:resource="&mat;NitrideBasedCeramic"/>
        <owl:disjointWith rdf:resource="&mat;OxideBasedCeramic"/>
        <or:referenceURL rdf:datatype="&xsd;anyURI">http://www.matweb.com/index.aspx</or:referenceURL>
        <or:termString xml:lang="en">chalcogenide</or:termString>
        <or:termString xml:lang="en">chalcogenide ceramic</or:termString>
    </owl:Class>
    


    <!-- http://www.nist.gov/itl/ssd/Materials#ChemicalDiffusion -->

    <owl:Class rdf:about="&mat;ChemicalDiffusion">
        <rdfs:subClassOf rdf:resource="&mat;Diffusion"/>
        <owl:disjointWith rdf:resource="&mat;SelfDiffusion"/>
        <owl:disjointWith rdf:resource="&mat;Thermomigration"/>
        <rdfs:comment xml:lang="en">Chemical Diffusion is diffusion under the influence of a gradient in chemical composition.  In concentrated solid solutions, e.g. A(1-x)Bx, or in diffusion couples, the motion of one constituent causes a counterflow of the other constituent(s) or vacancies.  Also called ``interdiffusion&#39;&#39;.</rdfs:comment>
        <rdfs:seeAlso xml:lang="en">Definitions of terms for diffusion in the solid state (IUPAC Recommendations 1999), Pure Appl. Chem. 71, 1307-1325.</rdfs:seeAlso>
    </owl:Class>
    


    <!-- http://www.nist.gov/itl/ssd/Materials#ChemicalSolution -->

    <owl:Class rdf:about="&mat;ChemicalSolution">
        <rdfs:subClassOf rdf:resource="&mat;PhysicalMixture"/>
        <owl:disjointWith rdf:resource="&mat;Colloid"/>
        <owl:disjointWith rdf:resource="&mat;ComplexFluid"/>
        <owl:disjointWith rdf:resource="&mat;CompositeMaterial"/>
        <owl:disjointWith rdf:resource="&mat;GelSubstance"/>
        <owl:disjointWith rdf:resource="&mat;PasteSubstance"/>
        <rdfs:comment xml:lang="en">A Chemical Solution is a homogeneous mixture composed of only one phase. In such a mixture, one or more solutes (chemical substances) are dissolved in a larger quantity of another substance, known as a solvent.The solution more or less takes on the characteristics of the solvent, including its phase.</rdfs:comment>
    </owl:Class>
    


    <!-- http://www.nist.gov/itl/ssd/Materials#ChemicalSuspension -->

    <owl:Class rdf:about="&mat;ChemicalSuspension">
        <rdfs:subClassOf rdf:resource="&mat;ComplexFluid"/>
        <owl:disjointWith rdf:resource="&mat;Colloid"/>
        <owl:disjointWith rdf:resource="&mat;GelSubstance"/>
        <rdfs:comment xml:lang="en">A Chemical Suspension is a heterogeneous fluid containing solid particles that are sufficiently large that the particles will settle out (sedimentation) if the fluid is undisturbed for a sufficent length of time.. </rdfs:comment>
    </owl:Class>
    


    <!-- http://www.nist.gov/itl/ssd/Materials#ChromMolySteel -->

    <owl:Class rdf:about="&mat;ChromMolySteel">
        <rdfs:subClassOf rdf:resource="&mat;Steel"/>
        <owl:disjointWith rdf:resource="&mat;StainlessSteel"/>
        <or:referenceURL rdf:datatype="&xsd;anyURI">http://www.matweb.com/index.aspx</or:referenceURL>
        <or:termString xml:lang="en">CRMO</or:termString>
        <or:termString xml:lang="en">Crome-moly steels are steels that have chromium and molybdenum as alloying elements</or:termString>
        <or:termString xml:lang="en">chrome-moly steel</or:termString>
        <or:termString xml:lang="en">cromoly steel</or:termString>
    </owl:Class>
    


    <!-- http://www.nist.gov/itl/ssd/Materials#Clathrate -->

    <owl:Class rdf:about="&mat;Clathrate">
        <rdfs:subClassOf rdf:resource="&bc;ChemicalSubstance"/>
        <rdfs:subClassOf rdf:resource="&mat;PhysicalMixture"/>
        <owl:disjointWith rdf:resource="&mat;Vacuum"/>
        <rdfs:comment xml:lang="en">A clathrate is a chemical substance consisting of a lattice of one type of molecule trapping and containing a second type of molecule.</rdfs:comment>
    </owl:Class>
    


    <!-- http://www.nist.gov/itl/ssd/Materials#Clay -->

    <owl:Class rdf:about="&mat;Clay">
        <rdfs:subClassOf rdf:resource="&mat;PasteSubstance"/>
        <or:referenceURL rdf:datatype="&xsd;anyURI">http://www.matweb.com/index.aspx</or:referenceURL>
        <rdfs:comment xml:lang="en">Clay is an earthy material that is plastic when moist but hard when fired, that is composed mainly of fine particles of hydrous aluminum silicates and other minerals, and that is used for brick, tile, and pottery.  Particles of clay are less than 5 microns in size according to the sedimentologists&#39; definition; geologists and soil scientists use a limit of 2 microns, while colloid chemists define clays to have particles of under 1 micron in size.</rdfs:comment>
        <or:termString xml:lang="en">clay</or:termString>
    </owl:Class>
    


    <!-- http://www.nist.gov/itl/ssd/Materials#ClosedCellFoam -->

    <owl:Class rdf:about="&mat;ClosedCellFoam">
        <rdfs:subClassOf rdf:resource="&mat;SolidFoam"/>
        <owl:disjointWith rdf:resource="&mat;OpenCellFoam"/>
        <rdfs:comment xml:lang="en">A Closed-Cell Foam is a Solid Foam with a high proportion of intact bubbles.</rdfs:comment>
    </owl:Class>
    


    <!-- http://www.nist.gov/itl/ssd/Materials#CobaltAlloy -->

    <owl:Class rdf:about="&mat;CobaltAlloy">
        <rdfs:subClassOf rdf:resource="&mat;NonFerrousAlloy"/>
        <rdfs:subClassOf>
            <owl:Restriction>
                <owl:onProperty rdf:resource="&mat;physicalDecompositions"/>
                <owl:someValuesFrom rdf:resource="&bc;Cobalt"/>
            </owl:Restriction>
        </rdfs:subClassOf>
        <or:referenceURL rdf:datatype="&xsd;anyURI">http://www.matweb.com/index.aspx</or:referenceURL>
        <rdfs:comment xml:lang="en">An alloy that contains Cobalt but not Iron.</rdfs:comment>
    </owl:Class>
    


    <!-- http://www.nist.gov/itl/ssd/Materials#ColinearInterstitialcyMechanism -->

    <owl:Class rdf:about="&mat;ColinearInterstitialcyMechanism">
        <rdfs:subClassOf rdf:resource="&mat;InterstitialcyMechanism"/>
        <owl:disjointWith rdf:resource="&mat;DirectInterstitialMechanism"/>
        <owl:disjointWith rdf:resource="&mat;NonCollinearInterstitialcyMechanism"/>
        <rdfs:seeAlso>Definitions of terms for diffusion in the solid state (IUPAC Recommendations 1999), Pure Appl. Chem. 71, 1307-1325.</rdfs:seeAlso>
        <rdfs:comment xml:lang="en">The Collinear Iinterstitialcy Mechanism is an interstitialcy mechanism in which an interstitial atom and the lattice atom which it displaces move along the same straight line.</rdfs:comment>
    </owl:Class>
    


    <!-- http://www.nist.gov/itl/ssd/Materials#Colloid -->

    <owl:Class rdf:about="&mat;Colloid">
        <rdfs:subClassOf rdf:resource="&mat;PhysicalMixture"/>
        <owl:disjointWith rdf:resource="&mat;CompositeMaterial"/>
        <rdfs:comment xml:lang="en">A colloid is a solid, liquid, or gasseous substance comprised of one or more substances microscopically dispersed evenly throughout another substance (the dispersion medium).  

A colloidal system consists of two separate phases: a dispersed phase (or internal phase) and a continuous phase.  Either of the phases may be solid, liquid, or gas, however, both phases can not be gas.</rdfs:comment>
    </owl:Class>
    


    <!-- http://www.nist.gov/itl/ssd/Materials#ColloidalSol -->

    <owl:Class rdf:about="&mat;ColloidalSol">
        <rdfs:subClassOf rdf:resource="&mat;Colloid"/>
        <rdfs:subClassOf rdf:resource="&mat;LiquidSubstance"/>
        <owl:disjointWith rdf:resource="&mat;Emulsion"/>
        <owl:disjointWith rdf:resource="&mat;Foam"/>
        <owl:disjointWith rdf:resource="&mat;LiquidSlag"/>
        <owl:disjointWith rdf:resource="&mat;LiquidSolution"/>
        <rdfs:comment xml:lang="en">A Colloidal Sol is a colloidal suspension of very small solid particles in a continuous liquid medium.</rdfs:comment>
    </owl:Class>
    


    <!-- http://www.nist.gov/itl/ssd/Materials#CompactedPowderAlloy -->

    <owl:Class rdf:about="&mat;CompactedPowderAlloy">
        <rdfs:subClassOf rdf:resource="&mat;EngineeredAlloy"/>
        <owl:disjointWith rdf:resource="&mat;WroughtAlloy"/>
        <rdfs:comment xml:lang="en">A Compacted Powder Alloy is produced by the  powder metallurgy process, generally consisting of four basic steps: (1) powder manufacture, (2) powder blending,(3) compacting, (4) either sintering or metal injection molding. </rdfs:comment>
    </owl:Class>
    


    <!-- http://www.nist.gov/itl/ssd/Materials#Compaction -->

    <owl:Class rdf:about="&mat;Compaction">
        <rdfs:subClassOf rdf:resource="&mat;Deformation"/>
        <owl:disjointWith rdf:resource="&mat;MaterialCreep"/>
        <rdfs:comment xml:lang="en">Compaction is a process of pressing material such that it deforms and occupies less space.  Compaction can be intentional or not.</rdfs:comment>
    </owl:Class>
    


    <!-- http://www.nist.gov/itl/ssd/Materials#ComplexFluid -->

    <owl:Class rdf:about="&mat;ComplexFluid">
        <rdfs:subClassOf rdf:resource="&mat;FluidSubstance"/>
        <rdfs:subClassOf rdf:resource="&mat;PhysicalMixture"/>
        <owl:disjointWith rdf:resource="&mat;SolidSol"/>
        <rdfs:comment xml:lang="en">Complex fluids are mixtures that have a coexistence between two phases: solid–liquid (suspensions or solutions of macromolecules such as polymers), solid–gas (granular), liquid–gas (foams) and liquid–liquid (emulsions).</rdfs:comment>
    </owl:Class>
    


    <!-- http://www.nist.gov/itl/ssd/Materials#CompositeMaterial -->

    <owl:Class rdf:about="&mat;CompositeMaterial">
        <rdfs:subClassOf rdf:resource="&mat;PhysicalMixture"/>
        <rdfs:subClassOf rdf:resource="&mat;SolidSubstance"/>
        <owl:disjointWith rdf:resource="&mat;CrystallineSubstance"/>
        <owl:disjointWith rdf:resource="&mat;GlassyMaterial"/>
    </owl:Class>
    


    <!-- http://www.nist.gov/itl/ssd/Materials#CompositeMicrostructure -->

    <owl:Class rdf:about="&mat;CompositeMicrostructure">
        <rdfs:subClassOf rdf:resource="&mat;Microstructure"/>
        <owl:disjointWith rdf:resource="&mat;CrystalStructure"/>
        <owl:disjointWith rdf:resource="&mat;MetallicMicrostructure"/>
        <owl:disjointWith rdf:resource="&mat;PolymericMicrostructure"/>
        <rdfs:comment xml:lang="en">A Composite Microstructure is a material Microstructure of a materials made from two or more constituent materials with significantly different physical or chemical properties which remain separate and distinct at microscopic scale within the finished structure.</rdfs:comment>
    </owl:Class>
    


    <!-- http://www.nist.gov/itl/ssd/Materials#Compressibility -->

    <owl:Class rdf:about="&mat;Compressibility">
        <rdfs:subClassOf rdf:resource="&mat;DeformationProperty"/>
        <owl:disjointWith rdf:resource="&mat;ElasticModulus"/>
        <owl:disjointWith rdf:resource="&mat;FractureStrength"/>
        <owl:disjointWith rdf:resource="&mat;Hardness"/>
        <owl:disjointWith rdf:resource="&mat;Stiffness"/>
    </owl:Class>
    


    <!-- http://www.nist.gov/itl/ssd/Materials#ConcentrationProfile -->

    <owl:Class rdf:about="&mat;ConcentrationProfile">
        <rdfs:subClassOf rdf:resource="&or;CurveSegment"/>
        <rdfs:comment xml:lang="en">A Concentration Profile is a Curve of the variation in the concentration of a diffusing species as a function of distance in a material.</rdfs:comment>
        <rdfs:seeAlso xml:lang="en">Definitions of terms for diffusion in the solid state (IUPAC Recommendations 1999), Pure Appl. Chem. 71, 1307-1325.</rdfs:seeAlso>
    </owl:Class>
    


    <!-- http://www.nist.gov/itl/ssd/Materials#Concrete -->

    <owl:Class rdf:about="&mat;Concrete">
        <rdfs:subClassOf rdf:resource="&mat;CompositeMaterial"/>
        <rdfs:subClassOf rdf:resource="&mat;EngineeredMaterial"/>
        <or:referenceURL rdf:datatype="&xsd;anyURI">http://www.matweb.com/index.aspx</or:referenceURL>
        <or:termString xml:lang="en">concrete</or:termString>
    </owl:Class>
    


    <!-- http://www.nist.gov/itl/ssd/Materials#Condensing -->

    <owl:Class rdf:about="&mat;Condensing">
        <rdfs:subClassOf rdf:resource="&mat;PhaseChange"/>
        <owl:disjointWith rdf:resource="&mat;CrystallinePhaseChange"/>
        <owl:disjointWith rdf:resource="&mat;OrderDisorderPhaseTransformation"/>
        <owl:disjointWith rdf:resource="&mat;PrecipitationFromSolution"/>
        <owl:disjointWith rdf:resource="&mat;SolidToSolidPhaseTransformation"/>
        <owl:disjointWith rdf:resource="&mat;Solidification"/>
        <owl:disjointWith rdf:resource="&mat;Vaporization"/>
        <rdfs:comment xml:lang="en">Condensing is the Phase Change from a gasseous state to a liquid state.</rdfs:comment>
    </owl:Class>
    


    <!-- http://www.nist.gov/itl/ssd/Materials#CoolingCurve -->

    <owl:Class rdf:about="&mat;CoolingCurve">
        <rdfs:subClassOf rdf:resource="&mat;HeatingCoolingCurve"/>
        <or:termString xml:lang="en">cooling curve</or:termString>
    </owl:Class>
    


    <!-- http://www.nist.gov/itl/ssd/Materials#CoolingProcess -->

    <owl:Class rdf:about="&mat;CoolingProcess">
        <rdfs:subClassOf rdf:resource="&mat;TemperatureChangeProcess"/>
        <rdfs:comment xml:lang="en">A Cooling Process is a Temperature Change Process during which an object looses heat.  This could be due to endothermic reactions, the object radiating heat or warming up its environment, or some combination of these.. </rdfs:comment>
    </owl:Class>
    


    <!-- http://www.nist.gov/itl/ssd/Materials#CopperAlloy -->

    <owl:Class rdf:about="&mat;CopperAlloy">
        <rdfs:subClassOf rdf:resource="&mat;NonFerrousAlloy"/>
        <rdfs:subClassOf>
            <owl:Restriction>
                <owl:onProperty rdf:resource="&mat;physicalDecompositions"/>
                <owl:someValuesFrom rdf:resource="&bc;Copper"/>
            </owl:Restriction>
        </rdfs:subClassOf>
        <or:referenceURL rdf:datatype="&xsd;anyURI">http://www.matweb.com/index.aspx</or:referenceURL>
        <rdfs:comment xml:lang="en">An alloy that contains Copper but little or no Iron.</rdfs:comment>
    </owl:Class>
    


    <!-- http://www.nist.gov/itl/ssd/Materials#Cracking -->

    <owl:Class rdf:about="&mat;Cracking">
        <rdfs:subClassOf rdf:resource="&or;MechanicalProcess"/>
        <rdfs:subClassOf rdf:resource="&or;MovementEvent"/>
        <owl:disjointWith rdf:resource="&mat;MaterialFatigue"/>
        <owl:disjointWith rdf:resource="&mat;MicroscopicDiffusionMovement"/>
        <owl:disjointWith rdf:resource="&mat;PhaseChange"/>
        <owl:disjointWith rdf:resource="&mat;TemperatureChangeProcess"/>
        <owl:disjointWith rdf:resource="&mat;ThermalExpansion"/>
        <rdfs:comment xml:lang="en">Cracking is a Mechanical Process in which some solid object is cracked -- at either a macroscopic or microscopic level.  The cracked material need not be broken into separate pieces.</rdfs:comment>
    </owl:Class>
    


    <!-- http://www.nist.gov/itl/ssd/Materials#CrowdionMechanism -->

    <owl:Class rdf:about="&mat;CrowdionMechanism">
        <rdfs:subClassOf rdf:resource="&mat;NonCollinearInterstitialcyMechanism"/>
        <owl:disjointWith rdf:resource="&mat;DumbellIntersticialcyMechanism"/>
        <rdfs:comment>Definitions of terms for diffusion in the solid state (IUPAC Recommendations 1999), Pure Appl. Chem. 71, 1307-1325.</rdfs:comment>
        <rdfs:comment xml:lang="en">The Crowdion Mechanismi is a hypothesized mechanism in which diffusion takes place by a co-operative movement of a group of atoms one of which is typically centred on an interstitial position with the others relaxed from their normal lattice sites to accommodate the additional ‘crowdion’.</rdfs:comment>
        <skos:note xml:lang="en">There was a big scientific controversy over the question if crowdions actually exist as a metastable interstitial configuration in the seventies. This controversy has never been finally resolved; however, most researchers in the field believe that it does not exist.</skos:note>
        <rdfs:seeAlso xml:lang="en">http://www.tf.uni-kiel.de/matwis/amat/def_en/kap_1/advanced/t1_3_1.html</rdfs:seeAlso>
    </owl:Class>
    


    <!-- http://www.nist.gov/itl/ssd/Materials#CrystalGrain -->

    <owl:Class rdf:about="&mat;CrystalGrain">
        <rdfs:subClassOf rdf:resource="&mat;CrystallineSubstance"/>
        <rdfs:comment xml:lang="en">Crystal grains or crystallites are small, often microscopic crystals that, held together through highly defective boundaries, constitute a polycrystalline solid.</rdfs:comment>
    </owl:Class>
    


    <!-- http://www.nist.gov/itl/ssd/Materials#CrystalLattice -->

    <owl:Class rdf:about="&mat;CrystalLattice">
        <rdfs:subClassOf rdf:resource="&or;PhysicalObject"/>
        <owl:disjointWith rdf:resource="&mat;Vacuum"/>
    </owl:Class>
    


    <!-- http://www.nist.gov/itl/ssd/Materials#CrystalStructure -->

    <owl:Class rdf:about="&mat;CrystalStructure">
        <rdfs:subClassOf rdf:resource="&mat;Microstructure"/>
        <rdfs:subClassOf rdf:resource="&or;MaterialType"/>
        <owl:disjointWith rdf:resource="&mat;MineralType"/>
        <owl:disjointWith rdf:resource="&mat;MultiphaseMaterialType"/>
        <owl:disjointWith rdf:resource="&mat;PolymericMicrostructure"/>
        <rdfs:comment xml:lang="en">A crystal structure is composed of a pattern, a set of atoms arranged in a particular way, and a lattice exhibiting long-range order and symmetry.</rdfs:comment>
    </owl:Class>
    


    <!-- http://www.nist.gov/itl/ssd/Materials#CrystallinePhaseChange -->

    <owl:Class rdf:about="&mat;CrystallinePhaseChange">
        <rdfs:subClassOf rdf:resource="&mat;MicrostructureEvolution"/>
        <rdfs:subClassOf rdf:resource="&mat;SolidToSolidPhaseTransformation"/>
        <owl:disjointWith rdf:resource="&mat;OrderDisorderPhaseTransformation"/>
        <owl:disjointWith rdf:resource="&mat;Solidification"/>
        <owl:disjointWith rdf:resource="&mat;Vaporization"/>
        <rdfs:comment xml:lang="en">A Crystalline Phase Change is a Phase Change in which the phase changes between crystalline phases.</rdfs:comment>
    </owl:Class>
    


    <!-- http://www.nist.gov/itl/ssd/Materials#CrystallineSubstance -->

    <owl:Class rdf:about="&mat;CrystallineSubstance">
        <rdfs:subClassOf rdf:resource="&bc;MaterialSubstance"/>
        <owl:disjointWith rdf:resource="&mat;GaseousSubstance"/>
        <owl:disjointWith rdf:resource="&mat;PasteSubstance"/>
        <owl:disjointWith rdf:resource="&mat;PolymerSubstance"/>
        <owl:disjointWith rdf:resource="&mat;Vacuum"/>
        <rdfs:comment xml:lang="en">Material in a crystalline phase</rdfs:comment>
    </owl:Class>
    


    <!-- http://www.nist.gov/itl/ssd/Materials#CubicCrystalStructure -->

    <owl:Class rdf:about="&mat;CubicCrystalStructure">
        <rdfs:subClassOf rdf:resource="&mat;CrystalLattice"/>
        <owl:disjointWith rdf:resource="&mat;MonoclinicCrystalStructure"/>
        <owl:disjointWith rdf:resource="&mat;OrthorhombicCrystalStructure"/>
        <owl:disjointWith rdf:resource="&mat;TetragonalCrystalStructure"/>
        <owl:disjointWith rdf:resource="&mat;TriclinicCrystalStructure"/>
        <owl:disjointWith rdf:resource="&mat;TrigonalCrystalStructure"/>
    </owl:Class>
    


    <!-- http://www.nist.gov/itl/ssd/Materials#Deformation -->

    <owl:Class rdf:about="&mat;Deformation">
        <rdfs:subClassOf rdf:resource="&or;MechanicalProcess"/>
        <rdfs:comment xml:lang="en">Deformation is a Mechanical Process in which a solid or semi-solid object changes shape in response to outside forces.</rdfs:comment>
    </owl:Class>
    


    <!-- http://www.nist.gov/itl/ssd/Materials#DeformationProperty -->

    <owl:Class rdf:about="&mat;DeformationProperty">
        <rdfs:subClassOf rdf:resource="&mat;MeasurableMechanicalProperty"/>
        <owl:disjointWith rdf:resource="&mat;Entropy"/>
        <owl:disjointWith rdf:resource="&mat;Strength"/>
        <owl:disjointWith rdf:resource="&mat;TransportProperty"/>
    </owl:Class>
    


    <!-- http://www.nist.gov/itl/ssd/Materials#DeviatonicDominantPhaseTransformation -->

    <owl:Class rdf:about="&mat;DeviatonicDominantPhaseTransformation">
        <rdfs:subClassOf rdf:resource="&mat;LatticeDistortivePhaseTransformation"/>
        <owl:disjointWith rdf:resource="&mat;DilationDominantPhaseTransformation"/>
        <rdfs:comment xml:lang="en">A deviatonic Dominant Phase Transformation is dominated in a sheer distortion in the lattice, with cutting plates perpendicular to the sheer undistorted.</rdfs:comment>
    </owl:Class>
    


    <!-- http://www.nist.gov/itl/ssd/Materials#Diamond -->

    <owl:Class rdf:about="&mat;Diamond">
        <rdfs:subClassOf rdf:resource="&bc;Carbon"/>
        <rdfs:subClassOf rdf:resource="&mat;SolidCrystallineSubstance"/>
        <owl:disjointWith rdf:resource="&mat;Graphite"/>
        <or:referenceURL rdf:datatype="&xsd;anyURI">http://www.matweb.com/index.aspx</or:referenceURL>
        <or:termString xml:lang="en">diamond</or:termString>
    </owl:Class>
    


    <!-- http://www.nist.gov/itl/ssd/Materials#DielectricProperty -->

    <owl:Class rdf:about="&mat;DielectricProperty">
        <rdfs:subClassOf rdf:resource="&mat;ElectricalProperty"/>
        <owl:disjointWith rdf:resource="&mat;ElectricPolarizability"/>
        <rdfs:comment xml:lang="en">Dielectric Properties are properties of a Dielectric -- an insulating material that undergoes polarization in an electric field.</rdfs:comment>
    </owl:Class>
    


    <!-- http://www.nist.gov/itl/ssd/Materials#Diffusion -->

    <owl:Class rdf:about="&mat;Diffusion">
        <rdfs:subClassOf rdf:resource="&or;MechanicalProcess"/>
        <rdfs:subClassOf rdf:resource="&or;MovementEvent"/>
        <owl:disjointWith rdf:resource="&mat;MaterialFatigue"/>
        <owl:disjointWith rdf:resource="&mat;PhaseChange"/>
        <owl:disjointWith rdf:resource="&mat;TemperatureChangeProcess"/>
        <owl:disjointWith rdf:resource="&mat;ThermalExpansion"/>
        <rdfs:comment xml:lang="en">Diffusion is the process of the spread of particles through random motion from regions of higher concentration to regions of lower concentration. The time dependence of the statistical distribution in space is given by the diffusion equation.</rdfs:comment>
    </owl:Class>
    


    <!-- http://www.nist.gov/itl/ssd/Materials#DiffusionBonding -->

    <owl:Class rdf:about="&mat;DiffusionBonding">
        <rdfs:subClassOf rdf:resource="&bc;ChemicalProcess"/>
        <rdfs:seeAlso xml:lang="en">Definitions of terms for diffusion in the solid state (IUPAC Recommendations 1999), Pure Appl. Chem. 71, 1307-1325.</rdfs:seeAlso>
        <rdfs:comment xml:lang="en">Diffusion Bonding is a solid state bonding process that joins two materials by a diffusion reaction.</rdfs:comment>
    </owl:Class>
    


    <!-- http://www.nist.gov/itl/ssd/Materials#DiffusionInducedGrainBoundaryMigration -->

    <owl:Class rdf:about="&mat;DiffusionInducedGrainBoundaryMigration">
        <rdfs:subClassOf rdf:resource="&mat;MicroscopicDiffusionMovement"/>
        <rdfs:subClassOf rdf:resource="&mat;MicrostructureEvolution"/>
        <owl:disjointWith rdf:resource="&mat;ExchangeMechanismForDiffusion"/>
        <owl:disjointWith rdf:resource="&mat;FiveFrequencyDiffusionModel"/>
        <owl:disjointWith rdf:resource="&mat;InterstitialcyMechanism"/>
        <owl:disjointWith rdf:resource="&mat;RelaxationMethodForDiffusion"/>
        <rdfs:seeAlso>Definitions of terms for diffusion in the solid state (IUPAC Recommendations 1999), Pure Appl. Chem. 71, 1307-1325.</rdfs:seeAlso>
        <rdfs:comment xml:lang="en">If a polycrystalline material undergoes an interdiffusion process, the grain boundaries move in a direction perpendicular to the diffusion flux.  As a result the concentrations in the regions swept by the boundaries change.  This is called ``Diffusion-Induced Grain boundary Migration&#39;&#39; (DIGM).</rdfs:comment>
        <or:termString xml:lang="en">diffusion induced grain boundary migration</or:termString>
    </owl:Class>
    


    <!-- http://www.nist.gov/itl/ssd/Materials#DiffusionMovementMechanism -->

    <owl:Class rdf:about="&mat;DiffusionMovementMechanism">
        <rdfs:subClassOf rdf:resource="&or;EventType"/>
        <rdfs:comment xml:lang="en">A Diffusion Movement Mechanism is a type of microscopic movement which is responsible for diffusion.</rdfs:comment>
    </owl:Class>
    


    <!-- http://www.nist.gov/itl/ssd/Materials#DiffusionProperty -->

    <owl:Class rdf:about="&mat;DiffusionProperty">
        <rdfs:subClassOf rdf:resource="&or;MeasurableMaterialProperty"/>
        <rdfs:comment xml:lang="en">A Diffusion Property is a physical property of some physical material or object, related from diffusion, whether chemical, electrical, magnetic, or thermal diffusion. </rdfs:comment>
    </owl:Class>
    


    <!-- http://www.nist.gov/itl/ssd/Materials#DiffusionalPhaseTransformation -->

    <owl:Class rdf:about="&mat;DiffusionalPhaseTransformation">
        <rdfs:subClassOf rdf:resource="&mat;PhaseChange"/>
        <rdfs:comment xml:lang="en">A diffusional transformation is a phase change that occurs via the long-range diffusion of atoms</rdfs:comment>
    </owl:Class>
    


    <!-- http://www.nist.gov/itl/ssd/Materials#DiffusionlessPhaseTransformation -->

    <owl:Class rdf:about="&mat;DiffusionlessPhaseTransformation">
        <rdfs:subClassOf rdf:resource="&mat;CrystallinePhaseChange"/>
        <rdfs:comment xml:lang="en">A diffusionless transformation is a phase change that occurs without the long-range diffusion of atoms but rather by some form of cooperative, homogeneous movement of many atoms that results in a change in crystal structure. These movements are small, usually less than the interatomic distances, and the atoms maintain their relative relationships.</rdfs:comment>
        <oil:seeAlso>http://en.wikipedia.org/w/index.php?title=File:Diffusionless_classification.svg</oil:seeAlso>
    </owl:Class>
    


    <!-- http://www.nist.gov/itl/ssd/Materials#DilationDominantPhaseTransformation -->

    <owl:Class rdf:about="&mat;DilationDominantPhaseTransformation">
        <rdfs:subClassOf rdf:resource="&mat;LatticeDistortivePhaseTransformation"/>
        <rdfs:comment xml:lang="en">A Dilation Dominant Phase Transformation is dominated by the expansion or contraction of the atomic lattice.</rdfs:comment>
    </owl:Class>
    


    <!-- http://www.nist.gov/itl/ssd/Materials#DirectInterstitialMechanism -->

    <owl:Class rdf:about="&mat;DirectInterstitialMechanism">
        <rdfs:subClassOf rdf:resource="&mat;InterstitialcyMechanism"/>
        <owl:disjointWith rdf:resource="&mat;NonCollinearInterstitialcyMechanism"/>
        <rdfs:seeAlso xml:lang="en">Definitions of terms for diffusion in the solid state (IUPAC Recommendations 1999), Pure Appl. Chem. 71, 1307-1325.</rdfs:seeAlso>
        <rdfs:comment xml:lang="en">In the Direct Interstitial Mechanism diffusion takes place by the direct migration of an interstitial species from one interstitial position to another.</rdfs:comment>
    </owl:Class>
    


    <!-- http://www.nist.gov/itl/ssd/Materials#DisorderedBCCPhase -->

    <owl:Class rdf:about="&mat;DisorderedBCCPhase">
        <rdfs:subClassOf rdf:resource="&mat;BodyCenteredCubicCrystalStructure"/>
        <owl:disjointWith rdf:resource="&mat;OrderedBCCPhase"/>
    </owl:Class>
    


    <!-- http://www.nist.gov/itl/ssd/Materials#DisorderedFCCPhase -->

    <owl:Class rdf:about="&mat;DisorderedFCCPhase">
        <rdfs:subClassOf rdf:resource="&mat;FaceCenteredCubicCrystalStructure"/>
        <owl:disjointWith rdf:resource="&mat;OrderedFCCPhase"/>
    </owl:Class>
    


    <!-- http://www.nist.gov/itl/ssd/Materials#DisorderedHCPPhase -->

    <owl:Class rdf:about="&mat;DisorderedHCPPhase">
        <rdfs:subClassOf rdf:resource="&mat;HexagonalClosePackedCrystalStructure"/>
        <owl:disjointWith rdf:resource="&mat;OrderedHCPPhase"/>
    </owl:Class>
    


    <!-- http://www.nist.gov/itl/ssd/Materials#DisorderedSolidSolution -->

    <owl:Class rdf:about="&mat;DisorderedSolidSolution">
        <rdfs:subClassOf rdf:resource="&mat;MaterialPhaseComposition"/>
    </owl:Class>
    


    <!-- http://www.nist.gov/itl/ssd/Materials#DissociativeDiffusion -->

    <owl:Class rdf:about="&mat;DissociativeDiffusion">
        <rdfs:subClassOf rdf:resource="&mat;Heterodiffusion"/>
        <owl:disjointWith rdf:resource="&mat;InterchangeDiffusion"/>
        <rdfs:seeAlso xml:lang="en">Definitions of terms for diffusion in the solid state (IUPAC Recommendations 1999), Pure Appl. Chem. 71, 1307-1325.</rdfs:seeAlso>
        <rdfs:comment xml:lang="en">Dissociative diffusion is the process by which foreign atoms predominantly present at normal lattice sites migrate via interstitial sites.</rdfs:comment>
    </owl:Class>
    


    <!-- http://www.nist.gov/itl/ssd/Materials#DistortedHexagonalCrystalStructure -->

    <owl:Class rdf:about="&mat;DistortedHexagonalCrystalStructure">
        <rdfs:subClassOf rdf:resource="&mat;HexagonalCrystalStructure"/>
        <owl:disjointWith rdf:resource="&mat;DoubleHexagonalClosePackedCrystalStructure"/>
        <owl:disjointWith rdf:resource="&mat;HexagonalClosePackedCrystalStructure"/>
    </owl:Class>
    


    <!-- http://www.nist.gov/itl/ssd/Materials#DivacancyMechanism -->

    <owl:Class rdf:about="&mat;DivacancyMechanism">
        <rdfs:subClassOf rdf:resource="&mat;VacancyDiffusionMechanism"/>
        <owl:disjointWith rdf:resource="&mat;FiveFrequencyDiffusionModel"/>
        <owl:disjointWith rdf:resource="&mat;RelaxationMethodForDiffusion"/>
        <rdfs:seeAlso xml:lang="en">Definitions of terms for diffusion in the solid state (IUPAC Recommendations 1999), Pure Appl. Chem. 71, 1307-1325.</rdfs:seeAlso>
        <rdfs:comment xml:lang="en">The Divacancy Mechanism is the diffusion process by which a crystal lattice vacancy pair is used by any constituent species of the material to effect diffusion.</rdfs:comment>
    </owl:Class>
    


    <!-- http://www.nist.gov/itl/ssd/Materials#DoubleHexagonalClosePackedCrystalStructure -->

    <owl:Class rdf:about="&mat;DoubleHexagonalClosePackedCrystalStructure">
        <rdfs:subClassOf rdf:resource="&mat;HexagonalCrystalStructure"/>
        <owl:disjointWith rdf:resource="&mat;HexagonalClosePackedCrystalStructure"/>
    </owl:Class>
    


    <!-- http://www.nist.gov/itl/ssd/Materials#DuctileIron -->

    <owl:Class rdf:about="&mat;DuctileIron">
        <rdfs:subClassOf rdf:resource="&mat;CastIron"/>
        <owl:disjointWith rdf:resource="&mat;GrayCastIron"/>
        <owl:disjointWith rdf:resource="&mat;MalleableIron"/>
        <owl:disjointWith rdf:resource="&mat;WhiteCastIron"/>
        <or:referenceURL rdf:datatype="&xsd;anyURI">http://www.matweb.com/index.aspx</or:referenceURL>
        <rdfs:comment xml:lang="en">Ductile iron, also known as ductile cast iron, nodular cast iron, spheroidal graphite iron, spherulitic graphite cast iron, and SG iron, is a type of cast iron that is much more flexible and elastic than other cast irons, due to its nodular graphite inclusions.</rdfs:comment>
        <or:termString xml:lang="en">SG iron</or:termString>
        <or:termString xml:lang="en">ductile cast iron</or:termString>
        <or:termString xml:lang="en">ductile iron</or:termString>
        <or:termString xml:lang="en">nodular cast iron</or:termString>
        <or:termString xml:lang="en">spheroidal graphite iron</or:termString>
        <or:termString xml:lang="en">spherulitic graphite cast iron</or:termString>
    </owl:Class>
    


    <!-- http://www.nist.gov/itl/ssd/Materials#DumbellIntersticialcyMechanism -->

    <owl:Class rdf:about="&mat;DumbellIntersticialcyMechanism">
        <rdfs:subClassOf rdf:resource="&mat;NonCollinearInterstitialcyMechanism"/>
        <rdfs:seeAlso xml:lang="en">Definitions of terms for diffusion in the solid state (IUPAC Recommendations 1999), Pure Appl. Chem. 71, 1307-1325.</rdfs:seeAlso>
        <rdfs:comment xml:lang="en">In some diffusion systems the equilibrium configuration during an interstitialcy jump consists of a dumbbell-like defect with each of the moving ions being displaced by an equal amount from the normal lattice position.  Diffusion taking place via such species is said to proceed by a Dumbbell Interstitialcy Mechanism.</rdfs:comment>
    </owl:Class>
    


    <!-- http://www.nist.gov/itl/ssd/Materials#DuplexStainlessSteel -->

    <owl:Class rdf:about="&mat;DuplexStainlessSteel">
        <rdfs:subClassOf rdf:resource="&mat;StainlessSteel"/>
        <owl:disjointWith rdf:resource="&mat;FerriticStainlessSteel"/>
        <or:referenceURL rdf:datatype="&xsd;anyURI">http://www.matweb.com/index.aspx</or:referenceURL>
        <rdfs:comment xml:lang="en">Duplex Stainless Steels have a mixed microstructure of austenite and ferrite, the aim usually being to produce a 50/50 mix, although in commercial alloys the ratio may be 40/60. Duplex stainless steels have roughly twice the strength compared to austenitic stainless steels and also improved resistance to localized corrosion, particularly pitting, crevice corrosion and stress corrosion cracking. They are characterized by high chromium (19–32%) and molybdenum (up to 5%) and lower nickel contents than austenitic stainless steels.</rdfs:comment>
        <or:termString xml:lang="en">duplex</or:termString>
        <or:termString xml:lang="en">duplex stainless steel</or:termString>
    </owl:Class>
    


    <!-- http://www.nist.gov/itl/ssd/Materials#Duterium -->

    <owl:Class rdf:about="&mat;Duterium">
        <rdfs:subClassOf rdf:resource="&bc;Hydrogen"/>
        <rdfs:subClassOf rdf:resource="&mat;RadioactiveMaterial"/>
    </owl:Class>
    


    <!-- http://www.nist.gov/itl/ssd/Materials#ElasticModulus -->

    <owl:Class rdf:about="&mat;ElasticModulus">
        <rdfs:subClassOf rdf:resource="&mat;DeformationProperty"/>
        <owl:disjointWith rdf:resource="&mat;FractureStrength"/>
        <owl:disjointWith rdf:resource="&mat;Hardness"/>
        <owl:disjointWith rdf:resource="&mat;TransportProperty"/>
        <rdfs:comment xml:lang="en">An elastic modulus is defined as the slope of its stress–strain curve of a substance within the range where the deformation is elastic.  Three varieties of this are Young&#39;s modulus, the sheer modulus, and the bulk modulus.</rdfs:comment>
    </owl:Class>
    


    <!-- http://www.nist.gov/itl/ssd/Materials#Elastomer -->

    <owl:Class rdf:about="&mat;Elastomer">
        <rdfs:subClassOf rdf:resource="&mat;PolymerSubstance"/>
        <owl:disjointWith rdf:resource="&mat;Polyester"/>
        <rdfs:comment xml:lang="en">An elastomer is a polymer with viscoelasticity, generally having low Young&#39;s modulus and high yield strain compared with other materials. Each of the monomers which link to form the polymer is usually made of carbon, hydrogen, oxygen and/or silicon. Elastomers are amorphous polymers existing above their glass transition temperature, so that considerable segmental motion is possible. At ambient temperatures, rubbers are thus relatively soft and deformable.  Rubber is an example elastomer.

Elastomers are usually thermosets but may also be thermoplastic.</rdfs:comment>
    </owl:Class>
    


    <!-- http://www.nist.gov/itl/ssd/Materials#ElectricPolarizability -->

    <owl:Class rdf:about="&mat;ElectricPolarizability">
        <rdfs:subClassOf rdf:resource="&mat;ElectricalProperty"/>
        <rdfs:comment xml:lang="en">Electric Polarizability is the tendency of a substance&#39;s charge distribution to be distorted from its normal shape by an external electric field.  It is specified by the material&#39;s relative permittivity (dielectric constant).</rdfs:comment>
    </owl:Class>
    


    <!-- http://www.nist.gov/itl/ssd/Materials#ElectricalProperty -->

    <owl:Class rdf:about="&mat;ElectricalProperty">
        <rdfs:subClassOf rdf:resource="&or;MeasurableMaterialProperty"/>
        <owl:disjointWith rdf:resource="&mat;MechanicalProperty"/>
        <owl:disjointWith rdf:resource="&mat;OpticalProperty"/>
        <owl:disjointWith rdf:resource="&mat;RadiologicalProperty"/>
        <owl:disjointWith rdf:resource="&mat;ThermalProperty"/>
    </owl:Class>
    


    <!-- http://www.nist.gov/itl/ssd/Materials#Electromigration -->

    <owl:Class rdf:about="&mat;Electromigration">
        <rdfs:subClassOf rdf:resource="&or;MovementEvent"/>
        <rdfs:comment xml:lang="en">Electromigration is the transport of particles under the influence of an electric field</rdfs:comment>
    </owl:Class>
    


    <!-- http://www.nist.gov/itl/ssd/Materials#ElectronicMagneticAlloy -->

    <owl:Class rdf:about="&mat;ElectronicMagneticAlloy">
        <rdfs:subClassOf rdf:resource="&mat;Alloy"/>
        <or:referenceURL rdf:datatype="&xsd;anyURI">http://www.matweb.com/index.aspx</or:referenceURL>
        <rdfs:comment xml:lang="en">This means `Electronic/Magnetic Alloy&#39; as the term is used in MatWeb.  The term exculdes most ferrous metals.</rdfs:comment>
        <or:termString xml:lang="en">electronic/magnetic alloy</or:termString>
    </owl:Class>
    


    <!-- http://www.nist.gov/itl/ssd/Materials#ElementalMetal -->

    <owl:Class rdf:about="&mat;ElementalMetal">
        <rdfs:subClassOf rdf:resource="&bc;ElementalSubstance"/>
        <rdfs:subClassOf rdf:resource="&bc;Metal"/>
        <owl:disjointWith rdf:resource="&mat;PhysicalMixture"/>
        <rdfs:comment xml:lang="en">ElementalMetal is Metal composed of a single element.  It is disjoint from Alloy.</rdfs:comment>
    </owl:Class>
    


    <!-- http://www.nist.gov/itl/ssd/Materials#Emulsion -->

    <owl:Class rdf:about="&mat;Emulsion">
        <rdfs:subClassOf rdf:resource="&mat;Colloid"/>
        <rdfs:subClassOf rdf:resource="&mat;ComplexFluid"/>
        <owl:disjointWith rdf:resource="&mat;Foam"/>
        <owl:disjointWith rdf:resource="&mat;GelSubstance"/>
        <rdfs:comment xml:lang="en">An Emulsion is a Colloid of two or more liquids that are normally immiscible.</rdfs:comment>
    </owl:Class>
    


    <!-- http://www.nist.gov/itl/ssd/Materials#EnergyPerMass -->

    <owl:Class rdf:about="&mat;EnergyPerMass">
        <owl:equivalentClass>
            <owl:Class>
                <owl:intersectionOf rdf:parseType="Collection">
                    <rdf:Description rdf:about="&or;MeasurableQuantity"/>
                    <owl:Restriction>
                        <owl:onProperty rdf:resource="&or;unitsFor"/>
                        <owl:someValuesFrom rdf:resource="&mat;UnitOfEnergyPerMass"/>
                    </owl:Restriction>
                </owl:intersectionOf>
            </owl:Class>
        </owl:equivalentClass>
        <rdfs:subClassOf rdf:resource="&or;MeasurableQuantity"/>
        <rdfs:subClassOf>
            <owl:Restriction>
                <owl:onProperty rdf:resource="&or;unitsFor"/>
                <owl:someValuesFrom rdf:resource="&mat;UnitOfEnergyPerMass"/>
            </owl:Restriction>
        </rdfs:subClassOf>
        <owl:disjointWith rdf:resource="&or;Area"/>
        <owl:disjointWith rdf:resource="&or;ComputerStorageCapacity"/>
        <owl:disjointWith rdf:resource="&or;Distance"/>
        <owl:disjointWith rdf:resource="&or;Duration"/>
        <owl:disjointWith rdf:resource="&or;Energy"/>
        <owl:disjointWith rdf:resource="&or;Force"/>
        <owl:disjointWith rdf:resource="&or;Mass"/>
        <owl:disjointWith rdf:resource="&or;Pressure"/>
        <owl:disjointWith rdf:resource="&or;Temperature"/>
        <owl:disjointWith rdf:resource="&or;Volume"/>
        <rdfs:comment xml:lang="en">Energy Per Mass is an amount of Energy divided by an amount of Mass.  It is used to specify the amount of energy that enters or leaves a system dependent upon the mass of the system that results in, or is caused by, some type of change.</rdfs:comment>
    </owl:Class>
    


    <!-- http://www.nist.gov/itl/ssd/Materials#EngineeredAlloy -->

    <owl:Class rdf:about="&mat;EngineeredAlloy">
        <owl:equivalentClass>
            <owl:Class>
                <owl:intersectionOf rdf:parseType="Collection">
                    <rdf:Description rdf:about="&mat;Alloy"/>
                    <rdf:Description rdf:about="&mat;EngineeredMaterial"/>
                </owl:intersectionOf>
            </owl:Class>
        </owl:equivalentClass>
        <rdfs:subClassOf rdf:resource="&mat;Alloy"/>
        <rdfs:subClassOf rdf:resource="&mat;EngineeredMaterial"/>
        <rdfs:comment xml:lang="en">An Engineered Alloy is one that has been deliberately manufactured, not one that occurs naturally.</rdfs:comment>
    </owl:Class>
    


    <!-- http://www.nist.gov/itl/ssd/Materials#EngineeredMaterial -->

    <owl:Class rdf:about="&mat;EngineeredMaterial">
        <owl:equivalentClass>
            <owl:Class>
                <owl:intersectionOf rdf:parseType="Collection">
                    <rdf:Description rdf:about="&bc;MaterialSubstance"/>
                    <rdf:Description rdf:about="&or;Artifact"/>
                </owl:intersectionOf>
            </owl:Class>
        </owl:equivalentClass>
        <rdfs:subClassOf rdf:resource="&bc;MaterialSubstance"/>
        <rdfs:subClassOf rdf:resource="&or;Artifact"/>
    </owl:Class>
    


    <!-- http://www.nist.gov/itl/ssd/Materials#Entropy -->

    <owl:Class rdf:about="&mat;Entropy">
        <rdfs:subClassOf rdf:resource="&mat;MeasurableMechanicalProperty"/>
        <rdfs:subClassOf>
            <owl:Restriction>
                <owl:onProperty rdf:resource="&or;unitTypeFor"/>
                <owl:someValuesFrom rdf:resource="&mat;UnitOfEnergyPerTemperatureDifference"/>
            </owl:Restriction>
        </rdfs:subClassOf>
        <owl:disjointWith rdf:resource="&mat;Strength"/>
        <owl:disjointWith rdf:resource="&mat;TransportProperty"/>
    </owl:Class>
    


    <!-- http://www.nist.gov/itl/ssd/Materials#Ethulose -->

    <owl:Class rdf:about="&mat;Ethulose">
        <rdfs:subClassOf rdf:resource="&mat;HydroxyalkylCelluloseEther"/>
        <owl:disjointWith rdf:resource="&mat;HydroxyethylCellulose"/>
        <owl:disjointWith rdf:resource="&mat;HydroxyethylMethylCellulose"/>
        <owl:disjointWith rdf:resource="&mat;HydroxypropylCellulose"/>
        <owl:disjointWith rdf:resource="&mat;Hypromellose"/>
        <rdfs:comment xml:lang="en">Ethulose (or ethylhydroxyethylcellulose)  is a cellulose derivative with CH2CH3 and -CH2-CH2OH groups bound to some of the hydroxyl groups of the glucopyranose monomers that make up the cellulose backbone.</rdfs:comment>
    </owl:Class>
    


    <!-- http://www.nist.gov/itl/ssd/Materials#EthylCellulose -->

    <owl:Class rdf:about="&mat;EthylCellulose">
        <rdfs:subClassOf rdf:resource="&mat;AlkylCelluloseEthers"/>
        <owl:disjointWith rdf:resource="&mat;EthylMethylCellulose"/>
        <owl:disjointWith rdf:resource="&mat;Methylcellulose"/>
        <rdfs:comment xml:lang="en">Ethyl cellulose is a derivative of cellulose in which some of the hydroxyl groups on the repeating glucose units are converted into ethyl ether groups. The number of ethyl groups can vary.</rdfs:comment>
    </owl:Class>
    


    <!-- http://www.nist.gov/itl/ssd/Materials#EthylMethylCellulose -->

    <owl:Class rdf:about="&mat;EthylMethylCellulose">
        <rdfs:subClassOf rdf:resource="&mat;AlkylCelluloseEthers"/>
        <owl:disjointWith rdf:resource="&mat;Methylcellulose"/>
        <rdfs:comment xml:lang="en">Ethyl cellulose is a derivative of cellulose in which some of the hydroxyl groups on the repeating glucose units are converted into ethyl ether groups and some into methyl ether groups. </rdfs:comment>
    </owl:Class>
    


    <!-- http://www.nist.gov/itl/ssd/Materials#EutecticAlloy -->

    <owl:Class rdf:about="&mat;EutecticAlloy">
        <rdfs:subClassOf rdf:resource="&mat;EngineeredAlloy"/>
        <rdfs:comment xml:lang="en">A Eutectic Alloy is an alloy that has a specific ratio of component metals that solidifies at a lower temperature than any other composition made up of the same ingredients.</rdfs:comment>
    </owl:Class>
    


    <!-- http://www.nist.gov/itl/ssd/Materials#EutecticTransformation -->

    <owl:Class rdf:about="&mat;EutecticTransformation">
        <rdfs:subClassOf rdf:resource="&mat;Solidification"/>
        <owl:disjointWith rdf:resource="&mat;PeritecticReaction"/>
        <owl:disjointWith rdf:resource="&mat;SublimatingToSolid"/>
        <rdfs:comment xml:lang="en">A Eutectic Transformation is a phase change in which a two component single phase liquid is cooled and transforms into two solid phases.</rdfs:comment>
    </owl:Class>
    


    <!-- http://www.nist.gov/itl/ssd/Materials#EutectoidAlloy -->

    <owl:Class rdf:about="&mat;EutectoidAlloy">
        <rdfs:subClassOf rdf:resource="&mat;EngineeredAlloy"/>
        <rdfs:comment xml:lang="en">A Eutectoid Alloy is one in which a solid phase has transformed into two different phases on cooling past the eutectoid point. </rdfs:comment>
    </owl:Class>
    


    <!-- http://www.nist.gov/itl/ssd/Materials#EutectoidPhaseTransformation -->

    <owl:Class rdf:about="&mat;EutectoidPhaseTransformation">
        <rdfs:subClassOf rdf:resource="&mat;CrystallinePhaseChange"/>
    </owl:Class>
    


    <!-- http://www.nist.gov/itl/ssd/Materials#EutectoidSteel -->

    <owl:Class rdf:about="&mat;EutectoidSteel">
        <rdfs:subClassOf rdf:resource="&mat;EutectoidAlloy"/>
    </owl:Class>
    


    <!-- http://www.nist.gov/itl/ssd/Materials#Evaporating -->

    <owl:Class rdf:about="&mat;Evaporating">
        <rdfs:subClassOf rdf:resource="&mat;Vaporization"/>
        <owl:disjointWith rdf:resource="&mat;OrderDisorderPhaseTransformation"/>
        <owl:disjointWith rdf:resource="&mat;Sublimating"/>
        <rdfs:comment xml:lang="en">Evaporating is the Phase Change from a liquid state to a gasseous state.</rdfs:comment>
    </owl:Class>
    


    <!-- http://www.nist.gov/itl/ssd/Materials#ExchangeMechanismForDiffusion -->

    <owl:Class rdf:about="&mat;ExchangeMechanismForDiffusion">
        <rdfs:subClassOf rdf:resource="&mat;MicroscopicDiffusionMovement"/>
        <owl:disjointWith rdf:resource="&mat;InterstitialcyMechanism"/>
        <owl:disjointWith rdf:resource="&mat;VacancyDiffusionMechanism"/>
        <rdfs:seeAlso xml:lang="en">Definitions of terms for diffusion in the solid state (IUPAC Recommendations 1999), Pure Appl. Chem. 71, 1307-1325.</rdfs:seeAlso>
        <rdfs:comment xml:lang="en">The Exchange mechanism for Diffusion is the atomic mechanism whereby diffusion takes place by the direct interchange of two neighbouring atoms.</rdfs:comment>
        <or:termString xml:lang="en">exchange mechanism</or:termString>
    </owl:Class>
    


    <!-- http://www.nist.gov/itl/ssd/Materials#FaceCenteredCubicCrystalStructure -->

    <owl:Class rdf:about="&mat;FaceCenteredCubicCrystalStructure">
        <rdfs:subClassOf rdf:resource="&mat;CubicCrystalStructure"/>
    </owl:Class>
    


    <!-- http://www.nist.gov/itl/ssd/Materials#FastIonicConductor -->

    <owl:Class rdf:about="&mat;FastIonicConductor">
        <rdfs:subClassOf rdf:resource="&mat;SolidSubstance"/>
        <owl:disjointWith rdf:resource="&mat;Semiconductor"/>
        <rdfs:comment xml:lang="en">A Fast Ionic Conductor (or ``fast ion conductor&#39;&#39;) is a solid material that exhibits a high ionic conductivity of the order of those found in molten salts ( Ωi &gt; 0.001 Siemen/cm). An alternate term is ``superionic conductor&#39;&#39;.</rdfs:comment>
        <rdfs:seeAlso xml:lang="en">Definitions of terms for diffusion in the solid state (IUPAC Recommendations 1999), Pure Appl. Chem. 71, 1307-1325.</rdfs:seeAlso>
    </owl:Class>
    


    <!-- http://www.nist.gov/itl/ssd/Materials#Feldspar -->

    <owl:Class rdf:about="&mat;Feldspar">
        <rdfs:subClassOf rdf:resource="&mat;Silicate"/>
        <rdfs:comment xml:lang="en">Feldspars (KAlSi3O8 – NaAlSi3O8 – CaAl2Si2O8) are a group of rock-forming tectosilicate minerals.</rdfs:comment>
        <or:termString xml:lang="en">feldspar</or:termString>
    </owl:Class>
    


    <!-- http://www.nist.gov/itl/ssd/Materials#FeldsparClay -->

    <owl:Class rdf:about="&mat;FeldsparClay">
        <rdfs:subClassOf rdf:resource="&mat;Clay"/>
        <rdfs:subClassOf>
            <owl:Restriction>
                <owl:onProperty rdf:resource="&bc;primaryConstituentType"/>
                <owl:someValuesFrom rdf:resource="&mat;Feldspar"/>
            </owl:Restriction>
        </rdfs:subClassOf>
        <or:referenceURL rdf:datatype="&xsd;anyURI">http://www.matweb.com/index.aspx</or:referenceURL>
        <or:termString xml:lang="en">feldspar clay</or:termString>
    </owl:Class>
    


    <!-- http://www.nist.gov/itl/ssd/Materials#FerriticStainlessSteel -->

    <owl:Class rdf:about="&mat;FerriticStainlessSteel">
        <rdfs:subClassOf rdf:resource="&mat;StainlessSteel"/>
        <or:referenceURL rdf:datatype="&xsd;anyURI">http://www.matweb.com/index.aspx</or:referenceURL>
        <rdfs:comment xml:lang="en">Ferritic stainless steels contain between 10.5% and 27% chromium and very little nickel, if any, but some types can contain lead. Most compositions include molybdenum; some, aluminium or titanium. Common ferritic grades include 18Cr-2Mo, 26Cr-1Mo, 29Cr-4Mo, and 29Cr-4Mo-2Ni.</rdfs:comment>
        <rdfs:comment xml:lang="en">ferritic stainless steel</rdfs:comment>
    </owl:Class>
    


    <!-- http://www.nist.gov/itl/ssd/Materials#FerrousAlloy -->

    <owl:Class rdf:about="&mat;FerrousAlloy">
        <owl:equivalentClass>
            <owl:Class>
                <owl:intersectionOf rdf:parseType="Collection">
                    <rdf:Description rdf:about="&mat;Alloy"/>
                    <owl:Restriction>
                        <owl:onProperty rdf:resource="&mat;physicalDecompositions"/>
                        <owl:someValuesFrom rdf:resource="&bc;Iron"/>
                    </owl:Restriction>
                </owl:intersectionOf>
            </owl:Class>
        </owl:equivalentClass>
        <rdfs:subClassOf rdf:resource="&mat;Alloy"/>
        <owl:disjointWith rdf:resource="&mat;NonFerrousAlloy"/>
        <or:referenceURL rdf:datatype="&xsd;anyURI">http://www.matweb.com/index.aspx</or:referenceURL>
        <rdfs:comment xml:lang="en">A Ferrous Alloy is one that contains iron.</rdfs:comment>
        <or:termString xml:lang="en">ferrous alloy</or:termString>
        <or:termString xml:lang="en">ferrous metal</or:termString>
    </owl:Class>
    


    <!-- http://www.nist.gov/itl/ssd/Materials#FiveFrequencyDiffusionModel -->

    <owl:Class rdf:about="&mat;FiveFrequencyDiffusionModel">
        <rdfs:subClassOf rdf:resource="&mat;VacancyDiffusionMechanism"/>
        <owl:disjointWith rdf:resource="&mat;RelaxationMethodForDiffusion"/>
        <rdfs:seeAlso xml:lang="en">Definitions of terms for diffusion in the solid state (IUPAC Recommendations 1999), Pure Appl. Chem. 71, 1307-1325.</rdfs:seeAlso>
        <rdfs:comment xml:lang="en">The Five-Frequency Diffusion Model is a type of movement of impurity diffusion via monovacancies in face-centred-cubic (fcc) metals or on an fcc sublattice in ionic crystals. It is assumed that the only host atom jumps that differ from jumps in the pure lattice are those made by nearest neighbours of the impurity.</rdfs:comment>
    </owl:Class>
    


    <!-- http://www.nist.gov/itl/ssd/Materials#FluidLubricant -->

    <owl:Class rdf:about="&mat;FluidLubricant">
        <rdfs:subClassOf rdf:resource="&mat;EngineeredMaterial"/>
        <rdfs:subClassOf rdf:resource="&mat;LiquidSubstance"/>
        <or:referenceURL rdf:datatype="&xsd;anyURI">http://www.matweb.com/index.aspx</or:referenceURL>
    </owl:Class>
    


    <!-- http://www.nist.gov/itl/ssd/Materials#FluidSubstance -->

    <owl:Class rdf:about="&mat;FluidSubstance">
        <rdfs:subClassOf rdf:resource="&bc;MaterialSubstance"/>
        <owl:disjointWith rdf:resource="&mat;SolidFoam"/>
        <owl:disjointWith rdf:resource="&mat;Vacuum"/>
        <rdfs:comment xml:lang="en">A Fluid is a Material Substance that continually flows under an applied shear stress. Fluids are a subset of the phases of matter and include liquids, gases, plasmas and, to some extent, granular substances and plastic solids.</rdfs:comment>
    </owl:Class>
    


    <!-- http://www.nist.gov/itl/ssd/Materials#Foam -->

    <owl:Class rdf:about="&mat;Foam">
        <rdfs:subClassOf rdf:resource="&mat;Colloid"/>
        <owl:disjointWith rdf:resource="&mat;GaseousSubstance"/>
        <owl:disjointWith rdf:resource="&mat;GelSubstance"/>
        <owl:disjointWith rdf:resource="&mat;SolidSol"/>
        <rdfs:comment xml:lang="en">A Foam is a Material Substance that is formed by trapping pockets of gas in a liquid (Liquid Foam) or solid (Solid Foam).</rdfs:comment>
    </owl:Class>
    


    <!-- http://www.nist.gov/itl/ssd/Materials#FractureStrength -->

    <owl:Class rdf:about="&mat;FractureStrength">
        <rdfs:subClassOf rdf:resource="&mat;DeformationProperty"/>
        <owl:disjointWith rdf:resource="&mat;Hardness"/>
        <owl:disjointWith rdf:resource="&mat;Stiffness"/>
        <rdfs:comment xml:lang="en">Fracture Strength,or breaking strength, is the stress at which a specimen fails via fracture</rdfs:comment>
    </owl:Class>
    


    <!-- http://www.nist.gov/itl/ssd/Materials#Fracturing -->

    <owl:Class rdf:about="&mat;Fracturing">
        <rdfs:subClassOf rdf:resource="&mat;Cracking"/>
        <rdfs:comment xml:lang="en">Fracturing is a Mechanical Process in which some solid object is cracked and separated into two, or more, pieces (at least locally) under the action of stress.</rdfs:comment>
    </owl:Class>
    


    <!-- http://www.nist.gov/itl/ssd/Materials#Freezing -->

    <owl:Class rdf:about="&mat;Freezing">
        <rdfs:subClassOf rdf:resource="&mat;Solidification"/>
        <owl:disjointWith rdf:resource="&mat;SublimatingToSolid"/>
        <rdfs:comment xml:lang="en">Freezing is the Phase Change from a liquid state to a solid state.</rdfs:comment>
    </owl:Class>
    


    <!-- http://www.nist.gov/itl/ssd/Materials#Fullerine -->

    <owl:Class rdf:about="&mat;Fullerine">
        <rdfs:subClassOf rdf:resource="&bc;Molecule"/>
        <rdfs:comment xml:lang="en">A Fullerene is a molecule composed entirely of carbon, in the form of a hollow sphere, ellipsoid or tube. Spherical fullerenes are called buckyballs. Cylindrical ones are called carbon nanotubes.</rdfs:comment>
        <or:termString xml:lang="en">fullerine</or:termString>
    </owl:Class>
    


    <!-- http://www.nist.gov/itl/ssd/Materials#FunctionalGradientMaterial -->

    <owl:Class rdf:about="&mat;FunctionalGradientMaterial">
        <rdfs:subClassOf rdf:resource="&mat;SolidSubstance"/>
    </owl:Class>
    


    <!-- http://www.nist.gov/itl/ssd/Materials#GasInLiquidSolution -->

    <owl:Class rdf:about="&mat;GasInLiquidSolution">
        <rdfs:subClassOf rdf:resource="&mat;LiquidSolution"/>
        <rdfs:subClassOf>
            <owl:Restriction>
                <owl:onProperty rdf:resource="&mat;solute"/>
                <owl:someValuesFrom rdf:resource="&mat;GaseousSubstance"/>
            </owl:Restriction>
        </rdfs:subClassOf>
        <rdfs:comment xml:lang="en">A Gas In Liquid Solution is a Chemical Solution in which the soute is gasseous and the solvent is liquid.</rdfs:comment>
    </owl:Class>
    


    <!-- http://www.nist.gov/itl/ssd/Materials#GasMixture -->

    <owl:Class rdf:about="&mat;GasMixture">
        <rdfs:subClassOf rdf:resource="&mat;GaseousSubstance"/>
        <rdfs:subClassOf rdf:resource="&mat;PhysicalMixture"/>
        <rdfs:comment xml:lang="en">A Gas Mixture is a  Physical Mixture of gasses.  Some definitions of the word &#39;solution&#39; subsume gas mixtures.</rdfs:comment>
    </owl:Class>
    


    <!-- http://www.nist.gov/itl/ssd/Materials#GaseousSubstance -->

    <owl:Class rdf:about="&mat;GaseousSubstance">
        <rdfs:subClassOf rdf:resource="&mat;FluidSubstance"/>
        <owl:disjointWith rdf:resource="&mat;GelSubstance"/>
        <owl:disjointWith rdf:resource="&mat;LiquidFoam"/>
        <owl:disjointWith rdf:resource="&mat;LiquidSubstance"/>
        <owl:disjointWith rdf:resource="&mat;PasteSubstance"/>
        <owl:disjointWith rdf:resource="&mat;SolidSubstance"/>
        <rdfs:comment xml:lang="en">Material in a gasseous phase.</rdfs:comment>
    </owl:Class>
    


    <!-- http://www.nist.gov/itl/ssd/Materials#GasseousDiffusion -->

    <owl:Class rdf:about="&mat;GasseousDiffusion">
        <rdfs:subClassOf rdf:resource="&mat;Diffusion"/>
    </owl:Class>
    


    <!-- http://www.nist.gov/itl/ssd/Materials#GelSubstance -->

    <owl:Class rdf:about="&mat;GelSubstance">
        <rdfs:subClassOf rdf:resource="&mat;AmorphousSubstance"/>
        <rdfs:subClassOf rdf:resource="&mat;Colloid"/>
        <rdfs:subClassOf rdf:resource="&mat;ComplexFluid"/>
        <owl:disjointWith rdf:resource="&mat;GlassyMaterial"/>
        <owl:disjointWith rdf:resource="&mat;PasteSubstance"/>
        <owl:disjointWith rdf:resource="&mat;PowderySubstance"/>
        <rdfs:comment xml:lang="en">Material in a gel phase.</rdfs:comment>
    </owl:Class>
    


    <!-- http://www.nist.gov/itl/ssd/Materials#GenericThermodynamicModel -->

    <owl:Class rdf:about="&mat;GenericThermodynamicModel">
        <owl:equivalentClass>
            <owl:Class>
                <owl:intersectionOf rdf:parseType="Collection">
                    <rdf:Description rdf:about="&doc;GenericScientificModel"/>
                    <rdf:Description rdf:about="&mat;ThermodynamicModel"/>
                </owl:intersectionOf>
            </owl:Class>
        </owl:equivalentClass>
        <rdfs:subClassOf rdf:resource="&doc;GenericScientificModel"/>
        <rdfs:subClassOf rdf:resource="&mat;ThermodynamicModel"/>
        <rdfs:comment xml:lang="en">A Generic Thermodynamic Model is a scientific System Model (law, principle, or theory) of how thermodynamic systems act in given types of circumstances.</rdfs:comment>
    </owl:Class>
    


    <!-- http://www.nist.gov/itl/ssd/Materials#GlassCeramic -->

    <owl:Class rdf:about="&mat;GlassCeramic">
        <rdfs:subClassOf rdf:resource="&mat;Ceramic"/>
        <rdfs:subClassOf rdf:resource="&mat;EngineeredMaterial"/>
        <rdfs:subClassOf rdf:resource="&mat;PolycrystallineMaterial"/>
        <or:referenceURL rdf:datatype="&xsd;anyURI">http://www.matweb.com/index.aspx</or:referenceURL>
        <rdfs:comment xml:lang="en">Glass-ceramics are polycrystalline material produced through controlled crystallization of base glass. Glass-ceramic materials share many properties with both glasses and ceramics. Glass-ceramics have an amorphous phase and one or more crystalline phases and are produced by a so called &#39;controlled crystallization&#39;.</rdfs:comment>
        <or:termString xml:lang="en">glass ceramic</or:termString>
        <or:termString xml:lang="en">glass-ceramic</or:termString>
    </owl:Class>
    


    <!-- http://www.nist.gov/itl/ssd/Materials#GlassyMaterial -->

    <owl:Class rdf:about="&mat;GlassyMaterial">
        <rdfs:subClassOf rdf:resource="&mat;AmorphousSubstance"/>
        <or:referenceURL rdf:datatype="&xsd;anyURI">http://www.matweb.com/index.aspx</or:referenceURL>
        <rdfs:comment xml:lang="en">A glassy material is a manufactured or natural glass, e.g. obsidian.</rdfs:comment>
        <or:termString xml:lang="en">glass</or:termString>
    </owl:Class>
    


    <!-- http://www.nist.gov/itl/ssd/Materials#GorskiEffect -->

    <owl:Class rdf:about="&mat;GorskiEffect">
        <rdfs:subClassOf rdf:resource="&mat;SolidDiffusion"/>
        <rdfs:seeAlso xml:lang="en">Definitions of terms for diffusion in the solid state (IUPAC Recommendations 1999), Pure Appl. Chem. 71, 1307-1325.</rdfs:seeAlso>
        <rdfs:comment xml:lang="en">The Gorski Effect is the migration of atoms in an elastically deformed material. The effect is particularly observed for solute atoms with a strong size effect and high diffusivity in a matrix, for instance hydrogen atoms in a metal.</rdfs:comment>
    </owl:Class>
    


    <!-- http://www.nist.gov/itl/ssd/Materials#GrainBoundaryDiffusion -->

    <owl:Class rdf:about="&mat;GrainBoundaryDiffusion">
        <rdfs:subClassOf rdf:resource="&mat;ShortCircuitDiffusion"/>
        <rdfs:seeAlso xml:lang="en">Definitions of terms for diffusion in the solid state (IUPAC Recommendations 1999), Pure Appl. Chem. 71, 1307-1325.</rdfs:seeAlso>
        <rdfs:comment xml:lang="en">Grain Boundary Diffusion is diffusion which takes place along a grain boundary.</rdfs:comment>
    </owl:Class>
    


    <!-- http://www.nist.gov/itl/ssd/Materials#Graphite -->

    <owl:Class rdf:about="&mat;Graphite">
        <rdfs:subClassOf rdf:resource="&bc;Carbon"/>
        <rdfs:subClassOf rdf:resource="&mat;SolidCrystallineSubstance"/>
        <or:referenceURL rdf:datatype="&xsd;anyURI">http://www.matweb.com/index.aspx</or:referenceURL>
        <or:termString xml:lang="en">graphite</or:termString>
    </owl:Class>
    


    <!-- http://www.nist.gov/itl/ssd/Materials#GrayCastIron -->

    <owl:Class rdf:about="&mat;GrayCastIron">
        <rdfs:subClassOf rdf:resource="&mat;CastIron"/>
        <owl:disjointWith rdf:resource="&mat;MalleableIron"/>
        <owl:disjointWith rdf:resource="&mat;WhiteCastIron"/>
        <or:referenceURL rdf:datatype="&xsd;anyURI">http://www.matweb.com/index.aspx</or:referenceURL>
        <rdfs:comment xml:lang="en">Gray (cast) iron, or grey (cast) iron, is a type of cast iron that has a graphitic microstructure. It is named after the gray color of the fracture it forms, which is due to the presence of graphite</rdfs:comment>
        <or:termString xml:lang="en">gray cast iron</or:termString>
        <or:termString xml:lang="en">gray iron</or:termString>
        <or:termString xml:lang="en">grey cast iron</or:termString>
        <or:termString xml:lang="en">grey iron</or:termString>
    </owl:Class>
    


    <!-- http://www.nist.gov/itl/ssd/Materials#Halide -->

    <owl:Class rdf:about="&mat;Halide">
        <rdfs:subClassOf rdf:resource="&mat;PureSubstance"/>
        <or:referenceURL rdf:datatype="&xsd;anyURI">http://www.matweb.com/index.aspx</or:referenceURL>
        <rdfs:comment xml:lang="en">A Halide is a binary compound, of which one part is a halogen atom and the other part is an element or radical that is less electronegative (or more electropositive) than the halogen, to make a fluoride, chloride, bromide, iodide, or astatide compound. Many salts are halides.</rdfs:comment>
        <or:termString xml:lang="en">halide</or:termString>
    </owl:Class>
    


    <!-- http://www.nist.gov/itl/ssd/Materials#HalideMineral -->

    <owl:Class rdf:about="&mat;HalideMineral">
        <rdfs:subClassOf rdf:resource="&mat;Mineral"/>
    </owl:Class>
    


    <!-- http://www.nist.gov/itl/ssd/Materials#Hardness -->

    <owl:Class rdf:about="&mat;Hardness">
        <rdfs:subClassOf rdf:resource="&mat;DeformationProperty"/>
        <owl:disjointWith rdf:resource="&mat;Stiffness"/>
    </owl:Class>
    


    <!-- http://www.nist.gov/itl/ssd/Materials#Hardwood -->

    <owl:Class rdf:about="&mat;Hardwood">
        <rdfs:subClassOf rdf:resource="&mat;Wood"/>
        <or:referenceURL rdf:datatype="&xsd;anyURI">http://www.matweb.com/index.aspx</or:referenceURL>
        <or:termString xml:lang="en">hardwood</or:termString>
    </owl:Class>
    


    <!-- http://www.nist.gov/itl/ssd/Materials#Hastelloy -->

    <owl:Class rdf:about="&mat;Hastelloy">
        <rdfs:subClassOf rdf:resource="&mat;NickelAlloy"/>
        <rdfs:subClassOf rdf:resource="&mat;Superalloy"/>
        <owl:disjointWith rdf:resource="&mat;Waspaloy"/>
        <rdfs:comment xml:lang="en">Hastelloys are Nickel-based Superalloys produced by Haynes International, Inc.  &quot;Hastelloy&quot; is a trademarked name for more than 10 different alloys, which are further distinguished with alphanumeric designations.</rdfs:comment>
    </owl:Class>
    


    <!-- http://www.nist.gov/itl/ssd/Materials#HeatResistingSteel -->

    <owl:Class rdf:about="&mat;HeatResistingSteel">
        <rdfs:subClassOf rdf:resource="&mat;Steel"/>
        <or:referenceURL rdf:datatype="&xsd;anyURI">http://www.matweb.com/index.aspx</or:referenceURL>
    </owl:Class>
    


    <!-- http://www.nist.gov/itl/ssd/Materials#HeatingCoolingCurve -->

    <owl:Class rdf:about="&mat;HeatingCoolingCurve">
        <rdfs:subClassOf rdf:resource="&or;Curve"/>
        <or:referenceURL rdf:datatype="&xsd;anyURI">http://www.iupac.org/namespaces/ThermoML</or:referenceURL>
        <or:termString xml:lang="en">A heating or cooling curve graphs the temperature of a substance being heated or cooled vs. either time or the amount of heat added/removed from the system.  Such curves often span phase transitions.</or:termString>
        <or:termString xml:lang="en">heating or cooling curve</or:termString>
        <or:termString xml:lang="en">heating/cooling curve</or:termString>
    </owl:Class>
    


    <!-- http://www.nist.gov/itl/ssd/Materials#HeatingCurve -->

    <owl:Class rdf:about="&mat;HeatingCurve">
        <rdfs:subClassOf rdf:resource="&mat;HeatingCoolingCurve"/>
        <or:termString xml:lang="en">heating curve</or:termString>
    </owl:Class>
    


    <!-- http://www.nist.gov/itl/ssd/Materials#HeatingProcess -->

    <owl:Class rdf:about="&mat;HeatingProcess">
        <rdfs:subClassOf rdf:resource="&mat;TemperatureChangeProcess"/>
        <rdfs:comment xml:lang="en">A Heating Process is a Temperature Change Process during which the temperature of an object increases.  This could be due to internal  generation of heat, external heat warming the object, or both. </rdfs:comment>
    </owl:Class>
    


    <!-- http://www.nist.gov/itl/ssd/Materials#Heterodiffusion -->

    <owl:Class rdf:about="&mat;Heterodiffusion">
        <rdfs:subClassOf rdf:resource="&mat;SolidDiffusion"/>
        <owl:disjointWith rdf:resource="&mat;SelfDiffusion"/>
        <rdfs:seeAlso>Definitions of terms for diffusion in the solid state (IUPAC Recommendations 1999), Pure Appl. Chem. 71, 1307-1325.</rdfs:seeAlso>
        <rdfs:seeAlso xml:lang="en">Heterodiffusion is the diffusion of foreign atoms in a material.  Also called ``imurity diffusion&#39;&#39; or ``solute diffusion&#39;&#39;.</rdfs:seeAlso>
    </owl:Class>
    


    <!-- http://www.nist.gov/itl/ssd/Materials#HexagonalClosePackedCrystalStructure -->

    <owl:Class rdf:about="&mat;HexagonalClosePackedCrystalStructure">
        <rdfs:subClassOf rdf:resource="&mat;HexagonalCrystalStructure"/>
    </owl:Class>
    


    <!-- http://www.nist.gov/itl/ssd/Materials#HexagonalCrystalStructure -->

    <owl:Class rdf:about="&mat;HexagonalCrystalStructure">
        <rdfs:subClassOf rdf:resource="&mat;TrigonalCrystalStructure"/>
        <owl:disjointWith rdf:resource="&mat;RhombohedralCrystalStructure"/>
        <rdfs:comment xml:lang="en">the hexagonal crystal system is one of the 7 crystal systems, the hexagonal lattice system is one of the 7 lattice systems, and the hexagonal crystal family is one of the 6 crystal families. They are closely related and often confused with each other, but they are not the same. The hexagonal lattice system consists of just one Bravais lattice type: the hexagonal one. The hexagonal crystal system consists of the 7 point groups such that all their space groups have the hexagonal lattice as underlying lattice. The hexagonal crystal family consists of the 12 point groups such that at least one of their space groups has the hexagonal lattice as underlying lattice, and is the union of the hexagonal crystal system and the trigonal crystal system.</rdfs:comment>
    </owl:Class>
    


    <!-- http://www.nist.gov/itl/ssd/Materials#HighCarbonSteel -->

    <owl:Class rdf:about="&mat;HighCarbonSteel">
        <rdfs:subClassOf rdf:resource="&mat;CarbonSteel"/>
        <owl:disjointWith rdf:resource="&mat;LowCarbonSteel"/>
        <owl:disjointWith rdf:resource="&mat;MediumCarbonSteel"/>
        <or:referenceURL rdf:datatype="&xsd;anyURI">http://www.matweb.com/index.aspx</or:referenceURL>
        <or:termString xml:lang="en">high carbon steel</or:termString>
    </owl:Class>
    


    <!-- http://www.nist.gov/itl/ssd/Materials#HighSpeedSteel -->

    <owl:Class rdf:about="&mat;HighSpeedSteel">
        <rdfs:subClassOf rdf:resource="&mat;ToolSteel"/>
        <rdfs:comment xml:lang="en">High speed steel (HSS or HS) is a subset of tool steels, commonly used in cutting tools. It is superior to the older high carbon steel tools in that it can withstand higher temperatures without losing its temper. This property allows HSS to cut faster than high carbon steel, hence the name high speed steel. At room temperature, in their generally recommended heat treatment, HSS grades generally display high hardness (above HRC60) and a high abrasion resistance (generally linked to vanadium content often used in HSS) compared to common carbon and tool steels.</rdfs:comment>
    </owl:Class>
    


    <!-- http://www.nist.gov/itl/ssd/Materials#HighStrengthSteel -->

    <owl:Class rdf:about="&mat;HighStrengthSteel">
        <rdfs:subClassOf rdf:resource="&mat;LowAlloySteel"/>
        <or:termString xml:lang="en">HSLA</or:termString>
        <rdfs:comment xml:lang="en">High-strength low-alloy steel (HSLA) is a type of alloy steel that provides better mechanical properties or greater resistance to corrosion than carbon steel.  HSLA steels vary from other steels in that they are not made to meet a specific chemical composition but rather to specific mechanical properties. They have a carbon content between 0.05–0.25% to retain formability and weldability. Other alloying elements include up to 2.0% manganese and small quantities of copper, nickel, niobium, nitrogen, vanadium, chromium, molybdenum, titanium, calcium, rare earth elements, or zirconium. Copper, titanium, vanadium, and niobium are added for strengthening purposes.</rdfs:comment>
        <or:termString xml:lang="en">high-strength low alloy steel</or:termString>
        <or:termString xml:lang="en">high-strength steel</or:termString>
    </owl:Class>
    


    <!-- http://www.nist.gov/itl/ssd/Materials#HydroxyalkylCelluloseEther -->

    <owl:Class rdf:about="&mat;HydroxyalkylCelluloseEther">
        <rdfs:subClassOf rdf:resource="&mat;CelluloseEther"/>
    </owl:Class>
    


    <!-- http://www.nist.gov/itl/ssd/Materials#HydroxyethylCellulose -->

    <owl:Class rdf:about="&mat;HydroxyethylCellulose">
        <rdfs:subClassOf rdf:resource="&mat;HydroxyalkylCelluloseEther"/>
        <owl:disjointWith rdf:resource="&mat;HydroxypropylCellulose"/>
        <owl:disjointWith rdf:resource="&mat;Hypromellose"/>
        <rdfs:comment xml:lang="en">Hydroxymethyl cellulose is a cellulose derivative with carboxymethyl groups (-CH2-CH2-OH) bound to some of the hydroxyl groups of the glucopyranose monomers that make up the cellulose backbone.</rdfs:comment>
    </owl:Class>
    


    <!-- http://www.nist.gov/itl/ssd/Materials#HydroxyethylMethylCellulose -->

    <owl:Class rdf:about="&mat;HydroxyethylMethylCellulose">
        <rdfs:subClassOf rdf:resource="&mat;HydroxyalkylCelluloseEther"/>
        <owl:disjointWith rdf:resource="&mat;Hypromellose"/>
        <rdfs:comment xml:lang="en">Hydroxy ethyl methyl cellulose (HPC) is an ether of cellulose in which some of the hydroxyl groups in the repeating glucose units have been replaced with -CH3 or -CH2CH2OH.  The percentage of hydroxyl groups substituted can vary.</rdfs:comment>
    </owl:Class>
    


    <!-- http://www.nist.gov/itl/ssd/Materials#HydroxypropylCellulose -->

    <owl:Class rdf:about="&mat;HydroxypropylCellulose">
        <rdfs:subClassOf rdf:resource="&mat;HydroxyalkylCelluloseEther"/>
        <owl:disjointWith rdf:resource="&mat;Hypromellose"/>
        <rdfs:comment xml:lang="en">Hydroxypropyl cellulose (HPC) is an ether of cellulose in which some of the hydroxyl groups in the repeating glucose units have been hydroxypropylated forming -OCH2CH(OH)CH3 groups using propylene oxide.  The percentage of hydroxyl groups substituted can vary.</rdfs:comment>
    </owl:Class>
    


    <!-- http://www.nist.gov/itl/ssd/Materials#Hypromellose -->

    <owl:Class rdf:about="&mat;Hypromellose">
        <rdfs:subClassOf rdf:resource="&mat;HydroxyalkylCelluloseEther"/>
        <rdfs:comment xml:lang="en">Hypromellose (INN), short for hydroxypropyl methylcellulose (HPMC), is a cellulose derivative with CH3 and -CH2-CH(OH)CH3 groups bound to some of the hydroxyl groups of the glucopyranose monomers that make up the cellulose backbone.</rdfs:comment>
    </owl:Class>
    


    <!-- http://www.nist.gov/itl/ssd/Materials#IndentationHardness -->

    <owl:Class rdf:about="&mat;IndentationHardness">
        <rdfs:subClassOf rdf:resource="&mat;Hardness"/>
        <rdfs:comment xml:lang="en">Indentation Hardness measures the resistance of a sample to permanent plastic deformation due to a constant compression load.  Scales used (depending upon the hardness of the material) are Vickers, Shore, Rockwell, and Brinell.</rdfs:comment>
    </owl:Class>
    


    <!-- http://www.nist.gov/itl/ssd/Materials#IndiumAlloy -->

    <owl:Class rdf:about="&mat;IndiumAlloy">
        <rdfs:subClassOf rdf:resource="&mat;NonFerrousAlloy"/>
        <rdfs:subClassOf>
            <owl:Restriction>
                <owl:onProperty rdf:resource="&mat;physicalDecompositions"/>
                <owl:someValuesFrom rdf:resource="&bc;Indium"/>
            </owl:Restriction>
        </rdfs:subClassOf>
        <or:referenceURL rdf:datatype="&xsd;anyURI">http://www.matweb.com/index.aspx</or:referenceURL>
    </owl:Class>
    


    <!-- http://www.nist.gov/itl/ssd/Materials#InterchangeDiffusion -->

    <owl:Class rdf:about="&mat;InterchangeDiffusion">
        <rdfs:subClassOf rdf:resource="&mat;Heterodiffusion"/>
        <rdfs:seeAlso xml:lang="en">Definitions of terms for diffusion in the solid state (IUPAC Recommendations 1999), Pure Appl. Chem. 71, 1307-1325.</rdfs:seeAlso>
        <rdfs:comment xml:lang="en">Interchange Diffusion is diffusion in which foreign atoms predominately present at interstitital lattice sites migrate via normal sites.</rdfs:comment>
    </owl:Class>
    


    <!-- http://www.nist.gov/itl/ssd/Materials#InterstitialDiffusion -->

    <owl:Class rdf:about="&mat;InterstitialDiffusion">
        <rdfs:subClassOf rdf:resource="&mat;LatticeDiffusion"/>
        <owl:disjointWith rdf:resource="&mat;VacancyWindEffect"/>
        <rdfs:seeAlso xml:lang="en">Definitions of terms for diffusion in the solid state (IUPAC Recommendations 1999), Pure Appl. Chem. 71, 1307-1325.</rdfs:seeAlso>
        <rdfs:comment xml:lang="en">Interstitial Diffusion is diffusion that takes place via interstitial sites.</rdfs:comment>
        <or:termString xml:lang="en">interstitial diffusion</or:termString>
    </owl:Class>
    


    <!-- http://www.nist.gov/itl/ssd/Materials#InterstitialcyMechanism -->

    <owl:Class rdf:about="&mat;InterstitialcyMechanism">
        <rdfs:subClassOf rdf:resource="&mat;MicroscopicDiffusionMovement"/>
        <owl:disjointWith rdf:resource="&mat;VacancyDiffusionMechanism"/>
        <rdfs:comment xml:lang="en">A Interstitialcy Mechanism is a mechanism where migration of atoms in diffusion  occurs by an interstitial atom moving onto a normal lattice site whilst simultaneously the original lattice atom moves into an interstitial position.</rdfs:comment>
        <rdfs:seeAlso>Definitions of terms for diffusion in the solid state (IUPAC Recommendations 1999), Pure Appl. Chem. 71, 1307-1325.</rdfs:seeAlso>
        <or:termString xml:lang="en">interstitialcy mechanism</or:termString>
    </owl:Class>
    


    <!-- http://www.nist.gov/itl/ssd/Materials#IonicLiquid -->

    <owl:Class rdf:about="&mat;IonicLiquid">
        <rdfs:subClassOf rdf:resource="&mat;LiquidSubstance"/>
        <rdfs:comment xml:lang="en">An ionic liquid is a salt in the liquid state.</rdfs:comment>
    </owl:Class>
    


    <!-- http://www.nist.gov/itl/ssd/Materials#IonicLiquidSolution -->

    <owl:Class rdf:about="&mat;IonicLiquidSolution">
        <owl:equivalentClass>
            <owl:Class>
                <owl:intersectionOf rdf:parseType="Collection">
                    <rdf:Description rdf:about="&mat;IonicLiquid"/>
                    <rdf:Description rdf:about="&mat;LiquidSolution"/>
                </owl:intersectionOf>
            </owl:Class>
        </owl:equivalentClass>
        <rdfs:subClassOf rdf:resource="&mat;LiquidSolution"/>
        <owl:disjointWith rdf:resource="&mat;NonIonicOrAqueousLiquidSolution"/>
    </owl:Class>
    


    <!-- http://www.nist.gov/itl/ssd/Materials#KaolinClay -->

    <owl:Class rdf:about="&mat;KaolinClay">
        <rdfs:subClassOf rdf:resource="&mat;Clay"/>
        <or:referenceURL rdf:datatype="&xsd;anyURI">http://www.matweb.com/index.aspx</or:referenceURL>
        <or:termString xml:lang="en">kaolin clay</or:termString>
    </owl:Class>
    


    <!-- http://www.nist.gov/itl/ssd/Materials#KirkendallEffect -->

    <owl:Class rdf:about="&mat;KirkendallEffect">
        <rdfs:subClassOf rdf:resource="&mat;Heterodiffusion"/>
        <rdfs:seeAlso xml:lang="en">Definitions of terms for diffusion in the solid state (IUPAC Recommendations 1999), Pure Appl. Chem. 71, 1307-1325.</rdfs:seeAlso>
        <rdfs:comment xml:lang="en">The Kirkendall Effect occurs during interdiffusion between specimens in a diffusion couple when the intrinsic diffusion coefficients of the components are different. The greater flux of atoms in one direction over the other direction causes the original interface, called the Kirkendall plane, to be displaced by a distance called the Kirkendall shift. This shift can be observed by the movement of inert markers.</rdfs:comment>
    </owl:Class>
    


    <!-- http://www.nist.gov/itl/ssd/Materials#KirkendallPlane -->

    <owl:Class rdf:about="&mat;KirkendallPlane">
        <rdfs:subClassOf rdf:resource="&or;PlanarRegion"/>
        <owl:disjointWith rdf:resource="&mat;MatanoPlane"/>
        <rdfs:seeAlso>Definitions of terms for diffusion in the solid state (IUPAC Recommendations 1999), Pure Appl. Chem. 71, 1307-1325.</rdfs:seeAlso>
        <or:termString xml:lang="en">Kirkendall plane</or:termString>
        <rdfs:comment xml:lang="en">The Kirkendall effect occurs during interdiffusion between specimens in a diffusion couple when the intrinsic diffusion coefficients of the components are different. The greater flux of atoms in one direction over the other direction causes the original interface, called the Kirkendall plane, to be displaced by a distance called the Kirkendall shift. This shift can be observed by the movement of inert markers.</rdfs:comment>
    </owl:Class>
    


    <!-- http://www.nist.gov/itl/ssd/Materials#LaboratoryFrameOfReference -->

    <owl:Class rdf:about="&mat;LaboratoryFrameOfReference">
        <rdfs:subClassOf rdf:resource="&or;SpatialFrameOfReference"/>
        <or:termString xml:lang="en">laboratory frame of reference</or:termString>
    </owl:Class>
    


    <!-- http://www.nist.gov/itl/ssd/Materials#LaboratoryFrameOfReferenceForDiffusion -->

    <owl:Class rdf:about="&mat;LaboratoryFrameOfReferenceForDiffusion">
        <rdfs:subClassOf rdf:resource="&mat;LaboratoryFrameOfReference"/>
        <rdfs:seeAlso>Definitions of terms for diffusion in the solid state (IUPAC Recommendations 1999), Pure Appl. Chem. 71, 1307-1325.</rdfs:seeAlso>
        <rdfs:comment xml:lang="en">In binary diffusion the fluxes JA and JB of species A and B generally will be different. A frame of reference defined by the condition J=JB=0 is called the laboratory frame. A convenient laboratory frame is the end of the specimen since at the ends JA=JB=0, so that the condition JA=JB=0 is always fulfilled. The Matano plane is an example of a laboratory frame.</rdfs:comment>
        <or:termString xml:lang="en">laboratory frame</or:termString>
    </owl:Class>
    


    <!-- http://www.nist.gov/itl/ssd/Materials#LatticeDiffusion -->

    <owl:Class rdf:about="&mat;LatticeDiffusion">
        <rdfs:subClassOf rdf:resource="&mat;SolidDiffusion"/>
        <owl:disjointWith rdf:resource="&mat;ShortCircuitDiffusion"/>
        <owl:disjointWith rdf:resource="&mat;SurfaceDiffusion"/>
        <rdfs:seeAlso xml:lang="en">Definitions of terms for diffusion in the solid state (IUPAC Recommendations 1999), Pure Appl. Chem. 71, 1307-1325.</rdfs:seeAlso>
        <rdfs:comment xml:lang="en">Lattice diffusion is a diffusion process which takes place through the bulk lattice of the crystal and excludes such mechanisms as Short Circuit Diffusion along dislocations, Grain Boundary Diffusion, and Surface Diffusion.  Also called ``bulk diffusion&#39;&#39; or ``volume diffusion&#39;&#39;.</rdfs:comment>
        <or:termString xml:lang="en">lattice diffusion</or:termString>
    </owl:Class>
    


    <!-- http://www.nist.gov/itl/ssd/Materials#LatticeDistortivePhaseTransformation -->

    <owl:Class rdf:about="&mat;LatticeDistortivePhaseTransformation">
        <rdfs:subClassOf rdf:resource="&mat;DiffusionlessPhaseTransformation"/>
        <owl:disjointWith rdf:resource="&mat;ShufflePhaseTransformation"/>
        <rdfs:comment xml:lang="en">Homogeneous lattice-distortive phase transformations are transformations from one Bravais lattice into a different one.</rdfs:comment>
    </owl:Class>
    


    <!-- http://www.nist.gov/itl/ssd/Materials#LatticeFixedFrame -->

    <owl:Class rdf:about="&mat;LatticeFixedFrame">
        <rdfs:subClassOf rdf:resource="&or;SpatialFrameOfReference"/>
        <rdfs:seeAlso xml:lang="en">Definitions of terms for diffusion in the solid state (IUPAC Recommendations 1999), Pure Appl. Chem. 71, 1307-1325.</rdfs:seeAlso>
        <or:termString xml:lang="en">Kirkendall frame</or:termString>
        <rdfs:comment xml:lang="en">The Lattice Fixed Frame is used when the diffusion flux gives rise to a net flux of material. The lattice fixed frame, also called inert-marker or Kirkendall frame, moves with the local flux of the material. The
Kirkendall plane is an example of a lattice fixed frame. The frame is in the general case not connected to an average velocity of the constituents, but to the velocity of the markers.</rdfs:comment>
        <or:termString xml:lang="en">inert marker frame</or:termString>
        <or:termString xml:lang="en">lattice fixed frame</or:termString>
    </owl:Class>
    


    <!-- http://www.nist.gov/itl/ssd/Materials#LavesPhase -->

    <owl:Class rdf:about="&mat;LavesPhase">
        <rdfs:subClassOf rdf:resource="&mat;ThermodynamicPhase"/>
        <rdfs:comment xml:lang="en">Laves phases are intermetallic phases that have composition AB2.  In general, the A atoms are ordered as in diamond, hexagonal diamond, or a related structure, and the B atoms form tetrahedra around the A atoms for the AB2 structure.  There are three different classification classes: cubic, hexagonal MgZn2, and hexagonal MgNi2. </rdfs:comment>
    </owl:Class>
    


    <!-- http://www.nist.gov/itl/ssd/Materials#LawOfThermodynamics -->

    <owl:Class rdf:about="&mat;LawOfThermodynamics">
        <rdfs:subClassOf rdf:resource="&mat;GenericThermodynamicModel"/>
        <rdfs:comment xml:lang="en">The four laws of thermodynamics define fundamental physical quantities (temperature, energy, and entropy) that characterize thermodynamic systems. The laws describe how these quantities behave under various circumstances, and forbid certain phenomena (such as perpetual motion).</rdfs:comment>
        <or:termString xml:lang="en">law of thermodynamics</or:termString>
    </owl:Class>
    


    <!-- http://www.nist.gov/itl/ssd/Materials#LeadAlloy -->

    <owl:Class rdf:about="&mat;LeadAlloy">
        <rdfs:subClassOf rdf:resource="&mat;NonFerrousAlloy"/>
        <rdfs:subClassOf>
            <owl:Restriction>
                <owl:onProperty rdf:resource="&mat;physicalDecompositions"/>
                <owl:someValuesFrom rdf:resource="&bc;Lead"/>
            </owl:Restriction>
        </rdfs:subClassOf>
        <or:referenceURL rdf:datatype="&xsd;anyURI">http://www.matweb.com/index.aspx</or:referenceURL>
        <rdfs:comment xml:lang="en">An alloy that contains Lead but not Iron.</rdfs:comment>
    </owl:Class>
    


    <!-- http://www.nist.gov/itl/ssd/Materials#LiquidAerosol -->

    <owl:Class rdf:about="&mat;LiquidAerosol">
        <rdfs:subClassOf rdf:resource="&mat;Aerosol"/>
        <owl:disjointWith rdf:resource="&mat;SolidAerosol"/>
        <rdfs:comment xml:lang="en">A Liquid Aerosol is a colloid suspension of liquid droplets in a gas.</rdfs:comment>
    </owl:Class>
    


    <!-- http://www.nist.gov/itl/ssd/Materials#LiquidCrystallineSubstance -->

    <owl:Class rdf:about="&mat;LiquidCrystallineSubstance">
        <rdfs:subClassOf rdf:resource="&mat;CrystallineSubstance"/>
        <owl:disjointWith rdf:resource="&mat;SolidCrystallineSubstance"/>
    </owl:Class>
    


    <!-- http://www.nist.gov/itl/ssd/Materials#LiquidDiffusion -->

    <owl:Class rdf:about="&mat;LiquidDiffusion">
        <rdfs:subClassOf rdf:resource="&mat;Diffusion"/>
    </owl:Class>
    


    <!-- http://www.nist.gov/itl/ssd/Materials#LiquidFoam -->

    <owl:Class rdf:about="&mat;LiquidFoam">
        <rdfs:subClassOf rdf:resource="&mat;ComplexFluid"/>
        <rdfs:subClassOf rdf:resource="&mat;Foam"/>
        <rdfs:comment xml:lang="en">A Liqulid Foam is a substance that is formed by trapping pockets of gas within liquid membranes.</rdfs:comment>
    </owl:Class>
    


    <!-- http://www.nist.gov/itl/ssd/Materials#LiquidInLiquidSolution -->

    <owl:Class rdf:about="&mat;LiquidInLiquidSolution">
        <rdfs:subClassOf rdf:resource="&mat;LiquidSolution"/>
        <rdfs:subClassOf>
            <owl:Restriction>
                <owl:onProperty rdf:resource="&mat;solute"/>
                <owl:someValuesFrom rdf:resource="&mat;LiquidSubstance"/>
            </owl:Restriction>
        </rdfs:subClassOf>
        <rdfs:comment xml:lang="en">A Liquid In Liquid Solution is a Chemical Solution in which the soute and solvent are both liquid.</rdfs:comment>
    </owl:Class>
    


    <!-- http://www.nist.gov/itl/ssd/Materials#LiquidSlag -->

    <owl:Class rdf:about="&mat;LiquidSlag">
        <rdfs:subClassOf rdf:resource="&mat;EngineeredMaterial"/>
        <rdfs:subClassOf rdf:resource="&mat;LiquidSubstance"/>
        <rdfs:subClassOf rdf:resource="&mat;PhysicalMixture"/>
        <rdfs:comment xml:lang="en">Liquid Slag is formed during steel production, floating on top of the liquid steel.</rdfs:comment>
    </owl:Class>
    


    <!-- http://www.nist.gov/itl/ssd/Materials#LiquidSolution -->

    <owl:Class rdf:about="&mat;LiquidSolution">
        <rdfs:subClassOf rdf:resource="&mat;ChemicalSolution"/>
        <rdfs:subClassOf rdf:resource="&mat;LiquidSubstance"/>
        <rdfs:subClassOf>
            <owl:Restriction>
                <owl:onProperty rdf:resource="&mat;solvent"/>
                <owl:onClass rdf:resource="&mat;LiquidSubstance"/>
                <owl:qualifiedCardinality rdf:datatype="&xsd;nonNegativeInteger">1</owl:qualifiedCardinality>
            </owl:Restriction>
        </rdfs:subClassOf>
        <rdfs:comment xml:lang="en">A Liquid Solution is a Chemical Solution in which both the solvent and the solution itself are liquids.  The solute may be solid, liquid, or gas.</rdfs:comment>
    </owl:Class>
    


    <!-- http://www.nist.gov/itl/ssd/Materials#LiquidSubstance -->

    <owl:Class rdf:about="&mat;LiquidSubstance">
        <rdfs:subClassOf rdf:resource="&mat;FluidSubstance"/>
        <owl:disjointWith rdf:resource="&mat;SolidSubstance"/>
        <rdfs:comment xml:lang="en">Material in a liquid phase.</rdfs:comment>
    </owl:Class>
    


    <!-- http://www.nist.gov/itl/ssd/Materials#Liquidus -->

    <owl:Class rdf:about="&mat;Liquidus">
        <rdfs:subClassOf rdf:resource="&or;CurveSegment"/>
        <rdfs:comment xml:lang="en">A Liquidus is a Curve on a temperature-concentration Phase Diagram above which a given substance is completely liquid.  Between the Liquidus and the Solidus, the substance is a mixture of solid and liquid phases.</rdfs:comment>
    </owl:Class>
    


    <!-- http://www.nist.gov/itl/ssd/Materials#LithiumGellant -->

    <owl:Class rdf:about="&mat;LithiumGellant">
        <rdfs:subClassOf rdf:resource="&mat;FluidLubricant"/>
        <owl:disjointWith rdf:resource="&mat;MultiplyAlkylatedCyclopentane"/>
        <owl:disjointWith rdf:resource="&mat;OrganicSoapGellant"/>
        <owl:disjointWith rdf:resource="&mat;PTFEGellant"/>
        <owl:disjointWith rdf:resource="&mat;Perfluoropolyether"/>
        <owl:disjointWith rdf:resource="&mat;Polyalphaolefin"/>
        <owl:disjointWith rdf:resource="&mat;Polyglycol"/>
        <owl:disjointWith rdf:resource="&mat;PolyphenyletherBaseLubricant"/>
        <owl:disjointWith rdf:resource="&mat;Quenchant"/>
        <owl:disjointWith rdf:resource="&mat;SiliconeBaseLubricant"/>
        <owl:disjointWith rdf:resource="&mat;SiliconeGellant"/>
        <owl:disjointWith rdf:resource="&mat;SyntheticEtherBase"/>
        <owl:disjointWith rdf:resource="&mat;UreaGellant"/>
        <owl:disjointWith rdf:resource="&mat;WhiteMineralOil"/>
        <owl:disjointWith rdf:resource="&mat;ZincOxideLubricant"/>
        <or:referenceURL rdf:datatype="&xsd;anyURI">http://www.matweb.com/index.aspx</or:referenceURL>
        <or:termString xml:lang="en">lithium gellant</or:termString>
    </owl:Class>
    


    <!-- http://www.nist.gov/itl/ssd/Materials#LowAlloySteel -->

    <owl:Class rdf:about="&mat;LowAlloySteel">
        <rdfs:subClassOf rdf:resource="&mat;AlloySteel"/>
        <owl:disjointWith rdf:resource="&mat;MediumAlloySteel"/>
        <or:referenceURL rdf:datatype="&xsd;anyURI">http://www.matweb.com/index.aspx</or:referenceURL>
        <or:termString xml:lang="en">low alloy steel</or:termString>
    </owl:Class>
    


    <!-- http://www.nist.gov/itl/ssd/Materials#LowCarbonSteel -->

    <owl:Class rdf:about="&mat;LowCarbonSteel">
        <rdfs:subClassOf rdf:resource="&mat;CarbonSteel"/>
        <owl:disjointWith rdf:resource="&mat;MediumCarbonSteel"/>
        <or:referenceURL rdf:datatype="&xsd;anyURI">http://www.matweb.com/index.aspx</or:referenceURL>
        <or:termString xml:lang="en">low carbon steel</or:termString>
    </owl:Class>
    


    <!-- http://www.nist.gov/itl/ssd/Materials#MachinableCeramic -->

    <owl:Class rdf:about="&mat;MachinableCeramic">
        <rdfs:subClassOf rdf:resource="&mat;Ceramic"/>
        <rdfs:subClassOf rdf:resource="&mat;EngineeredMaterial"/>
        <or:referenceURL rdf:datatype="&xsd;anyURI">http://www.matweb.com/index.aspx</or:referenceURL>
        <rdfs:comment xml:lang="en">Machinable Ceramic is a ceramic substance that can be machined on conventional shop equipment with standard cutting tools.</rdfs:comment>
        <or:termString xml:lang="en">machinable ceramic</or:termString>
    </owl:Class>
    


    <!-- http://www.nist.gov/itl/ssd/Materials#MagnesiumAlloy -->

    <owl:Class rdf:about="&mat;MagnesiumAlloy">
        <rdfs:subClassOf rdf:resource="&mat;NonFerrousAlloy"/>
        <rdfs:subClassOf>
            <owl:Restriction>
                <owl:onProperty rdf:resource="&mat;physicalDecompositions"/>
                <owl:someValuesFrom rdf:resource="&bc;Magnesium"/>
            </owl:Restriction>
        </rdfs:subClassOf>
        <or:referenceURL rdf:datatype="&xsd;anyURI">http://www.matweb.com/index.aspx</or:referenceURL>
        <rdfs:comment xml:lang="en">An alloy that contains Magnesium but not Iron.</rdfs:comment>
    </owl:Class>
    


    <!-- http://www.nist.gov/itl/ssd/Materials#MagnesiumOxide -->

    <owl:Class rdf:about="&mat;MagnesiumOxide">
        <rdfs:subClassOf rdf:resource="&bc;Oxide"/>
        <owl:disjointWith rdf:resource="&mat;SiliconOxide"/>
        <owl:disjointWith rdf:resource="&mat;TitaniumOxide"/>
        <owl:disjointWith rdf:resource="&mat;ZirconiumOxide"/>
        <or:referenceURL rdf:datatype="&xsd;anyURI">http://www.matweb.com/index.aspx</or:referenceURL>
        <or:termString xml:lang="en">magnesium oxide</or:termString>
    </owl:Class>
    


    <!-- http://www.nist.gov/itl/ssd/Materials#MagneticProperty -->

    <owl:Class rdf:about="&mat;MagneticProperty">
        <rdfs:subClassOf rdf:resource="&or;MeasurableMaterialProperty"/>
        <owl:disjointWith rdf:resource="&mat;MechanicalProperty"/>
        <owl:disjointWith rdf:resource="&mat;OpticalProperty"/>
        <owl:disjointWith rdf:resource="&mat;RadiologicalProperty"/>
    </owl:Class>
    


    <!-- http://www.nist.gov/itl/ssd/Materials#MalleableIron -->

    <owl:Class rdf:about="&mat;MalleableIron">
        <rdfs:subClassOf rdf:resource="&mat;CastIron"/>
        <owl:disjointWith rdf:resource="&mat;WhiteCastIron"/>
        <or:referenceURL rdf:datatype="&xsd;anyURI">http://www.matweb.com/index.aspx</or:referenceURL>
        <rdfs:comment xml:lang="en">Malleable iron is cast as white iron, the structure being a metastable carbide in a pearlitic matrix. Through an annealing heat treatment, the brittle structure as first cast, is transformed into the malleable form. Carbon agglomerates into small roughly spherical aggregates of graphite leaving a matrix of ferrite or pearlite according to the exact heat treat used. Three basic types of malleable iron are recognized within the casting industry: Blackheart malleable iron, Whiteheart malleable iron and Pearlitic malleable iron.</rdfs:comment>
        <or:termString xml:lang="en">malleable iron</or:termString>
    </owl:Class>
    


    <!-- http://www.nist.gov/itl/ssd/Materials#ManufacturedGlass -->

    <owl:Class rdf:about="&mat;ManufacturedGlass">
        <owl:equivalentClass>
            <owl:Class>
                <owl:intersectionOf rdf:parseType="Collection">
                    <rdf:Description rdf:about="&mat;EngineeredMaterial"/>
                    <rdf:Description rdf:about="&mat;GlassyMaterial"/>
                </owl:intersectionOf>
            </owl:Class>
        </owl:equivalentClass>
        <rdfs:subClassOf rdf:resource="&mat;GlassyMaterial"/>
    </owl:Class>
    


    <!-- http://www.nist.gov/itl/ssd/Materials#MaragingSteel -->

    <owl:Class rdf:about="&mat;MaragingSteel">
        <rdfs:subClassOf rdf:resource="&mat;Steel"/>
        <or:referenceURL rdf:datatype="&xsd;anyURI">http://en.wikipedia.org/wiki/Maraging_steel</or:referenceURL>
        <or:referenceURL rdf:datatype="&xsd;anyURI">http://www.matweb.com/index.aspx</or:referenceURL>
        <rdfs:comment xml:lang="en">Maraging steels (a portmanteau of &quot;martensitic&quot; and &quot;aging&quot;) are steels which are known for possessing superior strength and toughness without losing malleability, although they cannot hold a good cutting edge. Aging refers to the extended heat-treatment process. These steels are a special class of low-carbon ultra-high-strength steels which derive their strength not from carbon, but from precipitation of inter-metallic compounds. The principal alloying element is 15 to 25 wt.% nickel.</rdfs:comment>
        <or:termString xml:lang="en">maraging steel</or:termString>
    </owl:Class>
    


    <!-- http://www.nist.gov/itl/ssd/Materials#MartensiticPhaseTransformation -->

    <owl:Class rdf:about="&mat;MartensiticPhaseTransformation">
        <rdfs:subClassOf rdf:resource="&mat;DeviatonicDominantPhaseTransformation"/>
        <owl:disjointWith rdf:resource="&mat;QuasimartensiticPhaseTranformation"/>
        <oil:seeAlso>http://en.wikipedia.org/w/index.php?title=File:Diffusionless_classification.svg</oil:seeAlso>
        <rdfs:comment xml:lang="en">Shear dominated transformations can be classified according to the magnitude of the strain energies involved compared to the innate vibrations of the atoms in the lattice and hence whether the strain energies have a notable influence on the kinetics of the transformation and the morphology of the resulting phase. If the strain energy is a significant factor then the transformations are dubbed martensitic and if it is not the transformation is referred to as quasi-martensitic.</rdfs:comment>
    </owl:Class>
    


    <!-- http://www.nist.gov/itl/ssd/Materials#MassSpectrometer -->

    <owl:Class rdf:about="&mat;MassSpectrometer">
        <rdfs:subClassOf rdf:resource="&mat;Spectrometer"/>
        <rdfs:comment xml:lang="en">A Mass Spectrometer is a device used for determining masses of particles, for determining the elemental composition of a sample or molecule, and for elucidating the chemical structures of molecules. Mass spectrometry works by ionizing chemical compounds to generate charged molecules or molecule fragments and measuring their mass-to-charge ratios.</rdfs:comment>
    </owl:Class>
    


    <!-- http://www.nist.gov/itl/ssd/Materials#MatanoPlane -->

    <owl:Class rdf:about="&mat;MatanoPlane">
        <rdfs:subClassOf rdf:resource="&or;PlanarRegion"/>
        <rdfs:seeAlso>Definitions of terms for diffusion in the solid state (IUPAC Recommendations 1999), Pure Appl. Chem. 71, 1307-1325.</rdfs:seeAlso>
        <or:termString xml:lang="en">Matano plane</or:termString>
        <rdfs:comment xml:lang="en">The Matano plane is the interface through which equal amounts of substance have moved in the positive and negative directions during interdiffusion.</rdfs:comment>
    </owl:Class>
    


    <!-- http://www.nist.gov/itl/ssd/Materials#MaterialCreep -->

    <owl:Class rdf:about="&mat;MaterialCreep">
        <rdfs:subClassOf rdf:resource="&mat;Deformation"/>
        <rdfs:comment xml:lang="en">Material Creep is a permanent deformation over time under the influence of stresses.</rdfs:comment>
    </owl:Class>
    


    <!-- http://www.nist.gov/itl/ssd/Materials#MaterialFatigue -->

    <owl:Class rdf:about="&mat;MaterialFatigue">
        <rdfs:subClassOf rdf:resource="&or;MechanicalProcess"/>
        <owl:disjointWith rdf:resource="&mat;MicroscopicDiffusionMovement"/>
        <owl:disjointWith rdf:resource="&mat;PhaseChange"/>
        <owl:disjointWith rdf:resource="&mat;TemperatureChangeProcess"/>
        <owl:disjointWith rdf:resource="&mat;ThermalExpansion"/>
        <rdfs:comment xml:lang="en">Material Fatigue is progressive and localized structural damage that occurs when a material is subjected to cyclic loading.</rdfs:comment>
    </owl:Class>
    


    <!-- http://www.nist.gov/itl/ssd/Materials#MaterialForm -->

    <owl:Class rdf:about="&mat;MaterialForm">
        <rdfs:subClassOf rdf:resource="&or;ObjectType"/>
        <rdfs:comment xml:lang="en">A Material Form designates a type of material by its form, e.g., Composite Substance, Alloy, Suspension, Pure Substance, Crystaline.</rdfs:comment>
    </owl:Class>
    


    <!-- http://www.nist.gov/itl/ssd/Materials#MaterialObject -->

    <owl:Class rdf:about="&mat;MaterialObject">
        <owl:equivalentClass>
            <owl:Class>
                <owl:intersectionOf rdf:parseType="Collection">
                    <rdf:Description rdf:about="&or;PhysicalObject"/>
                    <owl:Class>
                        <owl:complementOf rdf:resource="&mat;Vacuum"/>
                    </owl:Class>
                </owl:intersectionOf>
            </owl:Class>
        </owl:equivalentClass>
        <rdfs:subClassOf rdf:resource="&or;PhysicalObject"/>
        <owl:disjointWith rdf:resource="&mat;Vacuum"/>
    </owl:Class>
    


    <!-- http://www.nist.gov/itl/ssd/Materials#MaterialPhaseComposition -->

    <owl:Class rdf:about="&mat;MaterialPhaseComposition">
        <rdfs:subClassOf rdf:resource="&or;ObjectType"/>
        <rdfs:comment xml:lang="en">The class of Material Phases.</rdfs:comment>
    </owl:Class>
    


    <!-- http://www.nist.gov/itl/ssd/Materials#MaterialPortion -->

    <owl:Class rdf:about="&mat;MaterialPortion">
        <rdfs:subClassOf rdf:resource="&bc;MaterialSubstance"/>
        <owl:disjointWith rdf:resource="&mat;Vacuum"/>
        <oil:disjointWith xml:lang="en">A &#39;Material Portion&#39; is part of a portion of a Material Substance that has a certain property.  It is normally diffused throughout an object, but it may be in multiple pieces.  It could be all the grains of one type in a piece of granite, all the zinc in a piece of brass, all the Carbon Dioxide in a room, etc.  

A Material Portion comprises some percentage of the object of which it is a portion by volume and likely a different percentage of the same object by mass (weight).  The Material Portion has different properties than the object as a whole and different properties from other Material Portions of the same Physical Object.</oil:disjointWith>
    </owl:Class>
    


    <!-- http://www.nist.gov/itl/ssd/Materials#MeanMassFrameOfReference -->

    <owl:Class rdf:about="&mat;MeanMassFrameOfReference">
        <rdfs:subClassOf rdf:resource="&or;SpatialFrameOfReference"/>
        <rdfs:seeAlso>Definitions of terms for diffusion in the solid state (IUPAC Recommendations 1999), Pure Appl. Chem. 71, 1307-1325.</rdfs:seeAlso>
        <rdfs:comment xml:lang="en">The mean-mass frame RM moves in such a way that the net flux of mass traversing a plane normal to the diffusion direction is zero everywhere and at all times  The mean-mass reference frame is also known as the barycentric frame of reference.</rdfs:comment>
        <or:termString xml:lang="en">barycentric frame of reference</or:termString>
        <or:termString xml:lang="en">mean-mass frame</or:termString>
        <or:termString xml:lang="en">mean-mass frame of reference</or:termString>
    </owl:Class>
    


    <!-- http://www.nist.gov/itl/ssd/Materials#MeanMolarFrameOfReference -->

    <owl:Class rdf:about="&mat;MeanMolarFrameOfReference">
        <rdfs:subClassOf rdf:resource="&or;SpatialFrameOfReference"/>
        <rdfs:seeAlso>Definitions of terms for diffusion in the solid state (IUPAC Recommendations 1999), Pure Appl. Chem. 71, 1307-1325.</rdfs:seeAlso>
        <rdfs:comment xml:lang="en">The mean-molar frame of reference RN moves with respect to the laboratory frame so that the net flux expressed in number of moles of material traversing a plane normal to the diffusion direction is zero
everywhere and at all times  The frame is also called number-fixed frame.</rdfs:comment>
        <or:termString xml:lang="en">mean-molar frame</or:termString>
        <or:termString xml:lang="en">mean-molar frame of reference</or:termString>
        <or:termString xml:lang="en">number-fixed frame</or:termString>
        <or:termString xml:lang="en">number-fixed frame of reference</or:termString>
    </owl:Class>
    


    <!-- http://www.nist.gov/itl/ssd/Materials#MeanVolumeFrameOfReference -->

    <owl:Class rdf:about="&mat;MeanVolumeFrameOfReference">
        <rdfs:subClassOf rdf:resource="&or;SpatialFrameOfReference"/>
        <rdfs:seeAlso>Definitions of terms for diffusion in the solid state (IUPAC Recommendations 1999), Pure Appl. Chem. 71, 1307-1325.</rdfs:seeAlso>
        <or:termString xml:lang="en">Fick’s reference frame</or:termString>
        <rdfs:comment xml:lang="en">The mean-volume frame RV moves with respect to the laboratory frame R0 so that the net flux expressed in volume of material traversing a plane normal to the diffusion direction is zero everywhere and at all times.  The mean-volume frame is also known as Fick’s reference frame.</rdfs:comment>
        <or:termString xml:lang="en">mean-volume frame</or:termString>
        <or:termString xml:lang="en">mean-volume frame of reference</or:termString>
        <or:termString xml:lang="en">volume-fixed frame</or:termString>
        <or:termString xml:lang="en">volume-fixed frame of reference</or:termString>
    </owl:Class>
    


    <!-- http://www.nist.gov/itl/ssd/Materials#MeasurableMechanicalProperty -->

    <owl:Class rdf:about="&mat;MeasurableMechanicalProperty">
        <owl:equivalentClass>
            <owl:Class>
                <owl:intersectionOf rdf:parseType="Collection">
                    <rdf:Description rdf:about="&mat;MechanicalProperty"/>
                    <rdf:Description rdf:about="&or;MeasurableMaterialProperty"/>
                </owl:intersectionOf>
            </owl:Class>
        </owl:equivalentClass>
        <rdfs:subClassOf rdf:resource="&mat;MechanicalProperty"/>
        <rdfs:subClassOf rdf:resource="&or;MeasurableMaterialProperty"/>
        <rdfs:comment xml:lang="en">A Measurable Mechanical Property is any Mechanical Property of some physical material or object that has a numeric value with a unit of measure.  This includes properties as mass, melting point, and temperature.  A Mechanical Property is distinguished from a Chemical Property, Electrical Property, or Magnetic Property. </rdfs:comment>
    </owl:Class>
    


    <!-- http://www.nist.gov/itl/ssd/Materials#MechanicalProperty -->

    <owl:Class rdf:about="&mat;MechanicalProperty">
        <rdfs:subClassOf rdf:resource="&or;MaterialProperty"/>
        <owl:disjointWith rdf:resource="&mat;RadiologicalProperty"/>
        <owl:disjointWith rdf:resource="&mat;ThermalProperty"/>
        <rdfs:comment xml:lang="en">A Mechanical Property is a physical property of some physical material or object, such as mass,concentration, or microstructure.  A Mechanical Property is distinguished from a Chemical Property, Electrical Property, Magnetic Property, or Thermal Property. </rdfs:comment>
        <skos:note xml:lang="en">Similar to &quot;Mechanical&quot; in Ashino&#39;s 2010 Minerals Ontology.</skos:note>
    </owl:Class>
    


    <!-- http://www.nist.gov/itl/ssd/Materials#MediumAlloySteel -->

    <owl:Class rdf:about="&mat;MediumAlloySteel">
        <rdfs:subClassOf rdf:resource="&mat;AlloySteel"/>
        <or:referenceURL rdf:datatype="&xsd;anyURI">http://www.matweb.com/index.aspx</or:referenceURL>
        <or:termString xml:lang="en">mediumAlloySteel</or:termString>
    </owl:Class>
    


    <!-- http://www.nist.gov/itl/ssd/Materials#MediumCarbonSteel -->

    <owl:Class rdf:about="&mat;MediumCarbonSteel">
        <rdfs:subClassOf rdf:resource="&mat;CarbonSteel"/>
        <or:referenceURL rdf:datatype="&xsd;anyURI">http://www.matweb.com/index.aspx</or:referenceURL>
        <or:termString xml:lang="en">medium carbon steel</or:termString>
    </owl:Class>
    


    <!-- http://www.nist.gov/itl/ssd/Materials#Melting -->

    <owl:Class rdf:about="&mat;Melting">
        <rdfs:subClassOf rdf:resource="&mat;OrderDisorderPhaseTransformation"/>
        <owl:disjointWith rdf:resource="&mat;PeritecticDecomposition"/>
        <owl:disjointWith rdf:resource="&mat;Sublimating"/>
        <rdfs:comment xml:lang="en">Melting is the Phase Change from a solid state to a liquid state.</rdfs:comment>
    </owl:Class>
    


    <!-- http://www.nist.gov/itl/ssd/Materials#MetalMatrixComposite -->

    <owl:Class rdf:about="&mat;MetalMatrixComposite">
        <rdfs:subClassOf rdf:resource="&mat;CompositeMaterial"/>
        <rdfs:subClassOf rdf:resource="&mat;EngineeredMaterial"/>
    </owl:Class>
    


    <!-- http://www.nist.gov/itl/ssd/Materials#MetallicMicrostructure -->

    <owl:Class rdf:about="&mat;MetallicMicrostructure">
        <rdfs:subClassOf rdf:resource="&mat;Microstructure"/>
        <owl:disjointWith rdf:resource="&mat;PolymericMicrostructure"/>
        <rdfs:comment xml:lang="en">A Metallic Microstructure is a material Microstructure typical of metals.</rdfs:comment>
    </owl:Class>
    


    <!-- http://www.nist.gov/itl/ssd/Materials#Methylcellulose -->

    <owl:Class rdf:about="&mat;Methylcellulose">
        <rdfs:subClassOf rdf:resource="&mat;AlkylCelluloseEthers"/>
        <rdfs:comment xml:lang="en">Methyl cellulose is produced by heating cellulose with caustic solution and treating it with methyl chloride. In the substitution reaction, the hydroxyl residuesare replaced by methoxide (-OCH3 groups).  Different kinds of methyl cellulose can be prepared depending on the number of hydroxyl groups substituted.</rdfs:comment>
    </owl:Class>
    


    <!-- http://www.nist.gov/itl/ssd/Materials#Microfracturing -->

    <owl:Class rdf:about="&mat;Microfracturing">
        <rdfs:subClassOf rdf:resource="&mat;Cracking"/>
        <rdfs:subClassOf rdf:resource="&mat;MicroscopicMovement"/>
        <owl:disjointWith rdf:resource="&mat;MicroscopicDiffusionMovement"/>
        <rdfs:comment xml:lang="en">Microfracturing is Fracturing at a microscopic scale.</rdfs:comment>
    </owl:Class>
    


    <!-- http://www.nist.gov/itl/ssd/Materials#MicroscopicDiffusionMovement -->

    <owl:Class rdf:about="&mat;MicroscopicDiffusionMovement">
        <rdfs:subClassOf rdf:resource="&mat;MicroscopicMovement"/>
        <owl:disjointWith rdf:resource="&mat;PhaseChange"/>
        <owl:disjointWith rdf:resource="&mat;TemperatureChangeProcess"/>
        <owl:disjointWith rdf:resource="&mat;ThermalExpansion"/>
        <rdfs:comment xml:lang="en">A Microscopic Diffusion Movement is the movement of an atom or crystal vacancy from one site to another as part of a larger process of diffusion.</rdfs:comment>
    </owl:Class>
    


    <!-- http://www.nist.gov/itl/ssd/Materials#MicroscopicMovement -->

    <owl:Class rdf:about="&mat;MicroscopicMovement">
        <rdfs:subClassOf rdf:resource="&or;MovementEvent"/>
        <rdfs:comment xml:lang="en">Microscopic Movement is movement on a microscopic scale.</rdfs:comment>
    </owl:Class>
    


    <!-- http://www.nist.gov/itl/ssd/Materials#Microstructure -->

    <owl:Class rdf:about="&mat;Microstructure">
        <rdfs:subClassOf rdf:resource="&mat;MechanicalProperty"/>
        <rdfs:comment xml:lang="en">Microstructure is defined as the structure of a material, which can be examined by microscopic examination of a prepared surface or thin foil of the material. The microstructure of a material can be broadly classified as metallic, polymeric, ceramic, or composite.</rdfs:comment>
    </owl:Class>
    


    <!-- http://www.nist.gov/itl/ssd/Materials#MicrostructureEvolution -->

    <owl:Class rdf:about="&mat;MicrostructureEvolution">
        <rdfs:subClassOf rdf:resource="&or;PhysicalEvent"/>
        <owl:disjointWith rdf:resource="&mat;TemperatureChangeProcess"/>
        <owl:disjointWith rdf:resource="&or;PurposefulAction"/>
        <rdfs:comment xml:lang="en">Microstructural Evolution is the process of change in the Microstructure of materials by any mechanism.  Microsctructrure Evolution may alter a material&#39;s the macroscopic properties. This process can be a result of mechanical and thermal loading, chemical transformation, radiation, or by other conditions.</rdfs:comment>
    </owl:Class>
    


    <!-- http://www.nist.gov/itl/ssd/Materials#MicrostructurePrediction -->

    <owl:Class rdf:about="&mat;MicrostructurePrediction">
        <rdfs:subClassOf rdf:resource="&doc;Prediction"/>
        <rdfs:comment xml:lang="en">Microstructure Prediction is the prediction of the Microstructure of a material based on its component materials and method of production.</rdfs:comment>
    </owl:Class>
    


    <!-- http://www.nist.gov/itl/ssd/Materials#Mineral -->

    <owl:Class rdf:about="&mat;Mineral">
        <rdfs:subClassOf rdf:resource="&mat;SolidSubstance"/>
        <owl:disjointWith rdf:resource="&or;Artifact"/>
        <rdfs:comment xml:lang="en">A mineral is a naturally occurring non-biological substance that is solid and stable at room temperature, representable by a chemical formula, and has an ordered atomic structure.  Some rocks may be composed of a single mineral, while others are aggregates of minerals or non-minerals, and do not have a specific chemical composition.</rdfs:comment>
    </owl:Class>
    


    <!-- http://www.nist.gov/itl/ssd/Materials#MineralType -->

    <owl:Class rdf:about="&mat;MineralType">
        <rdfs:subClassOf rdf:resource="&or;MaterialType"/>
        <rdfs:comment xml:lang="en">A Mineral Type is a type of natural occuring mineral.</rdfs:comment>
    </owl:Class>
    


    <!-- http://www.nist.gov/itl/ssd/Materials#MolecularSimulationModel -->

    <owl:Class rdf:about="&mat;MolecularSimulationModel">
        <rdfs:subClassOf rdf:resource="&or;SimulationModel"/>
        <rdfs:comment xml:lang="en">Molecular Simulation Model is a model of the behaviour of a molecular system as a function of time.</rdfs:comment>
    </owl:Class>
    


    <!-- http://www.nist.gov/itl/ssd/Materials#MolybdenumAlloy -->

    <owl:Class rdf:about="&mat;MolybdenumAlloy">
        <rdfs:subClassOf rdf:resource="&mat;NonFerrousAlloy"/>
        <rdfs:subClassOf>
            <owl:Restriction>
                <owl:onProperty rdf:resource="&mat;physicalDecompositions"/>
                <owl:someValuesFrom rdf:resource="&bc;Molybdenum"/>
            </owl:Restriction>
        </rdfs:subClassOf>
        <or:referenceURL rdf:datatype="&xsd;anyURI">http://www.matweb.com/index.aspx</or:referenceURL>
        <rdfs:comment xml:lang="en">An alloy that contains Molybdenum but not Iron.</rdfs:comment>
    </owl:Class>
    


    <!-- http://www.nist.gov/itl/ssd/Materials#MonoclinicCrystalStructure -->

    <owl:Class rdf:about="&mat;MonoclinicCrystalStructure">
        <rdfs:subClassOf rdf:resource="&mat;CrystalLattice"/>
        <owl:disjointWith rdf:resource="&mat;OrthorhombicCrystalStructure"/>
        <owl:disjointWith rdf:resource="&mat;TetragonalCrystalStructure"/>
        <owl:disjointWith rdf:resource="&mat;TriclinicCrystalStructure"/>
        <owl:disjointWith rdf:resource="&mat;TrigonalCrystalStructure"/>
    </owl:Class>
    


    <!-- http://www.nist.gov/itl/ssd/Materials#MonotecticPhaseChange -->

    <owl:Class rdf:about="&mat;MonotecticPhaseChange">
        <rdfs:subClassOf rdf:resource="&mat;PhaseChange"/>
        <rdfs:comment xml:lang="en">A Monotectic Phase Change is a phase change in which  in which one liquid phase decomposes with decreasing temperature into a solid phase and a new liquid phase.</rdfs:comment>
    </owl:Class>
    


    <!-- http://www.nist.gov/itl/ssd/Materials#MultiphaseDiffusion -->

    <owl:Class rdf:about="&mat;MultiphaseDiffusion">
        <rdfs:subClassOf rdf:resource="&mat;SolidDiffusion"/>
        <rdfs:seeAlso xml:lang="en">Definitions of terms for diffusion in the solid state (IUPAC Recommendations 1999), Pure Appl. Chem. 71, 1307-1325.</rdfs:seeAlso>
        <rdfs:comment xml:lang="en">Multiphase Diffusion is a diffusion process leading to the formation of a new interface, such as occurs during formation of allotropic structures, new phases, solid solutions, and/or chemical reactions.  Also called ``reaction diffusion&#39;&#39;.</rdfs:comment>
        <or:termString xml:lang="en">multiphase diffusion</or:termString>
        <or:termString xml:lang="en">reaction diffusion</or:termString>
    </owl:Class>
    


    <!-- http://www.nist.gov/itl/ssd/Materials#MultiphaseMaterialType -->

    <owl:Class rdf:about="&mat;MultiphaseMaterialType">
        <rdfs:subClassOf rdf:resource="&or;MaterialType"/>
        <rdfs:comment xml:lang="en">A multiphase material consists of more than one material phases, with concentration (which could be specified by volume) for each phase.  The phases could be different states of matter or different Crystal Structures.</rdfs:comment>
    </owl:Class>
    


    <!-- http://www.nist.gov/itl/ssd/Materials#MultiplyAlkylatedCyclopentane -->

    <owl:Class rdf:about="&mat;MultiplyAlkylatedCyclopentane">
        <rdfs:subClassOf rdf:resource="&mat;FluidLubricant"/>
        <owl:disjointWith rdf:resource="&mat;OrganicSoapGellant"/>
        <owl:disjointWith rdf:resource="&mat;PTFEGellant"/>
        <owl:disjointWith rdf:resource="&mat;Perfluoropolyether"/>
        <owl:disjointWith rdf:resource="&mat;Polyalphaolefin"/>
        <owl:disjointWith rdf:resource="&mat;PolyphenyletherBaseLubricant"/>
        <owl:disjointWith rdf:resource="&mat;Quenchant"/>
        <owl:disjointWith rdf:resource="&mat;SiliconeBaseLubricant"/>
        <owl:disjointWith rdf:resource="&mat;SiliconeGellant"/>
        <owl:disjointWith rdf:resource="&mat;SyntheticEtherBase"/>
        <owl:disjointWith rdf:resource="&mat;UreaGellant"/>
        <owl:disjointWith rdf:resource="&mat;WhiteMineralOil"/>
        <owl:disjointWith rdf:resource="&mat;ZincOxideLubricant"/>
        <or:referenceURL rdf:datatype="&xsd;anyURI">http://www.matweb.com/index.aspx</or:referenceURL>
        <or:termString xml:lang="en">MAC</or:termString>
        <or:termString xml:lang="en">multiply-alkylated cyclopentane</or:termString>
    </owl:Class>
    


    <!-- http://www.nist.gov/itl/ssd/Materials#NanoMaterial -->

    <owl:Class rdf:about="&mat;NanoMaterial">
        <rdfs:subClassOf rdf:resource="&bc;MaterialSubstance"/>
        <rdfs:comment xml:lang="en">A nanomaterial (according to the European Commission) is ``a natural, incidental or manufactured material containing particles, in an unbound state or as an aggregate or as an agglomerate and where, for 50% or more of the particles in the number size distribution, one or more external dimensions is in the size range 1 nm – 100 nm. In specific cases and where warranted by concerns for the environment, health, safety or competitiveness the number size distribution threshold of 50% may be replaced by a threshold between 1 and 50%.&#39;&#39;
</rdfs:comment>
    </owl:Class>
    


    <!-- http://www.nist.gov/itl/ssd/Materials#NativeMetal -->

    <owl:Class rdf:about="&mat;NativeMetal">
        <rdfs:subClassOf rdf:resource="&mat;Mineral"/>
        <rdfs:comment xml:lang="en">A Native Metal is a mineral that is a metal that occurs in nature in uncombined form with a distinct mineral structure. This includes elemental metals and inatural ntermetallic alloys.</rdfs:comment>
    </owl:Class>
    


    <!-- http://www.nist.gov/itl/ssd/Materials#NickelAlloy -->

    <owl:Class rdf:about="&mat;NickelAlloy">
        <rdfs:subClassOf rdf:resource="&mat;NonFerrousAlloy"/>
        <rdfs:subClassOf>
            <owl:Restriction>
                <owl:onProperty rdf:resource="&mat;physicalDecompositions"/>
                <owl:someValuesFrom rdf:resource="&bc;Nickel"/>
            </owl:Restriction>
        </rdfs:subClassOf>
        <or:referenceURL rdf:datatype="&xsd;anyURI">http://www.matweb.com/index.aspx</or:referenceURL>
        <rdfs:comment xml:lang="en">An alloy that contains Nickel but not Iron.</rdfs:comment>
    </owl:Class>
    


    <!-- http://www.nist.gov/itl/ssd/Materials#NiobiumAlloy -->

    <owl:Class rdf:about="&mat;NiobiumAlloy">
        <rdfs:subClassOf rdf:resource="&mat;NonFerrousAlloy"/>
        <rdfs:subClassOf>
            <owl:Restriction>
                <owl:onProperty rdf:resource="&mat;physicalDecompositions"/>
                <owl:someValuesFrom rdf:resource="&bc;Niobium"/>
            </owl:Restriction>
        </rdfs:subClassOf>
        <or:referenceURL rdf:datatype="&xsd;anyURI">http://www.matweb.com/index.aspx</or:referenceURL>
    </owl:Class>
    


    <!-- http://www.nist.gov/itl/ssd/Materials#NitrateMineral -->

    <owl:Class rdf:about="&mat;NitrateMineral">
        <rdfs:subClassOf rdf:resource="&mat;Mineral"/>
    </owl:Class>
    


    <!-- http://www.nist.gov/itl/ssd/Materials#NitrideBasedCeramic -->

    <owl:Class rdf:about="&mat;NitrideBasedCeramic">
        <rdfs:subClassOf rdf:resource="&mat;PnictideCeramic"/>
        <owl:disjointWith rdf:resource="&mat;PhosphideBasedCeramic"/>
        <or:referenceURL rdf:datatype="&xsd;anyURI">http://www.matweb.com/index.aspx</or:referenceURL>
        <or:termString xml:lang="en">nitride</or:termString>
        <or:termString xml:lang="en">nitride ceramic</or:termString>
        <or:termString xml:lang="en">nitride-based ceramic</or:termString>
    </owl:Class>
    


    <!-- http://www.nist.gov/itl/ssd/Materials#Nitrocellulose -->

    <owl:Class rdf:about="&mat;Nitrocellulose">
        <rdfs:subClassOf rdf:resource="&mat;CelluloseEster"/>
        <rdfs:comment xml:lang="en">Nitrocellulose is a highly flammable resin compound formed by nitrating cellulose.</rdfs:comment>
    </owl:Class>
    


    <!-- http://www.nist.gov/itl/ssd/Materials#NonCollinearInterstitialcyMechanism -->

    <owl:Class rdf:about="&mat;NonCollinearInterstitialcyMechanism">
        <rdfs:subClassOf rdf:resource="&mat;InterstitialcyMechanism"/>
        <rdfs:seeAlso xml:lang="en">Definitions of terms for diffusion in the solid state (IUPAC Recommendations 1999), Pure Appl. Chem. 71, 1307-1325.</rdfs:seeAlso>
        <rdfs:comment xml:lang="en">The Non-Collinear Interstitialcy Mechanism is an interstitialcy mechanism in which the interstitial atom and the lattice atom which it displaces do not move along the same straight line.</rdfs:comment>
    </owl:Class>
    


    <!-- http://www.nist.gov/itl/ssd/Materials#NonFerrousAlloy -->

    <owl:Class rdf:about="&mat;NonFerrousAlloy">
        <owl:equivalentClass>
            <owl:Class>
                <owl:intersectionOf rdf:parseType="Collection">
                    <rdf:Description rdf:about="&mat;Alloy"/>
                    <owl:Class>
                        <owl:complementOf>
                            <owl:Restriction>
                                <owl:onProperty rdf:resource="&mat;physicalDecompositions"/>
                                <owl:someValuesFrom rdf:resource="&bc;Iron"/>
                            </owl:Restriction>
                        </owl:complementOf>
                    </owl:Class>
                </owl:intersectionOf>
            </owl:Class>
        </owl:equivalentClass>
        <rdfs:subClassOf rdf:resource="&mat;Alloy"/>
        <rdfs:comment xml:lang="en">A non-ferrous alloy is one that does not contain iron.</rdfs:comment>
    </owl:Class>
    


    <!-- http://www.nist.gov/itl/ssd/Materials#NonFerrousAlloyTypeByMainConstituent -->

    <owl:Class rdf:about="&mat;NonFerrousAlloyTypeByMainConstituent">
        <rdfs:subClassOf rdf:resource="&mat;AlloyTypeByMainConstituent"/>
    </owl:Class>
    


    <!-- http://www.nist.gov/itl/ssd/Materials#NonIonicOrAqueousLiquidSolution -->

    <owl:Class rdf:about="&mat;NonIonicOrAqueousLiquidSolution">
        <owl:equivalentClass>
            <owl:Class>
                <owl:intersectionOf rdf:parseType="Collection">
                    <rdf:Description rdf:about="&mat;LiquidSolution"/>
                    <owl:Class>
                        <owl:complementOf rdf:resource="&mat;AqueousSolution"/>
                    </owl:Class>
                    <owl:Class>
                        <owl:complementOf rdf:resource="&mat;IonicLiquid"/>
                    </owl:Class>
                </owl:intersectionOf>
            </owl:Class>
        </owl:equivalentClass>
        <rdfs:subClassOf rdf:resource="&mat;LiquidSolution"/>
    </owl:Class>
    


    <!-- http://www.nist.gov/itl/ssd/Materials#Obsidian -->

    <owl:Class rdf:about="&mat;Obsidian">
        <rdfs:subClassOf rdf:resource="&mat;GlassyMaterial"/>
        <owl:disjointWith rdf:resource="&or;Artifact"/>
        <rdfs:comment xml:lang="en">Obsidian is a naturally occuring glass.</rdfs:comment>
    </owl:Class>
    


    <!-- http://www.nist.gov/itl/ssd/Materials#OpenCellFoam -->

    <owl:Class rdf:about="&mat;OpenCellFoam">
        <rdfs:subClassOf rdf:resource="&mat;SolidFoam"/>
        <rdfs:comment xml:lang="en">An Open-Cell Foam is a solid foam with few a low proportion of intact bubbles.</rdfs:comment>
    </owl:Class>
    


    <!-- http://www.nist.gov/itl/ssd/Materials#OpticalGlass -->

    <owl:Class rdf:about="&mat;OpticalGlass">
        <rdfs:subClassOf rdf:resource="&mat;ManufacturedGlass"/>
        <or:referenceURL rdf:datatype="&xsd;anyURI">http://www.matweb.com/index.aspx</or:referenceURL>
        <rdfs:comment xml:lang="en">Optical Glass is a glass that is formulated very precisely so that its optical properties are known, and is manufactured to ensure that it is free of impurities and variability.</rdfs:comment>
        <or:termString xml:lang="en">optical glass</or:termString>
    </owl:Class>
    


    <!-- http://www.nist.gov/itl/ssd/Materials#OpticalProperty -->

    <owl:Class rdf:about="&mat;OpticalProperty">
        <rdfs:subClassOf rdf:resource="&or;MeasurableMaterialProperty"/>
        <owl:disjointWith rdf:resource="&mat;RadiologicalProperty"/>
        <owl:disjointWith rdf:resource="&mat;ThermalProperty"/>
    </owl:Class>
    


    <!-- http://www.nist.gov/itl/ssd/Materials#OrderDisorderPhaseTransformation -->

    <owl:Class rdf:about="&mat;OrderDisorderPhaseTransformation">
        <rdfs:subClassOf rdf:resource="&mat;PhaseChange"/>
        <owl:disjointWith rdf:resource="&mat;PrecipitationFromSolution"/>
        <owl:disjointWith rdf:resource="&mat;SolidToSolidPhaseTransformation"/>
        <owl:disjointWith rdf:resource="&mat;Solidification"/>
        <rdfs:comment xml:lang="en">An Order-Disorder Phase Transformation is one in which the phase changes from an ordered phase to a disordered one.</rdfs:comment>
    </owl:Class>
    


    <!-- http://www.nist.gov/itl/ssd/Materials#OrderedBCCPhase -->

    <owl:Class rdf:about="&mat;OrderedBCCPhase">
        <rdfs:subClassOf rdf:resource="&mat;BodyCenteredCubicCrystalStructure"/>
    </owl:Class>
    


    <!-- http://www.nist.gov/itl/ssd/Materials#OrderedFCCPhase -->

    <owl:Class rdf:about="&mat;OrderedFCCPhase">
        <rdfs:subClassOf rdf:resource="&mat;FaceCenteredCubicCrystalStructure"/>
    </owl:Class>
    


    <!-- http://www.nist.gov/itl/ssd/Materials#OrderedHCPPhase -->

    <owl:Class rdf:about="&mat;OrderedHCPPhase">
        <rdfs:subClassOf rdf:resource="&mat;HexagonalClosePackedCrystalStructure"/>
    </owl:Class>
    


    <!-- http://www.nist.gov/itl/ssd/Materials#OrderedSolidSolution -->

    <owl:Class rdf:about="&mat;OrderedSolidSolution">
        <rdfs:subClassOf rdf:resource="&mat;MaterialPhaseComposition"/>
    </owl:Class>
    


    <!-- http://www.nist.gov/itl/ssd/Materials#OrganicMineral -->

    <owl:Class rdf:about="&mat;OrganicMineral">
        <rdfs:subClassOf rdf:resource="&mat;Mineral"/>
    </owl:Class>
    


    <!-- http://www.nist.gov/itl/ssd/Materials#OrganicSoapGellant -->

    <owl:Class rdf:about="&mat;OrganicSoapGellant">
        <rdfs:subClassOf rdf:resource="&mat;FluidLubricant"/>
        <owl:disjointWith rdf:resource="&mat;PTFEGellant"/>
        <owl:disjointWith rdf:resource="&mat;Perfluoropolyether"/>
        <owl:disjointWith rdf:resource="&mat;Polyalphaolefin"/>
        <owl:disjointWith rdf:resource="&mat;Polyglycol"/>
        <owl:disjointWith rdf:resource="&mat;PolyphenyletherBaseLubricant"/>
        <owl:disjointWith rdf:resource="&mat;Quenchant"/>
        <owl:disjointWith rdf:resource="&mat;SiliconeBaseLubricant"/>
        <owl:disjointWith rdf:resource="&mat;SiliconeGellant"/>
        <owl:disjointWith rdf:resource="&mat;SyntheticEtherBase"/>
        <owl:disjointWith rdf:resource="&mat;UreaGellant"/>
        <owl:disjointWith rdf:resource="&mat;WhiteMineralOil"/>
        <owl:disjointWith rdf:resource="&mat;ZincOxideLubricant"/>
        <or:referenceURL rdf:datatype="&xsd;anyURI">http://www.matweb.com/index.aspx</or:referenceURL>
        <or:termString xml:lang="en">organic soap gellant</or:termString>
    </owl:Class>
    


    <!-- http://www.nist.gov/itl/ssd/Materials#OrthorhombicCrystalStructure -->

    <owl:Class rdf:about="&mat;OrthorhombicCrystalStructure">
        <rdfs:subClassOf rdf:resource="&mat;CrystalLattice"/>
        <owl:disjointWith rdf:resource="&mat;TetragonalCrystalStructure"/>
        <owl:disjointWith rdf:resource="&mat;TriclinicCrystalStructure"/>
        <owl:disjointWith rdf:resource="&mat;TrigonalCrystalStructure"/>
    </owl:Class>
    


    <!-- http://www.nist.gov/itl/ssd/Materials#OxideBasedCeramic -->

    <owl:Class rdf:about="&mat;OxideBasedCeramic">
        <rdfs:subClassOf rdf:resource="&mat;Ceramic"/>
        <owl:disjointWith rdf:resource="&mat;PnictideCeramic"/>
        <or:referenceURL rdf:datatype="&xsd;anyURI">http://www.matweb.com/index.aspx</or:referenceURL>
        <or:termString xml:lang="en">ceramic  oxide</or:termString>
        <or:termString xml:lang="en">oxide</or:termString>
    </owl:Class>
    


    <!-- http://www.nist.gov/itl/ssd/Materials#OxideMineral -->

    <owl:Class rdf:about="&mat;OxideMineral">
        <rdfs:subClassOf rdf:resource="&mat;Mineral"/>
    </owl:Class>
    


    <!-- http://www.nist.gov/itl/ssd/Materials#PTFEGellant -->

    <owl:Class rdf:about="&mat;PTFEGellant">
        <rdfs:subClassOf rdf:resource="&mat;FluidLubricant"/>
        <owl:disjointWith rdf:resource="&mat;Perfluoropolyether"/>
        <owl:disjointWith rdf:resource="&mat;Polyalphaolefin"/>
        <owl:disjointWith rdf:resource="&mat;Polyglycol"/>
        <owl:disjointWith rdf:resource="&mat;PolyphenyletherBaseLubricant"/>
        <owl:disjointWith rdf:resource="&mat;Quenchant"/>
        <owl:disjointWith rdf:resource="&mat;SiliconeBaseLubricant"/>
        <owl:disjointWith rdf:resource="&mat;SiliconeGellant"/>
        <owl:disjointWith rdf:resource="&mat;SyntheticEtherBase"/>
        <owl:disjointWith rdf:resource="&mat;UreaGellant"/>
        <owl:disjointWith rdf:resource="&mat;WhiteMineralOil"/>
        <owl:disjointWith rdf:resource="&mat;ZincOxideLubricant"/>
        <or:referenceURL rdf:datatype="&xsd;anyURI">http://www.matweb.com/index.aspx</or:referenceURL>
        <or:termString xml:lang="en">PTFE gellant</or:termString>
        <or:termString xml:lang="en">polytetrafluoroethylene gellant</or:termString>
    </owl:Class>
    


    <!-- http://www.nist.gov/itl/ssd/Materials#PasteSubstance -->

    <owl:Class rdf:about="&mat;PasteSubstance">
        <rdfs:subClassOf rdf:resource="&mat;ChemicalSuspension"/>
        <owl:disjointWith rdf:resource="&mat;PowderySubstance"/>
        <rdfs:comment xml:lang="en">A Paste is a substance that behaves as a solid until a sufficiently large load or stress is applied, at which point it flows like a fluid.  Pastes typically consist of a suspension of granular material in a background fluid.  Pastes are distinct from gels, whose particles interconnect.</rdfs:comment>
    </owl:Class>
    


    <!-- http://www.nist.gov/itl/ssd/Materials#Perfluoropolyether -->

    <owl:Class rdf:about="&mat;Perfluoropolyether">
        <rdfs:subClassOf rdf:resource="&mat;FluidLubricant"/>
        <owl:disjointWith rdf:resource="&mat;Polyalphaolefin"/>
        <owl:disjointWith rdf:resource="&mat;Polyglycol"/>
        <owl:disjointWith rdf:resource="&mat;PolyphenyletherBaseLubricant"/>
        <owl:disjointWith rdf:resource="&mat;Quenchant"/>
        <owl:disjointWith rdf:resource="&mat;SiliconeBaseLubricant"/>
        <owl:disjointWith rdf:resource="&mat;SiliconeGellant"/>
        <owl:disjointWith rdf:resource="&mat;SyntheticEtherBase"/>
        <owl:disjointWith rdf:resource="&mat;UreaGellant"/>
        <owl:disjointWith rdf:resource="&mat;WhiteMineralOil"/>
        <owl:disjointWith rdf:resource="&mat;ZincOxideLubricant"/>
        <or:referenceURL rdf:datatype="&xsd;anyURI">http://www.matweb.com/index.aspx</or:referenceURL>
        <or:termString xml:lang="en">PFPE</or:termString>
        <or:termString xml:lang="en">perfluoropolyether</or:termString>
    </owl:Class>
    


    <!-- http://www.nist.gov/itl/ssd/Materials#PeritecticAlloy -->

    <owl:Class rdf:about="&mat;PeritecticAlloy">
        <rdfs:subClassOf rdf:resource="&mat;EngineeredAlloy"/>
        <rdfs:comment xml:lang="en">A Peritectic Alloy is an alloy that has a specific ratio of component metals that solidifies (through a Pertectic Reaction) from a mixture of liquid and solid of a different crystalline structure.</rdfs:comment>
    </owl:Class>
    


    <!-- http://www.nist.gov/itl/ssd/Materials#PeritecticDecomposition -->

    <owl:Class rdf:about="&mat;PeritecticDecomposition">
        <rdfs:subClassOf rdf:resource="&mat;OrderDisorderPhaseTransformation"/>
        <owl:disjointWith rdf:resource="&mat;Vaporization"/>
        <rdfs:comment xml:lang="en">In Peritectic Decomposition a solid compound decomposes into another solid compound and a liquid.</rdfs:comment>
    </owl:Class>
    


    <!-- http://www.nist.gov/itl/ssd/Materials#PeritecticReaction -->

    <owl:Class rdf:about="&mat;PeritecticReaction">
        <rdfs:subClassOf rdf:resource="&mat;Solidification"/>
        <owl:disjointWith rdf:resource="&mat;SublimatingToSolid"/>
        <rdfs:comment xml:lang="en">A Peritectic Reaction is a Phase Change of a mixture of liquid and solid of a one crystalline structure solidifying into a solid with a different crystalline structure and a fixed ratio of constituant metals.  The resulting solid is a PeritecticAlloy.</rdfs:comment>
    </owl:Class>
    


    <!-- http://www.nist.gov/itl/ssd/Materials#PermanentMagnet -->

    <owl:Class rdf:about="&mat;PermanentMagnet">
        <rdfs:subClassOf rdf:resource="&mat;Ceramic"/>
        <owl:disjointWith rdf:resource="&mat;Piezoceramic"/>
    </owl:Class>
    


    <!-- http://www.nist.gov/itl/ssd/Materials#PhaseChange -->

    <owl:Class rdf:about="&mat;PhaseChange">
        <rdfs:subClassOf rdf:resource="&or;MechanicalProcess"/>
        <owl:disjointWith rdf:resource="&mat;ThermalExpansion"/>
        <rdfs:comment xml:lang="en">A Phase Change or phase transformation is a change in the Material Phase of an object.</rdfs:comment>
    </owl:Class>
    


    <!-- http://www.nist.gov/itl/ssd/Materials#PhosphateMineral -->

    <owl:Class rdf:about="&mat;PhosphateMineral">
        <rdfs:subClassOf rdf:resource="&mat;Mineral"/>
    </owl:Class>
    


    <!-- http://www.nist.gov/itl/ssd/Materials#PhosphideBasedCeramic -->

    <owl:Class rdf:about="&mat;PhosphideBasedCeramic">
        <rdfs:subClassOf rdf:resource="&mat;PnictideCeramic"/>
        <or:referenceURL rdf:datatype="&xsd;anyURI">http://www.matweb.com/index.aspx</or:referenceURL>
        <or:termString xml:lang="en">phosphide</or:termString>
        <or:termString xml:lang="en">phosphide ceramic</or:termString>
        <or:termString xml:lang="en">phosphide-based ceramic</or:termString>
    </owl:Class>
    


    <!-- http://www.nist.gov/itl/ssd/Materials#PhysicalMixture -->

    <owl:Class rdf:about="&mat;PhysicalMixture">
        <rdfs:subClassOf rdf:resource="&bc;MaterialSubstance"/>
        <owl:disjointWith rdf:resource="&mat;PureSubstance"/>
        <owl:disjointWith rdf:resource="&mat;Vacuum"/>
        <or:referenceURL rdf:datatype="&xsd;anyURI">http://www.iupac.org/namespaces/ThermoML#MulticomponentSubstance</or:referenceURL>
        <rdfs:comment xml:lang="en">A Physical Mixture is a material made up by two or more different substances which are mixed but are not combined chemically.  In the physical combination, the identities of the constituant substances are retained.  Types of mixture include alloys, solutions, suspensions, and colloids.</rdfs:comment>
    </owl:Class>
    


    <!-- http://www.nist.gov/itl/ssd/Materials#Piezoceramic -->

    <owl:Class rdf:about="&mat;Piezoceramic">
        <rdfs:subClassOf rdf:resource="&mat;Ceramic"/>
        <rdfs:subClassOf rdf:resource="&mat;EngineeredMaterial"/>
        <or:referenceURL rdf:datatype="&xsd;anyURI">http://www.matweb.com/index.aspx</or:referenceURL>
        <rdfs:comment xml:lang="en">piezoceramic</rdfs:comment>
        <rdfs:comment xml:lang="en">piezoceramic material</rdfs:comment>
        <rdfs:comment xml:lang="en">piezoelectric ceramic</rdfs:comment>
    </owl:Class>
    


    <!-- http://www.nist.gov/itl/ssd/Materials#PipeDiffusion -->

    <owl:Class rdf:about="&mat;PipeDiffusion">
        <rdfs:subClassOf rdf:resource="&mat;ShortCircuitDiffusion"/>
        <rdfs:seeAlso xml:lang="en">Definitions of terms for diffusion in the solid state (IUPAC Recommendations 1999), Pure Appl. Chem. 71, 1307-1325.</rdfs:seeAlso>
        <rdfs:comment xml:lang="en">Pipe Diffusion is diffusion which takes place along a dislocation line.</rdfs:comment>
    </owl:Class>
    


    <!-- http://www.nist.gov/itl/ssd/Materials#Plywood -->

    <owl:Class rdf:about="&mat;Plywood">
        <rdfs:subClassOf rdf:resource="&mat;SandwichComposite"/>
        <rdfs:subClassOf rdf:resource="&mat;Wood"/>
        <rdfs:comment xml:lang="en">Plywood is a manufactured wood panel Sadwich Composite of thin sheets of Wood.</rdfs:comment>
    </owl:Class>
    


    <!-- http://www.nist.gov/itl/ssd/Materials#PnictideCeramic -->

    <owl:Class rdf:about="&mat;PnictideCeramic">
        <rdfs:subClassOf rdf:resource="&mat;Ceramic"/>
        <or:referenceURL rdf:datatype="&xsd;anyURI">http://www.matweb.com/index.aspx</or:referenceURL>
        <rdfs:comment xml:lang="en">The pnictogens are the chemical elements in group 15 ( VB or VA) of the periodic table. This group is also known as the nitrogen family. It consists of the elements nitrogen (N), phosphorus (P), arsenic (As), antimony (Sb), bismuth (Bi).  Pnictides are binary compounds formed from this chemical group.</rdfs:comment>
        <or:termString xml:lang="en">pnictide</or:termString>
        <or:termString xml:lang="en">pnictide ceramic</or:termString>
    </owl:Class>
    


    <!-- http://www.nist.gov/itl/ssd/Materials#Polyacrylate -->

    <owl:Class rdf:about="&mat;Polyacrylate">
        <rdfs:subClassOf rdf:resource="&mat;Thermoplastic"/>
        <rdfs:comment xml:lang="en">Polyacrylates (`acrylate polymers&#39; or `acrylics&#39;) are polymers  polymers are based on the structure of acrylic acid, which consists of a vinyl group and a carboxylic acid terminus.</rdfs:comment>
    </owl:Class>
    


    <!-- http://www.nist.gov/itl/ssd/Materials#Polyacrylonitrile -->

    <owl:Class rdf:about="&mat;Polyacrylonitrile">
        <rdfs:subClassOf rdf:resource="&mat;VinylPolymer"/>
        <owl:disjointWith rdf:resource="&mat;Polybutadiene"/>
        <owl:disjointWith rdf:resource="&mat;Polyethylene"/>
        <owl:disjointWith rdf:resource="&mat;Polypropylene"/>
        <owl:disjointWith rdf:resource="&mat;Polystyrene"/>
        <owl:disjointWith rdf:resource="&mat;PolyvinylAcetate"/>
        <owl:disjointWith rdf:resource="&mat;PolyvinylAlcohol"/>
        <owl:disjointWith rdf:resource="&mat;PolyvinylChloride"/>
        <rdfs:comment xml:lang="en">Polyacrylonitrile is made by polymerization of the monomer acrylonitrile.</rdfs:comment>
    </owl:Class>
    


    <!-- http://www.nist.gov/itl/ssd/Materials#Polyalphaolefin -->

    <owl:Class rdf:about="&mat;Polyalphaolefin">
        <rdfs:subClassOf rdf:resource="&mat;FluidLubricant"/>
        <owl:disjointWith rdf:resource="&mat;Polyglycol"/>
        <owl:disjointWith rdf:resource="&mat;PolyphenyletherBaseLubricant"/>
        <owl:disjointWith rdf:resource="&mat;Quenchant"/>
        <owl:disjointWith rdf:resource="&mat;SiliconeBaseLubricant"/>
        <owl:disjointWith rdf:resource="&mat;SiliconeGellant"/>
        <owl:disjointWith rdf:resource="&mat;SyntheticEtherBase"/>
        <owl:disjointWith rdf:resource="&mat;UreaGellant"/>
        <owl:disjointWith rdf:resource="&mat;WhiteMineralOil"/>
        <owl:disjointWith rdf:resource="&mat;ZincOxideLubricant"/>
        <or:referenceURL rdf:datatype="&xsd;anyURI">http://www.matweb.com/index.aspx</or:referenceURL>
        <or:termString xml:lang="en">PAO</or:termString>
        <or:termString xml:lang="en">polyalphaolefin</or:termString>
    </owl:Class>
    


    <!-- http://www.nist.gov/itl/ssd/Materials#Polybutadiene -->

    <owl:Class rdf:about="&mat;Polybutadiene">
        <rdfs:subClassOf rdf:resource="&mat;VinylPolymer"/>
        <owl:disjointWith rdf:resource="&mat;Polyethylene"/>
        <owl:disjointWith rdf:resource="&mat;Polypropylene"/>
        <owl:disjointWith rdf:resource="&mat;Polystyrene"/>
        <owl:disjointWith rdf:resource="&mat;PolyvinylAcetate"/>
        <owl:disjointWith rdf:resource="&mat;PolyvinylAlcohol"/>
        <owl:disjointWith rdf:resource="&mat;PolyvinylChloride"/>
        <rdfs:comment xml:lang="en">Polybutadiene is a synthetic rubber that is a polymer formed from the polymerization process of the monomer 1,3-butadiene.</rdfs:comment>
    </owl:Class>
    


    <!-- http://www.nist.gov/itl/ssd/Materials#Polybutylene -->

    <owl:Class rdf:about="&mat;Polybutylene">
        <rdfs:subClassOf rdf:resource="&mat;Polyolefin"/>
        <owl:disjointWith rdf:resource="&mat;Polymethylpentene"/>
        <owl:disjointWith rdf:resource="&mat;VinylPolymer"/>
        <rdfs:comment xml:lang="en">Polybutylene (polybutene-1, poly(1-butene), PB-1) is a polyolefin or saturated polymer with the chemical formula (C4H8)n</rdfs:comment>
    </owl:Class>
    


    <!-- http://www.nist.gov/itl/ssd/Materials#PolycrystallineMaterial -->

    <owl:Class rdf:about="&mat;PolycrystallineMaterial">
        <rdfs:subClassOf rdf:resource="&mat;SolidCrystallineSubstance"/>
        <owl:disjointWith rdf:resource="&mat;SingleCrystallineMaterial"/>
        <rdfs:comment xml:lang="en">Polycrystalline material is solid material made up of multiple crystals.</rdfs:comment>
    </owl:Class>
    


    <!-- http://www.nist.gov/itl/ssd/Materials#Polyester -->

    <owl:Class rdf:about="&mat;Polyester">
        <rdfs:subClassOf rdf:resource="&mat;PolymerSubstance"/>
        <owl:disjointWith rdf:resource="&mat;Polyolefin"/>
        <owl:disjointWith rdf:resource="&mat;VinylPolymer"/>
        <rdfs:comment xml:lang="en">Polyester is a category of polymers which contain the ester functional group in their main chain. Although there are many polyesters, the term &quot;polyester&quot; as a specific material most commonly refers to polyethylene terephthalate (PET). Polyesters include naturally occurring chemicals, such as in the cutin of plant cuticles, as well as synthetics through step-growth polymerization such as polycarbonate and polybutyrate. Natural polyesters and a few synthetic ones are biodegradable, but most synthetic polyesters are not.

Depending on the chemical structure, polyester can be a thermoplastic or thermoset; however, the most common polyesters are thermoplastics.</rdfs:comment>
        <or:termString xml:lang="en">polyester</or:termString>
    </owl:Class>
    


    <!-- http://www.nist.gov/itl/ssd/Materials#Polyester-TP -->

    <owl:Class rdf:about="&mat;Polyester-TP">
        <rdfs:subClassOf rdf:resource="&mat;Polyester"/>
        <rdfs:subClassOf rdf:resource="&mat;Thermoplastic"/>
        <or:referenceURL rdf:datatype="&xsd;anyURI">http://www.matweb.com/index.aspx</or:referenceURL>
        <or:termString xml:lang="en">polyester, TP</or:termString>
        <or:termString xml:lang="en">thermoplastic polyester</or:termString>
    </owl:Class>
    


    <!-- http://www.nist.gov/itl/ssd/Materials#Polyester-TS -->

    <owl:Class rdf:about="&mat;Polyester-TS">
        <rdfs:subClassOf rdf:resource="&mat;Polyester"/>
        <rdfs:subClassOf rdf:resource="&mat;Thermoset"/>
        <or:referenceURL rdf:datatype="&xsd;anyURI">http://www.matweb.com/index.aspx</or:referenceURL>
        <or:termString xml:lang="en">polyester, TS</or:termString>
        <or:termString xml:lang="en">thermosetting polyester</or:termString>
    </owl:Class>
    


    <!-- http://www.nist.gov/itl/ssd/Materials#Polyethylene -->

    <owl:Class rdf:about="&mat;Polyethylene">
        <rdfs:subClassOf rdf:resource="&mat;Polyolefin"/>
        <rdfs:subClassOf rdf:resource="&mat;VinylPolymer"/>
        <owl:disjointWith rdf:resource="&mat;Polypropylene"/>
        <owl:disjointWith rdf:resource="&mat;Polystyrene"/>
        <owl:disjointWith rdf:resource="&mat;PolyvinylAcetate"/>
        <owl:disjointWith rdf:resource="&mat;PolyvinylAlcohol"/>
        <owl:disjointWith rdf:resource="&mat;PolyvinylChloride"/>
        <or:referenceURL rdf:datatype="&xsd;anyURI"></or:referenceURL>
        <rdfs:comment xml:lang="en">Polyethylene (abbreviated PE) or polythene (IUPAC name polyethene or poly(methylene)) is  made by polymerization of ethene. Many kinds of polyethylene are known, but they almost always have the chemical formula (C2H4)nH2.</rdfs:comment>
    </owl:Class>
    


    <!-- http://www.nist.gov/itl/ssd/Materials#Polyglycol -->

    <owl:Class rdf:about="&mat;Polyglycol">
        <rdfs:subClassOf rdf:resource="&mat;FluidLubricant"/>
        <owl:disjointWith rdf:resource="&mat;PolyphenyletherBaseLubricant"/>
        <owl:disjointWith rdf:resource="&mat;Quenchant"/>
        <owl:disjointWith rdf:resource="&mat;SiliconeBaseLubricant"/>
        <owl:disjointWith rdf:resource="&mat;SiliconeGellant"/>
        <owl:disjointWith rdf:resource="&mat;SyntheticEtherBase"/>
        <owl:disjointWith rdf:resource="&mat;UreaGellant"/>
        <owl:disjointWith rdf:resource="&mat;WhiteMineralOil"/>
        <owl:disjointWith rdf:resource="&mat;ZincOxideLubricant"/>
        <or:referenceURL rdf:datatype="&xsd;anyURI">http://www.matweb.com/index.aspx</or:referenceURL>
        <or:termString xml:lang="en">polyglycol</or:termString>
    </owl:Class>
    


    <!-- http://www.nist.gov/itl/ssd/Materials#PolymerMetalInteraction -->

    <owl:Class rdf:about="&mat;PolymerMetalInteraction">
        <rdfs:subClassOf rdf:resource="&bc;ChemicalProcess"/>
        <rdfs:subClassOf>
            <owl:Restriction>
                <owl:onProperty rdf:resource="&or;objectActedOn"/>
                <owl:someValuesFrom rdf:resource="&bc;Metal"/>
            </owl:Restriction>
        </rdfs:subClassOf>
        <rdfs:subClassOf>
            <owl:Restriction>
                <owl:onProperty rdf:resource="&or;objectActedOn"/>
                <owl:someValuesFrom rdf:resource="&mat;PolymerSubstance"/>
            </owl:Restriction>
        </rdfs:subClassOf>
        <rdfs:comment xml:lang="en">A Polymer-Metal Interaction is a Chemical Process in which a Polymer and metallic particles interact.</rdfs:comment>
    </owl:Class>
    


    <!-- http://www.nist.gov/itl/ssd/Materials#PolymerSubstance -->

    <owl:Class rdf:about="&mat;PolymerSubstance">
        <rdfs:subClassOf rdf:resource="&bc;MaterialSubstance"/>
    </owl:Class>
    


    <!-- http://www.nist.gov/itl/ssd/Materials#PolymericMicrostructure -->

    <owl:Class rdf:about="&mat;PolymericMicrostructure">
        <rdfs:subClassOf rdf:resource="&mat;Microstructure"/>
        <rdfs:comment xml:lang="en">Polymeric Microstructure is a non-crystalline material Microstructure of a substance composed of polymers.</rdfs:comment>
    </owl:Class>
    


    <!-- http://www.nist.gov/itl/ssd/Materials#Polymethylpentene -->

    <owl:Class rdf:about="&mat;Polymethylpentene">
        <rdfs:subClassOf rdf:resource="&mat;Polyolefin"/>
        <owl:disjointWith rdf:resource="&mat;VinylPolymer"/>
        <or:referenceURL rdf:datatype="&xsd;anyURI">http://www.matweb.com/index.aspx</or:referenceURL>
        <rdfs:comment xml:lang="en">Polymethylpentene (PMP) is a thermoplastic polymer of methylpentene monomer units.</rdfs:comment>
    </owl:Class>
    


    <!-- http://www.nist.gov/itl/ssd/Materials#Polyolefin -->

    <owl:Class rdf:about="&mat;Polyolefin">
        <rdfs:subClassOf rdf:resource="&mat;Thermoplastic"/>
        <or:referenceURL rdf:datatype="&xsd;anyURI">http://www.matweb.com/index.aspx</or:referenceURL>
        <rdfs:comment xml:lang="en">A polyolefin (or polyalkene) is a polymer produced from a simple olefin (or ``alkene&#39;&#39; with the general formula CnH2n) as a monomer.</rdfs:comment>
    </owl:Class>
    


    <!-- http://www.nist.gov/itl/ssd/Materials#PolyphenyletherBaseLubricant -->

    <owl:Class rdf:about="&mat;PolyphenyletherBaseLubricant">
        <rdfs:subClassOf rdf:resource="&mat;FluidLubricant"/>
        <owl:disjointWith rdf:resource="&mat;Quenchant"/>
        <owl:disjointWith rdf:resource="&mat;SiliconeBaseLubricant"/>
        <owl:disjointWith rdf:resource="&mat;SiliconeGellant"/>
        <owl:disjointWith rdf:resource="&mat;SyntheticEtherBase"/>
        <owl:disjointWith rdf:resource="&mat;UreaGellant"/>
        <owl:disjointWith rdf:resource="&mat;WhiteMineralOil"/>
        <owl:disjointWith rdf:resource="&mat;ZincOxideLubricant"/>
        <or:referenceURL rdf:datatype="&xsd;anyURI">http://www.matweb.com/index.aspx</or:referenceURL>
        <or:termString xml:lang="en">PPE base</or:termString>
        <or:termString xml:lang="en">PPE base lubricant</or:termString>
        <or:termString xml:lang="en">polyphenylether base</or:termString>
        <or:termString xml:lang="en">polyphenylether base lubricant</or:termString>
    </owl:Class>
    


    <!-- http://www.nist.gov/itl/ssd/Materials#Polypropylene -->

    <owl:Class rdf:about="&mat;Polypropylene">
        <rdfs:subClassOf rdf:resource="&mat;Polyolefin"/>
        <rdfs:subClassOf rdf:resource="&mat;VinylPolymer"/>
        <owl:disjointWith rdf:resource="&mat;Polystyrene"/>
        <owl:disjointWith rdf:resource="&mat;PolyvinylAcetate"/>
        <owl:disjointWith rdf:resource="&mat;PolyvinylAlcohol"/>
        <owl:disjointWith rdf:resource="&mat;PolyvinylChloride"/>
        <or:referenceURL rdf:datatype="&xsd;anyURI">http://www.matweb.com/index.aspx</or:referenceURL>
        <or:termString xml:lang="en">PP</or:termString>
        <rdfs:comment xml:lang="en">Polypropylene (PP), also known as polypropene, is a thermoplastic polymer from the monomer propylene.</rdfs:comment>
        <or:termString xml:lang="en">polypropylene</or:termString>
    </owl:Class>
    


    <!-- http://www.nist.gov/itl/ssd/Materials#Polystyrene -->

    <owl:Class rdf:about="&mat;Polystyrene">
        <rdfs:subClassOf rdf:resource="&mat;VinylPolymer"/>
        <owl:disjointWith rdf:resource="&mat;PolyvinylAcetate"/>
        <owl:disjointWith rdf:resource="&mat;PolyvinylAlcohol"/>
        <owl:disjointWith rdf:resource="&mat;PolyvinylChloride"/>
        <or:referenceURL rdf:datatype="&xsd;anyURI">http://www.matweb.com/index.aspx</or:referenceURL>
        <or:termString xml:lang="en">PS</or:termString>
        <rdfs:comment xml:lang="en">Polystyrene is made from styrene or &#39;vinyl benzene&#39;.</rdfs:comment>
        <or:termString xml:lang="en">polystyrene</or:termString>
    </owl:Class>
    


    <!-- http://www.nist.gov/itl/ssd/Materials#PolyvinylAcetate -->

    <owl:Class rdf:about="&mat;PolyvinylAcetate">
        <rdfs:subClassOf rdf:resource="&mat;VinylPolymer"/>
        <owl:disjointWith rdf:resource="&mat;PolyvinylAlcohol"/>
        <owl:disjointWith rdf:resource="&mat;PolyvinylChloride"/>
        <rdfs:comment xml:lang="en">Polyvinyl acetate (PVAc) is made by polymerization of vinyl acetate.</rdfs:comment>
    </owl:Class>
    


    <!-- http://www.nist.gov/itl/ssd/Materials#PolyvinylAlcohol -->

    <owl:Class rdf:about="&mat;PolyvinylAlcohol">
        <rdfs:subClassOf rdf:resource="&mat;VinylPolymer"/>
        <owl:disjointWith rdf:resource="&mat;PolyvinylChloride"/>
        <rdfs:comment xml:lang="en">Polyvinyl alcohol (PVA) is produced by hydrolysis of polyvinyl acetate.</rdfs:comment>
    </owl:Class>
    


    <!-- http://www.nist.gov/itl/ssd/Materials#PolyvinylChloride -->

    <owl:Class rdf:about="&mat;PolyvinylChloride">
        <rdfs:subClassOf rdf:resource="&mat;VinylPolymer"/>
        <or:referenceURL rdf:datatype="&xsd;anyURI">http://www.matweb.com/index.aspx</or:referenceURL>
        <or:termString xml:lang="en">PVC</or:termString>
        <rdfs:comment xml:lang="en">Polyvinyl chloride (PVC) is made by polymerization of the monomer vinyl chloride (chloroethene) CH2=CHCl</rdfs:comment>
        <or:termString xml:lang="en">polyvynl chloride</or:termString>
        <or:termString xml:lang="en">vinyl</or:termString>
    </owl:Class>
    


    <!-- http://www.nist.gov/itl/ssd/Materials#PowderySubstance -->

    <owl:Class rdf:about="&mat;PowderySubstance">
        <rdfs:subClassOf rdf:resource="&mat;SolidSubstance"/>
        <rdfs:comment xml:lang="en">material in a solid powdery phase</rdfs:comment>
    </owl:Class>
    


    <!-- http://www.nist.gov/itl/ssd/Materials#Power -->

    <owl:Class rdf:about="&mat;Power">
        <owl:equivalentClass>
            <owl:Class>
                <owl:intersectionOf rdf:parseType="Collection">
                    <rdf:Description rdf:about="&or;MeasurableQuantity"/>
                    <owl:Restriction>
                        <owl:onProperty rdf:resource="&or;unitsFor"/>
                        <owl:someValuesFrom rdf:resource="&mat;UnitOfPower"/>
                    </owl:Restriction>
                </owl:intersectionOf>
            </owl:Class>
        </owl:equivalentClass>
        <rdfs:subClassOf rdf:resource="&or;MeasurableQuantity"/>
        <rdfs:subClassOf>
            <owl:Restriction>
                <owl:onProperty rdf:resource="&or;unitsFor"/>
                <owl:allValuesFrom rdf:resource="&mat;UnitOfPower"/>
            </owl:Restriction>
        </rdfs:subClassOf>
    </owl:Class>
    


    <!-- http://www.nist.gov/itl/ssd/Materials#PrecipitationFromSolution -->

    <owl:Class rdf:about="&mat;PrecipitationFromSolution">
        <rdfs:subClassOf rdf:resource="&mat;DiffusionalPhaseTransformation"/>
        <owl:disjointWith rdf:resource="&mat;SolidToSolidPhaseTransformation"/>
        <owl:disjointWith rdf:resource="&mat;Solidification"/>
        <owl:disjointWith rdf:resource="&mat;Vaporization"/>
    </owl:Class>
    


    <!-- http://www.nist.gov/itl/ssd/Materials#PrecipitationHardeningStainlessSteel -->

    <owl:Class rdf:about="&mat;PrecipitationHardeningStainlessSteel">
        <rdfs:subClassOf rdf:resource="&mat;StainlessSteel"/>
        <or:referenceURL rdf:datatype="&xsd;anyURI">http://www.matweb.com/index.aspx</or:referenceURL>
        <or:termString xml:lang="en">precipitation hardening stainless</or:termString>
        <or:termString xml:lang="en">precipitation hardening stainless steel</or:termString>
    </owl:Class>
    


    <!-- http://www.nist.gov/itl/ssd/Materials#PressureDependentProperty -->

    <owl:Class rdf:about="&mat;PressureDependentProperty">
        <rdfs:subClassOf rdf:resource="&or;MaterialProperty"/>
        <rdfs:comment xml:lang="en">A Pressure Dependent Property is one whose value depends upon the ambient pressure, such as a liquid&#39;s boiling point.</rdfs:comment>
    </owl:Class>
    


    <!-- http://www.nist.gov/itl/ssd/Materials#PressureVesselSteel -->

    <owl:Class rdf:about="&mat;PressureVesselSteel">
        <rdfs:subClassOf rdf:resource="&mat;Steel"/>
        <or:referenceURL rdf:datatype="&xsd;anyURI">http://www.matweb.com/index.aspx</or:referenceURL>
        <or:termString xml:lang="en">pressure vessel steel</or:termString>
    </owl:Class>
    


    <!-- http://www.nist.gov/itl/ssd/Materials#PureSubstance -->

    <owl:Class rdf:about="&mat;PureSubstance">
        <rdfs:subClassOf rdf:resource="&bc;ChemicalSubstance"/>
        <rdfs:comment xml:lang="en">A Pure Substance is a substance made up of a single form of molecule, or in the case of a metal, a single type of atom.  This does not not mean that there may not be impurities.</rdfs:comment>
    </owl:Class>
    


    <!-- http://www.nist.gov/itl/ssd/Materials#Quartz -->

    <owl:Class rdf:about="&mat;Quartz">
        <rdfs:subClassOf rdf:resource="&mat;Silicate"/>
        <rdfs:comment xml:lang="en">Quartz is a common mineral of SiO4 with a hexagonal crystalline structure.  Impurities may color this otherwise colorless mineral.</rdfs:comment>
    </owl:Class>
    


    <!-- http://www.nist.gov/itl/ssd/Materials#QuasimartensiticPhaseTranformation -->

    <owl:Class rdf:about="&mat;QuasimartensiticPhaseTranformation">
        <rdfs:subClassOf rdf:resource="&mat;DeviatonicDominantPhaseTransformation"/>
        <rdfs:comment xml:lang="en">Shear dominated transformations can be classified according to the magnitude of the strain energies involved compared to the innate vibrations of the atoms in the lattice and hence whether the strain energies have a notable influence on the kinetics of the transformation and the morphology of the resulting phase. If the strain energy is a significant factor then the transformations are dubbed martensitic and if it is not the transformation is referred to as quasi-martensitic.</rdfs:comment>
    </owl:Class>
    


    <!-- http://www.nist.gov/itl/ssd/Materials#Quenchant -->

    <owl:Class rdf:about="&mat;Quenchant">
        <rdfs:subClassOf rdf:resource="&mat;FluidLubricant"/>
        <owl:disjointWith rdf:resource="&mat;SiliconeBaseLubricant"/>
        <owl:disjointWith rdf:resource="&mat;SiliconeGellant"/>
        <owl:disjointWith rdf:resource="&mat;SyntheticEtherBase"/>
        <owl:disjointWith rdf:resource="&mat;UreaGellant"/>
        <owl:disjointWith rdf:resource="&mat;WhiteMineralOil"/>
        <owl:disjointWith rdf:resource="&mat;ZincOxideLubricant"/>
        <or:referenceURL rdf:datatype="&xsd;anyURI">http://www.matweb.com/index.aspx</or:referenceURL>
        <or:termString xml:lang="en">quenchant</or:termString>
    </owl:Class>
    


    <!-- http://www.nist.gov/itl/ssd/Materials#RadioactiveMaterial -->

    <owl:Class rdf:about="&mat;RadioactiveMaterial">
        <rdfs:subClassOf rdf:resource="&bc;MaterialSubstance"/>
        <owl:disjointWith rdf:resource="&mat;Vacuum"/>
        <rdfs:comment xml:lang="en">The class of all material that is radioactive.</rdfs:comment>
    </owl:Class>
    


    <!-- http://www.nist.gov/itl/ssd/Materials#Radioisotope -->

    <owl:Class rdf:about="&mat;Radioisotope">
        <rdfs:subClassOf rdf:resource="&bc;Isotope"/>
        <owl:disjointWith rdf:resource="&mat;StableIsotope"/>
        <rdfs:comment xml:lang="en">A Radioisotope is an Isotope that is a subclass of Radioactive Material.</rdfs:comment>
    </owl:Class>
    


    <!-- http://www.nist.gov/itl/ssd/Materials#RadiologicalProperty -->

    <owl:Class rdf:about="&mat;RadiologicalProperty">
        <rdfs:subClassOf rdf:resource="&or;MeasurableMaterialProperty"/>
        <owl:disjointWith rdf:resource="&mat;ThermalProperty"/>
    </owl:Class>
    


    <!-- http://www.nist.gov/itl/ssd/Materials#ReinforcedPlastic -->

    <owl:Class rdf:about="&mat;ReinforcedPlastic">
        <rdfs:subClassOf rdf:resource="&mat;CompositeMaterial"/>
        <rdfs:subClassOf rdf:resource="&mat;EngineeredMaterial"/>
        <rdfs:subClassOf rdf:resource="&mat;PolymerSubstance"/>
        <rdfs:comment xml:lang="en">A Fibre-reinforced plastic (FRP) (also fibre-reinforced polymer) is a composite material made of a polymer matrix reinforced with fibres. The fibres may be glass, carbon, aramid, paper, wood, or asbestos. The polymer may be an epoxy, vinylester, polyester thermosetting plastic, or phenol formaldehyde resin.</rdfs:comment>
    </owl:Class>
    


    <!-- http://www.nist.gov/itl/ssd/Materials#RelaxationMethodForDiffusion -->

    <owl:Class rdf:about="&mat;RelaxationMethodForDiffusion">
        <rdfs:subClassOf rdf:resource="&mat;VacancyDiffusionMechanism"/>
        <rdfs:seeAlso xml:lang="en">Definitions of terms for diffusion in the solid state (IUPAC Recommendations 1999), Pure Appl. Chem. 71, 1307-1325.</rdfs:seeAlso>
        <rdfs:comment xml:lang="en">In the Relaxation Mechanism for diffusion, the atoms close to a vacancy relax to such an extent that the regular lattice structure out to several atom distances disappears and diffusion occurs by an irregular jostling motion similar to that for atoms in a liquid.</rdfs:comment>
    </owl:Class>
    


    <!-- http://www.nist.gov/itl/ssd/Materials#ReneAlloy -->

    <owl:Class rdf:about="&mat;ReneAlloy">
        <rdfs:subClassOf rdf:resource="&mat;NickelAlloy"/>
        <rdfs:subClassOf rdf:resource="&mat;Superalloy"/>
        <rdfs:comment xml:lang="en"> Rene Alloys are Superalloys developed by General Electric.</rdfs:comment>
    </owl:Class>
    


    <!-- http://www.nist.gov/itl/ssd/Materials#RheologicalProperty -->

    <owl:Class rdf:about="&mat;RheologicalProperty">
        <rdfs:subClassOf rdf:resource="&mat;MeasurableMechanicalProperty"/>
        <rdfs:comment xml:lang="en">Rheological Properties are the quantitative and qualitative relationships between deformations and stresses of a material.  Such properties include shear stress, viscosity, linear viscoelastic properties, and elongational properties.</rdfs:comment>
    </owl:Class>
    


    <!-- http://www.nist.gov/itl/ssd/Materials#RhombohedralCrystalStructure -->

    <owl:Class rdf:about="&mat;RhombohedralCrystalStructure">
        <rdfs:subClassOf rdf:resource="&mat;TrigonalCrystalStructure"/>
        <rdfs:comment xml:lang="en">A lattice system is described by three basis vectors. In the rhombohedral system, the crystal is described by vectors of equal length, no two of which are orthogonal. The rhombohedral system can be thought of as the cubic system stretched along a body diagonal. a = b = c; α = β = γ ≠ 90°. In some classification schemes, the rhombohedral lattice system is combined with the hexagonal lattice system and grouped into a larger hexagonal family.

There is only one rhombohedral Bravais lattice.</rdfs:comment>
    </owl:Class>
    


    <!-- http://www.nist.gov/itl/ssd/Materials#RingMechanismForDiffusion -->

    <owl:Class rdf:about="&mat;RingMechanismForDiffusion">
        <rdfs:subClassOf rdf:resource="&mat;MicroscopicDiffusionMovement"/>
        <rdfs:comment xml:lang="en">The Ring Mechanism for Diffusion is a variation of the exchange mechanism in which a group of atoms moves around in a circular fashion, each atom in the group taking the place of its neighbour in the direction of motion.</rdfs:comment>
        <or:termString xml:lang="en">ring mechanism</or:termString>
        <or:termString xml:lang="en">ring mechanism for diffusion</or:termString>
    </owl:Class>
    


    <!-- http://www.nist.gov/itl/ssd/Materials#SandwichComposite -->

    <owl:Class rdf:about="&mat;SandwichComposite">
        <rdfs:subClassOf rdf:resource="&mat;CompositeMaterial"/>
        <rdfs:subClassOf rdf:resource="&mat;EngineeredMaterial"/>
    </owl:Class>
    


    <!-- http://www.nist.gov/itl/ssd/Materials#ScratchHardness -->

    <owl:Class rdf:about="&mat;ScratchHardness">
        <rdfs:subClassOf rdf:resource="&mat;Hardness"/>
        <rdfs:comment xml:lang="en">Scratch hardness is the measure of how resistant a sample is to fracture or permanent plastic deformation due to friction from a sharp object.</rdfs:comment>
    </owl:Class>
    


    <!-- http://www.nist.gov/itl/ssd/Materials#SelfDiffusion -->

    <owl:Class rdf:about="&mat;SelfDiffusion">
        <rdfs:subClassOf rdf:resource="&mat;SolidDiffusion"/>
        <rdfs:seeAlso xml:lang="en">Definitions of terms for diffusion in the solid state (IUPAC Recommendations 1999), Pure Appl. Chem. 71, 1307-1325.</rdfs:seeAlso>
        <rdfs:comment xml:lang="en">Self-diffusion is diffusion which takes place in the absence of a chemical potential gradient, describing the uncorrelated movement of a particle.</rdfs:comment>
        <or:termString xml:lang="en">self-diffusion</or:termString>
    </owl:Class>
    


    <!-- http://www.nist.gov/itl/ssd/Materials#Semiconductor -->

    <owl:Class rdf:about="&mat;Semiconductor">
        <rdfs:subClassOf rdf:resource="&bc;MaterialSubstance"/>
        <or:referenceURL rdf:datatype="&xsd;anyURI">http://www.matweb.com/index.aspx</or:referenceURL>
        <rdfs:comment xml:lang="en">A semiconductor has electrical conductivity intermediate between that of a conductor and an insulator.  Semiconductors differ from metals in their characteristic property of decreasing electrical resistivity with increasing temperature.  Common semiconducting materials are crystalline solids, but amorphous and liquid semiconductors are also known</rdfs:comment>
    </owl:Class>
    


    <!-- http://www.nist.gov/itl/ssd/Materials#ShortCircuitDiffusion -->

    <owl:Class rdf:about="&mat;ShortCircuitDiffusion">
        <rdfs:subClassOf rdf:resource="&mat;SolidDiffusion"/>
        <rdfs:seeAlso xml:lang="en">Definitions of terms for diffusion in the solid state (IUPAC Recommendations 1999), Pure Appl. Chem. 71, 1307-1325.</rdfs:seeAlso>
        <rdfs:comment xml:lang="en">Short Circuit Diffusion is a diffusion process occurring via grain boundaries, surfaces, or dislocations.  Short circuit diffusion mechanisms often cause diffusion in polycrystalline materials to proceed more quickly than in single crystals.</rdfs:comment>
    </owl:Class>
    


    <!-- http://www.nist.gov/itl/ssd/Materials#ShufflePhaseTransformation -->

    <owl:Class rdf:about="&mat;ShufflePhaseTransformation">
        <rdfs:subClassOf rdf:resource="&mat;DiffusionlessPhaseTransformation"/>
        <rdfs:comment xml:lang="en">Shuffle transformations involve the small movement of atoms within the unit cell. As a result pure shuffles do not normally result in a shape change of the unit cell - only its symmetry and structure.</rdfs:comment>
    </owl:Class>
    


    <!-- http://www.nist.gov/itl/ssd/Materials#Silicate -->

    <owl:Class rdf:about="&mat;Silicate">
        <rdfs:subClassOf rdf:resource="&mat;Mineral"/>
    </owl:Class>
    


    <!-- http://www.nist.gov/itl/ssd/Materials#SiliconOxide -->

    <owl:Class rdf:about="&mat;SiliconOxide">
        <rdfs:subClassOf rdf:resource="&bc;Oxide"/>
        <owl:disjointWith rdf:resource="&mat;TitaniumOxide"/>
        <owl:disjointWith rdf:resource="&mat;ZirconiumOxide"/>
        <or:referenceURL rdf:datatype="&xsd;anyURI">http://www.matweb.com/index.aspx</or:referenceURL>
        <or:termString xml:lang="en">silicon oxide</or:termString>
    </owl:Class>
    


    <!-- http://www.nist.gov/itl/ssd/Materials#SiliconeBaseLubricant -->

    <owl:Class rdf:about="&mat;SiliconeBaseLubricant">
        <rdfs:subClassOf rdf:resource="&mat;FluidLubricant"/>
        <owl:disjointWith rdf:resource="&mat;SiliconeGellant"/>
        <owl:disjointWith rdf:resource="&mat;SyntheticEtherBase"/>
        <owl:disjointWith rdf:resource="&mat;UreaGellant"/>
        <owl:disjointWith rdf:resource="&mat;WhiteMineralOil"/>
        <owl:disjointWith rdf:resource="&mat;ZincOxideLubricant"/>
        <or:referenceURL rdf:datatype="&xsd;anyURI">http://www.matweb.com/index.aspx</or:referenceURL>
        <or:termString xml:lang="en">silicone base</or:termString>
        <or:termString xml:lang="en">silicone base lubricant</or:termString>
    </owl:Class>
    


    <!-- http://www.nist.gov/itl/ssd/Materials#SiliconeGellant -->

    <owl:Class rdf:about="&mat;SiliconeGellant">
        <rdfs:subClassOf rdf:resource="&mat;FluidLubricant"/>
        <owl:disjointWith rdf:resource="&mat;SyntheticEtherBase"/>
        <owl:disjointWith rdf:resource="&mat;UreaGellant"/>
        <owl:disjointWith rdf:resource="&mat;WhiteMineralOil"/>
        <owl:disjointWith rdf:resource="&mat;ZincOxideLubricant"/>
        <or:referenceURL rdf:datatype="&xsd;anyURI">http://www.matweb.com/index.aspx</or:referenceURL>
        <or:termString xml:lang="en">silicone gellant</or:termString>
    </owl:Class>
    


    <!-- http://www.nist.gov/itl/ssd/Materials#SingleCrystallineMaterial -->

    <owl:Class rdf:about="&mat;SingleCrystallineMaterial">
        <rdfs:subClassOf rdf:resource="&mat;SolidCrystallineSubstance"/>
        <rdfs:comment xml:lang="en">Single Crystalline Material, is material formed from a single crystal.</rdfs:comment>
    </owl:Class>
    


    <!-- http://www.nist.gov/itl/ssd/Materials#SinglePhaseMaterialPortion -->

    <owl:Class rdf:about="&mat;SinglePhaseMaterialPortion">
        <rdfs:subClassOf rdf:resource="&mat;MaterialPortion"/>
        <rdfs:comment xml:lang="en">A Single Phase Material Portion is a portion of an object all of which has the same Material Phase Composition.  For example, it might be the portion of an alloy consisting of all grains of a single metal that have a specific crystalline structure.</rdfs:comment>
    </owl:Class>
    


    <!-- http://www.nist.gov/itl/ssd/Materials#SingleWalledCarbonNanotube -->

    <owl:Class rdf:about="&mat;SingleWalledCarbonNanotube">
        <rdfs:subClassOf rdf:resource="&mat;CarbonNanotube"/>
        <rdfs:comment xml:lang="en">Single Walled Carbon Nanotubes (SWCNTs) are the simplest kind of Carbon Nanotubes -- without any concentric structures. </rdfs:comment>
    </owl:Class>
    


    <!-- http://www.nist.gov/itl/ssd/Materials#Softwood -->

    <owl:Class rdf:about="&mat;Softwood">
        <rdfs:subClassOf rdf:resource="&mat;Wood"/>
        <or:referenceURL rdf:datatype="&xsd;anyURI">http://www.matweb.com/index.aspx</or:referenceURL>
        <or:termString xml:lang="en">softwood</or:termString>
    </owl:Class>
    


    <!-- http://www.nist.gov/itl/ssd/Materials#SolidAerosol -->

    <owl:Class rdf:about="&mat;SolidAerosol">
        <rdfs:subClassOf rdf:resource="&mat;Aerosol"/>
        <rdfs:comment xml:lang="en">A Solid Aerosol is a colloid suspension of fine solid particles in a gas.</rdfs:comment>
    </owl:Class>
    


    <!-- http://www.nist.gov/itl/ssd/Materials#SolidCrystallineSubstance -->

    <owl:Class rdf:about="&mat;SolidCrystallineSubstance">
        <rdfs:subClassOf rdf:resource="&mat;CrystallineSubstance"/>
        <rdfs:subClassOf rdf:resource="&mat;SolidSubstance"/>
    </owl:Class>
    


    <!-- http://www.nist.gov/itl/ssd/Materials#SolidDiffusion -->

    <owl:Class rdf:about="&mat;SolidDiffusion">
        <rdfs:subClassOf rdf:resource="&mat;Diffusion"/>
    </owl:Class>
    


    <!-- http://www.nist.gov/itl/ssd/Materials#SolidFoam -->

    <owl:Class rdf:about="&mat;SolidFoam">
        <rdfs:subClassOf rdf:resource="&mat;Foam"/>
        <rdfs:subClassOf rdf:resource="&mat;SolidSubstance"/>
        <rdfs:comment xml:lang="en">A Solid Foam is a substance that is formed by trapping pockets of gas in a solid.</rdfs:comment>
    </owl:Class>
    


    <!-- http://www.nist.gov/itl/ssd/Materials#SolidInLiquidSolution -->

    <owl:Class rdf:about="&mat;SolidInLiquidSolution">
        <rdfs:subClassOf rdf:resource="&mat;LiquidSolution"/>
        <rdfs:subClassOf>
            <owl:Restriction>
                <owl:onProperty rdf:resource="&mat;solute"/>
                <owl:someValuesFrom rdf:resource="&mat;SolidSubstance"/>
            </owl:Restriction>
        </rdfs:subClassOf>
        <rdfs:comment xml:lang="en">A Solid In Liquid Solution is a Chemical Solution in which the soute is solid and the solvent is liquid.</rdfs:comment>
    </owl:Class>
    


    <!-- http://www.nist.gov/itl/ssd/Materials#SolidSol -->

    <owl:Class rdf:about="&mat;SolidSol">
        <rdfs:subClassOf rdf:resource="&mat;Colloid"/>
        <rdfs:subClassOf rdf:resource="&mat;SolidSubstance"/>
        <rdfs:comment xml:lang="en">A Solid Sol is a type of colloid, with one solid phase dispersed inside another solid phase.  The phases remain distinct, so the result is not a solution.</rdfs:comment>
    </owl:Class>
    


    <!-- http://www.nist.gov/itl/ssd/Materials#SolidSubstance -->

    <owl:Class rdf:about="&mat;SolidSubstance">
        <rdfs:subClassOf rdf:resource="&bc;MaterialSubstance"/>
        <owl:disjointWith rdf:resource="&mat;Vacuum"/>
        <rdfs:comment xml:lang="en">Material in a solid phase.</rdfs:comment>
    </owl:Class>
    


    <!-- http://www.nist.gov/itl/ssd/Materials#SolidToSolidPhaseTransformation -->

    <owl:Class rdf:about="&mat;SolidToSolidPhaseTransformation">
        <rdfs:subClassOf rdf:resource="&mat;PhaseChange"/>
        <owl:disjointWith rdf:resource="&mat;Solidification"/>
        <owl:disjointWith rdf:resource="&mat;Vaporization"/>
        <rdfs:comment xml:lang="en">A Solid to Solid Phase Transformation is a phase transition from one solid phase to another.</rdfs:comment>
    </owl:Class>
    


    <!-- http://www.nist.gov/itl/ssd/Materials#Solidification -->

    <owl:Class rdf:about="&mat;Solidification">
        <rdfs:subClassOf rdf:resource="&mat;PhaseChange"/>
        <owl:disjointWith rdf:resource="&mat;Vaporization"/>
        <rdfs:comment xml:lang="en">Solidification is a phase change of a material from a liquid, gasseous, or mixed state to a solid state.</rdfs:comment>
    </owl:Class>
    


    <!-- http://www.nist.gov/itl/ssd/Materials#Solidus -->

    <owl:Class rdf:about="&mat;Solidus">
        <rdfs:subClassOf rdf:resource="&or;CurveSegment"/>
        <rdfs:comment xml:lang="en">A Solidus is a Curve on a temperature-concentration Phase Diagram below which a given substance is completely solid.</rdfs:comment>
    </owl:Class>
    


    <!-- http://www.nist.gov/itl/ssd/Materials#Spectrometer -->

    <owl:Class rdf:about="&mat;Spectrometer">
        <rdfs:subClassOf rdf:resource="&or;LaboratoryEquipment"/>
        <rdfs:subClassOf rdf:resource="&or;MeasuringDevice"/>
    </owl:Class>
    


    <!-- http://www.nist.gov/itl/ssd/Materials#Spectrophotometer -->

    <owl:Class rdf:about="&mat;Spectrophotometer">
        <rdfs:subClassOf rdf:resource="&mat;Spectrometer"/>
        <rdfs:subClassOf rdf:resource="&or;Photometer"/>
        <rdfs:comment xml:lang="en">A  Spectrophotometer is a photometer that measures light intensity as a function of its wavelength.</rdfs:comment>
    </owl:Class>
    


    <!-- http://www.nist.gov/itl/ssd/Materials#SpringSteel -->

    <owl:Class rdf:about="&mat;SpringSteel">
        <rdfs:subClassOf rdf:resource="&mat;CarbonSteel"/>
        <rdfs:comment xml:lang="en">Spring steel is a low alloy, medium carbon steel or high carbon steel with a very high yield strength. This allows objects made of spring steel to return to their original shape despite significant bending or twist.</rdfs:comment>
    </owl:Class>
    


    <!-- http://www.nist.gov/itl/ssd/Materials#StableIsotope -->

    <owl:Class rdf:about="&mat;StableIsotope">
        <rdfs:subClassOf rdf:resource="&bc;Isotope"/>
        <rdfs:comment xml:lang="en">A Stable Isotope is one that is not radioactive</rdfs:comment>
    </owl:Class>
    


    <!-- http://www.nist.gov/itl/ssd/Materials#StainlessSteel -->

    <owl:Class rdf:about="&mat;StainlessSteel">
        <rdfs:subClassOf rdf:resource="&mat;Steel"/>
        <owl:disjointWith rdf:resource="&mat;ToolSteel"/>
        <or:termString xml:lang="en">CRES</or:termString>
        <or:termString xml:lang="en">Stainless steel is  a steel alloy with a minimum of 10.5% to 11% chromium content by mass.</or:termString>
        <or:termString xml:lang="en">corrosion-resistant steel</or:termString>
        <or:termString xml:lang="en">inox</or:termString>
        <or:termString xml:lang="en">inox steel</or:termString>
        <or:termString xml:lang="en">stainless steel</or:termString>
    </owl:Class>
    


    <!-- http://www.nist.gov/itl/ssd/Materials#StateOfMatter -->

    <owl:Class rdf:about="&mat;StateOfMatter">
        <rdfs:subClassOf rdf:resource="&mat;MaterialPhaseComposition"/>
        <rdfs:comment xml:lang="en">A basic State Of Matter is Solid, Liquid, Gas, or Plasma.  </rdfs:comment>
    </owl:Class>
    


    <!-- http://www.nist.gov/itl/ssd/Materials#Steel -->

    <owl:Class rdf:about="&mat;Steel">
        <rdfs:subClassOf rdf:resource="&mat;EngineeredAlloy"/>
        <rdfs:subClassOf rdf:resource="&mat;FerrousAlloy"/>
    </owl:Class>
    


    <!-- http://www.nist.gov/itl/ssd/Materials#Stiffness -->

    <owl:Class rdf:about="&mat;Stiffness">
        <rdfs:subClassOf rdf:resource="&mat;DeformationProperty"/>
    </owl:Class>
    


    <!-- http://www.nist.gov/itl/ssd/Materials#Strength -->

    <owl:Class rdf:about="&mat;Strength">
        <rdfs:subClassOf rdf:resource="&mat;MeasurableMechanicalProperty"/>
        <owl:disjointWith rdf:resource="&mat;TransportProperty"/>
    </owl:Class>
    


    <!-- http://www.nist.gov/itl/ssd/Materials#Sublimating -->

    <owl:Class rdf:about="&mat;Sublimating">
        <rdfs:subClassOf rdf:resource="&mat;OrderDisorderPhaseTransformation"/>
        <rdfs:subClassOf rdf:resource="&mat;Vaporization"/>
        <rdfs:comment xml:lang="en">Sublimating is the Phase Change from a solid state directly to a gasseous state without passing through an intermediate liquid state</rdfs:comment>
    </owl:Class>
    


    <!-- http://www.nist.gov/itl/ssd/Materials#SublimatingToSolid -->

    <owl:Class rdf:about="&mat;SublimatingToSolid">
        <rdfs:subClassOf rdf:resource="&mat;Solidification"/>
        <rdfs:comment xml:lang="en">SublimatingToSolid is the phase change from a gasseous state to a solid state without going through an intermediate liquid state.</rdfs:comment>
    </owl:Class>
    


    <!-- http://www.nist.gov/itl/ssd/Materials#Sulfate -->

    <owl:Class rdf:about="&mat;Sulfate">
        <rdfs:subClassOf rdf:resource="&mat;Mineral"/>
    </owl:Class>
    


    <!-- http://www.nist.gov/itl/ssd/Materials#SulfideCeramic -->

    <owl:Class rdf:about="&mat;SulfideCeramic">
        <rdfs:subClassOf rdf:resource="&mat;ChalcogenBasedCeramic"/>
        <or:referenceURL rdf:datatype="&xsd;anyURI">http://www.matweb.com/index.aspx</or:referenceURL>
        <or:termString xml:lang="en">sulfide</or:termString>
        <or:termString xml:lang="en">sulfide ceramic</or:termString>
    </owl:Class>
    


    <!-- http://www.nist.gov/itl/ssd/Materials#SulfideMineral -->

    <owl:Class rdf:about="&mat;SulfideMineral">
        <rdfs:subClassOf rdf:resource="&mat;Mineral"/>
    </owl:Class>
    


    <!-- http://www.nist.gov/itl/ssd/Materials#SulfosaltMineral -->

    <owl:Class rdf:about="&mat;SulfosaltMineral">
        <rdfs:subClassOf rdf:resource="&mat;Mineral"/>
    </owl:Class>
    


    <!-- http://www.nist.gov/itl/ssd/Materials#Superalloy -->

    <owl:Class rdf:about="&mat;Superalloy">
        <rdfs:subClassOf rdf:resource="&mat;EngineeredAlloy"/>
        <rdfs:comment xml:lang="en">A Superalloy, or high-performance alloy, is an alloy that exhibits excellent mechanical strength and creep resistance at high temperatures, good surface stability, and corrosion and oxidation resistance. Superalloys typically have a matrix with an austenitic face-centered cubic crystal structure. A superalloy&#39;s base alloying element is usually nickel, cobalt, or nickel-iron.</rdfs:comment>
    </owl:Class>
    


    <!-- http://www.nist.gov/itl/ssd/Materials#SurfaceDiffusion -->

    <owl:Class rdf:about="&mat;SurfaceDiffusion">
        <rdfs:subClassOf rdf:resource="&mat;ShortCircuitDiffusion"/>
        <rdfs:seeAlso xml:lang="en">Definitions of terms for diffusion in the solid state (IUPAC Recommendations 1999), Pure Appl. Chem. 71, 1307-1325.</rdfs:seeAlso>
        <rdfs:comment xml:lang="en">Surface diffusion is diffusion that takes place on a surface.</rdfs:comment>
    </owl:Class>
    


    <!-- http://www.nist.gov/itl/ssd/Materials#SyntheticEtherBase -->

    <owl:Class rdf:about="&mat;SyntheticEtherBase">
        <rdfs:subClassOf rdf:resource="&mat;FluidLubricant"/>
        <owl:disjointWith rdf:resource="&mat;UreaGellant"/>
        <owl:disjointWith rdf:resource="&mat;WhiteMineralOil"/>
        <owl:disjointWith rdf:resource="&mat;ZincOxideLubricant"/>
        <or:referenceURL rdf:datatype="&xsd;anyURI">http://www.matweb.com/index.aspx</or:referenceURL>
        <or:termString xml:lang="en">synthetic ether base</or:termString>
        <or:termString xml:lang="en">synthetic ether base lubricant</or:termString>
    </owl:Class>
    


    <!-- http://www.nist.gov/itl/ssd/Materials#T300SeriesStainlessSteel -->

    <owl:Class rdf:about="&mat;T300SeriesStainlessSteel">
        <rdfs:subClassOf rdf:resource="&mat;StainlessSteel"/>
        <owl:disjointWith rdf:resource="&mat;T400SeriesStainlessSteel"/>
        <owl:disjointWith rdf:resource="&mat;T600SeriesStainlessSteel"/>
        <owl:disjointWith rdf:resource="&mat;TS1000SeriesStainlessSteel"/>
        <owl:disjointWith rdf:resource="&mat;TS2000SeriesStainlessSteel"/>
        <owl:disjointWith rdf:resource="&mat;TS3000SeriesStainlessSteel"/>
        <owl:disjointWith rdf:resource="&mat;TS4000SeriesStainlessSteel"/>
        <or:referenceURL rdf:datatype="&xsd;anyURI">http://www.matweb.com/index.aspx</or:referenceURL>
        <or:termString xml:lang="en">T 300 Series Stainless Steel</or:termString>
    </owl:Class>
    


    <!-- http://www.nist.gov/itl/ssd/Materials#T400SeriesStainlessSteel -->

    <owl:Class rdf:about="&mat;T400SeriesStainlessSteel">
        <rdfs:subClassOf rdf:resource="&mat;StainlessSteel"/>
        <owl:disjointWith rdf:resource="&mat;T600SeriesStainlessSteel"/>
        <owl:disjointWith rdf:resource="&mat;TS1000SeriesStainlessSteel"/>
        <owl:disjointWith rdf:resource="&mat;TS2000SeriesStainlessSteel"/>
        <owl:disjointWith rdf:resource="&mat;TS3000SeriesStainlessSteel"/>
        <owl:disjointWith rdf:resource="&mat;TS4000SeriesStainlessSteel"/>
        <or:referenceURL rdf:datatype="&xsd;anyURI">http://www.matweb.com/index.aspx</or:referenceURL>
        <or:termString xml:lang="en">T 400 Series Stainless Steel</or:termString>
    </owl:Class>
    


    <!-- http://www.nist.gov/itl/ssd/Materials#T600SeriesStainlessSteel -->

    <owl:Class rdf:about="&mat;T600SeriesStainlessSteel">
        <rdfs:subClassOf rdf:resource="&mat;StainlessSteel"/>
        <owl:disjointWith rdf:resource="&mat;TS1000SeriesStainlessSteel"/>
        <owl:disjointWith rdf:resource="&mat;TS2000SeriesStainlessSteel"/>
        <owl:disjointWith rdf:resource="&mat;TS3000SeriesStainlessSteel"/>
        <owl:disjointWith rdf:resource="&mat;TS4000SeriesStainlessSteel"/>
        <or:referenceURL rdf:datatype="&xsd;anyURI">http://www.matweb.com/index.aspx</or:referenceURL>
        <or:termString xml:lang="en">T 600 Series Stainless Steel</or:termString>
    </owl:Class>
    


    <!-- http://www.nist.gov/itl/ssd/Materials#TS1000SeriesStainlessSteel -->

    <owl:Class rdf:about="&mat;TS1000SeriesStainlessSteel">
        <rdfs:subClassOf rdf:resource="&mat;StainlessSteel"/>
        <owl:disjointWith rdf:resource="&mat;TS2000SeriesStainlessSteel"/>
        <owl:disjointWith rdf:resource="&mat;TS3000SeriesStainlessSteel"/>
        <owl:disjointWith rdf:resource="&mat;TS4000SeriesStainlessSteel"/>
        <or:referenceURL rdf:datatype="&xsd;anyURI">http://www.matweb.com/index.aspx</or:referenceURL>
        <or:termString xml:lang="en">T S1000 Series Stainless Steel</or:termString>
    </owl:Class>
    


    <!-- http://www.nist.gov/itl/ssd/Materials#TS2000SeriesStainlessSteel -->

    <owl:Class rdf:about="&mat;TS2000SeriesStainlessSteel">
        <rdfs:subClassOf rdf:resource="&mat;StainlessSteel"/>
        <owl:disjointWith rdf:resource="&mat;TS3000SeriesStainlessSteel"/>
        <owl:disjointWith rdf:resource="&mat;TS4000SeriesStainlessSteel"/>
        <or:referenceURL rdf:datatype="&xsd;anyURI">http://www.matweb.com/index.aspx</or:referenceURL>
        <or:termString xml:lang="en">T S2000 Series Stainless Steel</or:termString>
    </owl:Class>
    


    <!-- http://www.nist.gov/itl/ssd/Materials#TS3000SeriesStainlessSteel -->

    <owl:Class rdf:about="&mat;TS3000SeriesStainlessSteel">
        <rdfs:subClassOf rdf:resource="&mat;StainlessSteel"/>
        <owl:disjointWith rdf:resource="&mat;TS4000SeriesStainlessSteel"/>
        <or:referenceURL rdf:datatype="&xsd;anyURI">http://www.matweb.com/index.aspx</or:referenceURL>
        <or:termString xml:lang="en">T S3000 Series Stainless Steel</or:termString>
    </owl:Class>
    


    <!-- http://www.nist.gov/itl/ssd/Materials#TS4000SeriesStainlessSteel -->

    <owl:Class rdf:about="&mat;TS4000SeriesStainlessSteel">
        <rdfs:subClassOf rdf:resource="&mat;StainlessSteel"/>
        <or:referenceURL rdf:datatype="&xsd;anyURI">http://www.matweb.com/index.aspx</or:referenceURL>
        <or:termString xml:lang="en">T S4000 Series Stainless Steel</or:termString>
    </owl:Class>
    


    <!-- http://www.nist.gov/itl/ssd/Materials#TemperatureChangeProcess -->

    <owl:Class rdf:about="&mat;TemperatureChangeProcess">
        <rdfs:subClassOf rdf:resource="&or;MechanicalProcess"/>
        <owl:disjointWith rdf:resource="&mat;ThermalExpansion"/>
        <rdfs:comment xml:lang="en">A Temperature Change Process is a process during which the temperature of an object increases or decreases.  </rdfs:comment>
    </owl:Class>
    


    <!-- http://www.nist.gov/itl/ssd/Materials#TemperatureDependentProperty -->

    <owl:Class rdf:about="&mat;TemperatureDependentProperty">
        <rdfs:subClassOf rdf:resource="&or;MaterialProperty"/>
        <rdfs:comment xml:lang="en">A Temperature Dependent Property is one whose value depends upon the ambient pressure, such as a vapor pressure.</rdfs:comment>
    </owl:Class>
    


    <!-- http://www.nist.gov/itl/ssd/Materials#TetragonalCrystalStructure -->

    <owl:Class rdf:about="&mat;TetragonalCrystalStructure">
        <rdfs:subClassOf rdf:resource="&mat;CrystalLattice"/>
        <owl:disjointWith rdf:resource="&mat;TriclinicCrystalStructure"/>
        <owl:disjointWith rdf:resource="&mat;TrigonalCrystalStructure"/>
        <rdfs:comment xml:lang="en">Tetragonal crystal lattices result from stretching a cubic lattice along one of its lattice vectors, so that the cube becomes a rectangular prism with a square base (a by a) and height (c, which is different from a).

There are two tetragonal Bravais lattices: the simple (or primitive) tetragonal (from stretching the simple-cubic lattice) and the body-centered tetragonal (from stretching either the face-centered or the body-centered cubic lattice).</rdfs:comment>
    </owl:Class>
    


    <!-- http://www.nist.gov/itl/ssd/Materials#ThermalExpansion -->

    <owl:Class rdf:about="&mat;ThermalExpansion">
        <rdfs:subClassOf rdf:resource="&or;MechanicalProcess"/>
        <rdfs:comment xml:lang="en">Thermal Expansion is a Mechanical Process in which an object changes size (expands or contracts) in response to a change in temperature.</rdfs:comment>
    </owl:Class>
    


    <!-- http://www.nist.gov/itl/ssd/Materials#ThermalProperty -->

    <owl:Class rdf:about="&mat;ThermalProperty">
        <rdfs:subClassOf rdf:resource="&or;MeasurableMaterialProperty"/>
        <skos:note xml:lang="en">Similar to &quot;Thermal&quot; in Ashino&#39;s 2010 Minerals Ontology.</skos:note>
    </owl:Class>
    


    <!-- http://www.nist.gov/itl/ssd/Materials#ThermochemicalProperty -->

    <owl:Class rdf:about="&mat;ThermochemicalProperty">
        <rdfs:subClassOf rdf:resource="&or;MeasurableMaterialProperty"/>
    </owl:Class>
    


    <!-- http://www.nist.gov/itl/ssd/Materials#ThermodynamicModel -->

    <owl:Class rdf:about="&mat;ThermodynamicModel">
        <rdfs:subClassOf rdf:resource="&doc;SystemModel"/>
        <rdfs:comment xml:lang="en">A Thermodynamic Model is a model of some aspects of a thermodynamic system.</rdfs:comment>
    </owl:Class>
    


    <!-- http://www.nist.gov/itl/ssd/Materials#ThermodynamicPhase -->

    <owl:Class rdf:about="&mat;ThermodynamicPhase">
        <rdfs:subClassOf rdf:resource="&or;ObjectType"/>
        <rdfs:comment xml:lang="en">A Thermodynamic Phase is defined as a type region of space throughout which all physical properties of a material (composition, enthalpy content, StateOfMatter, and other properties are essentially uniform.  A material may be of a single phase, or at a microscopic level, be composed of regions of two (or more) phases.  A thermodynamic Phase Diagram depicts the boundaries among Thermodynamic Phases and binary (or multi-) phase fields.  </rdfs:comment>
    </owl:Class>
    


    <!-- http://www.nist.gov/itl/ssd/Materials#ThermodynamicSystem -->

    <owl:Class rdf:about="&mat;ThermodynamicSystem">
        <rdfs:subClassOf rdf:resource="&or;PhysicalObject"/>
        <rdfs:comment xml:lang="en">A thermodynamic system is a precisely defined macroscopic region of the universe, often called a physical system.  The set of thermodynamic parameters necessary to uniquely define a system is called the thermodynamic state of a system. The state of a system is expressed as a functional relationship, the equation of state, between its parameters. A system is in thermodynamic equilibrium when the state of the system does not change with time.</rdfs:comment>
    </owl:Class>
    


    <!-- http://www.nist.gov/itl/ssd/Materials#Thermomigration -->

    <owl:Class rdf:about="&mat;Thermomigration">
        <rdfs:subClassOf rdf:resource="&mat;Diffusion"/>
        <rdfs:seeAlso xml:lang="en">Definitions of terms for diffusion in the solid state (IUPAC Recommendations 1999), Pure Appl. Chem. 71, 1307-1325.</rdfs:seeAlso>
        <rdfs:comment xml:lang="en">Thermomigration is diffusion resulting from a temperature gradient.  This is also called thermal diffusion, the Ludwig-Soret effect, or the Soret effect.</rdfs:comment>
    </owl:Class>
    


    <!-- http://www.nist.gov/itl/ssd/Materials#Thermoplastic -->

    <owl:Class rdf:about="&mat;Thermoplastic">
        <rdfs:subClassOf rdf:resource="&mat;EngineeredMaterial"/>
        <rdfs:subClassOf rdf:resource="&mat;PolymerSubstance"/>
        <owl:disjointWith rdf:resource="&mat;Thermoset"/>
        <or:referenceURL rdf:datatype="&xsd;anyURI">http://www.matweb.com/index.aspx</or:referenceURL>
        <rdfs:comment xml:lang="en">A Thermoplastic, or thermosoftening plastic, is a polymer that becomes pliable or moldable above a specific temperature, and returns to a solid state upon cooling. This property allows thermoplastics to be remolded.</rdfs:comment>
    </owl:Class>
    


    <!-- http://www.nist.gov/itl/ssd/Materials#Thermoset -->

    <owl:Class rdf:about="&mat;Thermoset">
        <rdfs:subClassOf rdf:resource="&mat;PolymerSubstance"/>
        <or:referenceURL rdf:datatype="&xsd;anyURI">http://www.matweb.com/index.aspx</or:referenceURL>
        <rdfs:comment xml:lang="en">A thermosetting plastic (or Thermoset) is polymer material that irreversibly cures. The cure may be done through heat (generally above 200 °C (392 °F)), through a chemical reaction (two-part epoxy, for example), or irradiation such as electron beam processing.</rdfs:comment>
        <or:termString xml:lang="en">thermoset</or:termString>
        <or:termString xml:lang="en">thermosetting plastic</or:termString>
    </owl:Class>
    


    <!-- http://www.nist.gov/itl/ssd/Materials#ThinFilm -->

    <owl:Class rdf:about="&mat;ThinFilm">
        <rdfs:subClassOf rdf:resource="&bc;MaterialSubstance"/>
        <rdfs:comment xml:lang="en">A thin film is a layer of material ranging from fractions of a nanometer (monolayer) to several microns in thickness.</rdfs:comment>
    </owl:Class>
    


    <!-- http://www.nist.gov/itl/ssd/Materials#TinAlloy -->

    <owl:Class rdf:about="&mat;TinAlloy">
        <rdfs:subClassOf rdf:resource="&mat;NonFerrousAlloy"/>
        <rdfs:subClassOf>
            <owl:Restriction>
                <owl:onProperty rdf:resource="&mat;physicalDecompositions"/>
                <owl:someValuesFrom rdf:resource="&bc;Tin"/>
            </owl:Restriction>
        </rdfs:subClassOf>
        <or:referenceURL rdf:datatype="&xsd;anyURI">http://www.matweb.com/index.aspx</or:referenceURL>
        <rdfs:comment xml:lang="en">An alloy that contains Tin but not Iron.</rdfs:comment>
    </owl:Class>
    


    <!-- http://www.nist.gov/itl/ssd/Materials#TitaniumAlloy -->

    <owl:Class rdf:about="&mat;TitaniumAlloy">
        <rdfs:subClassOf rdf:resource="&mat;NonFerrousAlloy"/>
        <rdfs:subClassOf>
            <owl:Restriction>
                <owl:onProperty rdf:resource="&mat;physicalDecompositions"/>
                <owl:someValuesFrom rdf:resource="&bc;Titanium"/>
            </owl:Restriction>
        </rdfs:subClassOf>
        <or:referenceURL rdf:datatype="&xsd;anyURI">http://www.matweb.com/index.aspx</or:referenceURL>
    </owl:Class>
    


    <!-- http://www.nist.gov/itl/ssd/Materials#TitaniumOxide -->

    <owl:Class rdf:about="&mat;TitaniumOxide">
        <rdfs:subClassOf rdf:resource="&bc;Oxide"/>
        <owl:disjointWith rdf:resource="&mat;ZirconiumOxide"/>
        <or:referenceURL rdf:datatype="&xsd;anyURI">http://www.matweb.com/index.aspx</or:referenceURL>
        <or:termString xml:lang="en">titanium oxide</or:termString>
    </owl:Class>
    


    <!-- http://www.nist.gov/itl/ssd/Materials#ToolSteel -->

    <owl:Class rdf:about="&mat;ToolSteel">
        <rdfs:subClassOf rdf:resource="&mat;Steel"/>
        <or:referenceURL rdf:datatype="&xsd;anyURI">http://www.matweb.com/index.aspx</or:referenceURL>
        <rdfs:comment xml:lang="en">Tool steel refers to a variety of carbon and alloy steels that are particularly well-suited to be made into tools. Their suitability comes from their distinctive hardness, resistance to abrasion, their ability to hold a cutting edge, and/or their resistance to deformation at elevated temperatures (red-hardness). Tool steel is generally heat-treated.

Tool steel has a carbon content between 0.7% and 1.5%. The manganese content is often kept low to minimize the possibility of cracking during water quenching.</rdfs:comment>
        <or:termString xml:lang="en">tool steel</or:termString>
    </owl:Class>
    


    <!-- http://www.nist.gov/itl/ssd/Materials#TracerDiffusion -->

    <owl:Class rdf:about="&mat;TracerDiffusion">
        <rdfs:subClassOf rdf:resource="&mat;Diffusion"/>
        <rdfs:seeAlso xml:lang="en">Definitions of terms for diffusion in the solid state (IUPAC Recommendations 1999), Pure Appl. Chem. 71, 1307-1325.</rdfs:seeAlso>
        <rdfs:comment xml:lang="en">Tracer diffusion refers to the migration of a tagged atom through a material of which it is a component.</rdfs:comment>
    </owl:Class>
    


    <!-- http://www.nist.gov/itl/ssd/Materials#TransparencyLevel -->

    <owl:Class rdf:about="&mat;TransparencyLevel">
        <rdfs:subClassOf rdf:resource="&or;Quantity"/>
    </owl:Class>
    


    <!-- http://www.nist.gov/itl/ssd/Materials#TransportProperty -->

    <owl:Class rdf:about="&mat;TransportProperty">
        <rdfs:subClassOf rdf:resource="&mat;MeasurableMechanicalProperty"/>
    </owl:Class>
    


    <!-- http://www.nist.gov/itl/ssd/Materials#TriclinicCrystalStructure -->

    <owl:Class rdf:about="&mat;TriclinicCrystalStructure">
        <rdfs:subClassOf rdf:resource="&mat;CrystalLattice"/>
        <rdfs:comment xml:lang="en">The triclinic lattice is the least symmetric of the 14 three-dimensional Bravais lattices. It has (itself) the minimum symmetry all lattices have: points of inversion at each lattice point and at 7 more points for each lattice point: at the midpoints of the edges and the faces, and at the center points. It is the only lattice type that itself has no mirror planes.</rdfs:comment>
    </owl:Class>
    


    <!-- http://www.nist.gov/itl/ssd/Materials#TrigonalCrystalStructure -->

    <owl:Class rdf:about="&mat;TrigonalCrystalStructure">
        <rdfs:subClassOf rdf:resource="&mat;CrystalLattice"/>
        <rdfs:comment xml:lang="en">The trigonal crystal system is the only crystal system whose point groups have more than one lattice system associated with their space groups: the hexagonal and rhombohedral lattices both appear.</rdfs:comment>
    </owl:Class>
    


    <!-- http://www.nist.gov/itl/ssd/Materials#Tritium -->

    <owl:Class rdf:about="&mat;Tritium">
        <rdfs:subClassOf rdf:resource="&bc;Hydrogen"/>
        <rdfs:subClassOf rdf:resource="&mat;RadioactiveMaterial"/>
    </owl:Class>
    


    <!-- http://www.nist.gov/itl/ssd/Materials#TungstenAlloy -->

    <owl:Class rdf:about="&mat;TungstenAlloy">
        <rdfs:subClassOf rdf:resource="&mat;NonFerrousAlloy"/>
        <rdfs:subClassOf>
            <owl:Restriction>
                <owl:onProperty rdf:resource="&mat;physicalDecompositions"/>
                <owl:someValuesFrom rdf:resource="&bc;Tungsten"/>
            </owl:Restriction>
        </rdfs:subClassOf>
        <or:referenceURL rdf:datatype="&xsd;anyURI">http://www.matweb.com/index.aspx</or:referenceURL>
    </owl:Class>
    


    <!-- http://www.nist.gov/itl/ssd/Materials#UnitOfAreaPerForce -->

    <owl:Class rdf:about="&mat;UnitOfAreaPerForce">
        <rdfs:subClassOf rdf:resource="&or;UnitOfMeasure"/>
    </owl:Class>
    


    <!-- http://www.nist.gov/itl/ssd/Materials#UnitOfAreaPerTime -->

    <owl:Class rdf:about="&mat;UnitOfAreaPerTime">
        <rdfs:subClassOf rdf:resource="&or;UnitOfMeasure"/>
        <owl:disjointWith rdf:resource="&mat;UnitOfCharge"/>
        <owl:disjointWith rdf:resource="&mat;UnitOfElectricCurrent"/>
        <owl:disjointWith rdf:resource="&mat;UnitOfElectricalConductivity"/>
        <owl:disjointWith rdf:resource="&mat;UnitOfElectricalResistance"/>
        <owl:disjointWith rdf:resource="&mat;UnitOfElectricalResistivity"/>
        <owl:disjointWith rdf:resource="&mat;UnitOfEnergyPerMass"/>
        <owl:disjointWith rdf:resource="&mat;UnitOfInverseAreaPerTime"/>
        <owl:disjointWith rdf:resource="&mat;UnitOfSpecificHeatCapacity"/>
        <owl:disjointWith rdf:resource="&mat;UnitOfThermalConductivity"/>
        <owl:disjointWith rdf:resource="&or;CurrencyUnit"/>
        <owl:disjointWith rdf:resource="&or;UnitOfArea"/>
        <owl:disjointWith rdf:resource="&or;UnitOfComputerStorageCapacity"/>
        <owl:disjointWith rdf:resource="&or;UnitOfDensity"/>
        <owl:disjointWith rdf:resource="&or;UnitOfDistance"/>
        <owl:disjointWith rdf:resource="&or;UnitOfDuration"/>
        <owl:disjointWith rdf:resource="&or;UnitOfEnergy"/>
        <owl:disjointWith rdf:resource="&or;UnitOfForce"/>
        <owl:disjointWith rdf:resource="&or;UnitOfMass"/>
    </owl:Class>
    


    <!-- http://www.nist.gov/itl/ssd/Materials#UnitOfCapacitance -->

    <owl:Class rdf:about="&mat;UnitOfCapacitance">
        <rdfs:subClassOf rdf:resource="&or;UnitOfMeasure"/>
    </owl:Class>
    


    <!-- http://www.nist.gov/itl/ssd/Materials#UnitOfCharge -->

    <owl:Class rdf:about="&mat;UnitOfCharge">
        <rdfs:subClassOf rdf:resource="&or;UnitOfMeasure"/>
        <owl:disjointWith rdf:resource="&mat;UnitOfElectricCurrent"/>
        <owl:disjointWith rdf:resource="&mat;UnitOfElectricalConductance"/>
        <owl:disjointWith rdf:resource="&mat;UnitOfElectricalConductivity"/>
        <owl:disjointWith rdf:resource="&mat;UnitOfElectricalResistance"/>
        <owl:disjointWith rdf:resource="&mat;UnitOfElectricalResistivity"/>
        <owl:disjointWith rdf:resource="&mat;UnitOfEnergyPerMass"/>
        <owl:disjointWith rdf:resource="&mat;UnitOfEnergyPerTemperatureDifference"/>
        <owl:disjointWith rdf:resource="&mat;UnitOfForcePerVolume"/>
        <owl:disjointWith rdf:resource="&mat;UnitOfInverseAreaPerTime"/>
        <owl:disjointWith rdf:resource="&mat;UnitOfInverseTemperatureDifference"/>
        <owl:disjointWith rdf:resource="&mat;UnitOfInverseTime"/>
        <owl:disjointWith rdf:resource="&mat;UnitOfPower"/>
        <owl:disjointWith rdf:resource="&mat;UnitOfSpecificHeatCapacity"/>
        <owl:disjointWith rdf:resource="&mat;UnitOfTemperatureDifference"/>
        <owl:disjointWith rdf:resource="&mat;UnitOfThermalConductivity"/>
        <owl:disjointWith rdf:resource="&mat;UnitOfToughness"/>
        <owl:disjointWith rdf:resource="&or;DimensionlessUnit"/>
        <owl:disjointWith rdf:resource="&or;UnitOfAcceleration"/>
        <owl:disjointWith rdf:resource="&or;UnitOfArea"/>
        <owl:disjointWith rdf:resource="&or;UnitOfComputerStorageCapacity"/>
        <owl:disjointWith rdf:resource="&or;UnitOfDensity"/>
        <owl:disjointWith rdf:resource="&or;UnitOfDistance"/>
        <owl:disjointWith rdf:resource="&or;UnitOfDuration"/>
        <owl:disjointWith rdf:resource="&or;UnitOfEnergy"/>
        <owl:disjointWith rdf:resource="&or;UnitOfForce"/>
        <owl:disjointWith rdf:resource="&or;UnitOfMass"/>
        <owl:disjointWith rdf:resource="&or;UnitOfPressure"/>
        <owl:disjointWith rdf:resource="&or;UnitOfSpreadRate"/>
        <owl:disjointWith rdf:resource="&or;UnitOfTemperature"/>
        <owl:disjointWith rdf:resource="&or;UnitOfVelocity"/>
        <owl:disjointWith rdf:resource="&or;UnitOfVelocitySquared"/>
        <owl:disjointWith rdf:resource="&or;UnitOfVoltage"/>
        <owl:disjointWith rdf:resource="&or;UnitOfVolume"/>
    </owl:Class>
    


    <!-- http://www.nist.gov/itl/ssd/Materials#UnitOfElectricCurrent -->

    <owl:Class rdf:about="&mat;UnitOfElectricCurrent">
        <rdfs:subClassOf rdf:resource="&or;UnitOfMeasure"/>
        <owl:disjointWith rdf:resource="&mat;UnitOfElectricalConductance"/>
        <owl:disjointWith rdf:resource="&mat;UnitOfElectricalConductivity"/>
        <owl:disjointWith rdf:resource="&mat;UnitOfElectricalResistance"/>
        <owl:disjointWith rdf:resource="&mat;UnitOfElectricalResistivity"/>
        <owl:disjointWith rdf:resource="&mat;UnitOfEnergyPerMass"/>
        <owl:disjointWith rdf:resource="&mat;UnitOfEnergyPerTemperatureDifference"/>
        <owl:disjointWith rdf:resource="&mat;UnitOfForcePerVolume"/>
        <owl:disjointWith rdf:resource="&mat;UnitOfInverseTemperatureDifference"/>
        <owl:disjointWith rdf:resource="&mat;UnitOfInverseTime"/>
        <owl:disjointWith rdf:resource="&mat;UnitOfPower"/>
        <owl:disjointWith rdf:resource="&mat;UnitOfSpecificHeatCapacity"/>
        <owl:disjointWith rdf:resource="&mat;UnitOfTemperatureDifference"/>
        <owl:disjointWith rdf:resource="&mat;UnitOfThermalConductivity"/>
        <owl:disjointWith rdf:resource="&mat;UnitOfToughness"/>
        <owl:disjointWith rdf:resource="&or;DimensionlessUnit"/>
        <owl:disjointWith rdf:resource="&or;UnitOfAcceleration"/>
        <owl:disjointWith rdf:resource="&or;UnitOfArea"/>
        <owl:disjointWith rdf:resource="&or;UnitOfComputerStorageCapacity"/>
        <owl:disjointWith rdf:resource="&or;UnitOfDensity"/>
        <owl:disjointWith rdf:resource="&or;UnitOfDistance"/>
        <owl:disjointWith rdf:resource="&or;UnitOfDuration"/>
        <owl:disjointWith rdf:resource="&or;UnitOfEnergy"/>
        <owl:disjointWith rdf:resource="&or;UnitOfForce"/>
        <owl:disjointWith rdf:resource="&or;UnitOfMass"/>
        <owl:disjointWith rdf:resource="&or;UnitOfPressure"/>
        <owl:disjointWith rdf:resource="&or;UnitOfSpreadRate"/>
        <owl:disjointWith rdf:resource="&or;UnitOfTemperature"/>
        <owl:disjointWith rdf:resource="&or;UnitOfVelocity"/>
        <owl:disjointWith rdf:resource="&or;UnitOfVelocitySquared"/>
        <owl:disjointWith rdf:resource="&or;UnitOfVoltage"/>
        <owl:disjointWith rdf:resource="&or;UnitOfVolume"/>
    </owl:Class>
    


    <!-- http://www.nist.gov/itl/ssd/Materials#UnitOfElectricalConductance -->

    <owl:Class rdf:about="&mat;UnitOfElectricalConductance">
        <rdfs:subClassOf rdf:resource="&or;UnitOfMeasure"/>
        <owl:disjointWith rdf:resource="&mat;UnitOfInverseAreaPerTime"/>
        <owl:disjointWith rdf:resource="&mat;UnitOfSpecificHeatCapacity"/>
        <owl:disjointWith rdf:resource="&mat;UnitOfTemperatureDifference"/>
    </owl:Class>
    


    <!-- http://www.nist.gov/itl/ssd/Materials#UnitOfElectricalConductivity -->

    <owl:Class rdf:about="&mat;UnitOfElectricalConductivity">
        <rdfs:subClassOf rdf:resource="&or;UnitOfMeasure"/>
        <owl:disjointWith rdf:resource="&mat;UnitOfElectricalResistance"/>
        <owl:disjointWith rdf:resource="&mat;UnitOfElectricalResistivity"/>
        <owl:disjointWith rdf:resource="&mat;UnitOfEnergyPerMass"/>
        <owl:disjointWith rdf:resource="&mat;UnitOfInverseAreaPerTime"/>
        <owl:disjointWith rdf:resource="&mat;UnitOfSpecificHeatCapacity"/>
        <owl:disjointWith rdf:resource="&mat;UnitOfTemperatureDifference"/>
        <owl:disjointWith rdf:resource="&mat;UnitOfThermalConductivity"/>
        <owl:disjointWith rdf:resource="&or;CurrencyUnit"/>
        <owl:disjointWith rdf:resource="&or;DimensionlessUnit"/>
        <owl:disjointWith rdf:resource="&or;UnitOfAcceleration"/>
        <owl:disjointWith rdf:resource="&or;UnitOfArea"/>
        <owl:disjointWith rdf:resource="&or;UnitOfComputerStorageCapacity"/>
        <owl:disjointWith rdf:resource="&or;UnitOfDensity"/>
        <owl:disjointWith rdf:resource="&or;UnitOfDistance"/>
        <owl:disjointWith rdf:resource="&or;UnitOfDuration"/>
        <owl:disjointWith rdf:resource="&or;UnitOfEnergy"/>
        <owl:disjointWith rdf:resource="&or;UnitOfForce"/>
        <owl:disjointWith rdf:resource="&or;UnitOfMass"/>
        <owl:disjointWith rdf:resource="&or;UnitOfPressure"/>
        <owl:disjointWith rdf:resource="&or;UnitOfSpreadRate"/>
        <owl:disjointWith rdf:resource="&or;UnitOfTemperature"/>
        <owl:disjointWith rdf:resource="&or;UnitOfVoltage"/>
        <owl:disjointWith rdf:resource="&or;UnitOfVolume"/>
    </owl:Class>
    


    <!-- http://www.nist.gov/itl/ssd/Materials#UnitOfElectricalResistance -->

    <owl:Class rdf:about="&mat;UnitOfElectricalResistance">
        <rdfs:subClassOf rdf:resource="&or;UnitOfMeasure"/>
        <owl:disjointWith rdf:resource="&mat;UnitOfElectricalResistivity"/>
        <owl:disjointWith rdf:resource="&mat;UnitOfEnergyPerMass"/>
        <owl:disjointWith rdf:resource="&mat;UnitOfInverseAreaPerTime"/>
        <owl:disjointWith rdf:resource="&mat;UnitOfSpecificHeatCapacity"/>
        <owl:disjointWith rdf:resource="&mat;UnitOfTemperatureDifference"/>
        <owl:disjointWith rdf:resource="&mat;UnitOfThermalConductivity"/>
        <owl:disjointWith rdf:resource="&or;CurrencyUnit"/>
        <owl:disjointWith rdf:resource="&or;UnitOfArea"/>
        <owl:disjointWith rdf:resource="&or;UnitOfComputerStorageCapacity"/>
        <owl:disjointWith rdf:resource="&or;UnitOfDensity"/>
        <owl:disjointWith rdf:resource="&or;UnitOfDistance"/>
        <owl:disjointWith rdf:resource="&or;UnitOfDuration"/>
        <owl:disjointWith rdf:resource="&or;UnitOfEnergy"/>
        <owl:disjointWith rdf:resource="&or;UnitOfMass"/>
        <owl:disjointWith rdf:resource="&or;UnitOfPressure"/>
        <owl:disjointWith rdf:resource="&or;UnitOfSpreadRate"/>
        <owl:disjointWith rdf:resource="&or;UnitOfTemperature"/>
        <owl:disjointWith rdf:resource="&or;UnitOfVoltage"/>
        <owl:disjointWith rdf:resource="&or;UnitOfVolume"/>
    </owl:Class>
    


    <!-- http://www.nist.gov/itl/ssd/Materials#UnitOfElectricalResistivity -->

    <owl:Class rdf:about="&mat;UnitOfElectricalResistivity">
        <rdfs:subClassOf rdf:resource="&or;UnitOfMeasure"/>
        <owl:disjointWith rdf:resource="&mat;UnitOfEnergyPerMass"/>
        <owl:disjointWith rdf:resource="&mat;UnitOfInverseAreaPerTime"/>
        <owl:disjointWith rdf:resource="&mat;UnitOfSpecificHeatCapacity"/>
        <owl:disjointWith rdf:resource="&mat;UnitOfTemperatureDifference"/>
        <owl:disjointWith rdf:resource="&mat;UnitOfThermalConductivity"/>
        <owl:disjointWith rdf:resource="&or;CurrencyUnit"/>
        <owl:disjointWith rdf:resource="&or;UnitOfArea"/>
        <owl:disjointWith rdf:resource="&or;UnitOfComputerStorageCapacity"/>
        <owl:disjointWith rdf:resource="&or;UnitOfDensity"/>
        <owl:disjointWith rdf:resource="&or;UnitOfDistance"/>
        <owl:disjointWith rdf:resource="&or;UnitOfDuration"/>
        <owl:disjointWith rdf:resource="&or;UnitOfEnergy"/>
        <owl:disjointWith rdf:resource="&or;UnitOfForce"/>
        <owl:disjointWith rdf:resource="&or;UnitOfMass"/>
        <owl:disjointWith rdf:resource="&or;UnitOfPressure"/>
        <owl:disjointWith rdf:resource="&or;UnitOfSpreadRate"/>
        <owl:disjointWith rdf:resource="&or;UnitOfTemperature"/>
        <owl:disjointWith rdf:resource="&or;UnitOfVoltage"/>
        <owl:disjointWith rdf:resource="&or;UnitOfVolume"/>
    </owl:Class>
    


    <!-- http://www.nist.gov/itl/ssd/Materials#UnitOfEnergyPerAmount -->

    <owl:Class rdf:about="&mat;UnitOfEnergyPerAmount">
        <rdfs:subClassOf rdf:resource="&or;UnitOfMeasure"/>
    </owl:Class>
    


    <!-- http://www.nist.gov/itl/ssd/Materials#UnitOfEnergyPerMass -->

    <owl:Class rdf:about="&mat;UnitOfEnergyPerMass">
        <rdfs:subClassOf rdf:resource="&or;UnitOfMeasure"/>
        <owl:disjointWith rdf:resource="&mat;UnitOfInverseAreaPerTime"/>
        <owl:disjointWith rdf:resource="&mat;UnitOfSpecificHeatCapacity"/>
        <owl:disjointWith rdf:resource="&mat;UnitOfTemperatureDifference"/>
        <owl:disjointWith rdf:resource="&mat;UnitOfThermalConductivity"/>
        <owl:disjointWith rdf:resource="&or;UnitOfArea"/>
        <owl:disjointWith rdf:resource="&or;UnitOfComputerStorageCapacity"/>
        <owl:disjointWith rdf:resource="&or;UnitOfDensity"/>
        <owl:disjointWith rdf:resource="&or;UnitOfDistance"/>
        <owl:disjointWith rdf:resource="&or;UnitOfDuration"/>
        <owl:disjointWith rdf:resource="&or;UnitOfEnergy"/>
        <owl:disjointWith rdf:resource="&or;UnitOfForce"/>
        <owl:disjointWith rdf:resource="&or;UnitOfMass"/>
        <owl:disjointWith rdf:resource="&or;UnitOfSpreadRate"/>
        <owl:disjointWith rdf:resource="&or;UnitOfTemperature"/>
        <owl:disjointWith rdf:resource="&or;UnitOfVoltage"/>
        <owl:disjointWith rdf:resource="&or;UnitOfVolume"/>
        <rdfs:comment xml:lang="en">A Unit Of Energy Per Mass is a Unit Of Energy divided by a Unit Of Mass.  E.g., Joules per Gram.</rdfs:comment>
    </owl:Class>
    


    <!-- http://www.nist.gov/itl/ssd/Materials#UnitOfEnergyPerTemperatureDifference -->

    <owl:Class rdf:about="&mat;UnitOfEnergyPerTemperatureDifference">
        <rdfs:subClassOf rdf:resource="&or;UnitOfMeasure"/>
        <owl:disjointWith rdf:resource="&mat;UnitOfTemperatureDifference"/>
    </owl:Class>
    


    <!-- http://www.nist.gov/itl/ssd/Materials#UnitOfForcePerVolume -->

    <owl:Class rdf:about="&mat;UnitOfForcePerVolume">
        <rdfs:subClassOf rdf:resource="&or;UnitOfMeasure"/>
        <owl:disjointWith rdf:resource="&mat;UnitOfSpecificHeatCapacity"/>
        <owl:disjointWith rdf:resource="&mat;UnitOfTemperatureDifference"/>
    </owl:Class>
    


    <!-- http://www.nist.gov/itl/ssd/Materials#UnitOfInductance -->

    <owl:Class rdf:about="&mat;UnitOfInductance">
        <rdfs:subClassOf rdf:resource="&or;UnitOfMeasure"/>
    </owl:Class>
    


    <!-- http://www.nist.gov/itl/ssd/Materials#UnitOfInverseAreaPerTime -->

    <owl:Class rdf:about="&mat;UnitOfInverseAreaPerTime">
        <rdfs:subClassOf rdf:resource="&or;UnitOfMeasure"/>
        <owl:disjointWith rdf:resource="&mat;UnitOfSpecificHeatCapacity"/>
        <owl:disjointWith rdf:resource="&mat;UnitOfTemperatureDifference"/>
        <owl:disjointWith rdf:resource="&mat;UnitOfThermalConductivity"/>
        <owl:disjointWith rdf:resource="&or;CurrencyUnit"/>
        <owl:disjointWith rdf:resource="&or;DimensionlessUnit"/>
        <owl:disjointWith rdf:resource="&or;UnitOfAcceleration"/>
        <owl:disjointWith rdf:resource="&or;UnitOfArea"/>
        <owl:disjointWith rdf:resource="&or;UnitOfComputerStorageCapacity"/>
        <owl:disjointWith rdf:resource="&or;UnitOfDensity"/>
        <owl:disjointWith rdf:resource="&or;UnitOfDistance"/>
        <owl:disjointWith rdf:resource="&or;UnitOfDuration"/>
        <owl:disjointWith rdf:resource="&or;UnitOfEnergy"/>
        <owl:disjointWith rdf:resource="&or;UnitOfForce"/>
        <owl:disjointWith rdf:resource="&or;UnitOfMass"/>
        <owl:disjointWith rdf:resource="&or;UnitOfPressure"/>
        <owl:disjointWith rdf:resource="&or;UnitOfSpreadRate"/>
        <owl:disjointWith rdf:resource="&or;UnitOfTemperature"/>
        <owl:disjointWith rdf:resource="&or;UnitOfVelocity"/>
        <owl:disjointWith rdf:resource="&or;UnitOfVoltage"/>
        <owl:disjointWith rdf:resource="&or;UnitOfVolume"/>
        <rdfs:comment xml:lang="en">A Unit of Inverse Area per Time has the dimension of 1/ Area / Duration.</rdfs:comment>
    </owl:Class>
    


    <!-- http://www.nist.gov/itl/ssd/Materials#UnitOfInverseTemperatureDifference -->

    <owl:Class rdf:about="&mat;UnitOfInverseTemperatureDifference">
        <rdfs:subClassOf rdf:resource="&or;UnitOfMeasure"/>
        <owl:disjointWith rdf:resource="&mat;UnitOfTemperatureDifference"/>
    </owl:Class>
    


    <!-- http://www.nist.gov/itl/ssd/Materials#UnitOfInverseTime -->

    <owl:Class rdf:about="&mat;UnitOfInverseTime">
        <rdfs:subClassOf rdf:resource="&or;UnitOfMeasure"/>
        <owl:disjointWith rdf:resource="&mat;UnitOfSpecificHeatCapacity"/>
        <owl:disjointWith rdf:resource="&mat;UnitOfTemperatureDifference"/>
    </owl:Class>
    


    <!-- http://www.nist.gov/itl/ssd/Materials#UnitOfPower -->

    <owl:Class rdf:about="&mat;UnitOfPower">
        <rdfs:subClassOf rdf:resource="&or;UnitOfMeasure"/>
    </owl:Class>
    


    <!-- http://www.nist.gov/itl/ssd/Materials#UnitOfPrecision -->

    <owl:Class rdf:about="&mat;UnitOfPrecision">
        <rdfs:subClassOf rdf:resource="&or;UnitOfMeasure"/>
        <owl:disjointWith rdf:resource="&mat;UnitOfSpecificHeatCapacity"/>
    </owl:Class>
    


    <!-- http://www.nist.gov/itl/ssd/Materials#UnitOfSpecificHeatCapacity -->

    <owl:Class rdf:about="&mat;UnitOfSpecificHeatCapacity">
        <rdfs:subClassOf rdf:resource="&or;UnitOfMeasure"/>
        <owl:disjointWith rdf:resource="&mat;UnitOfTemperatureDifference"/>
        <owl:disjointWith rdf:resource="&mat;UnitOfThermalConductivity"/>
        <owl:disjointWith rdf:resource="&mat;UnitOfToughness"/>
        <owl:disjointWith rdf:resource="&or;CurrencyUnit"/>
        <owl:disjointWith rdf:resource="&or;DimensionlessUnit"/>
        <owl:disjointWith rdf:resource="&or;UnitOfAcceleration"/>
        <owl:disjointWith rdf:resource="&or;UnitOfArea"/>
        <owl:disjointWith rdf:resource="&or;UnitOfComputerStorageCapacity"/>
        <owl:disjointWith rdf:resource="&or;UnitOfDensity"/>
        <owl:disjointWith rdf:resource="&or;UnitOfDuration"/>
        <owl:disjointWith rdf:resource="&or;UnitOfEnergy"/>
        <owl:disjointWith rdf:resource="&or;UnitOfForce"/>
        <owl:disjointWith rdf:resource="&or;UnitOfMass"/>
        <owl:disjointWith rdf:resource="&or;UnitOfPressure"/>
        <owl:disjointWith rdf:resource="&or;UnitOfSpreadRate"/>
        <owl:disjointWith rdf:resource="&or;UnitOfTemperature"/>
        <owl:disjointWith rdf:resource="&or;UnitOfVelocity"/>
        <owl:disjointWith rdf:resource="&or;UnitOfVelocitySquared"/>
        <owl:disjointWith rdf:resource="&or;UnitOfVoltage"/>
        <owl:disjointWith rdf:resource="&or;UnitOfVolume"/>
    </owl:Class>
    


    <!-- http://www.nist.gov/itl/ssd/Materials#UnitOfTemperatureDifference -->

    <owl:Class rdf:about="&mat;UnitOfTemperatureDifference">
        <rdfs:subClassOf rdf:resource="&or;UnitOfMeasure"/>
        <owl:disjointWith rdf:resource="&mat;UnitOfThermalConductivity"/>
        <owl:disjointWith rdf:resource="&mat;UnitOfToughness"/>
        <owl:disjointWith rdf:resource="&or;UnitOfEnergy"/>
        <owl:disjointWith rdf:resource="&or;UnitOfForce"/>
        <owl:disjointWith rdf:resource="&or;UnitOfMass"/>
        <owl:disjointWith rdf:resource="&or;UnitOfPressure"/>
        <owl:disjointWith rdf:resource="&or;UnitOfSpreadRate"/>
        <owl:disjointWith rdf:resource="&or;UnitOfVelocity"/>
        <owl:disjointWith rdf:resource="&or;UnitOfVelocitySquared"/>
        <owl:disjointWith rdf:resource="&or;UnitOfVoltage"/>
        <owl:disjointWith rdf:resource="&or;UnitOfVolume"/>
        <rdfs:comment xml:lang="en">A Unit of Temperature Difference is a Unit of Measure that indicates the differnce in temperature between two things.  A Celsius Degree and a Kelvin Degree have the same magnitude, and thus there is no difference between them as units of Temperature Difference.</rdfs:comment>
    </owl:Class>
    


    <!-- http://www.nist.gov/itl/ssd/Materials#UnitOfThermalConductivity -->

    <owl:Class rdf:about="&mat;UnitOfThermalConductivity">
        <rdfs:subClassOf rdf:resource="&or;UnitOfMeasure"/>
        <owl:disjointWith rdf:resource="&or;CurrencyUnit"/>
        <owl:disjointWith rdf:resource="&or;UnitOfArea"/>
        <owl:disjointWith rdf:resource="&or;UnitOfComputerStorageCapacity"/>
        <owl:disjointWith rdf:resource="&or;UnitOfDensity"/>
        <owl:disjointWith rdf:resource="&or;UnitOfDistance"/>
        <owl:disjointWith rdf:resource="&or;UnitOfDuration"/>
        <owl:disjointWith rdf:resource="&or;UnitOfEnergy"/>
        <owl:disjointWith rdf:resource="&or;UnitOfForce"/>
        <owl:disjointWith rdf:resource="&or;UnitOfMass"/>
        <owl:disjointWith rdf:resource="&or;UnitOfPressure"/>
        <owl:disjointWith rdf:resource="&or;UnitOfSpreadRate"/>
        <owl:disjointWith rdf:resource="&or;UnitOfTemperature"/>
        <owl:disjointWith rdf:resource="&or;UnitOfVoltage"/>
        <owl:disjointWith rdf:resource="&or;UnitOfVolume"/>
        <rdfs:comment xml:lang="en">Units Of Thermal Conductivity have the dimension Mass * Distance / (Temperature * Duration^3) .  The SI unit is Watts/(m K).</rdfs:comment>
    </owl:Class>
    


    <!-- http://www.nist.gov/itl/ssd/Materials#UnitOfToughness -->

    <owl:Class rdf:about="&mat;UnitOfToughness">
        <rdfs:subClassOf rdf:resource="&or;UnitOfMeasure"/>
        <owl:disjointWith rdf:resource="&or;UnitOfSpreadRate"/>
    </owl:Class>
    


    <!-- http://www.nist.gov/itl/ssd/Materials#UnitOfVolumePerMass -->

    <owl:Class rdf:about="&mat;UnitOfVolumePerMass">
        <rdfs:subClassOf rdf:resource="&or;UnitOfMeasure"/>
    </owl:Class>
    


    <!-- http://www.nist.gov/itl/ssd/Materials#UphillDiffusion -->

    <owl:Class rdf:about="&mat;UphillDiffusion">
        <rdfs:subClassOf rdf:resource="&mat;SolidDiffusion"/>
        <rdfs:seeAlso xml:lang="en">Definitions of terms for diffusion in the solid state (IUPAC Recommendations 1999), Pure Appl. Chem. 71, 1307-1325.</rdfs:seeAlso>
        <rdfs:comment xml:lang="en">Uphill Diffusion is a diffusion process in which a diffusing species migrates against its concentration gradient. It occurs in ternary and higher order systems either because of therymodynamic effects or because of differences in mobilities of the species.</rdfs:comment>
        <or:termString xml:lang="en">uphill diffusion</or:termString>
    </owl:Class>
    


    <!-- http://www.nist.gov/itl/ssd/Materials#UreaGellant -->

    <owl:Class rdf:about="&mat;UreaGellant">
        <rdfs:subClassOf rdf:resource="&mat;FluidLubricant"/>
        <owl:disjointWith rdf:resource="&mat;WhiteMineralOil"/>
        <owl:disjointWith rdf:resource="&mat;ZincOxideLubricant"/>
        <or:referenceURL rdf:datatype="&xsd;anyURI">http://www.matweb.com/index.aspx</or:referenceURL>
        <or:termString xml:lang="en">urea gellant</or:termString>
    </owl:Class>
    


    <!-- http://www.nist.gov/itl/ssd/Materials#VacancyDiffusionMechanism -->

    <owl:Class rdf:about="&mat;VacancyDiffusionMechanism">
        <rdfs:subClassOf rdf:resource="&mat;MicroscopicDiffusionMovement"/>
        <rdfs:seeAlso xml:lang="en">Definitions of terms for diffusion in the solid state (IUPAC Recommendations 1999), Pure Appl. Chem. 71, 1307-1325.</rdfs:seeAlso>
        <rdfs:comment xml:lang="en">The Vacancy Diffusion Mechanism is a mechanism where diffusion is made possible by the exchange of positions between the diffusing species and a vacancy.</rdfs:comment>
    </owl:Class>
    


    <!-- http://www.nist.gov/itl/ssd/Materials#VacancyWindEffect -->

    <owl:Class rdf:about="&mat;VacancyWindEffect">
        <rdfs:subClassOf rdf:resource="&mat;SolidDiffusion"/>
        <rdfs:seeAlso>Definitions of terms for diffusion in the solid state (IUPAC Recommendations 1999), Pure Appl. Chem. 71, 1307-1325.</rdfs:seeAlso>
        <rdfs:comment xml:lang="en">The Vacancy WindEffect occurs if diffusion gives rise to a flux of vacancies in one direction.  In this case, the availability of vacancies for a given substitutional atom is biased. The atoms will be able to jump more frequently to the ‘windward’ side since the vacancy concentration at that side is higher than at the ‘leeward’ side. Therefore there is a preferential diffusion against the vacancy wind.</rdfs:comment>
        <or:termString xml:lang="en">vacancy wind effect</or:termString>
    </owl:Class>
    


    <!-- http://www.nist.gov/itl/ssd/Materials#Vacuum -->

    <owl:Class rdf:about="&mat;Vacuum">
        <rdfs:subClassOf rdf:resource="&bc;MaterialSubstance"/>
        <owl:disjointWith rdf:resource="&or;Artifact"/>
        <rdfs:comment xml:lang="en">Vacuum is the absense of Material Substance, but can be considered to be the substance that something in a vacuum is surrounded by.</rdfs:comment>
    </owl:Class>
    


    <!-- http://www.nist.gov/itl/ssd/Materials#VanadateMineral -->

    <owl:Class rdf:about="&mat;VanadateMineral">
        <rdfs:subClassOf rdf:resource="&mat;Mineral"/>
    </owl:Class>
    


    <!-- http://www.nist.gov/itl/ssd/Materials#Vaporization -->

    <owl:Class rdf:about="&mat;Vaporization">
        <rdfs:subClassOf rdf:resource="&mat;PhaseChange"/>
        <rdfs:comment xml:lang="en">Vaporization is the Phase Change from a solid or liquid state to a gasseous state.</rdfs:comment>
    </owl:Class>
    


    <!-- http://www.nist.gov/itl/ssd/Materials#VinylPolymer -->

    <owl:Class rdf:about="&mat;VinylPolymer">
        <rdfs:subClassOf rdf:resource="&mat;Thermoplastic"/>
        <rdfs:comment xml:lang="en">Vinyl polymers are a group of polymers derived from vinyl monomers. Their backbone is an extended alkane chain, made by polymerizing an alkene group (C=C) into a chain (..-C-C-C-C-..).  Vinyl polymers are produced catalytically.</rdfs:comment>
    </owl:Class>
    


    <!-- http://www.nist.gov/itl/ssd/Materials#Viscosity -->

    <owl:Class rdf:about="&mat;Viscosity">
        <rdfs:subClassOf rdf:resource="&mat;TransportProperty"/>
        <rdfs:comment xml:lang="en">Diffusivity is the ratio between the molar flux due to molecular diffusion and the gradient in the concentration of the species (or the driving force for diffusion).  Diffusivity is generally prescribed for a given pair of species in a given phase at a given temperature. For a multi-component system, it is prescribed for each pair of species in the system.  Diffusivity is measured in Area per unit time -- in SI, m^2/s.</rdfs:comment>
    </owl:Class>
    


    <!-- http://www.nist.gov/itl/ssd/Materials#Waspaloy -->

    <owl:Class rdf:about="&mat;Waspaloy">
        <rdfs:subClassOf rdf:resource="&mat;NickelAlloy"/>
        <rdfs:subClassOf rdf:resource="&mat;Superalloy"/>
        <rdfs:comment xml:lang="en">Waspaloy is a registered trademark of United Technologies Corp that refers to an age hardening austenitic nickel-based superalloy used for high-temperature applications.</rdfs:comment>
    </owl:Class>
    


    <!-- http://www.nist.gov/itl/ssd/Materials#WhiteCastIron -->

    <owl:Class rdf:about="&mat;WhiteCastIron">
        <rdfs:subClassOf rdf:resource="&mat;CastIron"/>
        <or:referenceURL rdf:datatype="&xsd;anyURI">http://www.matweb.com/index.aspx</or:referenceURL>
        <rdfs:comment xml:lang="en">White cast iron, is a type of cast iron that is named after the white color of the fracture it forms, which is due to the presence of cementite.</rdfs:comment>
        <or:termString xml:lang="en">white cast iron</or:termString>
    </owl:Class>
    


    <!-- http://www.nist.gov/itl/ssd/Materials#WhiteMineralOil -->

    <owl:Class rdf:about="&mat;WhiteMineralOil">
        <rdfs:subClassOf rdf:resource="&mat;FluidLubricant"/>
        <owl:disjointWith rdf:resource="&mat;ZincOxideLubricant"/>
        <or:referenceURL rdf:datatype="&xsd;anyURI">http://www.matweb.com/index.aspx</or:referenceURL>
        <or:termString xml:lang="en">white mineral oil</or:termString>
    </owl:Class>
    


    <!-- http://www.nist.gov/itl/ssd/Materials#Wood -->

    <owl:Class rdf:about="&mat;Wood">
        <rdfs:subClassOf rdf:resource="&mat;CompositeMaterial"/>
        <rdfs:subClassOf rdf:resource="&mat;SolidSubstance"/>
        <or:referenceURL rdf:datatype="&xsd;anyURI">http://www.matweb.com/index.aspx</or:referenceURL>
        <rdfs:comment xml:lang="en">Wood is a hard, fibrous tissue found in many trees. It is an organic material, a natural composite of cellulose fibers (which are strong in tension) embedded in a matrix of lignin which resists compression.</rdfs:comment>
    </owl:Class>
    


    <!-- http://www.nist.gov/itl/ssd/Materials#WroughtAlloy -->

    <owl:Class rdf:about="&mat;WroughtAlloy">
        <rdfs:subClassOf rdf:resource="&mat;EngineeredAlloy"/>
        <rdfs:comment xml:lang="en">A Wrought Alloy is one in which soft heated metal is mechanically worked (often by hammering) into shape, possibly after casting.</rdfs:comment>
    </owl:Class>
    


    <!-- http://www.nist.gov/itl/ssd/Materials#ZeroFluxPlane -->

    <owl:Class rdf:about="&mat;ZeroFluxPlane">
        <rdfs:subClassOf rdf:resource="&or;PlanarRegion"/>
        <rdfs:seeAlso xml:lang="en">Definitions of terms for diffusion in the solid state (IUPAC Recommendations 1999), Pure Appl. Chem. 71, 1307-1325.</rdfs:seeAlso>
        <rdfs:comment xml:lang="en">In multicomponent diffusion-couple experiments the fluxes of individual components may go to zero at specific locations along the axis of the couple. These locations are called Zero Flux Planes.</rdfs:comment>
        <or:termString xml:lang="en">zero flux plane</or:termString>
    </owl:Class>
    


    <!-- http://www.nist.gov/itl/ssd/Materials#ZincAlloy -->

    <owl:Class rdf:about="&mat;ZincAlloy">
        <rdfs:subClassOf rdf:resource="&mat;NonFerrousAlloy"/>
        <rdfs:subClassOf>
            <owl:Restriction>
                <owl:onProperty rdf:resource="&mat;physicalDecompositions"/>
                <owl:someValuesFrom rdf:resource="&bc;Zinc"/>
            </owl:Restriction>
        </rdfs:subClassOf>
        <or:referenceURL rdf:datatype="&xsd;anyURI">http://www.matweb.com/index.aspx</or:referenceURL>
        <rdfs:comment xml:lang="en">An alloy that contains Zinc but not Iron.</rdfs:comment>
    </owl:Class>
    


    <!-- http://www.nist.gov/itl/ssd/Materials#ZincOxide -->

    <owl:Class rdf:about="&mat;ZincOxide">
        <rdfs:subClassOf rdf:resource="&bc;Oxide"/>
        <or:termString xml:lang="en">zinc oxide</or:termString>
    </owl:Class>
    


    <!-- http://www.nist.gov/itl/ssd/Materials#ZincOxideLubricant -->

    <owl:Class rdf:about="&mat;ZincOxideLubricant">
        <rdfs:subClassOf rdf:resource="&mat;FluidLubricant"/>
        <or:referenceURL rdf:datatype="&xsd;anyURI">http://www.matweb.com/index.aspx</or:referenceURL>
        <rdfs:comment xml:lang="en">Zinc Oxide Lubricant is an artificial lubricant with Zinc Oxide as a gellant.</rdfs:comment>
        <or:termString xml:lang="en">zinc oxide lubricant</or:termString>
    </owl:Class>
    


    <!-- http://www.nist.gov/itl/ssd/Materials#ZirconiumAlloy -->

    <owl:Class rdf:about="&mat;ZirconiumAlloy">
        <rdfs:subClassOf rdf:resource="&mat;NonFerrousAlloy"/>
        <rdfs:subClassOf>
            <owl:Restriction>
                <owl:onProperty rdf:resource="&mat;physicalDecompositions"/>
                <owl:someValuesFrom rdf:resource="&bc;Zirconium"/>
            </owl:Restriction>
        </rdfs:subClassOf>
        <or:referenceURL rdf:datatype="&xsd;anyURI">http://www.matweb.com/index.aspx</or:referenceURL>
    </owl:Class>
    


    <!-- http://www.nist.gov/itl/ssd/Materials#ZirconiumOxide -->

    <owl:Class rdf:about="&mat;ZirconiumOxide">
        <rdfs:subClassOf rdf:resource="&bc;Oxide"/>
        <or:referenceURL rdf:datatype="&xsd;anyURI">http://www.matweb.com/index.aspx</or:referenceURL>
        <or:termString xml:lang="en">zirconium oxide</or:termString>
    </owl:Class>
    


    <!-- http://www.nist.gov/itl/ssd/OntologyRequirements#Algorithm -->

    <owl:Class rdf:about="&or;Algorithm"/>
    


    <!-- http://www.nist.gov/itl/ssd/OntologyRequirements#ApplicationProgram -->

    <owl:Class rdf:about="&or;ApplicationProgram"/>
    


    <!-- http://www.nist.gov/itl/ssd/OntologyRequirements#Area -->

    <rdf:Description rdf:about="&or;Area">
        <rdfs:subClassOf>
            <owl:Restriction>
                <owl:onProperty rdf:resource="&or;unitsFor"/>
                <owl:allValuesFrom rdf:resource="&or;UnitOfArea"/>
            </owl:Restriction>
        </rdfs:subClassOf>
    </rdf:Description>
    


    <!-- http://www.nist.gov/itl/ssd/OntologyRequirements#AreaChart -->

    <owl:Class rdf:about="&or;AreaChart"/>
    


    <!-- http://www.nist.gov/itl/ssd/OntologyRequirements#Artifact -->

    <rdf:Description rdf:about="&or;Artifact"/>
    


    <!-- http://www.nist.gov/itl/ssd/OntologyRequirements#Certifying -->

    <owl:Class rdf:about="&or;Certifying"/>
    


    <!-- http://www.nist.gov/itl/ssd/OntologyRequirements#ComputerImageFile -->

    <owl:Class rdf:about="&or;ComputerImageFile"/>
    


    <!-- http://www.nist.gov/itl/ssd/OntologyRequirements#ComputerStorageCapacity -->

    <rdf:Description rdf:about="&or;ComputerStorageCapacity">
        <owl:disjointWith rdf:resource="&or;Energy"/>
        <owl:disjointWith rdf:resource="&or;Force"/>
        <owl:disjointWith rdf:resource="&or;Pressure"/>
    </rdf:Description>
    


    <!-- http://www.nist.gov/itl/ssd/OntologyRequirements#CreationEvent -->

    <owl:Class rdf:about="&or;CreationEvent"/>
    


    <!-- http://www.nist.gov/itl/ssd/OntologyRequirements#CurrencyUnit -->

    <rdf:Description rdf:about="&or;CurrencyUnit"/>
    


    <!-- http://www.nist.gov/itl/ssd/OntologyRequirements#CurveSegment -->

    <owl:Class rdf:about="&or;CurveSegment"/>
    


    <!-- http://www.nist.gov/itl/ssd/OntologyRequirements#DataCollection -->

    <owl:Class rdf:about="&or;DataCollection"/>
    


    <!-- http://www.nist.gov/itl/ssd/OntologyRequirements#DataTable -->

    <owl:Class rdf:about="&or;DataTable"/>
    


    <!-- http://www.nist.gov/itl/ssd/OntologyRequirements#DatabaseSearch -->

    <owl:Class rdf:about="&or;DatabaseSearch"/>
    


    <!-- http://www.nist.gov/itl/ssd/OntologyRequirements#DeployingAProduct -->

    <owl:Class rdf:about="&or;DeployingAProduct"/>
    


    <!-- http://www.nist.gov/itl/ssd/OntologyRequirements#Design -->

    <owl:Class rdf:about="&or;Design"/>
    


    <!-- http://www.nist.gov/itl/ssd/OntologyRequirements#Designing -->

    <owl:Class rdf:about="&or;Designing">
        <owl:disjointWith rdf:resource="&or;Development"/>
    </owl:Class>
    


    <!-- http://www.nist.gov/itl/ssd/OntologyRequirements#Development -->

    <rdf:Description rdf:about="&or;Development"/>
    


    <!-- http://www.nist.gov/itl/ssd/OntologyRequirements#DimensionlessUnit -->

    <rdf:Description rdf:about="&or;DimensionlessUnit"/>
    


    <!-- http://www.nist.gov/itl/ssd/OntologyRequirements#Distance -->

    <rdf:Description rdf:about="&or;Distance">
        <owl:disjointWith rdf:resource="&or;Energy"/>
        <owl:disjointWith rdf:resource="&or;Force"/>
        <owl:disjointWith rdf:resource="&or;Pressure"/>
    </rdf:Description>
    


    <!-- http://www.nist.gov/itl/ssd/OntologyRequirements#Duration -->

    <rdf:Description rdf:about="&or;Duration">
        <owl:disjointWith rdf:resource="&or;Energy"/>
        <owl:disjointWith rdf:resource="&or;Force"/>
        <owl:disjointWith rdf:resource="&or;Pressure"/>
    </rdf:Description>
    


    <!-- http://www.nist.gov/itl/ssd/OntologyRequirements#Energy -->

    <owl:Class rdf:about="&or;Energy">
        <owl:disjointWith rdf:resource="&or;Force"/>
        <owl:disjointWith rdf:resource="&or;Mass"/>
        <owl:disjointWith rdf:resource="&or;Pressure"/>
        <owl:disjointWith rdf:resource="&or;Temperature"/>
        <owl:disjointWith rdf:resource="&or;Volume"/>
    </owl:Class>
    


    <!-- http://www.nist.gov/itl/ssd/OntologyRequirements#Evaluation -->

    <owl:Class rdf:about="&or;Evaluation"/>
    


    <!-- http://www.nist.gov/itl/ssd/OntologyRequirements#EventType -->

    <owl:Class rdf:about="&or;EventType"/>
    


    <!-- http://www.nist.gov/itl/ssd/OntologyRequirements#ExperimentPlanning -->

    <owl:Class rdf:about="&or;ExperimentPlanning">
        <rdfs:subClassOf>
            <owl:Restriction>
                <owl:onProperty rdf:resource="&or;outputCreated"/>
                <owl:someValuesFrom rdf:resource="&exp;Experiment"/>
            </owl:Restriction>
        </rdfs:subClassOf>
    </owl:Class>
    


    <!-- http://www.nist.gov/itl/ssd/OntologyRequirements#ExpressedQuantity -->

    <owl:Class rdf:about="&or;ExpressedQuantity">
        <rdfs:subClassOf>
            <owl:Restriction>
                <owl:onProperty rdf:resource="&or;unitsFor"/>
                <owl:onClass rdf:resource="&or;UnitOfMeasure"/>
                <owl:qualifiedCardinality rdf:datatype="&xsd;nonNegativeInteger">1</owl:qualifiedCardinality>
            </owl:Restriction>
        </rdfs:subClassOf>
    </owl:Class>
    


    <!-- http://www.nist.gov/itl/ssd/OntologyRequirements#Force -->

    <owl:Class rdf:about="&or;Force">
        <owl:disjointWith rdf:resource="&or;Mass"/>
        <owl:disjointWith rdf:resource="&or;Pressure"/>
        <owl:disjointWith rdf:resource="&or;Temperature"/>
        <owl:disjointWith rdf:resource="&or;Volume"/>
    </owl:Class>
    


    <!-- http://www.nist.gov/itl/ssd/OntologyRequirements#GovernmentalOrganization -->

    <owl:Class rdf:about="&or;GovernmentalOrganization"/>
    


    <!-- http://www.nist.gov/itl/ssd/OntologyRequirements#GraphicalImage -->

    <owl:Class rdf:about="&or;GraphicalImage">
        <rdfs:subClassOf rdf:resource="&or;Information"/>
    </owl:Class>
    


    <!-- http://www.nist.gov/itl/ssd/OntologyRequirements#Manufacturing -->

    <owl:Class rdf:about="&or;Manufacturing"/>
    


    <!-- http://www.nist.gov/itl/ssd/OntologyRequirements#Mass -->

    <rdf:Description rdf:about="&or;Mass">
        <owl:disjointWith rdf:resource="&or;Pressure"/>
    </rdf:Description>
    


    <!-- http://www.nist.gov/itl/ssd/OntologyRequirements#MechanicalProcess -->

    <owl:Class rdf:about="&or;MechanicalProcess"/>
    


    <!-- http://www.nist.gov/itl/ssd/OntologyRequirements#NonTangibleThing -->

    <rdf:Description rdf:about="&or;NonTangibleThing">
        <rdfs:subClassOf rdf:resource="&owl;Thing"/>
    </rdf:Description>
    


    <!-- http://www.nist.gov/itl/ssd/OntologyRequirements#PredictionMethod -->

    <owl:Class rdf:about="&or;PredictionMethod"/>
    


    <!-- http://www.nist.gov/itl/ssd/OntologyRequirements#Pressure -->

    <rdf:Description rdf:about="&or;Pressure">
        <owl:disjointWith rdf:resource="&or;Temperature"/>
        <owl:disjointWith rdf:resource="&or;Volume"/>
    </rdf:Description>
    


    <!-- http://www.nist.gov/itl/ssd/OntologyRequirements#PurposefulAction -->

    <rdf:Description rdf:about="&or;PurposefulAction"/>
    


    <!-- http://www.nist.gov/itl/ssd/OntologyRequirements#Quantity -->

    <owl:Class rdf:about="&or;Quantity">
        <skos:note xml:lang="en">Similar to &quot;Property&quot; in Ashino&#39;s 2010 Minerals Ontology.</skos:note>
    </owl:Class>
    


    <!-- http://www.nist.gov/itl/ssd/OntologyRequirements#Recommending -->

    <owl:Class rdf:about="&or;Recommending"/>
    


    <!-- http://www.nist.gov/itl/ssd/OntologyRequirements#ResearchOrganization -->

    <owl:Class rdf:about="&or;ResearchOrganization"/>
    


    <!-- http://www.nist.gov/itl/ssd/OntologyRequirements#SimulationModel -->

    <owl:Class rdf:about="&or;SimulationModel"/>
    


    <!-- http://www.nist.gov/itl/ssd/OntologyRequirements#Software -->

    <owl:Class rdf:about="&or;Software"/>
    


    <!-- http://www.nist.gov/itl/ssd/OntologyRequirements#StateOfBeing -->

    <owl:Class rdf:about="&or;StateOfBeing"/>
    


    <!-- http://www.nist.gov/itl/ssd/OntologyRequirements#Technique -->

    <owl:Class rdf:about="&or;Technique"/>
    


    <!-- http://www.nist.gov/itl/ssd/OntologyRequirements#Temperature -->

    <rdf:Description rdf:about="&or;Temperature"/>
    


    <!-- http://www.nist.gov/itl/ssd/OntologyRequirements#UnitOfAcceleration -->

    <rdf:Description rdf:about="&or;UnitOfAcceleration"/>
    


    <!-- http://www.nist.gov/itl/ssd/OntologyRequirements#UnitOfArea -->

    <rdf:Description rdf:about="&or;UnitOfArea">
        <owl:disjointWith rdf:resource="&or;UnitOfDensity"/>
        <owl:disjointWith rdf:resource="&or;UnitOfSpreadRate"/>
    </rdf:Description>
    


    <!-- http://www.nist.gov/itl/ssd/OntologyRequirements#UnitOfComputerStorageCapacity -->

    <rdf:Description rdf:about="&or;UnitOfComputerStorageCapacity">
        <owl:disjointWith rdf:resource="&or;UnitOfDensity"/>
        <owl:disjointWith rdf:resource="&or;UnitOfVoltage"/>
        <owl:disjointWith rdf:resource="&or;UnitOfVolume"/>
    </rdf:Description>
    


    <!-- http://www.nist.gov/itl/ssd/OntologyRequirements#UnitOfDensity -->

    <rdf:Description rdf:about="&or;UnitOfDensity">
        <owl:disjointWith rdf:resource="&or;UnitOfDistance"/>
        <owl:disjointWith rdf:resource="&or;UnitOfDuration"/>
    </rdf:Description>
    


    <!-- http://www.nist.gov/itl/ssd/OntologyRequirements#UnitOfDistance -->

    <rdf:Description rdf:about="&or;UnitOfDistance"/>
    


    <!-- http://www.nist.gov/itl/ssd/OntologyRequirements#UnitOfDuration -->

    <rdf:Description rdf:about="&or;UnitOfDuration"/>
    


    <!-- http://www.nist.gov/itl/ssd/OntologyRequirements#UnitOfEnergy -->

    <rdf:Description rdf:about="&or;UnitOfEnergy"/>
    


    <!-- http://www.nist.gov/itl/ssd/OntologyRequirements#UnitOfForce -->

    <rdf:Description rdf:about="&or;UnitOfForce">
        <rdfs:comment xml:lang="en">A Unit Of Force is a Unit Of Measure for measuring force.  It is the product of Unit Of Mass times a Unit Of Acceleration. The SI unit is the Newton.</rdfs:comment>
    </rdf:Description>
    


    <!-- http://www.nist.gov/itl/ssd/OntologyRequirements#UnitOfMass -->

    <rdf:Description rdf:about="&or;UnitOfMass"/>
    


    <!-- http://www.nist.gov/itl/ssd/OntologyRequirements#UnitOfPressure -->

    <rdf:Description rdf:about="&or;UnitOfPressure"/>
    


    <!-- http://www.nist.gov/itl/ssd/OntologyRequirements#UnitOfSpreadRate -->

    <rdf:Description rdf:about="&or;UnitOfSpreadRate">
        <owl:disjointWith rdf:resource="&or;UnitOfTemperature"/>
        <owl:disjointWith rdf:resource="&or;UnitOfVelocity"/>
        <owl:disjointWith rdf:resource="&or;UnitOfVelocitySquared"/>
        <owl:disjointWith rdf:resource="&or;UnitOfVoltage"/>
        <owl:disjointWith rdf:resource="&or;UnitOfVolume"/>
    </rdf:Description>
    


    <!-- http://www.nist.gov/itl/ssd/OntologyRequirements#UnitOfTemperature -->

    <rdf:Description rdf:about="&or;UnitOfTemperature">
        <owl:disjointWith rdf:resource="&or;UnitOfVolume"/>
        <rdfs:comment xml:lang="en">A Unit of Temperature is a Unit of Measure used for specifying the temperature of something.  Two different Units of Temperatures may have the same magnitude, but different offsets, so are not the same.  A Degree Celsius is different from a Degree Kelvin, for example since 100 C = 373.15 K.</rdfs:comment>
    </rdf:Description>
    


    <!-- http://www.nist.gov/itl/ssd/OntologyRequirements#UnitOfVelocity -->

    <rdf:Description rdf:about="&or;UnitOfVelocity"/>
    


    <!-- http://www.nist.gov/itl/ssd/OntologyRequirements#UnitOfVelocitySquared -->

    <rdf:Description rdf:about="&or;UnitOfVelocitySquared"/>
    


    <!-- http://www.nist.gov/itl/ssd/OntologyRequirements#UnitOfVoltage -->

    <rdf:Description rdf:about="&or;UnitOfVoltage"/>
    


    <!-- http://www.nist.gov/itl/ssd/OntologyRequirements#UnitOfVolume -->

    <rdf:Description rdf:about="&or;UnitOfVolume"/>
    


    <!-- http://www.nist.gov/itl/ssd/OntologyRequirements#Volume -->

    <rdf:Description rdf:about="&or;Volume"/>
    


    <!-- 
    ///////////////////////////////////////////////////////////////////////////////////////
    //
    // Individuals
    //
    ///////////////////////////////////////////////////////////////////////////////////////
     -->

    


    <!-- http://www.nist.gov/itl/ssd/Biochem#Actinium -->

    <owl:NamedIndividual rdf:about="&bc;Actinium"/>
    


    <!-- http://www.nist.gov/itl/ssd/Biochem#Aluminum -->

    <owl:NamedIndividual rdf:about="&bc;Aluminum"/>
    


    <!-- http://www.nist.gov/itl/ssd/Biochem#Americium -->

    <owl:NamedIndividual rdf:about="&bc;Americium"/>
    


    <!-- http://www.nist.gov/itl/ssd/Biochem#Antimony -->

    <owl:NamedIndividual rdf:about="&bc;Antimony"/>
    


    <!-- http://www.nist.gov/itl/ssd/Biochem#Argon -->

    <owl:NamedIndividual rdf:about="&bc;Argon"/>
    


    <!-- http://www.nist.gov/itl/ssd/Biochem#Arsenic -->

    <owl:NamedIndividual rdf:about="&bc;Arsenic"/>
    


    <!-- http://www.nist.gov/itl/ssd/Biochem#Astatine -->

    <owl:NamedIndividual rdf:about="&bc;Astatine"/>
    


    <!-- http://www.nist.gov/itl/ssd/Biochem#Barium -->

    <owl:NamedIndividual rdf:about="&bc;Barium"/>
    


    <!-- http://www.nist.gov/itl/ssd/Biochem#Berkelium -->

    <owl:NamedIndividual rdf:about="&bc;Berkelium"/>
    


    <!-- http://www.nist.gov/itl/ssd/Biochem#Beryllium -->

    <owl:NamedIndividual rdf:about="&bc;Beryllium"/>
    


    <!-- http://www.nist.gov/itl/ssd/Biochem#Bismuth -->

    <owl:NamedIndividual rdf:about="&bc;Bismuth"/>
    


    <!-- http://www.nist.gov/itl/ssd/Biochem#Bohrium -->

    <owl:NamedIndividual rdf:about="&bc;Bohrium"/>
    


    <!-- http://www.nist.gov/itl/ssd/Biochem#Boron -->

    <owl:NamedIndividual rdf:about="&bc;Boron"/>
    


    <!-- http://www.nist.gov/itl/ssd/Biochem#Bromine -->

    <owl:NamedIndividual rdf:about="&bc;Bromine"/>
    


    <!-- http://www.nist.gov/itl/ssd/Biochem#Cadmium -->

    <owl:NamedIndividual rdf:about="&bc;Cadmium"/>
    


    <!-- http://www.nist.gov/itl/ssd/Biochem#Calcium -->

    <owl:NamedIndividual rdf:about="&bc;Calcium"/>
    


    <!-- http://www.nist.gov/itl/ssd/Biochem#Californium -->

    <owl:NamedIndividual rdf:about="&bc;Californium"/>
    


    <!-- http://www.nist.gov/itl/ssd/Biochem#Carbon -->

    <owl:NamedIndividual rdf:about="&bc;Carbon"/>
    


    <!-- http://www.nist.gov/itl/ssd/Biochem#CcsPerLiter -->

    <or:MetricUnit rdf:about="&bc;CcsPerLiter">
        <rdf:type rdf:resource="&or;DimensionlessUnit"/>
    </or:MetricUnit>
    


    <!-- http://www.nist.gov/itl/ssd/Biochem#Cerium -->

    <owl:NamedIndividual rdf:about="&bc;Cerium"/>
    


    <!-- http://www.nist.gov/itl/ssd/Biochem#Cesium -->

    <owl:NamedIndividual rdf:about="&bc;Cesium"/>
    


    <!-- http://www.nist.gov/itl/ssd/Biochem#Chlorine -->

    <owl:NamedIndividual rdf:about="&bc;Chlorine"/>
    


    <!-- http://www.nist.gov/itl/ssd/Biochem#Chromium -->

    <owl:NamedIndividual rdf:about="&bc;Chromium"/>
    


    <!-- http://www.nist.gov/itl/ssd/Biochem#Cobalt -->

    <owl:NamedIndividual rdf:about="&bc;Cobalt"/>
    


    <!-- http://www.nist.gov/itl/ssd/Biochem#ConcentrationByMass -->

    <rdf:Description rdf:about="&bc;ConcentrationByMass">
        <or:unitTypeFor rdf:resource="&bc;UnitOfConcentrationByMass"/>
    </rdf:Description>
    


    <!-- http://www.nist.gov/itl/ssd/Biochem#ConcentrationByVolume -->

    <rdf:Description rdf:about="&bc;ConcentrationByVolume">
        <or:unitTypeFor rdf:resource="&bc;UnitOfConcentrationByVolume"/>
    </rdf:Description>
    


    <!-- http://www.nist.gov/itl/ssd/Biochem#Copernicium -->

    <owl:NamedIndividual rdf:about="&bc;Copernicium"/>
    


    <!-- http://www.nist.gov/itl/ssd/Biochem#Copper -->

    <owl:NamedIndividual rdf:about="&bc;Copper"/>
    


    <!-- http://www.nist.gov/itl/ssd/Biochem#Curium -->

    <owl:NamedIndividual rdf:about="&bc;Curium"/>
    


    <!-- http://www.nist.gov/itl/ssd/Biochem#Dubnium -->

    <owl:NamedIndividual rdf:about="&bc;Dubnium"/>
    


    <!-- http://www.nist.gov/itl/ssd/Biochem#Dysprosium -->

    <owl:NamedIndividual rdf:about="&bc;Dysprosium"/>
    


    <!-- http://www.nist.gov/itl/ssd/Biochem#Einsteinium -->

    <owl:NamedIndividual rdf:about="&bc;Einsteinium"/>
    


    <!-- http://www.nist.gov/itl/ssd/Biochem#Erbium -->

    <owl:NamedIndividual rdf:about="&bc;Erbium"/>
    


    <!-- http://www.nist.gov/itl/ssd/Biochem#Europium -->

    <owl:NamedIndividual rdf:about="&bc;Europium"/>
    


    <!-- http://www.nist.gov/itl/ssd/Biochem#Fermium -->

    <owl:NamedIndividual rdf:about="&bc;Fermium"/>
    


    <!-- http://www.nist.gov/itl/ssd/Biochem#Fluorine -->

    <owl:NamedIndividual rdf:about="&bc;Fluorine"/>
    


    <!-- http://www.nist.gov/itl/ssd/Biochem#Francium -->

    <owl:NamedIndividual rdf:about="&bc;Francium"/>
    


    <!-- http://www.nist.gov/itl/ssd/Biochem#Germanium -->

    <owl:NamedIndividual rdf:about="&bc;Germanium"/>
    


    <!-- http://www.nist.gov/itl/ssd/Biochem#Gold -->

    <owl:NamedIndividual rdf:about="&bc;Gold"/>
    


    <!-- http://www.nist.gov/itl/ssd/Biochem#GramsPerLiter -->

    <or:UnitOfDensity rdf:about="&bc;GramsPerLiter">
        <rdf:type rdf:resource="&or;MetricUnit"/>
    </or:UnitOfDensity>
    


    <!-- http://www.nist.gov/itl/ssd/Biochem#Hafnium -->

    <owl:NamedIndividual rdf:about="&bc;Hafnium"/>
    


    <!-- http://www.nist.gov/itl/ssd/Biochem#Hassium -->

    <owl:NamedIndividual rdf:about="&bc;Hassium"/>
    


    <!-- http://www.nist.gov/itl/ssd/Biochem#Helium -->

    <owl:NamedIndividual rdf:about="&bc;Helium"/>
    


    <!-- http://www.nist.gov/itl/ssd/Biochem#Holmium -->

    <owl:NamedIndividual rdf:about="&bc;Holmium"/>
    


    <!-- http://www.nist.gov/itl/ssd/Biochem#Hydrogen -->

    <owl:NamedIndividual rdf:about="&bc;Hydrogen"/>
    


    <!-- http://www.nist.gov/itl/ssd/Biochem#Indium -->

    <owl:NamedIndividual rdf:about="&bc;Indium"/>
    


    <!-- http://www.nist.gov/itl/ssd/Biochem#Iodine -->

    <owl:NamedIndividual rdf:about="&bc;Iodine"/>
    


    <!-- http://www.nist.gov/itl/ssd/Biochem#Iridium -->

    <owl:NamedIndividual rdf:about="&bc;Iridium"/>
    


    <!-- http://www.nist.gov/itl/ssd/Biochem#Iron -->

    <owl:NamedIndividual rdf:about="&bc;Iron"/>
    


    <!-- http://www.nist.gov/itl/ssd/Biochem#Krypton -->

    <owl:NamedIndividual rdf:about="&bc;Krypton"/>
    


    <!-- http://www.nist.gov/itl/ssd/Biochem#Lanthanum -->

    <owl:NamedIndividual rdf:about="&bc;Lanthanum"/>
    


    <!-- http://www.nist.gov/itl/ssd/Biochem#Lawrencium -->

    <owl:NamedIndividual rdf:about="&bc;Lawrencium"/>
    


    <!-- http://www.nist.gov/itl/ssd/Biochem#Lead -->

    <owl:NamedIndividual rdf:about="&bc;Lead"/>
    


    <!-- http://www.nist.gov/itl/ssd/Biochem#Lithium -->

    <owl:NamedIndividual rdf:about="&bc;Lithium"/>
    


    <!-- http://www.nist.gov/itl/ssd/Biochem#Lutetium -->

    <owl:NamedIndividual rdf:about="&bc;Lutetium"/>
    


    <!-- http://www.nist.gov/itl/ssd/Biochem#Magnesium -->

    <owl:NamedIndividual rdf:about="&bc;Magnesium"/>
    


    <!-- http://www.nist.gov/itl/ssd/Biochem#Manganese -->

    <owl:NamedIndividual rdf:about="&bc;Manganese"/>
    


    <!-- http://www.nist.gov/itl/ssd/Biochem#Meitnerium -->

    <owl:NamedIndividual rdf:about="&bc;Meitnerium"/>
    


    <!-- http://www.nist.gov/itl/ssd/Biochem#Mendelevium -->

    <owl:NamedIndividual rdf:about="&bc;Mendelevium"/>
    


    <!-- http://www.nist.gov/itl/ssd/Biochem#Mercury -->

    <owl:NamedIndividual rdf:about="&bc;Mercury"/>
    


    <!-- http://www.nist.gov/itl/ssd/Biochem#Molybdenum -->

    <owl:NamedIndividual rdf:about="&bc;Molybdenum"/>
    


    <!-- http://www.nist.gov/itl/ssd/Biochem#Neodymium -->

    <owl:NamedIndividual rdf:about="&bc;Neodymium"/>
    


    <!-- http://www.nist.gov/itl/ssd/Biochem#Neon -->

    <owl:NamedIndividual rdf:about="&bc;Neon"/>
    


    <!-- http://www.nist.gov/itl/ssd/Biochem#Neptunium -->

    <owl:NamedIndividual rdf:about="&bc;Neptunium"/>
    


    <!-- http://www.nist.gov/itl/ssd/Biochem#Nickel -->

    <owl:NamedIndividual rdf:about="&bc;Nickel"/>
    


    <!-- http://www.nist.gov/itl/ssd/Biochem#Niobium -->

    <owl:NamedIndividual rdf:about="&bc;Niobium"/>
    


    <!-- http://www.nist.gov/itl/ssd/Biochem#Nitrogen -->

    <owl:NamedIndividual rdf:about="&bc;Nitrogen"/>
    


    <!-- http://www.nist.gov/itl/ssd/Biochem#Nobelium -->

    <owl:NamedIndividual rdf:about="&bc;Nobelium"/>
    


    <!-- http://www.nist.gov/itl/ssd/Biochem#Osmium -->

    <owl:NamedIndividual rdf:about="&bc;Osmium"/>
    


    <!-- http://www.nist.gov/itl/ssd/Biochem#Oxide -->

    <owl:NamedIndividual rdf:about="&bc;Oxide"/>
    


    <!-- http://www.nist.gov/itl/ssd/Biochem#Oxygen -->

    <owl:NamedIndividual rdf:about="&bc;Oxygen"/>
    


    <!-- http://www.nist.gov/itl/ssd/Biochem#PH -->

    <rdf:Description rdf:about="&bc;PH">
        <or:unitTypeFor rdf:resource="&or;DimensionlessUnit"/>
    </rdf:Description>
    


    <!-- http://www.nist.gov/itl/ssd/Biochem#Palladium -->

    <owl:NamedIndividual rdf:about="&bc;Palladium"/>
    


    <!-- http://www.nist.gov/itl/ssd/Biochem#PercentByVolume -->

    <or:DimensionlessUnit rdf:about="&bc;PercentByVolume"/>
    


    <!-- http://www.nist.gov/itl/ssd/Biochem#PercentByWeight -->

    <or:DimensionlessUnit rdf:about="&bc;PercentByWeight">
        <or:termString xml:lang="en">mass percent</or:termString>
        <or:termString xml:lang="en">percent by weight</or:termString>
        <or:termString xml:lang="en">weight percent</or:termString>
    </or:DimensionlessUnit>
    


    <!-- http://www.nist.gov/itl/ssd/Biochem#Phosphorus -->

    <owl:NamedIndividual rdf:about="&bc;Phosphorus"/>
    


    <!-- http://www.nist.gov/itl/ssd/Biochem#Platinum -->

    <owl:NamedIndividual rdf:about="&bc;Platinum"/>
    


    <!-- http://www.nist.gov/itl/ssd/Biochem#Plutonium -->

    <owl:NamedIndividual rdf:about="&bc;Plutonium"/>
    


    <!-- http://www.nist.gov/itl/ssd/Biochem#Polonium -->

    <owl:NamedIndividual rdf:about="&bc;Polonium"/>
    


    <!-- http://www.nist.gov/itl/ssd/Biochem#Potassium -->

    <owl:NamedIndividual rdf:about="&bc;Potassium"/>
    


    <!-- http://www.nist.gov/itl/ssd/Biochem#Praseodymium -->

    <owl:NamedIndividual rdf:about="&bc;Praseodymium"/>
    


    <!-- http://www.nist.gov/itl/ssd/Biochem#Promethium -->

    <owl:NamedIndividual rdf:about="&bc;Promethium"/>
    


    <!-- http://www.nist.gov/itl/ssd/Biochem#Protactinium -->

    <owl:NamedIndividual rdf:about="&bc;Protactinium"/>
    


    <!-- http://www.nist.gov/itl/ssd/Biochem#Radium -->

    <owl:NamedIndividual rdf:about="&bc;Radium"/>
    


    <!-- http://www.nist.gov/itl/ssd/Biochem#Radon -->

    <owl:NamedIndividual rdf:about="&bc;Radon"/>
    


    <!-- http://www.nist.gov/itl/ssd/Biochem#Rhenium -->

    <owl:NamedIndividual rdf:about="&bc;Rhenium"/>
    


    <!-- http://www.nist.gov/itl/ssd/Biochem#Rhodium -->

    <owl:NamedIndividual rdf:about="&bc;Rhodium"/>
    


    <!-- http://www.nist.gov/itl/ssd/Biochem#Samarium -->

    <owl:NamedIndividual rdf:about="&bc;Samarium"/>
    


    <!-- http://www.nist.gov/itl/ssd/Biochem#Scandium -->

    <owl:NamedIndividual rdf:about="&bc;Scandium"/>
    


    <!-- http://www.nist.gov/itl/ssd/Biochem#Seaborgium -->

    <owl:NamedIndividual rdf:about="&bc;Seaborgium"/>
    


    <!-- http://www.nist.gov/itl/ssd/Biochem#Selenium -->

    <owl:NamedIndividual rdf:about="&bc;Selenium"/>
    


    <!-- http://www.nist.gov/itl/ssd/Biochem#Silicon -->

    <owl:NamedIndividual rdf:about="&bc;Silicon"/>
    


    <!-- http://www.nist.gov/itl/ssd/Biochem#Silver -->

    <owl:NamedIndividual rdf:about="&bc;Silver"/>
    


    <!-- http://www.nist.gov/itl/ssd/Biochem#Sodium -->

    <owl:NamedIndividual rdf:about="&bc;Sodium"/>
    


    <!-- http://www.nist.gov/itl/ssd/Biochem#Strontium -->

    <owl:NamedIndividual rdf:about="&bc;Strontium"/>
    


    <!-- http://www.nist.gov/itl/ssd/Biochem#Sulfur -->

    <owl:NamedIndividual rdf:about="&bc;Sulfur"/>
    


    <!-- http://www.nist.gov/itl/ssd/Biochem#Tantalum -->

    <owl:NamedIndividual rdf:about="&bc;Tantalum"/>
    


    <!-- http://www.nist.gov/itl/ssd/Biochem#Technetium -->

    <owl:NamedIndividual rdf:about="&bc;Technetium"/>
    


    <!-- http://www.nist.gov/itl/ssd/Biochem#Tellurium -->

    <owl:NamedIndividual rdf:about="&bc;Tellurium"/>
    


    <!-- http://www.nist.gov/itl/ssd/Biochem#Terbium -->

    <owl:NamedIndividual rdf:about="&bc;Terbium"/>
    


    <!-- http://www.nist.gov/itl/ssd/Biochem#Thallium -->

    <owl:NamedIndividual rdf:about="&bc;Thallium"/>
    


    <!-- http://www.nist.gov/itl/ssd/Biochem#Thorium -->

    <owl:NamedIndividual rdf:about="&bc;Thorium"/>
    


    <!-- http://www.nist.gov/itl/ssd/Biochem#Thulium -->

    <owl:NamedIndividual rdf:about="&bc;Thulium"/>
    


    <!-- http://www.nist.gov/itl/ssd/Biochem#Tin -->

    <owl:NamedIndividual rdf:about="&bc;Tin"/>
    


    <!-- http://www.nist.gov/itl/ssd/Biochem#Titanium -->

    <owl:NamedIndividual rdf:about="&bc;Titanium"/>
    


    <!-- http://www.nist.gov/itl/ssd/Biochem#Uranium -->

    <owl:NamedIndividual rdf:about="&bc;Uranium"/>
    


    <!-- http://www.nist.gov/itl/ssd/Biochem#Vanadium -->

    <owl:NamedIndividual rdf:about="&bc;Vanadium"/>
    


    <!-- http://www.nist.gov/itl/ssd/Biochem#Water -->

    <owl:NamedIndividual rdf:about="&bc;Water"/>
    


    <!-- http://www.nist.gov/itl/ssd/Biochem#Xenon -->

    <owl:NamedIndividual rdf:about="&bc;Xenon"/>
    


    <!-- http://www.nist.gov/itl/ssd/Biochem#Ytterbium -->

    <owl:NamedIndividual rdf:about="&bc;Ytterbium"/>
    


    <!-- http://www.nist.gov/itl/ssd/Biochem#Yttrium -->

    <owl:NamedIndividual rdf:about="&bc;Yttrium"/>
    


    <!-- http://www.nist.gov/itl/ssd/Biochem#Zinc -->

    <owl:NamedIndividual rdf:about="&bc;Zinc"/>
    


    <!-- http://www.nist.gov/itl/ssd/Biochem#Zirconium -->

    <owl:NamedIndividual rdf:about="&bc;Zirconium"/>
    


    <!-- http://www.nist.gov/itl/ssd/Materials#ActivationVolumeForDiffusion -->

    <owl:NamedIndividual rdf:about="&mat;ActivationVolumeForDiffusion">
        <rdf:type rdf:resource="&mat;DiffusionProperty"/>
        <rdfs:seeAlso xml:lang="en">Definitions of terms for diffusion in the solid state (IUPAC Recommendations 1999), Pure Appl. Chem. 71, 1307-1325.</rdfs:seeAlso>
        <rdfs:comment xml:lang="en">The Activiation Volume for Diffusion is a parameter for a diffusiive system </rdfs:comment>
        <or:unitTypeFor rdf:resource="&or;UnitOfVolume"/>
    </owl:NamedIndividual>
    


    <!-- http://www.nist.gov/itl/ssd/Materials#Alloy -->

    <owl:NamedIndividual rdf:about="&mat;Alloy">
        <rdf:type rdf:resource="&mat;MaterialForm"/>
    </owl:NamedIndividual>
    


    <!-- http://www.nist.gov/itl/ssd/Materials#AluminumAlloy -->

    <owl:NamedIndividual rdf:about="&mat;AluminumAlloy">
        <rdf:type rdf:resource="&mat;NonFerrousAlloyTypeByMainConstituent"/>
        <or:referenceURL rdf:datatype="&xsd;anyURI">http://www.matweb.com/index.aspx</or:referenceURL>
        <rdfs:comment xml:lang="en">An alloy that contains Aluminum but not Iron.</rdfs:comment>
        <bc:primaryConstituentType rdf:resource="&bc;Aluminum"/>
    </owl:NamedIndividual>
    


    <!-- http://www.nist.gov/itl/ssd/Materials#AluminumOxide -->

    <owl:NamedIndividual rdf:about="&mat;AluminumOxide">
        <rdf:type rdf:resource="&bc;ChemicalSubstanceTypeByChemicalSpecies"/>
        <or:referenceURL rdf:datatype="&xsd;anyURI">http://www.matweb.com/index.aspx</or:referenceURL>
        <or:termString xml:lang="en">aluminum oxide</or:termString>
    </owl:NamedIndividual>
    


    <!-- http://www.nist.gov/itl/ssd/Materials#AmorphousSubstance -->

    <owl:NamedIndividual rdf:about="&mat;AmorphousSubstance">
        <rdf:type rdf:resource="&mat;MaterialForm"/>
        <rdf:type rdf:resource="&mat;MaterialPhaseComposition"/>
        <rdfs:comment xml:lang="en">Material in a solid amorphous (non-crystalline) phase.</rdfs:comment>
    </owl:NamedIndividual>
    


    <!-- http://www.nist.gov/itl/ssd/Materials#Ampere -->

    <owl:NamedIndividual rdf:about="&mat;Ampere">
        <rdf:type rdf:resource="&mat;UnitOfElectricCurrent"/>
        <rdf:type rdf:resource="&or;SI_Unit"/>
    </owl:NamedIndividual>
    


    <!-- http://www.nist.gov/itl/ssd/Materials#AreaOfSurface -->

    <owl:NamedIndividual rdf:about="&mat;AreaOfSurface">
        <rdf:type rdf:resource="&mat;MeasurableMechanicalProperty"/>
        <or:unitTypeFor rdf:resource="&or;UnitOfArea"/>
    </owl:NamedIndividual>
    


    <!-- http://www.nist.gov/itl/ssd/Materials#AreaPerTime -->

    <owl:NamedIndividual rdf:about="&mat;AreaPerTime">
        <rdf:type rdf:resource="&or;MeasurableQuantityType"/>
    </owl:NamedIndividual>
    


    <!-- http://www.nist.gov/itl/ssd/Materials#Auricupride -->

    <owl:NamedIndividual rdf:about="&mat;Auricupride">
        <rdf:type rdf:resource="&mat;AlloyType"/>
        <rdf:type rdf:resource="&mat;MineralType"/>
        <strunzClassification rdf:datatype="&xsd;string">01.AA.10a</strunzClassification>
        <rdfs:comment xml:lang="en">Auricupride is a natural alloy that combines copper and gold. Its chemical formula is Cu3Au. The alloy crystallizes in the Cubic crystal system and occurs as malleable grains or platey masses. It is an opaque yellow with a reddish tint. It has a hardness of 3.5 and a specific gravity of 11.5.</rdfs:comment>
        <bc:primaryConstituentType rdf:resource="&bc;Copper"/>
        <bc:componentElement rdf:resource="&bc;Copper"/>
        <bc:componentElement rdf:resource="&bc;Gold"/>
    </owl:NamedIndividual>
    


    <!-- http://www.nist.gov/itl/ssd/Materials#AziotropicPressure -->

    <owl:NamedIndividual rdf:about="&mat;AziotropicPressure">
        <rdf:type rdf:resource="&mat;ThermalProperty"/>
        <or:referenceURL rdf:datatype="&xsd;anyURI">http://www.iupac.org/namespaces/ThermoML</or:referenceURL>
        <rdfs:comment xml:lang="en">The aziotropic pressure of an aziotrope (a liquid mixture in which the composition is the same for a boiling liquid and the gas boiling off) is the pressure at which boiling occurs at a given temperature.</rdfs:comment>
        <or:termString xml:lang="en">aziotropic pressure</or:termString>
        <or:unitTypeFor rdf:resource="&or;UnitOfPressure"/>
    </owl:NamedIndividual>
    


    <!-- http://www.nist.gov/itl/ssd/Materials#AziotropicTemperature -->

    <owl:NamedIndividual rdf:about="&mat;AziotropicTemperature">
        <rdf:type rdf:resource="&mat;PressureDependentProperty"/>
        <rdf:type rdf:resource="&mat;ThermalProperty"/>
        <or:referenceURL rdf:datatype="&xsd;anyURI">http://www.iupac.org/namespaces/ThermoML</or:referenceURL>
        <rdfs:comment xml:lang="en">The aziotropic temperature of an aziotrope (a liquid mixture in which the composition is the same for a boiling liquid and the gas boiling off) is the temperature at which boiling occurs at a given pressure.</rdfs:comment>
        <or:termString xml:lang="en">aziotropic temperature</or:termString>
        <or:unitTypeFor rdf:resource="&or;UnitOfTemperature"/>
    </owl:NamedIndividual>
    


    <!-- http://www.nist.gov/itl/ssd/Materials#BTUperFtHourFahrenheit -->

    <owl:NamedIndividual rdf:about="&mat;BTUperFtHourFahrenheit">
        <rdf:type rdf:resource="&mat;UnitOfThermalConductivity"/>
        <rdf:type rdf:resource="&or;NonMetricUnit"/>
    </owl:NamedIndividual>
    


    <!-- http://www.nist.gov/itl/ssd/Materials#BodyCenteredCubicCrystalStructure -->

    <owl:NamedIndividual rdf:about="&mat;BodyCenteredCubicCrystalStructure">
        <rdf:type rdf:resource="&mat;CrystalStructure"/>
        <or:nickName>bcc</or:nickName>
    </owl:NamedIndividual>
    


    <!-- http://www.nist.gov/itl/ssd/Materials#BoilingTemperature -->

    <owl:NamedIndividual rdf:about="&mat;BoilingTemperature">
        <rdf:type rdf:resource="&mat;PressureDependentProperty"/>
        <rdf:type rdf:resource="&mat;ThermalProperty"/>
        <or:referenceURL rdf:datatype="&xsd;anyURI">http://www.iupac.org/namespaces/ThermoML</or:referenceURL>
        <or:termString xml:lang="en">boiling point</or:termString>
        <or:termString xml:lang="en">boiling temperature</or:termString>
        <or:unitTypeFor rdf:resource="&or;UnitOfTemperature"/>
    </owl:NamedIndividual>
    


    <!-- http://www.nist.gov/itl/ssd/Materials#BoilingTemperatureAt1Atmosphere -->

    <owl:NamedIndividual rdf:about="&mat;BoilingTemperatureAt1Atmosphere">
        <rdf:type rdf:resource="&mat;ThermalProperty"/>
        <or:referenceURL rdf:datatype="&xsd;anyURI">http://www.iupac.org/namespaces/ThermoML</or:referenceURL>
        <or:termString xml:lang="en">boiling temperature at 1.0 atmospheres</or:termString>
        <or:termString xml:lang="en">boiling temperature at 101.325 kPa</or:termString>
        <or:termString xml:lang="en">boiling temperature at P=10132.5 Pa</or:termString>
        <or:termString xml:lang="en">boiling temperature at standard pressure</or:termString>
        <or:termString xml:lang="en">normal boiling temperature</or:termString>
        <or:termString xml:lang="en">normal melting temperature</or:termString>
        <or:unitTypeFor rdf:resource="&or;UnitOfTemperature"/>
    </owl:NamedIndividual>
    


    <!-- http://www.nist.gov/itl/ssd/Materials#Brass -->

    <owl:NamedIndividual rdf:about="&mat;Brass">
        <rdf:type rdf:resource="&mat;AlloyType"/>
        <rdfs:comment xml:lang="en">Brass is an alloy of copper and zinc; the proportions of zinc and copper can be varied to create a range of brasses with varying properties.  Other metals (lead, tin, aluminum, nickel, traces of iron) may be added in specific proportions for specific brass alloys.</rdfs:comment>
        <bc:componentElement rdf:resource="&bc;Copper"/>
        <bc:primaryConstituentType rdf:resource="&bc;Copper"/>
        <bc:componentElement rdf:resource="&bc;Zinc"/>
    </owl:NamedIndividual>
    


    <!-- http://www.nist.gov/itl/ssd/Materials#BreakdownPotential -->

    <owl:NamedIndividual rdf:about="&mat;BreakdownPotential">
        <rdf:type rdf:resource="&mat;DielectricProperty"/>
    </owl:NamedIndividual>
    


    <!-- http://www.nist.gov/itl/ssd/Materials#BrinellHardness -->

    <owl:NamedIndividual rdf:about="&mat;BrinellHardness">
        <rdf:type rdf:resource="&mat;IndentationHardness"/>
    </owl:NamedIndividual>
    


    <!-- http://www.nist.gov/itl/ssd/Materials#Bronze -->

    <owl:NamedIndividual rdf:about="&mat;Bronze">
        <rdf:type rdf:resource="&mat;AlloyType"/>
        <rdfs:comment xml:lang="en">Bronze is a metal alloy consisting primarily of copper, usually with tin as the main additive. There are many different bronze alloys but modern bronze is typically 88% copper and 12% tin.  Bronzes with the secondary additive other than tin or zinc include Aluminum Bronze and Silicon Bronze.  Phosphor Bronze is a Brass (main additive is zinc) with a significant amount of Phosphor (up to 1%) as an additional additive.</rdfs:comment>
        <bc:primaryConstituentType rdf:resource="&bc;Copper"/>
        <bc:componentElement rdf:resource="&bc;Copper"/>
        <bc:componentElement rdf:resource="&bc;Tin"/>
    </owl:NamedIndividual>
    


    <!-- http://www.nist.gov/itl/ssd/Materials#BulkDensity -->

    <owl:NamedIndividual rdf:about="&mat;BulkDensity">
        <rdf:type rdf:resource="&mat;MeasurableMechanicalProperty"/>
        <rdfs:comment xml:lang="en">Bulk density is a property of powders, granules and other particulate matter. It is defined as the mass of the particles of the material divided by the total volume they occupy. The total volume includes particle volume, inter-particle void volume and internal pore volume.</rdfs:comment>
        <or:unitTypeFor rdf:resource="&or;UnitOfDensity"/>
    </owl:NamedIndividual>
    


    <!-- http://www.nist.gov/itl/ssd/Materials#BulkModulus -->

    <owl:NamedIndividual rdf:about="&mat;BulkModulus">
        <rdf:type rdf:resource="&mat;ElasticModulus"/>
        <rdf:type rdf:resource="&mat;Stiffness"/>
        <rdfs:comment>bulk modulus</rdfs:comment>
        <rdfs:comment xml:lang="en">The Bulk Modulus is the inverse of the Isothermal Compressibility.</rdfs:comment>
        <or:unitTypeFor rdf:resource="&or;UnitOfPressure"/>
    </owl:NamedIndividual>
    


    <!-- http://www.nist.gov/itl/ssd/Materials#BulkModulusPressureDerivitive -->

    <owl:NamedIndividual rdf:about="&mat;BulkModulusPressureDerivitive">
        <rdf:type rdf:resource="&mat;DeformationProperty"/>
    </owl:NamedIndividual>
    


    <!-- http://www.nist.gov/itl/ssd/Materials#CALAPHAD -->

    <owl:NamedIndividual rdf:about="&mat;CALAPHAD">
        <rdf:type rdf:resource="&or;PredictionMethod"/>
        <rdfs:comment xml:lang="en">CALPHAD is a method for the CALculation of PHAse Diagrams of multi-phase mixtures such as alloys.</rdfs:comment>
    </owl:NamedIndividual>
    


    <!-- http://www.nist.gov/itl/ssd/Materials#CaloriePerGramKelvin -->

    <owl:NamedIndividual rdf:about="&mat;CaloriePerGramKelvin">
        <rdf:type rdf:resource="&mat;UnitOfSpecificHeatCapacity"/>
        <rdf:type rdf:resource="&or;NonMetricUnit"/>
        <or:termString>cal/g/K</or:termString>
        <or:termString xml:lang="en">calorie per gram Kelvin</or:termString>
    </owl:NamedIndividual>
    


    <!-- http://www.nist.gov/itl/ssd/Materials#CaloriePerMole -->

    <owl:NamedIndividual rdf:about="&mat;CaloriePerMole">
        <rdf:type rdf:resource="&mat;UnitOfEnergyPerAmount"/>
        <rdf:type rdf:resource="&or;NonMetricUnit"/>
        <or:termString xml:lang="en">cal/mol</or:termString>
        <or:termString xml:lang="en">calorie per mole</or:termString>
        <or:termString xml:lang="en">gram-calorie per mole</or:termString>
    </owl:NamedIndividual>
    


    <!-- http://www.nist.gov/itl/ssd/Materials#CastAlloy -->

    <owl:NamedIndividual rdf:about="&mat;CastAlloy">
        <rdf:type rdf:resource="&mat;AlloyTypeByFormingProcess"/>
        <rdfs:comment xml:lang="en">A Cast Alloy is one which is formed by pouring molten metal into a mold and letting it harden.</rdfs:comment>
    </owl:NamedIndividual>
    


    <!-- http://www.nist.gov/itl/ssd/Materials#Casting_MaterialProcessing -->

    <owl:NamedIndividual rdf:about="&mat;Casting_MaterialProcessing"/>
    


    <!-- http://www.nist.gov/itl/ssd/Materials#CelsiusDegree -->

    <owl:NamedIndividual rdf:about="&mat;CelsiusDegree">
        <rdf:type rdf:resource="&mat;UnitOfTemperatureDifference"/>
        <rdfs:comment xml:lang="en">A Celsius Degree is the Unit Of Temperature Difference equal to the differerence between zero and one Degrees Celsius or zero and one Degrees Kelvin.   A Celsius Degree has the same magnitude as a Kelvin degree.  A Fahrenheit Degree is 5/9 of a Celsius Degree.</rdfs:comment>
        <or:termString xml:lang="en">Celsius degree</or:termString>
        <or:termString xml:lang="en">Kelvin degree</or:termString>
    </owl:NamedIndividual>
    


    <!-- http://www.nist.gov/itl/ssd/Materials#ChannelDieCompression -->

    <owl:NamedIndividual rdf:about="&mat;ChannelDieCompression"/>
    


    <!-- http://www.nist.gov/itl/ssd/Materials#ChemicalDiffusionCoefficient -->

    <owl:NamedIndividual rdf:about="&mat;ChemicalDiffusionCoefficient">
        <rdf:type rdf:resource="&bc;MeasurableChemicalProperty"/>
        <rdf:type rdf:resource="&mat;DiffusionProperty"/>
        <rdfs:seeAlso xml:lang="en">Definitions of terms for diffusion in the solid state (IUPAC Recommendations 1999), Pure Appl. Chem. 71, 1307-1325.</rdfs:seeAlso>
        <or:unitTypeFor rdf:resource="&mat;UnitOfAreaPerTime"/>
    </owl:NamedIndividual>
    


    <!-- http://www.nist.gov/itl/ssd/Materials#ChemicalPotential -->

    <owl:NamedIndividual rdf:about="&mat;ChemicalPotential">
        <rdf:type rdf:resource="&bc;MeasurableChemicalProperty"/>
        <rdfs:comment xml:lang="en">The chemical potential of a species in a mixture can be defined as the ratio of the free energy of the mixture to the amount of that species in the mixture (usually calculated in moles).  Electrons in solids have a similar chemical potential, being the change in free energy when electrons are added or removed from the system. In the case of electrons, the chemical potential is usually expressed in energy per particle rather than energy per mole</rdfs:comment>
        <or:termString xml:lang="en">chemical potential</or:termString>
        <or:termString xml:lang="en">partial molar free energy</or:termString>
        <or:unitTypeFor rdf:resource="&mat;UnitOfEnergyPerAmount"/>
    </owl:NamedIndividual>
    


    <!-- http://www.nist.gov/itl/ssd/Materials#Coating -->

    <owl:NamedIndividual rdf:about="&mat;Coating"/>
    


    <!-- http://www.nist.gov/itl/ssd/Materials#CobaltAlloy -->

    <owl:NamedIndividual rdf:about="&mat;CobaltAlloy">
        <rdf:type rdf:resource="&mat;NonFerrousAlloyTypeByMainConstituent"/>
        <or:referenceURL rdf:datatype="&xsd;anyURI">http://www.matweb.com/index.aspx</or:referenceURL>
        <rdfs:comment xml:lang="en">An alloy that contains Cobalt but not Iron.</rdfs:comment>
        <bc:primaryConstituentType rdf:resource="&bc;Cobalt"/>
    </owl:NamedIndividual>
    


    <!-- http://www.nist.gov/itl/ssd/Materials#ColinearInterstitialcyMechanism -->

    <owl:NamedIndividual rdf:about="&mat;ColinearInterstitialcyMechanism">
        <rdf:type rdf:resource="&mat;DiffusionMovementMechanism"/>
        <rdfs:seeAlso>Definitions of terms for diffusion in the solid state (IUPAC Recommendations 1999), Pure Appl. Chem. 71, 1307-1325.</rdfs:seeAlso>
        <rdfs:comment xml:lang="en">The Collinear Iinterstitialcy Mechanism is an interstitialcy mechanism in which an interstitial atom and the lattice atom which it displaces move along the same straight line.</rdfs:comment>
    </owl:NamedIndividual>
    


    <!-- http://www.nist.gov/itl/ssd/Materials#CompactedPowderAlloy -->

    <owl:NamedIndividual rdf:about="&mat;CompactedPowderAlloy">
        <rdf:type rdf:resource="&mat;AlloyTypeByFormingProcess"/>
        <rdfs:comment xml:lang="en">A Compacted Powder Alloy is produced by the  powder metallurgy process, generally consisting of four basic steps: (1) powder manufacture, (2) powder blending,(3) compacting, (4) either sintering or metal injection molding. </rdfs:comment>
    </owl:NamedIndividual>
    


    <!-- http://www.nist.gov/itl/ssd/Materials#CompositeSubstance -->

    <owl:NamedIndividual rdf:about="&mat;CompositeSubstance">
        <rdf:type rdf:resource="&mat;MaterialForm"/>
    </owl:NamedIndividual>
    


    <!-- http://www.nist.gov/itl/ssd/Materials#CompressiveStrength -->

    <owl:NamedIndividual rdf:about="&mat;CompressiveStrength">
        <rdf:type rdf:resource="&mat;DeformationProperty"/>
        <rdfs:comment xml:lang="en">Compressive strength is the capacity of a material or structure to withstand axially directed pushing forces before being crushed.</rdfs:comment>
        <or:termString xml:lang="en">compressive strength</or:termString>
        <or:unitTypeFor rdf:resource="&or;UnitOfPressure"/>
    </owl:NamedIndividual>
    


    <!-- http://www.nist.gov/itl/ssd/Materials#ConductivityDiffusionCoefficient -->

    <owl:NamedIndividual rdf:about="&mat;ConductivityDiffusionCoefficient">
        <rdf:type rdf:resource="&mat;DiffusionProperty"/>
        <rdf:type rdf:resource="&mat;ElectricalProperty"/>
        <rdfs:seeAlso xml:lang="en">Definitions of terms for diffusion in the solid state (IUPAC Recommendations 1999), Pure Appl. Chem. 71, 1307-1325.</rdfs:seeAlso>
        <rdfs:comment xml:lang="en">The Conductivity Diffusion Coefficient of a mobile charged particle species (ion or electron) is derived from the measured partial electrical conductivity of that species by the Nernst-Einstein equation.</rdfs:comment>
        <or:unitTypeFor rdf:resource="&mat;AreaPerTime"/>
    </owl:NamedIndividual>
    


    <!-- http://www.nist.gov/itl/ssd/Materials#CopperAlloy -->

    <owl:NamedIndividual rdf:about="&mat;CopperAlloy">
        <rdf:type rdf:resource="&mat;NonFerrousAlloyTypeByMainConstituent"/>
        <or:referenceURL rdf:datatype="&xsd;anyURI">http://www.matweb.com/index.aspx</or:referenceURL>
        <rdfs:comment xml:lang="en">An alloy that contains Copper but little or no Iron.</rdfs:comment>
        <bc:primaryConstituentType rdf:resource="&bc;Copper"/>
    </owl:NamedIndividual>
    


    <!-- http://www.nist.gov/itl/ssd/Materials#Coulomb -->

    <owl:NamedIndividual rdf:about="&mat;Coulomb">
        <rdf:type rdf:resource="&mat;UnitOfCharge"/>
        <rdf:type rdf:resource="&or;SI_Unit"/>
    </owl:NamedIndividual>
    


    <!-- http://www.nist.gov/itl/ssd/Materials#Creep -->

    <owl:NamedIndividual rdf:about="&mat;Creep">
        <rdf:type rdf:resource="&mat;DeformationProperty"/>
        <rdfs:comment xml:lang="en">Creep is the tendency of a solid material to move slowly or deform (via Material Creep) permanently under the influence of stresses. </rdfs:comment>
        <or:termString xml:lang="en">creep</or:termString>
    </owl:NamedIndividual>
    


    <!-- http://www.nist.gov/itl/ssd/Materials#CriticalDensity -->

    <owl:NamedIndividual rdf:about="&mat;CriticalDensity">
        <rdf:type rdf:resource="&mat;MeasurableMechanicalProperty"/>
        <or:referenceURL rdf:datatype="&xsd;anyURI">http://www.iupac.org/namespaces/ThermoML/ThermoML.xsd</or:referenceURL>
        <rdfs:comment xml:lang="en">The Critical Density of a substance is the density of that substance at the critical point.</rdfs:comment>
        <or:termString xml:lang="en">critical density</or:termString>
        <or:unitTypeFor rdf:resource="&or;UnitOfDensity"/>
    </owl:NamedIndividual>
    


    <!-- http://www.nist.gov/itl/ssd/Materials#CriticalMolarVolume -->

    <owl:NamedIndividual rdf:about="&mat;CriticalMolarVolume">
        <rdf:type rdf:resource="&mat;MeasurableMechanicalProperty"/>
        <or:referenceURL rdf:datatype="&xsd;anyURI">http://www.iupac.org/namespaces/ThermoML/ThermoML.xsd</or:referenceURL>
        <rdfs:comment xml:lang="en">The `critical Molar Volume&#39; of a substance is the volume of one mole of that substance at the critical point.</rdfs:comment>
        <or:termString xml:lang="en">critical molar volume</or:termString>
        <or:unitTypeFor rdf:resource="&or;UnitOfVolume"/>
    </owl:NamedIndividual>
    


    <!-- http://www.nist.gov/itl/ssd/Materials#CriticalPressure -->

    <owl:NamedIndividual rdf:about="&mat;CriticalPressure">
        <rdf:type rdf:resource="&mat;MeasurableMechanicalProperty"/>
        <rdf:type rdf:resource="&mat;ThermalProperty"/>
        <or:referenceURL rdf:datatype="&xsd;anyURI">http://www.iupac.org/namespaces/ThermoML/ThermoML.xsd</or:referenceURL>
        <rdfs:comment xml:lang="en">A critical point for a substance is defined as the  temperature (Critical Temperature) and  pressure (Critical Pressure) at which phase boundaries cease to exist.</rdfs:comment>
        <or:termString xml:lang="en">critical temperature</or:termString>
        <or:unitTypeFor rdf:resource="&or;UnitOfPressure"/>
    </owl:NamedIndividual>
    


    <!-- http://www.nist.gov/itl/ssd/Materials#CriticalSpecificVolume -->

    <owl:NamedIndividual rdf:about="&mat;CriticalSpecificVolume">
        <rdf:type rdf:resource="&mat;MeasurableMechanicalProperty"/>
        <rdfs:comment xml:lang="en">The Critical Specific Volume is the ratio of a substance&#39;s volume to its mass (Specific Volume) at its Critical Temperature.</rdfs:comment>
        <or:termString xml:lang="en">critical specific volume</or:termString>
        <or:unitTypeFor rdf:resource="&mat;UnitOfVolumePerMass"/>
    </owl:NamedIndividual>
    


    <!-- http://www.nist.gov/itl/ssd/Materials#CriticalTemperature -->

    <owl:NamedIndividual rdf:about="&mat;CriticalTemperature">
        <rdf:type rdf:resource="&mat;MeasurableMechanicalProperty"/>
        <rdf:type rdf:resource="&mat;ThermalProperty"/>
        <or:referenceURL rdf:datatype="&xsd;anyURI">http://www.iupac.org/namespaces/ThermoML/ThermoML.xsd</or:referenceURL>
        <rdfs:comment xml:lang="en">A critical point for a substance is defined as the  temperature (Critical Temperature) and  pressure (Critical Pressure) at which phase boundaries cease to exist.</rdfs:comment>
        <or:termString xml:lang="en">critical temperature</or:termString>
        <or:unitTypeFor rdf:resource="&or;UnitOfTemperature"/>
    </owl:NamedIndividual>
    


    <!-- http://www.nist.gov/itl/ssd/Materials#CrowdionMechanism -->

    <owl:NamedIndividual rdf:about="&mat;CrowdionMechanism">
        <rdf:type rdf:resource="&mat;DiffusionMovementMechanism"/>
        <rdfs:comment>Definitions of terms for diffusion in the solid state (IUPAC Recommendations 1999), Pure Appl. Chem. 71, 1307-1325.</rdfs:comment>
        <rdfs:comment xml:lang="en">The Crowdion Mechanismi is a hypothesized mechanism in which diffusion takes place by a co-operative movement of a group of atoms one of which is typically centred on an interstitial position with the others relaxed from their normal lattice sites to accommodate the additional ‘crowdion’.</rdfs:comment>
        <skos:note xml:lang="en">There was a big scientific controversy over the question if crowdions actually exist as a metastable interstitial configuration in the seventies. This controversy has never been finally resolved; however, most researchers in the field believe that it does not exist.</skos:note>
        <rdfs:seeAlso xml:lang="en">http://www.tf.uni-kiel.de/matwis/amat/def_en/kap_1/advanced/t1_3_1.html</rdfs:seeAlso>
    </owl:NamedIndividual>
    


    <!-- http://www.nist.gov/itl/ssd/Materials#CrystallineSubstance -->

    <owl:NamedIndividual rdf:about="&mat;CrystallineSubstance">
        <rdf:type rdf:resource="&mat;MaterialPhaseComposition"/>
        <rdfs:comment xml:lang="en">Material in a crystalline phase</rdfs:comment>
    </owl:NamedIndividual>
    


    <!-- http://www.nist.gov/itl/ssd/Materials#CubicInch -->

    <owl:NamedIndividual rdf:about="&mat;CubicInch">
        <rdf:type rdf:resource="&or;NonMetricUnit"/>
        <rdf:type rdf:resource="&or;UnitOfVolume"/>
        <or:termString xml:lang="en">cubic inch</or:termString>
        <or:termString xml:lang="en">in^3</or:termString>
    </owl:NamedIndividual>
    


    <!-- http://www.nist.gov/itl/ssd/Materials#CurieTemperature -->

    <owl:NamedIndividual rdf:about="&mat;CurieTemperature">
        <rdf:type rdf:resource="&mat;MagneticProperty"/>
        <rdf:type rdf:resource="&mat;ThermalProperty"/>
        <or:termString xml:lang="en">Curie point</or:termString>
        <or:termString xml:lang="en">Curie temperature</or:termString>
        <rdfs:comment xml:lang="en">The Curie temperature (Tc), or Curie point, is the temperature at which a ferromagnetic or a ferrimagnetic material becomes paramagnetic on heating.</rdfs:comment>
        <or:unitTypeFor rdf:resource="&or;UnitOfTemperature"/>
    </owl:NamedIndividual>
    


    <!-- http://www.nist.gov/itl/ssd/Materials#DarkenEquation -->

    <owl:NamedIndividual rdf:about="&mat;DarkenEquation">
        <rdf:type rdf:resource="&or;Equation"/>
        <rdfs:seeAlso xml:lang="en">Definitions of terms for diffusion in the solid state (IUPAC Recommendations 1999), Pure Appl. Chem. 71, 1307-1325.</rdfs:seeAlso>
        <rdfs:comment xml:lang="en">The Darken equation represents Fick&#39;s laws adapted to binary systems.</rdfs:comment>
    </owl:NamedIndividual>
    


    <!-- http://www.nist.gov/itl/ssd/Materials#DefectDiffusionCoefficient -->

    <owl:NamedIndividual rdf:about="&mat;DefectDiffusionCoefficient">
        <rdf:type rdf:resource="&mat;DiffusionProperty"/>
        <rdfs:seeAlso xml:lang="en">Definitions of terms for diffusion in the solid state (IUPAC Recommendations 1999), Pure Appl. Chem. 71, 1307-1325.</rdfs:seeAlso>
        <rdfs:comment xml:lang="en">In the case of diffusion via a vacancy mechanism, the diffusion coefficient associated with the movement of vacancies in the opposite direction to the movement of diffusing species is called the Vacancy Diffusion Coefficient.  The Defect Diffusion Coefficient covers not only the diffusion of vacancies, but also of other defects such as interstitials.</rdfs:comment>
        <or:termString xml:lang="en">defect diffusion coefficient</or:termString>
        <or:unitTypeFor rdf:resource="&mat;AreaPerTime"/>
    </owl:NamedIndividual>
    


    <!-- http://www.nist.gov/itl/ssd/Materials#DielectricConstant -->

    <owl:NamedIndividual rdf:about="&mat;DielectricConstant">
        <rdf:type rdf:resource="&mat;DielectricProperty"/>
    </owl:NamedIndividual>
    


    <!-- http://www.nist.gov/itl/ssd/Materials#DielectricStrength -->

    <owl:NamedIndividual rdf:about="&mat;DielectricStrength">
        <rdf:type rdf:resource="&mat;DielectricProperty"/>
        <rdfs:comment xml:lang="en">Dielectric Strength is the maximum electric field strength that a material can withstand without breaking down.  This has slightly different meanings for insulators, dielectrics, and combinations of dielectrics and conductors.</rdfs:comment>
    </owl:NamedIndividual>
    


    <!-- http://www.nist.gov/itl/ssd/Materials#DiffusionCorrelationFactor -->

    <owl:NamedIndividual rdf:about="&mat;DiffusionCorrelationFactor">
        <rdf:type rdf:resource="&mat;DiffusionProperty"/>
        <rdfs:seeAlso xml:lang="en">Definitions of terms for diffusion in the solid state (IUPAC Recommendations 1999), Pure Appl. Chem. 71, 1307-1325.</rdfs:seeAlso>
        <rdfs:comment xml:lang="en">When the motion of a diffusing species is dependent on the presence of a defect on a neighbouring site, e.g. a tracer diffusing by a vacancy mechanism, the jumps of the diffusing species will not be random, but are correlated. The Diffusion Correlation Factor, f, is a measure of the deviation of the motion of the diffusing atoms from the random walk.</rdfs:comment>
        <or:unitTypeFor rdf:resource="&or;DimensionlessUnit"/>
    </owl:NamedIndividual>
    


    <!-- http://www.nist.gov/itl/ssd/Materials#DiffusionFlux -->

    <owl:NamedIndividual rdf:about="&mat;DiffusionFlux">
        <rdf:type rdf:resource="&mat;DiffusionProperty"/>
        <rdfs:seeAlso xml:lang="en">Definitions of terms for diffusion in the solid state (IUPAC Recommendations 1999), Pure Appl. Chem. 71, 1307-1325.</rdfs:seeAlso>
        <rdfs:comment xml:lang="en">The diffusion flux Ji gives the number of species i crossing a unit area, fixed relative to the local centre of mass, per unit of time.</rdfs:comment>
        <or:unitTypeFor rdf:resource="&mat;UnitOfInverseAreaPerTime"/>
    </owl:NamedIndividual>
    


    <!-- http://www.nist.gov/itl/ssd/Materials#DiffusionInducedGrainBoundaryMigration -->

    <owl:NamedIndividual rdf:about="&mat;DiffusionInducedGrainBoundaryMigration">
        <rdf:type rdf:resource="&mat;DiffusionMovementMechanism"/>
        <rdfs:seeAlso>Definitions of terms for diffusion in the solid state (IUPAC Recommendations 1999), Pure Appl. Chem. 71, 1307-1325.</rdfs:seeAlso>
        <rdfs:comment xml:lang="en">If a polycrystalline material undergoes an interdiffusion process, the grain boundaries move in a direction perpendicular to the diffusion flux.  As a result the concentrations in the regions swept by the boundaries change.  This is called ``Diffusion-Induced Grain boundary Migration&#39;&#39; (DIGM).</rdfs:comment>
        <or:termString xml:lang="en">diffusion induced grain boundary migration</or:termString>
    </owl:NamedIndividual>
    


    <!-- http://www.nist.gov/itl/ssd/Materials#DiffusionJumpFrequency -->

    <owl:NamedIndividual rdf:about="&mat;DiffusionJumpFrequency">
        <rdf:type rdf:resource="&mat;DiffusionProperty"/>
        <rdfs:seeAlso>Definitions of terms for diffusion in the solid state (IUPAC Recommendations 1999), Pure Appl. Chem. 71, 1307-1325.</rdfs:seeAlso>
        <rdfs:comment xml:lang="en">In Diffusion, the jump frequency of a particle i towards a given nearest-neighbour site is denoted by Gamma(i). The total Diffusion Jump Frequency, Gamma, denotes the average number of jumps of particles per unit time.</rdfs:comment>
        <or:termString xml:lang="en">diffusion jump frequency</or:termString>
        <or:termString xml:lang="en">jump frequency</or:termString>
        <or:unitTypeFor rdf:resource="&mat;UnitOfInverseTime"/>
    </owl:NamedIndividual>
    


    <!-- http://www.nist.gov/itl/ssd/Materials#DiffusionPath -->

    <owl:NamedIndividual rdf:about="&mat;DiffusionPath">
        <rdf:type rdf:resource="&doc;GenericScientificModel"/>
        <rdfs:seeAlso xml:lang="en">Definitions of terms for diffusion in the solid state (IUPAC Recommendations 1999), Pure Appl. Chem. 71, 1307-1325.</rdfs:seeAlso>
        <rdfs:comment xml:lang="en">The sequence of structural and compositional modifications developed during isothermal diffusion in multiphase, multicomponent diffusion systems is called a Diffusion Path. This path is generally plotted superposed upon an isothermal phase diagram.</rdfs:comment>
    </owl:NamedIndividual>
    


    <!-- http://www.nist.gov/itl/ssd/Materials#DiffusionPotential -->

    <owl:NamedIndividual rdf:about="&mat;DiffusionPotential">
        <rdf:type rdf:resource="&mat;DiffusionProperty"/>
        <rdfs:seeAlso xml:lang="en">Definitions of terms for diffusion in the solid state (IUPAC Recommendations 1999), Pure Appl. Chem. 71, 1307-1325.</rdfs:seeAlso>
        <rdfs:comment xml:lang="en">During diffusion of charged particles in ionic or electronic conducting solids an electrical charge is built up due to the differences in mobilities of the diffusing particles. The corresponding electrostatic potential, phi, is known as the Diffusion Potential.</rdfs:comment>
        <or:unitTypeFor rdf:resource="&or;UnitOfVoltage"/>
    </owl:NamedIndividual>
    


    <!-- http://www.nist.gov/itl/ssd/Materials#Diffusivity -->

    <owl:NamedIndividual rdf:about="&mat;Diffusivity">
        <rdf:type rdf:resource="&mat;TransportProperty"/>
        <rdfs:comment xml:lang="en">Diffusivity is the ratio between the molar flux due to molecular diffusion and the gradient in the concentration of the species (or the driving force for diffusion).  Diffusivity is generally prescribed for a given pair of species in a given phase at a given temperature. For a multi-component system, it is prescribed for each pair of species in the system.  Diffusivity is measured in Area per unit time -- in SI, m^2/s.</rdfs:comment>
        <or:unitTypeFor rdf:resource="&mat;AreaPerTime"/>
    </owl:NamedIndividual>
    


    <!-- http://www.nist.gov/itl/ssd/Materials#DiffusivityTensor -->

    <owl:NamedIndividual rdf:about="&mat;DiffusivityTensor">
        <rdf:type rdf:resource="&mat;DiffusionProperty"/>
        <rdfs:seeAlso xml:lang="en">Definitions of terms for diffusion in the solid state (IUPAC Recommendations 1999), Pure Appl. Chem. 71, 1307-1325.</rdfs:seeAlso>
        <rdfs:comment xml:lang="en">In an anisotropic crystal lattice the diffusion coefficient is generally direction dependent and has to be represented by a three-dimensional tensor with components Dij. Under these circumstances the diffusion coefficient is also called the ``Diffusivity Tensor or ``diffusion tensor&#39;&#39;.</rdfs:comment>
    </owl:NamedIndividual>
    


    <!-- http://www.nist.gov/itl/ssd/Materials#DirectInterstitialMechanism -->

    <owl:NamedIndividual rdf:about="&mat;DirectInterstitialMechanism">
        <rdf:type rdf:resource="&mat;DiffusionMovementMechanism"/>
        <rdfs:seeAlso xml:lang="en">Definitions of terms for diffusion in the solid state (IUPAC Recommendations 1999), Pure Appl. Chem. 71, 1307-1325.</rdfs:seeAlso>
        <rdfs:comment xml:lang="en">In the Direct Interstitial Mechanism diffusion takes place by the direct migration of an interstitial species from one interstitial position to another.</rdfs:comment>
    </owl:NamedIndividual>
    


    <!-- http://www.nist.gov/itl/ssd/Materials#DistortedHexagonalCrystalStructure -->

    <owl:NamedIndividual rdf:about="&mat;DistortedHexagonalCrystalStructure">
        <rdf:type rdf:resource="&mat;CrystalStructure"/>
    </owl:NamedIndividual>
    


    <!-- http://www.nist.gov/itl/ssd/Materials#DivacancyMechanism -->

    <owl:NamedIndividual rdf:about="&mat;DivacancyMechanism">
        <rdf:type rdf:resource="&mat;DiffusionMovementMechanism"/>
        <rdfs:seeAlso xml:lang="en">Definitions of terms for diffusion in the solid state (IUPAC Recommendations 1999), Pure Appl. Chem. 71, 1307-1325.</rdfs:seeAlso>
        <rdfs:comment xml:lang="en">The Divacancy Mechanism is the diffusion process by which a crystal lattice vacancy pair is used by any constituent species of the material to effect diffusion.</rdfs:comment>
    </owl:NamedIndividual>
    


    <!-- http://www.nist.gov/itl/ssd/Materials#DollarUS -->

    <owl:NamedIndividual rdf:about="&mat;DollarUS">
        <rdf:type rdf:resource="&or;PrimaryCurrencyUnit"/>
    </owl:NamedIndividual>
    


    <!-- http://www.nist.gov/itl/ssd/Materials#DoubleHexagonalClosePackedCrystalStructure -->

    <owl:NamedIndividual rdf:about="&mat;DoubleHexagonalClosePackedCrystalStructure">
        <rdf:type rdf:resource="&mat;CrystalStructure"/>
    </owl:NamedIndividual>
    


    <!-- http://www.nist.gov/itl/ssd/Materials#DriftVelocity -->

    <owl:NamedIndividual rdf:about="&mat;DriftVelocity">
        <rdf:type rdf:resource="&mat;DiffusionProperty"/>
        <rdfs:seeAlso>Definitions of terms for diffusion in the solid state (IUPAC Recommendations 1999), Pure Appl. Chem. 71, 1307-1325.</rdfs:seeAlso>
        <rdfs:comment xml:lang="en">The application of a driving force gives atoms a greater than random probability of jumping in the direction of the gradient. Atoms are said to have an average Drift Velocity vF in that direction and contribute a term cvF to the diffusion flux.</rdfs:comment>
        <or:unitTypeFor rdf:resource="&or;UnitOfVelocity"/>
    </owl:NamedIndividual>
    


    <!-- http://www.nist.gov/itl/ssd/Materials#DumbellIntersticialcyMechanism -->

    <owl:NamedIndividual rdf:about="&mat;DumbellIntersticialcyMechanism">
        <rdf:type rdf:resource="&mat;DiffusionMovementMechanism"/>
        <rdfs:seeAlso xml:lang="en">Definitions of terms for diffusion in the solid state (IUPAC Recommendations 1999), Pure Appl. Chem. 71, 1307-1325.</rdfs:seeAlso>
        <rdfs:comment xml:lang="en">In some diffusion systems the equilibrium configuration during an interstitialcy jump consists of a dumbbell-like defect with each of the moving ions being displaced by an equal amount from the normal lattice position.  Diffusion taking place via such species is said to proceed by a Dumbbell Interstitialcy Mechanism.</rdfs:comment>
    </owl:NamedIndividual>
    


    <!-- http://www.nist.gov/itl/ssd/Materials#Duterium -->

    <owl:NamedIndividual rdf:about="&mat;Duterium">
        <rdf:type rdf:resource="&mat;Radioisotope"/>
    </owl:NamedIndividual>
    


    <!-- http://www.nist.gov/itl/ssd/Materials#Dyne -->

    <owl:NamedIndividual rdf:about="&mat;Dyne">
        <rdf:type rdf:resource="&or;CGS_Unit"/>
        <rdf:type rdf:resource="&or;UnitOfForce"/>
    </owl:NamedIndividual>
    


    <!-- http://www.nist.gov/itl/ssd/Materials#EffectiveBohrMagnetonNumber -->

    <owl:NamedIndividual rdf:about="&mat;EffectiveBohrMagnetonNumber">
        <rdf:type rdf:resource="&mat;MagneticProperty"/>
        <or:termString xml:lang="en">Bohr magneton number</or:termString>
        <rdfs:comment xml:lang="en">The effective Bohr magneton number is a dimensionless quantity specifying a paramagnetic property of a material.</rdfs:comment>
        <or:termString xml:lang="en">effective Bohr magneton number</or:termString>
        <or:unitTypeFor rdf:resource="&or;DimensionlessUnit"/>
    </owl:NamedIndividual>
    


    <!-- http://www.nist.gov/itl/ssd/Materials#EffectiveDiffusionCoefficient -->

    <owl:NamedIndividual rdf:about="&mat;EffectiveDiffusionCoefficient">
        <rdf:type rdf:resource="&mat;DiffusionProperty"/>
        <rdfs:seeAlso xml:lang="en">Definitions of terms for diffusion in the solid state (IUPAC Recommendations 1999), Pure Appl. Chem. 71, 1307-1325.</rdfs:seeAlso>
        <rdfs:comment xml:lang="en">In alloys or compounds transport of material can occur under the influence of a driving force, at constant composition in the whole sample. Examples are found in viscous creep and sintering processes. In this case the fluxes of the diffusing species must be coupled. In an ionic crystal a similar condition holds due to the necessity of preserving electroneutrality.  The Effective Diffusion Coefficient is a weighted average of the diffusion coefficients of the various diffusing species to provide an overall measure of the diffusion rate.</rdfs:comment>
        <or:unitTypeFor rdf:resource="&mat;UnitOfAreaPerTime"/>
    </owl:NamedIndividual>
    


    <!-- http://www.nist.gov/itl/ssd/Materials#EinsteinSmoluchowskiEquation -->

    <owl:NamedIndividual rdf:about="&mat;EinsteinSmoluchowskiEquation">
        <rdf:type rdf:resource="&or;Equation"/>
        <rdfs:seeAlso xml:lang="en">Definitions of terms for diffusion in the solid state (IUPAC Recommendations 1999), Pure Appl. Chem. 71, 1307-1325.</rdfs:seeAlso>
        <rdfs:comment xml:lang="en">The Einstein-Smoluchowski Equation relates diffusivity to the mobility of particles in a substance and the temperature.  Specializations of this equation specify the mobility in terms of electrical or other parameters.</rdfs:comment>
    </owl:NamedIndividual>
    


    <!-- http://www.nist.gov/itl/ssd/Materials#ElasticModulus -->

    <owl:NamedIndividual rdf:about="&mat;ElasticModulus">
        <rdfs:comment xml:lang="en">An elastic modulus is defined as the slope of its stress–strain curve of a substance within the range where the deformation is elastic.  Three varieties of this are Young&#39;s modulus, the sheer modulus, and the bulk modulus.</rdfs:comment>
        <or:unitTypeFor rdf:resource="&or;UnitOfPressure"/>
    </owl:NamedIndividual>
    


    <!-- http://www.nist.gov/itl/ssd/Materials#ElectrialResistivity -->

    <owl:NamedIndividual rdf:about="&mat;ElectrialResistivity">
        <rdf:type rdf:resource="&or;MeasurableQuantityType"/>
    </owl:NamedIndividual>
    


    <!-- http://www.nist.gov/itl/ssd/Materials#ElectricPolarizability -->

    <owl:NamedIndividual rdf:about="&mat;ElectricPolarizability">
        <rdf:type rdf:resource="&mat;DielectricProperty"/>
        <rdf:type rdf:resource="&or;MeasurableQuantityType"/>
        <rdfs:comment xml:lang="en">Electric Polarizability is the tendency of a substance&#39;s charge distribution to be distorted from its normal shape by an external electric field.  It is specified by the material&#39;s relative permittivity (dielectric constant).</rdfs:comment>
    </owl:NamedIndividual>
    


    <!-- http://www.nist.gov/itl/ssd/Materials#ElectricalConductivity -->

    <owl:NamedIndividual rdf:about="&mat;ElectricalConductivity">
        <rdf:type rdf:resource="&mat;ElectricalProperty"/>
        <rdf:type rdf:resource="&or;MeasurableQuantityType"/>
        <rdfs:comment xml:lang="en">Electrical Conductivity is a measure of how easily electric current flows through a material. High conductivity indicates a material readily allows the movement of electric charge.  The  SI unit of electrical conductivity is siemens per metre (S/m).

The inverse of Electrical Conductivity is Electrical Resistivity.</rdfs:comment>
        <or:termString xml:lang="en">electrical conductivity</or:termString>
        <or:termString xml:lang="en">specific conductance</or:termString>
        <or:unitTypeFor rdf:resource="&mat;UnitOfElectricalConductivity"/>
    </owl:NamedIndividual>
    


    <!-- http://www.nist.gov/itl/ssd/Materials#ElectricalDiffusionMobility -->

    <owl:NamedIndividual rdf:about="&mat;ElectricalDiffusionMobility">
        <rdf:type rdf:resource="&mat;DiffusionProperty"/>
        <rdfs:seeAlso>Definitions of terms for diffusion in the solid state (IUPAC Recommendations 1999), Pure Appl. Chem. 71, 1307-1325.</rdfs:seeAlso>
        <rdfs:comment xml:lang="en">Mass transport of charged species due to electrical force is described as Electrical Mobility (or &#39;electrochemical mobility&#39;) and is calculated as the average drift velocity per unit of electrical field strength.  Note that this is different from the Species Diffusion Mobility that is a ration of the drift velocity to the force, not a field strength.  The electrical mobility is thus the species mobility devided by the absolute electrical charge on the species.</rdfs:comment>
        <or:termString xml:lang="en">electrical diffusion mobility</or:termString>
        <or:termString xml:lang="en">electrical mobility</or:termString>
        <or:termString xml:lang="en">electrochemical mobility</or:termString>
    </owl:NamedIndividual>
    


    <!-- http://www.nist.gov/itl/ssd/Materials#ElectricalPotential -->

    <owl:NamedIndividual rdf:about="&mat;ElectricalPotential">
        <rdf:type rdf:resource="&mat;ElectricalProperty"/>
        <rdfs:comment xml:lang="en">Electrical Potential (``voltage&quot; or &quot;electric tension&quot;), is the difference in electric potential between two points — or the difference in electric potential energy of a unit test charge transported between two points. It is is equal to the work which would have to be done, per unit charge, against a static electric field to move the charge between two points.  It is measured in units of electric potential: volts (equal to joules per coulomb).</rdfs:comment>
        <or:termString xml:lang="en">electrical potential</or:termString>
        <or:termString xml:lang="en">voltage</or:termString>
        <or:unitTypeFor rdf:resource="&or;Volt"/>
    </owl:NamedIndividual>
    


    <!-- http://www.nist.gov/itl/ssd/Materials#ElectricalResistivity -->

    <owl:NamedIndividual rdf:about="&mat;ElectricalResistivity">
        <rdf:type rdf:resource="&mat;ElectricalProperty"/>
        <rdfs:comment xml:lang="en">Electrical Resistivity is a measure of how strongly a material opposes the flow of electric current. Low resistivity indicates a material readily allows the movement of electric charge. The SI unit of electrical resistivity is the ohm⋅metre (Ω⋅m).

Electrical Resistivity is the inverse of Electrical Conductivity.</rdfs:comment>
        <or:termString xml:lang="en">electrical resistivity</or:termString>
        <or:termString xml:lang="en">resistivity</or:termString>
        <or:termString xml:lang="en">specific electrical resistance</or:termString>
        <or:termString xml:lang="en">volume resistivity</or:termString>
        <or:unitTypeFor rdf:resource="&mat;UnitOfElectricalResistivity"/>
    </owl:NamedIndividual>
    


    <!-- http://www.nist.gov/itl/ssd/Materials#Elongation -->

    <owl:NamedIndividual rdf:about="&mat;Elongation">
        <rdf:type rdf:resource="&mat;DeformationProperty"/>
        <rdfs:comment xml:lang="en">Elongation is the ratio of the reference length of an object to its changed length, whether caused by external loads, gravitation, or thermal expansion/contraction.</rdfs:comment>
        <or:termString xml:lang="en">elongation</or:termString>
        <or:unitTypeFor rdf:resource="&or;DimensionlessUnit"/>
    </owl:NamedIndividual>
    


    <!-- http://www.nist.gov/itl/ssd/Materials#EnergyPerMass -->

    <owl:NamedIndividual rdf:about="&mat;EnergyPerMass">
        <rdf:type rdf:resource="&or;MeasurableQuantityType"/>
        <rdfs:comment xml:lang="en">Energy Per Mass is an amount of Energy divided by an amount of Mass.  It is used to specify the amount of energy that enters or leaves a system dependent upon the mass of the system that results in, or is caused by, some type of change.</rdfs:comment>
    </owl:NamedIndividual>
    


    <!-- http://www.nist.gov/itl/ssd/Materials#EnthalpyOfFormation -->

    <owl:NamedIndividual rdf:about="&mat;EnthalpyOfFormation">
        <rdf:type rdf:resource="&mat;ThermochemicalProperty"/>
        <rdfs:comment xml:lang="en">The standard enthalpy of formation or standard heat of formation of a compound is the change of enthalpy that accompanies the formation of 1 mole of the compound from its elements, with all substances in their standard states.</rdfs:comment>
        <or:termString xml:lang="en">enthalpy of formation</or:termString>
        <or:termString xml:lang="en">heat of formation</or:termString>
        <or:termString xml:lang="en">standard enthalpy of formation</or:termString>
        <or:termString xml:lang="en">standard heat of formation</or:termString>
        <or:unitTypeFor rdf:resource="&or;UnitOfEnergy"/>
    </owl:NamedIndividual>
    


    <!-- http://www.nist.gov/itl/ssd/Materials#EnthalpyOfMixing -->

    <owl:NamedIndividual rdf:about="&mat;EnthalpyOfMixing">
        <rdf:type rdf:resource="&mat;ThermalProperty"/>
        <rdfs:comment xml:lang="en">The enthalpy of mixing (or ``heat of mixing&#39;&#39;) is the heat that is taken up or released upon mixing of two (non-reactive) chemical substances.</rdfs:comment>
        <or:termString xml:lang="en">enthalpy of mixing</or:termString>
        <or:termString xml:lang="en">heat of mixing</or:termString>
        <or:unitTypeFor rdf:resource="&or;UnitOfEnergy"/>
    </owl:NamedIndividual>
    


    <!-- http://www.nist.gov/itl/ssd/Materials#EnthalpyOfTransformation -->

    <owl:NamedIndividual rdf:about="&mat;EnthalpyOfTransformation">
        <rdf:type rdf:resource="&mat;ThermalProperty"/>
        <or:termString xml:lang="en">Enthalpy of transformation is the heat released or absorbed by a body or a thermodynamic system during a phase transition such as the melting (Latent Heat of Fusion) or boiling (Latent Heat of Vaporization).  </or:termString>
        <or:termString xml:lang="en">enthalpy of transformation</or:termString>
        <or:termString xml:lang="en">latent heat</or:termString>
        <or:unitTypeFor rdf:resource="&or;UnitOfEnergy"/>
    </owl:NamedIndividual>
    


    <!-- http://www.nist.gov/itl/ssd/Materials#Euro -->

    <owl:NamedIndividual rdf:about="&mat;Euro">
        <rdf:type rdf:resource="&or;PrimaryCurrencyUnit"/>
    </owl:NamedIndividual>
    


    <!-- http://www.nist.gov/itl/ssd/Materials#EuroCent -->

    <owl:NamedIndividual rdf:about="&mat;EuroCent">
        <rdf:type rdf:resource="&or;SecondaryCurrencyUnit"/>
    </owl:NamedIndividual>
    


    <!-- http://www.nist.gov/itl/ssd/Materials#EutecticTemperature -->

    <owl:NamedIndividual rdf:about="&mat;EutecticTemperature">
        <rdf:type rdf:resource="&mat;PressureDependentProperty"/>
        <rdf:type rdf:resource="&mat;ThermalProperty"/>
        <or:referenceURL rdf:datatype="&xsd;anyURI">http://www.iupac.org/namespaces/ThermoML</or:referenceURL>
        <rdfs:comment xml:lang="en">The Eutectic Temperature for a mixture is the temperature of the eutectic point of that mixture at a given pressure.</rdfs:comment>
        <or:termString xml:lang="en">eutectic temperature</or:termString>
        <or:unitTypeFor rdf:resource="&or;UnitOfTemperature"/>
    </owl:NamedIndividual>
    


    <!-- http://www.nist.gov/itl/ssd/Materials#ExchangeMechansimForDiffusion -->

    <owl:NamedIndividual rdf:about="&mat;ExchangeMechansimForDiffusion">
        <rdf:type rdf:resource="&mat;DiffusionMovementMechanism"/>
    </owl:NamedIndividual>
    


    <!-- http://www.nist.gov/itl/ssd/Materials#Extruding -->

    <owl:NamedIndividual rdf:about="&mat;Extruding"/>
    


    <!-- http://www.nist.gov/itl/ssd/Materials#FaceCenteredCubicCrystalStructure -->

    <owl:NamedIndividual rdf:about="&mat;FaceCenteredCubicCrystalStructure">
        <rdf:type rdf:resource="&mat;CrystalStructure"/>
        <or:nickName>fcc</or:nickName>
    </owl:NamedIndividual>
    


    <!-- http://www.nist.gov/itl/ssd/Materials#FahrenheitDegree -->

    <owl:NamedIndividual rdf:about="&mat;FahrenheitDegree">
        <rdf:type rdf:resource="&mat;UnitOfTemperatureDifference"/>
        <rdfs:comment xml:lang="en">A Fahrenheit Degree is the Unit Of Temperature Difference equal to the differerence between zero and one Degrees Fahrenheit.  A Fahrenheit Degree is 5/9 of a CelsiusDegree.</rdfs:comment>
        <or:termString xml:lang="en">Fahrenheight degree</or:termString>
    </owl:NamedIndividual>
    


    <!-- http://www.nist.gov/itl/ssd/Materials#Farad -->

    <owl:NamedIndividual rdf:about="&mat;Farad">
        <rdf:type rdf:resource="&mat;UnitOfCapacitance"/>
        <rdf:type rdf:resource="&or;SI_Unit"/>
    </owl:NamedIndividual>
    


    <!-- http://www.nist.gov/itl/ssd/Materials#FatigueEnduranceLimit -->

    <owl:NamedIndividual rdf:about="&mat;FatigueEnduranceLimit">
        <rdf:type rdf:resource="&mat;DeformationProperty"/>
        <rdfs:comment xml:lang="en">Fatigue endurance limit (fatigue limit, endurance limit,  fatigue strength) is the amplitude (or range) of cyclic stress that can be applied to the material without causing fatigue failure.</rdfs:comment>
        <or:termString xml:lang="en">endurance limit</or:termString>
        <or:termString xml:lang="en">fatigue endurance limit</or:termString>
        <or:termString xml:lang="en">fatigue limit</or:termString>
        <or:termString xml:lang="en">fatigue strength</or:termString>
        <or:unitTypeFor rdf:resource="&or;UnitOfPressure"/>
    </owl:NamedIndividual>
    


    <!-- http://www.nist.gov/itl/ssd/Materials#FerrousAlloy -->

    <owl:NamedIndividual rdf:about="&mat;FerrousAlloy">
        <rdf:type rdf:resource="&mat;AlloyTypeByMainConstituent"/>
        <or:referenceURL rdf:datatype="&xsd;anyURI">http://www.matweb.com/index.aspx</or:referenceURL>
        <rdfs:comment xml:lang="en">A Ferrous Alloy is one that contains iron.</rdfs:comment>
        <or:termString xml:lang="en">ferrous alloy</or:termString>
        <or:termString xml:lang="en">ferrous metal</or:termString>
        <bc:primaryConstituentType rdf:resource="&bc;Iron"/>
    </owl:NamedIndividual>
    


    <!-- http://www.nist.gov/itl/ssd/Materials#FicksFirstLawOfDiffusion -->

    <owl:NamedIndividual rdf:about="&mat;FicksFirstLawOfDiffusion">
        <rdf:type rdf:resource="&doc;GenericScientificModel"/>
        <rdfs:seeAlso xml:lang="en">Definitions of terms for diffusion in the solid state (IUPAC Recommendations 1999), Pure Appl. Chem. 71, 1307-1325.</rdfs:seeAlso>
        <rdfs:comment xml:lang="en">Fick’s First Law Of Diffusion states the relationship between the flux and the concentration gradient of a diffusing species.</rdfs:comment>
    </owl:NamedIndividual>
    


    <!-- http://www.nist.gov/itl/ssd/Materials#FicksSecondLawOfDiffusion -->

    <owl:NamedIndividual rdf:about="&mat;FicksSecondLawOfDiffusion">
        <rdf:type rdf:resource="&doc;GenericScientificModel"/>
        <rdfs:seeAlso xml:lang="en">Definitions of terms for diffusion in the solid state (IUPAC Recommendations 1999), Pure Appl. Chem. 71, 1307-1325.</rdfs:seeAlso>
        <rdfs:comment xml:lang="en">Fick’s Second Law Of Diffusion states the relationship between the concentration gradient of a species and the rate of change of its concentration (dc/dt) caused by its diffusion.</rdfs:comment>
    </owl:NamedIndividual>
    


    <!-- http://www.nist.gov/itl/ssd/Materials#FirstLawOfThermodynamics -->

    <owl:NamedIndividual rdf:about="&mat;FirstLawOfThermodynamics">
        <rdf:type rdf:resource="&mat;LawOfThermodynamics"/>
        <rdfs:comment xml:lang="en">The First Law of Thermodynamics states that the increase in internal energy of a body equals the heat supplied to the body (which may be negative) minus the work done by the body (which also may be negative).  Heat and work are thus forms of energy transfer.  Energy is conserved in an isolated closed system, but the internal energy of a system changes as heat and work are transferred into or out of it.</rdfs:comment>
        <or:termString xml:lang="en">first law of thermodynamics</or:termString>
    </owl:NamedIndividual>
    


    <!-- http://www.nist.gov/itl/ssd/Materials#FiveFrequencyDiffusionModel -->

    <owl:NamedIndividual rdf:about="&mat;FiveFrequencyDiffusionModel">
        <rdf:type rdf:resource="&mat;DiffusionMovementMechanism"/>
        <rdfs:seeAlso xml:lang="en">Definitions of terms for diffusion in the solid state (IUPAC Recommendations 1999), Pure Appl. Chem. 71, 1307-1325.</rdfs:seeAlso>
        <rdfs:comment xml:lang="en">The Five-Frequency Diffusion Model is a type of movement of impurity diffusion via monovacancies in face-centred-cubic (fcc) metals or on an fcc sublattice in ionic crystals. It is assumed that the only host atom jumps that differ from jumps in the pure lattice are those made by nearest neighbours of the impurity.</rdfs:comment>
    </owl:NamedIndividual>
    


    <!-- http://www.nist.gov/itl/ssd/Materials#Forging_MaterialProcessing -->

    <owl:NamedIndividual rdf:about="&mat;Forging_MaterialProcessing"/>
    


    <!-- http://www.nist.gov/itl/ssd/Materials#FractureToughness -->

    <owl:NamedIndividual rdf:about="&mat;FractureToughness">
        <rdf:type rdf:resource="&mat;DeformationProperty"/>
        <rdfs:comment xml:lang="en">Fracture Toughness is a measure of a substance&#39;s ability to resist Fracturing.</rdfs:comment>
        <or:termString xml:lang="en">fracture toughness</or:termString>
        <or:termString xml:lang="en">toughness</or:termString>
        <or:unitTypeFor rdf:resource="&mat;UnitOfToughness"/>
    </owl:NamedIndividual>
    


    <!-- http://www.nist.gov/itl/ssd/Materials#Franklin -->

    <owl:NamedIndividual rdf:about="&mat;Franklin">
        <rdf:type rdf:resource="&mat;UnitOfCharge"/>
        <rdf:type rdf:resource="&or;MetricUnit"/>
        <or:termString xml:lang="en">franklin</or:termString>
    </owl:NamedIndividual>
    


    <!-- http://www.nist.gov/itl/ssd/Materials#FreeElectronDensity -->

    <owl:NamedIndividual rdf:about="&mat;FreeElectronDensity">
        <rdf:type rdf:resource="&mat;ElectricalProperty"/>
        <rdf:type rdf:resource="&or;MeasurableQuantityType"/>
    </owl:NamedIndividual>
    


    <!-- http://www.nist.gov/itl/ssd/Materials#Fugacity -->

    <owl:NamedIndividual rdf:about="&mat;Fugacity">
        <rdf:type rdf:resource="&mat;MeasurableMechanicalProperty"/>
        <or:termString xml:lang="en">The Fugacity of a gas is an effective pressure which replaces the true mechanical pressure in accurate chemical equilibrium calculations. It is equal to the pressure of an ideal gas which has the same chemical potential as the real gas.</or:termString>
        <or:termString xml:lang="en">fugacity</or:termString>
        <or:unitTypeFor rdf:resource="&or;UnitOfPressure"/>
    </owl:NamedIndividual>
    


    <!-- http://www.nist.gov/itl/ssd/Materials#Gadolinium -->

    <owl:NamedIndividual rdf:about="&mat;Gadolinium"/>
    


    <!-- http://www.nist.gov/itl/ssd/Materials#Gallium -->

    <owl:NamedIndividual rdf:about="&mat;Gallium"/>
    


    <!-- http://www.nist.gov/itl/ssd/Materials#GaseousSubstance -->

    <owl:NamedIndividual rdf:about="&mat;GaseousSubstance">
        <rdf:type rdf:resource="&mat;MaterialForm"/>
        <rdf:type rdf:resource="&mat;StateOfMatter"/>
        <rdfs:comment xml:lang="en">Material in a gasseous phase.</rdfs:comment>
    </owl:NamedIndividual>
    


    <!-- http://www.nist.gov/itl/ssd/Materials#GelSubstance -->

    <owl:NamedIndividual rdf:about="&mat;GelSubstance">
        <rdf:type rdf:resource="&mat;MaterialPhaseComposition"/>
        <rdfs:comment xml:lang="en">Material in a gel phase.</rdfs:comment>
    </owl:NamedIndividual>
    


    <!-- http://www.nist.gov/itl/ssd/Materials#GibbsFreeEnergy -->

    <owl:NamedIndividual rdf:about="&mat;GibbsFreeEnergy">
        <rdf:type rdf:resource="&mat;ThermalProperty"/>
        <or:termString xml:lang="en">Gibbs energy</or:termString>
        <or:termString xml:lang="en">Gibbs free energy</or:termString>
        <or:termString xml:lang="en">Gibbs function</or:termString>
        <rdfs:comment xml:lang="en">The property `Gibbs Free Energy&#39;  specifies the Gibbs free energy of a Thermodynamic System, which specifies the “useful” work obtainable from a closed thermodynamic system at a constant temperature and pressure.</rdfs:comment>
        <or:termString xml:lang="en">free enthalpy</or:termString>
        <or:unitTypeFor rdf:resource="&or;UnitOfEnergy"/>
    </owl:NamedIndividual>
    


    <!-- http://www.nist.gov/itl/ssd/Materials#GlassTemperature -->

    <owl:NamedIndividual rdf:about="&mat;GlassTemperature">
        <rdf:type rdf:resource="&mat;ThermalProperty"/>
        <rdfs:comment xml:lang="en">The Glass Temperature (``glass-liquid transition temperature&#39;&#39; or ``glass transition temperature&#39;&#39;) is the reversible transition in amorphous materials (or in amorphous regions within semicrystalline materials) from a hard and relatively brittle state into a molten or rubber-like state.</rdfs:comment>
        <or:termString xml:lang="en">glass temperature</or:termString>
        <or:termString xml:lang="en">glass transition temperature</or:termString>
        <or:termString xml:lang="en">glass-liquid transition temperature</or:termString>
        <or:unitTypeFor rdf:resource="&or;UnitOfTemperature"/>
    </owl:NamedIndividual>
    


    <!-- http://www.nist.gov/itl/ssd/Materials#GramsPerCubicMeter -->

    <owl:NamedIndividual rdf:about="&mat;GramsPerCubicMeter">
        <rdf:type rdf:resource="&or;MetricUnit"/>
        <rdf:type rdf:resource="&or;UnitOfDensity"/>
        <or:termString>g m^-3</or:termString>
        <or:termString>g/m^3</or:termString>
        <or:termString xml:lang="en">gram per cubic meter</or:termString>
    </owl:NamedIndividual>
    


    <!-- http://www.nist.gov/itl/ssd/Materials#HeatCapacity -->

    <owl:NamedIndividual rdf:about="&mat;HeatCapacity">
        <rdf:type rdf:resource="&mat;ThermalProperty"/>
        <rdfs:comment>Heat capacity (thermal capacity) is the measurable physical quantity that characterizes the amount of heat required to change a substance&#39;s temperature by a given amount.  It is commonly expressed in expressed in units of joule(s) (J) per degree kelvin (K).</rdfs:comment>
        <or:termString xml:lang="en">enthalpy difference</or:termString>
        <or:termString xml:lang="en">heat capacity</or:termString>
        <or:termString xml:lang="en">thermal capacity</or:termString>
        <or:unitTypeFor rdf:resource="&or;UnitOfEnergy"/>
    </owl:NamedIndividual>
    


    <!-- http://www.nist.gov/itl/ssd/Materials#HeatTreating -->

    <owl:NamedIndividual rdf:about="&mat;HeatTreating"/>
    


    <!-- http://www.nist.gov/itl/ssd/Materials#HelmholtzFreeEnergy -->

    <owl:NamedIndividual rdf:about="&mat;HelmholtzFreeEnergy">
        <rdf:type rdf:resource="&mat;ThermalProperty"/>
        <or:termString xml:lang="en">Helmholtz energy</or:termString>
        <or:termString xml:lang="en">Helmholtz free energy</or:termString>
        <or:termString xml:lang="en">Helmholtz function</or:termString>
        <rdfs:comment xml:lang="en">Tthe Helmholtz free energy is a thermodynamic potential that measures the “useful” work obtainable from a closed thermodynamic system at a constant temperature and volume.</rdfs:comment>
        <or:termString xml:lang="en">free energy</or:termString>
        <or:unitTypeFor rdf:resource="&or;UnitOfEnergy"/>
    </owl:NamedIndividual>
    


    <!-- http://www.nist.gov/itl/ssd/Materials#Henry -->

    <owl:NamedIndividual rdf:about="&mat;Henry">
        <rdf:type rdf:resource="&mat;UnitOfInductance"/>
        <rdf:type rdf:resource="&or;SI_Unit"/>
    </owl:NamedIndividual>
    


    <!-- http://www.nist.gov/itl/ssd/Materials#HexagonalClosePackedCrystalStructure -->

    <owl:NamedIndividual rdf:about="&mat;HexagonalClosePackedCrystalStructure">
        <rdf:type rdf:resource="&mat;CrystalStructure"/>
    </owl:NamedIndividual>
    


    <!-- http://www.nist.gov/itl/ssd/Materials#Hydroforming -->

    <owl:NamedIndividual rdf:about="&mat;Hydroforming"/>
    


    <!-- http://www.nist.gov/itl/ssd/Materials#InHg -->

    <owl:NamedIndividual rdf:about="&mat;InHg">
        <rdf:type rdf:resource="&or;UnitOfPressure"/>
        <rdfs:comment xml:lang="en">in Hg</rdfs:comment>
        <rdfs:comment xml:lang="en">inch of mercury</rdfs:comment>
        <rdfs:comment xml:lang="en">inches of mercury</rdfs:comment>
    </owl:NamedIndividual>
    


    <!-- http://www.nist.gov/itl/ssd/Materials#IntrinsicDiffusionCoefficient -->

    <owl:NamedIndividual rdf:about="&mat;IntrinsicDiffusionCoefficient">
        <rdf:type rdf:resource="&mat;DiffusionProperty"/>
        <rdfs:seeAlso xml:lang="en">Definitions of terms for diffusion in the solid state (IUPAC Recommendations 1999), Pure Appl. Chem. 71, 1307-1325.</rdfs:seeAlso>
        <rdfs:comment xml:lang="en">In multicomponent diffusion, each individual component has its own Intrinsic Diffusion Coefficient.</rdfs:comment>
        <or:unitTypeFor rdf:resource="&mat;UnitOfAreaPerTime"/>
    </owl:NamedIndividual>
    


    <!-- http://www.nist.gov/itl/ssd/Materials#IntrinsicDiffusivity -->

    <owl:NamedIndividual rdf:about="&mat;IntrinsicDiffusivity">
        <rdf:type rdf:resource="&mat;MeasurableMechanicalProperty"/>
    </owl:NamedIndividual>
    


    <!-- http://www.nist.gov/itl/ssd/Materials#InverseDegreeCelsius -->

    <owl:NamedIndividual rdf:about="&mat;InverseDegreeCelsius">
        <rdf:type rdf:resource="&mat;UnitOfInverseTemperatureDifference"/>
        <rdf:type rdf:resource="&or;MetricUnit"/>
        <or:termString>1 / 1C</or:termString>
        <or:termString>1 / 1K</or:termString>
        <rdfs:comment xml:lang="en">An Inverse Degree Celsius is equal to 1/ (1 C)  ; equivalently 1/ (1 K) .</rdfs:comment>
        <or:termString xml:lang="en">inverse Celsius degree</or:termString>
        <or:termString xml:lang="en">inverse kelvin degree</or:termString>
    </owl:NamedIndividual>
    


    <!-- http://www.nist.gov/itl/ssd/Materials#InverseMeterSquaredPerSecond -->

    <owl:NamedIndividual rdf:about="&mat;InverseMeterSquaredPerSecond">
        <rdf:type rdf:resource="&mat;UnitOfInverseAreaPerTime"/>
        <rdf:type rdf:resource="&or;MetricUnit"/>
        <rdfs:comment xml:lang="en">The unit, Inverse Meter Squared per Second equals 1 meter^-2 / second.</rdfs:comment>
    </owl:NamedIndividual>
    


    <!-- http://www.nist.gov/itl/ssd/Materials#InversePSI -->

    <owl:NamedIndividual rdf:about="&mat;InversePSI">
        <rdf:type rdf:resource="&mat;UnitOfAreaPerForce"/>
        <or:termString xml:lang="en">PSI^-1</or:termString>
        <or:termString xml:lang="en">square inch per pound</or:termString>
    </owl:NamedIndividual>
    


    <!-- http://www.nist.gov/itl/ssd/Materials#InversePascal -->

    <owl:NamedIndividual rdf:about="&mat;InversePascal">
        <rdf:type rdf:resource="&mat;UnitOfAreaPerForce"/>
        <or:termString xml:lang="en">Pascal^-1</or:termString>
    </owl:NamedIndividual>
    


    <!-- http://www.nist.gov/itl/ssd/Materials#InverseSecond -->

    <owl:NamedIndividual rdf:about="&mat;InverseSecond">
        <rdf:type rdf:resource="&mat;UnitOfInverseTime"/>
        <rdfs:comment xml:lang="en">One Inverse Second = 1/second .</rdfs:comment>
    </owl:NamedIndividual>
    


    <!-- http://www.nist.gov/itl/ssd/Materials#IonBeamSputtering -->

    <owl:NamedIndividual rdf:about="&mat;IonBeamSputtering"/>
    


    <!-- http://www.nist.gov/itl/ssd/Materials#IsothermalCompressibility -->

    <owl:NamedIndividual rdf:about="&mat;IsothermalCompressibility">
        <rdf:type rdf:resource="&mat;Compressibility"/>
        <or:unitTypeFor rdf:resource="&mat;UnitOfAreaPerForce"/>
    </owl:NamedIndividual>
    


    <!-- http://www.nist.gov/itl/ssd/Materials#JoulePerGramKelvin -->

    <owl:NamedIndividual rdf:about="&mat;JoulePerGramKelvin">
        <rdf:type rdf:resource="&mat;UnitOfSpecificHeatCapacity"/>
        <rdf:type rdf:resource="&or;MetricUnit"/>
        <or:termString>J/g/K</or:termString>
        <or:termString xml:lang="en">joule per gram Kelvin</or:termString>
    </owl:NamedIndividual>
    


    <!-- http://www.nist.gov/itl/ssd/Materials#JoulePerKelvin -->

    <owl:NamedIndividual rdf:about="&mat;JoulePerKelvin">
        <rdf:type rdf:resource="&mat;UnitOfEnergyPerTemperatureDifference"/>
        <or:termString xml:lang="en">Joule/Celsius</or:termString>
        <or:termString xml:lang="en">Joule/Kelvin</or:termString>
    </owl:NamedIndividual>
    


    <!-- http://www.nist.gov/itl/ssd/Materials#JoulePerKg -->

    <owl:NamedIndividual rdf:about="&mat;JoulePerKg">
        <rdf:type rdf:resource="&mat;UnitOfEnergyPerMass"/>
        <rdf:type rdf:resource="&or;MetricUnit"/>
        <rdfs:comment xml:lang="en">Joules per kilogram</rdfs:comment>
    </owl:NamedIndividual>
    


    <!-- http://www.nist.gov/itl/ssd/Materials#JoulePerKgK -->

    <owl:NamedIndividual rdf:about="&mat;JoulePerKgK">
        <rdf:type rdf:resource="&mat;UnitOfSpecificHeatCapacity"/>
        <rdf:type rdf:resource="&or;SI_Unit"/>
        <or:termString>J/(kg*K)</or:termString>
        <or:termString xml:lang="en">joule per kg - degree kelvin</or:termString>
    </owl:NamedIndividual>
    


    <!-- http://www.nist.gov/itl/ssd/Materials#KgPerM3 -->

    <owl:NamedIndividual rdf:about="&mat;KgPerM3">
        <rdf:type rdf:resource="&or;SI_Unit"/>
        <rdf:type rdf:resource="&or;UnitOfDensity"/>
        <rdfs:comment xml:lang="en">Kilograms per cubic meter</rdfs:comment>
    </owl:NamedIndividual>
    


    <!-- http://www.nist.gov/itl/ssd/Materials#Kilobar -->

    <owl:NamedIndividual rdf:about="&mat;Kilobar">
        <rdf:type rdf:resource="&or;UnitOfPressure"/>
        <rdfs:comment xml:lang="en">A kilobar is 1000 bars.</rdfs:comment>
        <or:termString xml:lang="en">kbar</or:termString>
        <or:termString xml:lang="en">kilobar</or:termString>
    </owl:NamedIndividual>
    


    <!-- http://www.nist.gov/itl/ssd/Materials#KilocaloriePerKelvin -->

    <owl:NamedIndividual rdf:about="&mat;KilocaloriePerKelvin">
        <rdf:type rdf:resource="&mat;UnitOfEnergyPerTemperatureDifference"/>
        <or:termString>Cal/K</or:termString>
        <or:termString xml:lang="en">Calorie per Kelvin</or:termString>
        <or:termString xml:lang="en">kilocalorie per Kelvin</or:termString>
    </owl:NamedIndividual>
    


    <!-- http://www.nist.gov/itl/ssd/Materials#KirkendallVelocity -->

    <owl:NamedIndividual rdf:about="&mat;KirkendallVelocity">
        <rdf:type rdf:resource="&mat;DiffusionProperty"/>
        <rdfs:seeAlso>Definitions of terms for diffusion in the solid state (IUPAC Recommendations 1999), Pure Appl. Chem. 71, 1307-1325.</rdfs:seeAlso>
        <or:termString>Kirkendall velocity</or:termString>
        <rdfs:comment xml:lang="en">The Kirkendall velocity is the velocity of the diffusion zone in a multicomponent system, relative to the fixed ends of the specimen. It results from the net nonzero flux of vacancies in the diffusion region.</rdfs:comment>
    </owl:NamedIndividual>
    


    <!-- http://www.nist.gov/itl/ssd/Materials#KsiSquareRootOfInch -->

    <owl:NamedIndividual rdf:about="&mat;KsiSquareRootOfInch">
        <rdf:type rdf:resource="&mat;UnitOfToughness"/>
        <rdf:type rdf:resource="&or;NonMetricUnit"/>
        <or:termString>ksi*(inch)^1/2</or:termString>
        <owl:sameAs rdf:resource="&mat;PascalSquareRootOfMeter"/>
    </owl:NamedIndividual>
    


    <!-- http://www.nist.gov/itl/ssd/Materials#LAMMPS -->

    <owl:NamedIndividual rdf:about="&mat;LAMMPS">
        <rdf:type rdf:resource="&or;ApplicationProgram"/>
        <rdfs:comment xml:lang="en">LAMMPS (Large-scale Atomic/Molecular Massively Parallel Simulator) is an open-source molecular dynamics program from Sandia National Laboratories</rdfs:comment>
    </owl:NamedIndividual>
    


    <!-- http://www.nist.gov/itl/ssd/Materials#Lapping -->

    <owl:NamedIndividual rdf:about="&mat;Lapping"/>
    


    <!-- http://www.nist.gov/itl/ssd/Materials#LatentHeatOfFusion -->

    <owl:NamedIndividual rdf:about="&mat;LatentHeatOfFusion">
        <rdf:type rdf:resource="&mat;ThermalProperty"/>
        <rdfs:comment xml:lang="en">The latent heat of fusion (or ``enthalpy of fusion&#39;&#39;) is the change in enthalpy resulting from heating one mole of a substance to change its state from a solid to a liquid.</rdfs:comment>
        <or:termString xml:lang="en">enthalpy of fusion</or:termString>
        <or:termString xml:lang="en">latent heat of fusion</or:termString>
        <or:unitTypeFor rdf:resource="&or;UnitOfEnergy"/>
    </owl:NamedIndividual>
    


    <!-- http://www.nist.gov/itl/ssd/Materials#LatentHeatOfVaporization -->

    <owl:NamedIndividual rdf:about="&mat;LatentHeatOfVaporization">
        <rdf:type rdf:resource="&mat;PressureDependentProperty"/>
        <rdf:type rdf:resource="&mat;ThermalProperty"/>
        <rdfs:comment xml:lang="en">The latent heat of vaporization (or ``enthalpy of vaporization&#39;&#39; or ``heat of evaporation&#39;&#39;) is the energy required to transform a given quantity of a substance from a liquid into a gas at a given pressure (often atmospheric pressure).</rdfs:comment>
        <or:termString xml:lang="en">enthalpy of vaporization</or:termString>
        <or:termString xml:lang="en">heat of evaporation</or:termString>
        <or:termString xml:lang="en">heat of vaporization</or:termString>
        <or:termString xml:lang="en">latent heat of vaporization</or:termString>
        <or:unitTypeFor rdf:resource="&or;UnitOfEnergy"/>
    </owl:NamedIndividual>
    


    <!-- http://www.nist.gov/itl/ssd/Materials#LatheSectioning -->

    <owl:NamedIndividual rdf:about="&mat;LatheSectioning"/>
    


    <!-- http://www.nist.gov/itl/ssd/Materials#LeadAlloy -->

    <owl:NamedIndividual rdf:about="&mat;LeadAlloy">
        <rdf:type rdf:resource="&mat;NonFerrousAlloyTypeByMainConstituent"/>
        <or:referenceURL rdf:datatype="&xsd;anyURI">http://www.matweb.com/index.aspx</or:referenceURL>
        <rdfs:comment xml:lang="en">An alloy that contains Lead but not Iron.</rdfs:comment>
        <bc:primaryConstituentType rdf:resource="&bc;Lead"/>
    </owl:NamedIndividual>
    


    <!-- http://www.nist.gov/itl/ssd/Materials#LinearCompressibility -->

    <owl:NamedIndividual rdf:about="&mat;LinearCompressibility">
        <rdf:type rdf:resource="&mat;Compressibility"/>
    </owl:NamedIndividual>
    


    <!-- http://www.nist.gov/itl/ssd/Materials#LiquidSubstance -->

    <owl:NamedIndividual rdf:about="&mat;LiquidSubstance">
        <rdf:type rdf:resource="&mat;MaterialForm"/>
        <rdf:type rdf:resource="&mat;StateOfMatter"/>
        <rdfs:comment xml:lang="en">Material in a liquid phase.</rdfs:comment>
    </owl:NamedIndividual>
    


    <!-- http://www.nist.gov/itl/ssd/Materials#LiquidusTemperature -->

    <owl:NamedIndividual rdf:about="&mat;LiquidusTemperature">
        <rdf:type rdf:resource="&mat;ThermalProperty"/>
        <rdfs:comment xml:lang="en">The liquidus temperature, TL or Tliq, is mostly used for glasses, alloys and rocks. It specifies the maximum temperature at which crystals can co-exist with liquid in thermodynamic equilibrium.  For a mixture the solidus temperature depends upon the relative concentration of the substances in the liquid   Above the liquidus temperature the material is homogeneous and liquid at equilibrium. Below the liquidus temperature  crystals form in the liquid..</rdfs:comment>
        <or:unitTypeFor rdf:resource="&or;UnitOfTemperature"/>
    </owl:NamedIndividual>
    


    <!-- http://www.nist.gov/itl/ssd/Materials#LongTon -->

    <owl:NamedIndividual rdf:about="&mat;LongTon">
        <rdf:type rdf:resource="&or;NonMetricUnit"/>
        <rdf:type rdf:resource="&or;UnitOfForce"/>
        <rdfs:comment xml:lang="en">A Long Ton is a unit of weight/force equal to 2240 pounds.</rdfs:comment>
        <or:termString xml:lang="en">long ton</or:termString>
    </owl:NamedIndividual>
    


    <!-- http://www.nist.gov/itl/ssd/Materials#LossCoefficient -->

    <owl:NamedIndividual rdf:about="&mat;LossCoefficient">
        <rdf:type rdf:resource="&mat;DeformationProperty"/>
        <rdfs:comment xml:lang="en">The Loss Coefficient measures the degree to which a material dissipates vibrational energy.  It is the natural log of the ratio of successive amplitudes of vibration in the material.</rdfs:comment>
        <or:termString xml:lang="en">damping capacity</or:termString>
        <or:termString xml:lang="en">loss coefficient</or:termString>
        <or:unitTypeFor rdf:resource="&or;DimensionlessUnit"/>
    </owl:NamedIndividual>
    


    <!-- http://www.nist.gov/itl/ssd/Materials#MagnesiumAlloy -->

    <owl:NamedIndividual rdf:about="&mat;MagnesiumAlloy">
        <rdf:type rdf:resource="&mat;NonFerrousAlloyTypeByMainConstituent"/>
        <or:referenceURL rdf:datatype="&xsd;anyURI">http://www.matweb.com/index.aspx</or:referenceURL>
        <rdfs:comment xml:lang="en">An alloy that contains Magnesium but not Iron.</rdfs:comment>
        <bc:primaryConstituentType rdf:resource="&bc;Magnesium"/>
    </owl:NamedIndividual>
    


    <!-- http://www.nist.gov/itl/ssd/Materials#MagnesiumOxide -->

    <owl:NamedIndividual rdf:about="&mat;MagnesiumOxide">
        <rdf:type rdf:resource="&bc;ChemicalSubstanceTypeByChemicalSpecies"/>
        <or:referenceURL rdf:datatype="&xsd;anyURI">http://www.matweb.com/index.aspx</or:referenceURL>
        <or:termString xml:lang="en">magnesium oxide</or:termString>
    </owl:NamedIndividual>
    


    <!-- http://www.nist.gov/itl/ssd/Materials#MagneticMoment -->

    <owl:NamedIndividual rdf:about="&mat;MagneticMoment">
        <rdf:type rdf:resource="&mat;MagneticProperty"/>
    </owl:NamedIndividual>
    


    <!-- http://www.nist.gov/itl/ssd/Materials#MagneticPermeability -->

    <owl:NamedIndividual rdf:about="&mat;MagneticPermeability">
        <rdf:type rdf:resource="&mat;MagneticProperty"/>
        <rdfs:comment xml:lang="en">Magnetic Permeability is the measure of the ability of a material to support the formation of a magnetic field within itself. In other words, it is the degree of magnetization that a material obtains in response to an applied magnetic field.  The reciprocal of magnetic permeability is magnetic reluctivity.

In SI units, permeability is measured in henrys per meter (H·m−1), or newtons per ampere squared (N·A−2).</rdfs:comment>
    </owl:NamedIndividual>
    


    <!-- http://www.nist.gov/itl/ssd/Materials#MagneticSuscepibility -->

    <owl:NamedIndividual rdf:about="&mat;MagneticSuscepibility">
        <rdf:type rdf:resource="&mat;MagneticProperty"/>
        <rdfs:comment xml:lang="en">Magnetic Susceptibility is a dimensionless proportionality constant that indicates the degree of magnetization of a material in response to an applied magnetic field.</rdfs:comment>
    </owl:NamedIndividual>
    


    <!-- http://www.nist.gov/itl/ssd/Materials#MassFraction -->

    <owl:NamedIndividual rdf:about="&mat;MassFraction">
        <rdf:type rdf:resource="&bc;UnitOfConcentrationByMass"/>
        <rdf:type rdf:resource="&or;DimensionlessUnit"/>
        <or:termString xml:lang="en">mass fraction</or:termString>
    </owl:NamedIndividual>
    


    <!-- http://www.nist.gov/itl/ssd/Materials#MassOfObject -->

    <owl:NamedIndividual rdf:about="&mat;MassOfObject">
        <rdf:type rdf:resource="&mat;MeasurableMechanicalProperty"/>
        <or:unitTypeFor rdf:resource="&or;UnitOfMass"/>
    </owl:NamedIndividual>
    


    <!-- http://www.nist.gov/itl/ssd/Materials#MaterialSuspension -->

    <owl:NamedIndividual rdf:about="&mat;MaterialSuspension">
        <rdf:type rdf:resource="&mat;MaterialForm"/>
    </owl:NamedIndividual>
    


    <!-- http://www.nist.gov/itl/ssd/Materials#MaterialToughness -->

    <owl:NamedIndividual rdf:about="&mat;MaterialToughness">
        <rdf:type rdf:resource="&mat;DeformationProperty"/>
        <rdfs:comment xml:lang="en">Material  Toughness is the ability of a material to absorb energy and plastically deform without fracturing.  It can be defined as the amount of energy per volume that a material can absorb before rupturing or as the resistance to fracture of a material when stressed.</rdfs:comment>
        <or:termString xml:lang="en">material toughness</or:termString>
        <or:termString xml:lang="en">toughness</or:termString>
    </owl:NamedIndividual>
    


    <!-- http://www.nist.gov/itl/ssd/Materials#MaximumServiceTemperature -->

    <owl:NamedIndividual rdf:about="&mat;MaximumServiceTemperature">
        <rdf:type rdf:resource="&mat;ThermalProperty"/>
        <or:unitTypeFor rdf:resource="&or;UnitOfTemperature"/>
    </owl:NamedIndividual>
    


    <!-- http://www.nist.gov/itl/ssd/Materials#MechanicalStress -->

    <owl:NamedIndividual rdf:about="&mat;MechanicalStress">
        <rdf:type rdf:resource="&mat;DeformationProperty"/>
        <rdfs:comment xml:lang="en">Stress is a measure of the internal forces acting within a deformable body. Quantitatively, it is a measure of the average force per unit area of a surface within the body on which internal forces which arise as a reaction to external forces applied to the body act.</rdfs:comment>
        <or:termString xml:lang="en">mechanical stress</or:termString>
        <or:termString xml:lang="en">stress</or:termString>
        <or:unitTypeFor rdf:resource="&or;UnitOfPressure"/>
    </owl:NamedIndividual>
    


    <!-- http://www.nist.gov/itl/ssd/Materials#MeltingPoint -->

    <owl:NamedIndividual rdf:about="&mat;MeltingPoint">
        <rdf:type rdf:resource="&mat;PressureDependentProperty"/>
        <rdf:type rdf:resource="&mat;ThermalProperty"/>
        <or:referenceURL rdf:datatype="&xsd;anyURI">http://www.iupac.org/namespaces/ThermoML</or:referenceURL>
        <rdfs:comment xml:lang="en">Melting or freezing point</rdfs:comment>
        <or:termString xml:lang="en">freezing point</or:termString>
        <or:termString xml:lang="en">melting point</or:termString>
        <or:termString xml:lang="en">melting temperature</or:termString>
        <or:unitTypeFor rdf:resource="&or;UnitOfTemperature"/>
    </owl:NamedIndividual>
    


    <!-- http://www.nist.gov/itl/ssd/Materials#MicrosectioningThroughAnodizing -->

    <owl:NamedIndividual rdf:about="&mat;MicrosectioningThroughAnodizing"/>
    


    <!-- http://www.nist.gov/itl/ssd/Materials#MicrosectioningThroughChemicalDissolution -->

    <owl:NamedIndividual rdf:about="&mat;MicrosectioningThroughChemicalDissolution"/>
    


    <!-- http://www.nist.gov/itl/ssd/Materials#MicrosectioningThroughSputtering -->

    <owl:NamedIndividual rdf:about="&mat;MicrosectioningThroughSputtering"/>
    


    <!-- http://www.nist.gov/itl/ssd/Materials#MicrotomeSectioning -->

    <owl:NamedIndividual rdf:about="&mat;MicrotomeSectioning"/>
    


    <!-- http://www.nist.gov/itl/ssd/Materials#MohsHardness -->

    <owl:NamedIndividual rdf:about="&mat;MohsHardness">
        <rdf:type rdf:resource="&mat;ScratchHardness"/>
        <rdfs:comment xml:lang="en">The Mohs scale of mineral hardness characterizes the scratch resistance of various minerals through the ability of a harder material to scratch a softer material.  On the scale Talc is 1; Gypsum is 2; Calcite is 3; Fluorite is 4; Apatite is 5; Orthoclase Feldspar is 6; Quartz is 7; Topaz is 8; Corundum is 9; and Diamond is 10.</rdfs:comment>
    </owl:NamedIndividual>
    


    <!-- http://www.nist.gov/itl/ssd/Materials#Molality -->

    <owl:NamedIndividual rdf:about="&mat;Molality">
        <rdf:type rdf:resource="&bc;ConcentrationProperty"/>
        <rdfs:comment xml:lang="en">In chemistry, Molality of a solvent/solute combination is defined as the amount of solute, (in moles), divided by the mass of the solvent (in kg), (not the mass of the solution).</rdfs:comment>
        <or:unitTypeFor rdf:resource="&or;DimensionlessUnit"/>
    </owl:NamedIndividual>
    


    <!-- http://www.nist.gov/itl/ssd/Materials#MolarHeatCapacity -->

    <owl:NamedIndividual rdf:about="&mat;MolarHeatCapacity">
        <rdf:type rdf:resource="&mat;ThermalProperty"/>
        <rdfs:comment xml:lang="en">The Molar Heat Capacity is the heat capacity per unit mass of a material, measured in Joules/(mole K)  (in SI units). </rdfs:comment>
    </owl:NamedIndividual>
    


    <!-- http://www.nist.gov/itl/ssd/Materials#Molarity -->

    <owl:NamedIndividual rdf:about="&mat;Molarity">
        <rdf:type rdf:resource="&bc;ConcentrationProperty"/>
        <rdfs:comment xml:lang="en">In chemistry, the Molarity (or molar concentration), is defined as the amount of a mixture constituent (in moles) divided by the volume of the mixture.</rdfs:comment>
        <or:termString xml:lang="en">molar concentration</or:termString>
        <or:termString xml:lang="en">molarity</or:termString>
        <or:unitTypeFor rdf:resource="&or;DimensionlessUnit"/>
    </owl:NamedIndividual>
    


    <!-- http://www.nist.gov/itl/ssd/Materials#MoleFraction -->

    <owl:NamedIndividual rdf:about="&mat;MoleFraction">
        <rdf:type rdf:resource="&bc;UnitOfConcentration"/>
        <rdf:type rdf:resource="&or;DimensionlessUnit"/>
        <rdfs:comment xml:lang="en">A concentration in Mole Fraction is the number of molecules of a constituent in a mixture divided by the number of molecules of all constituents in the mixture.  This is 0.01 times the Mole Percent of the substance in the mixture.</rdfs:comment>
    </owl:NamedIndividual>
    


    <!-- http://www.nist.gov/itl/ssd/Materials#MolePercent -->

    <owl:NamedIndividual rdf:about="&mat;MolePercent">
        <rdf:type rdf:resource="&bc;UnitOfConcentration"/>
        <rdf:type rdf:resource="&or;DimensionlessUnit"/>
        <rdfs:comment xml:lang="en">A concentration in Mole Percent is 100 times the number of molecules of a constituent in a mixture divided by the number of molecules of all constituents in the mixture.  This is 100 times the Mole Fraction of the substance in the mixture.</rdfs:comment>
    </owl:NamedIndividual>
    


    <!-- http://www.nist.gov/itl/ssd/Materials#Mole_Unit -->

    <owl:NamedIndividual rdf:about="&mat;Mole_Unit">
        <rdf:type rdf:resource="&or;DimensionlessUnit"/>
        <rdfs:comment xml:lang="en">A Mole is a Unit of Measure used to measure amounts of matter in terms of the number of atoms present. One mole of a given substance is a portion of the substance consisting of as many atoms as the number of atoms in twelve grams of carbon-12. This number, known as AvogadrosNumber, is equal to 6.0221421 x 10^23. </rdfs:comment>
        <or:termString xml:lang="en">mole</or:termString>
    </owl:NamedIndividual>
    


    <!-- http://www.nist.gov/itl/ssd/Materials#MolybdenumAlloy -->

    <owl:NamedIndividual rdf:about="&mat;MolybdenumAlloy">
        <rdf:type rdf:resource="&mat;NonFerrousAlloyTypeByMainConstituent"/>
        <or:referenceURL rdf:datatype="&xsd;anyURI">http://www.matweb.com/index.aspx</or:referenceURL>
        <rdfs:comment xml:lang="en">An alloy that contains Molybdenum but not Iron.</rdfs:comment>
        <bc:primaryConstituentType rdf:resource="&bc;Molybdenum"/>
    </owl:NamedIndividual>
    


    <!-- http://www.nist.gov/itl/ssd/Materials#MonoclinicCrystalStructure -->

    <owl:NamedIndividual rdf:about="&mat;MonoclinicCrystalStructure">
        <rdf:type rdf:resource="&mat;CrystalStructure"/>
    </owl:NamedIndividual>
    


    <!-- http://www.nist.gov/itl/ssd/Materials#MonotecticTemperature -->

    <owl:NamedIndividual rdf:about="&mat;MonotecticTemperature">
        <rdf:type rdf:resource="&mat;PressureDependentProperty"/>
        <rdf:type rdf:resource="&mat;ThermalProperty"/>
        <or:referenceURL rdf:datatype="&xsd;anyURI">http://www.iupac.org/namespaces/ThermoML</or:referenceURL>
        <rdfs:comment xml:lang="en">The Monotectic Temperature for a mixture is the temperature of the monotectic point of that mixture at a given pressure.</rdfs:comment>
        <or:termString xml:lang="en">monotectic temperature</or:termString>
        <or:unitTypeFor rdf:resource="&or;UnitOfTemperature"/>
    </owl:NamedIndividual>
    


    <!-- http://www.nist.gov/itl/ssd/Materials#NernstPlanckEquation -->

    <owl:NamedIndividual rdf:about="&mat;NernstPlanckEquation">
        <rdf:type rdf:resource="&or;Equation"/>
        <rdfs:seeAlso xml:lang="en">Definitions of terms for diffusion in the solid state (IUPAC Recommendations 1999), Pure Appl. Chem. 71, 1307-1325.</rdfs:seeAlso>
        <rdfs:comment xml:lang="en">For interdiffusion of two ionic crystals, the Nernst-Planck Equation expresses the relationsip between the intrinsic diffusion coefficients and the tracer diffusion coefficients depending on the mole fractio ns of the two constiuents.  This relation holds under that assumption that only the two specified components are moble, and that they diffuse on a common sublatice.</rdfs:comment>
    </owl:NamedIndividual>
    


    <!-- http://www.nist.gov/itl/ssd/Materials#NeumannsPrinciple -->

    <owl:NamedIndividual rdf:about="&mat;NeumannsPrinciple">
        <rdf:type rdf:resource="&doc;GenericScientificModel"/>
        <rdfs:seeAlso xml:lang="en">Definitions of terms for diffusion in the solid state (IUPAC Recommendations 1999), Pure Appl. Chem. 71, 1307-1325.</rdfs:seeAlso>
        <rdfs:comment xml:lang="en">Neumann’s principle (also known as Curie principle or Curie–Neumann’s principle) states that if a coordinate transformation follows the symmetry operations of the crystalline lattice in question, then that transformation leaves the diffusivity tensor invariant.</rdfs:comment>
    </owl:NamedIndividual>
    


    <!-- http://www.nist.gov/itl/ssd/Materials#NickelAlloy -->

    <owl:NamedIndividual rdf:about="&mat;NickelAlloy">
        <rdf:type rdf:resource="&mat;NonFerrousAlloyTypeByMainConstituent"/>
        <or:referenceURL rdf:datatype="&xsd;anyURI">http://www.matweb.com/index.aspx</or:referenceURL>
        <rdfs:comment xml:lang="en">An alloy that contains Nickel but not Iron.</rdfs:comment>
        <bc:primaryConstituentType rdf:resource="&bc;Nickel"/>
    </owl:NamedIndividual>
    


    <!-- http://www.nist.gov/itl/ssd/Materials#NonFerrousAlloy -->

    <owl:NamedIndividual rdf:about="&mat;NonFerrousAlloy">
        <rdf:type rdf:resource="&mat;AlloyTypeByMainConstituent"/>
        <rdfs:comment xml:lang="en">A non-ferrous alloy is one that does not contain iron.</rdfs:comment>
    </owl:NamedIndividual>
    <rdf:Description>
        <rdf:type rdf:resource="&owl;NegativePropertyAssertion"/>
        <owl:targetIndividual rdf:resource="&bc;Iron"/>
        <owl:assertionProperty rdf:resource="&bc;primaryConstituentType"/>
        <owl:sourceIndividual rdf:resource="&mat;NonFerrousAlloy"/>
    </rdf:Description>
    


    <!-- http://www.nist.gov/itl/ssd/Materials#Ohm -->

    <owl:NamedIndividual rdf:about="&mat;Ohm">
        <rdf:type rdf:resource="&mat;UnitOfElectricalResistance"/>
        <rdf:type rdf:resource="&or;SI_Unit"/>
    </owl:NamedIndividual>
    


    <!-- http://www.nist.gov/itl/ssd/Materials#OhmMeter -->

    <owl:NamedIndividual rdf:about="&mat;OhmMeter">
        <rdf:type rdf:resource="&mat;UnitOfElectricalResistivity"/>
        <rdf:type rdf:resource="&or;SI_Unit"/>
    </owl:NamedIndividual>
    


    <!-- http://www.nist.gov/itl/ssd/Materials#OnsagersGeneralizedDiffusionEquation -->

    <owl:NamedIndividual rdf:about="&mat;OnsagersGeneralizedDiffusionEquation">
        <rdf:type rdf:resource="&or;Equation"/>
        <rdfs:seeAlso xml:lang="en">Definitions of terms for diffusion in the solid state (IUPAC Recommendations 1999), Pure Appl. Chem. 71, 1307-1325.</rdfs:seeAlso>
    </owl:NamedIndividual>
    


    <!-- http://www.nist.gov/itl/ssd/Materials#Opaque -->

    <owl:NamedIndividual rdf:about="&mat;Opaque">
        <rdf:type rdf:resource="&mat;TransparencyLevel"/>
    </owl:NamedIndividual>
    


    <!-- http://www.nist.gov/itl/ssd/Materials#OrthorhombicCrystalStructure -->

    <owl:NamedIndividual rdf:about="&mat;OrthorhombicCrystalStructure">
        <rdf:type rdf:resource="&mat;CrystalStructure"/>
    </owl:NamedIndividual>
    


    <!-- http://www.nist.gov/itl/ssd/Materials#PascalSquareRootOfMeter -->

    <owl:NamedIndividual rdf:about="&mat;PascalSquareRootOfMeter">
        <rdf:type rdf:resource="&mat;UnitOfToughness"/>
        <rdf:type rdf:resource="&or;SI_Unit"/>
        <or:termString>Ps*(m)^1/2</or:termString>
        <rdfs:comment xml:lang="en">This is equal to 1 Pa*(M)^1/2 .</rdfs:comment>
    </owl:NamedIndividual>
    


    <!-- http://www.nist.gov/itl/ssd/Materials#PasteSubstance -->

    <owl:NamedIndividual rdf:about="&mat;PasteSubstance">
        <rdf:type rdf:resource="&mat;MaterialPhaseComposition"/>
        <rdfs:comment xml:lang="en">A Paste is a substance that behaves as a solid until a sufficiently large load or stress is applied, at which point it flows like a fluid.  Pastes typically consist of a suspension of granular material in a background fluid.  Pastes are distinct from gels, whose particles interconnect.</rdfs:comment>
    </owl:NamedIndividual>
    


    <!-- http://www.nist.gov/itl/ssd/Materials#PeritecticTemperature -->

    <owl:NamedIndividual rdf:about="&mat;PeritecticTemperature">
        <rdf:type rdf:resource="&mat;PressureDependentProperty"/>
        <rdf:type rdf:resource="&mat;ThermalProperty"/>
        <or:referenceURL rdf:datatype="&xsd;anyURI">http://www.iupac.org/namespaces/ThermoML</or:referenceURL>
        <rdfs:comment xml:lang="en">The Peritectic Temperature for a mixture is the temperature of the peritectic point of that mixture at a given pressure.</rdfs:comment>
        <or:termString xml:lang="en">peritectic temperature</or:termString>
        <or:unitTypeFor rdf:resource="&or;UnitOfTemperature"/>
    </owl:NamedIndividual>
    


    <!-- http://www.nist.gov/itl/ssd/Materials#PoissonRatio -->

    <owl:NamedIndividual rdf:about="&mat;PoissonRatio">
        <rdf:type rdf:resource="&mat;DeformationProperty"/>
        <or:termString xml:lang="en">Poisson ratio</or:termString>
        <or:unitTypeFor xml:lang="en">The Poisson Ratio of a material is the ratio, when an object composed of that material is stretched, of the transverse contraction or strain (perpendicular to the applied load), to the extension or axial strain in the direction of the applied load.</or:unitTypeFor>
        <or:unitTypeFor rdf:resource="&or;DimensionlessUnit"/>
    </owl:NamedIndividual>
    


    <!-- http://www.nist.gov/itl/ssd/Materials#Polishing -->

    <owl:NamedIndividual rdf:about="&mat;Polishing"/>
    


    <!-- http://www.nist.gov/itl/ssd/Materials#PoundForce -->

    <owl:NamedIndividual rdf:about="&mat;PoundForce">
        <rdf:type rdf:resource="&or;NonMetricUnit"/>
        <rdf:type rdf:resource="&or;UnitOfForce"/>
        <or:termString xml:lang="en">pound</or:termString>
    </owl:NamedIndividual>
    


    <!-- http://www.nist.gov/itl/ssd/Materials#PoundSterling -->

    <owl:NamedIndividual rdf:about="&mat;PoundSterling">
        <rdf:type rdf:resource="&or;PrimaryCurrencyUnit"/>
    </owl:NamedIndividual>
    


    <!-- http://www.nist.gov/itl/ssd/Materials#PowderySubstance -->

    <owl:NamedIndividual rdf:about="&mat;PowderySubstance">
        <rdf:type rdf:resource="&mat;MaterialPhaseComposition"/>
        <rdfs:comment xml:lang="en">material in a solid powdery phase</rdfs:comment>
    </owl:NamedIndividual>
    


    <!-- http://www.nist.gov/itl/ssd/Materials#PureSubstance -->

    <owl:NamedIndividual rdf:about="&mat;PureSubstance">
        <rdf:type rdf:resource="&mat;MaterialForm"/>
        <rdfs:comment xml:lang="en">A Pure Substance is a substance made up of a single form of molecule, or in the case of a metal, a single type of atom.  This does not not mean that there may not be impurities.</rdfs:comment>
    </owl:NamedIndividual>
    


    <!-- http://www.nist.gov/itl/ssd/Materials#Quartz -->

    <owl:NamedIndividual rdf:about="&mat;Quartz">
        <rdf:type rdf:resource="&mat;MineralType"/>
        <rdfs:comment xml:lang="en">Quartz is a common mineral of SiO4 with a hexagonal crystalline structure.  Impurities may color this otherwise colorless mineral.</rdfs:comment>
    </owl:NamedIndividual>
    


    <!-- http://www.nist.gov/itl/ssd/Materials#ReboundHardness -->

    <owl:NamedIndividual rdf:about="&mat;ReboundHardness">
        <rdf:type rdf:resource="&mat;Hardness"/>
    </owl:NamedIndividual>
    


    <!-- http://www.nist.gov/itl/ssd/Materials#RefractiveIndex -->

    <owl:NamedIndividual rdf:about="&mat;RefractiveIndex">
        <rdf:type rdf:resource="&mat;OpticalProperty"/>
        <or:unitTypeFor rdf:resource="&or;DimensionlessUnit"/>
    </owl:NamedIndividual>
    


    <!-- http://www.nist.gov/itl/ssd/Materials#RelaxationMethodForDiffusion -->

    <owl:NamedIndividual rdf:about="&mat;RelaxationMethodForDiffusion">
        <rdf:type rdf:resource="&mat;DiffusionMovementMechanism"/>
        <rdfs:seeAlso xml:lang="en">Definitions of terms for diffusion in the solid state (IUPAC Recommendations 1999), Pure Appl. Chem. 71, 1307-1325.</rdfs:seeAlso>
        <rdfs:comment xml:lang="en">In the Relaxation Mechanism for diffusion, the atoms close to a vacancy relax to such an extent that the regular lattice structure out to several atom distances disappears and diffusion occurs by an irregular jostling motion similar to that for atoms in a liquid.</rdfs:comment>
    </owl:NamedIndividual>
    


    <!-- http://www.nist.gov/itl/ssd/Materials#RhombohedralCrystalStructure -->

    <owl:NamedIndividual rdf:about="&mat;RhombohedralCrystalStructure">
        <rdf:type rdf:resource="&mat;CrystalStructure"/>
        <rdfs:comment xml:lang="en">A lattice system is described by three basis vectors. In the rhombohedral system, the crystal is described by vectors of equal length, no two of which are orthogonal. The rhombohedral system can be thought of as the cubic system stretched along a body diagonal. a = b = c; α = β = γ ≠ 90°. In some classification schemes, the rhombohedral lattice system is combined with the hexagonal lattice system and grouped into a larger hexagonal family.

There is only one rhombohedral Bravais lattice.</rdfs:comment>
    </owl:NamedIndividual>
    


    <!-- http://www.nist.gov/itl/ssd/Materials#Rinsing -->

    <owl:NamedIndividual rdf:about="&mat;Rinsing"/>
    


    <!-- http://www.nist.gov/itl/ssd/Materials#RockwellAHardness -->

    <owl:NamedIndividual rdf:about="&mat;RockwellAHardness">
        <rdf:type rdf:resource="&mat;IndentationHardness"/>
        <rdfs:comment xml:lang="en">A Rockwell Hardness scale using a load of 60 kgf and a 120° diamond cone indenter.</rdfs:comment>
        <or:acronym>HRA</or:acronym>
    </owl:NamedIndividual>
    


    <!-- http://www.nist.gov/itl/ssd/Materials#RockwellBHardness -->

    <owl:NamedIndividual rdf:about="&mat;RockwellBHardness">
        <rdf:type rdf:resource="&mat;IndentationHardness"/>
        <rdfs:comment xml:lang="en">A Rockwell Hardness scale using a load of 100 kgf and a 1⁄8-inch-diameter (1.588 mm) steel sphere indenter.</rdfs:comment>
        <or:acronym>HRB</or:acronym>
    </owl:NamedIndividual>
    


    <!-- http://www.nist.gov/itl/ssd/Materials#RockwellCHardness -->

    <owl:NamedIndividual rdf:about="&mat;RockwellCHardness">
        <rdf:type rdf:resource="&mat;IndentationHardness"/>
        <rdfs:comment xml:lang="en">A Rockwell Hardness scale using a load of 150 kgf and a 120° diamond cone indenter.</rdfs:comment>
        <or:acronym>HRC</or:acronym>
    </owl:NamedIndividual>
    


    <!-- http://www.nist.gov/itl/ssd/Materials#RockwellDHardness -->

    <owl:NamedIndividual rdf:about="&mat;RockwellDHardness">
        <rdf:type rdf:resource="&mat;IndentationHardness"/>
        <or:acronym>HRD</or:acronym>
        <rdfs:comment xml:lang="en">A Rockwell Hardness scale using a load of 100 kgf and a 120° diamond cone indenter.</rdfs:comment>
    </owl:NamedIndividual>
    


    <!-- http://www.nist.gov/itl/ssd/Materials#RockwellEHardness -->

    <owl:NamedIndividual rdf:about="&mat;RockwellEHardness">
        <rdf:type rdf:resource="&mat;IndentationHardness"/>
        <rdfs:comment xml:lang="en">A Rockwell Hardness scale using a load of 100 kgf and a 1⁄8-inch-diameter (3.175 mm) steel sphere indenter.</rdfs:comment>
        <or:acronym>HRE</or:acronym>
    </owl:NamedIndividual>
    


    <!-- http://www.nist.gov/itl/ssd/Materials#RockwellFHardness -->

    <owl:NamedIndividual rdf:about="&mat;RockwellFHardness">
        <rdf:type rdf:resource="&mat;IndentationHardness"/>
        <or:acronym>HRF</or:acronym>
        <rdfs:comment xml:lang="en">A Rockwell Hardness scale using a load of 60 kgf and a 1⁄16-inch-diameter (1.588 mm) steel sphere indenter.</rdfs:comment>
    </owl:NamedIndividual>
    


    <!-- http://www.nist.gov/itl/ssd/Materials#RockwellGHardness -->

    <owl:NamedIndividual rdf:about="&mat;RockwellGHardness">
        <rdf:type rdf:resource="&mat;IndentationHardness"/>
        <or:acronym>HRG</or:acronym>
        <rdfs:comment xml:lang="en">A Rockwell Hardness scale using a load of 150 kgf and a 1⁄16-inch-diameter (1.588 mm) steel sphere indenter.</rdfs:comment>
    </owl:NamedIndividual>
    


    <!-- http://www.nist.gov/itl/ssd/Materials#Rolling_MaterialProcessing -->

    <owl:NamedIndividual rdf:about="&mat;Rolling_MaterialProcessing"/>
    


    <!-- http://www.nist.gov/itl/ssd/Materials#Rubidium -->

    <owl:NamedIndividual rdf:about="&mat;Rubidium"/>
    


    <!-- http://www.nist.gov/itl/ssd/Materials#Ruthenium -->

    <owl:NamedIndividual rdf:about="&mat;Ruthenium"/>
    


    <!-- http://www.nist.gov/itl/ssd/Materials#Rutherfordium -->

    <owl:NamedIndividual rdf:about="&mat;Rutherfordium"/>
    


    <!-- http://www.nist.gov/itl/ssd/Materials#SandiaNationalLaboratories -->

    <owl:NamedIndividual rdf:about="&mat;SandiaNationalLaboratories">
        <rdf:type rdf:resource="&or;ResearchOrganization"/>
    </owl:NamedIndividual>
    


    <!-- http://www.nist.gov/itl/ssd/Materials#SecondLawOfThermodynamics -->

    <owl:NamedIndividual rdf:about="&mat;SecondLawOfThermodynamics">
        <rdf:type rdf:resource="&mat;LawOfThermodynamics"/>
        <rdfs:comment xml:lang="en">The Second Law of Thermodynamics states that the entropy of any isolated system not in thermal equilibrium almost always increases.</rdfs:comment>
        <or:termString xml:lang="en">second law of thermodynamics</or:termString>
    </owl:NamedIndividual>
    


    <!-- http://www.nist.gov/itl/ssd/Materials#SectioningByGrinding -->

    <owl:NamedIndividual rdf:about="&mat;SectioningByGrinding"/>
    


    <!-- http://www.nist.gov/itl/ssd/Materials#SelfDiffusionCoefficient -->

    <owl:NamedIndividual rdf:about="&mat;SelfDiffusionCoefficient">
        <rdf:type rdf:resource="&mat;DiffusionProperty"/>
        <rdfs:seeAlso>IUPAC Gold Book, http://goldbook.iupac.org/S05582.html</rdfs:seeAlso>
        <rdfs:seeAlso>Definitions of terms for diffusion in the solid state (IUPAC Recommendations 1999), Pure Appl. Chem. 71, 1307-1325.</rdfs:seeAlso>
        <rdfs:comment xml:lang="en">The Self-Diffusion Coefficient is the diffusion coefficient Di^* of species i when the chemical potential gradient equals zero.</rdfs:comment>
        <or:termString xml:lang="en">self-diffusion coefficient</or:termString>
        <or:unitTypeFor rdf:resource="&mat;UnitOfAreaPerTime"/>
    </owl:NamedIndividual>
    


    <!-- http://www.nist.gov/itl/ssd/Materials#ShearModulus -->

    <owl:NamedIndividual rdf:about="&mat;ShearModulus">
        <rdf:type rdf:resource="&mat;ElasticModulus"/>
        <rdf:type rdf:resource="&mat;Stiffness"/>
        <rdfs:comment xml:lang="en">The Shear Modulus (modulus of rigidity) describes a material&#39;s response to shearing strains. It is defined as the ratio of shear stress to the shear strain</rdfs:comment>
        <or:termString xml:lang="en">modulus of rigidity</or:termString>
        <rdfs:comment xml:lang="en">shear modulus</rdfs:comment>
        <or:unitTypeFor rdf:resource="&or;UnitOfPressure"/>
    </owl:NamedIndividual>
    


    <!-- http://www.nist.gov/itl/ssd/Materials#SheetForming -->

    <owl:NamedIndividual rdf:about="&mat;SheetForming"/>
    


    <!-- http://www.nist.gov/itl/ssd/Materials#ShoreHardness -->

    <owl:NamedIndividual rdf:about="&mat;ShoreHardness">
        <rdf:type rdf:resource="&mat;IndentationHardness"/>
    </owl:NamedIndividual>
    


    <!-- http://www.nist.gov/itl/ssd/Materials#ShortTon -->

    <owl:NamedIndividual rdf:about="&mat;ShortTon">
        <rdf:type rdf:resource="&or;NonMetricUnit"/>
        <rdf:type rdf:resource="&or;UnitOfForce"/>
        <rdfs:comment xml:lang="en">A Short Ton, or `ton&#39; is a unit of weight/force equal to 2000 pounds.</rdfs:comment>
        <or:termString xml:lang="en">short ton</or:termString>
        <or:termString xml:lang="en">ton</or:termString>
    </owl:NamedIndividual>
    


    <!-- http://www.nist.gov/itl/ssd/Materials#Siemens -->

    <owl:NamedIndividual rdf:about="&mat;Siemens">
        <rdf:type rdf:resource="&mat;UnitOfElectricalConductance"/>
        <rdf:type rdf:resource="&or;SI_Unit"/>
        <rdfs:comment xml:lang="en">The siemens (SI unit symbol: S) is the unit of electric conductance and electric admittance in the International System of Units (SI). Conductance and admittance are the reciprocals of resistance and impedance respectively, hence one siemens is equal to the reciprocal of one ohm, and is also referred to as the mho.</rdfs:comment>
        <or:termString xml:lang="en">mho</or:termString>
        <or:termString xml:lang="en">siemens</or:termString>
    </owl:NamedIndividual>
    


    <!-- http://www.nist.gov/itl/ssd/Materials#SiemensPerMeter -->

    <owl:NamedIndividual rdf:about="&mat;SiemensPerMeter">
        <rdf:type rdf:resource="&mat;UnitOfElectricalConductivity"/>
        <rdf:type rdf:resource="&or;SI_Unit"/>
    </owl:NamedIndividual>
    


    <!-- http://www.nist.gov/itl/ssd/Materials#SignificantDigits -->

    <owl:NamedIndividual rdf:about="&mat;SignificantDigits">
        <rdf:type rdf:resource="&mat;UnitOfPrecision"/>
        <rdf:type rdf:resource="&or;NonMetricUnit"/>
    </owl:NamedIndividual>
    


    <!-- http://www.nist.gov/itl/ssd/Materials#SiliconOxide -->

    <owl:NamedIndividual rdf:about="&mat;SiliconOxide">
        <rdf:type rdf:resource="&bc;ChemicalSubstanceTypeByChemicalSpecies"/>
        <or:referenceURL rdf:datatype="&xsd;anyURI">http://www.matweb.com/index.aspx</or:referenceURL>
        <or:termString xml:lang="en">silicon oxide</or:termString>
    </owl:NamedIndividual>
    


    <!-- http://www.nist.gov/itl/ssd/Materials#Sintering -->

    <owl:NamedIndividual rdf:about="&mat;Sintering"/>
    


    <!-- http://www.nist.gov/itl/ssd/Materials#SolidCrystallineSubstance -->

    <owl:NamedIndividual rdf:about="&mat;SolidCrystallineSubstance">
        <rdf:type rdf:resource="&mat;MaterialForm"/>
    </owl:NamedIndividual>
    


    <!-- http://www.nist.gov/itl/ssd/Materials#SolidSubstance -->

    <owl:NamedIndividual rdf:about="&mat;SolidSubstance">
        <rdf:type rdf:resource="&mat;MaterialForm"/>
        <rdf:type rdf:resource="&mat;StateOfMatter"/>
        <rdfs:comment xml:lang="en">Material in a solid phase.</rdfs:comment>
    </owl:NamedIndividual>
    


    <!-- http://www.nist.gov/itl/ssd/Materials#SolidusTemperature -->

    <owl:NamedIndividual rdf:about="&mat;SolidusTemperature">
        <rdf:type rdf:resource="&mat;PressureDependentProperty"/>
        <rdf:type rdf:resource="&mat;ThermalProperty"/>
        <rdfs:comment xml:lang="en">The solidus temperature is the temperature (at a given temperature) below which a given substance is completely solid and above which it it a mxture of a liquid of one composition and solid crystals of a different compostion.</rdfs:comment>
        <or:unitTypeFor rdf:resource="&or;UnitOfTemperature"/>
    </owl:NamedIndividual>
    


    <!-- http://www.nist.gov/itl/ssd/Materials#SoundVelocity -->

    <owl:NamedIndividual rdf:about="&mat;SoundVelocity">
        <rdf:type rdf:resource="&mat;AcousticProperty"/>
        <rdfs:comment xml:lang="en">Sound Velocity for a substance depends on temperature and to a greater or lesser extent on frequency.  For a gas or vapor it depends on temperature and pressure. For a solid, there are two speeds of sound at the same temperature and frequency, that of a longitudinal (compression) wave, and that of a transverse wave.  In thin rods, the interaction of these two types of waves results in a third sound velocity intermediate between the transverse and longitudinal velocities.</rdfs:comment>
        <or:unitTypeFor rdf:resource="&or;UnitOfVelocity"/>
    </owl:NamedIndividual>
    


    <!-- http://www.nist.gov/itl/ssd/Materials#SpeciesDiffusionMobility -->

    <owl:NamedIndividual rdf:about="&mat;SpeciesDiffusionMobility">
        <rdf:type rdf:resource="&mat;DiffusionProperty"/>
        <rdfs:seeAlso>Definitions of terms for diffusion in the solid state (IUPAC Recommendations 1999), Pure Appl. Chem. 71, 1307-1325.</rdfs:seeAlso>
        <rdfs:comment xml:lang="en">Mass transport in diffusion is described by the mobility of the diffusing species (`Species Diffusion Mobility&#39; -- called `atomic mobility&#39; if atoms are diffusing).  This mobility is equal to the drift velocity of the species divided by the force on the particles.</rdfs:comment>
        <or:termString xml:lang="en">atomic mobility</or:termString>
        <or:termString xml:lang="en">diffusion mobility</or:termString>
        <or:termString xml:lang="en">diffusion mobility of a species</or:termString>
        <or:termString xml:lang="en">mobility</or:termString>
        <or:termString xml:lang="en">species diffusion mobility</or:termString>
    </owl:NamedIndividual>
    


    <!-- http://www.nist.gov/itl/ssd/Materials#SpecificHeatCapacity -->

    <owl:NamedIndividual rdf:about="&mat;SpecificHeatCapacity">
        <rdf:type rdf:resource="&mat;PressureDependentProperty"/>
        <rdf:type rdf:resource="&mat;TemperatureDependentProperty"/>
        <rdf:type rdf:resource="&mat;ThermalProperty"/>
        <rdfs:comment xml:lang="en">The Specific Heat Capacity (or specific heat) is the heat capacity per unit mass of a material, measured in Joules/(kg K)  (in SI units). </rdfs:comment>
        <or:termString xml:lang="en">specific heat</or:termString>
        <or:termString xml:lang="en">specific heat capacity</or:termString>
        <or:unitTypeFor rdf:resource="&mat;UnitOfSpecificHeatCapacity"/>
    </owl:NamedIndividual>
    


    <!-- http://www.nist.gov/itl/ssd/Materials#SpecificStrength -->

    <owl:NamedIndividual rdf:about="&mat;SpecificStrength">
        <rdf:type rdf:resource="&mat;DeformationProperty"/>
        <rdfs:comment xml:lang="en">The specific strength is a material&#39;s ultimate tensile strength (force per unit area at failure) divided by its density. It is also known as the strength-to-weight ratio or strength/weight ratio. The SI unit for specific strength is N·m/kg which is equivalent to (m/s)^2.</rdfs:comment>
        <or:unitTypeFor rdf:resource="&or;UnitOfVelocitySquared"/>
    </owl:NamedIndividual>
    


    <!-- http://www.nist.gov/itl/ssd/Materials#SquareCmPerSecond -->

    <owl:NamedIndividual rdf:about="&mat;SquareCmPerSecond">
        <rdf:type rdf:resource="&mat;UnitOfAreaPerTime"/>
        <rdf:type rdf:resource="&or;CGS_Unit"/>
    </owl:NamedIndividual>
    


    <!-- http://www.nist.gov/itl/ssd/Materials#SquareMeterPerSecond -->

    <owl:NamedIndividual rdf:about="&mat;SquareMeterPerSecond">
        <rdf:type rdf:resource="&mat;UnitOfAreaPerTime"/>
        <rdf:type rdf:resource="&or;SI_Unit"/>
    </owl:NamedIndividual>
    


    <!-- http://www.nist.gov/itl/ssd/Materials#StressGradient -->

    <owl:NamedIndividual rdf:about="&mat;StressGradient">
        <rdf:type rdf:resource="&mat;DeformationProperty"/>
        <rdfs:seeAlso>Definitions of terms for diffusion in the solid state (IUPAC Recommendations 1999), Pure Appl. Chem. 71, 1307-1325.</rdfs:seeAlso>
        <or:termString xml:lang="en">gradient of stress</or:termString>
        <or:termString xml:lang="en">stress gradient</or:termString>
    </owl:NamedIndividual>
    


    <!-- http://www.nist.gov/itl/ssd/Materials#TemperatureOfObject -->

    <owl:NamedIndividual rdf:about="&mat;TemperatureOfObject">
        <rdf:type rdf:resource="&mat;ThermalProperty"/>
        <rdfs:comment xml:lang="en">The property ``Temperature Of Object&#39;&#39; specifies the temperature of some physical object.  The temperature can be expressed in Celcius or kelvins.</rdfs:comment>
        <or:unitTypeFor rdf:resource="&or;UnitOfTemperature"/>
    </owl:NamedIndividual>
    


    <!-- http://www.nist.gov/itl/ssd/Materials#TensileModulus -->

    <owl:NamedIndividual rdf:about="&mat;TensileModulus">
        <rdf:type rdf:resource="&mat;ElasticModulus"/>
        <rdf:type rdf:resource="&mat;Stiffness"/>
        <or:termString>Young&#39;s modulus</or:termString>
        <rdfs:comment xml:lang="en">The Tensile Modulus (or Young&#39;s modulus) is a measure of the stiffness of an elastic material and is a quantity used to characterize materials. It is defined as the ratio of the uniaxial stress over the uniaxial strain in the range of stress in which Hooke&#39;s Law holds.[</rdfs:comment>
        <rdfs:comment xml:lang="en">tensile modulus</rdfs:comment>
        <or:unitTypeFor rdf:resource="&or;UnitOfPressure"/>
    </owl:NamedIndividual>
    


    <!-- http://www.nist.gov/itl/ssd/Materials#TetragonalCrystalStructure -->

    <owl:NamedIndividual rdf:about="&mat;TetragonalCrystalStructure">
        <rdf:type rdf:resource="&mat;CrystalStructure"/>
        <rdfs:comment xml:lang="en">Tetragonal crystal lattices result from stretching a cubic lattice along one of its lattice vectors, so that the cube becomes a rectangular prism with a square base (a by a) and height (c, which is different from a).

There are two tetragonal Bravais lattices: the simple (or primitive) tetragonal (from stretching the simple-cubic lattice) and the body-centered tetragonal (from stretching either the face-centered or the body-centered cubic lattice).</rdfs:comment>
    </owl:NamedIndividual>
    


    <!-- http://www.nist.gov/itl/ssd/Materials#ThermalConductivity -->

    <owl:NamedIndividual rdf:about="&mat;ThermalConductivity">
        <rdf:type rdf:resource="&mat;TemperatureDependentProperty"/>
        <rdf:type rdf:resource="&mat;ThermalProperty"/>
        <rdfs:comment xml:lang="en">Thermal conductivity, (symbol: lambda or kappa), is the property of a material&#39;s ability to conduct heat, normally measured in W/(m·K).</rdfs:comment>
        <or:termString xml:lang="en">thermal conductivity</or:termString>
        <or:unitTypeFor rdf:resource="&mat;UnitOfThermalConductivity"/>
    </owl:NamedIndividual>
    


    <!-- http://www.nist.gov/itl/ssd/Materials#ThermalExpansionCoefficient -->

    <owl:NamedIndividual rdf:about="&mat;ThermalExpansionCoefficient">
        <rdf:type rdf:resource="&mat;PressureDependentProperty"/>
        <rdf:type rdf:resource="&mat;TemperatureDependentProperty"/>
        <rdf:type rdf:resource="&mat;ThermalProperty"/>
        <or:termString xml:lang="en"> temperature coefficient of linear expansion</or:termString>
        <rdfs:comment xml:lang="en">The Thermal Expansion Coefficient of a material is the relative amount it expands per unit increase in temperature.  In SI units it is measured in inverse Celsius degrees.</rdfs:comment>
        <or:termString xml:lang="en">isobaric coefficient of linear expansion</or:termString>
        <or:termString xml:lang="en">linear thermal expansion coefficient</or:termString>
        <or:termString xml:lang="en">thermal expansion coefficient</or:termString>
        <or:unitTypeFor rdf:resource="&mat;UnitOfInverseTemperatureDifference"/>
    </owl:NamedIndividual>
    


    <!-- http://www.nist.gov/itl/ssd/Materials#ThermalShockResistance -->

    <owl:NamedIndividual rdf:about="&mat;ThermalShockResistance">
        <rdf:type rdf:resource="&mat;ThermalProperty"/>
        <rdfs:comment xml:lang="en">Thermal Shock Resistance is a measure of the resistance of an object to the initiation of thermal fracturing, measured as the maximum temperature difference to allow a steady heat flow.</rdfs:comment>
        <or:termString xml:lang="en">thermal shock resistance</or:termString>
        <or:unitTypeFor rdf:resource="&mat;UnitOfTemperatureDifference"/>
    </owl:NamedIndividual>
    


    <!-- http://www.nist.gov/itl/ssd/Materials#ThermodynamicActivity -->

    <owl:NamedIndividual rdf:about="&mat;ThermodynamicActivity">
        <rdf:type rdf:resource="&bc;MeasurableChemicalProperty"/>
        <rdfs:comment xml:lang="en">In chemical thermodynamics, activity (symbol a) is a measure of the &#39;effective concentration&#39; of a species in a mixture, meaning that the species&#39;s chemical potential depends on the activity of a real solution in the same way that it would depend on concentration for an ideal solution.</rdfs:comment>
        <or:termString xml:lang="en">activity</or:termString>
        <or:termString xml:lang="en">thermodynamic activity</or:termString>
        <or:unitTypeFor rdf:resource="&or;DimensionlessUnit"/>
    </owl:NamedIndividual>
    


    <!-- http://www.nist.gov/itl/ssd/Materials#ThirdLawOfThermodynamics -->

    <owl:NamedIndividual rdf:about="&mat;ThirdLawOfThermodynamics">
        <rdf:type rdf:resource="&mat;LawOfThermodynamics"/>
        <rdfs:comment xml:lang="en">The Third Law of Thermodynamics states that the entropy of a system approaches a constant value as the temperature approaches absolute zero.</rdfs:comment>
        <or:termString xml:lang="en">third law of thermodynamics</or:termString>
    </owl:NamedIndividual>
    


    <!-- http://www.nist.gov/itl/ssd/Materials#TinAlloy -->

    <owl:NamedIndividual rdf:about="&mat;TinAlloy">
        <rdf:type rdf:resource="&mat;NonFerrousAlloyTypeByMainConstituent"/>
        <or:referenceURL rdf:datatype="&xsd;anyURI">http://www.matweb.com/index.aspx</or:referenceURL>
        <rdfs:comment xml:lang="en">An alloy that contains Tin but not Iron.</rdfs:comment>
        <bc:primaryConstituentType rdf:resource="&bc;Tin"/>
    </owl:NamedIndividual>
    


    <!-- http://www.nist.gov/itl/ssd/Materials#TitaniumOxide -->

    <owl:NamedIndividual rdf:about="&mat;TitaniumOxide">
        <rdf:type rdf:resource="&bc;ChemicalSubstanceTypeByChemicalSpecies"/>
        <or:referenceURL rdf:datatype="&xsd;anyURI">http://www.matweb.com/index.aspx</or:referenceURL>
        <or:termString xml:lang="en">titanium oxide</or:termString>
    </owl:NamedIndividual>
    


    <!-- http://www.nist.gov/itl/ssd/Materials#Tonne -->

    <owl:NamedIndividual rdf:about="&mat;Tonne">
        <rdf:type rdf:resource="&or;UnitOfMass"/>
        <rdfs:comment xml:lang="en">1000 kg is called a Tonne, sometimes inaccurately a &quot;ton&quot;.</rdfs:comment>
        <or:termString xml:lang="en">megagram</or:termString>
        <or:termString xml:lang="en">metric ton</or:termString>
        <or:termString xml:lang="en">ton</or:termString>
        <or:termString xml:lang="en">tonne</or:termString>
    </owl:NamedIndividual>
    


    <!-- http://www.nist.gov/itl/ssd/Materials#TracerDiffusionCoefficient -->

    <owl:NamedIndividual rdf:about="&mat;TracerDiffusionCoefficient">
        <rdf:type rdf:resource="&mat;DiffusionProperty"/>
        <rdfs:seeAlso>Definitions of terms for diffusion in the solid state (IUPAC Recommendations 1999), Pure Appl. Chem. 71, 1307-1325.</rdfs:seeAlso>
        <or:idString>Di*</or:idString>
        <rdfs:comment xml:lang="en">The Tracer diffusion coefficient is the diffusion coefficient Di* as defined by Fick’s First law for an isotopically labeled atom. The term is usually restricted to the particular simple situation in which a tracer isotope in very dilute concentration is diffused into an otherwise homogeneous material with no driving forces other than the concentration gradient of the tracer itself.</rdfs:comment>
        <or:termString xml:lang="en">tracer diffusion coefficient</or:termString>
        <or:unitTypeFor rdf:resource="&mat;UnitOfAreaPerTime"/>
    </owl:NamedIndividual>
    


    <!-- http://www.nist.gov/itl/ssd/Materials#Translucent -->

    <owl:NamedIndividual rdf:about="&mat;Translucent">
        <rdf:type rdf:resource="&mat;TransparencyLevel"/>
    </owl:NamedIndividual>
    


    <!-- http://www.nist.gov/itl/ssd/Materials#Transparency -->

    <owl:NamedIndividual rdf:about="&mat;Transparency">
        <rdf:type rdf:resource="&mat;OpticalProperty"/>
    </owl:NamedIndividual>
    


    <!-- http://www.nist.gov/itl/ssd/Materials#Transparent -->

    <owl:NamedIndividual rdf:about="&mat;Transparent">
        <rdf:type rdf:resource="&mat;TransparencyLevel"/>
    </owl:NamedIndividual>
    


    <!-- http://www.nist.gov/itl/ssd/Materials#TriclinicCrystalStructure -->

    <owl:NamedIndividual rdf:about="&mat;TriclinicCrystalStructure">
        <rdf:type rdf:resource="&mat;CrystalStructure"/>
        <rdfs:comment xml:lang="en">The triclinic lattice is the least symmetric of the 14 three-dimensional Bravais lattices. It has (itself) the minimum symmetry all lattices have: points of inversion at each lattice point and at 7 more points for each lattice point: at the midpoints of the edges and the faces, and at the center points. It is the only lattice type that itself has no mirror planes.</rdfs:comment>
    </owl:NamedIndividual>
    


    <!-- http://www.nist.gov/itl/ssd/Materials#TrigonalCrystalStructure -->

    <owl:NamedIndividual rdf:about="&mat;TrigonalCrystalStructure">
        <rdf:type rdf:resource="&mat;CrystalStructure"/>
        <rdfs:comment xml:lang="en">The trigonal crystal system is the only crystal system whose point groups have more than one lattice system associated with their space groups: the hexagonal and rhombohedral lattices both appear.</rdfs:comment>
    </owl:NamedIndividual>
    


    <!-- http://www.nist.gov/itl/ssd/Materials#TriplePointPressure -->

    <owl:NamedIndividual rdf:about="&mat;TriplePointPressure">
        <rdf:type rdf:resource="&mat;ThermalProperty"/>
        <or:referenceURL rdf:datatype="&xsd;anyURI">http://www.iupac.org/namespaces/ThermoML</or:referenceURL>
        <or:termString xml:lang="en">triple point pressure</or:termString>
        <or:unitTypeFor rdf:resource="&or;UnitOfPressure"/>
    </owl:NamedIndividual>
    


    <!-- http://www.nist.gov/itl/ssd/Materials#TriplePointTemperature -->

    <owl:NamedIndividual rdf:about="&mat;TriplePointTemperature">
        <rdf:type rdf:resource="&mat;ThermalProperty"/>
        <or:referenceURL rdf:datatype="&xsd;anyURI">http://www.iupac.org/namespaces/ThermoML</or:referenceURL>
        <or:termString xml:lang="en">triple point pressure</or:termString>
        <or:unitTypeFor rdf:resource="&or;UnitOfTemperature"/>
    </owl:NamedIndividual>
    


    <!-- http://www.nist.gov/itl/ssd/Materials#Tritium -->

    <owl:NamedIndividual rdf:about="&mat;Tritium">
        <rdf:type rdf:resource="&mat;Radioisotope"/>
    </owl:NamedIndividual>
    


    <!-- http://www.nist.gov/itl/ssd/Materials#UKPenny -->

    <owl:NamedIndividual rdf:about="&mat;UKPenny">
        <rdf:type rdf:resource="&or;SecondaryCurrencyUnit"/>
    </owl:NamedIndividual>
    


    <!-- http://www.nist.gov/itl/ssd/Materials#USCent -->

    <owl:NamedIndividual rdf:about="&mat;USCent">
        <rdf:type rdf:resource="&or;SecondaryCurrencyUnit"/>
    </owl:NamedIndividual>
    


    <!-- http://www.nist.gov/itl/ssd/Materials#UltimateTensileStrength -->

    <owl:NamedIndividual rdf:about="&mat;UltimateTensileStrength">
        <rdf:type rdf:resource="&mat;DeformationProperty"/>
        <or:unitTypeFor xml:lang="en">Ultimate tensile strength (UTS), often shortened to tensile strength (TS) or ultimate strength, is the maximum stress that a material can withstand while being stretched or pulled before necking, which is when the specimen&#39;s cross-section starts to significantly contract. Tensile strength is the opposite of compressive strength and the values can be quite different.</or:unitTypeFor>
        <or:termString xml:lang="en">tensile strength</or:termString>
        <rdfs:comment xml:lang="en">ultimate strength</rdfs:comment>
        <or:termString xml:lang="en">ultimate tensile strength</or:termString>
        <or:unitTypeFor rdf:resource="&or;UnitOfPressure"/>
    </owl:NamedIndividual>
    


    <!-- http://www.nist.gov/itl/ssd/Materials#UnitOfAreaPerForce -->

    <owl:NamedIndividual rdf:about="&mat;UnitOfAreaPerForce">
        <rdf:type rdf:resource="&or;InterconvertibleUnitType"/>
    </owl:NamedIndividual>
    


    <!-- http://www.nist.gov/itl/ssd/Materials#UnitOfAreaPerTime -->

    <owl:NamedIndividual rdf:about="&mat;UnitOfAreaPerTime">
        <rdf:type rdf:resource="&or;InterconvertibleUnitType"/>
    </owl:NamedIndividual>
    


    <!-- http://www.nist.gov/itl/ssd/Materials#UnitOfElectricalConductivity -->

    <owl:NamedIndividual rdf:about="&mat;UnitOfElectricalConductivity">
        <rdf:type rdf:resource="&or;InterconvertibleUnitType"/>
    </owl:NamedIndividual>
    


    <!-- http://www.nist.gov/itl/ssd/Materials#UnitOfElectricalResistivity -->

    <owl:NamedIndividual rdf:about="&mat;UnitOfElectricalResistivity">
        <rdf:type rdf:resource="&or;InterconvertibleUnitType"/>
    </owl:NamedIndividual>
    


    <!-- http://www.nist.gov/itl/ssd/Materials#UnitOfEnergyPerAmount -->

    <owl:NamedIndividual rdf:about="&mat;UnitOfEnergyPerAmount">
        <rdf:type rdf:resource="&or;InterconvertibleUnitType"/>
    </owl:NamedIndividual>
    


    <!-- http://www.nist.gov/itl/ssd/Materials#UnitOfEnergyPerMass -->

    <owl:NamedIndividual rdf:about="&mat;UnitOfEnergyPerMass">
        <rdf:type rdf:resource="&or;InterconvertibleUnitType"/>
        <rdfs:comment xml:lang="en">A Unit Of Energy Per Mass is a Unit Of Energy divided by a Unit Of Mass.  E.g., Joules per Gram.</rdfs:comment>
    </owl:NamedIndividual>
    


    <!-- http://www.nist.gov/itl/ssd/Materials#UnitOfEnergyPerTemperatureDifference -->

    <owl:NamedIndividual rdf:about="&mat;UnitOfEnergyPerTemperatureDifference">
        <rdf:type rdf:resource="&or;InterconvertibleUnitType"/>
    </owl:NamedIndividual>
    


    <!-- http://www.nist.gov/itl/ssd/Materials#UnitOfHeatCapacityPerMass -->

    <owl:NamedIndividual rdf:about="&mat;UnitOfHeatCapacityPerMass">
        <rdf:type rdf:resource="&or;InterconvertibleUnitType"/>
    </owl:NamedIndividual>
    


    <!-- http://www.nist.gov/itl/ssd/Materials#UnitOfInverseAreaPerTime -->

    <owl:NamedIndividual rdf:about="&mat;UnitOfInverseAreaPerTime">
        <rdf:type rdf:resource="&or;InterconvertibleUnitType"/>
        <rdfs:comment xml:lang="en">A Unit of Inverse Area per Time has the dimension of 1/ Area / Duration.</rdfs:comment>
    </owl:NamedIndividual>
    


    <!-- http://www.nist.gov/itl/ssd/Materials#UnitOfInverseTemperatureDifference -->

    <owl:NamedIndividual rdf:about="&mat;UnitOfInverseTemperatureDifference">
        <rdf:type rdf:resource="&or;InterconvertibleUnitType"/>
    </owl:NamedIndividual>
    


    <!-- http://www.nist.gov/itl/ssd/Materials#UnitOfInverseTime -->

    <owl:NamedIndividual rdf:about="&mat;UnitOfInverseTime">
        <rdf:type rdf:resource="&or;InterconvertibleUnitType"/>
    </owl:NamedIndividual>
    


    <!-- http://www.nist.gov/itl/ssd/Materials#UnitOfPower -->

    <owl:NamedIndividual rdf:about="&mat;UnitOfPower">
        <rdf:type rdf:resource="&or;InterconvertibleUnitType"/>
    </owl:NamedIndividual>
    


    <!-- http://www.nist.gov/itl/ssd/Materials#UnitOfSpecificHeatCapacity -->

    <owl:NamedIndividual rdf:about="&mat;UnitOfSpecificHeatCapacity">
        <rdf:type rdf:resource="&or;InterconvertibleUnitType"/>
    </owl:NamedIndividual>
    


    <!-- http://www.nist.gov/itl/ssd/Materials#UnitOfTemperatureDifference -->

    <owl:NamedIndividual rdf:about="&mat;UnitOfTemperatureDifference">
        <rdf:type rdf:resource="&or;InterconvertibleUnitType"/>
        <rdfs:comment xml:lang="en">A Unit of Temperature Difference is a Unit of Measure that indicates the differnce in temperature between two things.  A Celsius Degree and a Kelvin Degree have the same magnitude, and thus there is no difference between them as units of Temperature Difference.</rdfs:comment>
    </owl:NamedIndividual>
    


    <!-- http://www.nist.gov/itl/ssd/Materials#UnitOfThermalConductivity -->

    <owl:NamedIndividual rdf:about="&mat;UnitOfThermalConductivity">
        <rdf:type rdf:resource="&or;InterconvertibleUnitType"/>
        <rdfs:comment xml:lang="en">Units Of Thermal Conductivity have the dimension Mass * Distance / (Temperature * Duration^3) .  The SI unit is Watts/(m K).</rdfs:comment>
    </owl:NamedIndividual>
    


    <!-- http://www.nist.gov/itl/ssd/Materials#UnitOfToughness -->

    <owl:NamedIndividual rdf:about="&mat;UnitOfToughness">
        <rdf:type rdf:resource="&or;InterconvertibleUnitType"/>
    </owl:NamedIndividual>
    


    <!-- http://www.nist.gov/itl/ssd/Materials#UnitOfVolumePerMass -->

    <owl:NamedIndividual rdf:about="&mat;UnitOfVolumePerMass">
        <rdf:type rdf:resource="&or;InterconvertibleUnitType"/>
    </owl:NamedIndividual>
    


    <!-- http://www.nist.gov/itl/ssd/Materials#VacancyDiffusionCoefficient -->

    <owl:NamedIndividual rdf:about="&mat;VacancyDiffusionCoefficient">
        <rdf:type rdf:resource="&mat;DiffusionProperty"/>
        <rdfs:seeAlso>Definitions of terms for diffusion in the solid state (IUPAC Recommendations 1999), Pure Appl. Chem. 71, 1307-1325.</rdfs:seeAlso>
        <rdfs:comment xml:lang="en">In the case of diffusion via a vacancy mechanism, the diffusion coefficient associated with the movement of vacancies in the opposite direction to the movement of diffusing species is called the Vacancy Diffusion Coefficient.</rdfs:comment>
        <or:termString xml:lang="en">vacancy diffusion coefficient</or:termString>
    </owl:NamedIndividual>
    


    <!-- http://www.nist.gov/itl/ssd/Materials#VacancyDiffusionMechanism -->

    <owl:NamedIndividual rdf:about="&mat;VacancyDiffusionMechanism">
        <rdf:type rdf:resource="&mat;DiffusionMovementMechanism"/>
        <rdfs:seeAlso xml:lang="en">Definitions of terms for diffusion in the solid state (IUPAC Recommendations 1999), Pure Appl. Chem. 71, 1307-1325.</rdfs:seeAlso>
        <rdfs:comment xml:lang="en">The Vacancy Diffusion Mechanism is a mechanism where diffusion is made possible by the exchange of positions between the diffusing species and a vacancy.</rdfs:comment>
    </owl:NamedIndividual>
    


    <!-- http://www.nist.gov/itl/ssd/Materials#VaporPressure -->

    <owl:NamedIndividual rdf:about="&mat;VaporPressure">
        <rdf:type rdf:resource="&mat;TemperatureDependentProperty"/>
        <or:referenceURL rdf:datatype="&xsd;anyURI">http://www.iupac.org/namespaces/ThermoML</or:referenceURL>
        <rdfs:comment xml:lang="en">The (equilibrium) Vapor Pressure of an object or substance is the pressure exerted by a vapor in thermodynamic equilibrium with its condensed phases (solid or liquid) at a given temperature in a closed system.  This property is dependent upon the material(s) comprising the object or substance and its temperature.  It is not dependent upon the external pressure.</rdfs:comment>
        <or:termString xml:lang="en">sublimation pressure</or:termString>
        <or:termString xml:lang="en">vapor pressure</or:termString>
        <or:termString xml:lang="en">vapour pressure</or:termString>
        <or:unitTypeFor rdf:resource="&or;UnitOfPressure"/>
    </owl:NamedIndividual>
    


    <!-- http://www.nist.gov/itl/ssd/Materials#VickersHardness -->

    <owl:NamedIndividual rdf:about="&mat;VickersHardness">
        <rdf:type rdf:resource="&mat;IndentationHardness"/>
    </owl:NamedIndividual>
    


    <!-- http://www.nist.gov/itl/ssd/Materials#VolumeCompressibility -->

    <owl:NamedIndividual rdf:about="&mat;VolumeCompressibility">
        <rdf:type rdf:resource="&mat;Compressibility"/>
    </owl:NamedIndividual>
    


    <!-- http://www.nist.gov/itl/ssd/Materials#VolumeOfObject -->

    <owl:NamedIndividual rdf:about="&mat;VolumeOfObject">
        <rdf:type rdf:resource="&mat;MeasurableMechanicalProperty"/>
        <or:unitTypeFor rdf:resource="&or;UnitOfVolume"/>
    </owl:NamedIndividual>
    


    <!-- http://www.nist.gov/itl/ssd/Materials#VolumetricExpansionCoefficient -->

    <owl:NamedIndividual rdf:about="&mat;VolumetricExpansionCoefficient">
        <rdf:type rdf:resource="&mat;PressureDependentProperty"/>
        <rdf:type rdf:resource="&mat;TemperatureDependentProperty"/>
        <rdf:type rdf:resource="&mat;ThermalProperty"/>
        <or:termString xml:lang="en">thermal expansion coefficient</or:termString>
        <or:termString xml:lang="en">thermal expansivity</or:termString>
        <or:termString xml:lang="en">volume thermal expansion coefficient</or:termString>
        <or:termString xml:lang="en">volumetric expansion coefficient</or:termString>
        <or:unitTypeFor rdf:resource="&mat;UnitOfInverseTemperatureDifference"/>
    </owl:NamedIndividual>
    


    <!-- http://www.nist.gov/itl/ssd/Materials#Washing -->

    <owl:NamedIndividual rdf:about="&mat;Washing"/>
    


    <!-- http://www.nist.gov/itl/ssd/Materials#Watt -->

    <owl:NamedIndividual rdf:about="&mat;Watt">
        <rdf:type rdf:resource="&mat;UnitOfPower"/>
        <rdf:type rdf:resource="&or;SI_Unit"/>
    </owl:NamedIndividual>
    


    <!-- http://www.nist.gov/itl/ssd/Materials#WattsPerMeterKelvin -->

    <owl:NamedIndividual rdf:about="&mat;WattsPerMeterKelvin">
        <rdf:type rdf:resource="&mat;UnitOfThermalConductivity"/>
        <rdf:type rdf:resource="&or;SI_Unit"/>
    </owl:NamedIndividual>
    


    <!-- http://www.nist.gov/itl/ssd/Materials#WearRateCoefficient -->

    <owl:NamedIndividual rdf:about="&mat;WearRateCoefficient">
        <rdf:type rdf:resource="&mat;MeasurableMechanicalProperty"/>
    </owl:NamedIndividual>
    


    <!-- http://www.nist.gov/itl/ssd/Materials#Welding -->

    <owl:NamedIndividual rdf:about="&mat;Welding"/>
    


    <!-- http://www.nist.gov/itl/ssd/Materials#WroughtAlloy -->

    <owl:NamedIndividual rdf:about="&mat;WroughtAlloy">
        <rdf:type rdf:resource="&mat;AlloyTypeByFormingProcess"/>
        <rdfs:comment xml:lang="en">A Wrought Alloy is one in which soft heated metal is mechanically worked (often by hammering) into shape, possibly after casting.</rdfs:comment>
    </owl:NamedIndividual>
    


    <!-- http://www.nist.gov/itl/ssd/Materials#YieldStrength -->

    <owl:NamedIndividual rdf:about="&mat;YieldStrength">
        <rdf:type rdf:resource="&mat;DeformationProperty"/>
        <rdfs:comment xml:lang="en">The yield strength or yield point of a material is defined as the stress at which a material begins to deform plastically. Below the yield point the material will deform elastically and will return to its original shape when the applied stress is removed. Once the yield point is passed, some fraction of the deformation will be permanent and non-reversible.</rdfs:comment>
        <or:unitTypeFor rdf:resource="&or;UnitOfPressure"/>
    </owl:NamedIndividual>
    


    <!-- http://www.nist.gov/itl/ssd/Materials#ZerothLawOfThermodynamics -->

    <owl:NamedIndividual rdf:about="&mat;ZerothLawOfThermodynamics">
        <rdf:type rdf:resource="&mat;LawOfThermodynamics"/>
        <rdfs:comment xml:lang="en">The Zeroth Law of Thermodynamics states that if two systems are in thermal equilibrium with a third system, they must be in thermal equilibrium with each other.</rdfs:comment>
        <or:termString xml:lang="en">zeroth law of thermodynamics</or:termString>
    </owl:NamedIndividual>
    


    <!-- http://www.nist.gov/itl/ssd/Materials#ZincAlloy -->

    <owl:NamedIndividual rdf:about="&mat;ZincAlloy">
        <rdf:type rdf:resource="&mat;NonFerrousAlloyTypeByMainConstituent"/>
        <or:referenceURL rdf:datatype="&xsd;anyURI">http://www.matweb.com/index.aspx</or:referenceURL>
        <rdfs:comment xml:lang="en">An alloy that contains Zinc but not Iron.</rdfs:comment>
        <bc:primaryConstituentType rdf:resource="&bc;Zinc"/>
    </owl:NamedIndividual>
    


    <!-- http://www.nist.gov/itl/ssd/Materials#ZincOxide -->

    <owl:NamedIndividual rdf:about="&mat;ZincOxide">
        <rdf:type rdf:resource="&bc;ChemicalSubstanceTypeByChemicalSpecies"/>
        <or:termString xml:lang="en">zinc oxide</or:termString>
    </owl:NamedIndividual>
    


    <!-- http://www.nist.gov/itl/ssd/Materials#ZirconiumOxide -->

    <owl:NamedIndividual rdf:about="&mat;ZirconiumOxide">
        <rdf:type rdf:resource="&bc;ChemicalSubstanceTypeByChemicalSpecies"/>
        <or:referenceURL rdf:datatype="&xsd;anyURI">http://www.matweb.com/index.aspx</or:referenceURL>
        <or:termString xml:lang="en">zirconium oxide</or:termString>
    </owl:NamedIndividual>
    


    <!-- http://www.nist.gov/itl/ssd/OntologyRequirements#AvogadrosNumber -->

    <rdf:Description rdf:about="&or;AvogadrosNumber">
        <or:termString xml:lang="en">Avogadro&#39;s number</or:termString>
    </rdf:Description>
    


    <!-- http://www.nist.gov/itl/ssd/OntologyRequirements#ComputerStorageCapacity -->

    <rdf:Description rdf:about="&or;ComputerStorageCapacity">
        <or:unitTypeFor rdf:resource="&or;UnitOfComputerStorageCapacity"/>
    </rdf:Description>
    


    <!-- http://www.nist.gov/itl/ssd/OntologyRequirements#CubicMeter -->

    <rdf:Description rdf:about="&or;CubicMeter">
        <or:termString xml:lang="en">cubic meter</or:termString>
        <or:termString xml:lang="en">cubic metre</or:termString>
    </rdf:Description>
    


    <!-- http://www.nist.gov/itl/ssd/OntologyRequirements#DegreeCelsius -->

    <rdf:Description rdf:about="&or;DegreeCelsius">
        <rdfs:comment xml:lang="en">A Degree Celsius is a Unit of Temperature that specifies an an absolute temperature.-- how many Celsius Degrees the temperature is above (or if negative, below) the freezing point of water.  Adding 273.15 to a temperature specified in Degrees Celsius gives the value of the temperature in Degrees Kelvin.  To refer to temperature differences, use the Unit Of Temperature Difference, Celsius Degree.</rdfs:comment>
    </rdf:Description>
    


    <!-- http://www.nist.gov/itl/ssd/OntologyRequirements#DegreeKelvin -->

    <rdf:Description rdf:about="&or;DegreeKelvin">
        <rdfs:comment xml:lang="en">A Degree Kelvin is a Unit of Temperature that specifies an an absolute temperature.-- how many Celsius Degrees the temperature is above Absolute Zero.  Subtracting 273.15 from a temperature specified in Degrees Kelvin gives the value of the temperature in Degrees Celsius.  To refer to temperature differences, use the Unit Of Temperature Difference, Celsius Degree.</rdfs:comment>
    </rdf:Description>
    


    <!-- http://www.nist.gov/itl/ssd/OntologyRequirements#Femtoliter -->

    <rdf:Description rdf:about="&or;Femtoliter">
        <or:termString xml:lang="en">femtoliter</or:termString>
        <or:termString xml:lang="en">femtolitre</or:termString>
    </rdf:Description>
    


    <!-- http://www.nist.gov/itl/ssd/OntologyRequirements#GramCalorie -->

    <rdf:Description rdf:about="&or;GramCalorie">
        <rdfs:comment xml:lang="en">A Gram-Calorie is the amount of heat needed to raise 1 Gram of water 1 Degree Celsius at 1 Atmosphere Pressure.</rdfs:comment>
        <or:termString xml:lang="en">cal.</or:termString>
        <or:termString xml:lang="en">calorie</or:termString>
        <or:termString xml:lang="en">gram-calorie</or:termString>
    </rdf:Description>
    


    <!-- http://www.nist.gov/itl/ssd/OntologyRequirements#Kilocalorie -->

    <rdf:Description rdf:about="&or;Kilocalorie">
        <rdfs:comment xml:lang="en">A Kilocalorie is the amount of heat needed to raise 1 Kilogram of water 1 DegreeCelsius at 1 Atmosphere-UnitOfPressure.  It is equal to 1000 gram-calories.  In the US, the kilocalorie is called a `calorie&#39; when refering to the energy content of foodstuffs.  The abbreviation, `Cal.&#39;, for kilocalorie is capitalized while that of a gram-calorie, `cal.&#39; is lower case.</rdfs:comment>
        <or:termString xml:lang="en">Cal.</or:termString>
        <or:termString xml:lang="en">Calorie</or:termString>
        <or:termString xml:lang="en">kilocalorie</or:termString>
    </rdf:Description>
    


    <!-- http://www.nist.gov/itl/ssd/OntologyRequirements#Liter -->

    <rdf:Description rdf:about="&or;Liter">
        <or:termString xml:lang="en">cubic decimeter</or:termString>
        <or:termString xml:lang="en">dm^3</or:termString>
        <or:termString xml:lang="en">l</or:termString>
        <or:termString xml:lang="en">liter</or:termString>
        <or:termString xml:lang="en">litre</or:termString>
    </rdf:Description>
    


    <!-- http://www.nist.gov/itl/ssd/OntologyRequirements#Microliter -->

    <rdf:Description rdf:about="&or;Microliter">
        <or:termString xml:lang="en">cubic millimeter</or:termString>
        <or:termString xml:lang="en">microliter</or:termString>
        <or:termString xml:lang="en">microlitre</or:termString>
        <or:termString xml:lang="en">mm^3</or:termString>
    </rdf:Description>
    


    <!-- http://www.nist.gov/itl/ssd/OntologyRequirements#Milliliter -->

    <rdf:Description rdf:about="&or;Milliliter">
        <or:termString xml:lang="en">cc</or:termString>
        <or:termString xml:lang="en">cubic centimeter</or:termString>
        <or:termString xml:lang="en">cubic centimetre</or:termString>
        <or:termString xml:lang="en">milliliter</or:termString>
        <or:termString xml:lang="en">millilitre</or:termString>
        <or:termString xml:lang="en">ml</or:termString>
    </rdf:Description>
    


    <!-- http://www.nist.gov/itl/ssd/OntologyRequirements#Nanoliter -->

    <rdf:Description rdf:about="&or;Nanoliter">
        <or:termString xml:lang="en">nanoliter</or:termString>
        <or:termString xml:lang="en">nanolitre</or:termString>
        <or:termString xml:lang="en">nl</or:termString>
    </rdf:Description>
    


    <!-- http://www.nist.gov/itl/ssd/OntologyRequirements#UnitOfTemperature -->

    <rdf:Description rdf:about="&or;UnitOfTemperature">
        <rdfs:comment xml:lang="en">A Unit of Temperature is a Unit of Measure used for specifying the temperature of something.  Two different Units of Temperatures may have the same magnitude, but different offsets, so are not the same.  A Degree Celsius is different from a Degree Kelvin, for example since 100 C = 373.15 K.</rdfs:comment>
    </rdf:Description>
    


    <!-- http://www.nist.gov/itl/ssd/OntologyRequirements#Volt -->

    <rdf:Description rdf:about="&or;Volt">
        <or:termString xml:lang="en">joules per coulomb</or:termString>
        <or:termString xml:lang="en">volt</or:termString>
    </rdf:Description>
    


    <!-- 
    ///////////////////////////////////////////////////////////////////////////////////////
    //
    // Annotations
    //
    ///////////////////////////////////////////////////////////////////////////////////////
     -->

    <rdf:Description rdf:about="&or;Gram">
        <rdfs:comment xml:lang="en">g</rdfs:comment>
        <rdfs:comment xml:lang="en">gram</rdfs:comment>
        <rdfs:comment xml:lang="en">gramme</rdfs:comment>
    </rdf:Description>
    <rdf:Description rdf:about="&or;Pascal-UnitOfPressure">
        <or:termString xml:lang="en">pascal</or:termString>
    </rdf:Description>
    <rdf:Description rdf:about="&or;Nanometer">
        <or:termString xml:lang="en">nanometer</or:termString>
        <or:termString xml:lang="en">nanometre</or:termString>
    </rdf:Description>
    <rdf:Description rdf:about="&or;Meter">
        <or:termString xml:lang="en">meter</or:termString>
        <or:termString xml:lang="en">metre</or:termString>
    </rdf:Description>
    <rdf:Description rdf:about="&or;Centimeter">
        <or:termString xml:lang="en">centimeter</or:termString>
        <or:termString xml:lang="en">centimetre</or:termString>
    </rdf:Description>
    <rdf:Description rdf:about="&or;ElectronVolt">
        <or:termString xml:lang="en">electron volt</or:termString>
        <or:termString xml:lang="en">ev</or:termString>
    </rdf:Description>
    <rdf:Description rdf:about="&bc;hasChemicalFormula">
        <or:referenceURL rdf:datatype="&xsd;anyURI">http://www.iupac.org/namespaces/ThermoML#sFormulaMolec</or:referenceURL>
    </rdf:Description>
    <rdf:Description rdf:about="&or;MmHg">
        <or:termString xml:lang="en">millimeter of mercury</or:termString>
        <or:termString xml:lang="en">mm Hg</or:termString>
        <or:termString xml:lang="en">torr</or:termString>
    </rdf:Description>
    <rdf:Description rdf:about="&or;DegreeFahrenheit">
        <rdfs:comment xml:lang="en">A Degree Fahrenheit is a Unit of Temperature that specifies an an absolute temperature.-- how many Fahrenheit Degrees the temperature is above (or if negative, below) 32 Fahrenheit Degrees below the freezing point of water.  To refer to temperature differences, use the Unit Of Temperature Difference, Fahrenheit Degree.</rdfs:comment>
    </rdf:Description>
    <rdf:Description rdf:about="&or;Millimeter">
        <or:termString xml:lang="en">millimeter</or:termString>
        <or:termString xml:lang="en">millimetre</or:termString>
    </rdf:Description>
    <rdf:Description rdf:about="&bc;OrganicMaterial">
        <or:referenceURL rdf:datatype="&xsd;anyURI">http://www.iupac.org/namespaces/ThermoML#biomaterial</or:referenceURL>
    </rdf:Description>
    <rdf:Description rdf:about="&or;Bar-UnitOfPressure">
        <or:termString xml:lang="en">10^5 Pascals</or:termString>
        <or:termString xml:lang="en">Pa*10^5</or:termString>
        <or:termString xml:lang="en">bar</or:termString>
    </rdf:Description>
    <rdf:Description rdf:about="&or;Kilogram">
        <rdfs:comment xml:lang="en">kg</rdfs:comment>
        <rdfs:comment xml:lang="en">kilo</rdfs:comment>
        <rdfs:comment xml:lang="en">kilogram</rdfs:comment>
        <rdfs:comment xml:lang="en">kilogramme</rdfs:comment>
    </rdf:Description>
    <rdf:Description rdf:about="&or;catalogNumber">
        <skos:note xml:lang="en">Something can have different catalog numbers in different catalogs.  To be functional, a ternary relation that specifies the catalog is needed.  Specializations of this relation (XCatalogNumber) can be functional.</skos:note>
    </rdf:Description>
    <rdf:Description rdf:about="&or;BritishThermalUnit">
        <or:termString xml:lang="en">BTU</or:termString>
        <or:termString xml:lang="en">British thermal unit</or:termString>
    </rdf:Description>
    <rdf:Description rdf:about="&or;PSI">
        <or:termString xml:lang="en">PSI</or:termString>
    </rdf:Description>
    <rdf:Description rdf:about="&bc;atomicMass">
        <or:referenceURL rdf:datatype="&xsd;anyURI">http://www.iupac.org/namespaces/ThermoML#nNumberAvgMolMas</or:referenceURL>
    </rdf:Description>
    


    <!-- 
    ///////////////////////////////////////////////////////////////////////////////////////
    //
    // General axioms
    //
    ///////////////////////////////////////////////////////////////////////////////////////
     -->

    <rdf:Description>
        <rdf:type rdf:resource="&owl;AllDifferent"/>
        <owl:distinctMembers rdf:parseType="Collection">
            <rdf:Description rdf:about="&or;Femtoliter"/>
            <rdf:Description rdf:about="&or;Liter"/>
        </owl:distinctMembers>
    </rdf:Description>
    <rdf:Description>
        <rdf:type rdf:resource="&owl;AllDifferent"/>
        <owl:distinctMembers rdf:parseType="Collection">
            <rdf:Description rdf:about="&mat;Dyne"/>
            <rdf:Description rdf:about="&mat;ShortTon"/>
        </owl:distinctMembers>
    </rdf:Description>
    <rdf:Description>
        <rdf:type rdf:resource="&owl;AllDifferent"/>
        <owl:distinctMembers rdf:parseType="Collection">
            <rdf:Description rdf:about="&bc;CcsPerLiter"/>
            <rdf:Description rdf:about="&bc;PercentByWeight"/>
        </owl:distinctMembers>
    </rdf:Description>
    <rdf:Description>
        <rdf:type rdf:resource="&owl;AllDifferent"/>
        <owl:distinctMembers rdf:parseType="Collection">
            <rdf:Description rdf:about="&bc;CcsPerLiter"/>
            <rdf:Description rdf:about="&or;AvogadrosNumber"/>
        </owl:distinctMembers>
    </rdf:Description>
    <rdf:Description>
        <rdf:type rdf:resource="&owl;AllDifferent"/>
        <owl:distinctMembers rdf:parseType="Collection">
            <rdf:Description rdf:about="&or;Femtoliter"/>
            <rdf:Description rdf:about="&or;Milliliter"/>
        </owl:distinctMembers>
    </rdf:Description>
    <rdf:Description>
        <rdf:type rdf:resource="&owl;AllDifferent"/>
        <owl:distinctMembers rdf:parseType="Collection">
            <rdf:Description rdf:about="&or;CubicMeter"/>
            <rdf:Description rdf:about="&or;Milliliter"/>
        </owl:distinctMembers>
    </rdf:Description>
    <rdf:Description>
        <rdf:type rdf:resource="&owl;AllDifferent"/>
        <owl:distinctMembers rdf:parseType="Collection">
            <rdf:Description rdf:about="&mat;CubicInch"/>
            <rdf:Description rdf:about="&or;Microliter"/>
        </owl:distinctMembers>
    </rdf:Description>
    <rdf:Description>
        <rdf:type rdf:resource="&owl;AllDifferent"/>
        <owl:distinctMembers rdf:parseType="Collection">
            <rdf:Description rdf:about="&mat;JoulePerKelvin"/>
            <rdf:Description rdf:about="&mat;KilocaloriePerKelvin"/>
        </owl:distinctMembers>
    </rdf:Description>
    <rdf:Description>
        <rdf:type rdf:resource="&owl;AllDifferent"/>
        <owl:distinctMembers rdf:parseType="Collection">
            <rdf:Description rdf:about="&mat;LongTon"/>
            <rdf:Description rdf:about="&mat;PoundForce"/>
        </owl:distinctMembers>
    </rdf:Description>
    <rdf:Description>
        <rdf:type rdf:resource="&owl;AllDifferent"/>
        <owl:distinctMembers rdf:parseType="Collection">
            <rdf:Description rdf:about="&or;CubicMeter"/>
            <rdf:Description rdf:about="&or;Femtoliter"/>
        </owl:distinctMembers>
    </rdf:Description>
    <rdf:Description>
        <rdf:type rdf:resource="&owl;AllDifferent"/>
        <owl:distinctMembers rdf:parseType="Collection">
            <rdf:Description rdf:about="&mat;Opaque"/>
            <rdf:Description rdf:about="&mat;Translucent"/>
        </owl:distinctMembers>
    </rdf:Description>
    <rdf:Description>
        <rdf:type rdf:resource="&owl;AllDifferent"/>
        <owl:distinctMembers rdf:parseType="Collection">
            <rdf:Description rdf:about="&mat;Dyne"/>
            <rdf:Description rdf:about="&or;Newton"/>
        </owl:distinctMembers>
    </rdf:Description>
    <rdf:Description>
        <rdf:type rdf:resource="&owl;AllDifferent"/>
        <owl:distinctMembers rdf:parseType="Collection">
            <rdf:Description rdf:about="&bc;PercentByWeight"/>
            <rdf:Description rdf:about="&mat;MassFraction"/>
        </owl:distinctMembers>
    </rdf:Description>
    <rdf:Description>
        <rdf:type rdf:resource="&owl;AllDifferent"/>
        <owl:distinctMembers rdf:parseType="Collection">
            <rdf:Description rdf:about="&mat;LongTon"/>
            <rdf:Description rdf:about="&or;Newton"/>
        </owl:distinctMembers>
    </rdf:Description>
    <rdf:Description>
        <rdf:type rdf:resource="&owl;AllDifferent"/>
        <owl:distinctMembers rdf:parseType="Collection">
            <rdf:Description rdf:about="&mat;CubicInch"/>
            <rdf:Description rdf:about="&or;Nanoliter"/>
        </owl:distinctMembers>
    </rdf:Description>
    <rdf:Description>
        <rdf:type rdf:resource="&owl;AllDifferent"/>
        <owl:distinctMembers rdf:parseType="Collection">
            <rdf:Description rdf:about="&or;Liter"/>
            <rdf:Description rdf:about="&or;Nanoliter"/>
        </owl:distinctMembers>
    </rdf:Description>
    <rdf:Description>
        <rdf:type rdf:resource="&owl;AllDifferent"/>
        <owl:distinctMembers rdf:parseType="Collection">
            <rdf:Description rdf:about="&or;Microliter"/>
            <rdf:Description rdf:about="&or;Nanoliter"/>
        </owl:distinctMembers>
    </rdf:Description>
    <rdf:Description>
        <rdf:type rdf:resource="&owl;AllDifferent"/>
        <owl:distinctMembers rdf:parseType="Collection">
            <rdf:Description rdf:about="&mat;ShortTon"/>
            <rdf:Description rdf:about="&or;Newton"/>
        </owl:distinctMembers>
    </rdf:Description>
    <rdf:Description>
        <rdf:type rdf:resource="&owl;AllDifferent"/>
        <owl:distinctMembers rdf:parseType="Collection">
            <rdf:Description rdf:about="&or;CubicMeter"/>
            <rdf:Description rdf:about="&or;Liter"/>
        </owl:distinctMembers>
    </rdf:Description>
    <rdf:Description>
        <rdf:type rdf:resource="&owl;AllDifferent"/>
        <owl:distinctMembers rdf:parseType="Collection">
            <rdf:Description rdf:about="&mat;CubicInch"/>
            <rdf:Description rdf:about="&or;Milliliter"/>
        </owl:distinctMembers>
    </rdf:Description>
    <rdf:Description>
        <rdf:type rdf:resource="&owl;AllDifferent"/>
        <owl:distinctMembers rdf:parseType="Collection">
            <rdf:Description rdf:about="&mat;CaloriePerGramKelvin"/>
            <rdf:Description rdf:about="&mat;JoulePerKgK"/>
        </owl:distinctMembers>
    </rdf:Description>
    <rdf:Description>
        <rdf:type rdf:resource="&owl;AllDifferent"/>
        <owl:distinctMembers rdf:parseType="Collection">
            <rdf:Description rdf:about="&bc;GramsPerLiter"/>
            <rdf:Description rdf:about="&mat;KgPerM3"/>
        </owl:distinctMembers>
    </rdf:Description>
    <rdf:Description>
        <rdf:type rdf:resource="&owl;AllDifferent"/>
        <owl:distinctMembers rdf:parseType="Collection">
            <rdf:Description rdf:about="&mat;CubicInch"/>
            <rdf:Description rdf:about="&or;CubicMeter"/>
        </owl:distinctMembers>
    </rdf:Description>
    <rdf:Description>
        <rdf:type rdf:resource="&owl;AllDifferent"/>
        <owl:distinctMembers rdf:parseType="Collection">
            <rdf:Description rdf:about="&mat;CelsiusDegree"/>
            <rdf:Description rdf:about="&mat;FahrenheitDegree"/>
            <rdf:Description rdf:about="&or;DegreeCelsius"/>
            <rdf:Description rdf:about="&or;DegreeKelvin"/>
        </owl:distinctMembers>
    </rdf:Description>
    <rdf:Description>
        <rdf:type rdf:resource="&owl;AllDifferent"/>
        <owl:distinctMembers rdf:parseType="Collection">
            <rdf:Description rdf:about="&mat;Opaque"/>
            <rdf:Description rdf:about="&mat;Transparent"/>
        </owl:distinctMembers>
    </rdf:Description>
    <rdf:Description>
        <rdf:type rdf:resource="&owl;AllDifferent"/>
        <owl:distinctMembers rdf:parseType="Collection">
            <rdf:Description rdf:about="&bc;CcsPerLiter"/>
            <rdf:Description rdf:about="&mat;Mole_Unit"/>
        </owl:distinctMembers>
    </rdf:Description>
    <rdf:Description>
        <rdf:type rdf:resource="&owl;AllDifferent"/>
        <owl:distinctMembers rdf:parseType="Collection">
            <rdf:Description rdf:about="&mat;Translucent"/>
            <rdf:Description rdf:about="&mat;Transparent"/>
        </owl:distinctMembers>
    </rdf:Description>
    <rdf:Description>
        <rdf:type rdf:resource="&owl;AllDifferent"/>
        <owl:distinctMembers rdf:parseType="Collection">
            <rdf:Description rdf:about="&or;CubicMeter"/>
            <rdf:Description rdf:about="&or;Microliter"/>
        </owl:distinctMembers>
    </rdf:Description>
    <rdf:Description>
        <rdf:type rdf:resource="&owl;AllDifferent"/>
        <owl:distinctMembers rdf:parseType="Collection">
            <rdf:Description rdf:about="&mat;LongTon"/>
            <rdf:Description rdf:about="&mat;ShortTon"/>
        </owl:distinctMembers>
    </rdf:Description>
    <rdf:Description>
        <rdf:type rdf:resource="&owl;AllDifferent"/>
        <owl:distinctMembers rdf:parseType="Collection">
            <rdf:Description rdf:about="&mat;Dyne"/>
            <rdf:Description rdf:about="&mat;PoundForce"/>
        </owl:distinctMembers>
    </rdf:Description>
    <rdf:Description>
        <rdf:type rdf:resource="&owl;AllDifferent"/>
        <owl:distinctMembers rdf:parseType="Collection">
            <rdf:Description rdf:about="&bc;GramsPerLiter"/>
            <rdf:Description rdf:about="&mat;MoleFraction"/>
        </owl:distinctMembers>
    </rdf:Description>
    <rdf:Description>
        <rdf:type rdf:resource="&owl;AllDifferent"/>
        <owl:distinctMembers rdf:parseType="Collection">
            <rdf:Description rdf:about="&bc;CcsPerLiter"/>
            <rdf:Description rdf:about="&or;Percent"/>
        </owl:distinctMembers>
    </rdf:Description>
    <rdf:Description>
        <rdf:type rdf:resource="&owl;AllDifferent"/>
        <owl:distinctMembers rdf:parseType="Collection">
            <rdf:Description rdf:about="&mat;CubicInch"/>
            <rdf:Description rdf:about="&or;Femtoliter"/>
        </owl:distinctMembers>
    </rdf:Description>
    <rdf:Description>
        <rdf:type rdf:resource="&owl;AllDifferent"/>
        <owl:distinctMembers rdf:parseType="Collection">
            <rdf:Description rdf:about="&or;Microliter"/>
            <rdf:Description rdf:about="&or;Milliliter"/>
        </owl:distinctMembers>
    </rdf:Description>
    <rdf:Description>
        <rdf:type rdf:resource="&owl;AllDifferent"/>
        <owl:distinctMembers rdf:parseType="Collection">
            <rdf:Description rdf:about="&or;Liter"/>
            <rdf:Description rdf:about="&or;Microliter"/>
        </owl:distinctMembers>
    </rdf:Description>
    <rdf:Description>
        <rdf:type rdf:resource="&owl;AllDifferent"/>
        <owl:distinctMembers rdf:parseType="Collection">
            <rdf:Description rdf:about="&bc;CcsPerLiter"/>
            <rdf:Description rdf:about="&bc;PercentByVolume"/>
        </owl:distinctMembers>
    </rdf:Description>
    <rdf:Description>
        <rdf:type rdf:resource="&owl;AllDifferent"/>
        <owl:distinctMembers rdf:parseType="Collection">
            <rdf:Description rdf:about="&or;Femtoliter"/>
            <rdf:Description rdf:about="&or;Nanoliter"/>
        </owl:distinctMembers>
    </rdf:Description>
    <rdf:Description>
        <rdf:type rdf:resource="&owl;AllDifferent"/>
        <owl:distinctMembers rdf:parseType="Collection">
            <rdf:Description rdf:about="&or;Liter"/>
            <rdf:Description rdf:about="&or;Milliliter"/>
        </owl:distinctMembers>
    </rdf:Description>
    <rdf:Description>
        <rdf:type rdf:resource="&owl;AllDifferent"/>
        <owl:distinctMembers rdf:parseType="Collection">
            <rdf:Description rdf:about="&mat;CubicInch"/>
            <rdf:Description rdf:about="&or;Liter"/>
        </owl:distinctMembers>
    </rdf:Description>
    <rdf:Description>
        <rdf:type rdf:resource="&owl;AllDifferent"/>
        <owl:distinctMembers rdf:parseType="Collection">
            <rdf:Description rdf:about="&or;GramCalorie"/>
            <rdf:Description rdf:about="&or;Kilocalorie"/>
        </owl:distinctMembers>
    </rdf:Description>
    <rdf:Description>
        <rdf:type rdf:resource="&owl;AllDifferent"/>
        <owl:distinctMembers rdf:parseType="Collection">
            <rdf:Description rdf:about="&or;CubicMeter"/>
            <rdf:Description rdf:about="&or;Nanoliter"/>
        </owl:distinctMembers>
    </rdf:Description>
    <rdf:Description>
        <rdf:type rdf:resource="&owl;AllDifferent"/>
        <owl:distinctMembers rdf:parseType="Collection">
            <rdf:Description rdf:about="&or;Milliliter"/>
            <rdf:Description rdf:about="&or;Nanoliter"/>
        </owl:distinctMembers>
    </rdf:Description>
    <rdf:Description>
        <rdf:type rdf:resource="&owl;AllDifferent"/>
        <owl:distinctMembers rdf:parseType="Collection">
            <rdf:Description rdf:about="&mat;PoundForce"/>
            <rdf:Description rdf:about="&mat;ShortTon"/>
        </owl:distinctMembers>
    </rdf:Description>
    <rdf:Description>
        <rdf:type rdf:resource="&owl;AllDifferent"/>
        <owl:distinctMembers rdf:parseType="Collection">
            <rdf:Description rdf:about="&mat;MoleFraction"/>
            <rdf:Description rdf:about="&mat;MolePercent"/>
        </owl:distinctMembers>
    </rdf:Description>
    <rdf:Description>
        <rdf:type rdf:resource="&owl;AllDifferent"/>
        <owl:distinctMembers rdf:parseType="Collection">
            <rdf:Description rdf:about="&mat;PoundForce"/>
            <rdf:Description rdf:about="&or;Newton"/>
        </owl:distinctMembers>
    </rdf:Description>
    <rdf:Description>
        <rdf:type rdf:resource="&owl;AllDifferent"/>
        <owl:distinctMembers rdf:parseType="Collection">
            <rdf:Description rdf:about="&mat;Dyne"/>
            <rdf:Description rdf:about="&mat;LongTon"/>
        </owl:distinctMembers>
    </rdf:Description>
    <rdf:Description>
        <rdf:type rdf:resource="&owl;AllDifferent"/>
        <owl:distinctMembers rdf:parseType="Collection">
            <rdf:Description rdf:about="&or;Femtoliter"/>
            <rdf:Description rdf:about="&or;Microliter"/>
        </owl:distinctMembers>
    </rdf:Description>
    <rdf:Description>
        <rdf:type rdf:resource="&owl;AllDifferent"/>
        <owl:distinctMembers rdf:parseType="Collection">
            <rdf:Description rdf:about="&bc;GramsPerLiter"/>
            <rdf:Description rdf:about="&mat;MolePercent"/>
        </owl:distinctMembers>
    </rdf:Description>
</rdf:RDF>



<!-- Generated by the OWL API (version 3.2.3.1824) http://owlapi.sourceforge.net -->

