<?xml version="1.0"?>


<!DOCTYPE rdf:RDF [
    <!ENTITY terms "http://purl.org/dc/terms/" >
    <!ENTITY owl "http://www.w3.org/2002/07/owl#" >
    <!ENTITY dc "http://purl.org/dc/elements/1.1/" >
    <!ENTITY xsd "http://www.w3.org/2001/XMLSchema#" >
    <!ENTITY skos "http://www.w3.org/2004/02/skos/core#" >
    <!ENTITY XMLSchema "http://www.w3.org/2000/10/XMLSchema#" >
    <!ENTITY oil "http://www.daml.org/2001/03/daml+oil#" >
    <!ENTITY rdfs "http://www.w3.org/2000/01/rdf-schema#" >
    <!ENTITY ont "http://www.co-ode.org/ontologies/ont.owl#" >
    <!ENTITY rdf "http://www.w3.org/1999/02/22-rdf-syntax-ns#" >
    <!ENTITY or "http://www.nist.gov/itl/ssd/OntologyRequirements#" >
]>


<rdf:RDF xmlns="http://www.nist.gov/itl/ssd/OntologyRequirements#"
     xml:base="http://www.nist.gov/itl/ssd/OntologyRequirements"
     xmlns:dc="http://purl.org/dc/elements/1.1/"
     xmlns:rdfs="http://www.w3.org/2000/01/rdf-schema#"
     xmlns:ont="http://www.co-ode.org/ontologies/ont.owl#"
     xmlns:or="http://www.nist.gov/itl/ssd/OntologyRequirements#"
     xmlns:terms="http://purl.org/dc/terms/"
     xmlns:owl="http://www.w3.org/2002/07/owl#"
     xmlns:xsd="http://www.w3.org/2001/XMLSchema#"
     xmlns:rdf="http://www.w3.org/1999/02/22-rdf-syntax-ns#"
     xmlns:XMLSchema="http://www.w3.org/2000/10/XMLSchema#"
     xmlns:skos="http://www.w3.org/2004/02/skos/core#"
     xmlns:oil="http://www.daml.org/2001/03/daml+oil#">
    <owl:Ontology rdf:about="http://www.nist.gov/itl/ssd/OntologyRequirements">
        <dc:date>12 October 2012</dc:date>
        <ont:creator>doug foxvog</ont:creator>
        <terms:title>Ontology Requirements Ontology</terms:title>
        <owl:imports rdf:resource="http://www.daml.org/2001/03/daml+oil"/>
    </owl:Ontology>
    


    <!-- 
    ///////////////////////////////////////////////////////////////////////////////////////
    //
    // Annotation properties
    //
    ///////////////////////////////////////////////////////////////////////////////////////
     -->

    <owl:AnnotationProperty rdf:about="&terms;description"/>
    <owl:AnnotationProperty rdf:about="&or;referenceURL">
        <rdfs:comment xml:lang="en">The property ``referenceURL&#39;  specifies a URI that provides reference for the term with this property.</rdfs:comment>
        <rdfs:range rdf:resource="&xsd;url"/>
    </owl:AnnotationProperty>
    <owl:AnnotationProperty rdf:about="&terms;hasVersion"/>
    <owl:AnnotationProperty rdf:about="&terms;publisher"/>
    <owl:AnnotationProperty rdf:about="&terms;modified"/>
    <owl:AnnotationProperty rdf:about="&skos;note"/>
    <owl:AnnotationProperty rdf:about="&terms;issued"/>
    <owl:AnnotationProperty rdf:about="&or;termString">
        <rdfs:comment xml:lang="en">The property &#39;termString&#39; gives a text string for a term.</rdfs:comment>
        <rdfs:range rdf:resource="&xsd;string"/>
    </owl:AnnotationProperty>
    <rdf:Description rdf:about="&dc;date">
        <rdfs:label xml:lang="en-us">Date</rdfs:label>
        <terms:issued>1999-07-02</terms:issued>
        <terms:modified>2008-01-14</terms:modified>
        <rdfs:comment xml:lang="en-us">A point or period of time associated with an event in the lifecycle of the resource.</rdfs:comment>
        <skos:note xml:lang="en-us">A second property with the same name as this property has been declared in the dcterms: namespace (http://purl.org/dc/terms/).  See the Introduction to the document &#39;DCMI Metadata Terms&#39; (http://dublincore.org/documents/dcmi-terms/) for an explanation.</skos:note>
        <terms:description xml:lang="en-us">Date may be used to express temporal information at any level of granularity.  Recommended best practice is to use an encoding scheme, such as the W3CDTF profile of ISO 8601 [W3CDTF].</terms:description>
        <terms:hasVersion rdf:resource="http://dublincore.org/usage/terms/history/#date-006"/>
        <rdfs:isDefinedBy rdf:resource="http://purl.org/dc/elements/1.1/"/>
    </rdf:Description>
    <owl:AnnotationProperty rdf:about="&terms;title"/>
    


    <!-- 
    ///////////////////////////////////////////////////////////////////////////////////////
    //
    // Datatypes
    //
    ///////////////////////////////////////////////////////////////////////////////////////
     -->

    


    <!-- 
    ///////////////////////////////////////////////////////////////////////////////////////
    //
    // Object Properties
    //
    ///////////////////////////////////////////////////////////////////////////////////////
     -->

    


    <!-- http://www.nist.gov/itl/ssd/OntologyRequirements#associatedInstitution -->

    <owl:ObjectProperty rdf:about="&or;associatedInstitution">
        <rdfs:comment xml:lang="en">An institution that a person is affiliated with.</rdfs:comment>
        <rdfs:domain rdf:resource="&or;Human"/>
        <rdfs:range rdf:resource="&or;Organization"/>
    </owl:ObjectProperty>
    


    <!-- http://www.nist.gov/itl/ssd/OntologyRequirements#dateOfEvent -->

    <owl:ObjectProperty rdf:about="&or;dateOfEvent">
        <rdfs:comment xml:lang="en">The property ``date Of Event&#39; &#39;is a specialization of both ``starts At&#39; &#39; and ``ends At&#39; &#39;. dateOfEvent relates an Event to a Date-Time on or in which it both started and ended.  The same event can be held to have different`Date-Times as `&#39;date Of Event&#39; &#39; when one time is more specific than another.  For example, the statement that dates a cell division to 9:23 on May 8, 2018, does not conflict with a statement that dates the same cell division to May 8, 2018.

Same as cyc:dateOfEvent.</rdfs:comment>
        <rdfs:range rdf:resource="&or;DateTime"/>
        <rdfs:domain rdf:resource="&or;Event"/>
        <rdfs:subPropertyOf rdf:resource="&or;endsAt"/>
        <rdfs:subPropertyOf rdf:resource="&or;startsAt"/>
    </owl:ObjectProperty>
    


    <!-- http://www.nist.gov/itl/ssd/OntologyRequirements#doneBy -->

    <owl:ObjectProperty rdf:about="&or;doneBy">
        <rdfs:comment xml:lang="en">If an Event is &#39;doer&#39; DOER, that means that some activity on the part of DOER causes or carries out EVENT, whether DOER does EVENT intentionally or not. DOER need not even be animate; e.g. the vocanic eruption that buried Pompeii was doneBy Mt. Vesuvius.  An event might have more than one doer; consider a chess game. </rdfs:comment>
        <oil:equivalentTo xml:lang="en">cyc#doneBy</oil:equivalentTo>
        <rdfs:domain rdf:resource="&or;Event"/>
        <rdfs:range rdf:resource="&or;TemporalThing"/>
    </owl:ObjectProperty>
    


    <!-- http://www.nist.gov/itl/ssd/OntologyRequirements#endsAt -->

    <owl:ObjectProperty rdf:about="&or;endsAt">
        <rdfs:comment xml:lang="en">The property ``ends At&#39; &#39; specifies the Date Time at which a given temporal thing ceases to happen or exist.  The same event (or object) can be held to ``end At&#39; &#39; different Date Times when one starting time is more specific than another.  For example, the statement that a cell division ends At 9:23 on May 8, 2018, does not conflict with a statement that the same cell division starts At 9:23:56 on May 8, 2018.

Same as cyc:endingDate.</rdfs:comment>
        <rdfs:range rdf:resource="&or;DateTime"/>
        <rdfs:domain rdf:resource="&or;TemporalThing"/>
    </owl:ObjectProperty>
    


    <!-- http://www.nist.gov/itl/ssd/OntologyRequirements#eventInSeries -->

    <owl:ObjectProperty rdf:about="&or;eventInSeries">
        <rdfs:comment xml:lang="en">The property ``eventInSeries&#39;&#39; relates an event to an event series of which it is a member.  For example, an inning in a baseball game, a presentation in a conference session, and a conference in a conference series.</rdfs:comment>
        <rdfs:domain rdf:resource="&or;Event"/>
        <rdfs:range rdf:resource="&or;EventSeries"/>
        <rdfs:subPropertyOf rdf:resource="&or;subEventOf"/>
    </owl:ObjectProperty>
    


    <!-- http://www.nist.gov/itl/ssd/OntologyRequirements#expressedAsValue -->

    <owl:ObjectProperty rdf:about="&or;expressedAsValue">
        <rdf:type rdf:resource="&owl;InverseFunctionalProperty"/>
        <rdfs:comment xml:lang="en">A given Measurable Quantity may be expressed using different units of measure.  Each such expression is deemed an &#39;Expressed Quantity&#39;. 

For example, a Volume or 1500 cc&#39;s, expressed as 1.5 Liters, has Liter as its expressed Unit Of Measure and 1.5 as its expressed Value.  The same Volume  expressed in Millileters has the expressed Unit Of Measure and 1500 as the expressed Value.  

The same Quantity has represenations as two different Expressed Quantities in this case.</rdfs:comment>
        <rdfs:range rdf:resource="&or;ExpressedQuantity"/>
        <rdfs:domain rdf:resource="&or;MeasurableQuantity"/>
    </owl:ObjectProperty>
    


    <!-- http://www.nist.gov/itl/ssd/OntologyRequirements#expressedUnit -->

    <owl:ObjectProperty rdf:about="&or;expressedUnit">
        <rdf:type rdf:resource="&owl;FunctionalProperty"/>
        <rdfs:comment xml:lang="en">The unit of measure in which a quantity is expressed.  

For example, a Volume expressed as 1.5 Liters has Liter as its expressed Unit Of Measure and 1.5 as its expressed Value.  The same volume may also be expressed as a different Expressed Quantity: with Millileter as the expressed Unit Of Measure and 1500 as the expressed Value.  

The same Quantity has represenations as two different Expressed Quantities in this case.</rdfs:comment>
        <rdfs:domain rdf:resource="&or;ExpressedQuantity"/>
        <rdfs:range rdf:resource="&or;UnitOfMeasure"/>
    </owl:ObjectProperty>
    


    <!-- http://www.nist.gov/itl/ssd/OntologyRequirements#extendsFormat -->

    <owl:ObjectProperty rdf:about="&or;extendsFormat">
        <rdf:type rdf:resource="&owl;AsymmetricProperty"/>
        <rdf:type rdf:resource="&owl;IrreflexiveProperty"/>
        <rdf:type rdf:resource="&owl;TransitiveProperty"/>
        <rdfs:comment xml:lang="en">The property &#39;extends Format&#39; means that the first Data Format listed includes and expands upon the second Data Format.</rdfs:comment>
        <rdfs:range rdf:resource="&or;DataFormat"/>
        <rdfs:domain rdf:resource="&or;DataFormat"/>
    </owl:ObjectProperty>
    


    <!-- http://www.nist.gov/itl/ssd/OntologyRequirements#firstImageInSequence -->

    <owl:ObjectProperty rdf:about="&or;firstImageInSequence">
        <rdf:type rdf:resource="&owl;InverseFunctionalProperty"/>
        <skos:note xml:lang="en">Maybe a more generic property -- firstItemSequence -- should be substituted for this more specific one.</skos:note>
        <rdfs:comment xml:lang="en">Specifies the first Image in an Image Sequence.</rdfs:comment>
        <oil:seeAlso rdf:resource="&oil;first"/>
        <rdfs:domain rdf:resource="&or;Image"/>
        <rdfs:range rdf:resource="&or;ImageSequence"/>
    </owl:ObjectProperty>
    


    <!-- http://www.nist.gov/itl/ssd/OntologyRequirements#formatsInformationAbout -->

    <owl:ObjectProperty rdf:about="&or;formatsInformationAbout">
        <rdfs:comment xml:lang="en">A Data Format `formats Information About&#39; a type of thing if provides a formatted way of describing something of that type and if an information structure with that format would normally provide such information.  See `optionally Formats information About&#39;.</rdfs:comment>
        <rdfs:domain rdf:resource="&or;DataFormat"/>
        <rdfs:range rdf:resource="&owl;Thing"/>
    </owl:ObjectProperty>
    


    <!-- http://www.nist.gov/itl/ssd/OntologyRequirements#frameOfVideo -->

    <owl:ObjectProperty rdf:about="&or;frameOfVideo">
        <rdfs:comment xml:lang="en">Frame Of Video rates a still image to a Moving Image in which it is contained as a single frame.  The same frame may appear in multiple Moving Images.  A single  Moving Image may have a large number of identifible individual single images as frames.</rdfs:comment>
        <rdfs:range rdf:resource="&or;MovingImage"/>
        <rdfs:domain rdf:resource="&or;StillImage"/>
        <rdfs:subPropertyOf rdf:resource="&or;partOf"/>
    </owl:ObjectProperty>
    


    <!-- http://www.nist.gov/itl/ssd/OntologyRequirements#hasComputerFileFormat -->

    <owl:ObjectProperty rdf:about="&or;hasComputerFileFormat">
        <rdfs:comment xml:lang="en">The predicate ``has Computer File Format&#39; &#39; relates a Computer File to an Electronic File Format that it follows.</rdfs:comment>
        <rdfs:domain rdf:resource="&or;ComputerFile"/>
        <rdfs:range rdf:resource="&or;ElectronicFileFormat"/>
    </owl:ObjectProperty>
    


    <!-- http://www.nist.gov/itl/ssd/OntologyRequirements#hasPropertyValue -->

    <owl:ObjectProperty rdf:about="&or;hasPropertyValue">
        <rdfs:comment xml:lang="en">The propety ``has Property Value&#39;&#39; relates something to a property it has that is associated with a value, such as an object&#39;s length being 3 meters or its melting point being 0 C.   Something can have many associated property values.</rdfs:comment>
        <rdfs:range rdf:resource="&or;PropertyWithValue"/>
        <rdfs:domain rdf:resource="&owl;Thing"/>
    </owl:ObjectProperty>
    


    <!-- http://www.nist.gov/itl/ssd/OntologyRequirements#imageCreatedBy -->

    <owl:ObjectProperty rdf:about="&or;imageCreatedBy">
        <rdfs:domain rdf:resource="&or;Image"/>
        <rdfs:range rdf:resource="&or;ImageInputDevice"/>
    </owl:ObjectProperty>
    


    <!-- http://www.nist.gov/itl/ssd/OntologyRequirements#imageOfObject -->

    <owl:ObjectProperty rdf:about="&or;imageOfObject">
        <rdfs:domain rdf:resource="&or;Image"/>
        <rdfs:range rdf:resource="&or;PhysicalObject"/>
    </owl:ObjectProperty>
    


    <!-- http://www.nist.gov/itl/ssd/OntologyRequirements#imageOfPatientPart -->

    <owl:ObjectProperty rdf:about="&or;imageOfPatientPart">
        <rdfs:comment xml:lang="en">This image is an image of part of the human patient.  [For veternary use, create a different predicate.  Legal restrictions apply to informatiion linking images to people that do not apply to non-human animals.]</rdfs:comment>
        <rdfs:range rdf:resource="&or;Human"/>
        <rdfs:domain rdf:resource="&or;Image"/>
    </owl:ObjectProperty>
    


    <!-- http://www.nist.gov/itl/ssd/OntologyRequirements#implementsAlgorithm -->

    <owl:ObjectProperty rdf:about="&or;implementsAlgorithm">
        <rdfs:comment xml:lang="en">The relation ``implements Algorithm&#39; &#39; indicates that the specified piece of software implements the specified algorithm (among others).</rdfs:comment>
        <rdfs:range rdf:resource="&or;Algorithm"/>
        <rdfs:domain rdf:resource="&or;Software"/>
    </owl:ObjectProperty>
    


    <!-- http://www.nist.gov/itl/ssd/OntologyRequirements#inputData -->

    <owl:ObjectProperty rdf:about="&or;inputData">
        <rdfs:comment xml:lang="en">The property `input Data&#39; relates a Computer Process Execution to data which it has as input.</rdfs:comment>
        <rdfs:range rdf:resource="&or;AbstractStructuredInformationStore"/>
        <rdfs:domain rdf:resource="&or;ComputerProcessExecution"/>
    </owl:ObjectProperty>
    


    <!-- http://www.nist.gov/itl/ssd/OntologyRequirements#measurementComponent -->

    <owl:ObjectProperty rdf:about="&or;measurementComponent">
        <oil:seeAlso xml:lang="en"> The property `measurement Component&#39; descripes how an Image Series plays a role in the measurement.</oil:seeAlso>
        <rdfs:domain rdf:resource="&or;ImageSequence"/>
        <rdfs:range rdf:resource="&or;MeasurementRole"/>
        <rdfs:subPropertyOf rdf:resource="&owl;topObjectProperty"/>
    </owl:ObjectProperty>
    


    <!-- http://www.nist.gov/itl/ssd/OntologyRequirements#memberOfOrganization -->

    <owl:ObjectProperty rdf:about="&or;memberOfOrganization">
        <rdf:type rdf:resource="&owl;IrreflexiveProperty"/>
        <rdfs:domain rdf:resource="&or;IntelligentAgent"/>
        <rdfs:range rdf:resource="&or;Organization"/>
    </owl:ObjectProperty>
    


    <!-- http://www.nist.gov/itl/ssd/OntologyRequirements#moreSpecificSoftwareObject -->

    <owl:ObjectProperty rdf:about="&or;moreSpecificSoftwareObject">
        <rdf:type rdf:resource="&owl;AsymmetricProperty"/>
        <rdfs:comment xml:lang="en">The property ``more Specific Software Object&#39; &#39; relates a Software Object With Versions to more specific software, either one with a more constrained set of versions or a Software Object Version (in which case the more specific property ``software Has Version&#39; &#39; applies).</rdfs:comment>
        <rdfs:range rdf:resource="&or;Software"/>
        <rdfs:domain rdf:resource="&or;SoftwareObjectWithVersions"/>
    </owl:ObjectProperty>
    


    <!-- http://www.nist.gov/itl/ssd/OntologyRequirements#objectActedOn -->

    <owl:ObjectProperty rdf:about="&or;objectActedOn">
        <rdfs:comment>The property objectActedOn is used to relate an event to any object significantly affected in that event. The object(s) in question must exist before the event, but may be either destroyed in the event or merely affected by it

Same as cyc:objectActedOn.</rdfs:comment>
        <rdfs:domain rdf:resource="&or;Event"/>
        <rdfs:range rdf:resource="&or;TemporalThing"/>
    </owl:ObjectProperty>
    


    <!-- http://www.nist.gov/itl/ssd/OntologyRequirements#objectImagedBy -->

    <owl:ObjectProperty rdf:about="&or;objectImagedBy">
        <rdfs:comment xml:lang="en">The property &#39;object Imaged By&#39; relates a Physical Object to an Image Input Device which captured an image of it.  A given Physical Object may be imaged by different imaging devices at different times and a given imaging device can be expected to produce images of many different Physical  Objects.</rdfs:comment>
        <rdfs:range rdf:resource="&or;ImageInputDevice"/>
        <rdfs:domain rdf:resource="&or;PhysicalObject"/>
    </owl:ObjectProperty>
    


    <!-- http://www.nist.gov/itl/ssd/OntologyRequirements#objectMoving -->

    <owl:ObjectProperty rdf:about="&or;objectMoving">
        <rdfs:comment xml:lang="en">The predicate objectMoving relates movement events to each object moving in the event.</rdfs:comment>
        <rdfs:domain rdf:resource="&or;MovementEvent"/>
        <rdfs:range rdf:resource="&or;PhysicalObject"/>
    </owl:ObjectProperty>
    


    <!-- http://www.nist.gov/itl/ssd/OntologyRequirements#ontologyDomain -->

    <owl:ObjectProperty rdf:about="&or;ontologyDomain">
        <rdfs:comment xml:lang="en">The domain of an Ontology is the Field Of Study which it covers.</rdfs:comment>
        <rdfs:domain rdf:resource="&oil;Ontology"/>
        <rdfs:range rdf:resource="&or;FieldOfStudy"/>
    </owl:ObjectProperty>
    


    <!-- http://www.nist.gov/itl/ssd/OntologyRequirements#optionallyFormatsInformationAbout -->

    <owl:ObjectProperty rdf:about="&or;optionallyFormatsInformationAbout">
        <rdfs:comment xml:lang="en">A Data Format `optionally Formats Information About&#39; a type of thing if provides a formatted way of describing something of that type but an information structure with that format would is not necessarily expected to provide such information.  See `formats information About&#39; for when such information is expected.</rdfs:comment>
        <rdfs:domain rdf:resource="&or;DataFormat"/>
        <rdfs:range rdf:resource="&owl;Thing"/>
    </owl:ObjectProperty>
    


    <!-- http://www.nist.gov/itl/ssd/OntologyRequirements#outputCreated -->

    <owl:ObjectProperty rdf:about="&or;outputCreated">
        <rdfs:comment xml:lang="en">The property &#39;output Created&#39; specifies something that was created in a Creation Event.  There may be many outputs of a single Creation Event.</rdfs:comment>
        <rdfs:domain rdf:resource="&or;CreationEvent"/>
        <rdfs:range rdf:resource="&or;TemporalThing"/>
    </owl:ObjectProperty>
    


    <!-- http://www.nist.gov/itl/ssd/OntologyRequirements#outputData -->

    <owl:ObjectProperty rdf:about="&or;outputData">
        <rdfs:comment xml:lang="en">The property `ioutput Data&#39; relates a Computer Process Execution to data which it outputs.  The output can be in the form of a computer file, display on a screen, or signals to a printer or robotic device.  The physical object printed by a printer, manufactured by a robot, and the motions made by the robot are not considered to be output DATA of the program.

The inputData and outputData for a program are usually different, but this is not always the case.</rdfs:comment>
        <rdfs:range rdf:resource="&or;AbstractStructuredInformationStore"/>
        <rdfs:domain rdf:resource="&or;ComputerProcessExecution"/>
        <rdfs:subPropertyOf rdf:resource="&or;outputCreated"/>
    </owl:ObjectProperty>
    


    <!-- http://www.nist.gov/itl/ssd/OntologyRequirements#parameterValue -->

    <owl:ObjectProperty rdf:about="&or;parameterValue">
        <rdfs:domain rdf:resource="&or;MaterialProperty"/>
        <rdfs:range rdf:resource="&or;Quantity"/>
    </owl:ObjectProperty>
    


    <!-- http://www.nist.gov/itl/ssd/OntologyRequirements#partOf -->

    <owl:ObjectProperty rdf:about="&or;partOf">
        <rdf:type rdf:resource="&owl;AsymmetricProperty"/>
        <rdf:type rdf:resource="&owl;TransitiveProperty"/>
        <rdfs:comment xml:lang="en">The first thing is in some way a proper part of the second thing.  [``Proper&#39; &#39; meaning that a thing is not considered to be part of itself.]  Parthood is transitive: a part of a part of a larger thing is itself a part of the larger thing. Parthood is not necesarily physical: subevents, subfields (of Fields Of Study), and software subroutines are also parthood relations.  Use a narrower relation if possible.

This is an inverse property to cyc:properParts.</rdfs:comment>
        <rdfs:range rdf:resource="&owl;Thing"/>
        <rdfs:domain rdf:resource="&owl;Thing"/>
    </owl:ObjectProperty>
    


    <!-- http://www.nist.gov/itl/ssd/OntologyRequirements#performedBy -->

    <owl:ObjectProperty rdf:about="&or;performedBy">
        <rdfs:comment xml:lang="en">A predicate that relates an Action to an Intelligent Agent who deliberately performs it.</rdfs:comment>
        <rdfs:domain rdf:resource="&or;Event"/>
        <rdfs:range rdf:resource="&or;IntelligentAgent"/>
        <rdfs:subPropertyOf rdf:resource="&or;doneBy"/>
    </owl:ObjectProperty>
    


    <!-- http://www.nist.gov/itl/ssd/OntologyRequirements#physicallyAssociatedComponent -->

    <owl:ObjectProperty rdf:about="&or;physicallyAssociatedComponent">
        <rdf:type rdf:resource="&owl;IrreflexiveProperty"/>
        <rdf:type rdf:resource="&owl;SymmetricProperty"/>
        <rdfs:comment xml:lang="en">The property, &#39;physically Associated Component&#39; relates one Physical Object to another one to which it is attached, is adjacent to, encloses or is enclosed by, or is related to by some similar relationship.</rdfs:comment>
        <rdfs:domain rdf:resource="&or;PhysicalObject"/>
        <rdfs:range rdf:resource="&or;PhysicalObject"/>
    </owl:ObjectProperty>
    


    <!-- http://www.nist.gov/itl/ssd/OntologyRequirements#productSource -->

    <owl:ObjectProperty rdf:about="&or;productSource">
        <rdfs:range rdf:resource="&or;Organization"/>
        <rdfs:domain rdf:resource="&or;PhysicalObject"/>
    </owl:ObjectProperty>
    


    <!-- http://www.nist.gov/itl/ssd/OntologyRequirements#propertyIs -->

    <owl:ObjectProperty rdf:about="&or;propertyIs">
        <rdf:type rdf:resource="&owl;FunctionalProperty"/>
        <rdfs:comment xml:lang="en">The relation ``property Is&#39;&#39; relates a Property With Value to the Generic Property that it instantiates.</rdfs:comment>
        <rdfs:range rdf:resource="&or;GenericProperty"/>
        <rdfs:domain rdf:resource="&or;PropertyWithValue"/>
    </owl:ObjectProperty>
    


    <!-- http://www.nist.gov/itl/ssd/OntologyRequirements#propertysValue -->

    <owl:ObjectProperty rdf:about="&or;propertysValue">
        <rdf:type rdf:resource="&owl;FunctionalProperty"/>
        <rdfs:comment xml:lang="en">The relation ``property&#39;s Value&#39;&#39; relates a Property With Value to the quantity that is the value of that property.</rdfs:comment>
        <rdfs:domain rdf:resource="&or;PropertyWithValue"/>
        <rdfs:range rdf:resource="&or;Quantity"/>
    </owl:ObjectProperty>
    


    <!-- http://www.nist.gov/itl/ssd/OntologyRequirements#restOfImageSequence -->

    <owl:ObjectProperty rdf:about="&or;restOfImageSequence">
        <rdf:type rdf:resource="&owl;AsymmetricProperty"/>
        <rdf:type rdf:resource="&owl;FunctionalProperty"/>
        <skos:note>Maybe a more generic property -- restOfSequence -- should be substituted for this more specific one.</skos:note>
        <rdfs:comment xml:lang="en">Specifies the rest of an Image Sequence after the first Image.</rdfs:comment>
        <rdfs:subPropertyOf rdf:resource="&oil;rest"/>
        <rdfs:range rdf:resource="&or;ImageSequence"/>
        <rdfs:domain rdf:resource="&or;ImageSequence"/>
    </owl:ObjectProperty>
    


    <!-- http://www.nist.gov/itl/ssd/OntologyRequirements#softwareCodedIn -->

    <owl:ObjectProperty rdf:about="&or;softwareCodedIn">
        <rdfs:comment xml:lang="en">The specified software is at least partially coded in the specified computer language.</rdfs:comment>
        <rdfs:range rdf:resource="&or;ComputerLanguage"/>
        <rdfs:domain rdf:resource="&or;Software"/>
    </owl:ObjectProperty>
    


    <!-- http://www.nist.gov/itl/ssd/OntologyRequirements#softwareHasVersion -->

    <owl:ObjectProperty rdf:about="&or;softwareHasVersion">
        <rdfs:comment xml:lang="en">A predicate relating an instance of Software Object With Versions to one of its specific versions (which is an instance of Software Object Version).

Same as cyc:versionOfSoftware.</rdfs:comment>
        <rdfs:domain rdf:resource="&or;SoftwareObjectWithVersions"/>
        <rdfs:range rdf:resource="&or;SofwareObjectVersion"/>
        <rdfs:subPropertyOf rdf:resource="&or;moreSpecificSoftwareObject"/>
    </owl:ObjectProperty>
    


    <!-- http://www.nist.gov/itl/ssd/OntologyRequirements#softwareObjectComponent -->

    <owl:ObjectProperty rdf:about="&or;softwareObjectComponent">
        <rdf:type rdf:resource="&owl;AsymmetricProperty"/>
        <rdf:type rdf:resource="&owl;TransitiveProperty"/>
        <rdfs:comment xml:lang="en">The property ``softwareObjectComponent&#39; &#39; relates a Software object to a smaller Software object which comprises it.  This property relates a Software Package to programs and methods which it contains, a Software Library to the elements of the library, and a Computer Program to threads, methods, and subroutines which it calls.</rdfs:comment>
        <rdfs:domain rdf:resource="&or;Software"/>
        <rdfs:range rdf:resource="&or;Software"/>
        <rdfs:subPropertyOf rdf:resource="&or;partOf"/>
    </owl:ObjectProperty>
    


    <!-- http://www.nist.gov/itl/ssd/OntologyRequirements#specializedTypeOf -->

    <owl:ObjectProperty rdf:about="&or;specializedTypeOf">
        <rdf:type rdf:resource="&owl;AsymmetricProperty"/>
        <rdf:type rdf:resource="&owl;TransitiveProperty"/>
        <rdfs:comment xml:lang="en">A `specialized Type Of&#39; an instance of Second Order Class is a subclass of that second class.</rdfs:comment>
        <skos:note xml:lang="en">A `specialized Type&#39; would be modeled as a subClass relation if OWL handled metaclasses.</skos:note>
        <rdfs:domain rdf:resource="&or;FirstOrderClass"/>
        <rdfs:range rdf:resource="&or;FirstOrderClass"/>
    </owl:ObjectProperty>
    


    <!-- http://www.nist.gov/itl/ssd/OntologyRequirements#startsAt -->

    <owl:ObjectProperty rdf:about="&or;startsAt">
        <rdfs:comment xml:lang="en">The property ``starts At&#39; &#39; specifies the Date Time at which a given temporal thing starts to happen or exist.  The same event (or object) can be held to ``start At&#39; &#39; different Date Times when one starting time is more specific than another.  For example, the statement that a cell division starts At 9:23 on May 8, 2018, does not conflict with a statement that the same cell division starts At 9:23:16 on May 8, 2018.

Same as cyc:startingDate.</rdfs:comment>
        <rdfs:range rdf:resource="&or;DateTime"/>
        <rdfs:domain rdf:resource="&or;TemporalThing"/>
    </owl:ObjectProperty>
    


    <!-- http://www.nist.gov/itl/ssd/OntologyRequirements#storesInformationAbout -->

    <owl:ObjectProperty rdf:about="&or;storesInformationAbout">
        <rdfs:comment xml:lang="en">The property &#39;stores Information About&#39; relates a Data Object to something about which it stores data.</rdfs:comment>
        <rdfs:domain rdf:resource="&or;DataObject"/>
        <rdfs:range rdf:resource="&owl;Thing"/>
    </owl:ObjectProperty>
    


    <!-- http://www.nist.gov/itl/ssd/OntologyRequirements#subEventOf -->

    <owl:ObjectProperty rdf:about="&or;subEventOf">
        <rdf:type rdf:resource="&owl;AsymmetricProperty"/>
        <rdf:type rdf:resource="&owl;TransitiveProperty"/>
        <rdfs:comment xml:lang="en">If one event is a subEvent Of another event, than it is a proper part of that event.  This is a transitive relationship: if A is a subEvent Of B AND B is a subEvent Of C, then A is a subEvent Of C. The subevent can not start before or end after the main event.  This is an inverse property of cyc:properSubEvents.

The relation subEventOf relates an Event to Events of which it is a proper part. Events can be decomposed into subevents temporally, spatially, and in other ways.

For example, an Experiment might have subvents of preparing a sample, sensing properties of that sample, and processing the sensor results.  Each of these subevents would have a set of their own subevents.

The property subEventOf is transitive (a subEventOf a subevent is a subEventOf the main event) but irreflexive -- an event can not be a subEventOf itself. </rdfs:comment>
        <rdfs:domain rdf:resource="&or;Event"/>
        <rdfs:range rdf:resource="&or;Event"/>
        <rdfs:subPropertyOf rdf:resource="&or;partOf"/>
    </owl:ObjectProperty>
    


    <!-- http://www.nist.gov/itl/ssd/OntologyRequirements#subFieldOf -->

    <owl:ObjectProperty rdf:about="&or;subFieldOf">
        <rdf:type rdf:resource="&owl;AsymmetricProperty"/>
        <rdf:type rdf:resource="&owl;TransitiveProperty"/>
        <rdfs:comment xml:lang="en">If one Field Of Study is a subField of another Field Of Study, that means that the subField is a narrower Field Of Study and is part of the broader field.  This is the same as cyc:subFields.</rdfs:comment>
        <rdfs:range rdf:resource="&or;FieldOfStudy"/>
        <rdfs:domain rdf:resource="&or;FieldOfStudy"/>
        <rdfs:subPropertyOf rdf:resource="&or;partOf"/>
    </owl:ObjectProperty>
    


    <!-- http://www.nist.gov/itl/ssd/OntologyRequirements#unitTypeFor -->

    <owl:ObjectProperty rdf:about="&or;unitTypeFor">
        <rdf:type rdf:resource="&owl;FunctionalProperty"/>
        <rdfs:comment xml:lang="en">The property &#39;unit Type For&#39; specifies the type of Unit Of Measure that can be used for a given Measurable Property.</rdfs:comment>
        <rdfs:range rdf:resource="&or;InterconvertibleUnitType"/>
        <rdfs:domain>
            <owl:Class>
                <owl:unionOf rdf:parseType="Collection">
                    <rdf:Description rdf:about="&or;MeasurableProperty"/>
                    <rdf:Description rdf:about="&or;MeasurableQuantity"/>
                </owl:unionOf>
            </owl:Class>
        </rdfs:domain>
    </owl:ObjectProperty>
    


    <!-- http://www.nist.gov/itl/ssd/OntologyRequirements#unitsFor -->

    <owl:ObjectProperty rdf:about="&or;unitsFor">
        <rdfs:comment xml:lang="en">The property &#39;units For&#39; specifies Units Of Measurement that can be used for an Expressed  Quantity.</rdfs:comment>
        <rdfs:range rdf:resource="&or;MeasurableQuantity"/>
        <rdfs:domain rdf:resource="&or;UnitOfMeasure"/>
    </owl:ObjectProperty>
    


    <!-- 
    ///////////////////////////////////////////////////////////////////////////////////////
    //
    // Data properties
    //
    ///////////////////////////////////////////////////////////////////////////////////////
     -->

    


    <!-- http://www.nist.gov/itl/ssd/OntologyRequirements#acronym -->

    <owl:DatatypeProperty rdf:about="&or;acronym">
        <rdfs:comment xml:lang="en">The relation ``acronym&#39;&#39; relates something (organization, conference, ...) to an acronym -- a string of (normally) letters that are the first (few) letters in the name of the thing.

Normally something will have only a single acronym.</rdfs:comment>
        <rdfs:subPropertyOf rdf:resource="&or;nameString"/>
        <rdfs:range rdf:resource="&xsd;Name"/>
        <rdfs:domain rdf:resource="&owl;Thing"/>
    </owl:DatatypeProperty>
    


    <!-- http://www.nist.gov/itl/ssd/OntologyRequirements#catalogNumber -->

    <owl:DatatypeProperty rdf:about="&or;catalogNumber">
        <rdfs:comment xml:lang="en">The `catalog Number&#39; of some (type of) artifact is the text string it has listed as a catalog number in the appropriate product catalog.</rdfs:comment>
        <rdfs:subPropertyOf rdf:resource="&or;idString"/>
        <rdfs:range rdf:resource="&xsd;NMTOKEN"/>
        <rdfs:domain>
            <owl:Class>
                <owl:unionOf rdf:parseType="Collection">
                    <rdf:Description rdf:about="&or;Artifact"/>
                    <rdf:Description rdf:about="&or;EventType"/>
                    <rdf:Description rdf:about="&or;ObjectType"/>
                </owl:unionOf>
            </owl:Class>
        </rdfs:domain>
    </owl:DatatypeProperty>
    


    <!-- http://www.nist.gov/itl/ssd/OntologyRequirements#contactInformation -->

    <owl:DatatypeProperty rdf:about="&or;contactInformation">
        <rdfs:domain rdf:resource="&or;IntelligentAgent"/>
        <rdfs:range rdf:resource="&xsd;string"/>
    </owl:DatatypeProperty>
    


    <!-- http://www.nist.gov/itl/ssd/OntologyRequirements#defaultFileExtension -->

    <owl:DatatypeProperty rdf:about="&or;defaultFileExtension">
        <rdfs:domain rdf:resource="&or;ElectronicFileFormat"/>
        <rdfs:range rdf:resource="&xsd;NMTOKEN"/>
    </owl:DatatypeProperty>
    


    <!-- http://www.nist.gov/itl/ssd/OntologyRequirements#emailAddress -->

    <owl:DatatypeProperty rdf:about="&or;emailAddress">
        <rdfs:domain rdf:resource="&or;IntelligentAgent"/>
        <rdfs:subPropertyOf rdf:resource="&or;contactInformation"/>
        <rdfs:range rdf:resource="&xsd;anyURI"/>
    </owl:DatatypeProperty>
    


    <!-- http://www.nist.gov/itl/ssd/OntologyRequirements#endingDate -->

    <owl:DatatypeProperty rdf:about="&or;endingDate">
        <rdf:type rdf:resource="&owl;FunctionalProperty"/>
        <rdfs:domain rdf:resource="&or;Event"/>
        <rdfs:range rdf:resource="&xsd;dateTime"/>
    </owl:DatatypeProperty>
    


    <!-- http://www.nist.gov/itl/ssd/OntologyRequirements#expressedValue -->

    <owl:DatatypeProperty rdf:about="&or;expressedValue">
        <rdf:type rdf:resource="&owl;FunctionalProperty"/>
        <rdfs:comment xml:lang="en">The number of units (of a particular Units Of Measure) in which an Expressed Quantity is specified.  For example, a Volume expressed as 1.5 Liters has Liter as its expressed Unit Of Measure and 1.5 as its expressed Value.  The same volume may also be expressed as a different Expressed Quantity: with Millileter as the expressed Unit Of Measure and 1500 as the expressed Value.  

The same Quantity has represenations as two different Expressed Quantities in this case.</rdfs:comment>
        <rdfs:domain rdf:resource="&or;ExpressedQuantity"/>
    </owl:DatatypeProperty>
    


    <!-- http://www.nist.gov/itl/ssd/OntologyRequirements#faxNumber -->

    <owl:DatatypeProperty rdf:about="&or;faxNumber">
        <rdfs:domain rdf:resource="&or;IntelligentAgent"/>
        <rdfs:subPropertyOf rdf:resource="&or;contactInformation"/>
        <rdfs:range rdf:resource="&xsd;string"/>
    </owl:DatatypeProperty>
    


    <!-- http://www.nist.gov/itl/ssd/OntologyRequirements#idString -->

    <owl:DatatypeProperty rdf:about="&or;idString">
        <rdfs:range rdf:resource="&xsd;Name"/>
        <rdfs:domain rdf:resource="&owl;Thing"/>
    </owl:DatatypeProperty>
    


    <!-- http://www.nist.gov/itl/ssd/OntologyRequirements#imageCollectionDate -->

    <owl:DatatypeProperty rdf:about="&or;imageCollectionDate">
        <rdf:type rdf:resource="&owl;FunctionalProperty"/>
        <rdfs:range rdf:resource="&xsd;dateTime"/>
        <rdfs:domain>
            <owl:Class>
                <owl:unionOf rdf:parseType="Collection">
                    <rdf:Description rdf:about="&or;Image"/>
                    <rdf:Description rdf:about="&or;ImageSequence"/>
                </owl:unionOf>
            </owl:Class>
        </rdfs:domain>
    </owl:DatatypeProperty>
    


    <!-- http://www.nist.gov/itl/ssd/OntologyRequirements#imageSeriesCollectionBasis -->

    <owl:DatatypeProperty rdf:about="&or;imageSeriesCollectionBasis">
        <skos:note xml:lang="en"> Should the posible bases be ontologized, allowing this to be an object property?</skos:note>
        <rdfs:comment xml:lang="en">The basis of the images in the series.   For example, fields in a well, wells, time, microfluidic chambers, etc.</rdfs:comment>
        <rdfs:domain rdf:resource="&or;ImageSequence"/>
        <rdfs:range rdf:resource="&xsd;string"/>
    </owl:DatatypeProperty>
    


    <!-- http://www.nist.gov/itl/ssd/OntologyRequirements#initiationDate -->

    <owl:DatatypeProperty rdf:about="&or;initiationDate">
        <rdf:type rdf:resource="&owl;FunctionalProperty"/>
        <rdfs:comment xml:lang="en">The date that an event, for example a research study, was started.</rdfs:comment>
        <rdfs:domain rdf:resource="&or;Event"/>
        <rdfs:range rdf:resource="&xsd;dateTime"/>
    </owl:DatatypeProperty>
    


    <!-- http://www.nist.gov/itl/ssd/OntologyRequirements#makeID -->

    <owl:DatatypeProperty rdf:about="&or;makeID">
        <rdf:type rdf:resource="&owl;FunctionalProperty"/>
        <rdfs:comment xml:lang="en">A commercially manufactured artifact often has make and model names.  The property, modelID relates such an artifact to the name of its make.</rdfs:comment>
        <rdfs:domain rdf:resource="&or;Artifact"/>
        <rdfs:subPropertyOf rdf:resource="&or;idString"/>
        <rdfs:range rdf:resource="&xsd;Name"/>
    </owl:DatatypeProperty>
    


    <!-- http://www.nist.gov/itl/ssd/OntologyRequirements#modelID -->

    <owl:DatatypeProperty rdf:about="&or;modelID">
        <rdf:type rdf:resource="&owl;FunctionalProperty"/>
        <rdfs:comment xml:lang="en">A commercially manufactured artifact often has a make and model name.  The property, modelID relates such an artifact to its model name.</rdfs:comment>
        <rdfs:domain rdf:resource="&or;Artifact"/>
        <rdfs:subPropertyOf rdf:resource="&or;idString"/>
        <rdfs:range rdf:resource="&xsd;Name"/>
    </owl:DatatypeProperty>
    


    <!-- http://www.nist.gov/itl/ssd/OntologyRequirements#nameSpaceURI -->

    <owl:DatatypeProperty rdf:about="&or;nameSpaceURI">
        <rdf:type rdf:resource="&owl;FunctionalProperty"/>
        <rdfs:comment xml:lang="en">The ``name Space URI&#39; &#39; property specifies the base URI to which the local name of a term in an ontology is appended to generate the expanded name (full URI) for that term.</rdfs:comment>
        <rdfs:domain rdf:resource="&oil;Ontology"/>
        <rdfs:range rdf:resource="&xsd;anyURI"/>
    </owl:DatatypeProperty>
    


    <!-- http://www.nist.gov/itl/ssd/OntologyRequirements#nameString -->

    <owl:DatatypeProperty rdf:about="&or;nameString">
        <rdfs:comment xml:lang="en">The property ``nameString&#39; &#39; relates something to a name it has.  Things in general can have multiple names.</rdfs:comment>
        <rdfs:subPropertyOf rdf:resource="&or;idString"/>
        <rdfs:range rdf:resource="&xsd;Name"/>
        <rdfs:domain rdf:resource="&owl;Thing"/>
    </owl:DatatypeProperty>
    


    <!-- http://www.nist.gov/itl/ssd/OntologyRequirements#nickName -->

    <owl:DatatypeProperty rdf:about="&or;nickName">
        <rdfs:comment xml:lang="en">A nickName is a short name for something, different from its normal name.</rdfs:comment>
        <rdfs:subPropertyOf rdf:resource="&or;nameString"/>
        <rdfs:range rdf:resource="&xsd;Name"/>
        <rdfs:domain rdf:resource="&owl;Thing"/>
    </owl:DatatypeProperty>
    


    <!-- http://www.nist.gov/itl/ssd/OntologyRequirements#numberOfImagesInSequence -->

    <owl:DatatypeProperty rdf:about="&or;numberOfImagesInSequence">
        <rdf:type rdf:resource="&owl;FunctionalProperty"/>
        <rdfs:comment>Maybe a more generic property -- numberOfItemsInSequence -- should be substituted for this more specific one.</rdfs:comment>
        <rdfs:comment xml:lang="en">Specifies the number of Images in an Image Sequence.</rdfs:comment>
        <rdfs:domain rdf:resource="&or;ImageSequence"/>
        <rdfs:range rdf:resource="&xsd;nonNegativeInteger"/>
        <oil:seeAlso rdf:resource="&owl;cardinality"/>
    </owl:DatatypeProperty>
    


    <!-- http://www.nist.gov/itl/ssd/OntologyRequirements#postalAddress -->

    <owl:DatatypeProperty rdf:about="&or;postalAddress">
        <rdfs:domain rdf:resource="&or;IntelligentAgent"/>
        <rdfs:subPropertyOf rdf:resource="&or;contactInformation"/>
        <rdfs:range rdf:resource="&xsd;string"/>
    </owl:DatatypeProperty>
    


    <!-- http://www.nist.gov/itl/ssd/OntologyRequirements#referenceURI -->

    <owl:DatatypeProperty rdf:about="&or;referenceURI">
        <rdfs:comment xml:lang="en">The property `referenceURI&#39;   specifies a URI that is a global identifier for the term.</rdfs:comment>
        <rdfs:range rdf:resource="&xsd;anyURI"/>
    </owl:DatatypeProperty>
    


    <!-- http://www.nist.gov/itl/ssd/OntologyRequirements#softwareVersionID -->

    <owl:DatatypeProperty rdf:about="&or;softwareVersionID">
        <rdf:type rdf:resource="&owl;FunctionalProperty"/>
        <rdfs:comment xml:lang="en">A software object version often has a version ID.  The property, softwareVersionID relates such a software object to the version ID.</rdfs:comment>
        <rdfs:domain rdf:resource="&or;SofwareObjectVersion"/>
        <rdfs:subPropertyOf rdf:resource="&or;nameString"/>
        <rdfs:range rdf:resource="&xsd;Name"/>
    </owl:DatatypeProperty>
    


    <!-- http://www.nist.gov/itl/ssd/OntologyRequirements#standardNamespacePrefix -->

    <owl:DatatypeProperty rdf:about="&or;standardNamespacePrefix">
        <rdfs:comment xml:lang="en">This property specifies the standard prefix used to identify the ontology, so that a qualified name for a term in that ontology can be specified by appending the term&#39;s local name to this prefix.  The full URI of the term can be expanded by appending its local name to the namespace URI of the ontology.</rdfs:comment>
        <rdfs:domain rdf:resource="&oil;Ontology"/>
        <rdfs:range rdf:resource="&xsd;NCName"/>
    </owl:DatatypeProperty>
    


    <!-- http://www.nist.gov/itl/ssd/OntologyRequirements#telephoneNumber -->

    <owl:DatatypeProperty rdf:about="&or;telephoneNumber">
        <rdfs:domain rdf:resource="&or;IntelligentAgent"/>
        <rdfs:subPropertyOf rdf:resource="&or;contactInformation"/>
        <rdfs:range rdf:resource="&xsd;string"/>
    </owl:DatatypeProperty>
    


    <!-- 
    ///////////////////////////////////////////////////////////////////////////////////////
    //
    // Classes
    //
    ///////////////////////////////////////////////////////////////////////////////////////
     -->

    


    <!-- http://www.daml.org/2001/03/daml+oil#Nothing -->

    <rdf:Description rdf:about="&oil;Nothing">
        <owl:disjointWith rdf:resource="&owl;Thing"/>
    </rdf:Description>
    


    <!-- http://www.daml.org/2001/03/daml+oil#ObjectProperty -->

    <rdf:Description rdf:about="&oil;ObjectProperty">
        <owl:equivalentClass rdf:resource="&owl;ObjectProperty"/>
    </rdf:Description>
    


    <!-- http://www.daml.org/2001/03/daml+oil#Ontology -->

    <rdf:Description rdf:about="&oil;Ontology">
        <rdfs:subClassOf rdf:resource="&or;AbstractStructuredInformationStore"/>
    </rdf:Description>
    


    <!-- http://www.daml.org/2001/03/daml+oil#Property -->

    <rdf:Description rdf:about="&oil;Property">
        <owl:equivalentClass rdf:resource="&rdf;Property"/>
        <rdfs:subClassOf rdf:resource="&or;NonTangibleThing"/>
        <owl:disjointWith rdf:resource="&or;Curve"/>
    </rdf:Description>
    


    <!-- http://www.daml.org/2001/03/daml+oil#TransitiveProperty -->

    <rdf:Description rdf:about="&oil;TransitiveProperty">
        <owl:disjointWith rdf:resource="&oil;UniqueProperty"/>
    </rdf:Description>
    


    <!-- http://www.daml.org/2001/03/daml+oil#UniqueProperty -->

    <rdf:Description rdf:about="&oil;UniqueProperty"/>
    


    <!-- http://www.nist.gov/itl/ssd/OntologyRequirements#AbstractStructuredInformationStore -->

    <owl:Class rdf:about="&or;AbstractStructuredInformationStore">
        <rdfs:subClassOf rdf:resource="&or;Information"/>
        <rdfs:subClassOf rdf:resource="&or;IntangibleCreatedThing"/>
        <rdfs:subClassOf rdf:resource="&or;StructuredInformationStore"/>
        <rdfs:comment xml:lang="en">A Structured Information Store that is abstract, such as a computer file, data base, or ontology, as opposed to a physical library or folded topographic map.  This does not include physical objects which encode such an information store, such as an optical disk or an arrangements of magnetic spots on a physical medium.</rdfs:comment>
    </owl:Class>
    


    <!-- http://www.nist.gov/itl/ssd/OntologyRequirements#ActionPlan -->

    <owl:Class rdf:about="&or;ActionPlan">
        <owl:equivalentClass>
            <owl:Restriction>
                <owl:onProperty rdf:resource="&or;outputCreated"/>
                <owl:someValuesFrom rdf:resource="&or;Planning"/>
            </owl:Restriction>
        </owl:equivalentClass>
        <rdfs:subClassOf rdf:resource="&or;ConceptualModel"/>
        <rdfs:comment xml:lang="en">An Action Plan is a plan for taking an action of a specified sort.</rdfs:comment>
    </owl:Class>
    


    <!-- http://www.nist.gov/itl/ssd/OntologyRequirements#Algorithm -->

    <owl:Class rdf:about="&or;Algorithm">
        <rdfs:subClassOf rdf:resource="&or;Technique"/>
        <owl:disjointWith rdf:resource="&or;TemporalThing"/>
    </owl:Class>
    


    <!-- http://www.nist.gov/itl/ssd/OntologyRequirements#ApplicationProgram -->

    <owl:Class rdf:about="&or;ApplicationProgram">
        <rdfs:subClassOf rdf:resource="&or;ComputerProgram"/>
        <rdfs:comment xml:lang="en">A specialization of ComputerProgram. An ApplicationProgram is a program a program distinct from a Systems Program, Operating System, or Operating System Kernel. </rdfs:comment>
    </owl:Class>
    


    <!-- http://www.nist.gov/itl/ssd/OntologyRequirements#April -->

    <owl:Class rdf:about="&or;April">
        <rdfs:subClassOf rdf:resource="&or;CalendarMonth"/>
        <rdfs:comment xml:lang="en">The month of April</rdfs:comment>
    </owl:Class>
    


    <!-- http://www.nist.gov/itl/ssd/OntologyRequirements#Area -->

    <owl:Class rdf:about="&or;Area">
        <owl:equivalentClass>
            <owl:Class>
                <owl:intersectionOf rdf:parseType="Collection">
                    <rdf:Description rdf:about="&or;MeasurableQuantity"/>
                    <owl:Restriction>
                        <owl:onProperty rdf:resource="&or;unitsFor"/>
                        <owl:someValuesFrom rdf:resource="&or;UnitOfArea"/>
                    </owl:Restriction>
                </owl:intersectionOf>
            </owl:Class>
        </owl:equivalentClass>
        <rdfs:subClassOf rdf:resource="&or;MeasurableQuantity"/>
        <rdfs:subClassOf>
            <owl:Restriction>
                <owl:onProperty rdf:resource="&or;unitsFor"/>
                <owl:allValuesFrom rdf:resource="&or;UnitOfArea"/>
            </owl:Restriction>
        </rdfs:subClassOf>
        <owl:disjointWith rdf:resource="&or;ComputerStorageCapacity"/>
        <owl:disjointWith rdf:resource="&or;Count"/>
        <owl:disjointWith rdf:resource="&or;Distance"/>
        <owl:disjointWith rdf:resource="&or;Duration"/>
        <owl:disjointWith rdf:resource="&or;Energy"/>
        <owl:disjointWith rdf:resource="&or;Force"/>
        <owl:disjointWith rdf:resource="&or;Mass"/>
        <owl:disjointWith rdf:resource="&or;Pressure"/>
        <owl:disjointWith rdf:resource="&or;Temperature"/>
        <owl:disjointWith rdf:resource="&or;Volume"/>
        <rdfs:comment xml:lang="en">An  Area is an amount of two-dimensional space.</rdfs:comment>
    </owl:Class>
    


    <!-- http://www.nist.gov/itl/ssd/OntologyRequirements#AreaChart -->

    <owl:Class rdf:about="&or;AreaChart">
        <rdfs:subClassOf rdf:resource="&or;GraphicalImage"/>
    </owl:Class>
    


    <!-- http://www.nist.gov/itl/ssd/OntologyRequirements#Array -->

    <owl:Class rdf:about="&or;Array">
        <rdfs:subClassOf rdf:resource="&or;AbstractStructuredInformationStore"/>
        <rdfs:comment xml:lang="en">An array is a list of items, which may themselves be lists.  An array may have one, two, or more dimensions.  If an arrray is a list of lists, each of the lists must be the same length and dimension.  

The (non-list) positions in an Array are called cells.  Cells may have numbers, strings, quantities, or variables representing such as values.</rdfs:comment>
    </owl:Class>
    


    <!-- http://www.nist.gov/itl/ssd/OntologyRequirements#Artifact -->

    <owl:Class rdf:about="&or;Artifact">
        <rdfs:subClassOf rdf:resource="&or;CreatedThing"/>
        <rdfs:subClassOf rdf:resource="&or;PhysicalObject"/>
        <rdfs:comment xml:lang="en">An Artifact is a physical object which was intentionally created to serve some purpose or perform some function.

Same as cyc:Artifact.</rdfs:comment>
    </owl:Class>
    


    <!-- http://www.nist.gov/itl/ssd/OntologyRequirements#AudioFileFormat -->

    <owl:Class rdf:about="&or;AudioFileFormat">
        <rdfs:subClassOf rdf:resource="&or;ElectronicFileFormat"/>
    </owl:Class>
    


    <!-- http://www.nist.gov/itl/ssd/OntologyRequirements#AudioVideoFileFormat -->

    <owl:Class rdf:about="&or;AudioVideoFileFormat">
        <rdfs:subClassOf rdf:resource="&or;ElectronicFileFormat"/>
    </owl:Class>
    


    <!-- http://www.nist.gov/itl/ssd/OntologyRequirements#AudioVisualImage -->

    <owl:Class rdf:about="&or;AudioVisualImage">
        <rdfs:subClassOf rdf:resource="&or;Image"/>
        <rdfs:comment xml:lang="en">An image with associated sound.  The image may be time varying or still.  It may be a Computer Image File, or a display or projection with sound.</rdfs:comment>
    </owl:Class>
    


    <!-- http://www.nist.gov/itl/ssd/OntologyRequirements#August -->

    <owl:Class rdf:about="&or;August">
        <rdfs:subClassOf rdf:resource="&or;CalendarMonth"/>
        <rdfs:comment xml:lang="en">The month of August</rdfs:comment>
    </owl:Class>
    


    <!-- http://www.nist.gov/itl/ssd/OntologyRequirements#BarGraph -->

    <owl:Class rdf:about="&or;BarGraph">
        <rdfs:subClassOf rdf:resource="&or;GraphicalImage"/>
    </owl:Class>
    


    <!-- http://www.nist.gov/itl/ssd/OntologyRequirements#BiomedicalFieldOfStudy -->

    <owl:Class rdf:about="&or;BiomedicalFieldOfStudy">
        <rdfs:subClassOf rdf:resource="&or;FieldOfStudy"/>
    </owl:Class>
    


    <!-- http://www.nist.gov/itl/ssd/OntologyRequirements#Block -->

    <owl:Class rdf:about="&or;Block">
        <rdfs:subClassOf rdf:resource="&or;RigidPortableObject"/>
        <rdfs:comment xml:lang="en">A Block is a solid tangible block-shaped object.</rdfs:comment>
    </owl:Class>
    


    <!-- http://www.nist.gov/itl/ssd/OntologyRequirements#CGS_Unit -->

    <owl:Class rdf:about="&or;CGS_Unit">
        <rdfs:subClassOf rdf:resource="&or;MetricUnit"/>
    </owl:Class>
    


    <!-- http://www.nist.gov/itl/ssd/OntologyRequirements#CalendarCentury -->

    <owl:Class rdf:about="&or;CalendarCentury">
        <rdfs:subClassOf rdf:resource="&or;DateTime"/>
        <owl:disjointWith rdf:resource="&or;CalendarDay"/>
        <owl:disjointWith rdf:resource="&or;CalendarHour"/>
        <owl:disjointWith rdf:resource="&or;CalendarMillisecond"/>
        <owl:disjointWith rdf:resource="&or;CalendarMinute"/>
        <owl:disjointWith rdf:resource="&or;CalendarMonth"/>
        <owl:disjointWith rdf:resource="&or;CalendarNanosecond"/>
        <owl:disjointWith rdf:resource="&or;CalendarWeek"/>
        <owl:disjointWith rdf:resource="&or;CalendarYear"/>
        <rdfs:comment xml:lang="en">A specialization of Date  Time, Calendar Century is the class of 100 year intervals that make up the calendar. Each Calendar Century is divided into one thousand contiguous Calendar Years. Note that a given instance of Calendar Century is a temporally continuous individual that occurs only once.

Note that different Calendar Centuries in the same calendary system can have different durations due to having different numbers of leap years.

Note also that Calendar Centuries defined by different systems can overlap.  Not only do the 15th century of the Muslim calendar, the 20th century of the Gregorian Calendar, and the 58th century of the Hebrew calendar overlap, but ``the 1900s (of the Gregorian Calendar)&#39; &#39; is a different Calendar century that has a 99 year overlap with the 20th Century.

Same as cyc:CalendarCentury.</rdfs:comment>
    </owl:Class>
    


    <!-- http://www.nist.gov/itl/ssd/OntologyRequirements#CalendarDay -->

    <owl:Class rdf:about="&or;CalendarDay">
        <rdfs:subClassOf rdf:resource="&or;DateTime"/>
        <owl:disjointWith rdf:resource="&or;CalendarHour"/>
        <owl:disjointWith rdf:resource="&or;CalendarMillisecond"/>
        <owl:disjointWith rdf:resource="&or;CalendarMinute"/>
        <owl:disjointWith rdf:resource="&or;CalendarMonth"/>
        <owl:disjointWith rdf:resource="&or;CalendarNanosecond"/>
        <owl:disjointWith rdf:resource="&or;CalendarWeek"/>
        <owl:disjointWith rdf:resource="&or;CalendarYear"/>
        <rdfs:comment xml:lang="en">A specialization  of Date  Time, Calendar Day is the class of 24-hour periods that make up the calendar. Each Calendar Day is divided into 24 contiguous Calendar Hours. Note that a given instance of Calendar Day is a temporally continuous individual that occurs only once.

Same as cyc:CalendarDay.</rdfs:comment>
    </owl:Class>
    


    <!-- http://www.nist.gov/itl/ssd/OntologyRequirements#CalendarHour -->

    <owl:Class rdf:about="&or;CalendarHour">
        <rdfs:subClassOf rdf:resource="&or;DateTime"/>
        <owl:disjointWith rdf:resource="&or;CalendarMillisecond"/>
        <owl:disjointWith rdf:resource="&or;CalendarMinute"/>
        <owl:disjointWith rdf:resource="&or;CalendarMonth"/>
        <owl:disjointWith rdf:resource="&or;CalendarNanosecond"/>
        <owl:disjointWith rdf:resource="&or;CalendarWeek"/>
        <owl:disjointWith rdf:resource="&or;CalendarYear"/>
        <rdfs:comment xml:lang="en">A specialization  of Date  Time, Calendar Hour is the class of 60 minute periods that make up the calendar. The sixty-minute interval from  9:00 through 9:59 AM GMT on May 4, 2013, is an instance of Calendar Minute, while the 60-minute interval from 8:54 through 9:53 AM of the same day is not.

Each Calendar Hour divided into sixty contiguous Calendar Minutes. Note that a given instance of Calendar Hour is a temporally continuous individual that occurs only once.

Same as cyc:CalendarHour.</rdfs:comment>
    </owl:Class>
    


    <!-- http://www.nist.gov/itl/ssd/OntologyRequirements#CalendarMillisecond -->

    <owl:Class rdf:about="&or;CalendarMillisecond">
        <rdfs:subClassOf rdf:resource="&or;DateTime"/>
        <owl:disjointWith rdf:resource="&or;CalendarMinute"/>
        <owl:disjointWith rdf:resource="&or;CalendarMonth"/>
        <owl:disjointWith rdf:resource="&or;CalendarNanosecond"/>
        <owl:disjointWith rdf:resource="&or;CalendarWeek"/>
        <owl:disjointWith rdf:resource="&or;CalendarYear"/>
        <rdfs:comment xml:lang="en">A specialization  of Date  Time, Calendar Millisecond is the class of milliseconds that make up the calendar. Each Calendar Secondis divided into one thousand contiguous Calendar Milliseconds. Note that a given instance of Calendar Millisecond is a temporally continuous individual that occurs only once.

Same as cyc:CalendarMilliSecond.</rdfs:comment>
    </owl:Class>
    


    <!-- http://www.nist.gov/itl/ssd/OntologyRequirements#CalendarMinute -->

    <owl:Class rdf:about="&or;CalendarMinute">
        <rdfs:subClassOf rdf:resource="&or;DateTime"/>
        <owl:disjointWith rdf:resource="&or;CalendarMonth"/>
        <owl:disjointWith rdf:resource="&or;CalendarNanosecond"/>
        <owl:disjointWith rdf:resource="&or;CalendarWeek"/>
        <owl:disjointWith rdf:resource="&or;CalendarYear"/>
        <rdfs:comment xml:lang="en">A specialization  of Date  Time, Calendar Minute is the class of 60-second periods that make up the calendar.  9:53 AM GMT on May 4, 2013 is an instance of Calendar Minute, while the 60-second interval from 9:53:16 through 9:54:15 of the same day is not.

Each Calendar Minute is divided into sixty contiguous Calendar Seconds. Note that a given instance of Calendar Minute is a temporally continuous individual that occurs only once.

Same as cyc:CalendarMinute.</rdfs:comment>
    </owl:Class>
    


    <!-- http://www.nist.gov/itl/ssd/OntologyRequirements#CalendarMonth -->

    <owl:Class rdf:about="&or;CalendarMonth">
        <rdfs:subClassOf rdf:resource="&or;DateTime"/>
        <owl:disjointWith rdf:resource="&or;CalendarNanosecond"/>
        <owl:disjointWith rdf:resource="&or;CalendarWeek"/>
        <owl:disjointWith rdf:resource="&or;CalendarYear"/>
        <rdfs:comment xml:lang="en">A specialization of DateTime. Each instance of CalendarMonth is a month in a particular calendar, and as such have durations ranging from 28 to 31 days. An example sub-collection of CalendarMonth is February, the collection of all months of February. One instance of the collection February (and thus one instance of the collection CalendarMonth) is February of 2012.</rdfs:comment>
    </owl:Class>
    


    <!-- http://www.nist.gov/itl/ssd/OntologyRequirements#CalendarNanosecond -->

    <owl:Class rdf:about="&or;CalendarNanosecond">
        <rdfs:subClassOf rdf:resource="&or;DateTime"/>
        <owl:disjointWith rdf:resource="&or;CalendarWeek"/>
        <owl:disjointWith rdf:resource="&or;CalendarYear"/>
        <rdfs:comment xml:lang="en">A specialization  of Date  Time, Calendar Nanosecond is the class of  one nanosecond periods that make up the calendar.  Each Calendar Millisecond divided into one thousand contiguous Calendar Nanoseconds. Note that a given instance of Calendar Nanosecond is a temporally continuous individual that occurs only once.</rdfs:comment>
    </owl:Class>
    


    <!-- http://www.nist.gov/itl/ssd/OntologyRequirements#CalendarWeek -->

    <owl:Class rdf:about="&or;CalendarWeek">
        <rdfs:subClassOf rdf:resource="&or;DateTime"/>
        <owl:disjointWith rdf:resource="&or;CalendarYear"/>
        <rdfs:comment xml:lang="en">A specialization  of Date  Time, Calendar Week is the class of 7-day intervals that make up some calendar. Each Calendar Week is divided into seven contiguous Calendar Days. Note that a given instance of Calendar Week is a temporally continuous individual that occurs only once.

Note that Calendar Weeks defined by different systems can overlap.  European calendars often define weeks as beginning with a Monday, while US calendars often define weeks as beginning with a Sunday.

Same as cyc:CalendarCentury.</rdfs:comment>
    </owl:Class>
    


    <!-- http://www.nist.gov/itl/ssd/OntologyRequirements#CalendarYear -->

    <owl:Class rdf:about="&or;CalendarYear">
        <rdfs:subClassOf rdf:resource="&or;DateTime"/>
        <rdfs:comment xml:lang="en">A specialization  of Date  Time, Calendar Year is the class of one year long periods that make up a calendar. The year 1953 on the Gregorian Calendar is an instance of Calendar Year, while the Time Interval from May 4, 1953s through May 3, 1954, is not.

Note that a given instance of Calendar Year is a temporally continuous individual that occurs only once. Note also, that due to leap years, different calendar years on the same calendar can have different durations.

Same as cyc:CalendarHour.</rdfs:comment>
    </owl:Class>
    


    <!-- http://www.nist.gov/itl/ssd/OntologyRequirements#Camera -->

    <owl:Class rdf:about="&or;Camera">
        <rdfs:subClassOf rdf:resource="&or;ImageInputDevice"/>
    </owl:Class>
    


    <!-- http://www.nist.gov/itl/ssd/OntologyRequirements#Certifying -->

    <owl:Class rdf:about="&or;Certifying">
        <rdfs:subClassOf rdf:resource="&or;PurposefulAction"/>
        <owl:disjointWith rdf:resource="&or;ComputerProcessExecution"/>
        <owl:disjointWith rdf:resource="&or;DataCollection"/>
        <owl:disjointWith rdf:resource="&or;DatabaseSearch"/>
        <owl:disjointWith rdf:resource="&or;DeployingAProduct"/>
        <owl:disjointWith rdf:resource="&or;Designing"/>
        <owl:disjointWith rdf:resource="&or;Development"/>
        <owl:disjointWith rdf:resource="&or;Evaluation"/>
        <owl:disjointWith rdf:resource="&or;Manufacturing"/>
        <owl:disjointWith rdf:resource="&or;Optimization"/>
        <owl:disjointWith rdf:resource="&or;Planning"/>
        <owl:disjointWith rdf:resource="&or;Recommending"/>
        <rdfs:comment xml:lang="en">Certifiction is the action of authoritatively attesting that something meets specified criteria.</rdfs:comment>
    </owl:Class>
    


    <!-- http://www.nist.gov/itl/ssd/OntologyRequirements#Computer -->

    <owl:Class rdf:about="&or;Computer">
        <rdfs:subClassOf rdf:resource="&or;PhysicalDevice"/>
        <rdfs:comment xml:lang="en">A Computer is an electronic device that acts on input according to some set of instructions (often in the form of software) producing some output. Instances of Computer have specialized parts to handle input and output, data storage, and processing.

Same as cyc:Computer.</rdfs:comment>
    </owl:Class>
    


    <!-- http://www.nist.gov/itl/ssd/OntologyRequirements#ComputerFile -->

    <owl:Class rdf:about="&or;ComputerFile">
        <rdfs:subClassOf rdf:resource="&or;DataObject"/>
        <rdfs:seeAlso>cyc:ComputerFile-AIS</rdfs:seeAlso>
        <rdfs:comment xml:lang="en">A Computer File is an abstract series of bits (qbits, etc.) encoding some information and conforming to some file system protocol. Any Computer File may be instantiated (e.g. on magnetic media) as an unlimited number of Computer File Copies.</rdfs:comment>
    </owl:Class>
    


    <!-- http://www.nist.gov/itl/ssd/OntologyRequirements#ComputerImageFile -->

    <owl:Class rdf:about="&or;ComputerImageFile">
        <rdfs:subClassOf rdf:resource="&or;ComputerFile"/>
        <owl:disjointWith rdf:resource="&or;VisualImage"/>
    </owl:Class>
    


    <!-- http://www.nist.gov/itl/ssd/OntologyRequirements#ComputerLanguage -->

    <owl:Class rdf:about="&or;ComputerLanguage">
        <rdfs:subClassOf rdf:resource="&or;Language"/>
        <rdfs:comment xml:lang="en">Computer Language is the collection of languages invented for the purpose of composing computer programs, for facilitating interaction between pieces of software, or for structuring data (including text).</rdfs:comment>
    </owl:Class>
    


    <!-- http://www.nist.gov/itl/ssd/OntologyRequirements#ComputerProcessExecution -->

    <owl:Class rdf:about="&or;ComputerProcessExecution">
        <rdfs:subClassOf rdf:resource="&or;PhysicalEvent"/>
        <rdfs:subClassOf rdf:resource="&or;PurposefulAction"/>
        <owl:disjointWith rdf:resource="&or;DeployingAProduct"/>
        <owl:disjointWith rdf:resource="&or;Designing"/>
        <owl:disjointWith rdf:resource="&or;Development"/>
        <owl:disjointWith rdf:resource="&or;Manufacturing"/>
        <owl:disjointWith rdf:resource="&or;Optimization"/>
        <owl:disjointWith rdf:resource="&or;Planning"/>
        <owl:disjointWith rdf:resource="&or;Recommending"/>
        <rdfs:comment xml:lang="en">Computer Process Execution is an event in which a Computer Program or Software Package is executed on a Computational System of one or more Computers, using the Computational System&#39;s resources. &#39;Process&#39; here refers to the act of a CPU or multiple CPUs executing the instructions in a Computer Program Copy. A process ends when it is terminated (by its own instructions, the operating system, a power outage, etc.) A Computer Process Execution can be suspended or swapped out by an Operating System (whereupon it temporarily ceases to exist) but when and if it is swapped back in, it will still be the same Computer Process Execution. Hence, the time during which a Computer Process Execution exists can be a discontinuous time interval.</rdfs:comment>
    </owl:Class>
    


    <!-- http://www.nist.gov/itl/ssd/OntologyRequirements#ComputerProgram -->

    <owl:Class rdf:about="&or;ComputerProgram">
        <rdfs:subClassOf rdf:resource="&or;Software"/>
        <owl:disjointWith rdf:resource="&or;SoftwarePackage"/>
        <owl:disjointWith rdf:resource="&or;SoftwareSubroutine"/>
        <rdfs:comment xml:lang="en">A Computer Program is a deliberately created abstract object composed of propositions that together constitute a list of instructions for computers to execute. 

The same program can be instantiated in both a high-level computer language and different binary forms that execute on different makes of computer.  Multiple copies of the same program can reside on different storage devices (hard disk, CD) and be accessible at different locations (both on the WWW and a local machine).  These  various instantiations and copies are related to a Computer Program, but they are not what is meant by the term.

Same as cyc:ComputerProgram-CW .</rdfs:comment>
    </owl:Class>
    


    <!-- http://www.nist.gov/itl/ssd/OntologyRequirements#ComputerStorageCapacity -->

    <owl:Class rdf:about="&or;ComputerStorageCapacity">
        <owl:equivalentClass>
            <owl:Class>
                <owl:intersectionOf rdf:parseType="Collection">
                    <rdf:Description rdf:about="&or;MeasurableQuantity"/>
                    <owl:Restriction>
                        <owl:onProperty rdf:resource="&or;unitsFor"/>
                        <owl:someValuesFrom rdf:resource="&or;UnitOfComputerStorageCapacity"/>
                    </owl:Restriction>
                </owl:intersectionOf>
            </owl:Class>
        </owl:equivalentClass>
        <rdfs:subClassOf rdf:resource="&or;MeasurableQuantity"/>
        <rdfs:subClassOf>
            <owl:Restriction>
                <owl:onProperty rdf:resource="&or;unitsFor"/>
                <owl:allValuesFrom rdf:resource="&or;UnitOfComputerStorageCapacity"/>
            </owl:Restriction>
        </rdfs:subClassOf>
        <owl:disjointWith rdf:resource="&or;Count"/>
        <owl:disjointWith rdf:resource="&or;Distance"/>
        <owl:disjointWith rdf:resource="&or;Duration"/>
        <owl:disjointWith rdf:resource="&or;Energy"/>
        <owl:disjointWith rdf:resource="&or;Force"/>
        <owl:disjointWith rdf:resource="&or;Mass"/>
        <owl:disjointWith rdf:resource="&or;Pressure"/>
        <owl:disjointWith rdf:resource="&or;Temperature"/>
        <owl:disjointWith rdf:resource="&or;Volume"/>
    </owl:Class>
    


    <!-- http://www.nist.gov/itl/ssd/OntologyRequirements#ConceptualModel -->

    <owl:Class rdf:about="&or;ConceptualModel">
        <rdfs:subClassOf rdf:resource="&or;AbstractStructuredInformationStore"/>
        <rdfs:comment xml:lang="en">A Conceptual Model is a non-physical model of a situation, activity, or structure of some (normally complex) thing.</rdfs:comment>
    </owl:Class>
    


    <!-- http://www.nist.gov/itl/ssd/OntologyRequirements#Count -->

    <owl:Class rdf:about="&or;Count">
        <rdfs:subClassOf rdf:resource="&or;MeasurableQuantity"/>
        <rdfs:subClassOf>
            <owl:Restriction>
                <owl:onProperty rdf:resource="&or;unitsFor"/>
                <owl:allValuesFrom rdf:resource="&or;DimensionlessUnit"/>
            </owl:Restriction>
        </rdfs:subClassOf>
        <owl:disjointWith rdf:resource="&or;Distance"/>
        <owl:disjointWith rdf:resource="&or;Duration"/>
        <owl:disjointWith rdf:resource="&or;Energy"/>
        <owl:disjointWith rdf:resource="&or;Force"/>
        <owl:disjointWith rdf:resource="&or;Mass"/>
        <owl:disjointWith rdf:resource="&or;Pressure"/>
        <owl:disjointWith rdf:resource="&or;Temperature"/>
        <owl:disjointWith rdf:resource="&or;Volume"/>
        <rdfs:comment xml:lang="en">A Count is a quantity that can be expressed in integers or some multiple of 1 such as moles.</rdfs:comment>
    </owl:Class>
    


    <!-- http://www.nist.gov/itl/ssd/OntologyRequirements#CreatedThing -->

    <owl:Class rdf:about="&or;CreatedThing">
        <rdfs:subClassOf rdf:resource="&or;TemporalThing"/>
        <owl:disjointWith rdf:resource="&or;Curve"/>
    </owl:Class>
    


    <!-- http://www.nist.gov/itl/ssd/OntologyRequirements#CreationEvent -->

    <owl:Class rdf:about="&or;CreationEvent">
        <rdfs:subClassOf rdf:resource="&or;Event"/>
        <rdfs:comment xml:lang="en">A Creation Event is an Event in which something comes into existence.</rdfs:comment>
    </owl:Class>
    


    <!-- http://www.nist.gov/itl/ssd/OntologyRequirements#CurrencyUnit -->

    <owl:Class rdf:about="&or;CurrencyUnit">
        <rdfs:subClassOf rdf:resource="&or;NonMetricUnit"/>
        <owl:disjointWith rdf:resource="&or;DimensionlessUnit"/>
        <owl:disjointWith rdf:resource="&or;MetricUnit"/>
        <owl:disjointWith rdf:resource="&or;UnitOfAcceleration"/>
        <owl:disjointWith rdf:resource="&or;UnitOfArea"/>
        <owl:disjointWith rdf:resource="&or;UnitOfComputerStorageCapacity"/>
        <owl:disjointWith rdf:resource="&or;UnitOfDensity"/>
        <owl:disjointWith rdf:resource="&or;UnitOfDistance"/>
        <owl:disjointWith rdf:resource="&or;UnitOfDuration"/>
        <owl:disjointWith rdf:resource="&or;UnitOfEnergy"/>
        <owl:disjointWith rdf:resource="&or;UnitOfForce"/>
        <owl:disjointWith rdf:resource="&or;UnitOfMass"/>
        <owl:disjointWith rdf:resource="&or;UnitOfPressure"/>
        <owl:disjointWith rdf:resource="&or;UnitOfSpreadRate"/>
        <owl:disjointWith rdf:resource="&or;UnitOfTemperature"/>
        <owl:disjointWith rdf:resource="&or;UnitOfVelocity"/>
        <owl:disjointWith rdf:resource="&or;UnitOfVoltage"/>
        <owl:disjointWith rdf:resource="&or;UnitOfVolume"/>
        <rdfs:comment xml:lang="en">A unit of currency such as Euro, USDollar, ChineseYuan, EuroCent, and USCent.See subclasses PrimaryCurrencyUnit and SecondaryCurrencyUnit to distinuish the basic unit (e.g., Euro) from secondary units (e.g., EuroCent).</rdfs:comment>
    </owl:Class>
    


    <!-- http://www.nist.gov/itl/ssd/OntologyRequirements#Curve -->

    <owl:Class rdf:about="&or;Curve">
        <rdfs:subClassOf rdf:resource="&or;NonTangibleThing"/>
        <rdfs:subClassOf rdf:resource="&or;SpatialThing"/>
        <owl:disjointWith rdf:resource="&or;Event"/>
        <owl:disjointWith rdf:resource="&or;FirstOrderClass"/>
        <owl:disjointWith rdf:resource="&or;Quantity"/>
        <owl:disjointWith rdf:resource="&or;StateOfBeing"/>
        <owl:disjointWith rdf:resource="&or;StructuredInformationStore"/>
        <owl:disjointWith rdf:resource="&or;TimeInterval"/>
        <owl:disjointWith rdf:resource="&or;UnitOfMeasure"/>
        <rdfs:comment xml:lang="en">A Curve is a continuous one-dimensional line passing through three dimensions.  It may be straight or curved.  It may have points at which its direction changes abruptly. It may close in upon itself or be open.  It may be finte or effectively infinite. Curves can be drawn or calculated, but they are not created.</rdfs:comment>
    </owl:Class>
    


    <!-- http://www.nist.gov/itl/ssd/OntologyRequirements#CurveSegment -->

    <owl:Class rdf:about="&or;CurveSegment">
        <rdfs:subClassOf rdf:resource="&or;Curve"/>
        <rdfs:comment xml:lang="en">A Curve Segment is a curve with two end points.</rdfs:comment>
    </owl:Class>
    


    <!-- http://www.nist.gov/itl/ssd/OntologyRequirements#DataBase -->

    <owl:Class rdf:about="&or;DataBase">
        <rdfs:subClassOf rdf:resource="&or;DataObject"/>
    </owl:Class>
    


    <!-- http://www.nist.gov/itl/ssd/OntologyRequirements#DataCollection -->

    <owl:Class rdf:about="&or;DataCollection">
        <rdfs:subClassOf rdf:resource="&or;CreationEvent"/>
        <rdfs:subClassOf>
            <owl:Restriction>
                <owl:onProperty rdf:resource="&or;outputCreated"/>
                <owl:someValuesFrom rdf:resource="&or;DataObject"/>
            </owl:Restriction>
        </rdfs:subClassOf>
        <owl:disjointWith rdf:resource="&or;Evaluation"/>
        <owl:disjointWith rdf:resource="&or;Recommending"/>
        <rdfs:comment xml:lang="en">Data Collection is the event of data being collected.  This includes collection by an activated sensor or the intentional collection of information by a person.  The output created by a Data Collection event is one or more Data Objects.</rdfs:comment>
    </owl:Class>
    


    <!-- http://www.nist.gov/itl/ssd/OntologyRequirements#DataFormat -->

    <owl:Class rdf:about="&or;DataFormat">
        <rdfs:subClassOf rdf:resource="&or;AbstractStructuredInformationStore"/>
        <rdfs:comment xml:lang="en">A data format is a preestablished layout for electronic data.  This includes formats for computer files, electronic messages, program I/O, and data base fields.</rdfs:comment>
    </owl:Class>
    


    <!-- http://www.nist.gov/itl/ssd/OntologyRequirements#DataGenerationTool -->

    <owl:Class rdf:about="&or;DataGenerationTool">
        <rdfs:subClassOf rdf:resource="&or;Software"/>
    </owl:Class>
    


    <!-- http://www.nist.gov/itl/ssd/OntologyRequirements#DataInputDevice -->

    <owl:Class rdf:about="&or;DataInputDevice">
        <rdfs:subClassOf rdf:resource="&or;PhysicalDevice"/>
    </owl:Class>
    


    <!-- http://www.nist.gov/itl/ssd/OntologyRequirements#DataObject -->

    <owl:Class rdf:about="&or;DataObject">
        <rdfs:subClassOf rdf:resource="&or;AbstractStructuredInformationStore"/>
        <owl:disjointWith rdf:resource="&or;Event"/>
    </owl:Class>
    


    <!-- http://www.nist.gov/itl/ssd/OntologyRequirements#DataOutputDevice -->

    <owl:Class rdf:about="&or;DataOutputDevice">
        <rdfs:subClassOf rdf:resource="&or;PhysicalDevice"/>
        <rdfs:comment xml:lang="en">A Data Output Device is an ElectronicDevice which delivers information from a computer to a user or external equipment.</rdfs:comment>
    </owl:Class>
    


    <!-- http://www.nist.gov/itl/ssd/OntologyRequirements#DataRepository -->

    <owl:Class rdf:about="&or;DataRepository">
        <rdfs:subClassOf rdf:resource="&or;DataObject"/>
    </owl:Class>
    


    <!-- http://www.nist.gov/itl/ssd/OntologyRequirements#DataStorageAndGenerationTool -->

    <owl:Class rdf:about="&or;DataStorageAndGenerationTool">
        <owl:equivalentClass>
            <owl:Class>
                <owl:intersectionOf rdf:parseType="Collection">
                    <rdf:Description rdf:about="&or;DataGenerationTool"/>
                    <rdf:Description rdf:about="&or;DataStorageTool"/>
                </owl:intersectionOf>
            </owl:Class>
        </owl:equivalentClass>
        <rdfs:subClassOf rdf:resource="&or;DataStorageTool"/>
    </owl:Class>
    


    <!-- http://www.nist.gov/itl/ssd/OntologyRequirements#DataStorageTool -->

    <owl:Class rdf:about="&or;DataStorageTool">
        <rdfs:subClassOf rdf:resource="&or;Software"/>
    </owl:Class>
    


    <!-- http://www.nist.gov/itl/ssd/OntologyRequirements#DataTable -->

    <owl:Class rdf:about="&or;DataTable">
        <rdfs:subClassOf rdf:resource="&or;DataObject"/>
    </owl:Class>
    


    <!-- http://www.nist.gov/itl/ssd/OntologyRequirements#DatabaseSearch -->

    <owl:Class rdf:about="&or;DatabaseSearch">
        <rdfs:subClassOf rdf:resource="&or;PurposefulAction"/>
        <owl:disjointWith rdf:resource="&or;DeployingAProduct"/>
        <owl:disjointWith rdf:resource="&or;Designing"/>
        <owl:disjointWith rdf:resource="&or;Development"/>
        <owl:disjointWith rdf:resource="&or;Manufacturing"/>
        <owl:disjointWith rdf:resource="&or;Optimization"/>
        <owl:disjointWith rdf:resource="&or;Planning"/>
        <owl:disjointWith rdf:resource="&or;Recommending"/>
    </owl:Class>
    


    <!-- http://www.nist.gov/itl/ssd/OntologyRequirements#DateTime -->

    <owl:Class rdf:about="&or;DateTime">
        <rdfs:subClassOf rdf:resource="&or;TimeInterval"/>
        <rdfs:comment xml:lang="en">A continuous Time Interval of any resolution (from nanosecond to millenium -- and beyond in both directions) that can be referred to as a standardly-defined location on particular calendar, without specifying a range. The interval is a standard unit of time (with respect to some calendar) whose start and end times can be specified in whole-number multiples of that and larger units. Thus the midnight hour GMT on 1 January 2000 CE is a Date-Time; but neither the five-hour-long Time Interval between midnight and 5:00 AM GMT nor the hour-long Time Interval between 12:15 and 1:15 AM GMT on that same day are Date-Times. 

Same as cyc:Date .</rdfs:comment>
    </owl:Class>
    


    <!-- http://www.nist.gov/itl/ssd/OntologyRequirements#December -->

    <owl:Class rdf:about="&or;December">
        <rdfs:subClassOf rdf:resource="&or;CalendarMonth"/>
        <rdfs:comment xml:lang="en">The month of December</rdfs:comment>
    </owl:Class>
    


    <!-- http://www.nist.gov/itl/ssd/OntologyRequirements#DeployingAProduct -->

    <owl:Class rdf:about="&or;DeployingAProduct">
        <rdfs:subClassOf rdf:resource="&or;PurposefulAction"/>
        <owl:disjointWith rdf:resource="&or;Designing"/>
        <owl:disjointWith rdf:resource="&or;Development"/>
        <owl:disjointWith rdf:resource="&or;Evaluation"/>
        <owl:disjointWith rdf:resource="&or;Manufacturing"/>
        <owl:disjointWith rdf:resource="&or;Optimization"/>
        <owl:disjointWith rdf:resource="&or;Planning"/>
        <owl:disjointWith rdf:resource="&or;Recommending"/>
        <rdfs:comment xml:lang="en">To Deploy a product is to distribute a product so that it can be provided to end users.  Before a product can be deployed, it has to have been designed and, if a physical product, manufactured.</rdfs:comment>
    </owl:Class>
    


    <!-- http://www.nist.gov/itl/ssd/OntologyRequirements#Design -->

    <owl:Class rdf:about="&or;Design">
        <rdfs:subClassOf rdf:resource="&or;ConceptualModel"/>
        <rdfs:comment xml:lang="en">A Design is a Conceptual Model of how something should be: how a product should be structured, how a product should be produced, how an experiment should be run, etc.  The thing that the design is for may be a physical artifact, a type of process, a specific action, </rdfs:comment>
    </owl:Class>
    


    <!-- http://www.nist.gov/itl/ssd/OntologyRequirements#DesignMethod -->

    <owl:Class rdf:about="&or;DesignMethod">
        <rdfs:subClassOf rdf:resource="&or;Technique"/>
        <owl:disjointWith rdf:resource="&or;PredictionMethod"/>
        <rdfs:comment xml:lang="en">A Design Method is a Technique for designing some type of thing.</rdfs:comment>
    </owl:Class>
    


    <!-- http://www.nist.gov/itl/ssd/OntologyRequirements#Designing -->

    <owl:Class rdf:about="&or;Designing">
        <rdfs:subClassOf rdf:resource="&or;IntentionalCreation"/>
        <rdfs:subClassOf>
            <owl:Restriction>
                <owl:onProperty rdf:resource="&or;outputCreated"/>
                <owl:someValuesFrom rdf:resource="&or;Design"/>
            </owl:Restriction>
        </rdfs:subClassOf>
        <owl:disjointWith rdf:resource="&or;Development"/>
        <owl:disjointWith rdf:resource="&or;Manufacturing"/>
        <owl:disjointWith rdf:resource="&or;Optimization"/>
        <rdfs:comment xml:lang="en">The act of designing something, whether physical object (e.g., computer chip), physical stuff (e.g., an alloy), or a conceptual thing such as a law or algorithm.</rdfs:comment>
    </owl:Class>
    


    <!-- http://www.nist.gov/itl/ssd/OntologyRequirements#Development -->

    <owl:Class rdf:about="&or;Development">
        <rdfs:subClassOf rdf:resource="&or;IntentionalCreation"/>
        <owl:disjointWith rdf:resource="&or;Manufacturing"/>
        <owl:disjointWith rdf:resource="&or;Optimization"/>
        <owl:disjointWith rdf:resource="&or;Planning"/>
        <rdfs:comment xml:lang="en">Development is a type of action in which one or more people thinks up a thing, and maybe prototype it. Sometimes this involves designing a specification for the thing as well as coming up with a specification for how to produce more of them. </rdfs:comment>
    </owl:Class>
    


    <!-- http://www.nist.gov/itl/ssd/OntologyRequirements#DiagonalArray -->

    <owl:Class rdf:about="&or;DiagonalArray">
        <rdfs:subClassOf rdf:resource="&or;Array"/>
        <rdfs:comment xml:lang="en">A Diagonal Array is an array of dimension two or higher, with length, width, height, etc. equal, and with the only non-zero (or non-blank) cells being on the diagonal.</rdfs:comment>
    </owl:Class>
    


    <!-- http://www.nist.gov/itl/ssd/OntologyRequirements#DimensionlessUnit -->

    <owl:Class rdf:about="&or;DimensionlessUnit">
        <rdfs:subClassOf rdf:resource="&or;UnitOfMeasure"/>
        <owl:disjointWith rdf:resource="&or;MetricUnit"/>
        <owl:disjointWith rdf:resource="&or;UnitOfAcceleration"/>
        <owl:disjointWith rdf:resource="&or;UnitOfArea"/>
        <owl:disjointWith rdf:resource="&or;UnitOfComputerStorageCapacity"/>
        <owl:disjointWith rdf:resource="&or;UnitOfDensity"/>
        <owl:disjointWith rdf:resource="&or;UnitOfDistance"/>
        <owl:disjointWith rdf:resource="&or;UnitOfDuration"/>
        <owl:disjointWith rdf:resource="&or;UnitOfEnergy"/>
        <owl:disjointWith rdf:resource="&or;UnitOfForce"/>
        <owl:disjointWith rdf:resource="&or;UnitOfMass"/>
        <owl:disjointWith rdf:resource="&or;UnitOfPressure"/>
        <owl:disjointWith rdf:resource="&or;UnitOfSpreadRate"/>
        <owl:disjointWith rdf:resource="&or;UnitOfTemperature"/>
        <owl:disjointWith rdf:resource="&or;UnitOfVelocity"/>
        <owl:disjointWith rdf:resource="&or;UnitOfVelocitySquared"/>
        <owl:disjointWith rdf:resource="&or;UnitOfVoltage"/>
        <owl:disjointWith rdf:resource="&or;UnitOfVolume"/>
        <rdfs:comment xml:lang="en">A Dimensionless Unit is a Unit of Measure that is a multiple of one.  100 Percent = 1 Unity = Avogadro&#39;s Number / ( 6.03 * 10^23).</rdfs:comment>
    </owl:Class>
    


    <!-- http://www.nist.gov/itl/ssd/OntologyRequirements#Distance -->

    <owl:Class rdf:about="&or;Distance">
        <owl:equivalentClass>
            <owl:Class>
                <owl:intersectionOf rdf:parseType="Collection">
                    <rdf:Description rdf:about="&or;MeasurableQuantity"/>
                    <owl:Restriction>
                        <owl:onProperty rdf:resource="&or;unitsFor"/>
                        <owl:someValuesFrom rdf:resource="&or;UnitOfDistance"/>
                    </owl:Restriction>
                </owl:intersectionOf>
            </owl:Class>
        </owl:equivalentClass>
        <rdfs:subClassOf rdf:resource="&or;MeasurableQuantity"/>
        <rdfs:subClassOf>
            <owl:Restriction>
                <owl:onProperty rdf:resource="&or;unitsFor"/>
                <owl:allValuesFrom rdf:resource="&or;UnitOfDistance"/>
            </owl:Restriction>
        </rdfs:subClassOf>
        <owl:disjointWith rdf:resource="&or;Duration"/>
        <owl:disjointWith rdf:resource="&or;Energy"/>
        <owl:disjointWith rdf:resource="&or;Force"/>
        <owl:disjointWith rdf:resource="&or;Mass"/>
        <owl:disjointWith rdf:resource="&or;Pressure"/>
        <owl:disjointWith rdf:resource="&or;Temperature"/>
        <owl:disjointWith rdf:resource="&or;Volume"/>
    </owl:Class>
    


    <!-- http://www.nist.gov/itl/ssd/OntologyRequirements#Duration -->

    <owl:Class rdf:about="&or;Duration">
        <owl:equivalentClass>
            <owl:Class>
                <owl:intersectionOf rdf:parseType="Collection">
                    <rdf:Description rdf:about="&or;MeasurableQuantity"/>
                    <owl:Restriction>
                        <owl:onProperty rdf:resource="&or;unitsFor"/>
                        <owl:someValuesFrom rdf:resource="&or;UnitOfDuration"/>
                    </owl:Restriction>
                </owl:intersectionOf>
            </owl:Class>
        </owl:equivalentClass>
        <rdfs:subClassOf rdf:resource="&or;MeasurableQuantity"/>
        <rdfs:subClassOf>
            <owl:Restriction>
                <owl:onProperty rdf:resource="&or;unitsFor"/>
                <owl:allValuesFrom rdf:resource="&or;UnitOfDuration"/>
            </owl:Restriction>
        </rdfs:subClassOf>
        <owl:disjointWith rdf:resource="&or;Energy"/>
        <owl:disjointWith rdf:resource="&or;Force"/>
        <owl:disjointWith rdf:resource="&or;Mass"/>
        <owl:disjointWith rdf:resource="&or;Pressure"/>
        <owl:disjointWith rdf:resource="&or;Temperature"/>
        <owl:disjointWith rdf:resource="&or;Volume"/>
        <rdfs:comment xml:lang="en">Each instance of Duration is a physical quantity, corresponding to a certain ``amount of time&#39; &#39;, that a TemporalThing exists, occurs over, or endures.

Same as cyc:Time-Quantity.</rdfs:comment>
    </owl:Class>
    


    <!-- http://www.nist.gov/itl/ssd/OntologyRequirements#ElectronicFileFormat -->

    <owl:Class rdf:about="&or;ElectronicFileFormat">
        <rdfs:subClassOf rdf:resource="&or;DataFormat"/>
        <rdfs:comment xml:lang="en">An Electronic File Format is a Data Format that is specific for Computer Files.</rdfs:comment>
    </owl:Class>
    


    <!-- http://www.nist.gov/itl/ssd/OntologyRequirements#Energy -->

    <owl:Class rdf:about="&or;Energy">
        <owl:equivalentClass>
            <owl:Class>
                <owl:intersectionOf rdf:parseType="Collection">
                    <rdf:Description rdf:about="&or;MeasurableQuantity"/>
                    <owl:Restriction>
                        <owl:onProperty rdf:resource="&or;unitsFor"/>
                        <owl:someValuesFrom rdf:resource="&or;UnitOfEnergy"/>
                    </owl:Restriction>
                </owl:intersectionOf>
            </owl:Class>
        </owl:equivalentClass>
        <rdfs:subClassOf rdf:resource="&or;MeasurableQuantity"/>
        <rdfs:subClassOf>
            <owl:Restriction>
                <owl:onProperty rdf:resource="&or;unitsFor"/>
                <owl:allValuesFrom rdf:resource="&or;UnitOfEnergy"/>
            </owl:Restriction>
        </rdfs:subClassOf>
        <owl:disjointWith rdf:resource="&or;Force"/>
        <owl:disjointWith rdf:resource="&or;Pressure"/>
        <owl:disjointWith rdf:resource="&or;Temperature"/>
        <owl:disjointWith rdf:resource="&or;Volume"/>
    </owl:Class>
    


    <!-- http://www.nist.gov/itl/ssd/OntologyRequirements#Equation -->

    <owl:Class rdf:about="&or;Equation">
        <rdfs:subClassOf rdf:resource="&or;MathematicalFormula"/>
        <rdfs:comment xml:lang="en">An Equation is a mathematical statement that two Mathematical Expressions are equal.</rdfs:comment>
    </owl:Class>
    


    <!-- http://www.nist.gov/itl/ssd/OntologyRequirements#Evaluation -->

    <owl:Class rdf:about="&or;Evaluation">
        <rdfs:subClassOf rdf:resource="&or;PurposefulAction"/>
        <owl:disjointWith rdf:resource="&or;MechanicalProcess"/>
        <owl:disjointWith rdf:resource="&or;MovementEvent"/>
        <owl:disjointWith rdf:resource="&or;Planning"/>
        <owl:disjointWith rdf:resource="&or;Recommending"/>
        <rdfs:comment xml:lang="en">Evaluation is the action of evaluating one or more qualities of something.</rdfs:comment>
    </owl:Class>
    


    <!-- http://www.nist.gov/itl/ssd/OntologyRequirements#Event -->

    <owl:Class rdf:about="&or;Event">
        <rdfs:subClassOf rdf:resource="&or;NonTangibleThing"/>
        <rdfs:subClassOf rdf:resource="&or;TemporalThing"/>
        <owl:disjointWith rdf:resource="&or;FieldOfStudy"/>
        <owl:disjointWith rdf:resource="&or;Language"/>
        <owl:disjointWith rdf:resource="&or;LogicalRule"/>
        <owl:disjointWith rdf:resource="&or;Metadata"/>
        <owl:disjointWith rdf:resource="&or;Organization"/>
        <owl:disjointWith rdf:resource="&or;Quantity"/>
        <owl:disjointWith rdf:resource="&or;RuleSet"/>
        <owl:disjointWith rdf:resource="&or;Software"/>
        <owl:disjointWith rdf:resource="&or;SpatialFrameOfReference"/>
        <owl:disjointWith rdf:resource="&or;StateOfBeing"/>
        <owl:disjointWith rdf:resource="&or;StructuredInformationStore"/>
        <owl:disjointWith rdf:resource="&or;Technique"/>
        <owl:disjointWith rdf:resource="&or;TimeInterval"/>
        <owl:disjointWith rdf:resource="&or;UnitOfMeasure"/>
        <rdfs:comment xml:lang="en">Each instance of Event is a dynamic situation in which the state of the world changes; each instance is something one would say &#39;happens&#39;.  See cyc:Event.</rdfs:comment>
    </owl:Class>
    


    <!-- http://www.nist.gov/itl/ssd/OntologyRequirements#EventSeries -->

    <owl:Class rdf:about="&or;EventSeries">
        <rdfs:subClassOf rdf:resource="&or;Event"/>
        <rdfs:comment xml:lang="en">An event series, such as a conference series, bi-annual elections, winter olympics, publications of journal issues, and a person&#39;s heartbeats.</rdfs:comment>
    </owl:Class>
    


    <!-- http://www.nist.gov/itl/ssd/OntologyRequirements#EventType -->

    <owl:Class rdf:about="&or;EventType">
        <rdfs:subClassOf rdf:resource="&or;FirstOrderClass"/>
        <owl:disjointWith rdf:resource="&or;InterconvertibleUnitType"/>
        <owl:disjointWith rdf:resource="&or;MeasurableQuantityType"/>
        <owl:disjointWith rdf:resource="&or;ObjectType"/>
        <rdfs:comment xml:lang="en">Each instance of InterconvertibleUnitType is a subclass of UnitOfMeasure, such   that quantities expressed using one of the units may also be expressed using any other unit in that subclass. 

Examples of InterconvertibleUnitTypes include UnitOfTime, UnitOfDistance and UnitOfComputerStorageCapacity. Thus, UnitOfTime includes HoursDuration and MinutesDuration, and any duration denoted as a quantity of HoursDuration can be expressed as a (different) quantity of MinutesDurationand vice versa.. </rdfs:comment>
    </owl:Class>
    


    <!-- http://www.nist.gov/itl/ssd/OntologyRequirements#ExperimentPlanning -->

    <owl:Class rdf:about="&or;ExperimentPlanning">
        <rdfs:subClassOf rdf:resource="&or;Planning"/>
    </owl:Class>
    


    <!-- http://www.nist.gov/itl/ssd/OntologyRequirements#ExpressedQuantity -->

    <owl:Class rdf:about="&or;ExpressedQuantity">
        <rdfs:subClassOf rdf:resource="&or;MeasurableQuantity"/>
        <rdfs:subClassOf>
            <owl:Restriction>
                <owl:onProperty rdf:resource="&or;unitsFor"/>
                <owl:onClass rdf:resource="&or;UnitOfMeasure"/>
                <owl:qualifiedCardinality rdf:datatype="&xsd;nonNegativeInteger">1</owl:qualifiedCardinality>
            </owl:Restriction>
        </rdfs:subClassOf>
    </owl:Class>
    


    <!-- http://www.nist.gov/itl/ssd/OntologyRequirements#February -->

    <owl:Class rdf:about="&or;February">
        <rdfs:subClassOf rdf:resource="&or;CalendarMonth"/>
        <rdfs:comment xml:lang="en">The month of February</rdfs:comment>
    </owl:Class>
    


    <!-- http://www.nist.gov/itl/ssd/OntologyRequirements#FieldOfStudy -->

    <owl:Class rdf:about="&or;FieldOfStudy">
        <rdfs:subClassOf rdf:resource="&or;IntangibleCreatedThing"/>
        <owl:disjointWith rdf:resource="&or;FirstOrderClass"/>
        <owl:disjointWith rdf:resource="&or;Image"/>
        <owl:disjointWith rdf:resource="&or;IntelligentAgent"/>
        <owl:disjointWith rdf:resource="&or;Language"/>
        <owl:disjointWith rdf:resource="&or;LogicalRule"/>
        <owl:disjointWith rdf:resource="&or;Metadata"/>
        <owl:disjointWith rdf:resource="&or;Quantity"/>
        <owl:disjointWith rdf:resource="&or;RuleSet"/>
        <owl:disjointWith rdf:resource="&or;Software"/>
        <owl:disjointWith rdf:resource="&or;SpatialThing"/>
        <owl:disjointWith rdf:resource="&or;StructuredInformationStore"/>
        <owl:disjointWith rdf:resource="&or;Technique"/>
        <owl:disjointWith rdf:resource="&or;UnitOfMeasure"/>
    </owl:Class>
    


    <!-- http://www.nist.gov/itl/ssd/OntologyRequirements#FirstOrderClass -->

    <owl:Class rdf:about="&or;FirstOrderClass">
        <rdfs:subClassOf rdf:resource="&or;NonTangibleThing"/>
        <owl:disjointWith rdf:resource="&or;Information"/>
        <owl:disjointWith rdf:resource="&or;Language"/>
        <owl:disjointWith rdf:resource="&or;LogicalRule"/>
        <owl:disjointWith rdf:resource="&or;Quantity"/>
        <owl:disjointWith rdf:resource="&or;RuleSet"/>
        <owl:disjointWith rdf:resource="&or;Software"/>
        <owl:disjointWith rdf:resource="&or;SpatialThing"/>
        <owl:disjointWith rdf:resource="&or;TemporalThing"/>
        <owl:disjointWith rdf:resource="&or;UnitOfMeasure"/>
        <rdfs:comment xml:lang="en">First Order Classes are metaclasses that have as instances classes which are not metaclasses.  For example, Species and Cell Type have as instances, not individual animals and cells, but TYPES of animals and cells.</rdfs:comment>
    </owl:Class>
    


    <!-- http://www.nist.gov/itl/ssd/OntologyRequirements#FlowChart -->

    <owl:Class rdf:about="&or;FlowChart">
        <rdfs:subClassOf rdf:resource="&or;GraphicalImage"/>
    </owl:Class>
    


    <!-- http://www.nist.gov/itl/ssd/OntologyRequirements#Force -->

    <owl:Class rdf:about="&or;Force">
        <owl:equivalentClass>
            <owl:Class>
                <owl:intersectionOf rdf:parseType="Collection">
                    <rdf:Description rdf:about="&or;MeasurableQuantity"/>
                    <owl:Restriction>
                        <owl:onProperty rdf:resource="&or;unitsFor"/>
                        <owl:someValuesFrom rdf:resource="&or;UnitOfForce"/>
                    </owl:Restriction>
                </owl:intersectionOf>
            </owl:Class>
        </owl:equivalentClass>
        <rdfs:subClassOf rdf:resource="&or;MeasurableQuantity"/>
        <rdfs:subClassOf>
            <owl:Restriction>
                <owl:onProperty rdf:resource="&or;unitsFor"/>
                <owl:allValuesFrom rdf:resource="&or;UnitOfForce"/>
            </owl:Restriction>
        </rdfs:subClassOf>
        <owl:disjointWith rdf:resource="&or;Mass"/>
        <owl:disjointWith rdf:resource="&or;Pressure"/>
        <owl:disjointWith rdf:resource="&or;Temperature"/>
        <owl:disjointWith rdf:resource="&or;Volume"/>
        <rdfs:comment xml:lang="en">Force is the agency by which change is produced.  In mechanics, a force on a free object yields an acceleration equal to the force divided by the mass of the object (F = mA). Physics recognizes five basic forces: gravitational, weak, electrical, magnetic, and strong forces, with electrical and magnetic forces unified.</rdfs:comment>
    </owl:Class>
    


    <!-- http://www.nist.gov/itl/ssd/OntologyRequirements#GenericProperty -->

    <owl:Class rdf:about="&or;GenericProperty">
        <rdfs:subClassOf rdf:resource="&or;NonTangibleThing"/>
        <owl:disjointWith rdf:resource="&or;StateOfBeing"/>
        <rdfs:comment xml:lang="en">A Generic Property is a property of one or more objects or types of object.</rdfs:comment>
    </owl:Class>
    


    <!-- http://www.nist.gov/itl/ssd/OntologyRequirements#GovernmentalOrganization -->

    <owl:Class rdf:about="&or;GovernmentalOrganization">
        <rdfs:subClassOf rdf:resource="&or;Organization"/>
        <rdfs:comment>A Governmental Organization is an Organization that is a government, a department or other part of one particular government, or a groups consisting of different governments or representatives from a number of different governments.

Same as cyc:GovernmentalOrganization.</rdfs:comment>
    </owl:Class>
    


    <!-- http://www.nist.gov/itl/ssd/OntologyRequirements#GraphicalImage -->

    <owl:Class rdf:about="&or;GraphicalImage">
        <rdfs:subClassOf rdf:resource="&or;MovingImage"/>
        <rdfs:subClassOf rdf:resource="&or;StillImage"/>
        <rdfs:comment xml:lang="en">A Graphical Image is a constructed Image designed to depict data.  It is not a visual image of a physical scene.</rdfs:comment>
    </owl:Class>
    


    <!-- http://www.nist.gov/itl/ssd/OntologyRequirements#Human -->

    <owl:Class rdf:about="&or;Human">
        <rdfs:subClassOf rdf:resource="&or;IntelligentAgent"/>
        <rdfs:subClassOf rdf:resource="&or;PhysicalObject"/>
        <rdfs:comment xml:lang="en">A human being</rdfs:comment>
    </owl:Class>
    


    <!-- http://www.nist.gov/itl/ssd/OntologyRequirements#Image -->

    <owl:Class rdf:about="&or;Image">
        <rdfs:subClassOf rdf:resource="&or;SpatialThing"/>
        <rdfs:subClassOf rdf:resource="&or;TemporalThing"/>
        <owl:disjointWith rdf:resource="&or;IntelligentAgent"/>
        <owl:disjointWith rdf:resource="&or;Language"/>
        <owl:disjointWith rdf:resource="&or;LogicalRule"/>
        <owl:disjointWith rdf:resource="&or;Metadata"/>
        <owl:disjointWith rdf:resource="&or;Quantity"/>
        <owl:disjointWith rdf:resource="&or;RuleSet"/>
        <owl:disjointWith rdf:resource="&or;Software"/>
        <owl:disjointWith rdf:resource="&or;StateOfBeing"/>
        <owl:disjointWith rdf:resource="&or;TimeInterval"/>
        <owl:disjointWith rdf:resource="&or;UnitOfMeasure"/>
        <rdfs:comment xml:lang="en">An image is either an abstract or concrete image of some sort.  Significant specializations include VisualImage (ones that can be directly viewed, whether on film or a computer screen)  and ComputerImageFile (which is a file which stores the information in an image so that it can be rendered on an ImageRenderingDevice.</rdfs:comment>
    </owl:Class>
    


    <!-- http://www.nist.gov/itl/ssd/OntologyRequirements#ImageDisplayDevice -->

    <owl:Class rdf:about="&or;ImageDisplayDevice">
        <rdfs:subClassOf rdf:resource="&or;ImageOutputDevice"/>
    </owl:Class>
    


    <!-- http://www.nist.gov/itl/ssd/OntologyRequirements#ImageFileFormat -->

    <owl:Class rdf:about="&or;ImageFileFormat">
        <rdfs:subClassOf rdf:resource="&or;ElectronicFileFormat"/>
        <rdfs:comment xml:lang="en">An Electronic File Format is a Data Format that is specific for Computer Image Files.</rdfs:comment>
    </owl:Class>
    


    <!-- http://www.nist.gov/itl/ssd/OntologyRequirements#ImageInputDevice -->

    <owl:Class rdf:about="&or;ImageInputDevice">
        <rdfs:subClassOf rdf:resource="&or;DataInputDevice"/>
        <rdfs:subClassOf rdf:resource="&or;ImagingDevice"/>
    </owl:Class>
    


    <!-- http://www.nist.gov/itl/ssd/OntologyRequirements#ImageOutputDevice -->

    <owl:Class rdf:about="&or;ImageOutputDevice">
        <rdfs:subClassOf rdf:resource="&or;DataOutputDevice"/>
        <rdfs:subClassOf rdf:resource="&or;ImagingDevice"/>
    </owl:Class>
    


    <!-- http://www.nist.gov/itl/ssd/OntologyRequirements#ImagePrintingDevice -->

    <owl:Class rdf:about="&or;ImagePrintingDevice">
        <rdfs:subClassOf rdf:resource="&or;ImageOutputDevice"/>
    </owl:Class>
    


    <!-- http://www.nist.gov/itl/ssd/OntologyRequirements#ImageProcessingSoftware -->

    <owl:Class rdf:about="&or;ImageProcessingSoftware">
        <rdfs:subClassOf rdf:resource="&or;Software"/>
        <owl:disjointWith rdf:resource="&or;OperatingSystem"/>
        <rdfs:comment xml:lang="en">Any instance of Image Processing Software is Software (ranging from a subroutine, through a program, to a Software Package) that implements at least one Image Processing Algorithm.</rdfs:comment>
    </owl:Class>
    


    <!-- http://www.nist.gov/itl/ssd/OntologyRequirements#ImageSequence -->

    <owl:Class rdf:about="&or;ImageSequence">
        <rdfs:subClassOf rdf:resource="&or;AbstractStructuredInformationStore"/>
        <rdfs:comment xml:lang="en">A sequence of images, that can be ordered spatially (in the Z dimension), temporally, or by some other feature.</rdfs:comment>
        <rdfs:comment>Maybe a more generic property -- firstItemInSequence -- should be substituted for this more specific one.</rdfs:comment>
    </owl:Class>
    


    <!-- http://www.nist.gov/itl/ssd/OntologyRequirements#ImagingDevice -->

    <owl:Class rdf:about="&or;ImagingDevice">
        <rdfs:subClassOf rdf:resource="&or;PhysicalDevice"/>
        <owl:disjointWith rdf:resource="&or;IntelligentAgent"/>
        <rdfs:comment xml:lang="en">The class of physical devices used to create images.  These may have as output electronic images, film images, or image projections.  They may have light, x-rays, or some other part of the electromagnetic spectrum as input.  They may also take input from particle beams, electrical sensors (as some types of scanning microscopes, or computer software.</rdfs:comment>
    </owl:Class>
    


    <!-- http://www.nist.gov/itl/ssd/OntologyRequirements#Information -->

    <owl:Class rdf:about="&or;Information">
        <rdfs:subClassOf rdf:resource="&or;NonTangibleThing"/>
        <owl:disjointWith rdf:resource="&or;SpatialThing"/>
        <rdfs:comment xml:lang="en">Abstract Information. Some types of information are structured (see Abstract Information Store and its subclasses), while others (such as Plans and Objectives) need not be.  Information is distinct from objects which store that information.</rdfs:comment>
    </owl:Class>
    


    <!-- http://www.nist.gov/itl/ssd/OntologyRequirements#IntangibleCreatedThing -->

    <owl:Class rdf:about="&or;IntangibleCreatedThing">
        <owl:equivalentClass>
            <owl:Class>
                <owl:intersectionOf rdf:parseType="Collection">
                    <rdf:Description rdf:about="&or;CreatedThing"/>
                    <rdf:Description rdf:about="&or;NonTangibleThing"/>
                </owl:intersectionOf>
            </owl:Class>
        </owl:equivalentClass>
        <rdfs:subClassOf rdf:resource="&or;CreatedThing"/>
        <owl:disjointWith rdf:resource="&or;SpatialFrameOfReference"/>
    </owl:Class>
    


    <!-- http://www.nist.gov/itl/ssd/OntologyRequirements#IntelligentAgent -->

    <owl:Class rdf:about="&or;IntelligentAgent">
        <rdfs:subClassOf rdf:resource="&or;TemporalThing"/>
        <owl:disjointWith rdf:resource="&or;Language"/>
        <owl:disjointWith rdf:resource="&or;LogicalRule"/>
        <owl:disjointWith rdf:resource="&or;Metadata"/>
        <owl:disjointWith rdf:resource="&or;Quantity"/>
        <owl:disjointWith rdf:resource="&or;RuleSet"/>
        <owl:disjointWith rdf:resource="&or;Software"/>
        <owl:disjointWith rdf:resource="&or;StateOfBeing"/>
        <owl:disjointWith rdf:resource="&or;StructuredInformationStore"/>
        <owl:disjointWith rdf:resource="&or;TimeInterval"/>
        <owl:disjointWith rdf:resource="&or;UnitOfMeasure"/>
        <rdfs:comment xml:lang="en">An IntelligentAgent is a Person or Organization that can perform actions and have contact information such as telephone numbers and addresses (including postal and email).</rdfs:comment>
    </owl:Class>
    


    <!-- http://www.nist.gov/itl/ssd/OntologyRequirements#IntentionalCreation -->

    <owl:Class rdf:about="&or;IntentionalCreation">
        <rdfs:subClassOf rdf:resource="&or;CreationEvent"/>
        <rdfs:subClassOf rdf:resource="&or;PurposefulAction"/>
        <owl:disjointWith rdf:resource="&or;Recommending"/>
        <rdfs:comment xml:lang="en">Intentional Creation is the purposeful creation of a physical or information object.</rdfs:comment>
    </owl:Class>
    


    <!-- http://www.nist.gov/itl/ssd/OntologyRequirements#InterconvertibleUnitType -->

    <owl:Class rdf:about="&or;InterconvertibleUnitType">
        <rdfs:subClassOf rdf:resource="&or;FirstOrderClass"/>
        <owl:disjointWith rdf:resource="&or;MeasurableQuantityType"/>
        <owl:disjointWith rdf:resource="&or;ObjectType"/>
    </owl:Class>
    


    <!-- http://www.nist.gov/itl/ssd/OntologyRequirements#January -->

    <owl:Class rdf:about="&or;January">
        <rdfs:subClassOf rdf:resource="&or;CalendarMonth"/>
        <rdfs:comment xml:lang="en">The month of January</rdfs:comment>
    </owl:Class>
    


    <!-- http://www.nist.gov/itl/ssd/OntologyRequirements#July -->

    <owl:Class rdf:about="&or;July">
        <rdfs:subClassOf rdf:resource="&or;CalendarMonth"/>
        <rdfs:comment xml:lang="en">The month of July</rdfs:comment>
    </owl:Class>
    


    <!-- http://www.nist.gov/itl/ssd/OntologyRequirements#June -->

    <owl:Class rdf:about="&or;June">
        <rdfs:subClassOf rdf:resource="&or;CalendarMonth"/>
        <rdfs:comment xml:lang="en">The month of June</rdfs:comment>
    </owl:Class>
    


    <!-- http://www.nist.gov/itl/ssd/OntologyRequirements#LaboratoryEquipment -->

    <owl:Class rdf:about="&or;LaboratoryEquipment">
        <rdfs:subClassOf rdf:resource="&or;PhysicalDevice"/>
        <rdfs:comment xml:lang="en">Each instance of LaboratoryEquipment is a physical tool or piece of equipment used by scientists to perform or record experiments in laboratories.</rdfs:comment>
    </owl:Class>
    


    <!-- http://www.nist.gov/itl/ssd/OntologyRequirements#Language -->

    <owl:Class rdf:about="&or;Language">
        <rdfs:subClassOf rdf:resource="&or;IntangibleCreatedThing"/>
        <owl:disjointWith rdf:resource="&or;LogicalRule"/>
        <owl:disjointWith rdf:resource="&or;Metadata"/>
        <owl:disjointWith rdf:resource="&or;Quantity"/>
        <owl:disjointWith rdf:resource="&or;RuleSet"/>
        <owl:disjointWith rdf:resource="&or;Software"/>
        <owl:disjointWith rdf:resource="&or;StructuredInformationStore"/>
        <owl:disjointWith rdf:resource="&or;Technique"/>
        <owl:disjointWith rdf:resource="&or;UnitOfMeasure"/>
        <rdfs:comment xml:lang="en">A language is is a generative system of signs for transmitting information. These signs are normally conventional and arbitrary in nature, although onomatopoeia, pictographs, and sign language symbols can be intrinsically representational.

Natural languages develop, while formal languages are designed, to be interpretable by some community (of people and/or machines).  They may be spoken, written, motioned, or represented in physical objects.

Same as cyc:Language.</rdfs:comment>
    </owl:Class>
    


    <!-- http://www.nist.gov/itl/ssd/OntologyRequirements#LineChart -->

    <owl:Class rdf:about="&or;LineChart">
        <rdfs:subClassOf rdf:resource="&or;GraphicalImage"/>
    </owl:Class>
    


    <!-- http://www.nist.gov/itl/ssd/OntologyRequirements#LineSegment -->

    <owl:Class rdf:about="&or;LineSegment">
        <owl:equivalentClass>
            <owl:Class>
                <owl:intersectionOf rdf:parseType="Collection">
                    <rdf:Description rdf:about="&or;CurveSegment"/>
                    <rdf:Description rdf:about="&or;StraightLine"/>
                </owl:intersectionOf>
            </owl:Class>
        </owl:equivalentClass>
        <rdfs:subClassOf rdf:resource="&or;CurveSegment"/>
        <rdfs:comment xml:lang="en">A LineSegment is a Straight Line with two end points.</rdfs:comment>
    </owl:Class>
    


    <!-- http://www.nist.gov/itl/ssd/OntologyRequirements#LogicalRule -->

    <owl:Class rdf:about="&or;LogicalRule">
        <rdfs:subClassOf rdf:resource="&or;IntangibleCreatedThing"/>
        <owl:disjointWith rdf:resource="&or;Metadata"/>
        <owl:disjointWith rdf:resource="&or;Quantity"/>
        <owl:disjointWith rdf:resource="&or;RuleSet"/>
        <owl:disjointWith rdf:resource="&or;Software"/>
        <owl:disjointWith rdf:resource="&or;SpatialThing"/>
        <owl:disjointWith rdf:resource="&or;StructuredInformationStore"/>
        <owl:disjointWith rdf:resource="&or;UnitOfMeasure"/>
    </owl:Class>
    


    <!-- http://www.nist.gov/itl/ssd/OntologyRequirements#Manufacturer -->

    <owl:Class rdf:about="&or;Manufacturer">
        <rdfs:subClassOf rdf:resource="&or;Organization"/>
        <rdfs:comment xml:lang="en">A Manufacturer is an organization that creates some products.</rdfs:comment>
    </owl:Class>
    


    <!-- http://www.nist.gov/itl/ssd/OntologyRequirements#Manufacturing -->

    <owl:Class rdf:about="&or;Manufacturing">
        <rdfs:subClassOf rdf:resource="&or;IntentionalCreation"/>
        <rdfs:subClassOf rdf:resource="&or;PhysicalEvent"/>
        <rdfs:subClassOf>
            <owl:Restriction>
                <owl:onProperty rdf:resource="&or;outputCreated"/>
                <owl:someValuesFrom rdf:resource="&or;Artifact"/>
            </owl:Restriction>
        </rdfs:subClassOf>
        <owl:disjointWith rdf:resource="&or;Optimization"/>
        <owl:disjointWith rdf:resource="&or;Planning"/>
        <rdfs:comment xml:lang="en">Manufacturing is the action of producing some physical products.</rdfs:comment>
    </owl:Class>
    


    <!-- http://www.nist.gov/itl/ssd/OntologyRequirements#Map -->

    <owl:Class rdf:about="&or;Map">
        <rdfs:subClassOf rdf:resource="&or;GraphicalImage"/>
    </owl:Class>
    


    <!-- http://www.nist.gov/itl/ssd/OntologyRequirements#March -->

    <owl:Class rdf:about="&or;March">
        <rdfs:subClassOf rdf:resource="&or;CalendarMonth"/>
        <rdfs:comment xml:lang="en">The month of March</rdfs:comment>
    </owl:Class>
    


    <!-- http://www.nist.gov/itl/ssd/OntologyRequirements#Mass -->

    <owl:Class rdf:about="&or;Mass">
        <owl:equivalentClass>
            <owl:Class>
                <owl:intersectionOf rdf:parseType="Collection">
                    <rdf:Description rdf:about="&or;MeasurableQuantity"/>
                    <owl:Restriction>
                        <owl:onProperty rdf:resource="&or;unitsFor"/>
                        <owl:someValuesFrom rdf:resource="&or;UnitOfMass"/>
                    </owl:Restriction>
                </owl:intersectionOf>
            </owl:Class>
        </owl:equivalentClass>
        <rdfs:subClassOf rdf:resource="&or;MeasurableQuantity"/>
        <rdfs:subClassOf>
            <owl:Restriction>
                <owl:onProperty rdf:resource="&or;unitsFor"/>
                <owl:allValuesFrom rdf:resource="&or;UnitOfMass"/>
            </owl:Restriction>
        </rdfs:subClassOf>
        <owl:disjointWith rdf:resource="&or;Pressure"/>
        <owl:disjointWith rdf:resource="&or;Temperature"/>
        <owl:disjointWith rdf:resource="&or;Volume"/>
    </owl:Class>
    


    <!-- http://www.nist.gov/itl/ssd/OntologyRequirements#MaterialProperty -->

    <owl:Class rdf:about="&or;MaterialProperty">
        <rdfs:subClassOf rdf:resource="&or;GenericProperty"/>
        <rdfs:comment xml:lang="en">A Material Property is a physical property of some physical material or object, such as its mass, melting point, or temperature.</rdfs:comment>
    </owl:Class>
    


    <!-- http://www.nist.gov/itl/ssd/OntologyRequirements#MaterialType -->

    <owl:Class rdf:about="&or;MaterialType">
        <rdfs:subClassOf rdf:resource="&or;ObjectType"/>
        <owl:disjointWith rdf:resource="&or;MeasurementRole"/>
    </owl:Class>
    


    <!-- http://www.nist.gov/itl/ssd/OntologyRequirements#MathematicalExpression -->

    <owl:Class rdf:about="&or;MathematicalExpression">
        <rdfs:subClassOf rdf:resource="&or;AbstractStructuredInformationStore"/>
        <rdfs:comment xml:lang="en">A Mathematical Expression is a structured set of symbols with some meaning in mathematics.</rdfs:comment>
    </owl:Class>
    


    <!-- http://www.nist.gov/itl/ssd/OntologyRequirements#MathematicalFormula -->

    <owl:Class rdf:about="&or;MathematicalFormula">
        <rdfs:subClassOf rdf:resource="&or;MathematicalExpression"/>
        <rdfs:comment xml:lang="en">A Mathematical Formula is a fact, rule, or principle that is expressed in terms of mathematical symbols. These include equations, inequalities, and expressions that can be evaluated. </rdfs:comment>
    </owl:Class>
    


    <!-- http://www.nist.gov/itl/ssd/OntologyRequirements#May -->

    <owl:Class rdf:about="&or;May">
        <rdfs:subClassOf rdf:resource="&or;CalendarMonth"/>
        <rdfs:comment xml:lang="en">The month of May</rdfs:comment>
    </owl:Class>
    


    <!-- http://www.nist.gov/itl/ssd/OntologyRequirements#MeasurableMaterialProperty -->

    <owl:Class rdf:about="&or;MeasurableMaterialProperty">
        <owl:equivalentClass>
            <owl:Class>
                <owl:intersectionOf rdf:parseType="Collection">
                    <rdf:Description rdf:about="&or;MaterialProperty"/>
                    <rdf:Description rdf:about="&or;MeasurableProperty"/>
                </owl:intersectionOf>
            </owl:Class>
        </owl:equivalentClass>
        <rdfs:subClassOf rdf:resource="&or;MaterialProperty"/>
        <rdfs:comment xml:lang="en">A Measurable Material Proparty is any Material Property that has a numerically measurable component.</rdfs:comment>
    </owl:Class>
    


    <!-- http://www.nist.gov/itl/ssd/OntologyRequirements#MeasurableProperty -->

    <owl:Class rdf:about="&or;MeasurableProperty">
        <rdfs:subClassOf rdf:resource="&or;GenericProperty"/>
        <owl:disjointWith rdf:resource="&or;MeasurableQuantity"/>
        <rdfs:comment xml:lang="en">A Measurable Property is a property of one or more objects or types of object whose value is an instance of MeasurableQuantity.  Some example instances are Melting Point of a substance and Concentration By Mass.</rdfs:comment>
    </owl:Class>
    


    <!-- http://www.nist.gov/itl/ssd/OntologyRequirements#MeasurableQuantity -->

    <owl:Class rdf:about="&or;MeasurableQuantity">
        <rdfs:subClassOf rdf:resource="&or;Quantity"/>
        <owl:disjointWith rdf:resource="&or;UnitPrice"/>
        <rdfs:comment xml:lang="en">Measurable Quantitites are those Quantities that have a numeric component and could be used to measure something, as opposed to merely ranking it on a scale.  This is the same as cyc:MeasurableQuantity.</rdfs:comment>
    </owl:Class>
    


    <!-- http://www.nist.gov/itl/ssd/OntologyRequirements#MeasurableQuantityType -->

    <owl:Class rdf:about="&or;MeasurableQuantityType">
        <rdfs:subClassOf rdf:resource="&or;FirstOrderClass"/>
        <owl:disjointWith rdf:resource="&or;ObjectType"/>
        <rdfs:comment xml:lang="en">A type quantity that can be measured, such as area, distance, duration, temperature, or volume.  Specific quantities (1.0 square cm, 3.14 kg, etc.) are NOT instances.  See `Specialized Measurable Quantity Type&#39; for restrictions of such quantity types to specific object types (such as cell area).</rdfs:comment>
    </owl:Class>
    


    <!-- http://www.nist.gov/itl/ssd/OntologyRequirements#MeasurementRole -->

    <owl:Class rdf:about="&or;MeasurementRole">
        <rdfs:subClassOf rdf:resource="&or;ObjectType"/>
        <rdfs:comment xml:lang="en">A `Measurement Role&#39; is the manner in which a result plays a role in a measurement.  For example, positive control, negative control, spatial benchmark, intensity benchmark, experimental sample, derived data.</rdfs:comment>
    </owl:Class>
    


    <!-- http://www.nist.gov/itl/ssd/OntologyRequirements#MeasuringDevice -->

    <owl:Class rdf:about="&or;MeasuringDevice">
        <rdfs:subClassOf rdf:resource="&or;PhysicalDevice"/>
        <rdfs:comment xml:lang="en">A measuring device is a physical device used for measuring some quantity.</rdfs:comment>
    </owl:Class>
    


    <!-- http://www.nist.gov/itl/ssd/OntologyRequirements#MechanicalProcess -->

    <owl:Class rdf:about="&or;MechanicalProcess">
        <rdfs:subClassOf rdf:resource="&or;PhysicalEvent"/>
        <owl:disjointWith rdf:resource="&or;Recommending"/>
        <rdfs:comment xml:lang="en">A Mechanical Process is a process that takes place as the result of mechanical forces, irrespective of whether the forces are natural, or the result of animate action whether intended or not. </rdfs:comment>
    </owl:Class>
    


    <!-- http://www.nist.gov/itl/ssd/OntologyRequirements#Metadata -->

    <owl:Class rdf:about="&or;Metadata">
        <rdfs:subClassOf rdf:resource="&or;Information"/>
        <owl:disjointWith rdf:resource="&or;Software"/>
        <owl:disjointWith rdf:resource="&or;StructuredInformationStore"/>
        <owl:disjointWith rdf:resource="&or;Technique"/>
    </owl:Class>
    


    <!-- http://www.nist.gov/itl/ssd/OntologyRequirements#MetricUnit -->

    <owl:Class rdf:about="&or;MetricUnit">
        <rdfs:subClassOf rdf:resource="&or;UnitOfMeasure"/>
        <owl:disjointWith rdf:resource="&or;UnitOfComputerStorageCapacity"/>
        <termString xml:lang="en">metric unit</termString>
        <termString xml:lang="en">metric unit of measure</termString>
    </owl:Class>
    


    <!-- http://www.nist.gov/itl/ssd/OntologyRequirements#MicroscopyImageFileFormat -->

    <owl:Class rdf:about="&or;MicroscopyImageFileFormat">
        <rdfs:subClassOf rdf:resource="&or;ImageFileFormat"/>
        <rdfs:comment>Image formats specificaly used for microscopy images</rdfs:comment>
    </owl:Class>
    


    <!-- http://www.nist.gov/itl/ssd/OntologyRequirements#Modeling -->

    <owl:Class rdf:about="&or;Modeling">
        <owl:equivalentClass>
            <owl:Class>
                <owl:intersectionOf rdf:parseType="Collection">
                    <rdf:Description rdf:about="&or;Development"/>
                    <owl:Restriction>
                        <owl:onProperty rdf:resource="&or;outputCreated"/>
                        <owl:someValuesFrom rdf:resource="&or;ConceptualModel"/>
                    </owl:Restriction>
                </owl:intersectionOf>
            </owl:Class>
        </owl:equivalentClass>
        <rdfs:subClassOf rdf:resource="&or;Development"/>
        <rdfs:subClassOf>
            <owl:Restriction>
                <owl:onProperty rdf:resource="&or;outputCreated"/>
                <owl:someValuesFrom rdf:resource="&or;ConceptualModel"/>
            </owl:Restriction>
        </rdfs:subClassOf>
        <rdfs:comment xml:lang="en">Modeling is a Purposeful Acition in which a Conceputal Model is created and developed for the way something works or is structured.</rdfs:comment>
    </owl:Class>
    


    <!-- http://www.nist.gov/itl/ssd/OntologyRequirements#MonthOfYearType -->

    <owl:Class rdf:about="&or;MonthOfYearType">
        <rdfs:subClassOf rdf:resource="&or;TimeOfYearType"/>
        <rdfs:comment xml:lang="en">A named month type in a Gregorian (or Julian) calendar.  I.e., January, February, March, April, ... December.</rdfs:comment>
    </owl:Class>
    


    <!-- http://www.nist.gov/itl/ssd/OntologyRequirements#MovementEvent -->

    <owl:Class rdf:about="&or;MovementEvent">
        <rdfs:subClassOf rdf:resource="&or;PhysicalEvent"/>
        <owl:disjointWith rdf:resource="&or;Recommending"/>
        <rdfs:comment xml:lang="en">A  Movement Event is an event in which at least one object either translates some distance or moves from one rotational orientation to another, relative to a frame of reference that is not part of the translating/rotating object. The movement in question might be periodic or not, continuous or not.</rdfs:comment>
    </owl:Class>
    


    <!-- http://www.nist.gov/itl/ssd/OntologyRequirements#MovingImage -->

    <owl:Class rdf:about="&or;MovingImage">
        <rdfs:subClassOf rdf:resource="&or;Image"/>
        <rdfs:subClassOf rdf:resource="&or;ImageSequence"/>
        <owl:disjointWith rdf:resource="&or;StillImage"/>
    </owl:Class>
    


    <!-- http://www.nist.gov/itl/ssd/OntologyRequirements#NonMetricUnit -->

    <owl:Class rdf:about="&or;NonMetricUnit">
        <rdfs:subClassOf rdf:resource="&or;UnitOfMeasure"/>
        <rdfs:comment xml:lang="en">A Non-Metric Unit is a Unit of Measure that is not part of the metric system.  This includes both fundamental units and composed units of which at least one of the component units are not metric.</rdfs:comment>
    </owl:Class>
    


    <!-- http://www.nist.gov/itl/ssd/OntologyRequirements#NonTangibleThing -->

    <owl:Class rdf:about="&or;NonTangibleThing">
        <rdfs:subClassOf rdf:resource="&owl;Thing"/>
        <owl:disjointWith rdf:resource="&or;PhysicalObject"/>
    </owl:Class>
    


    <!-- http://www.nist.gov/itl/ssd/OntologyRequirements#November -->

    <owl:Class rdf:about="&or;November">
        <rdfs:subClassOf rdf:resource="&or;CalendarMonth"/>
        <rdfs:comment xml:lang="en">The month of November</rdfs:comment>
    </owl:Class>
    


    <!-- http://www.nist.gov/itl/ssd/OntologyRequirements#NumericArray -->

    <owl:Class rdf:about="&or;NumericArray">
        <rdfs:subClassOf rdf:resource="&or;Array"/>
        <rdfs:comment xml:lang="en">A Numeric Array is an Array, each of whose cells is a number or variable reqpresenting a number.</rdfs:comment>
    </owl:Class>
    


    <!-- http://www.nist.gov/itl/ssd/OntologyRequirements#NumericalSimulationModel -->

    <owl:Class rdf:about="&or;NumericalSimulationModel">
        <rdfs:subClassOf rdf:resource="&or;SimulationModel"/>
    </owl:Class>
    


    <!-- http://www.nist.gov/itl/ssd/OntologyRequirements#ObjectType -->

    <owl:Class rdf:about="&or;ObjectType">
        <rdfs:subClassOf rdf:resource="&or;FirstOrderClass"/>
    </owl:Class>
    


    <!-- http://www.nist.gov/itl/ssd/OntologyRequirements#October -->

    <owl:Class rdf:about="&or;October">
        <rdfs:subClassOf rdf:resource="&or;CalendarMonth"/>
        <rdfs:comment xml:lang="en">The month of October</rdfs:comment>
    </owl:Class>
    


    <!-- http://www.nist.gov/itl/ssd/OntologyRequirements#OneDimensionalArray -->

    <owl:Class rdf:about="&or;OneDimensionalArray">
        <rdfs:subClassOf rdf:resource="&oil;List"/>
        <rdfs:subClassOf rdf:resource="&or;Array"/>
        <rdfs:comment xml:lang="en">A One Dimensional Array is a List, none of whose members is itself an Array.</rdfs:comment>
    </owl:Class>
    


    <!-- http://www.nist.gov/itl/ssd/OntologyRequirements#OperatingSystem -->

    <owl:Class rdf:about="&or;OperatingSystem">
        <rdfs:subClassOf rdf:resource="&or;SoftwarePackage"/>
        <rdfs:comment xml:lang="en">An OperatingSystem is a Software Package that provides an environment in which a user can execute Application Programs  on the hardware of a computer.</rdfs:comment>
    </owl:Class>
    


    <!-- http://www.nist.gov/itl/ssd/OntologyRequirements#Optimization -->

    <owl:Class rdf:about="&or;Optimization">
        <rdfs:subClassOf rdf:resource="&or;PurposefulAction"/>
        <owl:disjointWith rdf:resource="&or;Planning"/>
        <owl:disjointWith rdf:resource="&or;Recommending"/>
        <rdfs:comment xml:lang="en">Optimization is the activity of optimizing something, a product, a procedure, a design, a computation, etc.</rdfs:comment>
    </owl:Class>
    


    <!-- http://www.nist.gov/itl/ssd/OntologyRequirements#Organization -->

    <owl:Class rdf:about="&or;Organization">
        <rdfs:subClassOf rdf:resource="&or;IntangibleCreatedThing"/>
        <rdfs:subClassOf rdf:resource="&or;IntelligentAgent"/>
        <owl:disjointWith rdf:resource="&or;StructuredInformationStore"/>
        <rdfs:comment xml:lang="en">Each instance of Organization is a social structure whose members are instances of IntelligentAgent.  Members of an Organization may people or be Organizations themselves (e.g., the United Nations has countries as members).  Members of an Organization are not physical parts of that organization (since anatomical parts of the members would therefore also be parts of the organization).</rdfs:comment>
    </owl:Class>
    


    <!-- http://www.nist.gov/itl/ssd/OntologyRequirements#OrganizationalChart -->

    <owl:Class rdf:about="&or;OrganizationalChart">
        <rdfs:subClassOf rdf:resource="&or;GraphicalImage"/>
    </owl:Class>
    


    <!-- http://www.nist.gov/itl/ssd/OntologyRequirements#Photometer -->

    <owl:Class rdf:about="&or;Photometer">
        <rdfs:subClassOf rdf:resource="&or;MeasuringDevice"/>
        <rdfs:comment xml:lang="en">A Photometer is a device used to measure the intensity of light.</rdfs:comment>
    </owl:Class>
    


    <!-- http://www.nist.gov/itl/ssd/OntologyRequirements#PhysicalDevice -->

    <owl:Class rdf:about="&or;PhysicalDevice">
        <rdfs:subClassOf rdf:resource="&or;Artifact"/>
        <rdfs:comment xml:lang="en">A PhysicalDevice is an artifact with a relatively rigid, set shape (although pars may move in a constrained fashion relative to other parts), designed for a specific use (or set of uses) or to perform a specific function (or set of functions).

Same as cyc:PhysicalDevice.</rdfs:comment>
    </owl:Class>
    


    <!-- http://www.nist.gov/itl/ssd/OntologyRequirements#PhysicalEvent -->

    <owl:Class rdf:about="&or;PhysicalEvent">
        <rdfs:subClassOf rdf:resource="&or;Event"/>
        <rdfs:subClassOf rdf:resource="&or;SpatialThing"/>
        <rdfs:comment xml:lang="en">A Physical Event is a spatially localized event involving one or more physical objects or stuffs.</rdfs:comment>
        <rdfs:seeAlso>cyc:PhysicalEvent</rdfs:seeAlso>
    </owl:Class>
    


    <!-- http://www.nist.gov/itl/ssd/OntologyRequirements#PhysicalObject -->

    <owl:Class rdf:about="&or;PhysicalObject">
        <rdfs:subClassOf rdf:resource="&or;SpatialThing"/>
        <rdfs:subClassOf rdf:resource="&or;TemporalThing"/>
        <owl:disjointWith rdf:resource="&or;SpatialFrameOfReference"/>
    </owl:Class>
    


    <!-- http://www.nist.gov/itl/ssd/OntologyRequirements#PieChart -->

    <owl:Class rdf:about="&or;PieChart">
        <rdfs:subClassOf rdf:resource="&or;GraphicalImage"/>
    </owl:Class>
    


    <!-- http://www.nist.gov/itl/ssd/OntologyRequirements#PlanarRegion -->

    <owl:Class rdf:about="&or;PlanarRegion">
        <rdfs:subClassOf rdf:resource="&or;SpatialRegion"/>
        <rdfs:comment xml:lang="en">A Planar Region is a spatial region that has extent in at least two dimensions, and either has no significant thickness compared to its length and width.  It has mild or no curvature.</rdfs:comment>
    </owl:Class>
    


    <!-- http://www.nist.gov/itl/ssd/OntologyRequirements#Planning -->

    <owl:Class rdf:about="&or;Planning">
        <rdfs:subClassOf rdf:resource="&or;Modeling"/>
        <rdfs:subClassOf>
            <owl:Restriction>
                <owl:onProperty rdf:resource="&or;outputCreated"/>
                <owl:someValuesFrom rdf:resource="&or;ActionPlan"/>
            </owl:Restriction>
        </rdfs:subClassOf>
        <rdfs:comment xml:lang="en">Planning is the action of making plans.</rdfs:comment>
    </owl:Class>
    


    <!-- http://www.nist.gov/itl/ssd/OntologyRequirements#PredictionMethod -->

    <owl:Class rdf:about="&or;PredictionMethod">
        <rdfs:subClassOf rdf:resource="&or;Technique"/>
        <rdfs:comment xml:lang="en">A Prediction Method is a Technique for predicting some type of thing.</rdfs:comment>
    </owl:Class>
    


    <!-- http://www.nist.gov/itl/ssd/OntologyRequirements#Pressure -->

    <owl:Class rdf:about="&or;Pressure">
        <owl:equivalentClass>
            <owl:Class>
                <owl:intersectionOf rdf:parseType="Collection">
                    <rdf:Description rdf:about="&or;MeasurableQuantity"/>
                    <owl:Restriction>
                        <owl:onProperty rdf:resource="&or;unitsFor"/>
                        <owl:someValuesFrom rdf:resource="&or;UnitOfPressure"/>
                    </owl:Restriction>
                </owl:intersectionOf>
            </owl:Class>
        </owl:equivalentClass>
        <rdfs:subClassOf rdf:resource="&or;MeasurableQuantity"/>
        <rdfs:subClassOf>
            <owl:Restriction>
                <owl:onProperty rdf:resource="&or;unitsFor"/>
                <owl:allValuesFrom rdf:resource="&or;UnitOfPressure"/>
            </owl:Restriction>
        </rdfs:subClassOf>
        <rdfs:comment xml:lang="en">Pressure is the force per unit area perpendicular to the surface of an object.</rdfs:comment>
    </owl:Class>
    


    <!-- http://www.nist.gov/itl/ssd/OntologyRequirements#PrimaryCurrencyUnit -->

    <owl:Class rdf:about="&or;PrimaryCurrencyUnit">
        <rdfs:subClassOf rdf:resource="&or;CurrencyUnit"/>
        <owl:disjointWith rdf:resource="&or;SecondaryCurrencyUnit"/>
        <rdfs:comment xml:lang="en">A primary currency unit is the basic unit of currency used in a country (or Geopolitical Region).  A secondary currency unity may be defined as some fraction of the primary unit.</rdfs:comment>
    </owl:Class>
    


    <!-- http://www.nist.gov/itl/ssd/OntologyRequirements#Profilometer -->

    <owl:Class rdf:about="&or;Profilometer">
        <rdfs:subClassOf rdf:resource="&or;MeasuringDevice"/>
        <rdfs:comment xml:lang="en">A Profilometer is a measuring instrument used to measure a surface&#39;s profile.</rdfs:comment>
    </owl:Class>
    


    <!-- http://www.nist.gov/itl/ssd/OntologyRequirements#PropertyWithValue -->

    <owl:Class rdf:about="&or;PropertyWithValue">
        <rdfs:subClassOf rdf:resource="&or;StateOfBeing"/>
        <rdfs:comment xml:lang="en">A Property With Value is a combination of of the generic property (length, boiling point, ...) something has along with the value of that property .</rdfs:comment>
    </owl:Class>
    


    <!-- http://www.nist.gov/itl/ssd/OntologyRequirements#PurposefulAction -->

    <owl:Class rdf:about="&or;PurposefulAction">
        <rdfs:subClassOf rdf:resource="&or;Event"/>
        <rdfs:comment xml:lang="en">A PurposefulAction is an action consciously, volitionally, and purposefully done by at least one actor.</rdfs:comment>
        <rdfs:seeAlso>cyc:PurposefulAction</rdfs:seeAlso>
    </owl:Class>
    


    <!-- http://www.nist.gov/itl/ssd/OntologyRequirements#Quantity -->

    <owl:Class rdf:about="&or;Quantity">
        <rdfs:subClassOf rdf:resource="&or;NonTangibleThing"/>
        <owl:disjointWith rdf:resource="&or;RuleSet"/>
        <owl:disjointWith rdf:resource="&or;Software"/>
        <owl:disjointWith rdf:resource="&or;SpatialFrameOfReference"/>
        <owl:disjointWith rdf:resource="&or;StructuredInformationStore"/>
        <owl:disjointWith rdf:resource="&or;Technique"/>
        <owl:disjointWith rdf:resource="&or;TemporalThing"/>
        <owl:disjointWith rdf:resource="&or;UnitOfMeasure"/>
    </owl:Class>
    


    <!-- http://www.nist.gov/itl/ssd/OntologyRequirements#Recommending -->

    <owl:Class rdf:about="&or;Recommending">
        <rdfs:subClassOf rdf:resource="&or;PurposefulAction"/>
    </owl:Class>
    


    <!-- http://www.nist.gov/itl/ssd/OntologyRequirements#ResearchOrganization -->

    <owl:Class rdf:about="&or;ResearchOrganization">
        <rdfs:subClassOf rdf:resource="&or;Organization"/>
        <rdfs:comment xml:lang="en">A Research Organization is an Organization that carries out basic or applied research as one of its main functions.

Same as cyc:ResearchOrganization.</rdfs:comment>
    </owl:Class>
    


    <!-- http://www.nist.gov/itl/ssd/OntologyRequirements#RigidPortableObject -->

    <owl:Class rdf:about="&or;RigidPortableObject">
        <rdfs:subClassOf rdf:resource="&or;PhysicalObject"/>
        <rdfs:comment xml:lang="en">A  Rigid Portable Object is a portable physical object with a medium to very high level of rigidity</rdfs:comment>
    </owl:Class>
    


    <!-- http://www.nist.gov/itl/ssd/OntologyRequirements#Rod -->

    <owl:Class rdf:about="&or;Rod">
        <rdfs:subClassOf rdf:resource="&or;Artifact"/>
        <rdfs:subClassOf rdf:resource="&or;RigidPortableObject"/>
        <rdfs:comment xml:lang="en">A Rod  is a long thin implement made of metal or wood.</rdfs:comment>
    </owl:Class>
    


    <!-- http://www.nist.gov/itl/ssd/OntologyRequirements#RuleSet -->

    <owl:Class rdf:about="&or;RuleSet">
        <rdfs:subClassOf rdf:resource="&or;IntangibleCreatedThing"/>
        <owl:disjointWith rdf:resource="&or;Software"/>
        <owl:disjointWith rdf:resource="&or;SpatialThing"/>
        <owl:disjointWith rdf:resource="&or;Technique"/>
        <owl:disjointWith rdf:resource="&or;UnitOfMeasure"/>
    </owl:Class>
    


    <!-- http://www.nist.gov/itl/ssd/OntologyRequirements#SI_Unit -->

    <owl:Class rdf:about="&or;SI_Unit">
        <rdfs:subClassOf rdf:resource="&or;MetricUnit"/>
        <termString xml:lang="en">SI unit</termString>
        <termString xml:lang="en">SI unit of measure</termString>
    </owl:Class>
    


    <!-- http://www.nist.gov/itl/ssd/OntologyRequirements#Scale-MeasuringDevice -->

    <owl:Class rdf:about="&or;Scale-MeasuringDevice">
        <rdfs:subClassOf rdf:resource="&or;MeasuringDevice"/>
        <owl:disjointWith rdf:resource="&or;Thermometer"/>
        <rdfs:comment xml:lang="en">A Scale (measuring device) is a device for measuring weight -- either absolute weight or the relative weight of two or more items.</rdfs:comment>
    </owl:Class>
    


    <!-- http://www.nist.gov/itl/ssd/OntologyRequirements#SecondaryCurrencyUnit -->

    <owl:Class rdf:about="&or;SecondaryCurrencyUnit">
        <rdfs:subClassOf rdf:resource="&or;CurrencyUnit"/>
        <rdfs:comment xml:lang="en">A secondary currency unit such as USCent, UKPenny, or ChineseFen is defined as some fraction of a primary currency unity (such as USDollar).</rdfs:comment>
    </owl:Class>
    


    <!-- http://www.nist.gov/itl/ssd/OntologyRequirements#September -->

    <owl:Class rdf:about="&or;September">
        <rdfs:subClassOf rdf:resource="&or;CalendarMonth"/>
        <rdfs:comment xml:lang="en">The month of September</rdfs:comment>
    </owl:Class>
    


    <!-- http://www.nist.gov/itl/ssd/OntologyRequirements#Simulating -->

    <owl:Class rdf:about="&or;Simulating">
        <rdfs:subClassOf rdf:resource="&or;Modeling"/>
        <rdfs:subClassOf>
            <owl:Restriction>
                <owl:onProperty rdf:resource="&or;outputCreated"/>
                <owl:someValuesFrom rdf:resource="&or;SimulationModel"/>
            </owl:Restriction>
        </rdfs:subClassOf>
    </owl:Class>
    


    <!-- http://www.nist.gov/itl/ssd/OntologyRequirements#SimulationModel -->

    <owl:Class rdf:about="&or;SimulationModel">
        <owl:equivalentClass>
            <owl:Restriction>
                <owl:onProperty rdf:resource="&or;outputCreated"/>
                <owl:onClass rdf:resource="&or;Simulating"/>
                <owl:qualifiedCardinality rdf:datatype="&xsd;nonNegativeInteger">1</owl:qualifiedCardinality>
            </owl:Restriction>
        </owl:equivalentClass>
        <rdfs:subClassOf rdf:resource="&or;ConceptualModel"/>
        <rdfs:comment xml:lang="en">A Simulation Model is a model of an event, whether real or potential, that has been created as the result of the process of Simulating</rdfs:comment>
    </owl:Class>
    


    <!-- http://www.nist.gov/itl/ssd/OntologyRequirements#Software -->

    <owl:Class rdf:about="&or;Software">
        <rdfs:subClassOf rdf:resource="&or;IntangibleCreatedThing"/>
        <owl:disjointWith rdf:resource="&or;UnitOfMeasure"/>
        <rdfs:comment xml:lang="en">An instance of Software is an individual computer program, a computer program module, a software package, a software library file, or a version or series thereof. Each instance of Software could conceivably be instantiated in code that could run on some computer system, even if the code has not been written yet, and even if it could not run independently of other code. This concept does not include purely data objects that software could operate on. 

 Same as cyc:SoftwareObject .</rdfs:comment>
    </owl:Class>
    


    <!-- http://www.nist.gov/itl/ssd/OntologyRequirements#SoftwareObjectWithVersions -->

    <owl:Class rdf:about="&or;SoftwareObjectWithVersions">
        <rdfs:subClassOf rdf:resource="&or;Software"/>
        <rdfs:comment xml:lang="en">A Software Object With Versions is a computer program, software package, subroutine, or library with two or more versions (Software Object Versions). 
Any instantiation of a Software Object With Versions that runs on some computer is more specifically an instance of one of its Software Object Versions.

Same as cyc:UnversionedSoftwareObject.</rdfs:comment>
    </owl:Class>
    


    <!-- http://www.nist.gov/itl/ssd/OntologyRequirements#SoftwarePackage -->

    <owl:Class rdf:about="&or;SoftwarePackage">
        <rdfs:subClassOf rdf:resource="&or;Software"/>
        <owl:disjointWith rdf:resource="&or;SoftwareSubroutine"/>
        <rdfs:comment xml:lang="en">A Software Package is the collection of programs (including configuration data files) designed to provide a set of related funcitionalities to users.  A Software Package is composed of loosely coupled component programs, possibly including libraries, tool sets, or system software.

Same as cyc:SoftwarePackage.</rdfs:comment>
    </owl:Class>
    


    <!-- http://www.nist.gov/itl/ssd/OntologyRequirements#SoftwareSubroutine -->

    <owl:Class rdf:about="&or;SoftwareSubroutine">
        <rdfs:subClassOf rdf:resource="&or;Software"/>
        <rdfs:comment xml:lang="en">A Software Subroutine is a piece of Software called by another piece of Software to which control will return when (and if) the subroutine completes ``normally&#39; &#39;.  A ``method&#39; &#39; in an object-oriented Computer Language is a common type of subroutine.</rdfs:comment>
    </owl:Class>
    


    <!-- http://www.nist.gov/itl/ssd/OntologyRequirements#SofwareObjectVersion -->

    <owl:Class rdf:about="&or;SofwareObjectVersion">
        <rdfs:subClassOf rdf:resource="&or;Software"/>
        <rdfs:comment xml:lang="en">A Software Object Version is a specific version of a computer program, software package, subroutine, or library.  Two different instantiations of a Versioned Software Object running on the same data, inputs, and equipment iwill produce the same results, with the proviso that programs that are affected by the external environment (sensor input, resource contension, etc.) may produce different results as their inputs differ).  Note that since a random number seed, is input data to a random number generator, results of instantiations of the same Software Object Version relying on the output of a random number generator may differ although all other inputs and data are the same.

Same as cyc:VersionedSoftwareObject.</rdfs:comment>
    </owl:Class>
    


    <!-- http://www.nist.gov/itl/ssd/OntologyRequirements#SpatialFrameOfReference -->

    <owl:Class rdf:about="&or;SpatialFrameOfReference">
        <rdfs:subClassOf rdf:resource="&or;NonTangibleThing"/>
        <rdfs:subClassOf rdf:resource="&or;SpatialThing"/>
        <owl:disjointWith rdf:resource="&or;StateOfBeing"/>
        <owl:disjointWith rdf:resource="&or;TimeInterval"/>
        <rdfs:comment xml:lang="en">A Spatial Frame of Reference is a spatial framework, normally fixed to some physical object or structure, relative to which observations are made.  Such a frame of refrerence is defined, not &quot;created&quot;.</rdfs:comment>
        <termString>reference frame</termString>
        <termString>frame of reference</termString>
    </owl:Class>
    


    <!-- http://www.nist.gov/itl/ssd/OntologyRequirements#SpatialRegion -->

    <owl:Class rdf:about="&or;SpatialRegion">
        <rdfs:subClassOf rdf:resource="&or;SpatialThing"/>
        <rdfs:comment xml:lang="en">A Spatial Region is a two- or three-dimensional intangible Spatial Thing whose instances are regions of space that may be fixed or move relative to physical objects. Spatial Regions can be occupied by solid (or other) objects or may be located within or without such objects.</rdfs:comment>
    </owl:Class>
    


    <!-- http://www.nist.gov/itl/ssd/OntologyRequirements#SpatialThing -->

    <owl:Class rdf:about="&or;SpatialThing">
        <rdfs:subClassOf rdf:resource="&owl;Thing"/>
        <owl:disjointWith rdf:resource="&or;UnitOfMeasure"/>
        <owl:disjointWith rdf:resource="&or;UnitPrice"/>
        <rdfs:comment xml:lang="en">A Spatial Thing is something that has a spatial extent or location relative to some other Spatial Thing or in some embedding space. A Spatial Thing may be tangible (e.g. a person) or wholly intangible (e.g. the ArcticCircle). A SpatialThing normally would be located in the physical universe but need not be (e.g., a trajectory through the phase space of some physical system is a curve and thus a spatial thing).</rdfs:comment>
    </owl:Class>
    


    <!-- http://www.nist.gov/itl/ssd/OntologyRequirements#SpecializedMeasurableQuantityType -->

    <owl:Class rdf:about="&or;SpecializedMeasurableQuantityType">
        <rdfs:subClassOf rdf:resource="&or;MeasurableQuantityType"/>
        <rdfs:comment xml:lang="en">A specialization of `Measurable Quantity Type&#39; restricted to quantity types for specific object types (such as cell area).  Specific quantities (1.0 square cm, 3.14 kg, etc.) are NOT instances.</rdfs:comment>
    </owl:Class>
    


    <!-- http://www.nist.gov/itl/ssd/OntologyRequirements#StateOfBeing -->

    <owl:Class rdf:about="&or;StateOfBeing">
        <rdfs:subClassOf rdf:resource="&or;NonTangibleThing"/>
        <owl:disjointWith rdf:resource="&or;StructuredInformationStore"/>
        <owl:disjointWith rdf:resource="&or;TimeInterval"/>
        <rdfs:comment xml:lang="en">A `State Of Being&#39; is a state which something is in.  Something may be in multiple states if the states are of different types.</rdfs:comment>
    </owl:Class>
    


    <!-- http://www.nist.gov/itl/ssd/OntologyRequirements#StillImage -->

    <owl:Class rdf:about="&or;StillImage">
        <rdfs:subClassOf rdf:resource="&or;Image"/>
        <rdfs:comment xml:lang="en">A stationary image.  It may be a single frame of a Moving Image.</rdfs:comment>
    </owl:Class>
    


    <!-- http://www.nist.gov/itl/ssd/OntologyRequirements#StraightLine -->

    <owl:Class rdf:about="&or;StraightLine">
        <rdfs:subClassOf rdf:resource="&or;Curve"/>
        <rdfs:comment xml:lang="en">A Straight Line is a Curve that is straight -- it does not curve or bend.  It may be a segment, a ray, or an (effectively) infinite line.</rdfs:comment>
    </owl:Class>
    


    <!-- http://www.nist.gov/itl/ssd/OntologyRequirements#StructuredInformationStore -->

    <owl:Class rdf:about="&or;StructuredInformationStore">
        <rdfs:subClassOf rdf:resource="&or;CreatedThing"/>
        <owl:disjointWith rdf:resource="&or;TimeInterval"/>
        <owl:disjointWith rdf:resource="&or;UnitOfMeasure"/>
        <owl:disjointWith rdf:resource="&rdf;Property"/>
        <rdfs:comment xml:lang="en">Each instance of Structured Information Source is an abstract or physical object in which items of information are represented as related in a systematic way that is easily characterized by some type of formal structure, including spatial or architectural terms (used metaphorically). Examples include: a database organized in fields and values; a spreadsheet organized in rows and columns with entries; a computer ontology, an organizational tree diagram with nodes and branches; and a topographical map.

See cyc:StructuredInformationStore.</rdfs:comment>
    </owl:Class>
    


    <!-- http://www.nist.gov/itl/ssd/OntologyRequirements#Technique -->

    <owl:Class rdf:about="&or;Technique">
        <rdfs:subClassOf rdf:resource="&or;EventType"/>
        <owl:disjointWith rdf:resource="&or;UnitOfMeasure"/>
        <rdfs:comment xml:lang="en">A Technique is a method of doing something.</rdfs:comment>
    </owl:Class>
    


    <!-- http://www.nist.gov/itl/ssd/OntologyRequirements#Temperature -->

    <owl:Class rdf:about="&or;Temperature">
        <rdfs:subClassOf rdf:resource="&or;MeasurableQuantity"/>
        <rdfs:subClassOf>
            <owl:Restriction>
                <owl:onProperty rdf:resource="&or;unitsFor"/>
                <owl:allValuesFrom rdf:resource="&or;UnitOfTemperature"/>
            </owl:Restriction>
        </rdfs:subClassOf>
        <owl:disjointWith rdf:resource="&or;Volume"/>
    </owl:Class>
    


    <!-- http://www.nist.gov/itl/ssd/OntologyRequirements#TemporalThing -->

    <owl:Class rdf:about="&or;TemporalThing">
        <rdfs:subClassOf rdf:resource="&owl;Thing"/>
        <owl:disjointWith rdf:resource="&or;UnitOfMeasure"/>
    </owl:Class>
    


    <!-- http://www.nist.gov/itl/ssd/OntologyRequirements#Thermometer -->

    <owl:Class rdf:about="&or;Thermometer">
        <rdfs:subClassOf rdf:resource="&or;MeasuringDevice"/>
        <rdfs:comment xml:lang="en">A thermometer is a device for measuring Temperature.</rdfs:comment>
    </owl:Class>
    


    <!-- http://www.nist.gov/itl/ssd/OntologyRequirements#ThreeDimensionalArray -->

    <owl:Class rdf:about="&or;ThreeDimensionalArray">
        <rdfs:subClassOf rdf:resource="&or;Array"/>
        <rdfs:comment xml:lang="en">A Three Dimensional Array is an Array of rows, columns, and levels, with each row the same length and each column the same length, and a Two Dimensional Array of the same dimensions at each level.  Any cell of the array can be uniquely referenced by its row, column, and level.</rdfs:comment>
    </owl:Class>
    


    <!-- http://www.nist.gov/itl/ssd/OntologyRequirements#ThreeDimensionalImage -->

    <owl:Class rdf:about="&or;ThreeDimensionalImage">
        <rdfs:subClassOf rdf:resource="&or;Image"/>
        <owl:disjointWith rdf:resource="&or;TwoDimensionalImage"/>
        <rdfs:comment xml:lang="en">An image with three spatial dimensions, in contrast with a TwoDimensionalImage.</rdfs:comment>
    </owl:Class>
    


    <!-- http://www.nist.gov/itl/ssd/OntologyRequirements#TimeInterval -->

    <owl:Class rdf:about="&or;TimeInterval">
        <rdfs:subClassOf rdf:resource="&or;NonTangibleThing"/>
        <rdfs:subClassOf rdf:resource="&or;TemporalThing"/>
    </owl:Class>
    


    <!-- http://www.nist.gov/itl/ssd/OntologyRequirements#TimeOfYearType -->

    <owl:Class rdf:about="&or;TimeOfYearType">
        <rdfs:subClassOf rdf:resource="&or;FirstOrderClass"/>
        <rdfs:comment xml:lang="en">A time of year type is a metaclass.  It&#39;s intances are types of time periods, such as a named month (October), season (Summer), fiscal quarter (ThirdQuarterOfYear), or named day (Thanksgiving, NewYearsDay, MarchFourth).  Any instance of TimeOfYearType would have a single instance in any given year (October of 2012, Summer of 1998, ...).</rdfs:comment>
    </owl:Class>
    


    <!-- http://www.nist.gov/itl/ssd/OntologyRequirements#TwoDimensionalArray -->

    <owl:Class rdf:about="&or;TwoDimensionalArray">
        <rdfs:subClassOf rdf:resource="&or;Array"/>
        <rdfs:comment xml:lang="en">A Two Dimensional Array is an Array of rows and columns, with each row the same length and each column the same length.  Any cell of the array can be uniquely referenced by its row and column.</rdfs:comment>
    </owl:Class>
    


    <!-- http://www.nist.gov/itl/ssd/OntologyRequirements#TwoDimensionalImage -->

    <owl:Class rdf:about="&or;TwoDimensionalImage">
        <rdfs:subClassOf rdf:resource="&or;Image"/>
        <rdfs:comment xml:lang="en">An image with two spatial dimensions, in contrast with a ThreeDimensionalImage.</rdfs:comment>
    </owl:Class>
    


    <!-- http://www.nist.gov/itl/ssd/OntologyRequirements#UnitOfAcceleration -->

    <owl:Class rdf:about="&or;UnitOfAcceleration">
        <rdfs:subClassOf rdf:resource="&or;UnitOfMeasure"/>
        <owl:disjointWith rdf:resource="&or;UnitOfArea"/>
        <owl:disjointWith rdf:resource="&or;UnitOfComputerStorageCapacity"/>
        <owl:disjointWith rdf:resource="&or;UnitOfDensity"/>
        <owl:disjointWith rdf:resource="&or;UnitOfDistance"/>
        <owl:disjointWith rdf:resource="&or;UnitOfDuration"/>
        <owl:disjointWith rdf:resource="&or;UnitOfEnergy"/>
        <owl:disjointWith rdf:resource="&or;UnitOfForce"/>
        <owl:disjointWith rdf:resource="&or;UnitOfMass"/>
        <owl:disjointWith rdf:resource="&or;UnitOfPressure"/>
        <owl:disjointWith rdf:resource="&or;UnitOfSpreadRate"/>
        <owl:disjointWith rdf:resource="&or;UnitOfTemperature"/>
        <owl:disjointWith rdf:resource="&or;UnitOfVelocity"/>
        <owl:disjointWith rdf:resource="&or;UnitOfVoltage"/>
        <owl:disjointWith rdf:resource="&or;UnitOfVolume"/>
        <rdfs:comment xml:lang="en">A Unit of Acceleration is a Unit Of Measure specifying an amout of distance per unit of duration squared, for example centimeters per second per second.</rdfs:comment>
    </owl:Class>
    


    <!-- http://www.nist.gov/itl/ssd/OntologyRequirements#UnitOfArea -->

    <owl:Class rdf:about="&or;UnitOfArea">
        <rdfs:subClassOf rdf:resource="&or;UnitOfMeasure"/>
        <owl:disjointWith rdf:resource="&or;UnitOfDistance"/>
        <owl:disjointWith rdf:resource="&or;UnitOfDuration"/>
        <owl:disjointWith rdf:resource="&or;UnitOfEnergy"/>
        <owl:disjointWith rdf:resource="&or;UnitOfForce"/>
        <owl:disjointWith rdf:resource="&or;UnitOfMass"/>
        <owl:disjointWith rdf:resource="&or;UnitOfPressure"/>
        <owl:disjointWith rdf:resource="&or;UnitOfSpreadRate"/>
        <owl:disjointWith rdf:resource="&or;UnitOfTemperature"/>
        <owl:disjointWith rdf:resource="&or;UnitOfVelocity"/>
        <owl:disjointWith rdf:resource="&or;UnitOfVoltage"/>
        <owl:disjointWith rdf:resource="&or;UnitOfVolume"/>
        <rdfs:comment xml:lang="en">A Unit of Area is a Unit Of Measure specifying an amout of area, for example square centimeter.</rdfs:comment>
    </owl:Class>
    


    <!-- http://www.nist.gov/itl/ssd/OntologyRequirements#UnitOfComputerStorageCapacity -->

    <owl:Class rdf:about="&or;UnitOfComputerStorageCapacity">
        <rdfs:subClassOf rdf:resource="&or;UnitOfMeasure"/>
        <owl:disjointWith rdf:resource="&or;UnitOfDistance"/>
        <owl:disjointWith rdf:resource="&or;UnitOfDuration"/>
        <owl:disjointWith rdf:resource="&or;UnitOfEnergy"/>
        <owl:disjointWith rdf:resource="&or;UnitOfForce"/>
        <owl:disjointWith rdf:resource="&or;UnitOfMass"/>
        <owl:disjointWith rdf:resource="&or;UnitOfPressure"/>
        <owl:disjointWith rdf:resource="&or;UnitOfSpreadRate"/>
        <owl:disjointWith rdf:resource="&or;UnitOfTemperature"/>
        <owl:disjointWith rdf:resource="&or;UnitOfVelocity"/>
        <owl:disjointWith rdf:resource="&or;UnitOfVoltage"/>
        <owl:disjointWith rdf:resource="&or;UnitOfVolume"/>
        <rdfs:comment xml:lang="en">A Unit of Comuter Storage Capacity is a Unit Of Measure specifying an amout of computer memory, for example bit, byte, pixel.</rdfs:comment>
    </owl:Class>
    


    <!-- http://www.nist.gov/itl/ssd/OntologyRequirements#UnitOfDensity -->

    <owl:Class rdf:about="&or;UnitOfDensity">
        <rdfs:subClassOf rdf:resource="&or;UnitOfMeasure"/>
        <owl:disjointWith rdf:resource="&or;UnitOfEnergy"/>
        <owl:disjointWith rdf:resource="&or;UnitOfForce"/>
        <owl:disjointWith rdf:resource="&or;UnitOfMass"/>
        <owl:disjointWith rdf:resource="&or;UnitOfPressure"/>
        <owl:disjointWith rdf:resource="&or;UnitOfSpreadRate"/>
        <owl:disjointWith rdf:resource="&or;UnitOfTemperature"/>
        <owl:disjointWith rdf:resource="&or;UnitOfVelocity"/>
        <owl:disjointWith rdf:resource="&or;UnitOfVoltage"/>
        <owl:disjointWith rdf:resource="&or;UnitOfVolume"/>
        <rdfs:comment xml:lang="en">A Unit of Density is a Unit Of Measure specifying an amout of mass per unit of volume, for example grams per cc.</rdfs:comment>
    </owl:Class>
    


    <!-- http://www.nist.gov/itl/ssd/OntologyRequirements#UnitOfDistance -->

    <owl:Class rdf:about="&or;UnitOfDistance">
        <rdfs:subClassOf rdf:resource="&or;UnitOfMeasure"/>
        <owl:disjointWith rdf:resource="&or;UnitOfDuration"/>
        <owl:disjointWith rdf:resource="&or;UnitOfEnergy"/>
        <owl:disjointWith rdf:resource="&or;UnitOfForce"/>
        <owl:disjointWith rdf:resource="&or;UnitOfMass"/>
        <owl:disjointWith rdf:resource="&or;UnitOfPressure"/>
        <owl:disjointWith rdf:resource="&or;UnitOfSpreadRate"/>
        <owl:disjointWith rdf:resource="&or;UnitOfTemperature"/>
        <owl:disjointWith rdf:resource="&or;UnitOfVelocity"/>
        <owl:disjointWith rdf:resource="&or;UnitOfVoltage"/>
        <owl:disjointWith rdf:resource="&or;UnitOfVolume"/>
        <rdfs:comment xml:lang="en">A Unit of Distance is a Unit Of Measure specifying the length between two points, for example a centimeter.</rdfs:comment>
    </owl:Class>
    


    <!-- http://www.nist.gov/itl/ssd/OntologyRequirements#UnitOfDuration -->

    <owl:Class rdf:about="&or;UnitOfDuration">
        <rdfs:subClassOf rdf:resource="&or;UnitOfMeasure"/>
        <owl:disjointWith rdf:resource="&or;UnitOfEnergy"/>
        <owl:disjointWith rdf:resource="&or;UnitOfForce"/>
        <owl:disjointWith rdf:resource="&or;UnitOfMass"/>
        <owl:disjointWith rdf:resource="&or;UnitOfPressure"/>
        <owl:disjointWith rdf:resource="&or;UnitOfSpreadRate"/>
        <owl:disjointWith rdf:resource="&or;UnitOfTemperature"/>
        <owl:disjointWith rdf:resource="&or;UnitOfVelocity"/>
        <owl:disjointWith rdf:resource="&or;UnitOfVoltage"/>
        <owl:disjointWith rdf:resource="&or;UnitOfVolume"/>
        <rdfs:comment xml:lang="en">A Unit of Duration is a Unit Of Measure specifying an amout of time between two time points, for example a second.</rdfs:comment>
    </owl:Class>
    


    <!-- http://www.nist.gov/itl/ssd/OntologyRequirements#UnitOfEnergy -->

    <owl:Class rdf:about="&or;UnitOfEnergy">
        <rdfs:subClassOf rdf:resource="&or;UnitOfMeasure"/>
        <owl:disjointWith rdf:resource="&or;UnitOfForce"/>
        <owl:disjointWith rdf:resource="&or;UnitOfMass"/>
        <owl:disjointWith rdf:resource="&or;UnitOfPressure"/>
        <owl:disjointWith rdf:resource="&or;UnitOfSpreadRate"/>
        <owl:disjointWith rdf:resource="&or;UnitOfTemperature"/>
        <owl:disjointWith rdf:resource="&or;UnitOfVelocity"/>
        <owl:disjointWith rdf:resource="&or;UnitOfVoltage"/>
        <owl:disjointWith rdf:resource="&or;UnitOfVolume"/>
        <rdfs:comment xml:lang="en">A Unit of Energy is a Unit Of Measure specifying an amout of energy, for example joule or kilowatt hour.</rdfs:comment>
    </owl:Class>
    


    <!-- http://www.nist.gov/itl/ssd/OntologyRequirements#UnitOfForce -->

    <owl:Class rdf:about="&or;UnitOfForce">
        <rdfs:subClassOf rdf:resource="&or;UnitOfMeasure"/>
        <owl:disjointWith rdf:resource="&or;UnitOfMass"/>
        <owl:disjointWith rdf:resource="&or;UnitOfPressure"/>
        <owl:disjointWith rdf:resource="&or;UnitOfSpreadRate"/>
        <owl:disjointWith rdf:resource="&or;UnitOfTemperature"/>
        <owl:disjointWith rdf:resource="&or;UnitOfVelocity"/>
        <owl:disjointWith rdf:resource="&or;UnitOfVoltage"/>
        <owl:disjointWith rdf:resource="&or;UnitOfVolume"/>
        <rdfs:comment xml:lang="en">A Unit of Force is a Unit Of Measure specifying an amout of force (mass times acceleration), for example a newton.</rdfs:comment>
    </owl:Class>
    


    <!-- http://www.nist.gov/itl/ssd/OntologyRequirements#UnitOfMass -->

    <owl:Class rdf:about="&or;UnitOfMass">
        <rdfs:subClassOf rdf:resource="&or;UnitOfMeasure"/>
        <owl:disjointWith rdf:resource="&or;UnitOfPressure"/>
        <owl:disjointWith rdf:resource="&or;UnitOfSpreadRate"/>
        <owl:disjointWith rdf:resource="&or;UnitOfTemperature"/>
        <owl:disjointWith rdf:resource="&or;UnitOfVelocity"/>
        <owl:disjointWith rdf:resource="&or;UnitOfVoltage"/>
        <owl:disjointWith rdf:resource="&or;UnitOfVolume"/>
        <rdfs:comment xml:lang="en">A Unit of mass is a Unit Of Measure specifying an amout of mass, for example a gram or kilogram.</rdfs:comment>
    </owl:Class>
    


    <!-- http://www.nist.gov/itl/ssd/OntologyRequirements#UnitOfMeasure -->

    <owl:Class rdf:about="&or;UnitOfMeasure">
        <rdfs:subClassOf rdf:resource="&or;NonTangibleThing"/>
    </owl:Class>
    


    <!-- http://www.nist.gov/itl/ssd/OntologyRequirements#UnitOfPressure -->

    <owl:Class rdf:about="&or;UnitOfPressure">
        <rdfs:subClassOf rdf:resource="&or;UnitOfMeasure"/>
        <owl:disjointWith rdf:resource="&or;UnitOfSpreadRate"/>
        <owl:disjointWith rdf:resource="&or;UnitOfTemperature"/>
        <owl:disjointWith rdf:resource="&or;UnitOfVelocity"/>
        <owl:disjointWith rdf:resource="&or;UnitOfVoltage"/>
        <owl:disjointWith rdf:resource="&or;UnitOfVolume"/>
        <rdfs:comment xml:lang="en">A Unit of pressure is a Unit Of Measure specifying an amout of force per unit of area, for example pascal or PSI.</rdfs:comment>
    </owl:Class>
    


    <!-- http://www.nist.gov/itl/ssd/OntologyRequirements#UnitOfSpreadRate -->

    <owl:Class rdf:about="&or;UnitOfSpreadRate">
        <rdfs:subClassOf rdf:resource="&or;UnitOfMeasure"/>
        <owl:disjointWith rdf:resource="&or;UnitOfTemperature"/>
        <owl:disjointWith rdf:resource="&or;UnitOfVelocity"/>
        <owl:disjointWith rdf:resource="&or;UnitOfVoltage"/>
        <owl:disjointWith rdf:resource="&or;UnitOfVolume"/>
        <rdfs:comment xml:lang="en">A Unit of Spread Rate is a Unit Of Measure specifying an amout of area per unit of duration, for example square centimeters per second.</rdfs:comment>
    </owl:Class>
    


    <!-- http://www.nist.gov/itl/ssd/OntologyRequirements#UnitOfTemperature -->

    <owl:Class rdf:about="&or;UnitOfTemperature">
        <rdfs:subClassOf rdf:resource="&or;UnitOfMeasure"/>
        <owl:disjointWith rdf:resource="&or;UnitOfVelocity"/>
        <owl:disjointWith rdf:resource="&or;UnitOfVoltage"/>
        <owl:disjointWith rdf:resource="&or;UnitOfVolume"/>
        <rdfs:comment xml:lang="en">A Unit of Temperature is a Unit Of Measure specifying the temperature of something, for example Degree Celsius or Degree Kelvin.</rdfs:comment>
    </owl:Class>
    


    <!-- http://www.nist.gov/itl/ssd/OntologyRequirements#UnitOfVelocity -->

    <owl:Class rdf:about="&or;UnitOfVelocity">
        <rdfs:subClassOf rdf:resource="&or;UnitOfMeasure"/>
        <owl:disjointWith rdf:resource="&or;UnitOfVoltage"/>
        <owl:disjointWith rdf:resource="&or;UnitOfVolume"/>
        <rdfs:comment xml:lang="en">A Unit of Velocity is a Unit Of Measure for specifying a speed, for example meters per second.</rdfs:comment>
    </owl:Class>
    


    <!-- http://www.nist.gov/itl/ssd/OntologyRequirements#UnitOfVelocitySquared -->

    <owl:Class rdf:about="&or;UnitOfVelocitySquared">
        <rdfs:subClassOf rdf:resource="&or;UnitOfMeasure"/>
        <rdfs:comment xml:lang="en">A Unit of Velocity Squared is a Unit Of Measure specifying the square of a velocity, for example square centimeters per second per second.</rdfs:comment>
    </owl:Class>
    


    <!-- http://www.nist.gov/itl/ssd/OntologyRequirements#UnitOfVoltage -->

    <owl:Class rdf:about="&or;UnitOfVoltage">
        <rdfs:subClassOf rdf:resource="&or;UnitOfMeasure"/>
        <rdfs:comment xml:lang="en">A Unit of Voltge is a Unit Of Measure specifying an amout of electrical potential, for example a volt.</rdfs:comment>
    </owl:Class>
    


    <!-- http://www.nist.gov/itl/ssd/OntologyRequirements#UnitOfVolume -->

    <owl:Class rdf:about="&or;UnitOfVolume">
        <rdfs:subClassOf rdf:resource="&or;UnitOfMeasure"/>
        <rdfs:comment xml:lang="en">A Unit of Volume is a Unit Of Measure specifying an amout of space something takes up, for example a liter.</rdfs:comment>
    </owl:Class>
    


    <!-- http://www.nist.gov/itl/ssd/OntologyRequirements#UnitPrice -->

    <owl:Class rdf:about="&or;UnitPrice">
        <rdfs:subClassOf rdf:resource="&or;MeasurableProperty"/>
        <rdfs:comment xml:lang="en">A unit price is the price (in some currency) of a given amount of some type of thing.  The amount may be per physical object, per mass, per volume, per occurrence (of some type of event), per duration (of some type of event), etc.</rdfs:comment>
    </owl:Class>
    


    <!-- http://www.nist.gov/itl/ssd/OntologyRequirements#UnitPricePerDuration -->

    <owl:Class rdf:about="&or;UnitPricePerDuration">
        <rdfs:subClassOf rdf:resource="&or;UnitPrice"/>
        <owl:disjointWith rdf:resource="&or;UnitPricePerMass"/>
        <owl:disjointWith rdf:resource="&or;UnitPricePerObject"/>
        <owl:disjointWith rdf:resource="&or;UnitPricePerOccurrence"/>
        <owl:disjointWith rdf:resource="&or;UnitPricePerVolume"/>
        <rdfs:comment xml:lang="en">A unit price per duration is the price (in some currency) of asome type of event for some amount of time.</rdfs:comment>
    </owl:Class>
    


    <!-- http://www.nist.gov/itl/ssd/OntologyRequirements#UnitPricePerMass -->

    <owl:Class rdf:about="&or;UnitPricePerMass">
        <rdfs:subClassOf rdf:resource="&or;UnitPrice"/>
        <owl:disjointWith rdf:resource="&or;UnitPricePerObject"/>
        <owl:disjointWith rdf:resource="&or;UnitPricePerOccurrence"/>
        <owl:disjointWith rdf:resource="&or;UnitPricePerVolume"/>
        <rdfs:comment xml:lang="en">A unit price per mass is the price (in some currency) of a single object of some type.</rdfs:comment>
    </owl:Class>
    


    <!-- http://www.nist.gov/itl/ssd/OntologyRequirements#UnitPricePerObject -->

    <owl:Class rdf:about="&or;UnitPricePerObject">
        <rdfs:subClassOf rdf:resource="&or;UnitPrice"/>
        <rdfs:subClassOf>
            <owl:Restriction>
                <owl:onProperty rdf:resource="&or;unitsFor"/>
                <owl:someValuesFrom rdf:resource="&or;CurrencyUnit"/>
            </owl:Restriction>
        </rdfs:subClassOf>
        <owl:disjointWith rdf:resource="&or;UnitPricePerOccurrence"/>
        <owl:disjointWith rdf:resource="&or;UnitPricePerVolume"/>
    </owl:Class>
    


    <!-- http://www.nist.gov/itl/ssd/OntologyRequirements#UnitPricePerOccurrence -->

    <owl:Class rdf:about="&or;UnitPricePerOccurrence">
        <rdfs:subClassOf rdf:resource="&or;UnitPrice"/>
        <rdfs:subClassOf>
            <owl:Restriction>
                <owl:onProperty rdf:resource="&or;unitsFor"/>
                <owl:someValuesFrom rdf:resource="&or;CurrencyUnit"/>
            </owl:Restriction>
        </rdfs:subClassOf>
        <owl:disjointWith rdf:resource="&or;UnitPricePerVolume"/>
        <rdfs:comment xml:lang="en">A unit price is the price (in some currency) of a occurrence of some type of event.</rdfs:comment>
    </owl:Class>
    


    <!-- http://www.nist.gov/itl/ssd/OntologyRequirements#UnitPricePerVolume -->

    <owl:Class rdf:about="&or;UnitPricePerVolume">
        <rdfs:subClassOf rdf:resource="&or;UnitPrice"/>
        <rdfs:comment xml:lang="en">A unit price per volume is the price (in some currency) of a given volume of some type of thing.</rdfs:comment>
    </owl:Class>
    


    <!-- http://www.nist.gov/itl/ssd/OntologyRequirements#Validating -->

    <owl:Class rdf:about="&or;Validating">
        <rdfs:subClassOf rdf:resource="&or;Evaluation"/>
        <rdfs:comment xml:lang="en">Verifying is the action of determining that something meets specified criteria.</rdfs:comment>
    </owl:Class>
    


    <!-- http://www.nist.gov/itl/ssd/OntologyRequirements#VisualImage -->

    <owl:Class rdf:about="&or;VisualImage">
        <rdfs:subClassOf rdf:resource="&or;Image"/>
        <rdfs:comment xml:lang="en">Those images that can be directly viewed, including film, prints, displayed images on screens, and projected images.  Images stored in computer files are not included -- see Computer Image File.</rdfs:comment>
    </owl:Class>
    


    <!-- http://www.nist.gov/itl/ssd/OntologyRequirements#Volume -->

    <owl:Class rdf:about="&or;Volume">
        <owl:equivalentClass>
            <owl:Class>
                <owl:intersectionOf rdf:parseType="Collection">
                    <rdf:Description rdf:about="&or;MeasurableQuantity"/>
                    <owl:Restriction>
                        <owl:onProperty rdf:resource="&or;unitsFor"/>
                        <owl:someValuesFrom rdf:resource="&or;UnitOfVolume"/>
                    </owl:Restriction>
                </owl:intersectionOf>
            </owl:Class>
        </owl:equivalentClass>
        <rdfs:subClassOf rdf:resource="&or;MeasurableQuantity"/>
        <rdfs:subClassOf>
            <owl:Restriction>
                <owl:onProperty rdf:resource="&or;unitsFor"/>
                <owl:allValuesFrom rdf:resource="&or;UnitOfVolume"/>
            </owl:Restriction>
        </rdfs:subClassOf>
    </owl:Class>
    


    <!-- http://www.nist.gov/itl/ssd/OntologyRequirements#Wire -->

    <owl:Class rdf:about="&or;Wire">
        <rdfs:subClassOf rdf:resource="&or;Artifact"/>
        <rdfs:subClassOf rdf:resource="&or;RigidPortableObject"/>
    </owl:Class>
    


    <!-- http://www.w3.org/1999/02/22-rdf-syntax-ns#Property -->

    <rdf:Description rdf:about="&rdf;Property">
        <rdfs:subClassOf rdf:resource="&or;NonTangibleThing"/>
    </rdf:Description>
    


    <!-- http://www.w3.org/2000/10/XMLSchema#nonNegativeInteger -->

    <rdf:Description rdf:about="&XMLSchema;nonNegativeInteger">
        <rdfs:subClassOf rdf:resource="&rdfs;Literal"/>
    </rdf:Description>
    


    <!-- http://www.w3.org/2001/XMLSchema#url -->

    <owl:Class rdf:about="&xsd;url"/>
    


    <!-- http://www.w3.org/2002/07/owl#ObjectProperty -->

    <rdf:Description rdf:about="&owl;ObjectProperty">
        <rdfs:subClassOf rdf:resource="&rdf;Property"/>
    </rdf:Description>
    


    <!-- http://www.w3.org/2002/07/owl#Thing -->

    <rdf:Description rdf:about="&owl;Thing"/>
    


    <!-- 
    ///////////////////////////////////////////////////////////////////////////////////////
    //
    // Individuals
    //
    ///////////////////////////////////////////////////////////////////////////////////////
     -->

    


    <!-- http://www.nist.gov/itl/ssd/OntologyRequirements#AIFF_File_Format -->

    <owl:NamedIndividual rdf:about="&or;AIFF_File_Format">
        <rdf:type rdf:resource="&or;AudioFileFormat"/>
        <defaultFileExtension rdf:datatype="&xsd;Name">aif</defaultFileExtension>
        <defaultFileExtension rdf:datatype="&xsd;Name">aiff</defaultFileExtension>
        <rdfs:comment xml:lang="en">Apple Computer&#39;s audio file format based on the Interchange File Format (IFF).</rdfs:comment>
    </owl:NamedIndividual>
    


    <!-- http://www.nist.gov/itl/ssd/OntologyRequirements#Anatomy -->

    <owl:NamedIndividual rdf:about="&or;Anatomy">
        <rdf:type rdf:resource="&or;BiomedicalFieldOfStudy"/>
        <subFieldOf rdf:resource="&or;Biomedicine"/>
    </owl:NamedIndividual>
    


    <!-- http://www.nist.gov/itl/ssd/OntologyRequirements#April -->

    <owl:NamedIndividual rdf:about="&or;April">
        <rdf:type rdf:resource="&or;MonthOfYearType"/>
        <rdfs:comment xml:lang="en">The month of April</rdfs:comment>
    </owl:NamedIndividual>
    


    <!-- http://www.nist.gov/itl/ssd/OntologyRequirements#Area -->

    <owl:NamedIndividual rdf:about="&or;Area">
        <rdf:type rdf:resource="&or;MeasurableQuantityType"/>
        <rdfs:comment xml:lang="en">An  Area is an amount of two-dimensional space.</rdfs:comment>
    </owl:NamedIndividual>
    


    <!-- http://www.nist.gov/itl/ssd/OntologyRequirements#Atmosphere-UnitOfPressure -->

    <owl:NamedIndividual rdf:about="&or;Atmosphere-UnitOfPressure">
        <rdf:type rdf:resource="&or;NonMetricUnit"/>
        <rdf:type rdf:resource="&or;UnitOfPressure"/>
        <rdfs:comment xml:lang="en">One Atmosphere is the average pressure of the Earth&#39;s atmosphere at sea level,  It is defined as equal to 101,325 Pascals.</rdfs:comment>
    </owl:NamedIndividual>
    


    <!-- http://www.nist.gov/itl/ssd/OntologyRequirements#AtomicMassUnit -->

    <owl:NamedIndividual rdf:about="&or;AtomicMassUnit">
        <rdf:type rdf:resource="&or;NonMetricUnit"/>
        <rdf:type rdf:resource="&or;UnitOfMass"/>
    </owl:NamedIndividual>
    


    <!-- http://www.nist.gov/itl/ssd/OntologyRequirements#August -->

    <owl:NamedIndividual rdf:about="&or;August">
        <rdf:type rdf:resource="&or;MonthOfYearType"/>
        <rdfs:comment xml:lang="en">The month of August</rdfs:comment>
    </owl:NamedIndividual>
    


    <!-- http://www.nist.gov/itl/ssd/OntologyRequirements#AvogadrosNumber -->

    <owl:NamedIndividual rdf:about="&or;AvogadrosNumber">
        <rdf:type rdf:resource="&or;DimensionlessUnit"/>
        <rdfs:comment xml:lang="en">Avogadro&#39;s Number is the number of atoms in a mole of those atoms.  It is a Unit of Measure equal to about 6.0221421 x 10^23.</rdfs:comment>
    </owl:NamedIndividual>
    


    <!-- http://www.nist.gov/itl/ssd/OntologyRequirements#Bar-UnitOfPressure -->

    <owl:NamedIndividual rdf:about="&or;Bar-UnitOfPressure">
        <rdf:type rdf:resource="&or;MetricUnit"/>
        <rdf:type rdf:resource="&or;UnitOfPressure"/>
        <rdfs:comment xml:lang="en">A UnitOfPressure, one Bar is equal to 100,000 Pascals, about 1 Atmosphere presssure.</rdfs:comment>
    </owl:NamedIndividual>
    


    <!-- http://www.nist.gov/itl/ssd/OntologyRequirements#BioRadPic_File_Format -->

    <owl:NamedIndividual rdf:about="&or;BioRadPic_File_Format">
        <rdf:type rdf:resource="&or;MicroscopyImageFileFormat"/>
        <defaultFileExtension rdf:datatype="&xsd;Name">pic</defaultFileExtension>
        <defaultFileExtension rdf:datatype="&xsd;Name">raw</defaultFileExtension>
        <defaultFileExtension rdf:datatype="&xsd;Name">xml</defaultFileExtension>
        <rdfs:comment xml:lang="en">The Bio-Rad Pic file format for laser microscopy images.</rdfs:comment>
    </owl:NamedIndividual>
    


    <!-- http://www.nist.gov/itl/ssd/OntologyRequirements#Biochemistry -->

    <owl:NamedIndividual rdf:about="&or;Biochemistry">
        <rdf:type rdf:resource="&or;BiomedicalFieldOfStudy"/>
        <subFieldOf rdf:resource="&or;Chemistry"/>
    </owl:NamedIndividual>
    


    <!-- http://www.nist.gov/itl/ssd/OntologyRequirements#Bioinfomatics -->

    <owl:NamedIndividual rdf:about="&or;Bioinfomatics">
        <rdf:type rdf:resource="&or;BiomedicalFieldOfStudy"/>
        <subFieldOf rdf:resource="&or;Biomedicine"/>
        <subFieldOf rdf:resource="&or;ComputerScience"/>
    </owl:NamedIndividual>
    


    <!-- http://www.nist.gov/itl/ssd/OntologyRequirements#BiologicalFunctionFOS -->

    <owl:NamedIndividual rdf:about="&or;BiologicalFunctionFOS">
        <rdf:type rdf:resource="&or;BiomedicalFieldOfStudy"/>
        <subFieldOf rdf:resource="&or;Biology"/>
    </owl:NamedIndividual>
    


    <!-- http://www.nist.gov/itl/ssd/OntologyRequirements#BiologicalProcessFOS -->

    <owl:NamedIndividual rdf:about="&or;BiologicalProcessFOS">
        <rdf:type rdf:resource="&or;BiomedicalFieldOfStudy"/>
        <subFieldOf rdf:resource="&or;Biology"/>
    </owl:NamedIndividual>
    


    <!-- http://www.nist.gov/itl/ssd/OntologyRequirements#Biology -->

    <owl:NamedIndividual rdf:about="&or;Biology">
        <rdf:type rdf:resource="&or;BiomedicalFieldOfStudy"/>
    </owl:NamedIndividual>
    


    <!-- http://www.nist.gov/itl/ssd/OntologyRequirements#Biomedicine -->

    <owl:NamedIndividual rdf:about="&or;Biomedicine">
        <rdf:type rdf:resource="&or;BiomedicalFieldOfStudy"/>
        <rdfs:comment xml:lang="en">Biomedicine is a subfield of medical science that applies biological principles to clinical practice.</rdfs:comment>
        <subFieldOf rdf:resource="&or;Biology"/>
        <subFieldOf rdf:resource="&or;HealthCareFOS"/>
    </owl:NamedIndividual>
    


    <!-- http://www.nist.gov/itl/ssd/OntologyRequirements#Bit -->

    <owl:NamedIndividual rdf:about="&or;Bit">
        <rdf:type rdf:resource="&or;NonMetricUnit"/>
        <rdf:type rdf:resource="&or;UnitOfComputerStorageCapacity"/>
    </owl:NamedIndividual>
    


    <!-- http://www.nist.gov/itl/ssd/OntologyRequirements#BritishThermalUnit -->

    <owl:NamedIndividual rdf:about="&or;BritishThermalUnit">
        <rdf:type rdf:resource="&or;NonMetricUnit"/>
        <rdf:type rdf:resource="&or;UnitOfEnergy"/>
    </owl:NamedIndividual>
    


    <!-- http://www.nist.gov/itl/ssd/OntologyRequirements#Byte -->

    <owl:NamedIndividual rdf:about="&or;Byte">
        <rdf:type rdf:resource="&or;NonMetricUnit"/>
        <rdf:type rdf:resource="&or;UnitOfComputerStorageCapacity"/>
    </owl:NamedIndividual>
    


    <!-- http://www.nist.gov/itl/ssd/OntologyRequirements#CHEBI_Ontology -->

    <owl:NamedIndividual rdf:about="&or;CHEBI_Ontology">
        <rdf:type rdf:resource="&oil;Ontology"/>
        <standardNamespacePrefix rdf:datatype="&xsd;NMTOKEN">CHEBI</standardNamespacePrefix>
        <nameSpaceURI rdf:datatype="&xsd;anyURI">http://purl.org/obo/owl/CHEBI#</nameSpaceURI>
        <rdfs:comment>Chemical Entities of Biological Interest  ontology</rdfs:comment>
        <ontologyDomain rdf:resource="&or;Biochemistry"/>
    </owl:NamedIndividual>
    


    <!-- http://www.nist.gov/itl/ssd/OntologyRequirements#CellTypeOntology -->

    <owl:NamedIndividual rdf:about="&or;CellTypeOntology">
        <rdf:type rdf:resource="&oil;Ontology"/>
        <standardNamespacePrefix rdf:datatype="&xsd;NMTOKEN">CL</standardNamespacePrefix>
        <nameSpaceURI rdf:datatype="&xsd;anyURI">http://purl.obolibrary.org/obo/cl#</nameSpaceURI>
        <ontologyDomain rdf:resource="&or;Anatomy"/>
    </owl:NamedIndividual>
    


    <!-- http://www.nist.gov/itl/ssd/OntologyRequirements#Centimeter -->

    <owl:NamedIndividual rdf:about="&or;Centimeter">
        <rdf:type rdf:resource="&or;CGS_Unit"/>
        <rdf:type rdf:resource="&or;UnitOfDistance"/>
    </owl:NamedIndividual>
    


    <!-- http://www.nist.gov/itl/ssd/OntologyRequirements#Chemistry -->

    <owl:NamedIndividual rdf:about="&or;Chemistry">
        <rdf:type rdf:resource="&or;FieldOfStudy"/>
    </owl:NamedIndividual>
    


    <!-- http://www.nist.gov/itl/ssd/OntologyRequirements#ComputerScience -->

    <owl:NamedIndividual rdf:about="&or;ComputerScience">
        <rdf:type rdf:resource="&or;FieldOfStudy"/>
    </owl:NamedIndividual>
    


    <!-- http://www.nist.gov/itl/ssd/OntologyRequirements#ComputerStorageCapacity -->

    <owl:NamedIndividual rdf:about="&or;ComputerStorageCapacity">
        <rdf:type rdf:resource="&or;MeasurableQuantityType"/>
    </owl:NamedIndividual>
    


    <!-- http://www.nist.gov/itl/ssd/OntologyRequirements#Count -->

    <owl:NamedIndividual rdf:about="&or;Count">
        <rdf:type rdf:resource="&or;MeasurableQuantityType"/>
        <rdfs:comment xml:lang="en">A Count is a quantity that can be expressed in integers or some multiple of 1 such as moles.</rdfs:comment>
    </owl:NamedIndividual>
    


    <!-- http://www.nist.gov/itl/ssd/OntologyRequirements#CubicMeter -->

    <owl:NamedIndividual rdf:about="&or;CubicMeter">
        <rdf:type rdf:resource="&or;SI_Unit"/>
        <rdf:type rdf:resource="&or;UnitOfVolume"/>
    </owl:NamedIndividual>
    


    <!-- http://www.nist.gov/itl/ssd/OntologyRequirements#DIALOG_Ontology -->

    <owl:NamedIndividual rdf:about="&or;DIALOG_Ontology">
        <rdf:type rdf:resource="&oil;Ontology"/>
        <standardNamespacePrefix rdf:datatype="&xsd;NMTOKEN">di</standardNamespacePrefix>
        <referenceURL rdf:datatype="&xsd;anyURI">http://www.dfrws.org/2009/proceedings/p23-kahvedzic.pdf</referenceURL>
        <rdfs:comment xml:lang="en">DIALOG is the ``Digital Investigation Ontology&#39; &#39; designed as an ontology for Digital Forensics.  </rdfs:comment>
        <ontologyDomain rdf:resource="&or;DigitalForensics"/>
    </owl:NamedIndividual>
    


    <!-- http://www.nist.gov/itl/ssd/OntologyRequirements#DaysDuration -->

    <owl:NamedIndividual rdf:about="&or;DaysDuration">
        <rdf:type rdf:resource="&or;UnitOfDuration"/>
    </owl:NamedIndividual>
    


    <!-- http://www.nist.gov/itl/ssd/OntologyRequirements#December -->

    <owl:NamedIndividual rdf:about="&or;December">
        <rdf:type rdf:resource="&or;MonthOfYearType"/>
        <rdfs:comment xml:lang="en">The month of December</rdfs:comment>
    </owl:NamedIndividual>
    


    <!-- http://www.nist.gov/itl/ssd/OntologyRequirements#DegreeCelsius -->

    <owl:NamedIndividual rdf:about="&or;DegreeCelsius">
        <rdf:type rdf:resource="&or;MetricUnit"/>
        <rdf:type rdf:resource="&or;UnitOfTemperature"/>
        <rdfs:comment xml:lang="en">A Degree Celsius is a Unit of Measure for how many degrees the temperature of something is above the freezing point of water (0 C). the boiling point of water (at 1.05*10^5 pascals) is 100 C and absolute zero is -273.15 C.  </rdfs:comment>
        <termString xml:lang="en">Celsius</termString>
        <skos:note xml:lang="en">Note that as units of temperature, N Degrees Celsius = N + 273.15 Degrees Kelvin,  but as units of temperature difference N Celsius degrees = N Kelvin degrees.</skos:note>
        <termString xml:lang="en">centigrade</termString>
    </owl:NamedIndividual>
    


    <!-- http://www.nist.gov/itl/ssd/OntologyRequirements#DegreeFahrenheit -->

    <owl:NamedIndividual rdf:about="&or;DegreeFahrenheit">
        <rdf:type rdf:resource="&or;NonMetricUnit"/>
        <rdf:type rdf:resource="&or;UnitOfTemperature"/>
        <rdfs:comment xml:lang="en">A Degree Fahrenheit is a Unit of Measure such that the freezing point of water is 32 F and the boiling point of water (at 1.05*10^5 pascals) is 212 F.</rdfs:comment>
        <termString xml:lang="en">Fahrenheit</termString>
    </owl:NamedIndividual>
    


    <!-- http://www.nist.gov/itl/ssd/OntologyRequirements#DegreeKelvin -->

    <owl:NamedIndividual rdf:about="&or;DegreeKelvin">
        <rdf:type rdf:resource="&or;SI_Unit"/>
        <rdf:type rdf:resource="&or;UnitOfTemperature"/>
        <rdfs:comment xml:lang="en">A kelvin is a Unit of Measure for how many degrees the temperature of something is above absolute zero (0 K).  The freezing point of water is 273.15 K and the boiling point (at 1.05*10^5 pascals) is 373.15.  </rdfs:comment>
        <skos:note xml:lang="en">Note that as units of temperature, N Degrees Celsius = N + 273.15 Degrees Kelvin,  but as units of temperature difference N Celsius degrees = N Kelvin degrees.</skos:note>
        <termString xml:lang="en">kelvin</termString>
    </owl:NamedIndividual>
    


    <!-- http://www.nist.gov/itl/ssd/OntologyRequirements#DerivedDataRole -->

    <owl:NamedIndividual rdf:about="&or;DerivedDataRole">
        <rdf:type rdf:resource="&or;MeasurementRole"/>
    </owl:NamedIndividual>
    


    <!-- http://www.nist.gov/itl/ssd/OntologyRequirements#DigitalForensics -->

    <owl:NamedIndividual rdf:about="&or;DigitalForensics">
        <rdf:type rdf:resource="&or;FieldOfStudy"/>
        <rdfs:comment xml:lang="en">Digital Forensics is the subfield of Forensic Science dealing with investigation and recovery of information from digital devices, normally in the search for evidence of crime.</rdfs:comment>
        <subFieldOf rdf:resource="&or;ComputerScience"/>
        <subFieldOf rdf:resource="&or;ForensicScience"/>
    </owl:NamedIndividual>
    


    <!-- http://www.nist.gov/itl/ssd/OntologyRequirements#DimensionlessUnit -->

    <owl:NamedIndividual rdf:about="&or;DimensionlessUnit">
        <rdf:type rdf:resource="&or;InterconvertibleUnitType"/>
        <rdfs:comment xml:lang="en">A Dimensionless Unit is a Unit of Measure that is a multiple of one.  100 Percent = 1 Unity = Avogadro&#39;s Number / ( 6.03 * 10^23).</rdfs:comment>
    </owl:NamedIndividual>
    


    <!-- http://www.nist.gov/itl/ssd/OntologyRequirements#Distance -->

    <owl:NamedIndividual rdf:about="&or;Distance">
        <rdf:type rdf:resource="&or;MeasurableQuantityType"/>
    </owl:NamedIndividual>
    


    <!-- http://www.nist.gov/itl/ssd/OntologyRequirements#DublinCoreOntology -->

    <owl:NamedIndividual rdf:about="&or;DublinCoreOntology">
        <rdf:type rdf:resource="&oil;Ontology"/>
        <standardNamespacePrefix rdf:datatype="&xsd;NMTOKEN">dc</standardNamespacePrefix>
        <nameSpaceURI rdf:datatype="&xsd;anyURI">http://purl.org/dc/terms/</nameSpaceURI>
        <ontologyDomain rdf:resource="&or;ComputerScience"/>
    </owl:NamedIndividual>
    


    <!-- http://www.nist.gov/itl/ssd/OntologyRequirements#Duration -->

    <owl:NamedIndividual rdf:about="&or;Duration">
        <rdf:type rdf:resource="&or;MeasurableQuantityType"/>
        <rdfs:comment xml:lang="en">Each instance of Duration is a physical quantity, corresponding to a certain ``amount of time&#39; &#39;, that a TemporalThing exists, occurs over, or endures.

Same as cyc:Time-Quantity.</rdfs:comment>
    </owl:NamedIndividual>
    


    <!-- http://www.nist.gov/itl/ssd/OntologyRequirements#EMEM -->

    <owl:NamedIndividual rdf:about="&or;EMEM"/>
    


    <!-- http://www.nist.gov/itl/ssd/OntologyRequirements#ElectronVolt -->

    <owl:NamedIndividual rdf:about="&or;ElectronVolt">
        <rdf:type rdf:resource="&or;UnitOfEnergy"/>
    </owl:NamedIndividual>
    


    <!-- http://www.nist.gov/itl/ssd/OntologyRequirements#Energy -->

    <owl:NamedIndividual rdf:about="&or;Energy">
        <rdf:type rdf:resource="&or;MeasurableQuantityType"/>
    </owl:NamedIndividual>
    


    <!-- http://www.nist.gov/itl/ssd/OntologyRequirements#Erg -->

    <owl:NamedIndividual rdf:about="&or;Erg">
        <rdf:type rdf:resource="&or;CGS_Unit"/>
        <rdf:type rdf:resource="&or;UnitOfEnergy"/>
    </owl:NamedIndividual>
    


    <!-- http://www.nist.gov/itl/ssd/OntologyRequirements#February -->

    <owl:NamedIndividual rdf:about="&or;February">
        <rdf:type rdf:resource="&or;MonthOfYearType"/>
        <rdfs:comment xml:lang="en">The month of February</rdfs:comment>
    </owl:NamedIndividual>
    


    <!-- http://www.nist.gov/itl/ssd/OntologyRequirements#Femtoliter -->

    <owl:NamedIndividual rdf:about="&or;Femtoliter">
        <rdf:type rdf:resource="&or;MetricUnit"/>
        <rdf:type rdf:resource="&or;UnitOfVolume"/>
    </owl:NamedIndividual>
    


    <!-- http://www.nist.gov/itl/ssd/OntologyRequirements#Foot-UnitOfMeasure -->

    <owl:NamedIndividual rdf:about="&or;Foot-UnitOfMeasure">
        <rdf:type rdf:resource="&or;NonMetricUnit"/>
        <rdf:type rdf:resource="&or;UnitOfDistance"/>
        <termString xml:lang="en">feet</termString>
        <termString xml:lang="en">foot</termString>
    </owl:NamedIndividual>
    


    <!-- http://www.nist.gov/itl/ssd/OntologyRequirements#Force -->

    <owl:NamedIndividual rdf:about="&or;Force">
        <rdf:type rdf:resource="&or;MeasurableQuantityType"/>
        <rdfs:comment xml:lang="en">Force is the agency by which change is produced.  In mechanics, a force on a free object yields an acceleration equal to the force divided by the mass of the object (F = mA). Physics recognizes five basic forces: gravitational, weak, electrical, magnetic, and strong forces, with electrical and magnetic forces unified.</rdfs:comment>
    </owl:NamedIndividual>
    


    <!-- http://www.nist.gov/itl/ssd/OntologyRequirements#ForensicBiology -->

    <owl:NamedIndividual rdf:about="&or;ForensicBiology">
        <rdf:type rdf:resource="&or;BiomedicalFieldOfStudy"/>
        <rdfs:comment xml:lang="en">Forensic Biology is the subfield of Biology dealing with the use of bioogical science for solving crimes.</rdfs:comment>
        <subFieldOf rdf:resource="&or;Biology"/>
        <subFieldOf rdf:resource="&or;ForensicScience"/>
    </owl:NamedIndividual>
    


    <!-- http://www.nist.gov/itl/ssd/OntologyRequirements#ForensicScience -->

    <owl:NamedIndividual rdf:about="&or;ForensicScience">
        <rdf:type rdf:resource="&or;FieldOfStudy"/>
        <rdfs:comment xml:lang="en">Forensic Science is those aspects of science as used to detect crimes and identify the perpetrators or victims or crimes.  There are subfields of Forensic Science in many different scientific fields.</rdfs:comment>
    </owl:NamedIndividual>
    


    <!-- http://www.nist.gov/itl/ssd/OntologyRequirements#GIF_File_Format -->

    <owl:NamedIndividual rdf:about="&or;GIF_File_Format">
        <rdf:type rdf:resource="&or;ImageFileFormat"/>
        <defaultFileExtension rdf:datatype="&xsd;Name">gif</defaultFileExtension>
        <rdfs:comment xml:lang="en">The GIF (Grpahics Interchange Format) file format</rdfs:comment>
    </owl:NamedIndividual>
    


    <!-- http://www.nist.gov/itl/ssd/OntologyRequirements#GeneOntology -->

    <owl:NamedIndividual rdf:about="&or;GeneOntology">
        <rdf:type rdf:resource="&oil;Ontology"/>
        <standardNamespacePrefix rdf:datatype="&xsd;NMTOKEN">go</standardNamespacePrefix>
        <nameSpaceURI rdf:datatype="&xsd;anyURI">http://purl.obolibrary.org/obo/go#</nameSpaceURI>
        <ontologyDomain rdf:resource="&or;Anatomy"/>
        <ontologyDomain rdf:resource="&or;BiologicalProcessFOS"/>
        <ontologyDomain rdf:resource="&or;Genomics"/>
    </owl:NamedIndividual>
    


    <!-- http://www.nist.gov/itl/ssd/OntologyRequirements#Genomics -->

    <owl:NamedIndividual rdf:about="&or;Genomics">
        <rdf:type rdf:resource="&or;BiomedicalFieldOfStudy"/>
        <subFieldOf rdf:resource="&or;Biomedicine"/>
    </owl:NamedIndividual>
    


    <!-- http://www.nist.gov/itl/ssd/OntologyRequirements#Gram -->

    <owl:NamedIndividual rdf:about="&or;Gram">
        <rdf:type rdf:resource="&or;CGS_Unit"/>
        <rdf:type rdf:resource="&or;UnitOfMass"/>
    </owl:NamedIndividual>
    


    <!-- http://www.nist.gov/itl/ssd/OntologyRequirements#GramCalorie -->

    <owl:NamedIndividual rdf:about="&or;GramCalorie">
        <rdf:type rdf:resource="&or;NonMetricUnit"/>
        <rdf:type rdf:resource="&or;UnitOfEnergy"/>
    </owl:NamedIndividual>
    


    <!-- http://www.nist.gov/itl/ssd/OntologyRequirements#HDF4_Format -->

    <owl:NamedIndividual rdf:about="&or;HDF4_Format">
        <rdf:type rdf:resource="&or;ElectronicFileFormat"/>
        <oil:seeAlso rdf:datatype="&xsd;anyURI">http://www.hdfgroup.org/products/</oil:seeAlso>
        <rdfs:comment xml:lang="en">HDF4 (originally known as HDF) is a file format for storing scientific data and a software library that provides high-level APIs and a low-level data interface. </rdfs:comment>
    </owl:NamedIndividual>
    


    <!-- http://www.nist.gov/itl/ssd/OntologyRequirements#HDF5_Format -->

    <owl:NamedIndividual rdf:about="&or;HDF5_Format">
        <rdf:type rdf:resource="&or;ElectronicFileFormat"/>
        <oil:seeAlso rdf:datatype="&xsd;anyURI">http://www.hdfgroup.org/products/</oil:seeAlso>
        <rdfs:comment xml:lang="en">HDF5 is a general purpose library and file format for storing scientific data.</rdfs:comment>
    </owl:NamedIndividual>
    


    <!-- http://www.nist.gov/itl/ssd/OntologyRequirements#HEPES -->

    <owl:NamedIndividual rdf:about="&or;HEPES"/>
    


    <!-- http://www.nist.gov/itl/ssd/OntologyRequirements#HTML_Format -->

    <owl:NamedIndividual rdf:about="&or;HTML_Format">
        <rdf:type rdf:resource="&or;ElectronicFileFormat"/>
        <defaultFileExtension rdf:datatype="&xsd;Name">htm</defaultFileExtension>
        <defaultFileExtension rdf:datatype="&xsd;Name">html</defaultFileExtension>
        <rdfs:comment xml:lang="en">Hypertext Markup Language format</rdfs:comment>
    </owl:NamedIndividual>
    


    <!-- http://www.nist.gov/itl/ssd/OntologyRequirements#HealthCareFOS -->

    <owl:NamedIndividual rdf:about="&or;HealthCareFOS">
        <rdf:type rdf:resource="&or;BiomedicalFieldOfStudy"/>
    </owl:NamedIndividual>
    


    <!-- http://www.nist.gov/itl/ssd/OntologyRequirements#HoursDuration -->

    <owl:NamedIndividual rdf:about="&or;HoursDuration">
        <rdf:type rdf:resource="&or;MetricUnit"/>
        <rdf:type rdf:resource="&or;UnitOfDuration"/>
    </owl:NamedIndividual>
    


    <!-- http://www.nist.gov/itl/ssd/OntologyRequirements#ICSv2ImageFormat -->

    <owl:NamedIndividual rdf:about="&or;ICSv2ImageFormat">
        <rdf:type rdf:resource="&or;MicroscopyImageFileFormat"/>
        <rdfs:comment xml:lang="en">Version 2.0 of the Image Cytometry Standard (ICS) format.  It contains microscope settings metadata as well as pixel data.</rdfs:comment>
    </owl:NamedIndividual>
    


    <!-- http://www.nist.gov/itl/ssd/OntologyRequirements#IMDM -->

    <owl:NamedIndividual rdf:about="&or;IMDM"/>
    


    <!-- http://www.nist.gov/itl/ssd/OntologyRequirements#ImageCytometryStandard -->

    <owl:NamedIndividual rdf:about="&or;ImageCytometryStandard">
        <rdf:type rdf:resource="&or;MicroscopyImageFileFormat"/>
        <defaultFileExtension rdf:datatype="&xsd;Name">ics</defaultFileExtension>
        <defaultFileExtension rdf:datatype="&xsd;Name">ids</defaultFileExtension>
        <rdfs:comment xml:lang="en">The Image Cytometry Standard (ICS) is a digital multidimensional image file format that stores image data from multiple images and image acquisition parameters for the  microscope.  ICS verion 1.0 has plaintext metadata in aa .ics file and pixel data in a .ids file.  ICS verion 2.0 stores both pixel and metadata in an .ics file.</rdfs:comment>
    </owl:NamedIndividual>
    


    <!-- http://www.nist.gov/itl/ssd/OntologyRequirements#ImageProcessing -->

    <owl:NamedIndividual rdf:about="&or;ImageProcessing">
        <rdf:type rdf:resource="&or;FieldOfStudy"/>
        <subFieldOf rdf:resource="&or;ComputerScience"/>
    </owl:NamedIndividual>
    


    <!-- http://www.nist.gov/itl/ssd/OntologyRequirements#Immunology -->

    <owl:NamedIndividual rdf:about="&or;Immunology">
        <rdf:type rdf:resource="&or;BiomedicalFieldOfStudy"/>
        <subFieldOf rdf:resource="&or;Biomedicine"/>
    </owl:NamedIndividual>
    


    <!-- http://www.nist.gov/itl/ssd/OntologyRequirements#Inch -->

    <owl:NamedIndividual rdf:about="&or;Inch">
        <rdf:type rdf:resource="&or;NonMetricUnit"/>
        <rdf:type rdf:resource="&or;UnitOfDistance"/>
        <termString xml:lang="en">inch</termString>
    </owl:NamedIndividual>
    


    <!-- http://www.nist.gov/itl/ssd/OntologyRequirements#JPEG_File_Format -->

    <owl:NamedIndividual rdf:about="&or;JPEG_File_Format">
        <rdf:type rdf:resource="&or;ImageFileFormat"/>
        <defaultFileExtension rdf:datatype="&xsd;Name">jpeg</defaultFileExtension>
        <defaultFileExtension rdf:datatype="&xsd;Name">jpg</defaultFileExtension>
        <rdfs:comment xml:lang="en">The JPEG file format</rdfs:comment>
    </owl:NamedIndividual>
    


    <!-- http://www.nist.gov/itl/ssd/OntologyRequirements#January -->

    <owl:NamedIndividual rdf:about="&or;January">
        <rdf:type rdf:resource="&or;MonthOfYearType"/>
        <rdfs:comment xml:lang="en">The month of January</rdfs:comment>
    </owl:NamedIndividual>
    


    <!-- http://www.nist.gov/itl/ssd/OntologyRequirements#Joule -->

    <owl:NamedIndividual rdf:about="&or;Joule">
        <rdf:type rdf:resource="&or;SI_Unit"/>
        <rdf:type rdf:resource="&or;UnitOfEnergy"/>
    </owl:NamedIndividual>
    


    <!-- http://www.nist.gov/itl/ssd/OntologyRequirements#July -->

    <owl:NamedIndividual rdf:about="&or;July">
        <rdf:type rdf:resource="&or;MonthOfYearType"/>
        <rdfs:comment xml:lang="en">The month of July</rdfs:comment>
    </owl:NamedIndividual>
    


    <!-- http://www.nist.gov/itl/ssd/OntologyRequirements#June -->

    <owl:NamedIndividual rdf:about="&or;June">
        <rdf:type rdf:resource="&or;MonthOfYearType"/>
        <rdfs:comment xml:lang="en">The month of June</rdfs:comment>
    </owl:NamedIndividual>
    


    <!-- http://www.nist.gov/itl/ssd/OntologyRequirements#Kilocalorie -->

    <owl:NamedIndividual rdf:about="&or;Kilocalorie">
        <rdf:type rdf:resource="&or;NonMetricUnit"/>
        <rdf:type rdf:resource="&or;UnitOfEnergy"/>
    </owl:NamedIndividual>
    


    <!-- http://www.nist.gov/itl/ssd/OntologyRequirements#Kilogram -->

    <owl:NamedIndividual rdf:about="&or;Kilogram">
        <rdf:type rdf:resource="&or;SI_Unit"/>
        <rdf:type rdf:resource="&or;UnitOfMass"/>
    </owl:NamedIndividual>
    


    <!-- http://www.nist.gov/itl/ssd/OntologyRequirements#KilowattHour -->

    <owl:NamedIndividual rdf:about="&or;KilowattHour">
        <rdf:type rdf:resource="&or;UnitOfEnergy"/>
    </owl:NamedIndividual>
    


    <!-- http://www.nist.gov/itl/ssd/OntologyRequirements#Liter -->

    <owl:NamedIndividual rdf:about="&or;Liter">
        <rdf:type rdf:resource="&or;MetricUnit"/>
        <rdf:type rdf:resource="&or;UnitOfVolume"/>
    </owl:NamedIndividual>
    


    <!-- http://www.nist.gov/itl/ssd/OntologyRequirements#March -->

    <owl:NamedIndividual rdf:about="&or;March">
        <rdf:type rdf:resource="&or;MonthOfYearType"/>
        <rdfs:comment xml:lang="en">The month of March</rdfs:comment>
    </owl:NamedIndividual>
    


    <!-- http://www.nist.gov/itl/ssd/OntologyRequirements#Mass -->

    <owl:NamedIndividual rdf:about="&or;Mass">
        <rdf:type rdf:resource="&or;MeasurableQuantityType"/>
    </owl:NamedIndividual>
    


    <!-- http://www.nist.gov/itl/ssd/OntologyRequirements#May -->

    <owl:NamedIndividual rdf:about="&or;May">
        <rdf:type rdf:resource="&or;MonthOfYearType"/>
        <rdfs:comment xml:lang="en">The month of May</rdfs:comment>
    </owl:NamedIndividual>
    


    <!-- http://www.nist.gov/itl/ssd/OntologyRequirements#Meter -->

    <owl:NamedIndividual rdf:about="&or;Meter">
        <rdf:type rdf:resource="&or;SI_Unit"/>
        <rdf:type rdf:resource="&or;UnitOfDistance"/>
    </owl:NamedIndividual>
    


    <!-- http://www.nist.gov/itl/ssd/OntologyRequirements#MeterSquaredPerSecondSquared -->

    <owl:NamedIndividual rdf:about="&or;MeterSquaredPerSecondSquared">
        <rdf:type rdf:resource="&or;SI_Unit"/>
        <rdf:type rdf:resource="&or;UnitOfVelocitySquared"/>
    </owl:NamedIndividual>
    


    <!-- http://www.nist.gov/itl/ssd/OntologyRequirements#Microgram -->

    <owl:NamedIndividual rdf:about="&or;Microgram">
        <rdf:type rdf:resource="&or;MetricUnit"/>
        <rdf:type rdf:resource="&or;UnitOfMass"/>
    </owl:NamedIndividual>
    


    <!-- http://www.nist.gov/itl/ssd/OntologyRequirements#Microliter -->

    <owl:NamedIndividual rdf:about="&or;Microliter">
        <rdf:type rdf:resource="&or;MetricUnit"/>
        <rdf:type rdf:resource="&or;UnitOfVolume"/>
    </owl:NamedIndividual>
    


    <!-- http://www.nist.gov/itl/ssd/OntologyRequirements#Micron -->

    <owl:NamedIndividual rdf:about="&or;Micron">
        <rdf:type rdf:resource="&or;MetricUnit"/>
        <rdf:type rdf:resource="&or;UnitOfDistance"/>
    </owl:NamedIndividual>
    


    <!-- http://www.nist.gov/itl/ssd/OntologyRequirements#Mile -->

    <owl:NamedIndividual rdf:about="&or;Mile">
        <rdf:type rdf:resource="&or;NonMetricUnit"/>
        <rdf:type rdf:resource="&or;UnitOfDistance"/>
        <termString xml:lang="en">mile</termString>
    </owl:NamedIndividual>
    


    <!-- http://www.nist.gov/itl/ssd/OntologyRequirements#Milligram -->

    <owl:NamedIndividual rdf:about="&or;Milligram">
        <rdf:type rdf:resource="&or;MetricUnit"/>
        <rdf:type rdf:resource="&or;UnitOfMass"/>
    </owl:NamedIndividual>
    


    <!-- http://www.nist.gov/itl/ssd/OntologyRequirements#Milliliter -->

    <owl:NamedIndividual rdf:about="&or;Milliliter">
        <rdf:type rdf:resource="&or;CGS_Unit"/>
        <rdf:type rdf:resource="&or;UnitOfVolume"/>
    </owl:NamedIndividual>
    


    <!-- http://www.nist.gov/itl/ssd/OntologyRequirements#Millimeter -->

    <owl:NamedIndividual rdf:about="&or;Millimeter">
        <rdf:type rdf:resource="&or;MetricUnit"/>
        <rdf:type rdf:resource="&or;UnitOfDistance"/>
    </owl:NamedIndividual>
    


    <!-- http://www.nist.gov/itl/ssd/OntologyRequirements#MinutesDuration -->

    <owl:NamedIndividual rdf:about="&or;MinutesDuration">
        <rdf:type rdf:resource="&or;MetricUnit"/>
        <rdf:type rdf:resource="&or;UnitOfDuration"/>
    </owl:NamedIndividual>
    


    <!-- http://www.nist.gov/itl/ssd/OntologyRequirements#MmHg -->

    <owl:NamedIndividual rdf:about="&or;MmHg">
        <rdf:type rdf:resource="&or;NonMetricUnit"/>
        <rdf:type rdf:resource="&or;UnitOfPressure"/>
        <rdfs:comment xml:lang="en">The pressure of a column of one mm of mercury (at 1.0 g, 20 C).</rdfs:comment>
    </owl:NamedIndividual>
    


    <!-- http://www.nist.gov/itl/ssd/OntologyRequirements#Nanogram -->

    <owl:NamedIndividual rdf:about="&or;Nanogram">
        <rdf:type rdf:resource="&or;MetricUnit"/>
        <rdf:type rdf:resource="&or;UnitOfMass"/>
    </owl:NamedIndividual>
    


    <!-- http://www.nist.gov/itl/ssd/OntologyRequirements#Nanoliter -->

    <owl:NamedIndividual rdf:about="&or;Nanoliter">
        <rdf:type rdf:resource="&or;MetricUnit"/>
        <rdf:type rdf:resource="&or;UnitOfVolume"/>
    </owl:NamedIndividual>
    


    <!-- http://www.nist.gov/itl/ssd/OntologyRequirements#Nanometer -->

    <owl:NamedIndividual rdf:about="&or;Nanometer">
        <rdf:type rdf:resource="&or;MetricUnit"/>
        <rdf:type rdf:resource="&or;UnitOfDistance"/>
    </owl:NamedIndividual>
    


    <!-- http://www.nist.gov/itl/ssd/OntologyRequirements#NegativeControlRole -->

    <owl:NamedIndividual rdf:about="&or;NegativeControlRole">
        <rdf:type rdf:resource="&or;MeasurementRole"/>
    </owl:NamedIndividual>
    


    <!-- http://www.nist.gov/itl/ssd/OntologyRequirements#Newton -->

    <owl:NamedIndividual rdf:about="&or;Newton">
        <rdf:type rdf:resource="&or;SI_Unit"/>
        <rdf:type rdf:resource="&or;UnitOfForce"/>
        <rdfs:comment xml:lang="en">The Newton is the SI unit of force.</rdfs:comment>
    </owl:NamedIndividual>
    


    <!-- http://www.nist.gov/itl/ssd/OntologyRequirements#November -->

    <owl:NamedIndividual rdf:about="&or;November">
        <rdf:type rdf:resource="&or;MonthOfYearType"/>
        <rdfs:comment xml:lang="en">The month of November</rdfs:comment>
    </owl:NamedIndividual>
    


    <!-- http://www.nist.gov/itl/ssd/OntologyRequirements#OBO_Ontology -->

    <owl:NamedIndividual rdf:about="&or;OBO_Ontology">
        <rdf:type rdf:resource="&oil;Ontology"/>
        <nameSpaceURI rdf:datatype="&xsd;anyURI">http://purl.obolibrary.org/obo/</nameSpaceURI>
        <standardNamespacePrefix rdf:datatype="&xsd;NMTOKEN">obo</standardNamespacePrefix>
        <ontologyDomain rdf:resource="&or;ComputerScience"/>
    </owl:NamedIndividual>
    


    <!-- http://www.nist.gov/itl/ssd/OntologyRequirements#OMEM -->

    <owl:NamedIndividual rdf:about="&or;OMEM"/>
    


    <!-- http://www.nist.gov/itl/ssd/OntologyRequirements#OWL_Ontology -->

    <owl:NamedIndividual rdf:about="&or;OWL_Ontology">
        <rdf:type rdf:resource="&oil;Ontology"/>
        <nameSpaceURI rdf:datatype="&xsd;anyURI">http://www.w3.org/2002/07/owl#</nameSpaceURI>
        <standardNamespacePrefix rdf:datatype="&xsd;NMTOKEN">owl</standardNamespacePrefix>
        <ontologyDomain rdf:resource="&or;ComputerScience"/>
    </owl:NamedIndividual>
    


    <!-- http://www.nist.gov/itl/ssd/OntologyRequirements#October -->

    <owl:NamedIndividual rdf:about="&or;October">
        <rdf:type rdf:resource="&or;MonthOfYearType"/>
        <rdfs:comment xml:lang="en">The month of October</rdfs:comment>
    </owl:NamedIndividual>
    


    <!-- http://www.nist.gov/itl/ssd/OntologyRequirements#PSI -->

    <owl:NamedIndividual rdf:about="&or;PSI">
        <rdf:type rdf:resource="&or;NonMetricUnit"/>
        <rdf:type rdf:resource="&or;UnitOfPressure"/>
        <rdfs:comment xml:lang="en">Pounds per square inch</rdfs:comment>
    </owl:NamedIndividual>
    


    <!-- http://www.nist.gov/itl/ssd/OntologyRequirements#Pascal-UnitOfPressure -->

    <owl:NamedIndividual rdf:about="&or;Pascal-UnitOfPressure">
        <rdf:type rdf:resource="&or;SI_Unit"/>
        <rdf:type rdf:resource="&or;UnitOfPressure"/>
    </owl:NamedIndividual>
    


    <!-- http://www.nist.gov/itl/ssd/OntologyRequirements#Percent -->

    <owl:NamedIndividual rdf:about="&or;Percent">
        <rdf:type rdf:resource="&or;DimensionlessUnit"/>
        <rdfs:comment xml:lang="en">Percent is the dimensionless unit for 0.01 .</rdfs:comment>
    </owl:NamedIndividual>
    


    <!-- http://www.nist.gov/itl/ssd/OntologyRequirements#Phenomics -->

    <owl:NamedIndividual rdf:about="&or;Phenomics">
        <rdf:type rdf:resource="&or;BiomedicalFieldOfStudy"/>
        <rdfs:comment xml:lang="en">Phenomics is a subfield of Biology that studies physical and biochemical traits of organisms.</rdfs:comment>
        <subFieldOf rdf:resource="&or;Biology"/>
    </owl:NamedIndividual>
    


    <!-- http://www.nist.gov/itl/ssd/OntologyRequirements#PhenotypicQualityOntology -->

    <owl:NamedIndividual rdf:about="&or;PhenotypicQualityOntology">
        <rdf:type rdf:resource="&oil;Ontology"/>
        <nameSpaceURI rdf:datatype="&xsd;anyURI">http://purl.obolibrary.org/obo/pato#</nameSpaceURI>
        <standardNamespacePrefix rdf:datatype="&xsd;NMTOKEN">pato</standardNamespacePrefix>
        <rdfs:comment xml:lang="en">PATO is an ontology of phenotypic qualities, intended for use in a number of applications, primarily defining composite phenotypes and phenotype annotation. </rdfs:comment>
        <ontologyDomain rdf:resource="&or;Phenomics"/>
    </owl:NamedIndividual>
    


    <!-- http://www.nist.gov/itl/ssd/OntologyRequirements#Pixel -->

    <owl:NamedIndividual rdf:about="&or;Pixel">
        <rdf:type rdf:resource="&or;NonMetricUnit"/>
        <rdf:type rdf:resource="&or;UnitOfArea"/>
        <rdf:type rdf:resource="&or;UnitOfComputerStorageCapacity"/>
    </owl:NamedIndividual>
    


    <!-- http://www.nist.gov/itl/ssd/OntologyRequirements#PlantTraitOntology -->

    <owl:NamedIndividual rdf:about="&or;PlantTraitOntology">
        <rdf:type rdf:resource="&oil;Ontology"/>
        <standardNamespacePrefix rdf:datatype="&xsd;NMTOKEN">TO</standardNamespacePrefix>
        <nameSpaceURI rdf:datatype="&xsd;anyURI">http://purl.obolibrary.org/obo/to.owl</nameSpaceURI>
        <rdfs:comment xml:lang="en">The Plant Trait Ontology is a controlled vocabulary of describe phenotypic traits in plants. Each trait is a distinguishable feature, characteristic, quality or phenotypic feature of a developing or mature plant.</rdfs:comment>
        <ontologyDomain rdf:resource="&or;Phenomics"/>
    </owl:NamedIndividual>
    


    <!-- http://www.nist.gov/itl/ssd/OntologyRequirements#PositiveControlRole -->

    <owl:NamedIndividual rdf:about="&or;PositiveControlRole">
        <rdf:type rdf:resource="&or;MeasurementRole"/>
    </owl:NamedIndividual>
    


    <!-- http://www.nist.gov/itl/ssd/OntologyRequirements#Pressure -->

    <owl:NamedIndividual rdf:about="&or;Pressure">
        <rdf:type rdf:resource="&or;MeasurableQuantityType"/>
        <rdfs:comment xml:lang="en">Pressure is the force per unit area perpendicular to the surface of an object.</rdfs:comment>
    </owl:NamedIndividual>
    


    <!-- http://www.nist.gov/itl/ssd/OntologyRequirements#ProteinOntology -->

    <owl:NamedIndividual rdf:about="&or;ProteinOntology">
        <rdf:type rdf:resource="&oil;Ontology"/>
        <standardNamespacePrefix rdf:datatype="&xsd;NMTOKEN">PR</standardNamespacePrefix>
        <nameSpaceURI rdf:datatype="&xsd;anyURI">http://purl.obolibrary.org/obo/pr#</nameSpaceURI>
        <rdfs:comment xml:lang="en">The PRotein Ontology (PRO) has been designed to describe the relationships of proteins and protein evolutionary classes (ontology for ProEvo), to delineate the multiple protein forms of a gene locus (ontology for protein forms), and to interconnect existing ontologies.</rdfs:comment>
        <ontologyDomain rdf:resource="&or;Proteomics"/>
    </owl:NamedIndividual>
    


    <!-- http://www.nist.gov/itl/ssd/OntologyRequirements#Proteomics -->

    <owl:NamedIndividual rdf:about="&or;Proteomics">
        <rdf:type rdf:resource="&or;BiomedicalFieldOfStudy"/>
    </owl:NamedIndividual>
    


    <!-- http://www.nist.gov/itl/ssd/OntologyRequirements#SecondsDuration -->

    <owl:NamedIndividual rdf:about="&or;SecondsDuration">
        <rdf:type rdf:resource="&or;CGS_Unit"/>
        <rdf:type rdf:resource="&or;SI_Unit"/>
        <rdf:type rdf:resource="&or;UnitOfDuration"/>
    </owl:NamedIndividual>
    


    <!-- http://www.nist.gov/itl/ssd/OntologyRequirements#September -->

    <owl:NamedIndividual rdf:about="&or;September">
        <rdf:type rdf:resource="&or;MonthOfYearType"/>
        <rdfs:comment xml:lang="en">The month of September</rdfs:comment>
    </owl:NamedIndividual>
    


    <!-- http://www.nist.gov/itl/ssd/OntologyRequirements#SpatialBenchmarkRole -->

    <owl:NamedIndividual rdf:about="&or;SpatialBenchmarkRole">
        <rdf:type rdf:resource="&or;MeasurementRole"/>
    </owl:NamedIndividual>
    


    <!-- http://www.nist.gov/itl/ssd/OntologyRequirements#SquareCentimeter -->

    <owl:NamedIndividual rdf:about="&or;SquareCentimeter">
        <rdf:type rdf:resource="&or;CGS_Unit"/>
        <rdf:type rdf:resource="&or;UnitOfArea"/>
    </owl:NamedIndividual>
    


    <!-- http://www.nist.gov/itl/ssd/OntologyRequirements#SquareMeter -->

    <owl:NamedIndividual rdf:about="&or;SquareMeter">
        <rdf:type rdf:resource="&or;SI_Unit"/>
        <rdf:type rdf:resource="&or;UnitOfArea"/>
    </owl:NamedIndividual>
    


    <!-- http://www.nist.gov/itl/ssd/OntologyRequirements#SquareMicron -->

    <owl:NamedIndividual rdf:about="&or;SquareMicron">
        <rdf:type rdf:resource="&or;MetricUnit"/>
        <rdf:type rdf:resource="&or;UnitOfArea"/>
    </owl:NamedIndividual>
    


    <!-- http://www.nist.gov/itl/ssd/OntologyRequirements#SquareMillimeter -->

    <owl:NamedIndividual rdf:about="&or;SquareMillimeter">
        <rdf:type rdf:resource="&or;MetricUnit"/>
        <rdf:type rdf:resource="&or;UnitOfArea"/>
    </owl:NamedIndividual>
    


    <!-- http://www.nist.gov/itl/ssd/OntologyRequirements#TIFF_File_Format -->

    <owl:NamedIndividual rdf:about="&or;TIFF_File_Format">
        <rdf:type rdf:resource="&or;ImageFileFormat"/>
        <rdfs:comment xml:lang="en">The TIFF (Tagged Image File Format) image file format</rdfs:comment>
    </owl:NamedIndividual>
    


    <!-- http://www.nist.gov/itl/ssd/OntologyRequirements#Temperature -->

    <owl:NamedIndividual rdf:about="&or;Temperature">
        <rdf:type rdf:resource="&or;MeasurableQuantityType"/>
    </owl:NamedIndividual>
    


    <!-- http://www.nist.gov/itl/ssd/OntologyRequirements#Uberon -->

    <owl:NamedIndividual rdf:about="&or;Uberon">
        <rdf:type rdf:resource="&oil;Ontology"/>
        <nameSpaceURI rdf:datatype="&xsd;anyURI">http://purl.obolibrary.org/obo/uberon#</nameSpaceURI>
        <standardNamespacePrefix rdf:datatype="&xsd;NMTOKEN">uberon</standardNamespacePrefix>
        <rdfs:comment xml:lang="en">Uberon is an integrated cross-species anatomy ontology representing a variety of entities classified according to traditional anatomical criteria such as structure, function and developmental lineage. The ontology includes relationships to taxon-specific anatomical ontologies, allowing integration of functional, phenotype and expression data.</rdfs:comment>
        <ontologyDomain rdf:resource="&or;Anatomy"/>
    </owl:NamedIndividual>
    


    <!-- http://www.nist.gov/itl/ssd/OntologyRequirements#UnitOfArea -->

    <owl:NamedIndividual rdf:about="&or;UnitOfArea">
        <rdf:type rdf:resource="&or;InterconvertibleUnitType"/>
        <rdfs:comment xml:lang="en">A Unit of Area is a Unit Of Measure specifying an amout of area, for example square centimeter.</rdfs:comment>
    </owl:NamedIndividual>
    


    <!-- http://www.nist.gov/itl/ssd/OntologyRequirements#UnitOfComputerStorageCapacity -->

    <owl:NamedIndividual rdf:about="&or;UnitOfComputerStorageCapacity">
        <rdf:type rdf:resource="&or;InterconvertibleUnitType"/>
        <rdfs:comment xml:lang="en">A Unit of Comuter Storage Capacity is a Unit Of Measure specifying an amout of computer memory, for example bit, byte, pixel.</rdfs:comment>
    </owl:NamedIndividual>
    


    <!-- http://www.nist.gov/itl/ssd/OntologyRequirements#UnitOfDensity -->

    <owl:NamedIndividual rdf:about="&or;UnitOfDensity">
        <rdf:type rdf:resource="&or;InterconvertibleUnitType"/>
        <rdfs:comment xml:lang="en">A Unit of Density is a Unit Of Measure specifying an amout of mass per unit of volume, for example grams per cc.</rdfs:comment>
    </owl:NamedIndividual>
    


    <!-- http://www.nist.gov/itl/ssd/OntologyRequirements#UnitOfDistance -->

    <owl:NamedIndividual rdf:about="&or;UnitOfDistance">
        <rdf:type rdf:resource="&or;InterconvertibleUnitType"/>
        <rdfs:comment xml:lang="en">A Unit of Distance is a Unit Of Measure specifying the length between two points, for example a centimeter.</rdfs:comment>
    </owl:NamedIndividual>
    


    <!-- http://www.nist.gov/itl/ssd/OntologyRequirements#UnitOfDuration -->

    <owl:NamedIndividual rdf:about="&or;UnitOfDuration">
        <rdf:type rdf:resource="&or;InterconvertibleUnitType"/>
        <rdfs:comment xml:lang="en">A Unit of Duration is a Unit Of Measure specifying an amout of time between two time points, for example a second.</rdfs:comment>
    </owl:NamedIndividual>
    


    <!-- http://www.nist.gov/itl/ssd/OntologyRequirements#UnitOfEnergy -->

    <owl:NamedIndividual rdf:about="&or;UnitOfEnergy">
        <rdf:type rdf:resource="&or;InterconvertibleUnitType"/>
        <rdfs:comment xml:lang="en">A Unit of Energy is a Unit Of Measure specifying an amout of energy, for example joule or kilowatt hour.</rdfs:comment>
    </owl:NamedIndividual>
    


    <!-- http://www.nist.gov/itl/ssd/OntologyRequirements#UnitOfForce -->

    <owl:NamedIndividual rdf:about="&or;UnitOfForce">
        <rdf:type rdf:resource="&or;InterconvertibleUnitType"/>
        <rdfs:comment xml:lang="en">A Unit of Force is a Unit Of Measure specifying an amout of force (mass times acceleration), for example a newton.</rdfs:comment>
    </owl:NamedIndividual>
    


    <!-- http://www.nist.gov/itl/ssd/OntologyRequirements#UnitOfMass -->

    <owl:NamedIndividual rdf:about="&or;UnitOfMass">
        <rdf:type rdf:resource="&or;InterconvertibleUnitType"/>
        <rdfs:comment xml:lang="en">A Unit of mass is a Unit Of Measure specifying an amout of mass, for example a gram or kilogram.</rdfs:comment>
    </owl:NamedIndividual>
    


    <!-- http://www.nist.gov/itl/ssd/OntologyRequirements#UnitOfPressure -->

    <owl:NamedIndividual rdf:about="&or;UnitOfPressure">
        <rdf:type rdf:resource="&or;InterconvertibleUnitType"/>
        <rdfs:comment xml:lang="en">A Unit of pressure is a Unit Of Measure specifying an amout of force per unit of area, for example pascal or PSI.</rdfs:comment>
    </owl:NamedIndividual>
    


    <!-- http://www.nist.gov/itl/ssd/OntologyRequirements#UnitOfSpreadRate -->

    <owl:NamedIndividual rdf:about="&or;UnitOfSpreadRate">
        <rdf:type rdf:resource="&or;InterconvertibleUnitType"/>
        <rdfs:comment xml:lang="en">A Unit of Spread Rate is a Unit Of Measure specifying an amout of area per unit of duration, for example square centimeters per second.</rdfs:comment>
    </owl:NamedIndividual>
    


    <!-- http://www.nist.gov/itl/ssd/OntologyRequirements#UnitOfTemperature -->

    <owl:NamedIndividual rdf:about="&or;UnitOfTemperature">
        <rdf:type rdf:resource="&or;InterconvertibleUnitType"/>
        <rdfs:comment xml:lang="en">A Unit of Temperature is a Unit Of Measure specifying the temperature of something, for example Degree Celsius or Degree Kelvin.</rdfs:comment>
    </owl:NamedIndividual>
    


    <!-- http://www.nist.gov/itl/ssd/OntologyRequirements#UnitOfVelocity -->

    <owl:NamedIndividual rdf:about="&or;UnitOfVelocity">
        <rdf:type rdf:resource="&or;InterconvertibleUnitType"/>
        <rdfs:comment xml:lang="en">A Unit of Velocity is a Unit Of Measure for specifying a speed, for example meters per second.</rdfs:comment>
    </owl:NamedIndividual>
    


    <!-- http://www.nist.gov/itl/ssd/OntologyRequirements#UnitOfVelocitySquared -->

    <owl:NamedIndividual rdf:about="&or;UnitOfVelocitySquared">
        <rdf:type rdf:resource="&or;InterconvertibleUnitType"/>
        <rdfs:comment xml:lang="en">A Unit of Velocity Squared is a Unit Of Measure specifying the square of a velocity, for example square centimeters per second per second.</rdfs:comment>
    </owl:NamedIndividual>
    


    <!-- http://www.nist.gov/itl/ssd/OntologyRequirements#UnitOfVoltage -->

    <owl:NamedIndividual rdf:about="&or;UnitOfVoltage">
        <rdf:type rdf:resource="&or;InterconvertibleUnitType"/>
        <rdfs:comment xml:lang="en">A Unit of Voltge is a Unit Of Measure specifying an amout of electrical potential, for example a volt.</rdfs:comment>
    </owl:NamedIndividual>
    


    <!-- http://www.nist.gov/itl/ssd/OntologyRequirements#UnitOfVolume -->

    <owl:NamedIndividual rdf:about="&or;UnitOfVolume">
        <rdf:type rdf:resource="&or;InterconvertibleUnitType"/>
        <rdfs:comment xml:lang="en">A Unit of Volume is a Unit Of Measure specifying an amout of space something takes up, for example a liter.</rdfs:comment>
    </owl:NamedIndividual>
    


    <!-- http://www.nist.gov/itl/ssd/OntologyRequirements#Unity -->

    <owl:NamedIndividual rdf:about="&or;Unity">
        <rdf:type rdf:resource="&or;DimensionlessUnit"/>
        <rdfs:comment xml:lang="en">Unity is the Dimensionless Unit for 1.</rdfs:comment>
    </owl:NamedIndividual>
    


    <!-- http://www.nist.gov/itl/ssd/OntologyRequirements#Volt -->

    <owl:NamedIndividual rdf:about="&or;Volt">
        <rdf:type rdf:resource="&or;SI_Unit"/>
        <rdf:type rdf:resource="&or;UnitOfVoltage"/>
    </owl:NamedIndividual>
    


    <!-- http://www.nist.gov/itl/ssd/OntologyRequirements#Volume -->

    <owl:NamedIndividual rdf:about="&or;Volume">
        <rdf:type rdf:resource="&or;MeasurableQuantityType"/>
    </owl:NamedIndividual>
    


    <!-- http://www.nist.gov/itl/ssd/OntologyRequirements#WAV_File_Format -->

    <owl:NamedIndividual rdf:about="&or;WAV_File_Format">
        <rdf:type rdf:resource="&or;AudioFileFormat"/>
        <defaultFileExtension rdf:datatype="&xsd;Name">wav</defaultFileExtension>
    </owl:NamedIndividual>
    


    <!-- http://www.nist.gov/itl/ssd/OntologyRequirements#WeeksDuration -->

    <owl:NamedIndividual rdf:about="&or;WeeksDuration">
        <rdf:type rdf:resource="&or;UnitOfDuration"/>
    </owl:NamedIndividual>
    


    <!-- http://www.nist.gov/itl/ssd/OntologyRequirements#XMF_File_Format -->

    <owl:NamedIndividual rdf:about="&or;XMF_File_Format">
        <rdf:type rdf:resource="&or;AudioFileFormat"/>
        <rdfs:comment xml:lang="en">XMF (Extensible Music Format) is a container format for MIDI fiiles with metadata.</rdfs:comment>
    </owl:NamedIndividual>
    


    <!-- http://www.nist.gov/itl/ssd/OntologyRequirements#XML_Format -->

    <owl:NamedIndividual rdf:about="&or;XML_Format">
        <rdf:type rdf:resource="&or;ElectronicFileFormat"/>
        <defaultFileExtension rdf:datatype="&xsd;Name">xml</defaultFileExtension>
        <rdfs:comment xml:lang="en">A format corresponding to the XML Markup Language.</rdfs:comment>
    </owl:NamedIndividual>
    


    <!-- 
    ///////////////////////////////////////////////////////////////////////////////////////
    //
    // Annotations
    //
    ///////////////////////////////////////////////////////////////////////////////////////
     -->

    <rdf:Description rdf:about="&dc;format">
        <rdfs:label xml:lang="en-us">Format</rdfs:label>
        <terms:modified>2008-01-14</terms:modified>
        <terms:issued>1999-07-02</terms:issued>
        <skos:note xml:lang="en-us">A second property with the same name as this property has been declared in the dcterms: namespace (http://purl.org/dc/terms/).  See the Introduction to the document &#39;DCMI Metadata Terms&#39; (http://dublincore.org/documents/dcmi-terms/) for an explanation.</skos:note>
        <terms:description xml:lang="en-us">Examples of dimensions include size and duration. Recommended best practice is to use a controlled vocabulary such as the list of Internet Media Types [MIME].</terms:description>
        <rdfs:comment xml:lang="en-us">The file format, physical medium, or dimensions of the resource.</rdfs:comment>
        <terms:hasVersion rdf:resource="http://dublincore.org/usage/terms/history/#format-007"/>
        <rdfs:isDefinedBy rdf:resource="http://purl.org/dc/elements/1.1/"/>
    </rdf:Description>
    <rdf:Description rdf:about="&dc;creator">
        <rdfs:label xml:lang="en-us">Creator</rdfs:label>
        <terms:issued>1999-07-02</terms:issued>
        <terms:modified>2008-01-14</terms:modified>
        <skos:note xml:lang="en-us">A second property with the same name as this property has been declared in the dcterms: namespace (http://purl.org/dc/terms/).  See the Introduction to the document &#39;DCMI Metadata Terms&#39; (http://dublincore.org/documents/dcmi-terms/) for an explanation.</skos:note>
        <rdfs:comment xml:lang="en-us">An entity primarily responsible for making the resource.</rdfs:comment>
        <terms:description xml:lang="en-us">Examples of a Creator include a person, an organization, or a service. Typically, the name of a Creator should be used to indicate the entity.</terms:description>
        <terms:hasVersion rdf:resource="http://dublincore.org/usage/terms/history/#creator-006"/>
        <rdfs:isDefinedBy rdf:resource="http://purl.org/dc/elements/1.1/"/>
    </rdf:Description>
    <rdf:Description rdf:about="&dc;description">
        <rdfs:label xml:lang="en-us">Description</rdfs:label>
        <terms:modified>2008-01-14</terms:modified>
        <terms:issued>1999-07-02</terms:issued>
        <skos:note xml:lang="en-us">A second property with the same name as this property has been declared in the dcterms: namespace (http://purl.org/dc/terms/).  See the Introduction to the document &#39;DCMI Metadata Terms&#39; (http://dublincore.org/documents/dcmi-terms/) for an explanation.</skos:note>
        <rdfs:comment xml:lang="en-us">An account of the resource.</rdfs:comment>
        <terms:description xml:lang="en-us">Description may include but is not limited to: an abstract, a table of contents, a graphical representation, or a free-text account of the resource.</terms:description>
        <terms:hasVersion rdf:resource="http://dublincore.org/usage/terms/history/#description-006"/>
        <rdfs:isDefinedBy rdf:resource="http://purl.org/dc/elements/1.1/"/>
    </rdf:Description>
    <rdf:Description rdf:about="&dc;contributor">
        <rdfs:label xml:lang="en-us">Contributor</rdfs:label>
        <terms:issued>1999-07-02</terms:issued>
        <terms:modified>2008-01-14</terms:modified>
        <skos:note xml:lang="en-us">A second property with the same name as this property has been declared in the dcterms: namespace (http://purl.org/dc/terms/).  See the Introduction to the document &#39;DCMI Metadata Terms&#39; (http://dublincore.org/documents/dcmi-terms/) for an explanation.</skos:note>
        <rdfs:comment xml:lang="en-us">An entity responsible for making contributions to the resource.</rdfs:comment>
        <terms:description xml:lang="en-us">Examples of a Contributor include a person, an organization, or a service. Typically, the name of a Contributor should be used to indicate the entity.</terms:description>
        <terms:hasVersion rdf:resource="http://dublincore.org/usage/terms/history/#contributor-006"/>
        <rdfs:isDefinedBy rdf:resource="http://purl.org/dc/elements/1.1/"/>
    </rdf:Description>
    <rdf:Description rdf:about="&dc;language">
        <rdfs:label xml:lang="en-us">Language</rdfs:label>
        <terms:issued>1999-07-02</terms:issued>
        <terms:modified>2008-01-14</terms:modified>
        <rdfs:comment xml:lang="en-us">A language of the resource.</rdfs:comment>
        <skos:note xml:lang="en-us">A second property with the same name as this property has been declared in the dcterms: namespace (http://purl.org/dc/terms/).  See the Introduction to the document &#39;DCMI Metadata Terms&#39; (http://dublincore.org/documents/dcmi-terms/) for an explanation.</skos:note>
        <terms:description xml:lang="en-us">Recommended best practice is to use a controlled vocabulary such as RFC 4646 [RFC4646].</terms:description>
        <terms:hasVersion rdf:resource="http://dublincore.org/usage/terms/history/#language-007"/>
        <rdfs:isDefinedBy rdf:resource="http://purl.org/dc/elements/1.1/"/>
        <rdfs:seeAlso rdf:resource="http://www.ietf.org/rfc/rfc4646.txt"/>
    </rdf:Description>
    <rdf:Description rdf:about="&dc;identifier">
        <rdfs:label xml:lang="en-us">Identifier</rdfs:label>
        <terms:modified>2008-01-14</terms:modified>
        <terms:issued>1999-07-02</terms:issued>
        <skos:note xml:lang="en-us">A second property with the same name as this property has been declared in the dcterms: namespace (http://purl.org/dc/terms/).  See the Introduction to the document &#39;DCMI Metadata Terms&#39; (http://dublincore.org/documents/dcmi-terms/) for an explanation.</skos:note>
        <rdfs:comment xml:lang="en-us">An unambiguous reference to the resource within a given context.</rdfs:comment>
        <terms:description xml:lang="en-us">Recommended best practice is to identify the resource by means of a string conforming to a formal identification system. </terms:description>
        <terms:hasVersion rdf:resource="http://dublincore.org/usage/terms/history/#identifier-006"/>
        <rdfs:isDefinedBy rdf:resource="http://purl.org/dc/elements/1.1/"/>
    </rdf:Description>
    <rdf:Description rdf:about="http://purl.org/dc/elements/1.1/">
        <terms:modified>2010-10-11</terms:modified>
        <terms:title xml:lang="en-us">Dublin Core Metadata Element Set, Version 1.1</terms:title>
        <terms:publisher rdf:resource="http://purl.org/dc/aboutdcmi#DCMI"/>
    </rdf:Description>
    <rdf:Description rdf:about="&dc;publisher">
        <rdfs:label xml:lang="en-us">Publisher</rdfs:label>
        <terms:issued>1999-07-02</terms:issued>
        <terms:modified>2008-01-14</terms:modified>
        <skos:note xml:lang="en-us">A second property with the same name as this property has been declared in the dcterms: namespace (http://purl.org/dc/terms/).  See the Introduction to the document &#39;DCMI Metadata Terms&#39; (http://dublincore.org/documents/dcmi-terms/) for an explanation.</skos:note>
        <rdfs:comment xml:lang="en-us">An entity responsible for making the resource available.</rdfs:comment>
        <terms:description xml:lang="en-us">Examples of a Publisher include a person, an organization, or a service. Typically, the name of a Publisher should be used to indicate the entity.</terms:description>
        <terms:hasVersion rdf:resource="http://dublincore.org/usage/terms/history/#publisher-006"/>
        <rdfs:isDefinedBy rdf:resource="http://purl.org/dc/elements/1.1/"/>
    </rdf:Description>
    <rdf:Description rdf:about="&dc;source">
        <rdfs:label xml:lang="en-us">Source</rdfs:label>
        <terms:issued>1999-07-02</terms:issued>
        <terms:modified>2008-01-14</terms:modified>
        <rdfs:comment xml:lang="en-us">A related resource from which the described resource is derived.</rdfs:comment>
        <skos:note xml:lang="en-us">A second property with the same name as this property has been declared in the dcterms: namespace (http://purl.org/dc/terms/).  See the Introduction to the document &#39;DCMI Metadata Terms&#39; (http://dublincore.org/documents/dcmi-terms/) for an explanation.</skos:note>
        <terms:description xml:lang="en-us">The described resource may be derived from the related resource in whole or in part. Recommended best practice is to identify the related resource by means of a string conforming to a formal identification system.</terms:description>
        <terms:hasVersion rdf:resource="http://dublincore.org/usage/terms/history/#source-006"/>
        <rdfs:isDefinedBy rdf:resource="http://purl.org/dc/elements/1.1/"/>
    </rdf:Description>
    <rdf:Description rdf:about="&dc;rights">
        <rdfs:label xml:lang="en-us">Rights</rdfs:label>
        <terms:modified>2008-01-14</terms:modified>
        <terms:issued>1999-07-02</terms:issued>
        <skos:note xml:lang="en-us">A second property with the same name as this property has been declared in the dcterms: namespace (http://purl.org/dc/terms/).  See the Introduction to the document &#39;DCMI Metadata Terms&#39; (http://dublincore.org/documents/dcmi-terms/) for an explanation.</skos:note>
        <rdfs:comment xml:lang="en-us">Information about rights held in and over the resource.</rdfs:comment>
        <terms:description xml:lang="en-us">Typically, rights information includes a statement about various property rights associated with the resource, including intellectual property rights.</terms:description>
        <terms:hasVersion rdf:resource="http://dublincore.org/usage/terms/history/#rights-006"/>
        <rdfs:isDefinedBy rdf:resource="http://purl.org/dc/elements/1.1/"/>
    </rdf:Description>
    <rdf:Description rdf:about="&dc;coverage">
        <rdfs:label xml:lang="en-us">Coverage</rdfs:label>
        <terms:modified>2008-01-14</terms:modified>
        <terms:issued>1999-07-02</terms:issued>
        <skos:note xml:lang="en-us">A second property with the same name as this property has been declared in the dcterms: namespace (http://purl.org/dc/terms/).  See the Introduction to the document &#39;DCMI Metadata Terms&#39; (http://dublincore.org/documents/dcmi-terms/) for an explanation.</skos:note>
        <terms:description xml:lang="en-us">Spatial topic and spatial applicability may be a named place or a location specified by its geographic coordinates. Temporal topic may be a named period, date, or date range. A jurisdiction may be a named administrative entity or a geographic place to which the resource applies. Recommended best practice is to use a controlled vocabulary such as the Thesaurus of Geographic Names [TGN]. Where appropriate, named places or time periods can be used in preference to numeric identifiers such as sets of coordinates or date ranges.</terms:description>
        <rdfs:comment xml:lang="en-us">The spatial or temporal topic of the resource, the spatial applicability of the resource, or the jurisdiction under which the resource is relevant.</rdfs:comment>
        <terms:hasVersion rdf:resource="http://dublincore.org/usage/terms/history/#coverage-006"/>
        <rdfs:isDefinedBy rdf:resource="http://purl.org/dc/elements/1.1/"/>
    </rdf:Description>
    <rdf:Description rdf:about="&dc;subject">
        <rdfs:label xml:lang="en-us">Subject</rdfs:label>
        <terms:modified>2008-01-14</terms:modified>
        <terms:issued>1999-07-02</terms:issued>
        <skos:note xml:lang="en-us">A second property with the same name as this property has been declared in the dcterms: namespace (http://purl.org/dc/terms/).  See the Introduction to the document &#39;DCMI Metadata Terms&#39; (http://dublincore.org/documents/dcmi-terms/) for an explanation.</skos:note>
        <rdfs:comment xml:lang="en-us">The topic of the resource.</rdfs:comment>
        <terms:description xml:lang="en-us">Typically, the subject will be represented using keywords, key phrases, or classification codes. Recommended best practice is to use a controlled vocabulary. To describe the spatial or temporal topic of the resource, use the Coverage element.</terms:description>
        <terms:hasVersion rdf:resource="http://dublincore.org/usage/terms/history/#subject-006"/>
        <rdfs:isDefinedBy rdf:resource="http://purl.org/dc/elements/1.1/"/>
    </rdf:Description>
    <rdf:Description rdf:about="&dc;type">
        <rdfs:label xml:lang="en-us">Type</rdfs:label>
        <terms:modified>2008-01-14</terms:modified>
        <terms:issued>1999-07-02</terms:issued>
        <skos:note xml:lang="en-us">A second property with the same name as this property has been declared in the dcterms: namespace (http://purl.org/dc/terms/).  See the Introduction to the document &#39;DCMI Metadata Terms&#39; (http://dublincore.org/documents/dcmi-terms/) for an explanation.</skos:note>
        <terms:description xml:lang="en-us">Recommended best practice is to use a controlled vocabulary such as the DCMI Type Vocabulary [DCMITYPE]. To describe the file format, physical medium, or dimensions of the resource, use the Format element.</terms:description>
        <rdfs:comment xml:lang="en-us">The nature or genre of the resource.</rdfs:comment>
        <terms:hasVersion rdf:resource="http://dublincore.org/usage/terms/history/#type-006"/>
        <rdfs:isDefinedBy rdf:resource="http://purl.org/dc/elements/1.1/"/>
    </rdf:Description>
    <rdf:Description rdf:about="&dc;relation">
        <rdfs:label xml:lang="en-us">Relation</rdfs:label>
        <terms:modified>2008-01-14</terms:modified>
        <terms:issued>1999-07-02</terms:issued>
        <rdfs:comment xml:lang="en-us">A related resource.</rdfs:comment>
        <skos:note xml:lang="en-us">A second property with the same name as this property has been declared in the dcterms: namespace (http://purl.org/dc/terms/).  See the Introduction to the document &#39;DCMI Metadata Terms&#39; (http://dublincore.org/documents/dcmi-terms/) for an explanation.</skos:note>
        <terms:description xml:lang="en-us">Recommended best practice is to identify the related resource by means of a string conforming to a formal identification system. </terms:description>
        <terms:hasVersion rdf:resource="http://dublincore.org/usage/terms/history/#relation-006"/>
        <rdfs:isDefinedBy rdf:resource="http://purl.org/dc/elements/1.1/"/>
    </rdf:Description>
    <rdf:Description rdf:about="&dc;title">
        <rdfs:label xml:lang="en-us">Title</rdfs:label>
        <terms:issued>1999-07-02</terms:issued>
        <terms:modified>2008-01-14</terms:modified>
        <rdfs:comment xml:lang="en-us">A name given to the resource.</rdfs:comment>
        <skos:note xml:lang="en-us">A second property with the same name as this property has been declared in the dcterms: namespace (http://purl.org/dc/terms/).  See the Introduction to the document &#39;DCMI Metadata Terms&#39; (http://dublincore.org/documents/dcmi-terms/) for an explanation.</skos:note>
        <terms:hasVersion rdf:resource="http://dublincore.org/usage/terms/history/#title-006"/>
        <rdfs:isDefinedBy rdf:resource="http://purl.org/dc/elements/1.1/"/>
    </rdf:Description>
    


    <!-- 
    ///////////////////////////////////////////////////////////////////////////////////////
    //
    // General axioms
    //
    ///////////////////////////////////////////////////////////////////////////////////////
     -->

    <rdf:Description>
        <rdf:type rdf:resource="&owl;AllDifferent"/>
        <owl:distinctMembers rdf:parseType="Collection">
            <rdf:Description rdf:about="&or;EMEM"/>
            <rdf:Description rdf:about="&or;HEPES"/>
            <rdf:Description rdf:about="&or;IMDM"/>
            <rdf:Description rdf:about="&or;OMEM"/>
        </owl:distinctMembers>
    </rdf:Description>
    <rdf:Description>
        <rdf:type rdf:resource="&owl;AllDifferent"/>
        <owl:distinctMembers rdf:parseType="Collection">
            <rdf:Description rdf:about="&or;Atmosphere-UnitOfPressure"/>
            <rdf:Description rdf:about="&or;Bar-UnitOfPressure"/>
            <rdf:Description rdf:about="&or;PSI"/>
            <rdf:Description rdf:about="&or;Pascal-UnitOfPressure"/>
        </owl:distinctMembers>
    </rdf:Description>
    <rdf:Description>
        <rdf:type rdf:resource="&owl;AllDifferent"/>
        <owl:distinctMembers rdf:parseType="Collection">
            <rdf:Description rdf:about="&or;AtomicMassUnit"/>
            <rdf:Description rdf:about="&or;Gram"/>
            <rdf:Description rdf:about="&or;Kilogram"/>
            <rdf:Description rdf:about="&or;Microgram"/>
            <rdf:Description rdf:about="&or;Milligram"/>
            <rdf:Description rdf:about="&or;Nanogram"/>
        </owl:distinctMembers>
    </rdf:Description>
    <rdf:Description>
        <rdf:type rdf:resource="&owl;AllDifferent"/>
        <owl:distinctMembers rdf:parseType="Collection">
            <rdf:Description rdf:about="&or;DegreeCelsius"/>
            <rdf:Description rdf:about="&or;DegreeFahrenheit"/>
            <rdf:Description rdf:about="&or;DegreeKelvin"/>
        </owl:distinctMembers>
    </rdf:Description>
    <rdf:Description>
        <rdf:type rdf:resource="&owl;AllDifferent"/>
        <owl:distinctMembers rdf:parseType="Collection">
            <rdf:Description rdf:about="&or;Atmosphere-UnitOfPressure"/>
            <rdf:Description rdf:about="&or;MmHg"/>
        </owl:distinctMembers>
    </rdf:Description>
</rdf:RDF>



<!-- Generated by the OWL API (version 3.2.3.1824) http://owlapi.sourceforge.net -->

